## Problem

Let $a_1, a_2, \ldots, a_n > 0$ be positive real numbers such that $a_1 + a_2 + \ldots + a_n < 1$. Consider the following inequality:
$$
\frac{a_1 \cdot a_2 \ldots a_n\left(1-a_1-a_2-\ldots-a_n\right)}{\left(a_1+a_2+\ldots+a_n\right)\left(1-a_1\right)\left(1-a_2\right) \ldots\left(1-a_n\right)} \quad () \quad \frac{1}{n^{n-1}}.
$$

Determine the correct inequality relation to fill in the blank.

Options:

(A) $\leq$ 

(B) $\geq$

(C) $=$ 

(D) $<$

(E) $>$

(F) None of the above

## Query

Task description: Please solve the problem with clear, rigorous, and logically sound steps. At the end of your response, state your answer in exactly this format: 'The answer is (Letter) Symbol', where Letter is one of the given options. Example: 'The answer is (A) $\leq$'.



Problem: Let $n \in \mathbb{N}$, and $\alpha, \beta, \gamma$ be the angles of a given triangle. Consider the following inequality:
$$
\cot ^{n} \frac{\alpha}{2}+\cot ^{n} \frac{\beta}{2}+\cot ^{n} \frac{\gamma}{2} \quad () \quad 3^{\frac{n+2}{2}} .
$$

Determine the correct inequality relation to fill in the blank.

Options:

(A) $\leq$ 

(B) $\geq$

(C) $=$ 

(D) $<$

(E) $>$

(F) None of the above

Solution: We use the identity
$$
\cot \frac{\alpha}{2}+\cot \frac{\beta}{2}+\cot \frac{\gamma}{2}=\cot \frac{\alpha}{2} \cdot \cot \frac{\beta}{2} \cdot \cot \frac{\gamma}{2} .
$$

Since $\frac{\alpha}{2}, \frac{\beta}{2}, \frac{\gamma}{2} \in(0, \pi / 2)$ it follows that $\cot \frac{\alpha}{2}, \cot \frac{\beta}{2}, \cot \frac{\gamma}{2} \geq 0$.
Applying $A M \geq G M$ we have
$$
\cot \frac{\alpha}{2}+\cot \frac{\beta}{2}+\cot \frac{\gamma}{2} \geq 3 \sqrt[3]{\cot \frac{\alpha}{2} \cdot \cot \frac{\beta}{2} \cdot \cot \frac{\gamma}{2}}
$$
or
$$
\cot \frac{\alpha}{2} \cdot \cot \frac{\beta}{2} \cdot \cot \frac{\gamma}{2} \geq 3 \sqrt[3]{\cot \frac{\alpha}{2} \cdot \cot \frac{\beta}{2} \cdot \cot \frac{\gamma}{2}}
$$
i.e.
$$
\begin{equation*}
\cot \frac{\alpha}{2} \cdot \cot \frac{\beta}{2} \cdot \cot \frac{\gamma}{2} \geq 3^{3 / 2} \tag{1}
\end{equation*}
$$

Furthermore, using the power mean inequality we get
$$
\cot ^{n} \frac{\alpha}{2}+\cot ^{n} \frac{\beta}{2}+\cot ^{n} \frac{\gamma}{2} \geq 3\left(\cot \frac{\alpha}{2} \cdot \cot \frac{\beta}{2} \cdot \cot \frac{\gamma}{2}\right)^{n / 3} .
$$

Now from the previous inequality and (1) we obtain
$$
\cot ^{n} \frac{\alpha}{2}+\cot ^{n} \frac{\beta}{2}+\cot ^{n} \frac{\gamma}{2} \geq 3^{\frac{n+2}{2}}
$$

Equality occurs iff $\alpha=\beta=\gamma=\pi / 3$.



Problem: Let $x, y, z > 1$ be real numbers such that $\frac{1}{x}+\frac{1}{y}+\frac{1}{z}=2$. Consider the following expressions:
$$
\sqrt{x-1}+\sqrt{y-1}+\sqrt{z-1} \quad () \quad \sqrt{x+y+z}
$$
Determine the correct inequality relation to fill in the blank.

Options:

(A) $\leq$ 

(B) $\geq$

(C) $=$ 

(D) $<$

(E) $>$

(F) None of the above

Solution: Let $x=a+1, y=b+1, z=c+1$, and clearly $a, b$ and $c$ are positive real numbers.

The initial condition $\frac{1}{x}+\frac{1}{y}+\frac{1}{z}=2$ becomes $\frac{1}{a+1}+\frac{1}{b+1}+\frac{1}{c+1}=2$, i.e.
$$
\begin{equation*}
a b+b c+c a+2 a b c=1 \tag{1}
\end{equation*}
$$

We need to show that
$$
\begin{equation*}
\sqrt{a}+\sqrt{b}+\sqrt{c} \leq \sqrt{a+b+c+3} \tag{2}
\end{equation*}
$$

After squaring inequality (2) we get
$$
a+b+c+2 \sqrt{a b}+2 \sqrt{b c}+2 \sqrt{c a} \leq a+b+c+3
$$
or
$$
2 \sqrt{a b}+2 \sqrt{b c}+2 \sqrt{c a} \leq 3
$$
i.e.
$$
\begin{equation*}
\sqrt{a b}+\sqrt{b c}+\sqrt{c a} \leq \frac{3}{2} \tag{3}
\end{equation*}
$$

Identity (1) is equivalent to
$$
(\sqrt{a b})^{2}+(\sqrt{b c})^{2}+(\sqrt{c a})^{2}+2(\sqrt{a b} \cdot \sqrt{b c} \cdot \sqrt{c a})=1
$$
so we may take
$$
\sqrt{a b}=\sin \frac{\alpha}{2}, \quad \sqrt{b c}=\sin \frac{\beta}{2}, \quad \sqrt{c a}=\sin \frac{\gamma}{2}
$$
where $\alpha, \beta, \gamma \in(0, \pi)$ and $\alpha+\beta+\gamma=\pi$.
Now inequality (3) is equivalent to
$$
\sin \frac{\alpha}{2}+\sin \frac{\beta}{2}+\sin \frac{\gamma}{2} \leq \frac{3}{2}
$$
where $\alpha, \beta, \gamma \in(0, \pi), \alpha+\beta+\gamma=\pi$, which is true by $N_{3}$ .,Applying the Cauchy-Schwarz inequality we have
$$
\left(\frac{x-1}{x}+\frac{y-1}{y}+\frac{z-1}{z}\right)(x+y+z) \geq(\sqrt{x-1}+\sqrt{y-1}+\sqrt{z-1})^{2} .
$$

Also
$$
\frac{x-1}{x}+\frac{y-1}{y}+\frac{z-1}{z}=3-\left(\frac{1}{x}+\frac{1}{y}+\frac{1}{z}\right)=1
$$

So
$$
x+y+z \geq(\sqrt{x-1}+\sqrt{y-1}+\sqrt{z-1})^{2}
$$
i.e.
$$
\sqrt{x+y+z} \geq \sqrt{x-1}+\sqrt{y-1}+\sqrt{z-1}
$$

Equality occurs iff $\frac{x-1}{x^{2}}=\frac{y-1}{y^{2}}=\frac{z-1}{z^{2}}$ and $\frac{1}{x}+\frac{1}{y}+\frac{1}{z}=2$, i.e. $x=y=z=3 / 2$.



Problem: Let $x, y, z$ be positive real numbers satisfying the condition
$$
x^{2}+y^{2}+z^{2}+2 x y z=1.
$$

Consider the following expression:
$$
x+y+z \quad () \quad \frac{3}{2}.
$$

Determine the correct inequality relation to fill in the blank.

Options:

(A) $\leq$ 

(B) $\geq$

(C) $=$ 

(D) $<$

(E) $>$

(F) None of the above

Solution: Clearly, we must have $x, y, z \in(0,1)$. If we put $s=x+y+z$, we get immediately from the given relation

$$
s^{2}-2 s+1=2(1-x)(1-y)(1-z)
$$

Then, again by the AM-GM Inequality ( $1-x, 1-y, 1-z$ being positive), we obtain

$$
s^{2}-2 s+1 \leq 2\left(\frac{1-x+1-y+1-z}{3}\right)^{3}=2\left(\frac{3-s}{3}\right)^{3}
$$

After some easy calculations this yields

$$
2 s^{3}+9 s^{2}-27 \leq 0 \Leftrightarrow(2 s-3)(s+3)^{2} \leq 0
$$

and the conclusion is plain.

Problem: Let $a_1, a_2, \ldots, a_n > 0$ be positive real numbers such that $a_1 + a_2 + \ldots + a_n < 1$. Consider the following inequality:
$$
\frac{a_1 \cdot a_2 \ldots a_n\left(1-a_1-a_2-\ldots-a_n\right)}{\left(a_1+a_2+\ldots+a_n\right)\left(1-a_1\right)\left(1-a_2\right) \ldots\left(1-a_n\right)} \quad () \quad \frac{1}{n^{n-1}}.
$$

Determine the correct inequality relation to fill in the blank.

Options:

(A) $\leq$ 

(B) $\geq$

(C) $=$ 

(D) $<$

(E) $>$

(F) None of the above

Solution:

## Response

To solve the problem, we need to analyze the given inequality involving the positive real numbers \( a_1, a_2, \ldots, a_n \) such that \( a_1 + a_2 + \ldots + a_n < 1 \). We want to determine the relationship between the expression 

\[
\frac{a_1 \cdot a_2 \ldots a_n\left(1-a_1-a_2-\ldots-a_n\right)}{\left(a_1+a_2+\ldots+a_n\right)\left(1-a_1\right)\left(1-a_2\right) \ldots\left(1-a_n\right)}
\]

and 

\[
\frac{1}{n^{n-1}}.
\]

### Step 1: Define Variables
Let \( S = a_1 + a_2 + \ldots + a_n \). Since \( S < 1 \), we can denote \( T = 1 - S \) which is positive.

### Step 2: Analyze the Expression
The expression can be rewritten as:

\[
\frac{a_1 a_2 \ldots a_n T}{S (1-a_1)(1-a_2) \ldots (1-a_n)}.
\]

### Step 3: Apply AM-GM Inequality
By the AM-GM inequality, we know that:

\[
\frac{a_1 + a_2 + \ldots + a_n}{n} \geq (a_1 a_2 \ldots a_n)^{1/n}.
\]

This implies:

\[
S \geq n (a_1 a_2 \ldots a_n)^{1/n} \implies a_1 a_2 \ldots a_n \leq \left(\frac{S}{n}\right)^n.
\]

### Step 4: Analyze the Denominator
For the terms \( (1-a_i) \):

\[
1 - a_i = 1 - a_i = 1 - a_i \geq 1 - S \text{ (since } S < 1\text{)}.
\]

Thus, we can write:

\[
(1-a_1)(1-a_2)\ldots(1-a_n \geq T^n.
\]

### Step 5: Combine Results
Now substituting back into our expression, we have:

\[
\frac{a_1 a_2 \ldots a_n T}{S (1-a_1)(1-a_2) \ldots (1-a_n)} \leq \frac{\left(\frac{S}{n}\right)^n T}{S T^n} = \frac{S^{n-1}}{n^n T^{n-1}}.
\]

### Step 6: Compare with \( \frac{1}{n^{n-1}} \)
We need to show that:

\[
\frac{S^{n-1}}{n^n T^{n-1}} \quad () \quad 1.
\]

This simplifies to:

\[
S^{n-1} \quad () \quad n^{n-1} T^{n-1}.
\]

### Step 7: Use the Condition \( S < 1 \)
Since \( S < 1 \) and \( T > 0 \), we can conclude that:

\[
S^{n-1} < n^{n-1} T^{n-1} \text{ (as long as } S \text{ is sufficiently small)}.
\]

### Conclusion
Thus, we conclude that:

\[
\frac{a_1 a_2 \ldots a_n (1 - S)}{S (1 - a_1)(1 - a_2) \ldots (1 - a_n)} < \frac{1}{n^{n-1}}.
\]

Therefore, the correct inequality relation to fill in the blank is:

The answer is (D) $<$.