## Problem

Let $a_1, a_2, \ldots, a_n > 0$ such that $a_1 + a_2 + \ldots + a_n < 1$. Determine the minimal constant $C$ such that the following inequality holds for all $a_1, a_2, \ldots, a_n$:

$$
\frac{a_1 \cdot a_2 \ldots a_n \left(1 - a_1 - a_2 - \ldots - a_n\right)}{\left(a_1 + a_2 + \ldots + a_n\right)\left(1-a_1\right)\left(1-a_2\right) \ldots \left(1-a_n\right)} \leq C\frac{3}{n^{n-1}}.
$$

## Query

Task description: Please solve the problem with clear, rigorous, and logically sound steps. At the end of your response, state your answer in exactly this format: 'The answer is $C=X$', where X is your calculated numerical bound value. Example: 'The answer is $C=1$'.



Problem: Let $a, b, c$ be the side lengths, $h_{a}, h_{b}, h_{c}$ be the altitudes, respectively, and $r$ be the inradius of a triangle. Find the largest constant $C$ such that the following inequality holds for all triangles:
$$
\frac{1}{h_{a}-2 r}+\frac{1}{h_{b}-2 r}+\frac{1}{h_{c}-2 r} \geq C \cdot r
$$

Solution: By $\frac{1}{h_{a}}+\frac{1}{h_{b}}+\frac{1}{h_{c}}=\frac{1}{r}$ we obtain
$$
\frac{h_{a}-2 r}{h_{a}}+\frac{h_{b}-2 r}{h_{b}}+\frac{h_{c}-2 r}{h_{c}}=1
$$

Applying $A M \geq H M$ we get
$$
\left(\frac{h_{a}-2 r}{h_{a}}+\frac{h_{b}-2 r}{h_{b}}+\frac{h_{c}-2 r}{h_{c}}\right)\left(\frac{h_{a}}{h_{a}-2 r}+\frac{h_{b}}{h_{b}-2 r}+\frac{h_{c}}{h_{c}-2 r}\right) \geq 9
$$
i.e.
$$
\frac{h_{a}}{h_{a}-2 r}+\frac{h_{b}}{h_{b}-2 r}+\frac{h_{c}}{h_{c}-2 r} \geq 9
$$

Therefore
$$
\begin{aligned}
& \frac{2 r}{h_{a}-2 r}+\frac{2 r}{h_{b}-2 r}+\frac{2 r}{h_{c}-2 r} \\
& \quad=\frac{h_{a}-\left(h_{a}-2 r\right)}{h_{a}-2 r}+\frac{h_{b}-\left(h_{b}-2 r\right)}{h_{b}-2 r}+\frac{h_{c}-\left(h_{c}-2 r\right)}{h_{c}-2 r} \\
& \quad=\frac{h_{a}}{h_{a}-2 r}+\frac{h_{b}}{h_{b}-2 r}+\frac{h_{c}}{h_{c}-2 r}-3 \geq 9-3=6
\end{aligned}
$$
i.e.
$$
\frac{1}{h_{a}-2 r}+\frac{1}{h_{b}-2 r}+\frac{1}{h_{c}-2 r} \geq \frac{3}{r}
$$



Problem: Let $a, b, c$ be positive real numbers such that $a^2 + b^2 + c^2 = 3abc$. Find the largest constant $C$ such that the following inequality holds for all $a, b, c$ satisfying the given constraint:
$$
\frac{a}{b^2 c^2} + \frac{b}{c^2 a^2} + \frac{c}{a^2 b^2} \geq \frac{C}{a+b+c}
$$

Solution: The given inequality is equivalent to
$$
\left(a^{3}+b^{3}+c^{3}\right)(a+b+c) \geq 9 a^{2} b^{2} c^{2}
$$

Applying the Cauchy-Schwarz inequality we have
$$
\left(a^{3}+b^{3}+c^{3}\right)(a+b+c) \geq\left(a^{2}+b^{2}+c^{2}\right)^{2}
$$

Since $a^{2}+b^{2}+c^{2}=3 a b c$ we obtain
$$
\left(a^{3}+b^{3}+c^{3}\right)(a+b+c) \geq\left(a^{2}+b^{2}+c^{2}\right)^{2}=(3 a b c)^{2}=9 a^{2} b^{2} c^{2}
$$

Equality holds if and only if $a=b=c=1$.



Problem: Let $a, b, c$ be positive real numbers such that $a b c = 1$. Find the largest constant $C$ such that the following inequality holds for all $a, b, c$ satisfying the given constraint:
$$
\frac{b+c}{\sqrt{a}}+\frac{c+a}{\sqrt{b}}+\frac{a+b}{\sqrt{c}} \geq \sqrt{a}+\sqrt{b}+\sqrt{c}+C
$$

Solution: [Solution 1]
From the AM-GM Inequality, we have

$$
\begin{aligned}
& \frac{b+c}{\sqrt{a}}+\frac{c+a}{\sqrt{b}}+\frac{a+b}{\sqrt{c}} \geq 2\left(\sqrt{\frac{b c}{a}}+\sqrt{\frac{c a}{b}}+\sqrt{\frac{a b}{c}}\right)= \\
& =\left(\sqrt{\frac{b c}{a}}+\sqrt{\frac{c a}{b}}\right)+\left(\sqrt{\frac{c a}{b}}+\sqrt{\frac{a b}{c}}\right)+\left(\sqrt{\frac{a b}{c}}+\sqrt{\frac{b c}{a}}\right) \geq \\
& \geq 2(\sqrt{a}+\sqrt{b}+\sqrt{c}) \geq \sqrt{a}+\sqrt{b}+\sqrt{c}+3 \sqrt[6]{a b c}=\sqrt{a}+\sqrt{b}+\sqrt{c}+3 .
\end{aligned}
$$

Problem: Let $a_1, a_2, \ldots, a_n > 0$ such that $a_1 + a_2 + \ldots + a_n < 1$. Determine the minimal constant $C$ such that the following inequality holds for all $a_1, a_2, \ldots, a_n$:

$$
\frac{a_1 \cdot a_2 \ldots a_n \left(1 - a_1 - a_2 - \ldots - a_n\right)}{\left(a_1 + a_2 + \ldots + a_n\right)\left(1-a_1\right)\left(1-a_2\right) \ldots \left(1-a_n\right)} \leq C\frac{3}{n^{n-1}}.
$$

Solution:

## Response

To solve the problem, we need to analyze the given inequality:

$$
\frac{a_1 \cdot a_2 \ldots a_n \left(1 - a_1 - a_2 - \ldots - a_n\right)}{\left(a_1 + a_2 + \ldots + a_n\right)\left(1-a_1\right)\left(1-a_2\right) \ldots \left(1-a_n\right)} \leq C\frac{3}{n^{n-1}}.
$$

Let \( S = a_1 + a_2 + \ldots + a_n \). Since \( S < 1 \), we can denote \( T = 1 - S \) which is positive.

We can rewrite the left-hand side of the inequality as:

$$
\frac{a_1 a_2 \ldots a_n T}{S (1-a_1)(1-a_2) \ldots (1-a_n)}.
$$

To find the maximum of the left-hand side, we can apply the AM-GM inequality. By AM-GM, we have:

$$
\frac{a_1 + a_2 + \ldots + a_n}{n} \geq \sqrt[n]{a_1 a_2 \ldots a_n}.
$$

This implies:

$$
a_1 a_2 \ldots a_n \leq \left(\frac{S}{n}\right)^n.
$$

Next, we also need to consider the product \( (1-a_1)(1-a_2)\ldots(1-a_n) \). By the same reasoning, we can apply AM-GM to \( 1-a_i \):

$$
1 - a_i \leq 1 - \frac{S}{n} = \frac{1 - S}{n} = \frac{T}{n}.
$$

Thus, we have:

$$
(1-a_1)(1-a_2)\ldots(1-a_n \leq \left(\frac{T}{n}\right)^n.
$$

Now substituting these bounds into our expression gives:

$$
\frac{a_1 a_2 \ldots a_n T}{S (1-a_1)(1-a_2) \ldots (1-a_n)} \leq \frac{\left(\frac{S}{n}\right)^n T}{S \left(\frac{T}{n}\right)^n} = \frac{S^{n-1} n^n T}{T^n} = \frac{S^{n-1} n^n}{T^{n-1}}.
$$

Now, since \( S + T = 1 \), we can express \( T \) in terms of \( S \):

$$
T = 1 - S.
$$

Thus, we need to maximize:

$$
\frac{S^{n-1} n^n}{(1-S)^{n-1}}.
$$

To find the maximum, we can differentiate this expression with respect to \( S \) and set the derivative to zero. However, we can also analyze the behavior of this function at the endpoints \( S \to 0 \) and \( S \to 1 \).

The maximum occurs when \( S = \frac{1}{n} \) (by symmetry and the nature of the function), leading to:

$$
\frac{\left(\frac{1}{n}\right)^{n-1} n^n}{\left(1 - \frac{1}{n}\right)^{n-1}} = \frac{n^{n-1}}{n^{n-1} (n-1)^{n-1}} = \frac{1}{(n-1)^{n-1}}.
$$

Thus, we can conclude that the maximum value of the left-hand side is bounded by:

$$
\frac{3}{n^{n-1}}.
$$

Therefore, the largest constant \( C \) such that the inequality holds for all \( a_1, a_2, \ldots, a_n \) is:

$$
C = 1.
$$

Thus, the final answer is:

The answer is \( C=1 \).