## Problem

Let $a, b, c, x, y, z$ be positive real numbers such that $a+x \geq b+y \geq c+z$ and $a+b+c = x+y+z$. Find the largest constant $C$ such that the following inequality holds for all $a, b, c, x, y, z$ satisfying the given conditions:
$$
a y + b x \geq 3C(a c + x z).
$$

## Query

Task description: Please solve the problem with clear, rigorous, and logically sound steps. At the end of your response, state your answer in exactly this format: 'The answer is $C=X$', where X is your calculated numerical bound value. Example: 'The answer is $C=1$'.



Problem: Let $a, b, c$ be the side lengths, $h_{a}, h_{b}, h_{c}$ be the altitudes, respectively, and $r$ be the inradius of a triangle. Find the largest constant $C$ such that the following inequality holds for all triangles:
$$
\frac{1}{h_{a}-2 r}+\frac{1}{h_{b}-2 r}+\frac{1}{h_{c}-2 r} \geq C \cdot r
$$

Solution: By $\frac{1}{h_{a}}+\frac{1}{h_{b}}+\frac{1}{h_{c}}=\frac{1}{r}$ we obtain
$$
\frac{h_{a}-2 r}{h_{a}}+\frac{h_{b}-2 r}{h_{b}}+\frac{h_{c}-2 r}{h_{c}}=1
$$

Applying $A M \geq H M$ we get
$$
\left(\frac{h_{a}-2 r}{h_{a}}+\frac{h_{b}-2 r}{h_{b}}+\frac{h_{c}-2 r}{h_{c}}\right)\left(\frac{h_{a}}{h_{a}-2 r}+\frac{h_{b}}{h_{b}-2 r}+\frac{h_{c}}{h_{c}-2 r}\right) \geq 9
$$
i.e.
$$
\frac{h_{a}}{h_{a}-2 r}+\frac{h_{b}}{h_{b}-2 r}+\frac{h_{c}}{h_{c}-2 r} \geq 9
$$

Therefore
$$
\begin{aligned}
& \frac{2 r}{h_{a}-2 r}+\frac{2 r}{h_{b}-2 r}+\frac{2 r}{h_{c}-2 r} \\
& \quad=\frac{h_{a}-\left(h_{a}-2 r\right)}{h_{a}-2 r}+\frac{h_{b}-\left(h_{b}-2 r\right)}{h_{b}-2 r}+\frac{h_{c}-\left(h_{c}-2 r\right)}{h_{c}-2 r} \\
& \quad=\frac{h_{a}}{h_{a}-2 r}+\frac{h_{b}}{h_{b}-2 r}+\frac{h_{c}}{h_{c}-2 r}-3 \geq 9-3=6
\end{aligned}
$$
i.e.
$$
\frac{1}{h_{a}-2 r}+\frac{1}{h_{b}-2 r}+\frac{1}{h_{c}-2 r} \geq \frac{3}{r}
$$



Problem: Let $a, b, c$ be positive real numbers such that $a^2 + b^2 + c^2 = 3abc$. Find the largest constant $C$ such that the following inequality holds for all $a, b, c$ satisfying the given constraint:
$$
\frac{a}{b^2 c^2} + \frac{b}{c^2 a^2} + \frac{c}{a^2 b^2} \geq \frac{C}{a+b+c}
$$

Solution: The given inequality is equivalent to
$$
\left(a^{3}+b^{3}+c^{3}\right)(a+b+c) \geq 9 a^{2} b^{2} c^{2}
$$

Applying the Cauchy-Schwarz inequality we have
$$
\left(a^{3}+b^{3}+c^{3}\right)(a+b+c) \geq\left(a^{2}+b^{2}+c^{2}\right)^{2}
$$

Since $a^{2}+b^{2}+c^{2}=3 a b c$ we obtain
$$
\left(a^{3}+b^{3}+c^{3}\right)(a+b+c) \geq\left(a^{2}+b^{2}+c^{2}\right)^{2}=(3 a b c)^{2}=9 a^{2} b^{2} c^{2}
$$

Equality holds if and only if $a=b=c=1$.



Problem: Let $a, b, c$ be positive real numbers such that $a b c = 1$. Find the largest constant $C$ such that the following inequality holds for all $a, b, c$ satisfying the given constraint:
$$
\frac{b+c}{\sqrt{a}}+\frac{c+a}{\sqrt{b}}+\frac{a+b}{\sqrt{c}} \geq \sqrt{a}+\sqrt{b}+\sqrt{c}+C
$$

Solution: [Solution 1]
From the AM-GM Inequality, we have

$$
\begin{aligned}
& \frac{b+c}{\sqrt{a}}+\frac{c+a}{\sqrt{b}}+\frac{a+b}{\sqrt{c}} \geq 2\left(\sqrt{\frac{b c}{a}}+\sqrt{\frac{c a}{b}}+\sqrt{\frac{a b}{c}}\right)= \\
& =\left(\sqrt{\frac{b c}{a}}+\sqrt{\frac{c a}{b}}\right)+\left(\sqrt{\frac{c a}{b}}+\sqrt{\frac{a b}{c}}\right)+\left(\sqrt{\frac{a b}{c}}+\sqrt{\frac{b c}{a}}\right) \geq \\
& \geq 2(\sqrt{a}+\sqrt{b}+\sqrt{c}) \geq \sqrt{a}+\sqrt{b}+\sqrt{c}+3 \sqrt[6]{a b c}=\sqrt{a}+\sqrt{b}+\sqrt{c}+3 .
\end{aligned}
$$

Problem: Let $a, b, c, x, y, z$ be positive real numbers such that $a+x \geq b+y \geq c+z$ and $a+b+c = x+y+z$. Find the largest constant $C$ such that the following inequality holds for all $a, b, c, x, y, z$ satisfying the given conditions:
$$
a y + b x \geq 3C(a c + x z).
$$

Solution:

## Response

To solve the problem, we start with the given conditions:

1. \( a + x \geq b + y \geq c + z \)
2. \( a + b + c = x + y + z \)

We need to find the largest constant \( C \) such that the inequality 

\[
a y + b x \geq 3C(a c + x z)
\]

holds for all positive real numbers \( a, b, c, x, y, z \) satisfying the above conditions.

### Step 1: Analyze the conditions

From the conditions, we can derive some relationships. Since \( a + b + c = x + y + z \), we can express \( y \) and \( z \) in terms of \( a, b, c, x \):

- Let \( y = (x + y + z) - (a + x + z) = b + c - z \)
- Let \( z = (x + y + z) - (a + b + c) = y + c - b \)

### Step 2: Substitute and simplify

We can rewrite the inequality \( a y + b x \) using the expressions for \( y \) and \( z \):

\[
a y + b x = a(b + c - z) + b x = ab + ac - az + bx
\]

Now, we need to analyze the right-hand side:

\[
3C(ac + xz) = 3C(ac + x(y + c - b))
\]

### Step 3: Use the conditions

Using the conditions \( a + x \geq b + y \) and \( b + y \geq c + z \), we can derive bounds for \( a, b, c, x, y, z \). 

### Step 4: Test specific cases

To find the largest constant \( C \), we can test specific cases. 

1. **Case 1**: Let \( a = b = c = 1 \) and \( x = y = z = 1 \). Then:

\[
1 \cdot 1 + 1 \cdot 1 \geq 3C(1 \cdot 1 + 1 \cdot 1) \implies 2 \geq 6C \implies C \leq \frac{1}{3}
\]

2. **Case 2**: Let \( a = 1, b = 1, c = 0 \) and \( x = 1, y = 1, z = 0 \). Then:

\[
1 \cdot 1 + 1 \cdot 1 \geq 3C(1 \cdot 0 + 1 \cdot 0) \implies 2 \geq 0 \implies C \text{ can be any value.}
\]

3. **Case 3**: Let \( a = 1, b = 0, c = 0 \) and \( x = 1, y = 0, z = 0 \). Then:

\[
1 \cdot 0 + 0 \cdot 1 \geq 3C(1 \cdot 0 + 1 \cdot 0) \implies 0 \geq 0 \implies C \text{ can be any value.}
\]

### Step 5: Conclusion

From the first case, we found that \( C \leq \frac{1}{3} \). Testing other cases does not provide a tighter bound. Therefore, the largest constant \( C \) that satisfies the inequality for all valid \( a, b, c, x, y, z \) is:

\[
\boxed{C = \frac{1}{3}}
\]

Thus, the final answer is:

The answer is \( C = \frac{1}{3} \).