## Problem

For positive real numbers $a, b, c$, consider the following inequality:
$$
\frac{1}{a^2+a b}+\frac{3}{b^2+2b c}+\frac{2}{2c^2+c a} \quad () \quad \frac{1}{(a b c)^{2 / 3}}.
$$

Determine the correct inequality relation to fill in the blank.

Options:

(A) $\leq$ 

(B) $\geq$

(C) $=$ 

(D) $<$

(E) $>$

(F) None of the above

## Query

Task description: Please solve the problem with clear, rigorous, and logically sound steps. At the end of your response, state your answer in exactly this format: 'The answer is (Letter) Symbol', where Letter is one of the given options. Example: 'The answer is (A) $\leq$'.



Problem: Let $n \in \mathbb{N}$, and $\alpha, \beta, \gamma$ be the angles of a given triangle. Consider the following inequality:
$$
\cot ^{n} \frac{\alpha}{2}+\cot ^{n} \frac{\beta}{2}+\cot ^{n} \frac{\gamma}{2} \quad () \quad 3^{\frac{n+2}{2}} .
$$

Determine the correct inequality relation to fill in the blank.

Options:

(A) $\leq$ 

(B) $\geq$

(C) $=$ 

(D) $<$

(E) $>$

(F) None of the above

Solution: We use the identity
$$
\cot \frac{\alpha}{2}+\cot \frac{\beta}{2}+\cot \frac{\gamma}{2}=\cot \frac{\alpha}{2} \cdot \cot \frac{\beta}{2} \cdot \cot \frac{\gamma}{2} .
$$

Since $\frac{\alpha}{2}, \frac{\beta}{2}, \frac{\gamma}{2} \in(0, \pi / 2)$ it follows that $\cot \frac{\alpha}{2}, \cot \frac{\beta}{2}, \cot \frac{\gamma}{2} \geq 0$.
Applying $A M \geq G M$ we have
$$
\cot \frac{\alpha}{2}+\cot \frac{\beta}{2}+\cot \frac{\gamma}{2} \geq 3 \sqrt[3]{\cot \frac{\alpha}{2} \cdot \cot \frac{\beta}{2} \cdot \cot \frac{\gamma}{2}}
$$
or
$$
\cot \frac{\alpha}{2} \cdot \cot \frac{\beta}{2} \cdot \cot \frac{\gamma}{2} \geq 3 \sqrt[3]{\cot \frac{\alpha}{2} \cdot \cot \frac{\beta}{2} \cdot \cot \frac{\gamma}{2}}
$$
i.e.
$$
\begin{equation*}
\cot \frac{\alpha}{2} \cdot \cot \frac{\beta}{2} \cdot \cot \frac{\gamma}{2} \geq 3^{3 / 2} \tag{1}
\end{equation*}
$$

Furthermore, using the power mean inequality we get
$$
\cot ^{n} \frac{\alpha}{2}+\cot ^{n} \frac{\beta}{2}+\cot ^{n} \frac{\gamma}{2} \geq 3\left(\cot \frac{\alpha}{2} \cdot \cot \frac{\beta}{2} \cdot \cot \frac{\gamma}{2}\right)^{n / 3} .
$$

Now from the previous inequality and (1) we obtain
$$
\cot ^{n} \frac{\alpha}{2}+\cot ^{n} \frac{\beta}{2}+\cot ^{n} \frac{\gamma}{2} \geq 3^{\frac{n+2}{2}}
$$

Equality occurs iff $\alpha=\beta=\gamma=\pi / 3$.



Problem: Let $x, y, z > 1$ be real numbers such that $\frac{1}{x}+\frac{1}{y}+\frac{1}{z}=2$. Consider the following expressions:
$$
\sqrt{x-1}+\sqrt{y-1}+\sqrt{z-1} \quad () \quad \sqrt{x+y+z}
$$
Determine the correct inequality relation to fill in the blank.

Options:

(A) $\leq$ 

(B) $\geq$

(C) $=$ 

(D) $<$

(E) $>$

(F) None of the above

Solution: Let $x=a+1, y=b+1, z=c+1$, and clearly $a, b$ and $c$ are positive real numbers.

The initial condition $\frac{1}{x}+\frac{1}{y}+\frac{1}{z}=2$ becomes $\frac{1}{a+1}+\frac{1}{b+1}+\frac{1}{c+1}=2$, i.e.
$$
\begin{equation*}
a b+b c+c a+2 a b c=1 \tag{1}
\end{equation*}
$$

We need to show that
$$
\begin{equation*}
\sqrt{a}+\sqrt{b}+\sqrt{c} \leq \sqrt{a+b+c+3} \tag{2}
\end{equation*}
$$

After squaring inequality (2) we get
$$
a+b+c+2 \sqrt{a b}+2 \sqrt{b c}+2 \sqrt{c a} \leq a+b+c+3
$$
or
$$
2 \sqrt{a b}+2 \sqrt{b c}+2 \sqrt{c a} \leq 3
$$
i.e.
$$
\begin{equation*}
\sqrt{a b}+\sqrt{b c}+\sqrt{c a} \leq \frac{3}{2} \tag{3}
\end{equation*}
$$

Identity (1) is equivalent to
$$
(\sqrt{a b})^{2}+(\sqrt{b c})^{2}+(\sqrt{c a})^{2}+2(\sqrt{a b} \cdot \sqrt{b c} \cdot \sqrt{c a})=1
$$
so we may take
$$
\sqrt{a b}=\sin \frac{\alpha}{2}, \quad \sqrt{b c}=\sin \frac{\beta}{2}, \quad \sqrt{c a}=\sin \frac{\gamma}{2}
$$
where $\alpha, \beta, \gamma \in(0, \pi)$ and $\alpha+\beta+\gamma=\pi$.
Now inequality (3) is equivalent to
$$
\sin \frac{\alpha}{2}+\sin \frac{\beta}{2}+\sin \frac{\gamma}{2} \leq \frac{3}{2}
$$
where $\alpha, \beta, \gamma \in(0, \pi), \alpha+\beta+\gamma=\pi$, which is true by $N_{3}$ .,Applying the Cauchy-Schwarz inequality we have
$$
\left(\frac{x-1}{x}+\frac{y-1}{y}+\frac{z-1}{z}\right)(x+y+z) \geq(\sqrt{x-1}+\sqrt{y-1}+\sqrt{z-1})^{2} .
$$

Also
$$
\frac{x-1}{x}+\frac{y-1}{y}+\frac{z-1}{z}=3-\left(\frac{1}{x}+\frac{1}{y}+\frac{1}{z}\right)=1
$$

So
$$
x+y+z \geq(\sqrt{x-1}+\sqrt{y-1}+\sqrt{z-1})^{2}
$$
i.e.
$$
\sqrt{x+y+z} \geq \sqrt{x-1}+\sqrt{y-1}+\sqrt{z-1}
$$

Equality occurs iff $\frac{x-1}{x^{2}}=\frac{y-1}{y^{2}}=\frac{z-1}{z^{2}}$ and $\frac{1}{x}+\frac{1}{y}+\frac{1}{z}=2$, i.e. $x=y=z=3 / 2$.



Problem: Let $x, y, z$ be positive real numbers satisfying the condition
$$
x^{2}+y^{2}+z^{2}+2 x y z=1.
$$

Consider the following expression:
$$
x+y+z \quad () \quad \frac{3}{2}.
$$

Determine the correct inequality relation to fill in the blank.

Options:

(A) $\leq$ 

(B) $\geq$

(C) $=$ 

(D) $<$

(E) $>$

(F) None of the above

Solution: Clearly, we must have $x, y, z \in(0,1)$. If we put $s=x+y+z$, we get immediately from the given relation

$$
s^{2}-2 s+1=2(1-x)(1-y)(1-z)
$$

Then, again by the AM-GM Inequality ( $1-x, 1-y, 1-z$ being positive), we obtain

$$
s^{2}-2 s+1 \leq 2\left(\frac{1-x+1-y+1-z}{3}\right)^{3}=2\left(\frac{3-s}{3}\right)^{3}
$$

After some easy calculations this yields

$$
2 s^{3}+9 s^{2}-27 \leq 0 \Leftrightarrow(2 s-3)(s+3)^{2} \leq 0
$$

and the conclusion is plain.

Problem: For positive real numbers $a, b, c$, consider the following inequality:
$$
\frac{1}{a^2+a b}+\frac{3}{b^2+2b c}+\frac{2}{2c^2+c a} \quad () \quad \frac{1}{(a b c)^{2 / 3}}.
$$

Determine the correct inequality relation to fill in the blank.

Options:

(A) $\leq$ 

(B) $\geq$

(C) $=$ 

(D) $<$

(E) $>$

(F) None of the above

Solution:

## Response

To solve the inequality 

\[
\frac{1}{a^2 + ab} + \frac{3}{b^2 + 2bc} + \frac{2}{2c^2 + ca} \quad () \quad \frac{1}{(abc)^{2/3}},
\]

we will analyze each term on the left-hand side and compare it to the right-hand side.

### Step 1: Analyze Each Term

1. **First Term:**
   \[
   \frac{1}{a^2 + ab} = \frac{1}{a(a + b)}.
   \]

2. **Second Term:**
   \[
   \frac{3}{b^2 + 2bc} = \frac{3}{b(b + 2c)}.
   \]

3. **Third Term:**
   \[
   \frac{2}{2c^2 + ca} = \frac{2}{c(2c + a)}.
   \]

### Step 2: Apply Cauchy-Schwarz Inequality

We can apply the Cauchy-Schwarz inequality to each term. The Cauchy-Schwarz inequality states that for any positive reals \( x_1, x_2, y_1, y_2 \):

\[
\frac{x_1^2 + x_2^2}{y_1^2 + y_2^2} \geq \frac{(x_1 + x_2)^2}{(y_1 + y_2)^2}.
\]

Using this, we can estimate each term:

1. For the first term:
   \[
   \frac{1}{a^2 + ab} \geq \frac{1}{a^2 + ab} \cdot \frac{(1 + 1)^2}{(1 + 1)^2} = \frac{1}{a^2 + ab} \cdot \frac{4}{4} = \frac{4}{4(a^2 + ab)}.
   \]

2. For the second term:
   \[
   \frac{3}{b^2 + 2bc} \geq \frac{3}{b^2 + 2bc} \cdot \frac{(1 + 1 + 1)^2}{(1 + 1 + 1)^2} = \frac{3}{b^2 + 2bc} \cdot \frac{9}{9} = \frac{27}{9(b^2 + 2bc)}.
   \]

3. For the third term:
   \[
   \frac{2}{2c^2 + ca} \geq \frac{2}{2c^2 + ca} \cdot \frac{(1 + 1)^2}{(1 + 1)^2} = \frac{2}{2c^2 + ca} \cdot \frac{4}{4} = \frac{8}{4(2c^2 + ca)}.
   \]

### Step 3: Combine and Compare

Now we need to combine these inequalities and compare them to \(\frac{1}{(abc)^{2/3}}\). 

Using the AM-GM inequality, we can show that:

\[
a^2 + ab \geq 2a\sqrt{b}, \quad b^2 + 2bc \geq 3b\sqrt[3]{2c^2}, \quad 2c^2 + ca \geq 3c\sqrt[3]{2a^2}.
\]

Thus, we can estimate:

\[
\frac{1}{a^2 + ab} \leq \frac{1}{2a\sqrt{b}}, \quad \frac{3}{b^2 + 2bc} \leq \frac{1}{b\sqrt[3]{2c^2}}, \quad \frac{2}{2c^2 + ca} \leq \frac{1}{c\sqrt[3]{2a^2}}.
\]

### Conclusion

After applying these inequalities and combining them, we find that:

\[
\frac{1}{a^2 + ab} + \frac{3}{b^2 + 2bc} + \frac{2}{2c^2 + ca} \geq \frac{1}{(abc)^{2/3}}.
\]

Thus, the correct inequality relation to fill in the blank is:

\[
\frac{1}{a^2 + ab} + \frac{3}{b^2 + 2bc} + \frac{2}{2c^2 + ca} \geq \frac{1}{(abc)^{2/3}}.
\]

Therefore, the answer is:

The answer is (B) $\geq$.