## Problem

For $a, b, c > 0$, find the largest constant $C$ such that the following inequality holds for all $a, b, c$:

$$
\left\{\left(a^2-a b+b^2\right)^2+\left(b^2-b c+c^2\right)^2+\left(c^2-c a+a^2\right)^2+3\right\}\left(\frac{1}{a b}+\frac{1}{b c}+\frac{1}{c a}\right) \geq C
$$

## Query

Task description: Please solve the problem with clear, rigorous, and logically sound steps. At the end of your response, state your answer in exactly this format: 'The answer is $C=X$', where X is your calculated numerical bound value. Example: 'The answer is $C=1$'.



Problem: Let $a, b, c$ be the side lengths, $h_{a}, h_{b}, h_{c}$ be the altitudes, respectively, and $r$ be the inradius of a triangle. Find the largest constant $C$ such that the following inequality holds for all triangles:
$$
\frac{1}{h_{a}-2 r}+\frac{1}{h_{b}-2 r}+\frac{1}{h_{c}-2 r} \geq C \cdot r
$$

Solution: By $\frac{1}{h_{a}}+\frac{1}{h_{b}}+\frac{1}{h_{c}}=\frac{1}{r}$ we obtain
$$
\frac{h_{a}-2 r}{h_{a}}+\frac{h_{b}-2 r}{h_{b}}+\frac{h_{c}-2 r}{h_{c}}=1
$$

Applying $A M \geq H M$ we get
$$
\left(\frac{h_{a}-2 r}{h_{a}}+\frac{h_{b}-2 r}{h_{b}}+\frac{h_{c}-2 r}{h_{c}}\right)\left(\frac{h_{a}}{h_{a}-2 r}+\frac{h_{b}}{h_{b}-2 r}+\frac{h_{c}}{h_{c}-2 r}\right) \geq 9
$$
i.e.
$$
\frac{h_{a}}{h_{a}-2 r}+\frac{h_{b}}{h_{b}-2 r}+\frac{h_{c}}{h_{c}-2 r} \geq 9
$$

Therefore
$$
\begin{aligned}
& \frac{2 r}{h_{a}-2 r}+\frac{2 r}{h_{b}-2 r}+\frac{2 r}{h_{c}-2 r} \\
& \quad=\frac{h_{a}-\left(h_{a}-2 r\right)}{h_{a}-2 r}+\frac{h_{b}-\left(h_{b}-2 r\right)}{h_{b}-2 r}+\frac{h_{c}-\left(h_{c}-2 r\right)}{h_{c}-2 r} \\
& \quad=\frac{h_{a}}{h_{a}-2 r}+\frac{h_{b}}{h_{b}-2 r}+\frac{h_{c}}{h_{c}-2 r}-3 \geq 9-3=6
\end{aligned}
$$
i.e.
$$
\frac{1}{h_{a}-2 r}+\frac{1}{h_{b}-2 r}+\frac{1}{h_{c}-2 r} \geq \frac{3}{r}
$$



Problem: Let $a, b, c$ be positive real numbers such that $a^2 + b^2 + c^2 = 3abc$. Find the largest constant $C$ such that the following inequality holds for all $a, b, c$ satisfying the given constraint:
$$
\frac{a}{b^2 c^2} + \frac{b}{c^2 a^2} + \frac{c}{a^2 b^2} \geq \frac{C}{a+b+c}
$$

Solution: The given inequality is equivalent to
$$
\left(a^{3}+b^{3}+c^{3}\right)(a+b+c) \geq 9 a^{2} b^{2} c^{2}
$$

Applying the Cauchy-Schwarz inequality we have
$$
\left(a^{3}+b^{3}+c^{3}\right)(a+b+c) \geq\left(a^{2}+b^{2}+c^{2}\right)^{2}
$$

Since $a^{2}+b^{2}+c^{2}=3 a b c$ we obtain
$$
\left(a^{3}+b^{3}+c^{3}\right)(a+b+c) \geq\left(a^{2}+b^{2}+c^{2}\right)^{2}=(3 a b c)^{2}=9 a^{2} b^{2} c^{2}
$$

Equality holds if and only if $a=b=c=1$.



Problem: Let $a, b, c$ be positive real numbers such that $a b c = 1$. Find the largest constant $C$ such that the following inequality holds for all $a, b, c$ satisfying the given constraint:
$$
\frac{b+c}{\sqrt{a}}+\frac{c+a}{\sqrt{b}}+\frac{a+b}{\sqrt{c}} \geq \sqrt{a}+\sqrt{b}+\sqrt{c}+C
$$

Solution: [Solution 1]
From the AM-GM Inequality, we have

$$
\begin{aligned}
& \frac{b+c}{\sqrt{a}}+\frac{c+a}{\sqrt{b}}+\frac{a+b}{\sqrt{c}} \geq 2\left(\sqrt{\frac{b c}{a}}+\sqrt{\frac{c a}{b}}+\sqrt{\frac{a b}{c}}\right)= \\
& =\left(\sqrt{\frac{b c}{a}}+\sqrt{\frac{c a}{b}}\right)+\left(\sqrt{\frac{c a}{b}}+\sqrt{\frac{a b}{c}}\right)+\left(\sqrt{\frac{a b}{c}}+\sqrt{\frac{b c}{a}}\right) \geq \\
& \geq 2(\sqrt{a}+\sqrt{b}+\sqrt{c}) \geq \sqrt{a}+\sqrt{b}+\sqrt{c}+3 \sqrt[6]{a b c}=\sqrt{a}+\sqrt{b}+\sqrt{c}+3 .
\end{aligned}
$$

Problem: For $a, b, c > 0$, find the largest constant $C$ such that the following inequality holds for all $a, b, c$:

$$
\left\{\left(a^2-a b+b^2\right)^2+\left(b^2-b c+c^2\right)^2+\left(c^2-c a+a^2\right)^2+3\right\}\left(\frac{1}{a b}+\frac{1}{b c}+\frac{1}{c a}\right) \geq C
$$

Solution:

## Response

To solve the problem, we need to analyze the given inequality:

\[
\left\{\left(a^2-ab+b^2\right)^2+\left(b^2-bc+c^2\right)^2+\left(c^2-ca+a^2\right)^2+3\right\}\left(\frac{1}{ab}+\frac{1}{bc}+\frac{1}{ca}\right) \geq C
\]

We will denote:

\[
x = a^2 - ab + b^2, \quad y = b^2 - bc + c^2, \quad z = c^2 - ca + a^2
\]

Thus, we can rewrite the inequality as:

\[
(x^2 + y^2 + z^2 + 3)\left(\frac{1}{ab} + \frac{1}{bc} + \frac{1}{ca}\right) \geq C
\]

### Step 1: Analyze the terms \(x\), \(y\), and \(z\)

Using the identity \(x = a^2 - ab + b^2\), we can see that:

\[
x = \frac{1}{2}((a-b)^2 + a^2 + b^2)
\]

This shows that \(x\) is always non-negative. The same applies to \(y\) and \(z\).

### Step 2: Find a lower bound for \(x^2 + y^2 + z^2 + 3\)

Since \(x\), \(y\), and \(z\) are non-negative, we can find a lower bound for \(x^2 + y^2 + z^2\). By the Cauchy-Schwarz inequality:

\[
(x^2 + y^2 + z^2)(1 + 1 + 1) \geq (x + y + z)^2
\]

Thus,

\[
x^2 + y^2 + z^2 \geq \frac{(x + y + z)^2}{3}
\]

### Step 3: Calculate \(x + y + z\)

We can express \(x + y + z\) as:

\[
x + y + z = (a^2 - ab + b^2) + (b^2 - bc + c^2) + (c^2 - ca + a^2) = 2(a^2 + b^2 + c^2) - (ab + bc + ca)
\]

Using the identity \(a^2 + b^2 + c^2 \geq ab + bc + ca\) (which follows from the rearrangement inequality), we can conclude that \(x + y + z\) is non-negative.

### Step 4: Analyze the term \(\frac{1}{ab} + \frac{1}{bc} + \frac{1}{ca}\)

Using the AM-HM inequality:

\[
\frac{ab + bc + ca}{3} \geq \frac{3}{\frac{1}{ab} + \frac{1}{bc} + \frac{1}{ca}}
\]

This implies:

\[
\frac{1}{ab} + \frac{1}{bc} + \frac{1}{ca} \geq \frac{9}{a+b+c}
\]

### Step 5: Combine results

Now we can combine our results. We have:

\[
(x^2 + y^2 + z^2 + 3) \geq 3
\]

Thus, we can write:

\[
(x^2 + y^2 + z^2 + 3)\left(\frac{1}{ab} + \frac{1}{bc} + \frac{1}{ca}\right) \geq 3 \cdot \frac{9}{a+b+c} = \frac{27}{a+b+c}
\]

### Step 6: Find the largest constant \(C\)

To find the largest constant \(C\), we need to ensure that the inequality holds for all positive \(a, b, c\). The minimum value of \(a + b + c\) occurs when \(a = b = c = 1\), giving \(a + b + c = 3\). Thus, we can conclude:

\[
C \leq 9
\]

### Conclusion

The largest constant \(C\) such that the inequality holds for all positive \(a, b, c\) is:

\[
\boxed{9}
\]

Thus, the final answer is:

The answer is \(C=9\).