## Problem

Let $x_1, x_2, \ldots, x_n$ be positive real numbers such that $x_1 + x_2 + \cdots + x_n = 1$. Consider the following expression:
$$
\sum_{i=1}^n \frac{\min \left\{x_{i-1}, x_i\right\} \cdot \max \left\{x_i, x_{i+1}\right\}}{x_i} \quad () \quad 1
$$
where we denote $x_0 = x_n$ and $x_{n+1} = x_1$.

Determine the correct inequality relation to fill in the blank.

Options:

(A) $\leq$ 

(B) $\geq$

(C) $=$ 

(D) $<$

(E) $>$

(F) None of the above

## Query

Task description: Please solve the problem with clear, rigorous, and logically sound steps. At the end of your response, state your answer in exactly this format: 'The answer is (Letter) Symbol', where Letter is one of the given options. Example: 'The answer is (A) $\leq$'.



Problem: Let $n \in \mathbb{N}$, and $\alpha, \beta, \gamma$ be the angles of a given triangle. Consider the following inequality:
$$
\cot ^{n} \frac{\alpha}{2}+\cot ^{n} \frac{\beta}{2}+\cot ^{n} \frac{\gamma}{2} \quad () \quad 3^{\frac{n+2}{2}} .
$$

Determine the correct inequality relation to fill in the blank.

Options:

(A) $\leq$ 

(B) $\geq$

(C) $=$ 

(D) $<$

(E) $>$

(F) None of the above

Solution: We use the identity
$$
\cot \frac{\alpha}{2}+\cot \frac{\beta}{2}+\cot \frac{\gamma}{2}=\cot \frac{\alpha}{2} \cdot \cot \frac{\beta}{2} \cdot \cot \frac{\gamma}{2} .
$$

Since $\frac{\alpha}{2}, \frac{\beta}{2}, \frac{\gamma}{2} \in(0, \pi / 2)$ it follows that $\cot \frac{\alpha}{2}, \cot \frac{\beta}{2}, \cot \frac{\gamma}{2} \geq 0$.
Applying $A M \geq G M$ we have
$$
\cot \frac{\alpha}{2}+\cot \frac{\beta}{2}+\cot \frac{\gamma}{2} \geq 3 \sqrt[3]{\cot \frac{\alpha}{2} \cdot \cot \frac{\beta}{2} \cdot \cot \frac{\gamma}{2}}
$$
or
$$
\cot \frac{\alpha}{2} \cdot \cot \frac{\beta}{2} \cdot \cot \frac{\gamma}{2} \geq 3 \sqrt[3]{\cot \frac{\alpha}{2} \cdot \cot \frac{\beta}{2} \cdot \cot \frac{\gamma}{2}}
$$
i.e.
$$
\begin{equation*}
\cot \frac{\alpha}{2} \cdot \cot \frac{\beta}{2} \cdot \cot \frac{\gamma}{2} \geq 3^{3 / 2} \tag{1}
\end{equation*}
$$

Furthermore, using the power mean inequality we get
$$
\cot ^{n} \frac{\alpha}{2}+\cot ^{n} \frac{\beta}{2}+\cot ^{n} \frac{\gamma}{2} \geq 3\left(\cot \frac{\alpha}{2} \cdot \cot \frac{\beta}{2} \cdot \cot \frac{\gamma}{2}\right)^{n / 3} .
$$

Now from the previous inequality and (1) we obtain
$$
\cot ^{n} \frac{\alpha}{2}+\cot ^{n} \frac{\beta}{2}+\cot ^{n} \frac{\gamma}{2} \geq 3^{\frac{n+2}{2}}
$$

Equality occurs iff $\alpha=\beta=\gamma=\pi / 3$.



Problem: Let $x, y, z > 1$ be real numbers such that $\frac{1}{x}+\frac{1}{y}+\frac{1}{z}=2$. Consider the following expressions:
$$
\sqrt{x-1}+\sqrt{y-1}+\sqrt{z-1} \quad () \quad \sqrt{x+y+z}
$$
Determine the correct inequality relation to fill in the blank.

Options:

(A) $\leq$ 

(B) $\geq$

(C) $=$ 

(D) $<$

(E) $>$

(F) None of the above

Solution: Let $x=a+1, y=b+1, z=c+1$, and clearly $a, b$ and $c$ are positive real numbers.

The initial condition $\frac{1}{x}+\frac{1}{y}+\frac{1}{z}=2$ becomes $\frac{1}{a+1}+\frac{1}{b+1}+\frac{1}{c+1}=2$, i.e.
$$
\begin{equation*}
a b+b c+c a+2 a b c=1 \tag{1}
\end{equation*}
$$

We need to show that
$$
\begin{equation*}
\sqrt{a}+\sqrt{b}+\sqrt{c} \leq \sqrt{a+b+c+3} \tag{2}
\end{equation*}
$$

After squaring inequality (2) we get
$$
a+b+c+2 \sqrt{a b}+2 \sqrt{b c}+2 \sqrt{c a} \leq a+b+c+3
$$
or
$$
2 \sqrt{a b}+2 \sqrt{b c}+2 \sqrt{c a} \leq 3
$$
i.e.
$$
\begin{equation*}
\sqrt{a b}+\sqrt{b c}+\sqrt{c a} \leq \frac{3}{2} \tag{3}
\end{equation*}
$$

Identity (1) is equivalent to
$$
(\sqrt{a b})^{2}+(\sqrt{b c})^{2}+(\sqrt{c a})^{2}+2(\sqrt{a b} \cdot \sqrt{b c} \cdot \sqrt{c a})=1
$$
so we may take
$$
\sqrt{a b}=\sin \frac{\alpha}{2}, \quad \sqrt{b c}=\sin \frac{\beta}{2}, \quad \sqrt{c a}=\sin \frac{\gamma}{2}
$$
where $\alpha, \beta, \gamma \in(0, \pi)$ and $\alpha+\beta+\gamma=\pi$.
Now inequality (3) is equivalent to
$$
\sin \frac{\alpha}{2}+\sin \frac{\beta}{2}+\sin \frac{\gamma}{2} \leq \frac{3}{2}
$$
where $\alpha, \beta, \gamma \in(0, \pi), \alpha+\beta+\gamma=\pi$, which is true by $N_{3}$ .,Applying the Cauchy-Schwarz inequality we have
$$
\left(\frac{x-1}{x}+\frac{y-1}{y}+\frac{z-1}{z}\right)(x+y+z) \geq(\sqrt{x-1}+\sqrt{y-1}+\sqrt{z-1})^{2} .
$$

Also
$$
\frac{x-1}{x}+\frac{y-1}{y}+\frac{z-1}{z}=3-\left(\frac{1}{x}+\frac{1}{y}+\frac{1}{z}\right)=1
$$

So
$$
x+y+z \geq(\sqrt{x-1}+\sqrt{y-1}+\sqrt{z-1})^{2}
$$
i.e.
$$
\sqrt{x+y+z} \geq \sqrt{x-1}+\sqrt{y-1}+\sqrt{z-1}
$$

Equality occurs iff $\frac{x-1}{x^{2}}=\frac{y-1}{y^{2}}=\frac{z-1}{z^{2}}$ and $\frac{1}{x}+\frac{1}{y}+\frac{1}{z}=2$, i.e. $x=y=z=3 / 2$.



Problem: Let $x, y, z$ be positive real numbers satisfying the condition
$$
x^{2}+y^{2}+z^{2}+2 x y z=1.
$$

Consider the following expression:
$$
x+y+z \quad () \quad \frac{3}{2}.
$$

Determine the correct inequality relation to fill in the blank.

Options:

(A) $\leq$ 

(B) $\geq$

(C) $=$ 

(D) $<$

(E) $>$

(F) None of the above

Solution: Clearly, we must have $x, y, z \in(0,1)$. If we put $s=x+y+z$, we get immediately from the given relation

$$
s^{2}-2 s+1=2(1-x)(1-y)(1-z)
$$

Then, again by the AM-GM Inequality ( $1-x, 1-y, 1-z$ being positive), we obtain

$$
s^{2}-2 s+1 \leq 2\left(\frac{1-x+1-y+1-z}{3}\right)^{3}=2\left(\frac{3-s}{3}\right)^{3}
$$

After some easy calculations this yields

$$
2 s^{3}+9 s^{2}-27 \leq 0 \Leftrightarrow(2 s-3)(s+3)^{2} \leq 0
$$

and the conclusion is plain.

Problem: Let $x_1, x_2, \ldots, x_n$ be positive real numbers such that $x_1 + x_2 + \cdots + x_n = 1$. Consider the following expression:
$$
\sum_{i=1}^n \frac{\min \left\{x_{i-1}, x_i\right\} \cdot \max \left\{x_i, x_{i+1}\right\}}{x_i} \quad () \quad 1
$$
where we denote $x_0 = x_n$ and $x_{n+1} = x_1$.

Determine the correct inequality relation to fill in the blank.

Options:

(A) $\leq$ 

(B) $\geq$

(C) $=$ 

(D) $<$

(E) $>$

(F) None of the above

Solution:

## Response

To solve the problem, we need to analyze the expression 

\[
\sum_{i=1}^n \frac{\min \left\{x_{i-1}, x_i\right\} \cdot \max \left\{x_i, x_{i+1}\right\}}{x_i}
\]

given the constraint \(x_1 + x_2 + \cdots + x_n = 1\) where \(x_i > 0\) for all \(i\).

### Step 1: Understanding the Terms

For each term in the sum, we have:

- \(x_{i-1}\) and \(x_{i+1}\) are the neighboring terms of \(x_i\).
- The term \(\min \{x_{i-1}, x_i\}\) will take the smaller of \(x_{i-1}\) and \(x_i\).
- The term \(\max \{x_i, x_{i+1}\}\) will take the larger of \(x_i\) and \(x_{i+1}\).

### Step 2: Analyzing the Expression

We can rewrite the expression as:

\[
\sum_{i=1}^n \frac{\min \{x_{i-1}, x_i\} \cdot \max \{x_i, x_{i+1}\}}{x_i}
\]

This can be interpreted as a weighted average of the ratios of the minimum and maximum values of the neighboring terms, normalized by \(x_i\).

### Step 3: Applying the Cauchy-Schwarz Inequality

To analyze the sum, we can apply the Cauchy-Schwarz inequality. We can express the sum in a form that allows us to use this inequality effectively.

Let \(a_i = \min \{x_{i-1}, x_i\}\) and \(b_i = \max \{x_i, x_{i+1}\}\). Then we can write:

\[
\sum_{i=1}^n \frac{a_i b_i}{x_i}
\]

By Cauchy-Schwarz, we have:

\[
\left(\sum_{i=1}^n \frac{a_i b_i}{x_i}\right) \left(\sum_{i=1}^n x_i\right) \geq \left(\sum_{i=1}^n \sqrt{a_i b_i}\right)^2
\]

Since \(\sum_{i=1}^n x_i = 1\), we simplify this to:

\[
\sum_{i=1}^n \frac{a_i b_i}{x_i} \geq \left(\sum_{i=1}^n \sqrt{a_i b_i}\right)^2
\]

### Step 4: Bounding the Expression

Now, we need to show that:

\[
\sum_{i=1}^n \frac{\min \{x_{i-1}, x_i\} \cdot \max \{x_i, x_{i+1}\}}{x_i} \geq 1
\]

To do this, we can consider specific cases. For example, if all \(x_i\) are equal, say \(x_i = \frac{1}{n}\), then:

\[
\min \{x_{i-1}, x_i\} = \frac{1}{n}, \quad \max \{x_i, x_{i+1}\} = \frac{1}{n}
\]

Thus, each term in the sum becomes:

\[
\frac{\frac{1}{n} \cdot \frac{1}{n}}{\frac{1}{n}} = \frac{1}{n}
\]

Summing over \(n\) terms gives:

\[
\sum_{i=1}^n \frac{1}{n} = 1
\]

### Conclusion

Since we have shown that the expression equals 1 when all \(x_i\) are equal, and by the nature of the terms involved, we can conclude that:

\[
\sum_{i=1}^n \frac{\min \{x_{i-1}, x_i\} \cdot \max \{x_i, x_{i+1}\}}{x_i} \geq 1
\]

Thus, the correct inequality relation to fill in the blank is:

\[
\sum_{i=1}^n \frac{\min \left\{x_{i-1}, x_i\right\} \cdot \max \left\{x_i, x_{i+1}\right\}}{x_i} \geq 1
\]

Therefore, the answer is:

The answer is (B) $\geq$