## Problem

Let $a, b, c$ be real numbers such that $0 < a \leq b \leq c$. Find the largest constant $C$ such that the following inequality holds for all $a, b, c$ satisfying the given constraints:
$$
(a+b)(c+a)^2 \geq C a b c
$$

## Query

Task description: Please solve the problem with clear, rigorous, and logically sound steps. At the end of your response, state your answer in exactly this format: 'The answer is $C=X$', where X is your calculated numerical bound value. Example: 'The answer is $C=1$'.



Problem: Let $a, b, c$ be the side lengths, $h_{a}, h_{b}, h_{c}$ be the altitudes, respectively, and $r$ be the inradius of a triangle. Find the largest constant $C$ such that the following inequality holds for all triangles:
$$
\frac{1}{h_{a}-2 r}+\frac{1}{h_{b}-2 r}+\frac{1}{h_{c}-2 r} \geq C \cdot r
$$

Solution: By $\frac{1}{h_{a}}+\frac{1}{h_{b}}+\frac{1}{h_{c}}=\frac{1}{r}$ we obtain
$$
\frac{h_{a}-2 r}{h_{a}}+\frac{h_{b}-2 r}{h_{b}}+\frac{h_{c}-2 r}{h_{c}}=1
$$

Applying $A M \geq H M$ we get
$$
\left(\frac{h_{a}-2 r}{h_{a}}+\frac{h_{b}-2 r}{h_{b}}+\frac{h_{c}-2 r}{h_{c}}\right)\left(\frac{h_{a}}{h_{a}-2 r}+\frac{h_{b}}{h_{b}-2 r}+\frac{h_{c}}{h_{c}-2 r}\right) \geq 9
$$
i.e.
$$
\frac{h_{a}}{h_{a}-2 r}+\frac{h_{b}}{h_{b}-2 r}+\frac{h_{c}}{h_{c}-2 r} \geq 9
$$

Therefore
$$
\begin{aligned}
& \frac{2 r}{h_{a}-2 r}+\frac{2 r}{h_{b}-2 r}+\frac{2 r}{h_{c}-2 r} \\
& \quad=\frac{h_{a}-\left(h_{a}-2 r\right)}{h_{a}-2 r}+\frac{h_{b}-\left(h_{b}-2 r\right)}{h_{b}-2 r}+\frac{h_{c}-\left(h_{c}-2 r\right)}{h_{c}-2 r} \\
& \quad=\frac{h_{a}}{h_{a}-2 r}+\frac{h_{b}}{h_{b}-2 r}+\frac{h_{c}}{h_{c}-2 r}-3 \geq 9-3=6
\end{aligned}
$$
i.e.
$$
\frac{1}{h_{a}-2 r}+\frac{1}{h_{b}-2 r}+\frac{1}{h_{c}-2 r} \geq \frac{3}{r}
$$



Problem: Let $a, b, c$ be positive real numbers such that $a^2 + b^2 + c^2 = 3abc$. Find the largest constant $C$ such that the following inequality holds for all $a, b, c$ satisfying the given constraint:
$$
\frac{a}{b^2 c^2} + \frac{b}{c^2 a^2} + \frac{c}{a^2 b^2} \geq \frac{C}{a+b+c}
$$

Solution: The given inequality is equivalent to
$$
\left(a^{3}+b^{3}+c^{3}\right)(a+b+c) \geq 9 a^{2} b^{2} c^{2}
$$

Applying the Cauchy-Schwarz inequality we have
$$
\left(a^{3}+b^{3}+c^{3}\right)(a+b+c) \geq\left(a^{2}+b^{2}+c^{2}\right)^{2}
$$

Since $a^{2}+b^{2}+c^{2}=3 a b c$ we obtain
$$
\left(a^{3}+b^{3}+c^{3}\right)(a+b+c) \geq\left(a^{2}+b^{2}+c^{2}\right)^{2}=(3 a b c)^{2}=9 a^{2} b^{2} c^{2}
$$

Equality holds if and only if $a=b=c=1$.



Problem: Let $a, b, c$ be positive real numbers such that $a b c = 1$. Find the largest constant $C$ such that the following inequality holds for all $a, b, c$ satisfying the given constraint:
$$
\frac{b+c}{\sqrt{a}}+\frac{c+a}{\sqrt{b}}+\frac{a+b}{\sqrt{c}} \geq \sqrt{a}+\sqrt{b}+\sqrt{c}+C
$$

Solution: [Solution 1]
From the AM-GM Inequality, we have

$$
\begin{aligned}
& \frac{b+c}{\sqrt{a}}+\frac{c+a}{\sqrt{b}}+\frac{a+b}{\sqrt{c}} \geq 2\left(\sqrt{\frac{b c}{a}}+\sqrt{\frac{c a}{b}}+\sqrt{\frac{a b}{c}}\right)= \\
& =\left(\sqrt{\frac{b c}{a}}+\sqrt{\frac{c a}{b}}\right)+\left(\sqrt{\frac{c a}{b}}+\sqrt{\frac{a b}{c}}\right)+\left(\sqrt{\frac{a b}{c}}+\sqrt{\frac{b c}{a}}\right) \geq \\
& \geq 2(\sqrt{a}+\sqrt{b}+\sqrt{c}) \geq \sqrt{a}+\sqrt{b}+\sqrt{c}+3 \sqrt[6]{a b c}=\sqrt{a}+\sqrt{b}+\sqrt{c}+3 .
\end{aligned}
$$

Problem: Let $a, b, c$ be real numbers such that $0 < a \leq b \leq c$. Find the largest constant $C$ such that the following inequality holds for all $a, b, c$ satisfying the given constraints:
$$
(a+b)(c+a)^2 \geq C a b c
$$

Solution:

## Response

To solve the problem, we need to find the largest constant \( C \) such that the inequality 

\[
(a+b)(c+a)^2 \geq C a b c
\]

holds for all positive real numbers \( a, b, c \) satisfying \( 0 < a \leq b \leq c \).

### Step 1: Analyze the inequality

We can expand the left-hand side:

\[
(a+b)(c+a)^2 = (a+b)(c^2 + 2ac + a^2) = (a+b)(c^2 + 2ac + a^2) = ac^2 + 2a^2c + a^3 + bc^2 + 2abc + b^2a
\]

### Step 2: Test specific cases

To find the largest \( C \), we can test specific values of \( a, b, c \). A natural choice is to set \( a = 1 \), \( b = 1 \), and \( c = 1 \):

\[
(1+1)(1+1)^2 = 2 \cdot 4 = 8
\]
\[
C \cdot 1 \cdot 1 \cdot 1 = C
\]

This gives us:

\[
8 \geq C \implies C \leq 8
\]

### Step 3: Check if \( C = 8 \) holds for all \( a, b, c \)

Now we need to check if the inequality holds for \( C = 8 \):

\[
(a+b)(c+a)^2 \geq 8abc
\]

### Step 4: Use AM-GM inequality

Using the AM-GM inequality, we can analyze the terms:

1. \( a + b \geq 2\sqrt{ab} \)
2. \( c + a \geq 2\sqrt{ac} \)

Thus,

\[
(c+a)^2 \geq 4ac
\]

Now, substituting these into our inequality:

\[
(a+b)(c+a)^2 \geq (2\sqrt{ab})(4ac) = 8abc
\]

This shows that the inequality holds for \( C = 8 \).

### Step 5: Conclusion

Since we have shown that \( C = 8 \) satisfies the inequality for all \( a, b, c \) under the given conditions, we conclude that the largest constant \( C \) is:

\[
\boxed{8}
\]

Thus, the final answer is:

The answer is \( C=8 \).