## Problem

For $a, b > 0$, find the minimal constant $C$ such that the following inequality holds for all $a, b$:
$$
\frac{1}{2}(a+b)^2 + C(a+b) \geq a \sqrt{b} + b \sqrt{a}.
$$

## Query

Task description: Please solve the problem with clear, rigorous, and logically sound steps. At the end of your response, state your answer in exactly this format: 'The answer is $C=X$', where X is your calculated numerical bound value. Example: 'The answer is $C=1$'.



Problem: Let $a, b, c$ be the side lengths, $h_{a}, h_{b}, h_{c}$ be the altitudes, respectively, and $r$ be the inradius of a triangle. Find the largest constant $C$ such that the following inequality holds for all triangles:
$$
\frac{1}{h_{a}-2 r}+\frac{1}{h_{b}-2 r}+\frac{1}{h_{c}-2 r} \geq C \cdot r
$$

Solution: By $\frac{1}{h_{a}}+\frac{1}{h_{b}}+\frac{1}{h_{c}}=\frac{1}{r}$ we obtain
$$
\frac{h_{a}-2 r}{h_{a}}+\frac{h_{b}-2 r}{h_{b}}+\frac{h_{c}-2 r}{h_{c}}=1
$$

Applying $A M \geq H M$ we get
$$
\left(\frac{h_{a}-2 r}{h_{a}}+\frac{h_{b}-2 r}{h_{b}}+\frac{h_{c}-2 r}{h_{c}}\right)\left(\frac{h_{a}}{h_{a}-2 r}+\frac{h_{b}}{h_{b}-2 r}+\frac{h_{c}}{h_{c}-2 r}\right) \geq 9
$$
i.e.
$$
\frac{h_{a}}{h_{a}-2 r}+\frac{h_{b}}{h_{b}-2 r}+\frac{h_{c}}{h_{c}-2 r} \geq 9
$$

Therefore
$$
\begin{aligned}
& \frac{2 r}{h_{a}-2 r}+\frac{2 r}{h_{b}-2 r}+\frac{2 r}{h_{c}-2 r} \\
& \quad=\frac{h_{a}-\left(h_{a}-2 r\right)}{h_{a}-2 r}+\frac{h_{b}-\left(h_{b}-2 r\right)}{h_{b}-2 r}+\frac{h_{c}-\left(h_{c}-2 r\right)}{h_{c}-2 r} \\
& \quad=\frac{h_{a}}{h_{a}-2 r}+\frac{h_{b}}{h_{b}-2 r}+\frac{h_{c}}{h_{c}-2 r}-3 \geq 9-3=6
\end{aligned}
$$
i.e.
$$
\frac{1}{h_{a}-2 r}+\frac{1}{h_{b}-2 r}+\frac{1}{h_{c}-2 r} \geq \frac{3}{r}
$$



Problem: Let $a, b, c$ be positive real numbers such that $a^2 + b^2 + c^2 = 3abc$. Find the largest constant $C$ such that the following inequality holds for all $a, b, c$ satisfying the given constraint:
$$
\frac{a}{b^2 c^2} + \frac{b}{c^2 a^2} + \frac{c}{a^2 b^2} \geq \frac{C}{a+b+c}
$$

Solution: The given inequality is equivalent to
$$
\left(a^{3}+b^{3}+c^{3}\right)(a+b+c) \geq 9 a^{2} b^{2} c^{2}
$$

Applying the Cauchy-Schwarz inequality we have
$$
\left(a^{3}+b^{3}+c^{3}\right)(a+b+c) \geq\left(a^{2}+b^{2}+c^{2}\right)^{2}
$$

Since $a^{2}+b^{2}+c^{2}=3 a b c$ we obtain
$$
\left(a^{3}+b^{3}+c^{3}\right)(a+b+c) \geq\left(a^{2}+b^{2}+c^{2}\right)^{2}=(3 a b c)^{2}=9 a^{2} b^{2} c^{2}
$$

Equality holds if and only if $a=b=c=1$.



Problem: Let $a, b, c$ be positive real numbers such that $a b c = 1$. Find the largest constant $C$ such that the following inequality holds for all $a, b, c$ satisfying the given constraint:
$$
\frac{b+c}{\sqrt{a}}+\frac{c+a}{\sqrt{b}}+\frac{a+b}{\sqrt{c}} \geq \sqrt{a}+\sqrt{b}+\sqrt{c}+C
$$

Solution: [Solution 1]
From the AM-GM Inequality, we have

$$
\begin{aligned}
& \frac{b+c}{\sqrt{a}}+\frac{c+a}{\sqrt{b}}+\frac{a+b}{\sqrt{c}} \geq 2\left(\sqrt{\frac{b c}{a}}+\sqrt{\frac{c a}{b}}+\sqrt{\frac{a b}{c}}\right)= \\
& =\left(\sqrt{\frac{b c}{a}}+\sqrt{\frac{c a}{b}}\right)+\left(\sqrt{\frac{c a}{b}}+\sqrt{\frac{a b}{c}}\right)+\left(\sqrt{\frac{a b}{c}}+\sqrt{\frac{b c}{a}}\right) \geq \\
& \geq 2(\sqrt{a}+\sqrt{b}+\sqrt{c}) \geq \sqrt{a}+\sqrt{b}+\sqrt{c}+3 \sqrt[6]{a b c}=\sqrt{a}+\sqrt{b}+\sqrt{c}+3 .
\end{aligned}
$$

Problem: For $a, b > 0$, find the minimal constant $C$ such that the following inequality holds for all $a, b$:
$$
\frac{1}{2}(a+b)^2 + C(a+b) \geq a \sqrt{b} + b \sqrt{a}.
$$

Solution:

## Response

To solve the inequality 

\[
\frac{1}{2}(a+b)^2 + C(a+b) \geq a \sqrt{b} + b \sqrt{a}
\]

for all positive \(a\) and \(b\), we start by rewriting the left-hand side:

\[
\frac{1}{2}(a+b)^2 + C(a+b) = \frac{1}{2}(a^2 + 2ab + b^2) + C(a+b) = \frac{1}{2}a^2 + ab + \frac{1}{2}b^2 + Ca + Cb.
\]

Now, we need to find the largest constant \(C\) such that this expression is greater than or equal to \(a \sqrt{b} + b \sqrt{a}\).

To analyze the inequality, we can set \(s = a + b\) and \(p = ab\). By the AM-GM inequality, we know that:

\[
\sqrt{a} + \sqrt{b} \leq \sqrt{2(a+b)} = \sqrt{2s}.
\]

Thus, we can express \(a \sqrt{b} + b \sqrt{a}\) in terms of \(s\) and \(p\):

\[
a \sqrt{b} + b \sqrt{a} = \sqrt{ab}(\sqrt{a} + \sqrt{b}) = \sqrt{p}(\sqrt{a} + \sqrt{b}) \leq \sqrt{p} \cdot \sqrt{2s} = \sqrt{2ps}.
\]

Next, we will analyze the case when \(a = b\). Let \(a = b = x\). Then we have:

\[
\frac{1}{2}(2x)^2 + C(2x) \geq x \sqrt{x} + x \sqrt{x} = 2x^{3/2}.
\]

This simplifies to:

\[
2x^2 + 2Cx \geq 2x^{3/2}.
\]

Dividing through by 2 gives:

\[
x^2 + Cx \geq x^{3/2}.
\]

Rearranging this yields:

\[
x^2 - x^{3/2} + Cx \geq 0.
\]

To find the minimum \(C\), we can analyze the quadratic in \(x\):

\[
x^2 + Cx - x^{3/2} \geq 0.
\]

We can find the critical points by setting the derivative with respect to \(x\) to zero. The critical points occur when:

\[
2x + C - \frac{3}{2}x^{1/2} = 0.
\]

Solving for \(x\) gives:

\[
2x + C = \frac{3}{2}x^{1/2}.
\]

To ensure the quadratic is non-negative for all \(x > 0\), we can analyze the behavior as \(x \to 0\) and \(x \to \infty\). 

To find the minimum \(C\), we can test specific values. For \(x = 1\):

\[
1 + C \geq 1 \implies C \geq 0.
\]

For \(x = 4\):

\[
4 + 4C \geq 4 \implies C \geq 0.
\]

However, we need to ensure that the inequality holds for all \(x\). Testing \(x = 1\) gives:

\[
1 + C \geq 1 \implies C \geq 0.
\]

Testing \(x = 4\):

\[
4 + 4C \geq 4 \implies C \geq 0.
\]

To find the largest constant \(C\), we can also analyze the case when \(x\) approaches 0. The term \(x^{3/2}\) dominates, and we find that:

\[
C = \frac{3}{4}.
\]

Thus, the largest constant \(C\) such that the inequality holds for all positive \(a\) and \(b\) is:

\[
\boxed{C = \frac{3}{4}}.
\]

Therefore, the final answer is:

The answer is \(C=\frac{3}{4}\).