## Problem

Let $x, y, z > 0$ such that $x + y + z = xyz$. Find the smallest constant $C$ such that the following inequality holds for all $x, y, z$ satisfying the given constraint:
$$
(x-1)(y-1)(z-1) \leq C
$$

## Query

Task description: Please solve the problem with clear, rigorous, and logically sound steps. At the end of your response, state your answer in exactly this format: 'The answer is $C=X$', where X is your calculated numerical bound value. Example: 'The answer is $C=1$'.



Problem: Let $a, b, c$ be the side lengths, $h_{a}, h_{b}, h_{c}$ be the altitudes, respectively, and $r$ be the inradius of a triangle. Find the largest constant $C$ such that the following inequality holds for all triangles:
$$
\frac{1}{h_{a}-2 r}+\frac{1}{h_{b}-2 r}+\frac{1}{h_{c}-2 r} \geq C \cdot r
$$

Solution: By $\frac{1}{h_{a}}+\frac{1}{h_{b}}+\frac{1}{h_{c}}=\frac{1}{r}$ we obtain
$$
\frac{h_{a}-2 r}{h_{a}}+\frac{h_{b}-2 r}{h_{b}}+\frac{h_{c}-2 r}{h_{c}}=1
$$

Applying $A M \geq H M$ we get
$$
\left(\frac{h_{a}-2 r}{h_{a}}+\frac{h_{b}-2 r}{h_{b}}+\frac{h_{c}-2 r}{h_{c}}\right)\left(\frac{h_{a}}{h_{a}-2 r}+\frac{h_{b}}{h_{b}-2 r}+\frac{h_{c}}{h_{c}-2 r}\right) \geq 9
$$
i.e.
$$
\frac{h_{a}}{h_{a}-2 r}+\frac{h_{b}}{h_{b}-2 r}+\frac{h_{c}}{h_{c}-2 r} \geq 9
$$

Therefore
$$
\begin{aligned}
& \frac{2 r}{h_{a}-2 r}+\frac{2 r}{h_{b}-2 r}+\frac{2 r}{h_{c}-2 r} \\
& \quad=\frac{h_{a}-\left(h_{a}-2 r\right)}{h_{a}-2 r}+\frac{h_{b}-\left(h_{b}-2 r\right)}{h_{b}-2 r}+\frac{h_{c}-\left(h_{c}-2 r\right)}{h_{c}-2 r} \\
& \quad=\frac{h_{a}}{h_{a}-2 r}+\frac{h_{b}}{h_{b}-2 r}+\frac{h_{c}}{h_{c}-2 r}-3 \geq 9-3=6
\end{aligned}
$$
i.e.
$$
\frac{1}{h_{a}-2 r}+\frac{1}{h_{b}-2 r}+\frac{1}{h_{c}-2 r} \geq \frac{3}{r}
$$



Problem: Let $a, b, c$ be positive real numbers such that $a^2 + b^2 + c^2 = 3abc$. Find the largest constant $C$ such that the following inequality holds for all $a, b, c$ satisfying the given constraint:
$$
\frac{a}{b^2 c^2} + \frac{b}{c^2 a^2} + \frac{c}{a^2 b^2} \geq \frac{C}{a+b+c}
$$

Solution: The given inequality is equivalent to
$$
\left(a^{3}+b^{3}+c^{3}\right)(a+b+c) \geq 9 a^{2} b^{2} c^{2}
$$

Applying the Cauchy-Schwarz inequality we have
$$
\left(a^{3}+b^{3}+c^{3}\right)(a+b+c) \geq\left(a^{2}+b^{2}+c^{2}\right)^{2}
$$

Since $a^{2}+b^{2}+c^{2}=3 a b c$ we obtain
$$
\left(a^{3}+b^{3}+c^{3}\right)(a+b+c) \geq\left(a^{2}+b^{2}+c^{2}\right)^{2}=(3 a b c)^{2}=9 a^{2} b^{2} c^{2}
$$

Equality holds if and only if $a=b=c=1$.



Problem: Let $a, b, c$ be positive real numbers such that $a b c = 1$. Find the largest constant $C$ such that the following inequality holds for all $a, b, c$ satisfying the given constraint:
$$
\frac{b+c}{\sqrt{a}}+\frac{c+a}{\sqrt{b}}+\frac{a+b}{\sqrt{c}} \geq \sqrt{a}+\sqrt{b}+\sqrt{c}+C
$$

Solution: [Solution 1]
From the AM-GM Inequality, we have

$$
\begin{aligned}
& \frac{b+c}{\sqrt{a}}+\frac{c+a}{\sqrt{b}}+\frac{a+b}{\sqrt{c}} \geq 2\left(\sqrt{\frac{b c}{a}}+\sqrt{\frac{c a}{b}}+\sqrt{\frac{a b}{c}}\right)= \\
& =\left(\sqrt{\frac{b c}{a}}+\sqrt{\frac{c a}{b}}\right)+\left(\sqrt{\frac{c a}{b}}+\sqrt{\frac{a b}{c}}\right)+\left(\sqrt{\frac{a b}{c}}+\sqrt{\frac{b c}{a}}\right) \geq \\
& \geq 2(\sqrt{a}+\sqrt{b}+\sqrt{c}) \geq \sqrt{a}+\sqrt{b}+\sqrt{c}+3 \sqrt[6]{a b c}=\sqrt{a}+\sqrt{b}+\sqrt{c}+3 .
\end{aligned}
$$

Problem: Let $x, y, z > 0$ such that $x + y + z = xyz$. Find the smallest constant $C$ such that the following inequality holds for all $x, y, z$ satisfying the given constraint:
$$
(x-1)(y-1)(z-1) \leq C
$$

Solution:

## Response

To solve the problem, we start with the condition given: \( x + y + z = xyz \). We want to find the smallest constant \( C \) such that the inequality 

\[
(x-1)(y-1)(z-1) \leq C
\]

holds for all positive \( x, y, z \) satisfying the constraint.

First, we can rewrite the left-hand side of the inequality:

\[
(x-1)(y-1)(z-1) = xyz - (xy + xz + yz) + (x + y + z) - 1
\]

Using the condition \( x + y + z = xyz \), we can substitute this into our expression:

\[
(x-1)(y-1)(z-1) = xyz - (xy + xz + yz) + xyz - 1 = 2xyz - (xy + xz + yz) - 1
\]

Next, we will analyze the case when \( x = y = z \). Let \( x = y = z = t \). Then, the condition becomes:

\[
3t = t^3 \implies t^3 - 3t = 0 \implies t(t^2 - 3) = 0
\]

Since \( t > 0 \), we have \( t = \sqrt{3} \). Now we can evaluate \( (x-1)(y-1)(z-1) \) at this point:

\[
(x-1)(y-1)(z-1) = (t-1)^3 = (\sqrt{3} - 1)^3
\]

Calculating \( (\sqrt{3} - 1)^3 \):

\[
(\sqrt{3} - 1)^3 = (\sqrt{3} - 1)(\sqrt{3} - 1)(\sqrt{3} - 1) = (3 - 2\sqrt{3} + 1)(\sqrt{3} - 1) = (4 - 2\sqrt{3})(\sqrt{3} - 1)
\]

Expanding this:

\[
= 4\sqrt{3} - 4 - 2\cdot3 + 2\sqrt{3} = 6\sqrt{3} - 10
\]

Now we need to find the maximum value of \( (x-1)(y-1)(z-1) \) under the constraint \( x + y + z = xyz \). 

To find the maximum, we can also consider the case when two variables are equal and one is different. For example, let \( x = y = t \) and \( z = \frac{t^2}{t-1} \) (derived from the condition). 

Substituting this into the expression gives us a more complex function to analyze, but we can also check specific values. 

After testing various values, we find that the maximum occurs at \( x = y = z = \sqrt{3} \), yielding:

\[
(x-1)(y-1)(z-1) = (\sqrt{3} - 1)^3 = 6\sqrt{3} - 10
\]

To find \( C \), we need to evaluate \( 6\sqrt{3} - 10 \):

Calculating \( 6\sqrt{3} \approx 6 \cdot 1.732 = 10.392 \), thus:

\[
6\sqrt{3} - 10 \approx 10.392 - 10 = 0.392
\]

Since we are looking for the smallest constant \( C \) such that the inequality holds for all \( x, y, z \), we conclude that:

\[
C = 2
\]

Thus, the smallest constant \( C \) such that the inequality holds for all \( x, y, z \) satisfying \( x + y + z = xyz \) is:

\[
\boxed{2}
\]

The answer is \( C = 2 \).