## Problem

Find the largest constant $C$ such that for all real numbers $x, y, z$, the following inequality holds:
$$
\frac{x^2-y^2}{2 x^2+1}+\frac{y^2-z^2}{2 y^2+1}+\frac{z^2-x^2}{2 z^2+1} \geq C
$$

## Query

Task description: Please solve the problem with clear, rigorous, and logically sound steps. At the end of your response, state your answer in exactly this format: 'The answer is $C=X$', where X is your calculated numerical bound value. Example: 'The answer is $C=1$'.



Problem: Let $a, b, c$ be the side lengths, $h_{a}, h_{b}, h_{c}$ be the altitudes, respectively, and $r$ be the inradius of a triangle. Find the largest constant $C$ such that the following inequality holds for all triangles:
$$
\frac{1}{h_{a}-2 r}+\frac{1}{h_{b}-2 r}+\frac{1}{h_{c}-2 r} \geq C \cdot r
$$

Solution: By $\frac{1}{h_{a}}+\frac{1}{h_{b}}+\frac{1}{h_{c}}=\frac{1}{r}$ we obtain
$$
\frac{h_{a}-2 r}{h_{a}}+\frac{h_{b}-2 r}{h_{b}}+\frac{h_{c}-2 r}{h_{c}}=1
$$

Applying $A M \geq H M$ we get
$$
\left(\frac{h_{a}-2 r}{h_{a}}+\frac{h_{b}-2 r}{h_{b}}+\frac{h_{c}-2 r}{h_{c}}\right)\left(\frac{h_{a}}{h_{a}-2 r}+\frac{h_{b}}{h_{b}-2 r}+\frac{h_{c}}{h_{c}-2 r}\right) \geq 9
$$
i.e.
$$
\frac{h_{a}}{h_{a}-2 r}+\frac{h_{b}}{h_{b}-2 r}+\frac{h_{c}}{h_{c}-2 r} \geq 9
$$

Therefore
$$
\begin{aligned}
& \frac{2 r}{h_{a}-2 r}+\frac{2 r}{h_{b}-2 r}+\frac{2 r}{h_{c}-2 r} \\
& \quad=\frac{h_{a}-\left(h_{a}-2 r\right)}{h_{a}-2 r}+\frac{h_{b}-\left(h_{b}-2 r\right)}{h_{b}-2 r}+\frac{h_{c}-\left(h_{c}-2 r\right)}{h_{c}-2 r} \\
& \quad=\frac{h_{a}}{h_{a}-2 r}+\frac{h_{b}}{h_{b}-2 r}+\frac{h_{c}}{h_{c}-2 r}-3 \geq 9-3=6
\end{aligned}
$$
i.e.
$$
\frac{1}{h_{a}-2 r}+\frac{1}{h_{b}-2 r}+\frac{1}{h_{c}-2 r} \geq \frac{3}{r}
$$



Problem: Let $a, b, c$ be positive real numbers such that $a^2 + b^2 + c^2 = 3abc$. Find the largest constant $C$ such that the following inequality holds for all $a, b, c$ satisfying the given constraint:
$$
\frac{a}{b^2 c^2} + \frac{b}{c^2 a^2} + \frac{c}{a^2 b^2} \geq \frac{C}{a+b+c}
$$

Solution: The given inequality is equivalent to
$$
\left(a^{3}+b^{3}+c^{3}\right)(a+b+c) \geq 9 a^{2} b^{2} c^{2}
$$

Applying the Cauchy-Schwarz inequality we have
$$
\left(a^{3}+b^{3}+c^{3}\right)(a+b+c) \geq\left(a^{2}+b^{2}+c^{2}\right)^{2}
$$

Since $a^{2}+b^{2}+c^{2}=3 a b c$ we obtain
$$
\left(a^{3}+b^{3}+c^{3}\right)(a+b+c) \geq\left(a^{2}+b^{2}+c^{2}\right)^{2}=(3 a b c)^{2}=9 a^{2} b^{2} c^{2}
$$

Equality holds if and only if $a=b=c=1$.



Problem: Let $a, b, c$ be positive real numbers such that $a b c = 1$. Find the largest constant $C$ such that the following inequality holds for all $a, b, c$ satisfying the given constraint:
$$
\frac{b+c}{\sqrt{a}}+\frac{c+a}{\sqrt{b}}+\frac{a+b}{\sqrt{c}} \geq \sqrt{a}+\sqrt{b}+\sqrt{c}+C
$$

Solution: [Solution 1]
From the AM-GM Inequality, we have

$$
\begin{aligned}
& \frac{b+c}{\sqrt{a}}+\frac{c+a}{\sqrt{b}}+\frac{a+b}{\sqrt{c}} \geq 2\left(\sqrt{\frac{b c}{a}}+\sqrt{\frac{c a}{b}}+\sqrt{\frac{a b}{c}}\right)= \\
& =\left(\sqrt{\frac{b c}{a}}+\sqrt{\frac{c a}{b}}\right)+\left(\sqrt{\frac{c a}{b}}+\sqrt{\frac{a b}{c}}\right)+\left(\sqrt{\frac{a b}{c}}+\sqrt{\frac{b c}{a}}\right) \geq \\
& \geq 2(\sqrt{a}+\sqrt{b}+\sqrt{c}) \geq \sqrt{a}+\sqrt{b}+\sqrt{c}+3 \sqrt[6]{a b c}=\sqrt{a}+\sqrt{b}+\sqrt{c}+3 .
\end{aligned}
$$

Problem: Find the largest constant $C$ such that for all real numbers $x, y, z$, the following inequality holds:
$$
\frac{x^2-y^2}{2 x^2+1}+\frac{y^2-z^2}{2 y^2+1}+\frac{z^2-x^2}{2 z^2+1} \geq C
$$

Solution:

## Response

To solve the inequality 

\[
\frac{x^2-y^2}{2x^2+1} + \frac{y^2-z^2}{2y^2+1} + \frac{z^2-x^2}{2z^2+1} \geq C,
\]

we will analyze the left-hand side and find a suitable lower bound.

### Step 1: Simplifying the Terms

Each term in the sum can be rewritten as follows:

\[
\frac{x^2 - y^2}{2x^2 + 1} = \frac{(x-y)(x+y)}{2x^2 + 1}.
\]

This shows that the expression is dependent on the differences between the squares of the variables.

### Step 2: Analyzing the Expression

We can consider specific cases to find a lower bound for the entire expression. 

#### Case 1: Let \( x = y = z \)

If we set \( x = y = z = k \) for some real number \( k \), we have:

\[
\frac{k^2 - k^2}{2k^2 + 1} + \frac{k^2 - k^2}{2k^2 + 1} + \frac{k^2 - k^2}{2k^2 + 1} = 0.
\]

This indicates that the expression can equal zero when all variables are equal.

#### Case 2: Let \( x = 1, y = 0, z = 0 \)

Now, consider the case where \( x = 1 \), \( y = 0 \), and \( z = 0 \):

\[
\frac{1^2 - 0^2}{2 \cdot 1^2 + 1} + \frac{0^2 - 0^2}{2 \cdot 0^2 + 1} + \frac{0^2 - 1^2}{2 \cdot 0^2 + 1} = \frac{1}{3} + 0 - 1 = \frac{1}{3} - 1 = -\frac{2}{3}.
\]

This suggests that the expression can take negative values.

### Step 3: Finding the Minimum Value

To find the largest constant \( C \) such that the inequality holds for all \( x, y, z \), we need to determine the minimum value of the left-hand side expression. 

From the previous cases, we have seen that the expression can reach \( -\frac{2}{3} \). Therefore, we can conclude that:

\[
C \leq -\frac{2}{3}.
\]

### Step 4: Verifying if \( C = -\frac{2}{3} \) is Achievable

To check if \( C = -\frac{2}{3} \) is achievable, we can set \( x = 1, y = 0, z = 0 \) again, which gives us:

\[
\frac{1^2 - 0^2}{2 \cdot 1^2 + 1} + \frac{0^2 - 0^2}{2 \cdot 0^2 + 1} + \frac{0^2 - 1^2}{2 \cdot 0^2 + 1} = -\frac{2}{3}.
\]

Thus, the inequality holds with equality when \( C = -\frac{2}{3} \).

### Conclusion

The largest constant \( C \) such that the inequality holds for all real numbers \( x, y, z \) is 

\[
\boxed{-\frac{2}{3}}.
\]

Thus, we state the final answer in the required format:

The answer is \( C = -\frac{2}{3} \).