## Problem

Let $x, y, z > 0$ such that $x+y+z=1$. Determine the minimal constant $C$ such that the following inequality holds for all $x, y, z$:

$$
x y(y+4 z)+y z(z+4 x)+z x(x+4 y) \leq C.
$$

## Query

Task description: Please solve the problem with clear, rigorous, and logically sound steps. At the end of your response, state your answer in exactly this format: 'The answer is $C=X$', where X is your calculated numerical bound value. Example: 'The answer is $C=1$'.



Problem: Let $a, b, c$ be the side lengths, $h_{a}, h_{b}, h_{c}$ be the altitudes, respectively, and $r$ be the inradius of a triangle. Find the largest constant $C$ such that the following inequality holds for all triangles:
$$
\frac{1}{h_{a}-2 r}+\frac{1}{h_{b}-2 r}+\frac{1}{h_{c}-2 r} \geq C \cdot r
$$

Solution: By $\frac{1}{h_{a}}+\frac{1}{h_{b}}+\frac{1}{h_{c}}=\frac{1}{r}$ we obtain
$$
\frac{h_{a}-2 r}{h_{a}}+\frac{h_{b}-2 r}{h_{b}}+\frac{h_{c}-2 r}{h_{c}}=1
$$

Applying $A M \geq H M$ we get
$$
\left(\frac{h_{a}-2 r}{h_{a}}+\frac{h_{b}-2 r}{h_{b}}+\frac{h_{c}-2 r}{h_{c}}\right)\left(\frac{h_{a}}{h_{a}-2 r}+\frac{h_{b}}{h_{b}-2 r}+\frac{h_{c}}{h_{c}-2 r}\right) \geq 9
$$
i.e.
$$
\frac{h_{a}}{h_{a}-2 r}+\frac{h_{b}}{h_{b}-2 r}+\frac{h_{c}}{h_{c}-2 r} \geq 9
$$

Therefore
$$
\begin{aligned}
& \frac{2 r}{h_{a}-2 r}+\frac{2 r}{h_{b}-2 r}+\frac{2 r}{h_{c}-2 r} \\
& \quad=\frac{h_{a}-\left(h_{a}-2 r\right)}{h_{a}-2 r}+\frac{h_{b}-\left(h_{b}-2 r\right)}{h_{b}-2 r}+\frac{h_{c}-\left(h_{c}-2 r\right)}{h_{c}-2 r} \\
& \quad=\frac{h_{a}}{h_{a}-2 r}+\frac{h_{b}}{h_{b}-2 r}+\frac{h_{c}}{h_{c}-2 r}-3 \geq 9-3=6
\end{aligned}
$$
i.e.
$$
\frac{1}{h_{a}-2 r}+\frac{1}{h_{b}-2 r}+\frac{1}{h_{c}-2 r} \geq \frac{3}{r}
$$



Problem: Let $a, b, c$ be positive real numbers such that $a^2 + b^2 + c^2 = 3abc$. Find the largest constant $C$ such that the following inequality holds for all $a, b, c$ satisfying the given constraint:
$$
\frac{a}{b^2 c^2} + \frac{b}{c^2 a^2} + \frac{c}{a^2 b^2} \geq \frac{C}{a+b+c}
$$

Solution: The given inequality is equivalent to
$$
\left(a^{3}+b^{3}+c^{3}\right)(a+b+c) \geq 9 a^{2} b^{2} c^{2}
$$

Applying the Cauchy-Schwarz inequality we have
$$
\left(a^{3}+b^{3}+c^{3}\right)(a+b+c) \geq\left(a^{2}+b^{2}+c^{2}\right)^{2}
$$

Since $a^{2}+b^{2}+c^{2}=3 a b c$ we obtain
$$
\left(a^{3}+b^{3}+c^{3}\right)(a+b+c) \geq\left(a^{2}+b^{2}+c^{2}\right)^{2}=(3 a b c)^{2}=9 a^{2} b^{2} c^{2}
$$

Equality holds if and only if $a=b=c=1$.



Problem: Let $a, b, c$ be positive real numbers such that $a b c = 1$. Find the largest constant $C$ such that the following inequality holds for all $a, b, c$ satisfying the given constraint:
$$
\frac{b+c}{\sqrt{a}}+\frac{c+a}{\sqrt{b}}+\frac{a+b}{\sqrt{c}} \geq \sqrt{a}+\sqrt{b}+\sqrt{c}+C
$$

Solution: [Solution 1]
From the AM-GM Inequality, we have

$$
\begin{aligned}
& \frac{b+c}{\sqrt{a}}+\frac{c+a}{\sqrt{b}}+\frac{a+b}{\sqrt{c}} \geq 2\left(\sqrt{\frac{b c}{a}}+\sqrt{\frac{c a}{b}}+\sqrt{\frac{a b}{c}}\right)= \\
& =\left(\sqrt{\frac{b c}{a}}+\sqrt{\frac{c a}{b}}\right)+\left(\sqrt{\frac{c a}{b}}+\sqrt{\frac{a b}{c}}\right)+\left(\sqrt{\frac{a b}{c}}+\sqrt{\frac{b c}{a}}\right) \geq \\
& \geq 2(\sqrt{a}+\sqrt{b}+\sqrt{c}) \geq \sqrt{a}+\sqrt{b}+\sqrt{c}+3 \sqrt[6]{a b c}=\sqrt{a}+\sqrt{b}+\sqrt{c}+3 .
\end{aligned}
$$

Problem: Let $x, y, z > 0$ such that $x+y+z=1$. Determine the minimal constant $C$ such that the following inequality holds for all $x, y, z$:

$$
x y(y+4 z)+y z(z+4 x)+z x(x+4 y) \leq C.
$$

Solution:

## Response

To solve the problem, we need to analyze the expression given in the inequality:

\[
xy(y + 4z) + yz(z + 4x) + zx(x + 4y).
\]

We can expand this expression:

\[
xy^2 + 4xyz + y^2z + 4xyz + zx^2 + 4xyz = xy^2 + yz^2 + zx^2 + 12xyz.
\]

Now, we want to find the maximum value of this expression under the constraint \(x + y + z = 1\) with \(x, y, z > 0\).

### Step 1: Use Symmetry and Substitution

Since the expression is symmetric in \(x, y, z\), we can assume without loss of generality that \(x \leq y \leq z\). We can also use the method of Lagrange multipliers or test specific cases to find the maximum.

### Step 2: Test Specific Cases

1. **Case 1: \(x = y = z = \frac{1}{3}\)**

   Substituting \(x = y = z = \frac{1}{3}\):

   \[
   xy(y + 4z) = \left(\frac{1}{3}\right)\left(\frac{1}{3}\right)\left(\frac{1}{3} + 4 \cdot \frac{1}{3}\right) = \frac{1}{9} \cdot \frac{5}{3} = \frac{5}{27}.
   \]

   Similarly, for the other terms:

   \[
   yz(z + 4x) = \frac{5}{27}, \quad zx(x + 4y) = \frac{5}{27}.
   \]

   Therefore, the total is:

   \[
   3 \cdot \frac{5}{27} = \frac{15}{27} = \frac{5}{9}.
   \]

2. **Case 2: \(x = 1, y = 0, z = 0\)**

   In this case, the expression evaluates to:

   \[
   0 \cdot 0 + 0 \cdot 0 + 0 \cdot 0 = 0.
   \]

3. **Case 3: \(x = \frac{1}{2}, y = \frac{1}{2}, z = 0\)**

   The expression evaluates to:

   \[
   \frac{1}{2} \cdot \frac{1}{2} \cdot (0 + 4 \cdot 0) + 0 + 0 = 0.
   \]

### Step 3: Conclusion

From the cases tested, the maximum value occurs when \(x = y = z = \frac{1}{3}\), yielding:

\[
xy(y + 4z) + yz(z + 4x) + zx(x + 4y) \leq \frac{5}{9}.
\]

Thus, the largest constant \(C\) such that the inequality holds for all \(x, y, z > 0\) with \(x + y + z = 1\) is:

\[
\boxed{\frac{5}{9}}.
\]

Therefore, the answer is \(C = \frac{5}{9}\). 

The answer is \(C = \frac{5}{9}\).