## Problem

Let $a, b, c > 0$ such that $a+b+c=1$. Determine the maximal constant $C$ such that the following inequality holds for all $a, b, c$:

$$
\frac{1+a+b}{2+c}+\frac{1+b+c}{2+a}+\frac{1+c+a}{2+b} \geq C.
$$

## Query

Task description: Please solve the problem with clear, rigorous, and logically sound steps. At the end of your response, state your answer in exactly this format: 'The answer is $C=X$', where X is your calculated numerical bound value. Example: 'The answer is $C=1$'.



Problem: Let $a, b, c$ be the side lengths, $h_{a}, h_{b}, h_{c}$ be the altitudes, respectively, and $r$ be the inradius of a triangle. Find the largest constant $C$ such that the following inequality holds for all triangles:
$$
\frac{1}{h_{a}-2 r}+\frac{1}{h_{b}-2 r}+\frac{1}{h_{c}-2 r} \geq C \cdot r
$$

Solution: By $\frac{1}{h_{a}}+\frac{1}{h_{b}}+\frac{1}{h_{c}}=\frac{1}{r}$ we obtain
$$
\frac{h_{a}-2 r}{h_{a}}+\frac{h_{b}-2 r}{h_{b}}+\frac{h_{c}-2 r}{h_{c}}=1
$$

Applying $A M \geq H M$ we get
$$
\left(\frac{h_{a}-2 r}{h_{a}}+\frac{h_{b}-2 r}{h_{b}}+\frac{h_{c}-2 r}{h_{c}}\right)\left(\frac{h_{a}}{h_{a}-2 r}+\frac{h_{b}}{h_{b}-2 r}+\frac{h_{c}}{h_{c}-2 r}\right) \geq 9
$$
i.e.
$$
\frac{h_{a}}{h_{a}-2 r}+\frac{h_{b}}{h_{b}-2 r}+\frac{h_{c}}{h_{c}-2 r} \geq 9
$$

Therefore
$$
\begin{aligned}
& \frac{2 r}{h_{a}-2 r}+\frac{2 r}{h_{b}-2 r}+\frac{2 r}{h_{c}-2 r} \\
& \quad=\frac{h_{a}-\left(h_{a}-2 r\right)}{h_{a}-2 r}+\frac{h_{b}-\left(h_{b}-2 r\right)}{h_{b}-2 r}+\frac{h_{c}-\left(h_{c}-2 r\right)}{h_{c}-2 r} \\
& \quad=\frac{h_{a}}{h_{a}-2 r}+\frac{h_{b}}{h_{b}-2 r}+\frac{h_{c}}{h_{c}-2 r}-3 \geq 9-3=6
\end{aligned}
$$
i.e.
$$
\frac{1}{h_{a}-2 r}+\frac{1}{h_{b}-2 r}+\frac{1}{h_{c}-2 r} \geq \frac{3}{r}
$$



Problem: Let $a, b, c$ be positive real numbers such that $a^2 + b^2 + c^2 = 3abc$. Find the largest constant $C$ such that the following inequality holds for all $a, b, c$ satisfying the given constraint:
$$
\frac{a}{b^2 c^2} + \frac{b}{c^2 a^2} + \frac{c}{a^2 b^2} \geq \frac{C}{a+b+c}
$$

Solution: The given inequality is equivalent to
$$
\left(a^{3}+b^{3}+c^{3}\right)(a+b+c) \geq 9 a^{2} b^{2} c^{2}
$$

Applying the Cauchy-Schwarz inequality we have
$$
\left(a^{3}+b^{3}+c^{3}\right)(a+b+c) \geq\left(a^{2}+b^{2}+c^{2}\right)^{2}
$$

Since $a^{2}+b^{2}+c^{2}=3 a b c$ we obtain
$$
\left(a^{3}+b^{3}+c^{3}\right)(a+b+c) \geq\left(a^{2}+b^{2}+c^{2}\right)^{2}=(3 a b c)^{2}=9 a^{2} b^{2} c^{2}
$$

Equality holds if and only if $a=b=c=1$.



Problem: Let $a, b, c$ be positive real numbers such that $a b c = 1$. Find the largest constant $C$ such that the following inequality holds for all $a, b, c$ satisfying the given constraint:
$$
\frac{b+c}{\sqrt{a}}+\frac{c+a}{\sqrt{b}}+\frac{a+b}{\sqrt{c}} \geq \sqrt{a}+\sqrt{b}+\sqrt{c}+C
$$

Solution: [Solution 1]
From the AM-GM Inequality, we have

$$
\begin{aligned}
& \frac{b+c}{\sqrt{a}}+\frac{c+a}{\sqrt{b}}+\frac{a+b}{\sqrt{c}} \geq 2\left(\sqrt{\frac{b c}{a}}+\sqrt{\frac{c a}{b}}+\sqrt{\frac{a b}{c}}\right)= \\
& =\left(\sqrt{\frac{b c}{a}}+\sqrt{\frac{c a}{b}}\right)+\left(\sqrt{\frac{c a}{b}}+\sqrt{\frac{a b}{c}}\right)+\left(\sqrt{\frac{a b}{c}}+\sqrt{\frac{b c}{a}}\right) \geq \\
& \geq 2(\sqrt{a}+\sqrt{b}+\sqrt{c}) \geq \sqrt{a}+\sqrt{b}+\sqrt{c}+3 \sqrt[6]{a b c}=\sqrt{a}+\sqrt{b}+\sqrt{c}+3 .
\end{aligned}
$$

Problem: Let $a, b, c > 0$ such that $a+b+c=1$. Determine the maximal constant $C$ such that the following inequality holds for all $a, b, c$:

$$
\frac{1+a+b}{2+c}+\frac{1+b+c}{2+a}+\frac{1+c+a}{2+b} \geq C.
$$

Solution:

## Response

To solve the problem, we start with the given inequality:

\[
\frac{1+a+b}{2+c}+\frac{1+b+c}{2+a}+\frac{1+c+a}{2+b} \geq C.
\]

Given that \( a + b + c = 1 \), we can express \( c \) in terms of \( a \) and \( b \):

\[
c = 1 - a - b.
\]

Substituting this into the inequality, we rewrite each term:

1. The first term becomes:
   \[
   \frac{1 + a + b}{2 + (1 - a - b)} = \frac{1 + a + b}{2 + 1 - a - b} = \frac{1 + a + b}{3 - a - b}.
   \]

2. The second term becomes:
   \[
   \frac{1 + b + (1 - a - b)}{2 + a} = \frac{2 - a}{2 + a}.
   \]

3. The third term becomes:
   \[
   \frac{1 + (1 - a - b) + a}{2 + b} = \frac{2 - b}{2 + b}.
   \]

Thus, we can rewrite the entire expression as:

\[
\frac{1 + a + b}{3 - a - b} + \frac{2 - a}{2 + a} + \frac{2 - b}{2 + b}.
\]

Next, we simplify the first term:

\[
\frac{1 + a + b}{3 - a - b} = \frac{1 + (1 - c)}{3 - (1 - c)} = \frac{2 - c}{2 + c}.
\]

Now, we have:

\[
\frac{2 - c}{2 + c} + \frac{2 - a}{2 + a} + \frac{2 - b}{2 + b}.
\]

To find the maximum constant \( C \), we will analyze the behavior of the left-hand side as \( a, b, c \) vary under the constraint \( a + b + c = 1 \).

### Step 1: Test Equal Values

Letâ€™s test the case where \( a = b = c = \frac{1}{3} \):

\[
\frac{2 - \frac{1}{3}}{2 + \frac{1}{3}} + \frac{2 - \frac{1}{3}}{2 + \frac{1}{3}} + \frac{2 - \frac{1}{3}}{2 + \frac{1}{3}} = 3 \cdot \frac{\frac{5}{3}}{\frac{7}{3}} = 3 \cdot \frac{5}{7} = \frac{15}{7}.
\]

### Step 2: Check Other Cases

Next, we check the case where one variable approaches 1 and the others approach 0. For example, let \( a = 1 \) and \( b = c = 0 \):

\[
\frac{1 + 1 + 0}{2 + 0} + \frac{1 + 0 + 0}{2 + 1} + \frac{1 + 0 + 0}{2 + 0} = \frac{2}{2} + \frac{1}{2} + \frac{1}{2} = 1 + \frac{1}{2} + \frac{1}{2} = 2.
\]

### Step 3: Conclusion

From our tests, we see that the minimum value of the left-hand side occurs when \( a = b = c = \frac{1}{3} \), yielding \( \frac{15}{7} \approx 2.14 \). The maximum value occurs when one variable is 1 and the others are 0, yielding 2.

Thus, the largest constant \( C \) such that the inequality holds for all \( a, b, c > 0 \) with \( a + b + c = 1 \) is:

\[
C = 2.
\]

Therefore, the final answer is:

\[
\text{The answer is } C=2.
\]