## Problem

Given $a, b, c > 0$ such that $ab + bc + ca = abc$, find the smallest constant $C$ such that the following inequality holds for all $a, b, c$:
$$
\frac{1}{a+3b+2c} + \frac{1}{b+3c+2a} + \frac{1}{c+3a+2b} \leq C.
$$

## Query

Task description: Please solve the problem with clear, rigorous, and logically sound steps. At the end of your response, state your answer in exactly this format: 'The answer is $C=X$', where X is your calculated numerical bound value. Example: 'The answer is $C=1$'.



Problem: Let $a, b, c$ be the side lengths, $h_{a}, h_{b}, h_{c}$ be the altitudes, respectively, and $r$ be the inradius of a triangle. Find the largest constant $C$ such that the following inequality holds for all triangles:
$$
\frac{1}{h_{a}-2 r}+\frac{1}{h_{b}-2 r}+\frac{1}{h_{c}-2 r} \geq C \cdot r
$$

Solution: By $\frac{1}{h_{a}}+\frac{1}{h_{b}}+\frac{1}{h_{c}}=\frac{1}{r}$ we obtain
$$
\frac{h_{a}-2 r}{h_{a}}+\frac{h_{b}-2 r}{h_{b}}+\frac{h_{c}-2 r}{h_{c}}=1
$$

Applying $A M \geq H M$ we get
$$
\left(\frac{h_{a}-2 r}{h_{a}}+\frac{h_{b}-2 r}{h_{b}}+\frac{h_{c}-2 r}{h_{c}}\right)\left(\frac{h_{a}}{h_{a}-2 r}+\frac{h_{b}}{h_{b}-2 r}+\frac{h_{c}}{h_{c}-2 r}\right) \geq 9
$$
i.e.
$$
\frac{h_{a}}{h_{a}-2 r}+\frac{h_{b}}{h_{b}-2 r}+\frac{h_{c}}{h_{c}-2 r} \geq 9
$$

Therefore
$$
\begin{aligned}
& \frac{2 r}{h_{a}-2 r}+\frac{2 r}{h_{b}-2 r}+\frac{2 r}{h_{c}-2 r} \\
& \quad=\frac{h_{a}-\left(h_{a}-2 r\right)}{h_{a}-2 r}+\frac{h_{b}-\left(h_{b}-2 r\right)}{h_{b}-2 r}+\frac{h_{c}-\left(h_{c}-2 r\right)}{h_{c}-2 r} \\
& \quad=\frac{h_{a}}{h_{a}-2 r}+\frac{h_{b}}{h_{b}-2 r}+\frac{h_{c}}{h_{c}-2 r}-3 \geq 9-3=6
\end{aligned}
$$
i.e.
$$
\frac{1}{h_{a}-2 r}+\frac{1}{h_{b}-2 r}+\frac{1}{h_{c}-2 r} \geq \frac{3}{r}
$$



Problem: Let $a, b, c$ be positive real numbers such that $a^2 + b^2 + c^2 = 3abc$. Find the largest constant $C$ such that the following inequality holds for all $a, b, c$ satisfying the given constraint:
$$
\frac{a}{b^2 c^2} + \frac{b}{c^2 a^2} + \frac{c}{a^2 b^2} \geq \frac{C}{a+b+c}
$$

Solution: The given inequality is equivalent to
$$
\left(a^{3}+b^{3}+c^{3}\right)(a+b+c) \geq 9 a^{2} b^{2} c^{2}
$$

Applying the Cauchy-Schwarz inequality we have
$$
\left(a^{3}+b^{3}+c^{3}\right)(a+b+c) \geq\left(a^{2}+b^{2}+c^{2}\right)^{2}
$$

Since $a^{2}+b^{2}+c^{2}=3 a b c$ we obtain
$$
\left(a^{3}+b^{3}+c^{3}\right)(a+b+c) \geq\left(a^{2}+b^{2}+c^{2}\right)^{2}=(3 a b c)^{2}=9 a^{2} b^{2} c^{2}
$$

Equality holds if and only if $a=b=c=1$.



Problem: Let $a, b, c$ be positive real numbers such that $a b c = 1$. Find the largest constant $C$ such that the following inequality holds for all $a, b, c$ satisfying the given constraint:
$$
\frac{b+c}{\sqrt{a}}+\frac{c+a}{\sqrt{b}}+\frac{a+b}{\sqrt{c}} \geq \sqrt{a}+\sqrt{b}+\sqrt{c}+C
$$

Solution: [Solution 1]
From the AM-GM Inequality, we have

$$
\begin{aligned}
& \frac{b+c}{\sqrt{a}}+\frac{c+a}{\sqrt{b}}+\frac{a+b}{\sqrt{c}} \geq 2\left(\sqrt{\frac{b c}{a}}+\sqrt{\frac{c a}{b}}+\sqrt{\frac{a b}{c}}\right)= \\
& =\left(\sqrt{\frac{b c}{a}}+\sqrt{\frac{c a}{b}}\right)+\left(\sqrt{\frac{c a}{b}}+\sqrt{\frac{a b}{c}}\right)+\left(\sqrt{\frac{a b}{c}}+\sqrt{\frac{b c}{a}}\right) \geq \\
& \geq 2(\sqrt{a}+\sqrt{b}+\sqrt{c}) \geq \sqrt{a}+\sqrt{b}+\sqrt{c}+3 \sqrt[6]{a b c}=\sqrt{a}+\sqrt{b}+\sqrt{c}+3 .
\end{aligned}
$$

Problem: Given $a, b, c > 0$ such that $ab + bc + ca = abc$, find the smallest constant $C$ such that the following inequality holds for all $a, b, c$:
$$
\frac{1}{a+3b+2c} + \frac{1}{b+3c+2a} + \frac{1}{c+3a+2b} \leq C.
$$

Solution:

## Response

To solve the problem, we start with the given condition \( ab + bc + ca = abc \). We want to find the smallest constant \( C \) such that the following inequality holds for all positive \( a, b, c \):

\[
\frac{1}{a+3b+2c} + \frac{1}{b+3c+2a} + \frac{1}{c+3a+2b} \leq C.
\]

### Step 1: Analyze the condition

From the condition \( ab + bc + ca = abc \), we can rearrange it to:

\[
abc - ab - ac - bc = 0.
\]

This suggests that \( a, b, c \) are related in a way that can be expressed in terms of their products and sums.

### Step 2: Use substitutions

To simplify our analysis, we can use the substitutions \( a = \frac{x}{y}, b = \frac{y}{z}, c = \frac{z}{x} \) for positive \( x, y, z \). This substitution maintains the positivity of \( a, b, c \) and allows us to express the condition in terms of \( x, y, z \).

### Step 3: Rewrite the inequality

We rewrite the left-hand side of the inequality:

\[
\frac{1}{\frac{x}{y} + 3\frac{y}{z} + 2\frac{z}{x}} + \frac{1}{\frac{y}{z} + 3\frac{z}{x} + 2\frac{x}{y}} + \frac{1}{\frac{z}{x} + 3\frac{x}{y} + 2\frac{y}{z}}.
\]

### Step 4: Analyze the terms

Each term in the sum can be analyzed separately. For example, consider the first term:

\[
\frac{1}{\frac{x}{y} + 3\frac{y}{z} + 2\frac{z}{x}}.
\]

To find a common denominator, we can multiply through by \( xyz \):

\[
\frac{xyz}{x^2z + 3y^2x + 2y^2z}.
\]

### Step 5: Find bounds

To find the upper bound for the entire expression, we can apply the Cauchy-Schwarz inequality:

\[
\left( \frac{1}{a+3b+2c} + \frac{1}{b+3c+2a} + \frac{1}{c+3a+2b} \right) \left( (a+3b+2c) + (b+3c+2a) + (c+3a+2b) \right) \geq 9.
\]

Calculating the sum \( (a+3b+2c) + (b+3c+2a) + (c+3a+2b) \):

\[
= 6(a + b + c).
\]

Thus, we have:

\[
\left( \frac{1}{a+3b+2c} + \frac{1}{b+3c+2a} + \frac{1}{c+3a+2b} \right) \cdot 6(a + b + c) \geq 9.
\]

This implies:

\[
\frac{1}{a+3b+2c} + \frac{1}{b+3c+2a} + \frac{1}{c+3a+2b} \geq \frac{9}{6(a+b+c)} = \frac{3}{2(a+b+c)}.
\]

### Step 6: Find the constant \( C \)

To find the smallest constant \( C \), we need to analyze the maximum value of \( a + b + c \) under the constraint \( ab + ac + bc = abc \). 

By testing specific values, such as \( a = b = c = 3 \), we find:

\[
\frac{1}{3 + 9 + 6} = \frac{1}{18}.
\]

Thus, we can conclude that the maximum value of the left-hand side is bounded by \( \frac{3}{2} \).

### Conclusion

After analyzing the inequality and the conditions, we find that the smallest constant \( C \) such that the inequality holds for all positive \( a, b, c \) satisfying \( ab + ac + bc = abc \) is:

\[
\boxed{1}.
\]

Thus, the final answer is:

The answer is \( C=1 \).