## Problem

Let $n$ be a natural number such that $n \geq 2$. Find the largest constant $C$ such that the following inequality holds for all $n$:
$$
\frac{1}{n+1}\left(1+\frac{1}{3}+\cdots+\frac{1}{2n-1}\right) \geq C \cdot \frac{1}{n}\left(1+\frac{1}{2}+\cdots+\frac{1}{n}\right).
$$

## Query

Task description: Please solve the problem with clear, rigorous, and logically sound steps. At the end of your response, state your answer in exactly this format: 'The answer is $C=X$', where X is your calculated numerical bound value. Example: 'The answer is $C=1$'.



Problem: Let $a, b, c$ be the side lengths, $h_{a}, h_{b}, h_{c}$ be the altitudes, respectively, and $r$ be the inradius of a triangle. Find the largest constant $C$ such that the following inequality holds for all triangles:
$$
\frac{1}{h_{a}-2 r}+\frac{1}{h_{b}-2 r}+\frac{1}{h_{c}-2 r} \geq C \cdot r
$$

Solution: By $\frac{1}{h_{a}}+\frac{1}{h_{b}}+\frac{1}{h_{c}}=\frac{1}{r}$ we obtain
$$
\frac{h_{a}-2 r}{h_{a}}+\frac{h_{b}-2 r}{h_{b}}+\frac{h_{c}-2 r}{h_{c}}=1
$$

Applying $A M \geq H M$ we get
$$
\left(\frac{h_{a}-2 r}{h_{a}}+\frac{h_{b}-2 r}{h_{b}}+\frac{h_{c}-2 r}{h_{c}}\right)\left(\frac{h_{a}}{h_{a}-2 r}+\frac{h_{b}}{h_{b}-2 r}+\frac{h_{c}}{h_{c}-2 r}\right) \geq 9
$$
i.e.
$$
\frac{h_{a}}{h_{a}-2 r}+\frac{h_{b}}{h_{b}-2 r}+\frac{h_{c}}{h_{c}-2 r} \geq 9
$$

Therefore
$$
\begin{aligned}
& \frac{2 r}{h_{a}-2 r}+\frac{2 r}{h_{b}-2 r}+\frac{2 r}{h_{c}-2 r} \\
& \quad=\frac{h_{a}-\left(h_{a}-2 r\right)}{h_{a}-2 r}+\frac{h_{b}-\left(h_{b}-2 r\right)}{h_{b}-2 r}+\frac{h_{c}-\left(h_{c}-2 r\right)}{h_{c}-2 r} \\
& \quad=\frac{h_{a}}{h_{a}-2 r}+\frac{h_{b}}{h_{b}-2 r}+\frac{h_{c}}{h_{c}-2 r}-3 \geq 9-3=6
\end{aligned}
$$
i.e.
$$
\frac{1}{h_{a}-2 r}+\frac{1}{h_{b}-2 r}+\frac{1}{h_{c}-2 r} \geq \frac{3}{r}
$$



Problem: Let $a, b, c$ be positive real numbers such that $a^2 + b^2 + c^2 = 3abc$. Find the largest constant $C$ such that the following inequality holds for all $a, b, c$ satisfying the given constraint:
$$
\frac{a}{b^2 c^2} + \frac{b}{c^2 a^2} + \frac{c}{a^2 b^2} \geq \frac{C}{a+b+c}
$$

Solution: The given inequality is equivalent to
$$
\left(a^{3}+b^{3}+c^{3}\right)(a+b+c) \geq 9 a^{2} b^{2} c^{2}
$$

Applying the Cauchy-Schwarz inequality we have
$$
\left(a^{3}+b^{3}+c^{3}\right)(a+b+c) \geq\left(a^{2}+b^{2}+c^{2}\right)^{2}
$$

Since $a^{2}+b^{2}+c^{2}=3 a b c$ we obtain
$$
\left(a^{3}+b^{3}+c^{3}\right)(a+b+c) \geq\left(a^{2}+b^{2}+c^{2}\right)^{2}=(3 a b c)^{2}=9 a^{2} b^{2} c^{2}
$$

Equality holds if and only if $a=b=c=1$.



Problem: Let $a, b, c$ be positive real numbers such that $a b c = 1$. Find the largest constant $C$ such that the following inequality holds for all $a, b, c$ satisfying the given constraint:
$$
\frac{b+c}{\sqrt{a}}+\frac{c+a}{\sqrt{b}}+\frac{a+b}{\sqrt{c}} \geq \sqrt{a}+\sqrt{b}+\sqrt{c}+C
$$

Solution: [Solution 1]
From the AM-GM Inequality, we have

$$
\begin{aligned}
& \frac{b+c}{\sqrt{a}}+\frac{c+a}{\sqrt{b}}+\frac{a+b}{\sqrt{c}} \geq 2\left(\sqrt{\frac{b c}{a}}+\sqrt{\frac{c a}{b}}+\sqrt{\frac{a b}{c}}\right)= \\
& =\left(\sqrt{\frac{b c}{a}}+\sqrt{\frac{c a}{b}}\right)+\left(\sqrt{\frac{c a}{b}}+\sqrt{\frac{a b}{c}}\right)+\left(\sqrt{\frac{a b}{c}}+\sqrt{\frac{b c}{a}}\right) \geq \\
& \geq 2(\sqrt{a}+\sqrt{b}+\sqrt{c}) \geq \sqrt{a}+\sqrt{b}+\sqrt{c}+3 \sqrt[6]{a b c}=\sqrt{a}+\sqrt{b}+\sqrt{c}+3 .
\end{aligned}
$$

Problem: Let $n$ be a natural number such that $n \geq 2$. Find the largest constant $C$ such that the following inequality holds for all $n$:
$$
\frac{1}{n+1}\left(1+\frac{1}{3}+\cdots+\frac{1}{2n-1}\right) \geq C \cdot \frac{1}{n}\left(1+\frac{1}{2}+\cdots+\frac{1}{n}\right).
$$

Solution:

## Response

To solve the problem, we need to analyze the inequality given:

\[
\frac{1}{n+1}\left(1+\frac{1}{3}+\cdots+\frac{1}{2n-1}\right) \geq C \cdot \frac{1}{n}\left(1+\frac{1}{2}+\cdots+\frac{1}{n}\right).
\]

### Step 1: Simplifying the Left Side

The left side can be expressed as:

\[
\frac{1}{n+1} \sum_{k=1}^{n} \frac{1}{2k-1}.
\]

The sum \( \sum_{k=1}^{n} \frac{1}{2k-1} \) is the sum of the first \( n \) odd reciprocals. This can be approximated using the harmonic series:

\[
\sum_{k=1}^{n} \frac{1}{2k-1} \approx \frac{1}{2} \ln(n) + \frac{1}{2} \text{ (as } n \to \infty\text{)}.
\]

### Step 2: Simplifying the Right Side

The right side can be expressed as:

\[
C \cdot \frac{1}{n} \sum_{k=1}^{n} \frac{1}{k}.
\]

The sum \( \sum_{k=1}^{n} \frac{1}{k} \) is the \( n \)-th harmonic number, which can be approximated as:

\[
\sum_{k=1}^{n} \frac{1}{k} \approx \ln(n) + \gamma \text{ (where } \gamma \text{ is the Euler-Mascheroni constant)}.
\]

### Step 3: Setting Up the Inequality

Now we can rewrite the inequality as:

\[
\frac{1}{n+1} \left( \sum_{k=1}^{n} \frac{1}{2k-1} \right) \geq C \cdot \frac{1}{n} \left( \sum_{k=1}^{n} \frac{1}{k} \right).
\]

Substituting the approximations, we have:

\[
\frac{1}{n+1} \left( \frac{1}{2} \ln(n) + \frac{1}{2} \right) \geq C \cdot \frac{1}{n} \left( \ln(n) + \gamma \right).
\]

### Step 4: Analyzing the Limit as \( n \to \infty \)

As \( n \to \infty \), we can focus on the leading terms:

\[
\frac{1}{n+1} \cdot \frac{1}{2} \ln(n) \geq C \cdot \frac{1}{n} \ln(n).
\]

Dividing both sides by \( \ln(n) \) (valid for large \( n \)) gives:

\[
\frac{1}{2(n+1)} \geq \frac{C}{n}.
\]

### Step 5: Finding the Constant \( C \)

Rearranging gives:

\[
C \leq \frac{n+1}{2}.
\]

Taking the limit as \( n \to \infty \), we find that \( C \) can be at most \( \frac{1}{2} \).

### Conclusion

Thus, the largest constant \( C \) such that the inequality holds for all \( n \geq 2 \) is:

\[
\boxed{C = \frac{1}{2}}.
\]

The answer is \( C = \frac{1}{2} \).