## Problem

Let $a, b, c$ be the side lengths of a triangle. Determine the largest constant $C$ such that the following inequality holds for all $a, b, c$ satisfying the triangle inequality:
$$
\frac{b+c}{a}+\frac{c+a}{b}+\frac{a+b}{c}+\frac{(b+c-a)(c+a-b)(a+b-c)}{a b c} \geq C.
$$

## Query

Task description: Please solve the problem with clear, rigorous, and logically sound steps. At the end of your response, state your answer in exactly this format: 'The answer is $C=X$', where X is your calculated numerical bound value. Example: 'The answer is $C=1$'.



Problem: Let $a, b, c$ be the side lengths, $h_{a}, h_{b}, h_{c}$ be the altitudes, respectively, and $r$ be the inradius of a triangle. Find the largest constant $C$ such that the following inequality holds for all triangles:
$$
\frac{1}{h_{a}-2 r}+\frac{1}{h_{b}-2 r}+\frac{1}{h_{c}-2 r} \geq C \cdot r
$$

Solution: By $\frac{1}{h_{a}}+\frac{1}{h_{b}}+\frac{1}{h_{c}}=\frac{1}{r}$ we obtain
$$
\frac{h_{a}-2 r}{h_{a}}+\frac{h_{b}-2 r}{h_{b}}+\frac{h_{c}-2 r}{h_{c}}=1
$$

Applying $A M \geq H M$ we get
$$
\left(\frac{h_{a}-2 r}{h_{a}}+\frac{h_{b}-2 r}{h_{b}}+\frac{h_{c}-2 r}{h_{c}}\right)\left(\frac{h_{a}}{h_{a}-2 r}+\frac{h_{b}}{h_{b}-2 r}+\frac{h_{c}}{h_{c}-2 r}\right) \geq 9
$$
i.e.
$$
\frac{h_{a}}{h_{a}-2 r}+\frac{h_{b}}{h_{b}-2 r}+\frac{h_{c}}{h_{c}-2 r} \geq 9
$$

Therefore
$$
\begin{aligned}
& \frac{2 r}{h_{a}-2 r}+\frac{2 r}{h_{b}-2 r}+\frac{2 r}{h_{c}-2 r} \\
& \quad=\frac{h_{a}-\left(h_{a}-2 r\right)}{h_{a}-2 r}+\frac{h_{b}-\left(h_{b}-2 r\right)}{h_{b}-2 r}+\frac{h_{c}-\left(h_{c}-2 r\right)}{h_{c}-2 r} \\
& \quad=\frac{h_{a}}{h_{a}-2 r}+\frac{h_{b}}{h_{b}-2 r}+\frac{h_{c}}{h_{c}-2 r}-3 \geq 9-3=6
\end{aligned}
$$
i.e.
$$
\frac{1}{h_{a}-2 r}+\frac{1}{h_{b}-2 r}+\frac{1}{h_{c}-2 r} \geq \frac{3}{r}
$$



Problem: Let $a, b, c$ be positive real numbers such that $a^2 + b^2 + c^2 = 3abc$. Find the largest constant $C$ such that the following inequality holds for all $a, b, c$ satisfying the given constraint:
$$
\frac{a}{b^2 c^2} + \frac{b}{c^2 a^2} + \frac{c}{a^2 b^2} \geq \frac{C}{a+b+c}
$$

Solution: The given inequality is equivalent to
$$
\left(a^{3}+b^{3}+c^{3}\right)(a+b+c) \geq 9 a^{2} b^{2} c^{2}
$$

Applying the Cauchy-Schwarz inequality we have
$$
\left(a^{3}+b^{3}+c^{3}\right)(a+b+c) \geq\left(a^{2}+b^{2}+c^{2}\right)^{2}
$$

Since $a^{2}+b^{2}+c^{2}=3 a b c$ we obtain
$$
\left(a^{3}+b^{3}+c^{3}\right)(a+b+c) \geq\left(a^{2}+b^{2}+c^{2}\right)^{2}=(3 a b c)^{2}=9 a^{2} b^{2} c^{2}
$$

Equality holds if and only if $a=b=c=1$.



Problem: Let $a, b, c$ be positive real numbers such that $a b c = 1$. Find the largest constant $C$ such that the following inequality holds for all $a, b, c$ satisfying the given constraint:
$$
\frac{b+c}{\sqrt{a}}+\frac{c+a}{\sqrt{b}}+\frac{a+b}{\sqrt{c}} \geq \sqrt{a}+\sqrt{b}+\sqrt{c}+C
$$

Solution: [Solution 1]
From the AM-GM Inequality, we have

$$
\begin{aligned}
& \frac{b+c}{\sqrt{a}}+\frac{c+a}{\sqrt{b}}+\frac{a+b}{\sqrt{c}} \geq 2\left(\sqrt{\frac{b c}{a}}+\sqrt{\frac{c a}{b}}+\sqrt{\frac{a b}{c}}\right)= \\
& =\left(\sqrt{\frac{b c}{a}}+\sqrt{\frac{c a}{b}}\right)+\left(\sqrt{\frac{c a}{b}}+\sqrt{\frac{a b}{c}}\right)+\left(\sqrt{\frac{a b}{c}}+\sqrt{\frac{b c}{a}}\right) \geq \\
& \geq 2(\sqrt{a}+\sqrt{b}+\sqrt{c}) \geq \sqrt{a}+\sqrt{b}+\sqrt{c}+3 \sqrt[6]{a b c}=\sqrt{a}+\sqrt{b}+\sqrt{c}+3 .
\end{aligned}
$$

Problem: Let $a, b, c$ be the side lengths of a triangle. Determine the largest constant $C$ such that the following inequality holds for all $a, b, c$ satisfying the triangle inequality:
$$
\frac{b+c}{a}+\frac{c+a}{b}+\frac{a+b}{c}+\frac{(b+c-a)(c+a-b)(a+b-c)}{a b c} \geq C.
$$

Solution:

## Response

To solve the problem, we need to analyze the given inequality:

\[
\frac{b+c}{a}+\frac{c+a}{b}+\frac{a+b}{c}+\frac{(b+c-a)(c+a-b)(a+b-c)}{abc} \geq C
\]

for all \(a, b, c\) satisfying the triangle inequality.

### Step 1: Simplifying the Left-Hand Side

We start by rewriting the first part of the left-hand side:

\[
\frac{b+c}{a} + \frac{c+a}{b} + \frac{a+b}{c} = \frac{b}{a} + \frac{c}{a} + \frac{c}{b} + \frac{a}{b} + \frac{a}{c} + \frac{b}{c}
\]

This can be expressed as:

\[
\sum_{\text{cyc}} \left( \frac{b}{a} + \frac{c}{a} \right) = \sum_{\text{cyc}} \frac{b+c}{a}
\]

### Step 2: Applying the AM-GM Inequality

Using the AM-GM inequality, we have:

\[
\frac{b+c}{a} + \frac{c+a}{b} + \frac{a+b}{c} \geq 6
\]

This is because:

\[
\frac{b+c}{a} \geq 2\sqrt{\frac{bc}{a^2}}, \quad \frac{c+a}{b} \geq 2\sqrt{\frac{ca}{b^2}}, \quad \frac{a+b}{c} \geq 2\sqrt{\frac{ab}{c^2}}
\]

Adding these inequalities gives:

\[
\frac{b+c}{a} + \frac{c+a}{b} + \frac{a+b}{c} \geq 6
\]

### Step 3: Analyzing the Second Term

Next, we analyze the term:

\[
\frac{(b+c-a)(c+a-b)(a+b-c)}{abc}
\]

By the triangle inequality, \(b+c-a > 0\), \(c+a-b > 0\), and \(a+b-c > 0\). Therefore, the product \((b+c-a)(c+a-b)(a+b-c)\) is positive.

### Step 4: Finding the Minimum Value of the Second Term

To find a lower bound for the second term, we can use the fact that the maximum value of each of the terms \(b+c-a\), \(c+a-b\), and \(a+b-c\) occurs when \(a, b, c\) are equal. 

Assuming \(a = b = c\), we can set \(a = b = c = 1\):

\[
(b+c-a)(c+a-b)(a+b-c) = (1+1-1)(1+1-1)(1+1-1) = 1
\]

Thus, we have:

\[
\frac{(b+c-a)(c+a-b)(a+b-c)}{abc} = \frac{1}{1} = 1
\]

### Step 5: Combining the Results

Combining both parts, we have:

\[
\frac{b+c}{a} + \frac{c+a}{b} + \frac{a+b}{c} + \frac{(b+c-a)(c+a-b)(a+b-c)}{abc} \geq 6 + 1 = 7
\]

### Conclusion

Thus, the largest constant \(C\) such that the inequality holds for all triangles is:

\[
C = 7
\]

Therefore, the final answer is:

\[
\text{The answer is } C=7
\]