## Problem

Find the largest constant $C$ such that for all real numbers $a, b, c$, the following inequality holds:
$$
a(b-c)^4+b(a-c)^4+c(a-b)^4 \geq C
$$

## Query

Task description: Please solve the problem with clear, rigorous, and logically sound steps. At the end of your response, state your answer in exactly this format: 'The answer is $C=X$', where X is your calculated numerical bound value. Example: 'The answer is $C=1$'.



Problem: Let $a, b, c$ be the side lengths, $h_{a}, h_{b}, h_{c}$ be the altitudes, respectively, and $r$ be the inradius of a triangle. Find the largest constant $C$ such that the following inequality holds for all triangles:
$$
\frac{1}{h_{a}-2 r}+\frac{1}{h_{b}-2 r}+\frac{1}{h_{c}-2 r} \geq C \cdot r
$$

Solution: By $\frac{1}{h_{a}}+\frac{1}{h_{b}}+\frac{1}{h_{c}}=\frac{1}{r}$ we obtain
$$
\frac{h_{a}-2 r}{h_{a}}+\frac{h_{b}-2 r}{h_{b}}+\frac{h_{c}-2 r}{h_{c}}=1
$$

Applying $A M \geq H M$ we get
$$
\left(\frac{h_{a}-2 r}{h_{a}}+\frac{h_{b}-2 r}{h_{b}}+\frac{h_{c}-2 r}{h_{c}}\right)\left(\frac{h_{a}}{h_{a}-2 r}+\frac{h_{b}}{h_{b}-2 r}+\frac{h_{c}}{h_{c}-2 r}\right) \geq 9
$$
i.e.
$$
\frac{h_{a}}{h_{a}-2 r}+\frac{h_{b}}{h_{b}-2 r}+\frac{h_{c}}{h_{c}-2 r} \geq 9
$$

Therefore
$$
\begin{aligned}
& \frac{2 r}{h_{a}-2 r}+\frac{2 r}{h_{b}-2 r}+\frac{2 r}{h_{c}-2 r} \\
& \quad=\frac{h_{a}-\left(h_{a}-2 r\right)}{h_{a}-2 r}+\frac{h_{b}-\left(h_{b}-2 r\right)}{h_{b}-2 r}+\frac{h_{c}-\left(h_{c}-2 r\right)}{h_{c}-2 r} \\
& \quad=\frac{h_{a}}{h_{a}-2 r}+\frac{h_{b}}{h_{b}-2 r}+\frac{h_{c}}{h_{c}-2 r}-3 \geq 9-3=6
\end{aligned}
$$
i.e.
$$
\frac{1}{h_{a}-2 r}+\frac{1}{h_{b}-2 r}+\frac{1}{h_{c}-2 r} \geq \frac{3}{r}
$$



Problem: Let $a, b, c$ be positive real numbers such that $a^2 + b^2 + c^2 = 3abc$. Find the largest constant $C$ such that the following inequality holds for all $a, b, c$ satisfying the given constraint:
$$
\frac{a}{b^2 c^2} + \frac{b}{c^2 a^2} + \frac{c}{a^2 b^2} \geq \frac{C}{a+b+c}
$$

Solution: The given inequality is equivalent to
$$
\left(a^{3}+b^{3}+c^{3}\right)(a+b+c) \geq 9 a^{2} b^{2} c^{2}
$$

Applying the Cauchy-Schwarz inequality we have
$$
\left(a^{3}+b^{3}+c^{3}\right)(a+b+c) \geq\left(a^{2}+b^{2}+c^{2}\right)^{2}
$$

Since $a^{2}+b^{2}+c^{2}=3 a b c$ we obtain
$$
\left(a^{3}+b^{3}+c^{3}\right)(a+b+c) \geq\left(a^{2}+b^{2}+c^{2}\right)^{2}=(3 a b c)^{2}=9 a^{2} b^{2} c^{2}
$$

Equality holds if and only if $a=b=c=1$.



Problem: Let $a, b, c$ be positive real numbers such that $a b c = 1$. Find the largest constant $C$ such that the following inequality holds for all $a, b, c$ satisfying the given constraint:
$$
\frac{b+c}{\sqrt{a}}+\frac{c+a}{\sqrt{b}}+\frac{a+b}{\sqrt{c}} \geq \sqrt{a}+\sqrt{b}+\sqrt{c}+C
$$

Solution: [Solution 1]
From the AM-GM Inequality, we have

$$
\begin{aligned}
& \frac{b+c}{\sqrt{a}}+\frac{c+a}{\sqrt{b}}+\frac{a+b}{\sqrt{c}} \geq 2\left(\sqrt{\frac{b c}{a}}+\sqrt{\frac{c a}{b}}+\sqrt{\frac{a b}{c}}\right)= \\
& =\left(\sqrt{\frac{b c}{a}}+\sqrt{\frac{c a}{b}}\right)+\left(\sqrt{\frac{c a}{b}}+\sqrt{\frac{a b}{c}}\right)+\left(\sqrt{\frac{a b}{c}}+\sqrt{\frac{b c}{a}}\right) \geq \\
& \geq 2(\sqrt{a}+\sqrt{b}+\sqrt{c}) \geq \sqrt{a}+\sqrt{b}+\sqrt{c}+3 \sqrt[6]{a b c}=\sqrt{a}+\sqrt{b}+\sqrt{c}+3 .
\end{aligned}
$$

Problem: Find the largest constant $C$ such that for all real numbers $a, b, c$, the following inequality holds:
$$
a(b-c)^4+b(a-c)^4+c(a-b)^4 \geq C
$$

Solution:

## Response

To solve the problem, we need to analyze the inequality 

\[
a(b-c)^4 + b(a-c)^4 + c(a-b)^4 \geq C
\]

for all real numbers \(a\), \(b\), and \(c\). 

### Step 1: Analyze the case when \(a = b = c\)

First, let's consider the case when \(a = b = c\). In this case, we have:

\[
a(b-c)^4 + b(a-c)^4 + c(a-b)^4 = a(0)^4 + b(0)^4 + c(0)^4 = 0
\]

This means that the left-hand side equals \(0\) when \(a = b = c\). Therefore, for the inequality to hold, \(C\) must be less than or equal to \(0\).

### Step 2: Check for other cases

Next, we will check if we can find a lower bound for the expression when \(a\), \(b\), and \(c\) are not all equal. 

#### Case 1: Let \(a = 1\), \(b = 1\), and \(c = 0\)

Substituting these values into the inequality gives:

\[
1(1-0)^4 + 1(1-0)^4 + 0(1-1)^4 = 1 + 1 + 0 = 2
\]

This suggests that \(C\) could be \(2\) or less.

#### Case 2: Let \(a = 1\), \(b = 0\), and \(c = 0\)

Substituting these values gives:

\[
1(0-0)^4 + 0(1-0)^4 + 0(1-0)^4 = 0 + 0 + 0 = 0
\]

This does not provide a new lower bound.

### Step 3: General case analysis

To find a general lower bound, we can apply the AM-GM inequality. 

Notice that:

\[
(b-c)^4 \geq 0, \quad (a-c)^4 \geq 0, \quad (a-b)^4 \geq 0
\]

Thus, each term in the expression is non-negative. Therefore, we can conclude that:

\[
a(b-c)^4 + b(a-c)^4 + c(a-b)^4 \geq 0
\]

### Step 4: Conclusion

Since we have established that the expression can be \(0\) when \(a = b = c\) and can be \(2\) when \(a = 1\), \(b = 1\), and \(c = 0\), we can conclude that the largest constant \(C\) such that the inequality holds for all real numbers \(a\), \(b\), and \(c\) is:

\[
C = 0
\]

Thus, the final answer is:

\[
\text{The answer is } C=0
\]