## Problem

Let $x, y, z \in \mathbb{R}$ satisfy the following constraints:
$$
\left\{\begin{array}{r}
x^2+x y+y^2=16 ; \\
y^2+y z+z^2=3 ;
\end{array}\right.
$$

Find the smallest constant $C$ such that the following inequality holds for all $x, y, z$ satisfying the constraints:
$$
x y+y z+z x \leq C.
$$

## Query

Task description: Please solve the problem with clear, rigorous, and logically sound steps. At the end of your response, state your answer in exactly this format: 'The answer is $C=X$', where X is your calculated numerical bound value. Example: 'The answer is $C=1$'.



Problem: Let $a, b, c$ be the side lengths, $h_{a}, h_{b}, h_{c}$ be the altitudes, respectively, and $r$ be the inradius of a triangle. Find the largest constant $C$ such that the following inequality holds for all triangles:
$$
\frac{1}{h_{a}-2 r}+\frac{1}{h_{b}-2 r}+\frac{1}{h_{c}-2 r} \geq C \cdot r
$$

Solution: By $\frac{1}{h_{a}}+\frac{1}{h_{b}}+\frac{1}{h_{c}}=\frac{1}{r}$ we obtain
$$
\frac{h_{a}-2 r}{h_{a}}+\frac{h_{b}-2 r}{h_{b}}+\frac{h_{c}-2 r}{h_{c}}=1
$$

Applying $A M \geq H M$ we get
$$
\left(\frac{h_{a}-2 r}{h_{a}}+\frac{h_{b}-2 r}{h_{b}}+\frac{h_{c}-2 r}{h_{c}}\right)\left(\frac{h_{a}}{h_{a}-2 r}+\frac{h_{b}}{h_{b}-2 r}+\frac{h_{c}}{h_{c}-2 r}\right) \geq 9
$$
i.e.
$$
\frac{h_{a}}{h_{a}-2 r}+\frac{h_{b}}{h_{b}-2 r}+\frac{h_{c}}{h_{c}-2 r} \geq 9
$$

Therefore
$$
\begin{aligned}
& \frac{2 r}{h_{a}-2 r}+\frac{2 r}{h_{b}-2 r}+\frac{2 r}{h_{c}-2 r} \\
& \quad=\frac{h_{a}-\left(h_{a}-2 r\right)}{h_{a}-2 r}+\frac{h_{b}-\left(h_{b}-2 r\right)}{h_{b}-2 r}+\frac{h_{c}-\left(h_{c}-2 r\right)}{h_{c}-2 r} \\
& \quad=\frac{h_{a}}{h_{a}-2 r}+\frac{h_{b}}{h_{b}-2 r}+\frac{h_{c}}{h_{c}-2 r}-3 \geq 9-3=6
\end{aligned}
$$
i.e.
$$
\frac{1}{h_{a}-2 r}+\frac{1}{h_{b}-2 r}+\frac{1}{h_{c}-2 r} \geq \frac{3}{r}
$$



Problem: Let $a, b, c$ be positive real numbers such that $a^2 + b^2 + c^2 = 3abc$. Find the largest constant $C$ such that the following inequality holds for all $a, b, c$ satisfying the given constraint:
$$
\frac{a}{b^2 c^2} + \frac{b}{c^2 a^2} + \frac{c}{a^2 b^2} \geq \frac{C}{a+b+c}
$$

Solution: The given inequality is equivalent to
$$
\left(a^{3}+b^{3}+c^{3}\right)(a+b+c) \geq 9 a^{2} b^{2} c^{2}
$$

Applying the Cauchy-Schwarz inequality we have
$$
\left(a^{3}+b^{3}+c^{3}\right)(a+b+c) \geq\left(a^{2}+b^{2}+c^{2}\right)^{2}
$$

Since $a^{2}+b^{2}+c^{2}=3 a b c$ we obtain
$$
\left(a^{3}+b^{3}+c^{3}\right)(a+b+c) \geq\left(a^{2}+b^{2}+c^{2}\right)^{2}=(3 a b c)^{2}=9 a^{2} b^{2} c^{2}
$$

Equality holds if and only if $a=b=c=1$.



Problem: Let $a, b, c$ be positive real numbers such that $a b c = 1$. Find the largest constant $C$ such that the following inequality holds for all $a, b, c$ satisfying the given constraint:
$$
\frac{b+c}{\sqrt{a}}+\frac{c+a}{\sqrt{b}}+\frac{a+b}{\sqrt{c}} \geq \sqrt{a}+\sqrt{b}+\sqrt{c}+C
$$

Solution: [Solution 1]
From the AM-GM Inequality, we have

$$
\begin{aligned}
& \frac{b+c}{\sqrt{a}}+\frac{c+a}{\sqrt{b}}+\frac{a+b}{\sqrt{c}} \geq 2\left(\sqrt{\frac{b c}{a}}+\sqrt{\frac{c a}{b}}+\sqrt{\frac{a b}{c}}\right)= \\
& =\left(\sqrt{\frac{b c}{a}}+\sqrt{\frac{c a}{b}}\right)+\left(\sqrt{\frac{c a}{b}}+\sqrt{\frac{a b}{c}}\right)+\left(\sqrt{\frac{a b}{c}}+\sqrt{\frac{b c}{a}}\right) \geq \\
& \geq 2(\sqrt{a}+\sqrt{b}+\sqrt{c}) \geq \sqrt{a}+\sqrt{b}+\sqrt{c}+3 \sqrt[6]{a b c}=\sqrt{a}+\sqrt{b}+\sqrt{c}+3 .
\end{aligned}
$$

Problem: Let $x, y, z \in \mathbb{R}$ satisfy the following constraints:
$$
\left\{\begin{array}{r}
x^2+x y+y^2=16 ; \\
y^2+y z+z^2=3 ;
\end{array}\right.
$$

Find the smallest constant $C$ such that the following inequality holds for all $x, y, z$ satisfying the constraints:
$$
x y+y z+z x \leq C.
$$

Solution:

## Response

To solve the problem, we start with the given constraints:

1. \( x^2 + xy + y^2 = 16 \)
2. \( y^2 + yz + z^2 = 3 \)

We need to find the smallest constant \( C \) such that the inequality \( xy + yz + zx \leq C \) holds for all \( x, y, z \) satisfying the constraints.

### Step 1: Analyze the first constraint

From the first constraint, we can express \( x^2 + xy + y^2 = 16 \). This can be rearranged to:

\[
x^2 + xy + y^2 - 16 = 0
\]

This is a quadratic equation in \( x \):

\[
x^2 + xy + (y^2 - 16) = 0
\]

The discriminant of this quadratic must be non-negative for \( x \) to have real solutions:

\[
D = y^2 - 4(y^2 - 16) = -3y^2 + 64 \geq 0
\]

This gives us:

\[
3y^2 \leq 64 \implies y^2 \leq \frac{64}{3} \implies |y| \leq \frac{8}{\sqrt{3}} \approx 4.6188
\]

### Step 2: Analyze the second constraint

From the second constraint, we have:

\[
y^2 + yz + z^2 = 3
\]

This can also be rearranged to:

\[
y^2 + yz + z^2 - 3 = 0
\]

This is a quadratic equation in \( z \):

\[
z^2 + yz + (y^2 - 3) = 0
\]

The discriminant must also be non-negative:

\[
D = y^2 - 4(y^2 - 3) = -3y^2 + 12 \geq 0
\]

This gives us:

\[
3y^2 \leq 12 \implies y^2 \leq 4 \implies |y| \leq 2
\]

### Step 3: Combine the constraints on \( y \)

From the two analyses, we have:

\[
|y| \leq 2
\]

### Step 4: Find bounds for \( xy + yz + zx \)

We will express \( xy + yz + zx \) in terms of \( y \) and find its maximum value under the constraints.

Using the first constraint, we can express \( x \) in terms of \( y \):

\[
x = \frac{-y \pm \sqrt{-3y^2 + 64}}{2}
\]

Using the second constraint, we can express \( z \) in terms of \( y \):

\[
z = \frac{-y \pm \sqrt{-3y^2 + 12}}{2}
\]

Now we can substitute these expressions into \( xy + yz + zx \):

\[
xy + yz + zx = y \left( \frac{-y \pm \sqrt{-3y^2 + 64}}{2} + \frac{-y \pm \sqrt{-3y^2 + 12}}{2} \right) + \frac{-y \pm \sqrt{-3y^2 + 64}}{2} \cdot \frac{-y \pm \sqrt{-3y^2 + 12}}{2}
\]

This expression is quite complex, so we will evaluate specific values of \( y \) within the bounds \( -2 \leq y \leq 2 \) to find the maximum value of \( xy + yz + zx \).

### Step 5: Evaluate specific values

1. **For \( y = 2 \)**:
   - From \( x^2 + 2x + 4 = 16 \) gives \( x^2 + 2x - 12 = 0 \) with roots \( x = 2 \) or \( x = -6 \).
   - From \( 4 + 2z + z^2 = 3 \) gives \( z^2 + 2z + 1 = 0 \) with root \( z = -1 \).
   - Thus, \( xy + yz + zx = 2 \cdot 2 + 2 \cdot (-1) + 2 \cdot (-1) = 4 - 2 - 2 = 0 \).

2. **For \( y = 0 \)**:
   - From \( x^2 = 16 \) gives \( x = 4 \) or \( x = -4 \).
   - From \( 0 + 0 + z^2 = 3 \) gives \( z = \sqrt{3} \) or \( z = -\sqrt{3} \).
   - Thus, \( xy + yz + zx = 0 + 0 + 0 = 0 \).

3. **For \( y = -2 \)**:
   - From \( x^2 - 2x + 4 = 16 \) gives \( x^2 - 2x - 12 = 0 \) with roots \( x = 6 \) or \( x = -2 \).
   - From \( 4 - 2z + z^2 = 3 \) gives \( z^2 - 2z + 1 = 0 \) with root \( z = 1 \).
   - Thus, \( xy + yz + zx = -2 \cdot 6 + (-2) \cdot 1 + 6 \cdot 1 = -12 - 2 + 6 = -8 \).

### Conclusion

After evaluating these cases, we find that the maximum value of \( xy + yz + zx \) is \( 0 \). Therefore, the smallest constant \( C \) such that \( xy + yz + zx \leq C \) for all \( x, y, z \) satisfying the constraints is:

\[
C = 0
\]

Thus, the final answer is:

The answer is \( C=0 \).