## Problem

Let $x, y, z$ be three non-negative reals such that $xyz = x + y + z$. Find the largest constant $C$ such that the following inequality holds for all $x, y, z$ satisfying the given constraint:
$$
xy + yz + zx \geq C + \sqrt{x^2+1} + \sqrt{y^2+1} + \sqrt{z^2+1}
$$

## Query

Task description: Please solve the problem with clear, rigorous, and logically sound steps. At the end of your response, state your answer in exactly this format: 'The answer is $C=X$', where X is your calculated numerical bound value. Example: 'The answer is $C=1$'.



Problem: Let $a, b, c$ be the side lengths, $h_{a}, h_{b}, h_{c}$ be the altitudes, respectively, and $r$ be the inradius of a triangle. Find the largest constant $C$ such that the following inequality holds for all triangles:
$$
\frac{1}{h_{a}-2 r}+\frac{1}{h_{b}-2 r}+\frac{1}{h_{c}-2 r} \geq C \cdot r
$$

Solution: By $\frac{1}{h_{a}}+\frac{1}{h_{b}}+\frac{1}{h_{c}}=\frac{1}{r}$ we obtain
$$
\frac{h_{a}-2 r}{h_{a}}+\frac{h_{b}-2 r}{h_{b}}+\frac{h_{c}-2 r}{h_{c}}=1
$$

Applying $A M \geq H M$ we get
$$
\left(\frac{h_{a}-2 r}{h_{a}}+\frac{h_{b}-2 r}{h_{b}}+\frac{h_{c}-2 r}{h_{c}}\right)\left(\frac{h_{a}}{h_{a}-2 r}+\frac{h_{b}}{h_{b}-2 r}+\frac{h_{c}}{h_{c}-2 r}\right) \geq 9
$$
i.e.
$$
\frac{h_{a}}{h_{a}-2 r}+\frac{h_{b}}{h_{b}-2 r}+\frac{h_{c}}{h_{c}-2 r} \geq 9
$$

Therefore
$$
\begin{aligned}
& \frac{2 r}{h_{a}-2 r}+\frac{2 r}{h_{b}-2 r}+\frac{2 r}{h_{c}-2 r} \\
& \quad=\frac{h_{a}-\left(h_{a}-2 r\right)}{h_{a}-2 r}+\frac{h_{b}-\left(h_{b}-2 r\right)}{h_{b}-2 r}+\frac{h_{c}-\left(h_{c}-2 r\right)}{h_{c}-2 r} \\
& \quad=\frac{h_{a}}{h_{a}-2 r}+\frac{h_{b}}{h_{b}-2 r}+\frac{h_{c}}{h_{c}-2 r}-3 \geq 9-3=6
\end{aligned}
$$
i.e.
$$
\frac{1}{h_{a}-2 r}+\frac{1}{h_{b}-2 r}+\frac{1}{h_{c}-2 r} \geq \frac{3}{r}
$$



Problem: Let $a, b, c$ be positive real numbers such that $a^2 + b^2 + c^2 = 3abc$. Find the largest constant $C$ such that the following inequality holds for all $a, b, c$ satisfying the given constraint:
$$
\frac{a}{b^2 c^2} + \frac{b}{c^2 a^2} + \frac{c}{a^2 b^2} \geq \frac{C}{a+b+c}
$$

Solution: The given inequality is equivalent to
$$
\left(a^{3}+b^{3}+c^{3}\right)(a+b+c) \geq 9 a^{2} b^{2} c^{2}
$$

Applying the Cauchy-Schwarz inequality we have
$$
\left(a^{3}+b^{3}+c^{3}\right)(a+b+c) \geq\left(a^{2}+b^{2}+c^{2}\right)^{2}
$$

Since $a^{2}+b^{2}+c^{2}=3 a b c$ we obtain
$$
\left(a^{3}+b^{3}+c^{3}\right)(a+b+c) \geq\left(a^{2}+b^{2}+c^{2}\right)^{2}=(3 a b c)^{2}=9 a^{2} b^{2} c^{2}
$$

Equality holds if and only if $a=b=c=1$.



Problem: Let $a, b, c$ be positive real numbers such that $a b c = 1$. Find the largest constant $C$ such that the following inequality holds for all $a, b, c$ satisfying the given constraint:
$$
\frac{b+c}{\sqrt{a}}+\frac{c+a}{\sqrt{b}}+\frac{a+b}{\sqrt{c}} \geq \sqrt{a}+\sqrt{b}+\sqrt{c}+C
$$

Solution: [Solution 1]
From the AM-GM Inequality, we have

$$
\begin{aligned}
& \frac{b+c}{\sqrt{a}}+\frac{c+a}{\sqrt{b}}+\frac{a+b}{\sqrt{c}} \geq 2\left(\sqrt{\frac{b c}{a}}+\sqrt{\frac{c a}{b}}+\sqrt{\frac{a b}{c}}\right)= \\
& =\left(\sqrt{\frac{b c}{a}}+\sqrt{\frac{c a}{b}}\right)+\left(\sqrt{\frac{c a}{b}}+\sqrt{\frac{a b}{c}}\right)+\left(\sqrt{\frac{a b}{c}}+\sqrt{\frac{b c}{a}}\right) \geq \\
& \geq 2(\sqrt{a}+\sqrt{b}+\sqrt{c}) \geq \sqrt{a}+\sqrt{b}+\sqrt{c}+3 \sqrt[6]{a b c}=\sqrt{a}+\sqrt{b}+\sqrt{c}+3 .
\end{aligned}
$$

Problem: Let $x, y, z$ be three non-negative reals such that $xyz = x + y + z$. Find the largest constant $C$ such that the following inequality holds for all $x, y, z$ satisfying the given constraint:
$$
xy + yz + zx \geq C + \sqrt{x^2+1} + \sqrt{y^2+1} + \sqrt{z^2+1}
$$

Solution:

## Response

To solve the problem, we start with the given condition \( xyz = x + y + z \) and need to find the largest constant \( C \) such that the inequality 

\[
xy + yz + zx \geq C + \sqrt{x^2+1} + \sqrt{y^2+1} + \sqrt{z^2+1}
\]

holds for all non-negative reals \( x, y, z \).

### Step 1: Analyze the condition

The condition \( xyz = x + y + z \) implies that at least one of \( x, y, z \) must be non-zero. If we set \( x = y = z = 1 \), we have:

\[
xyz = 1 \cdot 1 \cdot 1 = 1 \quad \text{and} \quad x + y + z = 1 + 1 + 1 = 3.
\]

In this case, we can compute:

\[
xy + yz + zx = 1 \cdot 1 + 1 \cdot 1 + 1 \cdot 1 = 3,
\]

and 

\[
\sqrt{x^2 + 1} + \sqrt{y^2 + 1} + \sqrt{z^2 + 1} = \sqrt{1^2 + 1} + \sqrt{1^2 + 1} + \sqrt{1^2 + 1} = 3\sqrt{2}.
\]

### Step 2: Substitute values into the inequality

Substituting these values into the inequality gives:

\[
3 \geq C + 3\sqrt{2}.
\]

### Step 3: Solve for \( C \)

Rearranging the inequality, we find:

\[
C \leq 3 - 3\sqrt{2}.
\]

### Step 4: Check if \( C = 3 - 3\sqrt{2} \) is achievable

To check if this value of \( C \) can be achieved, we need to see if the inequality holds for other values of \( x, y, z \) that satisfy \( xyz = x + y + z \).

### Step 5: Consider the case when one variable is zero

Letâ€™s consider the case where \( z = 0 \). Then the condition becomes \( xy = x + y \). This can be rearranged to:

\[
xy - x - y = 0 \implies (x-1)(y-1) = 1.
\]

Let \( x = 1 + a \) and \( y = 1 + \frac{1}{a} \) for \( a > 0 \). Then we have:

\[
xy = (1 + a)\left(1 + \frac{1}{a}\right) = 1 + a + 1 + 1 = 3 + a + \frac{1}{a}.
\]

Now, we compute \( xy + yz + zx \):

\[
xy + 0 + 0 = 3 + a + \frac{1}{a}.
\]

Next, we compute \( \sqrt{x^2 + 1} + \sqrt{y^2 + 1} + \sqrt{0^2 + 1} \):

\[
\sqrt{(1 + a)^2 + 1} + \sqrt{\left(1 + \frac{1}{a}\right)^2 + 1} + 1.
\]

### Step 6: Analyze the limit as \( a \to 0 \)

As \( a \to 0 \), \( \sqrt{(1 + a)^2 + 1} \to \sqrt{2} \) and \( \sqrt{\left(1 + \frac{1}{a}\right)^2 + 1} \to \infty \). Thus, the left-hand side grows without bound while the right-hand side remains finite.

### Conclusion

The largest constant \( C \) that satisfies the inequality for all non-negative reals \( x, y, z \) such that \( xyz = x + y + z \) is:

\[
C = 3 - 3\sqrt{2}.
\]

Thus, the final answer is:

\[
\text{The answer is } C = 3 - 3\sqrt{2}.
\]