## Problem

Let $x, y, z$ be real numbers such that $0 \leq x, y, z \leq 1$. Find the smallest constant $C$ such that the following inequality holds for all $x, y, z$ in the given domain:
$$
\frac{x}{y+z+1}+\frac{y}{z+x+1}+\frac{z}{x+y+1} \leq 3C -(1-x)(1-y)(1-z).
$$

## Query

Task description: Please solve the problem with clear, rigorous, and logically sound steps. At the end of your response, state your answer in exactly this format: 'The answer is $C=X$', where X is your calculated numerical bound value. Example: 'The answer is $C=1$'.



Problem: Let $a, b, c$ be the side lengths, $h_{a}, h_{b}, h_{c}$ be the altitudes, respectively, and $r$ be the inradius of a triangle. Find the largest constant $C$ such that the following inequality holds for all triangles:
$$
\frac{1}{h_{a}-2 r}+\frac{1}{h_{b}-2 r}+\frac{1}{h_{c}-2 r} \geq C \cdot r
$$

Solution: By $\frac{1}{h_{a}}+\frac{1}{h_{b}}+\frac{1}{h_{c}}=\frac{1}{r}$ we obtain
$$
\frac{h_{a}-2 r}{h_{a}}+\frac{h_{b}-2 r}{h_{b}}+\frac{h_{c}-2 r}{h_{c}}=1
$$

Applying $A M \geq H M$ we get
$$
\left(\frac{h_{a}-2 r}{h_{a}}+\frac{h_{b}-2 r}{h_{b}}+\frac{h_{c}-2 r}{h_{c}}\right)\left(\frac{h_{a}}{h_{a}-2 r}+\frac{h_{b}}{h_{b}-2 r}+\frac{h_{c}}{h_{c}-2 r}\right) \geq 9
$$
i.e.
$$
\frac{h_{a}}{h_{a}-2 r}+\frac{h_{b}}{h_{b}-2 r}+\frac{h_{c}}{h_{c}-2 r} \geq 9
$$

Therefore
$$
\begin{aligned}
& \frac{2 r}{h_{a}-2 r}+\frac{2 r}{h_{b}-2 r}+\frac{2 r}{h_{c}-2 r} \\
& \quad=\frac{h_{a}-\left(h_{a}-2 r\right)}{h_{a}-2 r}+\frac{h_{b}-\left(h_{b}-2 r\right)}{h_{b}-2 r}+\frac{h_{c}-\left(h_{c}-2 r\right)}{h_{c}-2 r} \\
& \quad=\frac{h_{a}}{h_{a}-2 r}+\frac{h_{b}}{h_{b}-2 r}+\frac{h_{c}}{h_{c}-2 r}-3 \geq 9-3=6
\end{aligned}
$$
i.e.
$$
\frac{1}{h_{a}-2 r}+\frac{1}{h_{b}-2 r}+\frac{1}{h_{c}-2 r} \geq \frac{3}{r}
$$



Problem: Let $a, b, c$ be positive real numbers such that $a^2 + b^2 + c^2 = 3abc$. Find the largest constant $C$ such that the following inequality holds for all $a, b, c$ satisfying the given constraint:
$$
\frac{a}{b^2 c^2} + \frac{b}{c^2 a^2} + \frac{c}{a^2 b^2} \geq \frac{C}{a+b+c}
$$

Solution: The given inequality is equivalent to
$$
\left(a^{3}+b^{3}+c^{3}\right)(a+b+c) \geq 9 a^{2} b^{2} c^{2}
$$

Applying the Cauchy-Schwarz inequality we have
$$
\left(a^{3}+b^{3}+c^{3}\right)(a+b+c) \geq\left(a^{2}+b^{2}+c^{2}\right)^{2}
$$

Since $a^{2}+b^{2}+c^{2}=3 a b c$ we obtain
$$
\left(a^{3}+b^{3}+c^{3}\right)(a+b+c) \geq\left(a^{2}+b^{2}+c^{2}\right)^{2}=(3 a b c)^{2}=9 a^{2} b^{2} c^{2}
$$

Equality holds if and only if $a=b=c=1$.



Problem: Let $a, b, c$ be positive real numbers such that $a b c = 1$. Find the largest constant $C$ such that the following inequality holds for all $a, b, c$ satisfying the given constraint:
$$
\frac{b+c}{\sqrt{a}}+\frac{c+a}{\sqrt{b}}+\frac{a+b}{\sqrt{c}} \geq \sqrt{a}+\sqrt{b}+\sqrt{c}+C
$$

Solution: [Solution 1]
From the AM-GM Inequality, we have

$$
\begin{aligned}
& \frac{b+c}{\sqrt{a}}+\frac{c+a}{\sqrt{b}}+\frac{a+b}{\sqrt{c}} \geq 2\left(\sqrt{\frac{b c}{a}}+\sqrt{\frac{c a}{b}}+\sqrt{\frac{a b}{c}}\right)= \\
& =\left(\sqrt{\frac{b c}{a}}+\sqrt{\frac{c a}{b}}\right)+\left(\sqrt{\frac{c a}{b}}+\sqrt{\frac{a b}{c}}\right)+\left(\sqrt{\frac{a b}{c}}+\sqrt{\frac{b c}{a}}\right) \geq \\
& \geq 2(\sqrt{a}+\sqrt{b}+\sqrt{c}) \geq \sqrt{a}+\sqrt{b}+\sqrt{c}+3 \sqrt[6]{a b c}=\sqrt{a}+\sqrt{b}+\sqrt{c}+3 .
\end{aligned}
$$

Problem: Let $x, y, z$ be real numbers such that $0 \leq x, y, z \leq 1$. Find the smallest constant $C$ such that the following inequality holds for all $x, y, z$ in the given domain:
$$
\frac{x}{y+z+1}+\frac{y}{z+x+1}+\frac{z}{x+y+1} \leq 3C -(1-x)(1-y)(1-z).
$$

Solution:

## Response

To solve the problem, we need to analyze the inequality given:

\[
\frac{x}{y+z+1}+\frac{y}{z+x+1}+\frac{z}{x+y+1} \leq 3C -(1-x)(1-y)(1-z)
\]

for \(0 \leq x, y, z \leq 1\). 

### Step 1: Analyze the left-hand side

The left-hand side can be interpreted as a sum of fractions where each term is non-negative since \(x, y, z \geq 0\) and \(y+z+1, z+x+1, x+y+1 \geq 1\). 

### Step 2: Analyze the right-hand side

The right-hand side consists of two parts: \(3C\) and \(-(1-x)(1-y)(1-z)\). The term \(-(1-x)(1-y)(1-z)\) is non-positive since \(1-x, 1-y, 1-z \geq 0\) for \(x, y, z \leq 1\). 

### Step 3: Find the maximum of the left-hand side

To find the maximum of the left-hand side, we can consider specific cases for \(x, y, z\):

1. **Case 1**: Let \(x = y = z = 1\):
   \[
   \frac{1}{1+1+1} + \frac{1}{1+1+1} + \frac{1}{1+1+1} = 3 \cdot \frac{1}{3} = 1
   \]

2. **Case 2**: Let \(x = 1, y = 1, z = 0\):
   \[
   \frac{1}{1+0+1} + \frac{1}{0+1+1} + \frac{0}{1+1+1} = \frac{1}{2} + \frac{1}{2} + 0 = 1
   \]

3. **Case 3**: Let \(x = 1, y = 0, z = 0\):
   \[
   \frac{1}{0+0+1} + \frac{0}{0+1+1} + \frac{0}{1+0+1} = 1 + 0 + 0 = 1
   \]

In all these cases, the left-hand side achieves a maximum value of 1.

### Step 4: Analyze the right-hand side

Now, we need to ensure that the right-hand side can accommodate this maximum value. The term \(-(1-x)(1-y)(1-z)\) will be maximized when \(x, y, z\) are minimized. The maximum value of \((1-x)(1-y)(1-z)\) occurs when \(x = y = z = 0\), giving:

\[
-(1-0)(1-0)(1-0) = -1
\]

Thus, the right-hand side becomes:

\[
3C - 1
\]

### Step 5: Set up the inequality

To satisfy the inequality for the maximum value of the left-hand side, we need:

\[
1 \leq 3C - 1
\]

### Step 6: Solve for \(C\)

Rearranging gives:

\[
3C \geq 2 \implies C \geq \frac{2}{3}
\]

### Conclusion

To find the smallest constant \(C\) such that the inequality holds for all \(x, y, z\) in the given domain, we conclude:

\[
C = \frac{2}{3}
\]

Thus, the final answer is:

The answer is \(C=\frac{2}{3}\).