## Problem

Let $a, b, c$ be real numbers such that $a+b+c=1$. Find the smallest constant $C$ such that the following inequality holds for all $a, b, c$ satisfying the given constraint:
$$
\frac{11 a-2}{1+a^2}+\frac{11 b-2}{1+b^2}+\frac{11 c-2}{1+c^2} \leq C.
$$

## Query

Task description: Please solve the problem with clear, rigorous, and logically sound steps. At the end of your response, state your answer in exactly this format: 'The answer is $C=X$', where X is your calculated numerical bound value. Example: 'The answer is $C=1$'.



Problem: Let $a, b, c$ be the side lengths, $h_{a}, h_{b}, h_{c}$ be the altitudes, respectively, and $r$ be the inradius of a triangle. Find the largest constant $C$ such that the following inequality holds for all triangles:
$$
\frac{1}{h_{a}-2 r}+\frac{1}{h_{b}-2 r}+\frac{1}{h_{c}-2 r} \geq C \cdot r
$$

Solution: By $\frac{1}{h_{a}}+\frac{1}{h_{b}}+\frac{1}{h_{c}}=\frac{1}{r}$ we obtain
$$
\frac{h_{a}-2 r}{h_{a}}+\frac{h_{b}-2 r}{h_{b}}+\frac{h_{c}-2 r}{h_{c}}=1
$$

Applying $A M \geq H M$ we get
$$
\left(\frac{h_{a}-2 r}{h_{a}}+\frac{h_{b}-2 r}{h_{b}}+\frac{h_{c}-2 r}{h_{c}}\right)\left(\frac{h_{a}}{h_{a}-2 r}+\frac{h_{b}}{h_{b}-2 r}+\frac{h_{c}}{h_{c}-2 r}\right) \geq 9
$$
i.e.
$$
\frac{h_{a}}{h_{a}-2 r}+\frac{h_{b}}{h_{b}-2 r}+\frac{h_{c}}{h_{c}-2 r} \geq 9
$$

Therefore
$$
\begin{aligned}
& \frac{2 r}{h_{a}-2 r}+\frac{2 r}{h_{b}-2 r}+\frac{2 r}{h_{c}-2 r} \\
& \quad=\frac{h_{a}-\left(h_{a}-2 r\right)}{h_{a}-2 r}+\frac{h_{b}-\left(h_{b}-2 r\right)}{h_{b}-2 r}+\frac{h_{c}-\left(h_{c}-2 r\right)}{h_{c}-2 r} \\
& \quad=\frac{h_{a}}{h_{a}-2 r}+\frac{h_{b}}{h_{b}-2 r}+\frac{h_{c}}{h_{c}-2 r}-3 \geq 9-3=6
\end{aligned}
$$
i.e.
$$
\frac{1}{h_{a}-2 r}+\frac{1}{h_{b}-2 r}+\frac{1}{h_{c}-2 r} \geq \frac{3}{r}
$$



Problem: Let $a, b, c$ be positive real numbers such that $a^2 + b^2 + c^2 = 3abc$. Find the largest constant $C$ such that the following inequality holds for all $a, b, c$ satisfying the given constraint:
$$
\frac{a}{b^2 c^2} + \frac{b}{c^2 a^2} + \frac{c}{a^2 b^2} \geq \frac{C}{a+b+c}
$$

Solution: The given inequality is equivalent to
$$
\left(a^{3}+b^{3}+c^{3}\right)(a+b+c) \geq 9 a^{2} b^{2} c^{2}
$$

Applying the Cauchy-Schwarz inequality we have
$$
\left(a^{3}+b^{3}+c^{3}\right)(a+b+c) \geq\left(a^{2}+b^{2}+c^{2}\right)^{2}
$$

Since $a^{2}+b^{2}+c^{2}=3 a b c$ we obtain
$$
\left(a^{3}+b^{3}+c^{3}\right)(a+b+c) \geq\left(a^{2}+b^{2}+c^{2}\right)^{2}=(3 a b c)^{2}=9 a^{2} b^{2} c^{2}
$$

Equality holds if and only if $a=b=c=1$.



Problem: Let $a, b, c$ be positive real numbers such that $a b c = 1$. Find the largest constant $C$ such that the following inequality holds for all $a, b, c$ satisfying the given constraint:
$$
\frac{b+c}{\sqrt{a}}+\frac{c+a}{\sqrt{b}}+\frac{a+b}{\sqrt{c}} \geq \sqrt{a}+\sqrt{b}+\sqrt{c}+C
$$

Solution: [Solution 1]
From the AM-GM Inequality, we have

$$
\begin{aligned}
& \frac{b+c}{\sqrt{a}}+\frac{c+a}{\sqrt{b}}+\frac{a+b}{\sqrt{c}} \geq 2\left(\sqrt{\frac{b c}{a}}+\sqrt{\frac{c a}{b}}+\sqrt{\frac{a b}{c}}\right)= \\
& =\left(\sqrt{\frac{b c}{a}}+\sqrt{\frac{c a}{b}}\right)+\left(\sqrt{\frac{c a}{b}}+\sqrt{\frac{a b}{c}}\right)+\left(\sqrt{\frac{a b}{c}}+\sqrt{\frac{b c}{a}}\right) \geq \\
& \geq 2(\sqrt{a}+\sqrt{b}+\sqrt{c}) \geq \sqrt{a}+\sqrt{b}+\sqrt{c}+3 \sqrt[6]{a b c}=\sqrt{a}+\sqrt{b}+\sqrt{c}+3 .
\end{aligned}
$$

Problem: Let $a, b, c$ be real numbers such that $a+b+c=1$. Find the smallest constant $C$ such that the following inequality holds for all $a, b, c$ satisfying the given constraint:
$$
\frac{11 a-2}{1+a^2}+\frac{11 b-2}{1+b^2}+\frac{11 c-2}{1+c^2} \leq C.
$$

Solution:

## Response

To solve the problem, we need to analyze the expression 

\[
S = \frac{11a - 2}{1 + a^2} + \frac{11b - 2}{1 + b^2} + \frac{11c - 2}{1 + c^2}
\]

under the constraint \( a + b + c = 1 \).

### Step 1: Analyze the function

We will first analyze the function 

\[
f(x) = \frac{11x - 2}{1 + x^2}
\]

to find its maximum value for \( x \in [0, 1] \).

### Step 2: Find the derivative

To find the critical points, we compute the derivative \( f'(x) \):

\[
f'(x) = \frac{(11)(1 + x^2) - (11x - 2)(2x)}{(1 + x^2)^2}
\]

Simplifying the numerator:

\[
11 + 11x^2 - (22x^2 - 4x) = 11 + 11x^2 - 22x^2 + 4x = 11 - 11x^2 + 4x
\]

Setting the numerator equal to zero to find critical points:

\[
11 - 11x^2 + 4x = 0 \implies 11x^2 - 4x - 11 = 0
\]

### Step 3: Solve the quadratic equation

Using the quadratic formula:

\[
x = \frac{-b \pm \sqrt{b^2 - 4ac}}{2a} = \frac{-(-4) \pm \sqrt{(-4)^2 - 4 \cdot 11 \cdot (-11)}}{2 \cdot 11} = \frac{4 \pm \sqrt{16 + 484}}{22} = \frac{4 \pm \sqrt{500}}{22} = \frac{4 \pm 10\sqrt{5}}{22} = \frac{2 \pm 5\sqrt{5}}{11}
\]

Calculating the approximate values:

- \( x_1 = \frac{2 + 5\sqrt{5}}{11} \) (approximately 1.1, outside the interval [0, 1])
- \( x_2 = \frac{2 - 5\sqrt{5}}{11} \) (approximately -0.5, also outside the interval [0, 1])

### Step 4: Evaluate endpoints

Since there are no critical points in the interval [0, 1], we evaluate \( f(x) \) at the endpoints:

1. \( f(0) = \frac{11(0) - 2}{1 + 0^2} = -2 \)
2. \( f(1) = \frac{11(1) - 2}{1 + 1^2} = \frac{9}{2} = 4.5 \)

### Step 5: Combine results

Since \( f(x) \) is continuous and differentiable in the interval [0, 1], and we have evaluated the endpoints, the maximum value of \( f(x) \) on this interval is \( 4.5 \).

### Step 6: Find the maximum of \( S \)

Now, we can find the maximum of \( S \):

\[
S \leq f(a) + f(b) + f(c) \leq 3 \cdot 4.5 = 13.5
\]

### Conclusion

Thus, the smallest constant \( C \) such that 

\[
\frac{11a - 2}{1 + a^2} + \frac{11b - 2}{1 + b^2} + \frac{11c - 2}{1 + c^2} \leq C
\]

for all \( a, b, c \) satisfying \( a + b + c = 1 \) is 

\[
C = 13.5.
\]

Therefore, the final answer is:

The answer is \( C = 13.5 \).