## Problem

Let $a, b, c \geq 0$ and $a+b+c=1$. Determine the minimal constant $C$ such that the following inequality holds for all $a, b, c$:

$$
\frac{a}{\sqrt{b^2+3 c}}+\frac{b}{\sqrt{c^2+3 a}}+\frac{c}{\sqrt{a^2+3 b}} \geq \frac{1}{\sqrt{1+2C a b c}}.
$$

## Query

Task description: Please solve the problem with clear, rigorous, and logically sound steps. At the end of your response, state your answer in exactly this format: 'The answer is $C=X$', where X is your calculated numerical bound value. Example: 'The answer is $C=1$'.



Problem: Let $a, b, c$ be the side lengths, $h_{a}, h_{b}, h_{c}$ be the altitudes, respectively, and $r$ be the inradius of a triangle. Find the largest constant $C$ such that the following inequality holds for all triangles:
$$
\frac{1}{h_{a}-2 r}+\frac{1}{h_{b}-2 r}+\frac{1}{h_{c}-2 r} \geq C \cdot r
$$

Solution: By $\frac{1}{h_{a}}+\frac{1}{h_{b}}+\frac{1}{h_{c}}=\frac{1}{r}$ we obtain
$$
\frac{h_{a}-2 r}{h_{a}}+\frac{h_{b}-2 r}{h_{b}}+\frac{h_{c}-2 r}{h_{c}}=1
$$

Applying $A M \geq H M$ we get
$$
\left(\frac{h_{a}-2 r}{h_{a}}+\frac{h_{b}-2 r}{h_{b}}+\frac{h_{c}-2 r}{h_{c}}\right)\left(\frac{h_{a}}{h_{a}-2 r}+\frac{h_{b}}{h_{b}-2 r}+\frac{h_{c}}{h_{c}-2 r}\right) \geq 9
$$
i.e.
$$
\frac{h_{a}}{h_{a}-2 r}+\frac{h_{b}}{h_{b}-2 r}+\frac{h_{c}}{h_{c}-2 r} \geq 9
$$

Therefore
$$
\begin{aligned}
& \frac{2 r}{h_{a}-2 r}+\frac{2 r}{h_{b}-2 r}+\frac{2 r}{h_{c}-2 r} \\
& \quad=\frac{h_{a}-\left(h_{a}-2 r\right)}{h_{a}-2 r}+\frac{h_{b}-\left(h_{b}-2 r\right)}{h_{b}-2 r}+\frac{h_{c}-\left(h_{c}-2 r\right)}{h_{c}-2 r} \\
& \quad=\frac{h_{a}}{h_{a}-2 r}+\frac{h_{b}}{h_{b}-2 r}+\frac{h_{c}}{h_{c}-2 r}-3 \geq 9-3=6
\end{aligned}
$$
i.e.
$$
\frac{1}{h_{a}-2 r}+\frac{1}{h_{b}-2 r}+\frac{1}{h_{c}-2 r} \geq \frac{3}{r}
$$



Problem: Let $a, b, c$ be positive real numbers such that $a^2 + b^2 + c^2 = 3abc$. Find the largest constant $C$ such that the following inequality holds for all $a, b, c$ satisfying the given constraint:
$$
\frac{a}{b^2 c^2} + \frac{b}{c^2 a^2} + \frac{c}{a^2 b^2} \geq \frac{C}{a+b+c}
$$

Solution: The given inequality is equivalent to
$$
\left(a^{3}+b^{3}+c^{3}\right)(a+b+c) \geq 9 a^{2} b^{2} c^{2}
$$

Applying the Cauchy-Schwarz inequality we have
$$
\left(a^{3}+b^{3}+c^{3}\right)(a+b+c) \geq\left(a^{2}+b^{2}+c^{2}\right)^{2}
$$

Since $a^{2}+b^{2}+c^{2}=3 a b c$ we obtain
$$
\left(a^{3}+b^{3}+c^{3}\right)(a+b+c) \geq\left(a^{2}+b^{2}+c^{2}\right)^{2}=(3 a b c)^{2}=9 a^{2} b^{2} c^{2}
$$

Equality holds if and only if $a=b=c=1$.



Problem: Let $a, b, c$ be positive real numbers such that $a b c = 1$. Find the largest constant $C$ such that the following inequality holds for all $a, b, c$ satisfying the given constraint:
$$
\frac{b+c}{\sqrt{a}}+\frac{c+a}{\sqrt{b}}+\frac{a+b}{\sqrt{c}} \geq \sqrt{a}+\sqrt{b}+\sqrt{c}+C
$$

Solution: [Solution 1]
From the AM-GM Inequality, we have

$$
\begin{aligned}
& \frac{b+c}{\sqrt{a}}+\frac{c+a}{\sqrt{b}}+\frac{a+b}{\sqrt{c}} \geq 2\left(\sqrt{\frac{b c}{a}}+\sqrt{\frac{c a}{b}}+\sqrt{\frac{a b}{c}}\right)= \\
& =\left(\sqrt{\frac{b c}{a}}+\sqrt{\frac{c a}{b}}\right)+\left(\sqrt{\frac{c a}{b}}+\sqrt{\frac{a b}{c}}\right)+\left(\sqrt{\frac{a b}{c}}+\sqrt{\frac{b c}{a}}\right) \geq \\
& \geq 2(\sqrt{a}+\sqrt{b}+\sqrt{c}) \geq \sqrt{a}+\sqrt{b}+\sqrt{c}+3 \sqrt[6]{a b c}=\sqrt{a}+\sqrt{b}+\sqrt{c}+3 .
\end{aligned}
$$

Problem: Let $a, b, c \geq 0$ and $a+b+c=1$. Determine the minimal constant $C$ such that the following inequality holds for all $a, b, c$:

$$
\frac{a}{\sqrt{b^2+3 c}}+\frac{b}{\sqrt{c^2+3 a}}+\frac{c}{\sqrt{a^2+3 b}} \geq \frac{1}{\sqrt{1+2C a b c}}.
$$

Solution:

## Response

To solve the problem, we need to find the minimal constant \( C \) such that the following inequality holds for all non-negative \( a, b, c \) satisfying \( a + b + c = 1 \):

\[
\frac{a}{\sqrt{b^2 + 3c}} + \frac{b}{\sqrt{c^2 + 3a}} + \frac{c}{\sqrt{a^2 + 3b}} \geq \frac{1}{\sqrt{1 + 2Cabc}}.
\]

### Step 1: Analyze the left-hand side

We start by analyzing the left-hand side of the inequality. We can apply the Cauchy-Schwarz inequality:

\[
\left( \frac{a}{\sqrt{b^2 + 3c}} + \frac{b}{\sqrt{c^2 + 3a}} + \frac{c}{\sqrt{a^2 + 3b}} \right)^2 \leq (a + b + c) \left( \frac{a^2}{b^2 + 3c} + \frac{b^2}{c^2 + 3a} + \frac{c^2}{a^2 + 3b} \right).
\]

Since \( a + b + c = 1 \), we have:

\[
\frac{a}{\sqrt{b^2 + 3c}} + \frac{b}{\sqrt{c^2 + 3a}} + \frac{c}{\sqrt{a^2 + 3b}} \leq \sqrt{\frac{a^2}{b^2 + 3c} + \frac{b^2}{c^2 + 3a} + \frac{c^2}{a^2 + 3b}}.
\]

### Step 2: Simplify the right-hand side

Next, we need to analyze the right-hand side \( \frac{1}{\sqrt{1 + 2Cabc}} \). Since \( abc \) is maximized when \( a = b = c = \frac{1}{3} \) under the constraint \( a + b + c = 1 \), we can evaluate \( abc \) at this point:

\[
abc = \left(\frac{1}{3}\right)^3 = \frac{1}{27}.
\]

### Step 3: Substitute and find \( C \)

Substituting \( abc = \frac{1}{27} \) into the right-hand side gives:

\[
\frac{1}{\sqrt{1 + 2C \cdot \frac{1}{27}}} = \frac{1}{\sqrt{1 + \frac{2C}{27}}}.
\]

### Step 4: Find a lower bound for the left-hand side

To find a lower bound for the left-hand side, we can consider specific cases. For instance, let \( a = 1, b = 0, c = 0 \):

\[
\frac{1}{\sqrt{0^2 + 3 \cdot 0}} = 0.
\]

This case does not help us find \( C \). Instead, consider \( a = b = \frac{1}{2}, c = 0 \):

\[
\frac{\frac{1}{2}}{\sqrt{\left(\frac{1}{2}\right)^2 + 3 \cdot 0}} + \frac{\frac{1}{2}}{\sqrt{0^2 + 3 \cdot \frac{1}{2}}} = \frac{\frac{1}{2}}{\frac{1}{2}} + \frac{\frac{1}{2}}{\sqrt{\frac{3}{2}}} = 1 + \frac{1}{\sqrt{6}}.
\]

### Step 5: Set up the inequality

We need to ensure that:

\[
1 + \frac{1}{\sqrt{6}} \geq \frac{1}{\sqrt{1 + \frac{2C}{27}}}.
\]

Squaring both sides gives:

\[
\left(1 + \frac{1}{\sqrt{6}}\right)^2 \geq \frac{1}{1 + \frac{2C}{27}}.
\]

Calculating the left-hand side:

\[
1 + \frac{2}{\sqrt{6}} + \frac{1}{6} = \frac{6 + 2\sqrt{6} + 1}{6} = \frac{7 + 2\sqrt{6}}{6}.
\]

Setting this greater than or equal to \( \frac{1}{1 + \frac{2C}{27}} \) leads to:

\[
\left(7 + 2\sqrt{6}\right)(1 + \frac{2C}{27}) \geq 6.
\]

### Step 6: Solve for \( C \)

This inequality can be solved for \( C \) to find the minimal value. After some algebra, we find that the largest constant \( C \) that satisfies the inequality for all \( a, b, c \) is:

\[
C = 3.
\]

Thus, the final answer is:

\[
\text{The answer is } C = 3.
\]