## Problem

Let $x_1, x_2, \cdots, x_n$ be real numbers in the interval $[-1, 1]$ such that $\sum_{i=1}^{n} x_i^3 = 0$. Find the smallest constant $C$ such that the following inequality holds:
$$
\sum_{i=1}^{n} x_i \leq Cn.
$$

## Query

Task description: Please solve the problem with clear, rigorous, and logically sound steps. At the end of your response, state your answer in exactly this format: 'The answer is $C=X$', where X is your calculated numerical bound value. Example: 'The answer is $C=1$'.



Problem: Let $a, b, c$ be the side lengths, $h_{a}, h_{b}, h_{c}$ be the altitudes, respectively, and $r$ be the inradius of a triangle. Find the largest constant $C$ such that the following inequality holds for all triangles:
$$
\frac{1}{h_{a}-2 r}+\frac{1}{h_{b}-2 r}+\frac{1}{h_{c}-2 r} \geq C \cdot r
$$

Solution: By $\frac{1}{h_{a}}+\frac{1}{h_{b}}+\frac{1}{h_{c}}=\frac{1}{r}$ we obtain
$$
\frac{h_{a}-2 r}{h_{a}}+\frac{h_{b}-2 r}{h_{b}}+\frac{h_{c}-2 r}{h_{c}}=1
$$

Applying $A M \geq H M$ we get
$$
\left(\frac{h_{a}-2 r}{h_{a}}+\frac{h_{b}-2 r}{h_{b}}+\frac{h_{c}-2 r}{h_{c}}\right)\left(\frac{h_{a}}{h_{a}-2 r}+\frac{h_{b}}{h_{b}-2 r}+\frac{h_{c}}{h_{c}-2 r}\right) \geq 9
$$
i.e.
$$
\frac{h_{a}}{h_{a}-2 r}+\frac{h_{b}}{h_{b}-2 r}+\frac{h_{c}}{h_{c}-2 r} \geq 9
$$

Therefore
$$
\begin{aligned}
& \frac{2 r}{h_{a}-2 r}+\frac{2 r}{h_{b}-2 r}+\frac{2 r}{h_{c}-2 r} \\
& \quad=\frac{h_{a}-\left(h_{a}-2 r\right)}{h_{a}-2 r}+\frac{h_{b}-\left(h_{b}-2 r\right)}{h_{b}-2 r}+\frac{h_{c}-\left(h_{c}-2 r\right)}{h_{c}-2 r} \\
& \quad=\frac{h_{a}}{h_{a}-2 r}+\frac{h_{b}}{h_{b}-2 r}+\frac{h_{c}}{h_{c}-2 r}-3 \geq 9-3=6
\end{aligned}
$$
i.e.
$$
\frac{1}{h_{a}-2 r}+\frac{1}{h_{b}-2 r}+\frac{1}{h_{c}-2 r} \geq \frac{3}{r}
$$



Problem: Let $a, b, c$ be positive real numbers such that $a^2 + b^2 + c^2 = 3abc$. Find the largest constant $C$ such that the following inequality holds for all $a, b, c$ satisfying the given constraint:
$$
\frac{a}{b^2 c^2} + \frac{b}{c^2 a^2} + \frac{c}{a^2 b^2} \geq \frac{C}{a+b+c}
$$

Solution: The given inequality is equivalent to
$$
\left(a^{3}+b^{3}+c^{3}\right)(a+b+c) \geq 9 a^{2} b^{2} c^{2}
$$

Applying the Cauchy-Schwarz inequality we have
$$
\left(a^{3}+b^{3}+c^{3}\right)(a+b+c) \geq\left(a^{2}+b^{2}+c^{2}\right)^{2}
$$

Since $a^{2}+b^{2}+c^{2}=3 a b c$ we obtain
$$
\left(a^{3}+b^{3}+c^{3}\right)(a+b+c) \geq\left(a^{2}+b^{2}+c^{2}\right)^{2}=(3 a b c)^{2}=9 a^{2} b^{2} c^{2}
$$

Equality holds if and only if $a=b=c=1$.



Problem: Let $a, b, c$ be positive real numbers such that $a b c = 1$. Find the largest constant $C$ such that the following inequality holds for all $a, b, c$ satisfying the given constraint:
$$
\frac{b+c}{\sqrt{a}}+\frac{c+a}{\sqrt{b}}+\frac{a+b}{\sqrt{c}} \geq \sqrt{a}+\sqrt{b}+\sqrt{c}+C
$$

Solution: [Solution 1]
From the AM-GM Inequality, we have

$$
\begin{aligned}
& \frac{b+c}{\sqrt{a}}+\frac{c+a}{\sqrt{b}}+\frac{a+b}{\sqrt{c}} \geq 2\left(\sqrt{\frac{b c}{a}}+\sqrt{\frac{c a}{b}}+\sqrt{\frac{a b}{c}}\right)= \\
& =\left(\sqrt{\frac{b c}{a}}+\sqrt{\frac{c a}{b}}\right)+\left(\sqrt{\frac{c a}{b}}+\sqrt{\frac{a b}{c}}\right)+\left(\sqrt{\frac{a b}{c}}+\sqrt{\frac{b c}{a}}\right) \geq \\
& \geq 2(\sqrt{a}+\sqrt{b}+\sqrt{c}) \geq \sqrt{a}+\sqrt{b}+\sqrt{c}+3 \sqrt[6]{a b c}=\sqrt{a}+\sqrt{b}+\sqrt{c}+3 .
\end{aligned}
$$

Problem: Let $x_1, x_2, \cdots, x_n$ be real numbers in the interval $[-1, 1]$ such that $\sum_{i=1}^{n} x_i^3 = 0$. Find the smallest constant $C$ such that the following inequality holds:
$$
\sum_{i=1}^{n} x_i \leq Cn.
$$

Solution:

## Response

To solve the problem, we start with the given condition that \( \sum_{i=1}^{n} x_i^3 = 0 \) and the constraint that each \( x_i \) lies in the interval \([-1, 1]\). We want to find the smallest constant \( C \) such that the inequality 

\[
\sum_{i=1}^{n} x_i \leq Cn
\]

holds for all choices of \( x_1, x_2, \ldots, x_n \).

### Step 1: Analyze the condition

The condition \( \sum_{i=1}^{n} x_i^3 = 0 \) implies that the positive and negative contributions of the \( x_i^3 \) terms must balance out. Since \( x_i^3 \) is an increasing function in the interval \([-1, 1]\), this means that if some \( x_i \) are positive, there must be enough negative \( x_i \) to offset their cubes.

### Step 2: Consider extreme cases

To find the smallest \( C \), we can consider extreme cases of \( x_i \):

1. **All \( x_i = 1 \)**: In this case, \( \sum_{i=1}^{n} x_i^3 = n \), which does not satisfy the condition.
2. **All \( x_i = -1 \)**: Similarly, \( \sum_{i=1}^{n} x_i^3 = -n \), which also does not satisfy the condition.
3. **Mixed values**: Consider \( k \) values of \( x_i = 1 \) and \( n-k \) values of \( x_i = -1 \). The condition becomes:
   \[
   k \cdot 1^3 + (n-k)(-1)^3 = k - (n-k) = 2k - n = 0 \implies k = \frac{n}{2}
   \]
   This means we can have \( n/2 \) values of \( 1 \) and \( n/2 \) values of \( -1 \) when \( n \) is even.

### Step 3: Calculate the sum

For \( n \) even, if \( n = 2m \):
\[
\sum_{i=1}^{n} x_i = \frac{n}{2} \cdot 1 + \frac{n}{2} \cdot (-1) = 0
\]

For \( n \) odd, we can have \( (n-1)/2 \) values of \( 1 \) and \( (n+1)/2 \) values of \( -1 \):
\[
\sum_{i=1}^{n} x_i = \frac{n-1}{2} \cdot 1 + \frac{n+1}{2} \cdot (-1) = \frac{n-1 - (n+1)}{2} = -1
\]

### Step 4: Determine \( C \)

In both cases, we find that:
- For even \( n \), \( \sum_{i=1}^{n} x_i = 0 \leq Cn \) for any \( C \geq 0 \).
- For odd \( n \), \( \sum_{i=1}^{n} x_i = -1 \leq Cn \) implies \( C \geq -\frac{1}{n} \).

As \( n \) approaches infinity, the term \( -\frac{1}{n} \) approaches \( 0 \). Therefore, the smallest constant \( C \) that satisfies the inequality for all \( n \) is:

\[
C = 0
\]

### Conclusion

Thus, the smallest constant \( C \) such that the inequality holds for all \( x_1, x_2, \ldots, x_n \) satisfying the given condition is:

\[
\text{The answer is } C=0.
\]