## Problem

Let $a$ and $b$ be non-negative real numbers such that $a \geq b$. Determine the largest constant $C$ such that the following inequality holds for all $a \geq b \geq 0$:
$$
a + \frac{1}{b(a-b)} \geq C.
$$

## Query

Task description: Please solve the problem with clear, rigorous, and logically sound steps. At the end of your response, state your answer in exactly this format: 'The answer is $C=X$', where X is your calculated numerical bound value. Example: 'The answer is $C=1$'.



Problem: Let $a, b, c$ be the side lengths, $h_{a}, h_{b}, h_{c}$ be the altitudes, respectively, and $r$ be the inradius of a triangle. Find the largest constant $C$ such that the following inequality holds for all triangles:
$$
\frac{1}{h_{a}-2 r}+\frac{1}{h_{b}-2 r}+\frac{1}{h_{c}-2 r} \geq C \cdot r
$$

Solution: By $\frac{1}{h_{a}}+\frac{1}{h_{b}}+\frac{1}{h_{c}}=\frac{1}{r}$ we obtain
$$
\frac{h_{a}-2 r}{h_{a}}+\frac{h_{b}-2 r}{h_{b}}+\frac{h_{c}-2 r}{h_{c}}=1
$$

Applying $A M \geq H M$ we get
$$
\left(\frac{h_{a}-2 r}{h_{a}}+\frac{h_{b}-2 r}{h_{b}}+\frac{h_{c}-2 r}{h_{c}}\right)\left(\frac{h_{a}}{h_{a}-2 r}+\frac{h_{b}}{h_{b}-2 r}+\frac{h_{c}}{h_{c}-2 r}\right) \geq 9
$$
i.e.
$$
\frac{h_{a}}{h_{a}-2 r}+\frac{h_{b}}{h_{b}-2 r}+\frac{h_{c}}{h_{c}-2 r} \geq 9
$$

Therefore
$$
\begin{aligned}
& \frac{2 r}{h_{a}-2 r}+\frac{2 r}{h_{b}-2 r}+\frac{2 r}{h_{c}-2 r} \\
& \quad=\frac{h_{a}-\left(h_{a}-2 r\right)}{h_{a}-2 r}+\frac{h_{b}-\left(h_{b}-2 r\right)}{h_{b}-2 r}+\frac{h_{c}-\left(h_{c}-2 r\right)}{h_{c}-2 r} \\
& \quad=\frac{h_{a}}{h_{a}-2 r}+\frac{h_{b}}{h_{b}-2 r}+\frac{h_{c}}{h_{c}-2 r}-3 \geq 9-3=6
\end{aligned}
$$
i.e.
$$
\frac{1}{h_{a}-2 r}+\frac{1}{h_{b}-2 r}+\frac{1}{h_{c}-2 r} \geq \frac{3}{r}
$$



Problem: Let $a, b, c$ be positive real numbers such that $a^2 + b^2 + c^2 = 3abc$. Find the largest constant $C$ such that the following inequality holds for all $a, b, c$ satisfying the given constraint:
$$
\frac{a}{b^2 c^2} + \frac{b}{c^2 a^2} + \frac{c}{a^2 b^2} \geq \frac{C}{a+b+c}
$$

Solution: The given inequality is equivalent to
$$
\left(a^{3}+b^{3}+c^{3}\right)(a+b+c) \geq 9 a^{2} b^{2} c^{2}
$$

Applying the Cauchy-Schwarz inequality we have
$$
\left(a^{3}+b^{3}+c^{3}\right)(a+b+c) \geq\left(a^{2}+b^{2}+c^{2}\right)^{2}
$$

Since $a^{2}+b^{2}+c^{2}=3 a b c$ we obtain
$$
\left(a^{3}+b^{3}+c^{3}\right)(a+b+c) \geq\left(a^{2}+b^{2}+c^{2}\right)^{2}=(3 a b c)^{2}=9 a^{2} b^{2} c^{2}
$$

Equality holds if and only if $a=b=c=1$.



Problem: Let $a, b, c$ be positive real numbers such that $a b c = 1$. Find the largest constant $C$ such that the following inequality holds for all $a, b, c$ satisfying the given constraint:
$$
\frac{b+c}{\sqrt{a}}+\frac{c+a}{\sqrt{b}}+\frac{a+b}{\sqrt{c}} \geq \sqrt{a}+\sqrt{b}+\sqrt{c}+C
$$

Solution: [Solution 1]
From the AM-GM Inequality, we have

$$
\begin{aligned}
& \frac{b+c}{\sqrt{a}}+\frac{c+a}{\sqrt{b}}+\frac{a+b}{\sqrt{c}} \geq 2\left(\sqrt{\frac{b c}{a}}+\sqrt{\frac{c a}{b}}+\sqrt{\frac{a b}{c}}\right)= \\
& =\left(\sqrt{\frac{b c}{a}}+\sqrt{\frac{c a}{b}}\right)+\left(\sqrt{\frac{c a}{b}}+\sqrt{\frac{a b}{c}}\right)+\left(\sqrt{\frac{a b}{c}}+\sqrt{\frac{b c}{a}}\right) \geq \\
& \geq 2(\sqrt{a}+\sqrt{b}+\sqrt{c}) \geq \sqrt{a}+\sqrt{b}+\sqrt{c}+3 \sqrt[6]{a b c}=\sqrt{a}+\sqrt{b}+\sqrt{c}+3 .
\end{aligned}
$$

Problem: Let $a$ and $b$ be non-negative real numbers such that $a \geq b$. Determine the largest constant $C$ such that the following inequality holds for all $a \geq b \geq 0$:
$$
a + \frac{1}{b(a-b)} \geq C.
$$

Solution:

## Response

To solve the inequality 

\[
a + \frac{1}{b(a-b)} \geq C
\]

for non-negative real numbers \(a\) and \(b\) such that \(a \geq b \geq 0\), we will analyze the expression on the left-hand side.

### Step 1: Analyze the expression

We can rewrite the inequality as:

\[
\frac{1}{b(a-b)} \geq C - a.
\]

### Step 2: Consider the case when \(b\) approaches 0

As \(b\) approaches 0, the term \(\frac{1}{b(a-b)}\) approaches infinity if \(a > 0\). Therefore, for any positive \(C\), the inequality will hold for sufficiently small \(b\) as long as \(a > 0\).

### Step 3: Consider the case when \(b = a\)

If we set \(b = a\), then the expression simplifies to:

\[
a + \frac{1}{a(a-a)} = a + \frac{1}{0},
\]

which is undefined. Thus, we need to consider \(b < a\).

### Step 4: Consider the case when \(b\) is a small positive number

Let \(b\) be a small positive number, and we can analyze the limit as \(b\) approaches 0. In this case, we can write:

\[
\frac{1}{b(a-b)} \approx \frac{1}{ba} \quad \text{(as \(b \to 0\))}.
\]

Thus, we have:

\[
a + \frac{1}{ba} \to \infty \quad \text{(as \(b \to 0\))}.
\]

### Step 5: Find a lower bound for \(C\)

To find the largest constant \(C\), we need to consider the case when \(b\) is very small but positive. We can set \(b = 1\) and \(a = 1\) to find a specific value:

\[
1 + \frac{1}{1(1-1)} \text{ is undefined.}
\]

Instead, letâ€™s consider \(b = 1\) and \(a = 2\):

\[
2 + \frac{1}{1(2-1)} = 2 + 1 = 3.
\]

### Step 6: General case

To find the largest constant \(C\), we can analyze the expression more generally. We can set \(b = 1\) and \(a\) to be any value greater than or equal to 1:

\[
a + \frac{1}{1(a-1)}.
\]

As \(a\) increases, the term \(\frac{1}{1(a-1)}\) decreases. The minimum value occurs when \(a\) is at its smallest, which is \(a = 1\):

\[
1 + \frac{1}{1(1-1)} \text{ is undefined.}
\]

However, if we take \(a = 2\) and \(b = 1\):

\[
2 + 1 = 3.
\]

### Conclusion

After analyzing various cases, we find that the largest constant \(C\) that satisfies the inequality for all \(a \geq b \geq 0\) is:

\[
C = 3.
\]

Thus, the final answer is:

\[
\text{The answer is } C=3.
\]