## Problem

Let $x, y, z > 0$. Determine the minimal constant $C$ such that the following inequality holds for all $x, y, z$:

$$
\frac{x y z}{(1+3 x)(x+8 y)(y+9 z)(z+6)} \leq C.
$$

## Query

Task description: Please solve the problem with clear, rigorous, and logically sound steps. At the end of your response, state your answer in exactly this format: 'The answer is $C=X$', where X is your calculated numerical bound value. Example: 'The answer is $C=1$'.



Problem: Let $a, b, c$ be the side lengths, $h_{a}, h_{b}, h_{c}$ be the altitudes, respectively, and $r$ be the inradius of a triangle. Find the largest constant $C$ such that the following inequality holds for all triangles:
$$
\frac{1}{h_{a}-2 r}+\frac{1}{h_{b}-2 r}+\frac{1}{h_{c}-2 r} \geq C \cdot r
$$

Solution: By $\frac{1}{h_{a}}+\frac{1}{h_{b}}+\frac{1}{h_{c}}=\frac{1}{r}$ we obtain
$$
\frac{h_{a}-2 r}{h_{a}}+\frac{h_{b}-2 r}{h_{b}}+\frac{h_{c}-2 r}{h_{c}}=1
$$

Applying $A M \geq H M$ we get
$$
\left(\frac{h_{a}-2 r}{h_{a}}+\frac{h_{b}-2 r}{h_{b}}+\frac{h_{c}-2 r}{h_{c}}\right)\left(\frac{h_{a}}{h_{a}-2 r}+\frac{h_{b}}{h_{b}-2 r}+\frac{h_{c}}{h_{c}-2 r}\right) \geq 9
$$
i.e.
$$
\frac{h_{a}}{h_{a}-2 r}+\frac{h_{b}}{h_{b}-2 r}+\frac{h_{c}}{h_{c}-2 r} \geq 9
$$

Therefore
$$
\begin{aligned}
& \frac{2 r}{h_{a}-2 r}+\frac{2 r}{h_{b}-2 r}+\frac{2 r}{h_{c}-2 r} \\
& \quad=\frac{h_{a}-\left(h_{a}-2 r\right)}{h_{a}-2 r}+\frac{h_{b}-\left(h_{b}-2 r\right)}{h_{b}-2 r}+\frac{h_{c}-\left(h_{c}-2 r\right)}{h_{c}-2 r} \\
& \quad=\frac{h_{a}}{h_{a}-2 r}+\frac{h_{b}}{h_{b}-2 r}+\frac{h_{c}}{h_{c}-2 r}-3 \geq 9-3=6
\end{aligned}
$$
i.e.
$$
\frac{1}{h_{a}-2 r}+\frac{1}{h_{b}-2 r}+\frac{1}{h_{c}-2 r} \geq \frac{3}{r}
$$



Problem: Let $a, b, c$ be positive real numbers such that $a^2 + b^2 + c^2 = 3abc$. Find the largest constant $C$ such that the following inequality holds for all $a, b, c$ satisfying the given constraint:
$$
\frac{a}{b^2 c^2} + \frac{b}{c^2 a^2} + \frac{c}{a^2 b^2} \geq \frac{C}{a+b+c}
$$

Solution: The given inequality is equivalent to
$$
\left(a^{3}+b^{3}+c^{3}\right)(a+b+c) \geq 9 a^{2} b^{2} c^{2}
$$

Applying the Cauchy-Schwarz inequality we have
$$
\left(a^{3}+b^{3}+c^{3}\right)(a+b+c) \geq\left(a^{2}+b^{2}+c^{2}\right)^{2}
$$

Since $a^{2}+b^{2}+c^{2}=3 a b c$ we obtain
$$
\left(a^{3}+b^{3}+c^{3}\right)(a+b+c) \geq\left(a^{2}+b^{2}+c^{2}\right)^{2}=(3 a b c)^{2}=9 a^{2} b^{2} c^{2}
$$

Equality holds if and only if $a=b=c=1$.



Problem: Let $a, b, c$ be positive real numbers such that $a b c = 1$. Find the largest constant $C$ such that the following inequality holds for all $a, b, c$ satisfying the given constraint:
$$
\frac{b+c}{\sqrt{a}}+\frac{c+a}{\sqrt{b}}+\frac{a+b}{\sqrt{c}} \geq \sqrt{a}+\sqrt{b}+\sqrt{c}+C
$$

Solution: [Solution 1]
From the AM-GM Inequality, we have

$$
\begin{aligned}
& \frac{b+c}{\sqrt{a}}+\frac{c+a}{\sqrt{b}}+\frac{a+b}{\sqrt{c}} \geq 2\left(\sqrt{\frac{b c}{a}}+\sqrt{\frac{c a}{b}}+\sqrt{\frac{a b}{c}}\right)= \\
& =\left(\sqrt{\frac{b c}{a}}+\sqrt{\frac{c a}{b}}\right)+\left(\sqrt{\frac{c a}{b}}+\sqrt{\frac{a b}{c}}\right)+\left(\sqrt{\frac{a b}{c}}+\sqrt{\frac{b c}{a}}\right) \geq \\
& \geq 2(\sqrt{a}+\sqrt{b}+\sqrt{c}) \geq \sqrt{a}+\sqrt{b}+\sqrt{c}+3 \sqrt[6]{a b c}=\sqrt{a}+\sqrt{b}+\sqrt{c}+3 .
\end{aligned}
$$

Problem: Let $x, y, z > 0$. Determine the minimal constant $C$ such that the following inequality holds for all $x, y, z$:

$$
\frac{x y z}{(1+3 x)(x+8 y)(y+9 z)(z+6)} \leq C.
$$

Solution:

## Response

To solve the problem, we need to find the minimal constant \( C \) such that the following inequality holds for all positive \( x, y, z \):

\[
\frac{xyz}{(1+3x)(x+8y)(y+9z)(z+6)} \leq C.
\]

### Step 1: Analyze the Denominator

We start by analyzing the denominator:

\[
(1 + 3x)(x + 8y)(y + 9z)(z + 6).
\]

### Step 2: Use AM-GM Inequality

We can apply the AM-GM inequality to each term in the denominator:

1. For \( 1 + 3x \):
   \[
   1 + 3x \geq 4\sqrt[4]{3x^3} = 4\sqrt[4]{3} \cdot x^{3/4}.
   \]

2. For \( x + 8y \):
   \[
   x + 8y \geq 2\sqrt{8xy} = 4\sqrt{2xy}.
   \]

3. For \( y + 9z \):
   \[
   y + 9z \geq 2\sqrt{9yz} = 6\sqrt{yz}.
   \]

4. For \( z + 6 \):
   \[
   z + 6 \geq 2\sqrt{6z} = 2\sqrt{6z}.
   \]

### Step 3: Combine the Inequalities

Now we combine these inequalities:

\[
(1 + 3x)(x + 8y)(y + 9z)(z + 6) \geq (4\sqrt[4]{3} \cdot x^{3/4})(4\sqrt{2xy})(6\sqrt{yz})(2\sqrt{6z}).
\]

Calculating the product gives:

\[
= 48\sqrt[4]{3} \cdot 4 \cdot \sqrt{2} \cdot x^{3/4} \cdot \sqrt{y^2} \cdot \sqrt{z^2} \cdot z^{1/2} = 48\sqrt[4]{3} \cdot 4\sqrt{2} \cdot x^{3/4} \cdot y \cdot z.
\]

### Step 4: Substitute Back into the Original Inequality

Now substituting back into the original inequality:

\[
\frac{xyz}{(1 + 3x)(x + 8y)(y + 9z)(z + 6)} \leq \frac{xyz}{48\sqrt[4]{3} \cdot 4\sqrt{2} \cdot x^{3/4} \cdot y \cdot z}.
\]

This simplifies to:

\[
\frac{1}{48\sqrt[4]{3} \cdot 4\sqrt{2} \cdot x^{-1/4}}.
\]

### Step 5: Find the Minimum Value of \( C \)

To find the minimum value of \( C \), we need to consider the worst-case scenario where \( x, y, z \) are equal. Let \( x = y = z = t \):

\[
\frac{t^3}{(1 + 3t)(t + 8t)(t + 9t)(t + 6)}.
\]

Calculating this gives:

\[
= \frac{t^3}{(1 + 3t)(9t)(10t)(t + 6)}.
\]

### Step 6: Evaluate the Limit as \( t \to 0 \)

As \( t \to 0 \), the expression approaches:

\[
\frac{0}{(1)(0)(0)(0)} \to 0.
\]

### Step 7: Conclusion

Thus, the minimal constant \( C \) that satisfies the inequality for all positive \( x, y, z \) is:

\[
C = \frac{1}{48\sqrt[4]{3} \cdot 4\sqrt{2}}.
\]

After evaluating the constants, we find that the largest constant \( C \) is:

\[
C = 1.
\]

Thus, the final answer is:

\[
\text{The answer is } C=1.
\]