## Problem

Let $x \geq y \geq z \geq 0$. Find the largest constant $C$ such that the following inequality holds for all $x, y, z$:
$$
\frac{x^2 y}{z}+\frac{y^2 z}{x}+\frac{z^2 x}{y} \geq C(x^2+y^2+z^2)
$$

## Query

Task description: Please solve the problem with clear, rigorous, and logically sound steps. At the end of your response, state your answer in exactly this format: 'The answer is $C=X$', where X is your calculated numerical bound value. Example: 'The answer is $C=1$'.



Problem: Let $a, b, c$ be the side lengths, $h_{a}, h_{b}, h_{c}$ be the altitudes, respectively, and $r$ be the inradius of a triangle. Find the largest constant $C$ such that the following inequality holds for all triangles:
$$
\frac{1}{h_{a}-2 r}+\frac{1}{h_{b}-2 r}+\frac{1}{h_{c}-2 r} \geq C \cdot r
$$

Solution: By $\frac{1}{h_{a}}+\frac{1}{h_{b}}+\frac{1}{h_{c}}=\frac{1}{r}$ we obtain
$$
\frac{h_{a}-2 r}{h_{a}}+\frac{h_{b}-2 r}{h_{b}}+\frac{h_{c}-2 r}{h_{c}}=1
$$

Applying $A M \geq H M$ we get
$$
\left(\frac{h_{a}-2 r}{h_{a}}+\frac{h_{b}-2 r}{h_{b}}+\frac{h_{c}-2 r}{h_{c}}\right)\left(\frac{h_{a}}{h_{a}-2 r}+\frac{h_{b}}{h_{b}-2 r}+\frac{h_{c}}{h_{c}-2 r}\right) \geq 9
$$
i.e.
$$
\frac{h_{a}}{h_{a}-2 r}+\frac{h_{b}}{h_{b}-2 r}+\frac{h_{c}}{h_{c}-2 r} \geq 9
$$

Therefore
$$
\begin{aligned}
& \frac{2 r}{h_{a}-2 r}+\frac{2 r}{h_{b}-2 r}+\frac{2 r}{h_{c}-2 r} \\
& \quad=\frac{h_{a}-\left(h_{a}-2 r\right)}{h_{a}-2 r}+\frac{h_{b}-\left(h_{b}-2 r\right)}{h_{b}-2 r}+\frac{h_{c}-\left(h_{c}-2 r\right)}{h_{c}-2 r} \\
& \quad=\frac{h_{a}}{h_{a}-2 r}+\frac{h_{b}}{h_{b}-2 r}+\frac{h_{c}}{h_{c}-2 r}-3 \geq 9-3=6
\end{aligned}
$$
i.e.
$$
\frac{1}{h_{a}-2 r}+\frac{1}{h_{b}-2 r}+\frac{1}{h_{c}-2 r} \geq \frac{3}{r}
$$



Problem: Let $a, b, c$ be positive real numbers such that $a^2 + b^2 + c^2 = 3abc$. Find the largest constant $C$ such that the following inequality holds for all $a, b, c$ satisfying the given constraint:
$$
\frac{a}{b^2 c^2} + \frac{b}{c^2 a^2} + \frac{c}{a^2 b^2} \geq \frac{C}{a+b+c}
$$

Solution: The given inequality is equivalent to
$$
\left(a^{3}+b^{3}+c^{3}\right)(a+b+c) \geq 9 a^{2} b^{2} c^{2}
$$

Applying the Cauchy-Schwarz inequality we have
$$
\left(a^{3}+b^{3}+c^{3}\right)(a+b+c) \geq\left(a^{2}+b^{2}+c^{2}\right)^{2}
$$

Since $a^{2}+b^{2}+c^{2}=3 a b c$ we obtain
$$
\left(a^{3}+b^{3}+c^{3}\right)(a+b+c) \geq\left(a^{2}+b^{2}+c^{2}\right)^{2}=(3 a b c)^{2}=9 a^{2} b^{2} c^{2}
$$

Equality holds if and only if $a=b=c=1$.



Problem: Let $a, b, c$ be positive real numbers such that $a b c = 1$. Find the largest constant $C$ such that the following inequality holds for all $a, b, c$ satisfying the given constraint:
$$
\frac{b+c}{\sqrt{a}}+\frac{c+a}{\sqrt{b}}+\frac{a+b}{\sqrt{c}} \geq \sqrt{a}+\sqrt{b}+\sqrt{c}+C
$$

Solution: [Solution 1]
From the AM-GM Inequality, we have

$$
\begin{aligned}
& \frac{b+c}{\sqrt{a}}+\frac{c+a}{\sqrt{b}}+\frac{a+b}{\sqrt{c}} \geq 2\left(\sqrt{\frac{b c}{a}}+\sqrt{\frac{c a}{b}}+\sqrt{\frac{a b}{c}}\right)= \\
& =\left(\sqrt{\frac{b c}{a}}+\sqrt{\frac{c a}{b}}\right)+\left(\sqrt{\frac{c a}{b}}+\sqrt{\frac{a b}{c}}\right)+\left(\sqrt{\frac{a b}{c}}+\sqrt{\frac{b c}{a}}\right) \geq \\
& \geq 2(\sqrt{a}+\sqrt{b}+\sqrt{c}) \geq \sqrt{a}+\sqrt{b}+\sqrt{c}+3 \sqrt[6]{a b c}=\sqrt{a}+\sqrt{b}+\sqrt{c}+3 .
\end{aligned}
$$

Problem: Let $x \geq y \geq z \geq 0$. Find the largest constant $C$ such that the following inequality holds for all $x, y, z$:
$$
\frac{x^2 y}{z}+\frac{y^2 z}{x}+\frac{z^2 x}{y} \geq C(x^2+y^2+z^2)
$$

Solution:

## Response

To solve the problem, we need to find the largest constant \( C \) such that the following inequality holds for all non-negative \( x, y, z \) with \( x \geq y \geq z \):

\[
\frac{x^2 y}{z} + \frac{y^2 z}{x} + \frac{z^2 x}{y} \geq C(x^2 + y^2 + z^2).
\]

### Step 1: Analyze the inequality

We will analyze the left-hand side of the inequality:

\[
L = \frac{x^2 y}{z} + \frac{y^2 z}{x} + \frac{z^2 x}{y}.
\]

### Step 2: Test specific cases

To find the largest \( C \), we can test specific cases of \( x, y, z \).

#### Case 1: \( x = 1, y = 1, z = 1 \)

\[
L = \frac{1^2 \cdot 1}{1} + \frac{1^2 \cdot 1}{1} + \frac{1^2 \cdot 1}{1} = 3.
\]
\[
x^2 + y^2 + z^2 = 1^2 + 1^2 + 1^2 = 3.
\]
Thus, we have:
\[
3 \geq C \cdot 3 \implies C \leq 1.
\]

#### Case 2: \( x = 1, y = 1, z = 0 \)

\[
L = \frac{1^2 \cdot 1}{0} + \frac{1^2 \cdot 0}{1} + \frac{0^2 \cdot 1}{1} \text{ (undefined)}.
\]
This case is not valid since \( z = 0 \) leads to division by zero.

#### Case 3: \( x = 1, y = 0, z = 0 \)

\[
L = \frac{1^2 \cdot 0}{0} + \frac{0^2 \cdot 0}{1} + \frac{0^2 \cdot 1}{0} \text{ (undefined)}.
\]
This case is also not valid.

#### Case 4: \( x = 2, y = 1, z = 1 \)

\[
L = \frac{2^2 \cdot 1}{1} + \frac{1^2 \cdot 1}{2} + \frac{1^2 \cdot 2}{1} = 4 + \frac{1}{2} + 2 = 6.5.
\]
\[
x^2 + y^2 + z^2 = 2^2 + 1^2 + 1^2 = 4 + 1 + 1 = 6.
\]
Thus, we have:
\[
6.5 \geq C \cdot 6 \implies C \leq \frac{6.5}{6} = \frac{13}{12}.
\]

### Step 3: General case analysis

To find a general bound, we can apply the Cauchy-Schwarz inequality:

\[
\left( \frac{x^2 y}{z} + \frac{y^2 z}{x} + \frac{z^2 x}{y} \right) \left( z + x + y \right) \geq (x + y + z)^3.
\]

This gives us:

\[
\frac{x^2 y}{z} + \frac{y^2 z}{x} + \frac{z^2 x}{y} \geq \frac{(x + y + z)^3}{x + y + z} = (x + y + z)^2.
\]

### Step 4: Relate to \( x^2 + y^2 + z^2 \)

Using the identity \( (x + y + z)^2 = x^2 + y^2 + z^2 + 2(xy + xz + yz) \), we can express:

\[
(x + y + z)^2 \geq \frac{1}{3}(x^2 + y^2 + z^2) + \frac{2}{3}(xy + xz + yz).
\]

### Conclusion

After testing various cases and applying inequalities, we find that the largest constant \( C \) that satisfies the inequality for all non-negative \( x, y, z \) is:

\[
C = 1.
\]

Thus, the final answer is:

\[
\text{The answer is } C=1.
\]