## Problem

Let $0 \leq x \leq 1$ and $n \in \mathbb{N}$. Find the smallest constant $C$ such that the following inequality holds for all $x$ and $n$:
$$
\left(1-x+\frac{x^2}{2}\right)^n-(1-x)^n \leq Cx.
$$

## Query

Task description: Please solve the problem with clear, rigorous, and logically sound steps. At the end of your response, state your answer in exactly this format: 'The answer is $C=X$', where X is your calculated numerical bound value. Example: 'The answer is $C=1$'.



Problem: Let $a, b, c$ be the side lengths, $h_{a}, h_{b}, h_{c}$ be the altitudes, respectively, and $r$ be the inradius of a triangle. Find the largest constant $C$ such that the following inequality holds for all triangles:
$$
\frac{1}{h_{a}-2 r}+\frac{1}{h_{b}-2 r}+\frac{1}{h_{c}-2 r} \geq C \cdot r
$$

Solution: By $\frac{1}{h_{a}}+\frac{1}{h_{b}}+\frac{1}{h_{c}}=\frac{1}{r}$ we obtain
$$
\frac{h_{a}-2 r}{h_{a}}+\frac{h_{b}-2 r}{h_{b}}+\frac{h_{c}-2 r}{h_{c}}=1
$$

Applying $A M \geq H M$ we get
$$
\left(\frac{h_{a}-2 r}{h_{a}}+\frac{h_{b}-2 r}{h_{b}}+\frac{h_{c}-2 r}{h_{c}}\right)\left(\frac{h_{a}}{h_{a}-2 r}+\frac{h_{b}}{h_{b}-2 r}+\frac{h_{c}}{h_{c}-2 r}\right) \geq 9
$$
i.e.
$$
\frac{h_{a}}{h_{a}-2 r}+\frac{h_{b}}{h_{b}-2 r}+\frac{h_{c}}{h_{c}-2 r} \geq 9
$$

Therefore
$$
\begin{aligned}
& \frac{2 r}{h_{a}-2 r}+\frac{2 r}{h_{b}-2 r}+\frac{2 r}{h_{c}-2 r} \\
& \quad=\frac{h_{a}-\left(h_{a}-2 r\right)}{h_{a}-2 r}+\frac{h_{b}-\left(h_{b}-2 r\right)}{h_{b}-2 r}+\frac{h_{c}-\left(h_{c}-2 r\right)}{h_{c}-2 r} \\
& \quad=\frac{h_{a}}{h_{a}-2 r}+\frac{h_{b}}{h_{b}-2 r}+\frac{h_{c}}{h_{c}-2 r}-3 \geq 9-3=6
\end{aligned}
$$
i.e.
$$
\frac{1}{h_{a}-2 r}+\frac{1}{h_{b}-2 r}+\frac{1}{h_{c}-2 r} \geq \frac{3}{r}
$$



Problem: Let $a, b, c$ be positive real numbers such that $a^2 + b^2 + c^2 = 3abc$. Find the largest constant $C$ such that the following inequality holds for all $a, b, c$ satisfying the given constraint:
$$
\frac{a}{b^2 c^2} + \frac{b}{c^2 a^2} + \frac{c}{a^2 b^2} \geq \frac{C}{a+b+c}
$$

Solution: The given inequality is equivalent to
$$
\left(a^{3}+b^{3}+c^{3}\right)(a+b+c) \geq 9 a^{2} b^{2} c^{2}
$$

Applying the Cauchy-Schwarz inequality we have
$$
\left(a^{3}+b^{3}+c^{3}\right)(a+b+c) \geq\left(a^{2}+b^{2}+c^{2}\right)^{2}
$$

Since $a^{2}+b^{2}+c^{2}=3 a b c$ we obtain
$$
\left(a^{3}+b^{3}+c^{3}\right)(a+b+c) \geq\left(a^{2}+b^{2}+c^{2}\right)^{2}=(3 a b c)^{2}=9 a^{2} b^{2} c^{2}
$$

Equality holds if and only if $a=b=c=1$.



Problem: Let $a, b, c$ be positive real numbers such that $a b c = 1$. Find the largest constant $C$ such that the following inequality holds for all $a, b, c$ satisfying the given constraint:
$$
\frac{b+c}{\sqrt{a}}+\frac{c+a}{\sqrt{b}}+\frac{a+b}{\sqrt{c}} \geq \sqrt{a}+\sqrt{b}+\sqrt{c}+C
$$

Solution: [Solution 1]
From the AM-GM Inequality, we have

$$
\begin{aligned}
& \frac{b+c}{\sqrt{a}}+\frac{c+a}{\sqrt{b}}+\frac{a+b}{\sqrt{c}} \geq 2\left(\sqrt{\frac{b c}{a}}+\sqrt{\frac{c a}{b}}+\sqrt{\frac{a b}{c}}\right)= \\
& =\left(\sqrt{\frac{b c}{a}}+\sqrt{\frac{c a}{b}}\right)+\left(\sqrt{\frac{c a}{b}}+\sqrt{\frac{a b}{c}}\right)+\left(\sqrt{\frac{a b}{c}}+\sqrt{\frac{b c}{a}}\right) \geq \\
& \geq 2(\sqrt{a}+\sqrt{b}+\sqrt{c}) \geq \sqrt{a}+\sqrt{b}+\sqrt{c}+3 \sqrt[6]{a b c}=\sqrt{a}+\sqrt{b}+\sqrt{c}+3 .
\end{aligned}
$$

Problem: Let $0 \leq x \leq 1$ and $n \in \mathbb{N}$. Find the smallest constant $C$ such that the following inequality holds for all $x$ and $n$:
$$
\left(1-x+\frac{x^2}{2}\right)^n-(1-x)^n \leq Cx.
$$

Solution:

## Response

To solve the inequality 

\[
\left(1-x+\frac{x^2}{2}\right)^n - (1-x)^n \leq Cx
\]

for \(0 \leq x \leq 1\) and \(n \in \mathbb{N}\), we start by defining the functions involved:

Let 

\[
f(x) = \left(1 - x + \frac{x^2}{2}\right)^n - (1 - x)^n.
\]

We want to find the smallest constant \(C\) such that 

\[
f(x) \leq Cx
\]

for all \(x\) in the interval \([0, 1]\).

### Step 1: Analyze \(f(x)\)

First, we can expand \(f(x)\) using the binomial theorem. The binomial expansion gives us:

\[
(1 - x)^n = \sum_{k=0}^{n} \binom{n}{k} (-x)^k = 1 - nx + \frac{n(n-1)}{2}x^2 - \cdots
\]

Next, we expand \(1 - x + \frac{x^2}{2}\):

\[
1 - x + \frac{x^2}{2} = 1 - x + \frac{x^2}{2}.
\]

Using the binomial theorem again, we have:

\[
\left(1 - x + \frac{x^2}{2}\right)^n = \sum_{k=0}^{n} \binom{n}{k} \left(-x + \frac{x^2}{2}\right)^k.
\]

### Step 2: Calculate \(f(0)\)

At \(x = 0\):

\[
f(0) = \left(1 - 0 + 0\right)^n - (1 - 0)^n = 1 - 1 = 0.
\]

### Step 3: Calculate \(f'(x)\)

To find the behavior of \(f(x)\) as \(x\) increases, we compute the derivative \(f'(x)\):

Using the chain rule and product rule, we differentiate:

\[
f'(x) = n\left(1 - x + \frac{x^2}{2}\right)^{n-1}\left(-1 + x\right) - n(1 - x)^{n-1}(-1).
\]

This simplifies to:

\[
f'(x) = n\left(1 - x + \frac{x^2}{2}\right)^{n-1}\left(-1 + x\right) + n(1 - x)^{n-1}.
\]

### Step 4: Evaluate \(f(x)\) at \(x = 1\)

At \(x = 1\):

\[
f(1) = \left(1 - 1 + \frac{1^2}{2}\right)^n - (1 - 1)^n = \left(\frac{1}{2}\right)^n - 0 = \frac{1}{2^n}.
\]

### Step 5: Find the maximum of \(f(x)\)

To find the maximum value of \(f(x)\) on the interval \([0, 1]\), we need to evaluate \(f(x)\) at critical points and endpoints. 

Since \(f(0) = 0\) and \(f(1) = \frac{1}{2^n}\), we need to check if \(f(x)\) is increasing or decreasing in the interval. 

### Step 6: Determine \(C\)

The maximum value of \(f(x)\) occurs at \(x = 1\), giving us:

\[
f(1) = \frac{1}{2^n}.
\]

Thus, we need:

\[
\frac{1}{2^n} \leq C \cdot 1 \implies C \geq \frac{1}{2^n}.
\]

### Conclusion

The smallest constant \(C\) that satisfies the inequality for all \(x\) in \([0, 1]\) and \(n \in \mathbb{N}\) is:

\[
C = \frac{1}{2^n}.
\]

Thus, the answer is:

\[
\text{The answer is } C = \frac{1}{2^n}.
\]