## Problem

Let $a, b, c > 0$ such that $a+b+c=3$. Determine the largest constant $C$ such that the following inequality holds for all $a, b, c$:

$$
a b c + \frac{17}{a b + b c + c a} \geq C.
$$

## Query

Task description: Please solve the problem with clear, rigorous, and logically sound steps. At the end of your response, state your answer in exactly this format: 'The answer is $C=X$', where X is your calculated numerical bound value. Example: 'The answer is $C=1$'.



Problem: Let $a, b, c$ be the side lengths, $h_{a}, h_{b}, h_{c}$ be the altitudes, respectively, and $r$ be the inradius of a triangle. Find the largest constant $C$ such that the following inequality holds for all triangles:
$$
\frac{1}{h_{a}-2 r}+\frac{1}{h_{b}-2 r}+\frac{1}{h_{c}-2 r} \geq C \cdot r
$$

Solution: By $\frac{1}{h_{a}}+\frac{1}{h_{b}}+\frac{1}{h_{c}}=\frac{1}{r}$ we obtain
$$
\frac{h_{a}-2 r}{h_{a}}+\frac{h_{b}-2 r}{h_{b}}+\frac{h_{c}-2 r}{h_{c}}=1
$$

Applying $A M \geq H M$ we get
$$
\left(\frac{h_{a}-2 r}{h_{a}}+\frac{h_{b}-2 r}{h_{b}}+\frac{h_{c}-2 r}{h_{c}}\right)\left(\frac{h_{a}}{h_{a}-2 r}+\frac{h_{b}}{h_{b}-2 r}+\frac{h_{c}}{h_{c}-2 r}\right) \geq 9
$$
i.e.
$$
\frac{h_{a}}{h_{a}-2 r}+\frac{h_{b}}{h_{b}-2 r}+\frac{h_{c}}{h_{c}-2 r} \geq 9
$$

Therefore
$$
\begin{aligned}
& \frac{2 r}{h_{a}-2 r}+\frac{2 r}{h_{b}-2 r}+\frac{2 r}{h_{c}-2 r} \\
& \quad=\frac{h_{a}-\left(h_{a}-2 r\right)}{h_{a}-2 r}+\frac{h_{b}-\left(h_{b}-2 r\right)}{h_{b}-2 r}+\frac{h_{c}-\left(h_{c}-2 r\right)}{h_{c}-2 r} \\
& \quad=\frac{h_{a}}{h_{a}-2 r}+\frac{h_{b}}{h_{b}-2 r}+\frac{h_{c}}{h_{c}-2 r}-3 \geq 9-3=6
\end{aligned}
$$
i.e.
$$
\frac{1}{h_{a}-2 r}+\frac{1}{h_{b}-2 r}+\frac{1}{h_{c}-2 r} \geq \frac{3}{r}
$$



Problem: Let $a, b, c$ be positive real numbers such that $a^2 + b^2 + c^2 = 3abc$. Find the largest constant $C$ such that the following inequality holds for all $a, b, c$ satisfying the given constraint:
$$
\frac{a}{b^2 c^2} + \frac{b}{c^2 a^2} + \frac{c}{a^2 b^2} \geq \frac{C}{a+b+c}
$$

Solution: The given inequality is equivalent to
$$
\left(a^{3}+b^{3}+c^{3}\right)(a+b+c) \geq 9 a^{2} b^{2} c^{2}
$$

Applying the Cauchy-Schwarz inequality we have
$$
\left(a^{3}+b^{3}+c^{3}\right)(a+b+c) \geq\left(a^{2}+b^{2}+c^{2}\right)^{2}
$$

Since $a^{2}+b^{2}+c^{2}=3 a b c$ we obtain
$$
\left(a^{3}+b^{3}+c^{3}\right)(a+b+c) \geq\left(a^{2}+b^{2}+c^{2}\right)^{2}=(3 a b c)^{2}=9 a^{2} b^{2} c^{2}
$$

Equality holds if and only if $a=b=c=1$.



Problem: Let $a, b, c$ be positive real numbers such that $a b c = 1$. Find the largest constant $C$ such that the following inequality holds for all $a, b, c$ satisfying the given constraint:
$$
\frac{b+c}{\sqrt{a}}+\frac{c+a}{\sqrt{b}}+\frac{a+b}{\sqrt{c}} \geq \sqrt{a}+\sqrt{b}+\sqrt{c}+C
$$

Solution: [Solution 1]
From the AM-GM Inequality, we have

$$
\begin{aligned}
& \frac{b+c}{\sqrt{a}}+\frac{c+a}{\sqrt{b}}+\frac{a+b}{\sqrt{c}} \geq 2\left(\sqrt{\frac{b c}{a}}+\sqrt{\frac{c a}{b}}+\sqrt{\frac{a b}{c}}\right)= \\
& =\left(\sqrt{\frac{b c}{a}}+\sqrt{\frac{c a}{b}}\right)+\left(\sqrt{\frac{c a}{b}}+\sqrt{\frac{a b}{c}}\right)+\left(\sqrt{\frac{a b}{c}}+\sqrt{\frac{b c}{a}}\right) \geq \\
& \geq 2(\sqrt{a}+\sqrt{b}+\sqrt{c}) \geq \sqrt{a}+\sqrt{b}+\sqrt{c}+3 \sqrt[6]{a b c}=\sqrt{a}+\sqrt{b}+\sqrt{c}+3 .
\end{aligned}
$$

Problem: Let $a, b, c > 0$ such that $a+b+c=3$. Determine the largest constant $C$ such that the following inequality holds for all $a, b, c$:

$$
a b c + \frac{17}{a b + b c + c a} \geq C.
$$

Solution:

## Response

To solve the problem, we need to find the largest constant \( C \) such that the inequality 

\[
abc + \frac{17}{ab + bc + ca} \geq C
\]

holds for all positive \( a, b, c \) such that \( a + b + c = 3 \).

### Step 1: Analyze the expression

We start by analyzing the left-hand side of the inequality. We know that \( a, b, c > 0 \) and \( a + b + c = 3 \). 

### Step 2: Use AM-GM Inequality

By the AM-GM inequality, we have:

\[
\frac{a + b + c}{3} \geq \sqrt[3]{abc} \implies 1 \geq \sqrt[3]{abc} \implies abc \leq 1.
\]

### Step 3: Analyze \( ab + bc + ca \)

Using the identity \( (a + b + c)^2 = a^2 + b^2 + c^2 + 2(ab + ac + bc) \), we can express \( ab + ac + bc \):

\[
9 = a^2 + b^2 + c^2 + 2(ab + ac + bc) \implies ab + ac + bc = \frac{9 - (a^2 + b^2 + c^2)}{2}.
\]

Using the Cauchy-Schwarz inequality, we also have:

\[
(a + b + c)^2 \geq 3(ab + ac + bc) \implies 9 \geq 3(ab + ac + bc) \implies ab + ac + bc \leq 3.
\]

### Step 4: Find bounds for \( abc \) and \( ab + ac + bc \)

From the previous steps, we know:

- \( abc \leq 1 \)
- \( ab + ac + bc \leq 3 \)

### Step 5: Substitute values to find \( C \)

To find the largest \( C \), we can test specific values of \( a, b, c \). A natural choice is to set \( a = b = c = 1 \):

\[
abc = 1 \quad \text{and} \quad ab + ac + bc = 3.
\]

Substituting these values into the inequality gives:

\[
1 + \frac{17}{3} \geq C \implies 1 + \frac{17}{3} = \frac{3}{3} + \frac{17}{3} = \frac{20}{3}.
\]

### Step 6: Check if \( C = \frac{20}{3} \) is achievable

Now we need to check if \( C = \frac{20}{3} \) is indeed the largest constant. 

To do this, we can consider the case when \( a, b, c \) are not all equal. For example, let \( a = 2, b = 1, c = 0 \) (which is not allowed since \( c \) must be positive). Instead, we can try \( a = 1.5, b = 1.5, c = 0 \) (again not allowed). 

Instead, we can try \( a = 2, b = 1, c = 0 \) and check the limit as \( c \to 0 \):

\[
abc \to 0 \quad \text{and} \quad ab + ac + bc \to 2.
\]

Thus, we have:

\[
0 + \frac{17}{2} \geq C \implies \frac{17}{2} \geq C.
\]

### Conclusion

The maximum value of \( C \) that satisfies the inequality for all positive \( a, b, c \) such that \( a + b + c = 3 \) is:

\[
C = \frac{20}{3}.
\]

Thus, the final answer is:

\[
\text{The answer is } C = \frac{20}{3}.
\]