## Problem

Let $a, b, c > 0$ satisfy the condition $\sum \frac{1}{a^2+1} = \frac{1}{2}$. Find the smallest constant $C$ such that the following inequality holds for all $a, b, c$:
$$
\sum \frac{1}{a^3+2} \leq C.
$$

## Query

Task description: Please solve the problem with clear, rigorous, and logically sound steps. At the end of your response, state your answer in exactly this format: 'The answer is $C=X$', where X is your calculated numerical bound value. Example: 'The answer is $C=1$'.



Problem: Let $a, b, c$ be the side lengths, $h_{a}, h_{b}, h_{c}$ be the altitudes, respectively, and $r$ be the inradius of a triangle. Find the largest constant $C$ such that the following inequality holds for all triangles:
$$
\frac{1}{h_{a}-2 r}+\frac{1}{h_{b}-2 r}+\frac{1}{h_{c}-2 r} \geq C \cdot r
$$

Solution: By $\frac{1}{h_{a}}+\frac{1}{h_{b}}+\frac{1}{h_{c}}=\frac{1}{r}$ we obtain
$$
\frac{h_{a}-2 r}{h_{a}}+\frac{h_{b}-2 r}{h_{b}}+\frac{h_{c}-2 r}{h_{c}}=1
$$

Applying $A M \geq H M$ we get
$$
\left(\frac{h_{a}-2 r}{h_{a}}+\frac{h_{b}-2 r}{h_{b}}+\frac{h_{c}-2 r}{h_{c}}\right)\left(\frac{h_{a}}{h_{a}-2 r}+\frac{h_{b}}{h_{b}-2 r}+\frac{h_{c}}{h_{c}-2 r}\right) \geq 9
$$
i.e.
$$
\frac{h_{a}}{h_{a}-2 r}+\frac{h_{b}}{h_{b}-2 r}+\frac{h_{c}}{h_{c}-2 r} \geq 9
$$

Therefore
$$
\begin{aligned}
& \frac{2 r}{h_{a}-2 r}+\frac{2 r}{h_{b}-2 r}+\frac{2 r}{h_{c}-2 r} \\
& \quad=\frac{h_{a}-\left(h_{a}-2 r\right)}{h_{a}-2 r}+\frac{h_{b}-\left(h_{b}-2 r\right)}{h_{b}-2 r}+\frac{h_{c}-\left(h_{c}-2 r\right)}{h_{c}-2 r} \\
& \quad=\frac{h_{a}}{h_{a}-2 r}+\frac{h_{b}}{h_{b}-2 r}+\frac{h_{c}}{h_{c}-2 r}-3 \geq 9-3=6
\end{aligned}
$$
i.e.
$$
\frac{1}{h_{a}-2 r}+\frac{1}{h_{b}-2 r}+\frac{1}{h_{c}-2 r} \geq \frac{3}{r}
$$



Problem: Let $a, b, c$ be positive real numbers such that $a^2 + b^2 + c^2 = 3abc$. Find the largest constant $C$ such that the following inequality holds for all $a, b, c$ satisfying the given constraint:
$$
\frac{a}{b^2 c^2} + \frac{b}{c^2 a^2} + \frac{c}{a^2 b^2} \geq \frac{C}{a+b+c}
$$

Solution: The given inequality is equivalent to
$$
\left(a^{3}+b^{3}+c^{3}\right)(a+b+c) \geq 9 a^{2} b^{2} c^{2}
$$

Applying the Cauchy-Schwarz inequality we have
$$
\left(a^{3}+b^{3}+c^{3}\right)(a+b+c) \geq\left(a^{2}+b^{2}+c^{2}\right)^{2}
$$

Since $a^{2}+b^{2}+c^{2}=3 a b c$ we obtain
$$
\left(a^{3}+b^{3}+c^{3}\right)(a+b+c) \geq\left(a^{2}+b^{2}+c^{2}\right)^{2}=(3 a b c)^{2}=9 a^{2} b^{2} c^{2}
$$

Equality holds if and only if $a=b=c=1$.



Problem: Let $a, b, c$ be positive real numbers such that $a b c = 1$. Find the largest constant $C$ such that the following inequality holds for all $a, b, c$ satisfying the given constraint:
$$
\frac{b+c}{\sqrt{a}}+\frac{c+a}{\sqrt{b}}+\frac{a+b}{\sqrt{c}} \geq \sqrt{a}+\sqrt{b}+\sqrt{c}+C
$$

Solution: [Solution 1]
From the AM-GM Inequality, we have

$$
\begin{aligned}
& \frac{b+c}{\sqrt{a}}+\frac{c+a}{\sqrt{b}}+\frac{a+b}{\sqrt{c}} \geq 2\left(\sqrt{\frac{b c}{a}}+\sqrt{\frac{c a}{b}}+\sqrt{\frac{a b}{c}}\right)= \\
& =\left(\sqrt{\frac{b c}{a}}+\sqrt{\frac{c a}{b}}\right)+\left(\sqrt{\frac{c a}{b}}+\sqrt{\frac{a b}{c}}\right)+\left(\sqrt{\frac{a b}{c}}+\sqrt{\frac{b c}{a}}\right) \geq \\
& \geq 2(\sqrt{a}+\sqrt{b}+\sqrt{c}) \geq \sqrt{a}+\sqrt{b}+\sqrt{c}+3 \sqrt[6]{a b c}=\sqrt{a}+\sqrt{b}+\sqrt{c}+3 .
\end{aligned}
$$

Problem: Let $a, b, c > 0$ satisfy the condition $\sum \frac{1}{a^2+1} = \frac{1}{2}$. Find the smallest constant $C$ such that the following inequality holds for all $a, b, c$:
$$
\sum \frac{1}{a^3+2} \leq C.
$$

Solution:

## Response

To solve the problem, we start with the given condition:

\[
\sum \frac{1}{a^2 + 1} = \frac{1}{2}.
\]

We need to find the smallest constant \( C \) such that:

\[
\sum \frac{1}{a^3 + 2} \leq C.
\]

### Step 1: Analyze the function \( f(x) = \frac{1}{x^3 + 2} \)

We will analyze the function \( f(x) = \frac{1}{x^3 + 2} \) to understand its behavior. The function is decreasing for \( x > 0 \) because the derivative \( f'(x) \) is negative:

\[
f'(x) = -\frac{3x^2}{(x^3 + 2)^2} < 0 \quad \text{for } x > 0.
\]

### Step 2: Use the condition to find bounds for \( a, b, c \)

Given the condition \( \sum \frac{1}{a^2 + 1} = \frac{1}{2} \), we can derive bounds for \( a, b, c \). Since \( \frac{1}{a^2 + 1} \) is decreasing, we can apply the Cauchy-Schwarz inequality:

\[
\left( \sum \frac{1}{a^2 + 1} \right) \left( \sum (a^2 + 1) \right) \geq (1 + 1 + 1)^2 = 9.
\]

This gives us:

\[
\frac{1}{2} \left( \sum (a^2 + 1) \right) \geq 9 \implies \sum (a^2 + 1) \geq 18.
\]

Thus,

\[
\sum a^2 \geq 15.
\]

### Step 3: Find \( \sum \frac{1}{a^3 + 2} \)

Now we will estimate \( \sum \frac{1}{a^3 + 2} \). Since \( a^2 \geq 15 \), we can find a lower bound for \( a \):

\[
a^2 \geq 15 \implies a \geq \sqrt{15}.
\]

Now, we can estimate \( a^3 \):

\[
a^3 \geq (\sqrt{15})^3 = 15\sqrt{15}.
\]

Thus,

\[
a^3 + 2 \geq 15\sqrt{15} + 2.
\]

Now we can find \( \frac{1}{a^3 + 2} \):

\[
\frac{1}{a^3 + 2} \leq \frac{1}{15\sqrt{15} + 2}.
\]

### Step 4: Sum the inequalities

Now we can sum over \( a, b, c \):

\[
\sum \frac{1}{a^3 + 2} \leq 3 \cdot \frac{1}{15\sqrt{15} + 2}.
\]

### Step 5: Calculate \( C \)

To find \( C \), we need to evaluate:

\[
C \geq 3 \cdot \frac{1}{15\sqrt{15} + 2}.
\]

Calculating \( 15\sqrt{15} + 2 \):

\[
15\sqrt{15} \approx 15 \cdot 3.872 = 58.08 \implies 15\sqrt{15} + 2 \approx 60.08.
\]

Thus,

\[
\frac{1}{15\sqrt{15} + 2} \approx \frac{1}{60.08} \approx 0.01665.
\]

Therefore,

\[
C \geq 3 \cdot 0.01665 \approx 0.04995.
\]

### Conclusion

The smallest constant \( C \) that satisfies the inequality for all \( a, b, c \) under the given condition is:

\[
C = \frac{3}{60} = \frac{1}{20}.
\]

Thus, the final answer is:

\[
\text{The answer is } C = \frac{1}{20}.
\]