## Problem

Let $x, y, z$ be real numbers such that $x+y+z=xyz$. Find the largest constant $C$ such that the following inequality holds for all $x, y, z$ satisfying the given constraint:
$$
\frac{1}{1+x^2}+\frac{1}{1+y^2}+\frac{1}{1+z^2} \geq C.
$$

## Query

Task description: Please solve the problem with clear, rigorous, and logically sound steps. At the end of your response, state your answer in exactly this format: 'The answer is $C=X$', where X is your calculated numerical bound value. Example: 'The answer is $C=1$'.



Problem: Let $a, b, c$ be the side lengths, $h_{a}, h_{b}, h_{c}$ be the altitudes, respectively, and $r$ be the inradius of a triangle. Find the largest constant $C$ such that the following inequality holds for all triangles:
$$
\frac{1}{h_{a}-2 r}+\frac{1}{h_{b}-2 r}+\frac{1}{h_{c}-2 r} \geq C \cdot r
$$

Solution: By $\frac{1}{h_{a}}+\frac{1}{h_{b}}+\frac{1}{h_{c}}=\frac{1}{r}$ we obtain
$$
\frac{h_{a}-2 r}{h_{a}}+\frac{h_{b}-2 r}{h_{b}}+\frac{h_{c}-2 r}{h_{c}}=1
$$

Applying $A M \geq H M$ we get
$$
\left(\frac{h_{a}-2 r}{h_{a}}+\frac{h_{b}-2 r}{h_{b}}+\frac{h_{c}-2 r}{h_{c}}\right)\left(\frac{h_{a}}{h_{a}-2 r}+\frac{h_{b}}{h_{b}-2 r}+\frac{h_{c}}{h_{c}-2 r}\right) \geq 9
$$
i.e.
$$
\frac{h_{a}}{h_{a}-2 r}+\frac{h_{b}}{h_{b}-2 r}+\frac{h_{c}}{h_{c}-2 r} \geq 9
$$

Therefore
$$
\begin{aligned}
& \frac{2 r}{h_{a}-2 r}+\frac{2 r}{h_{b}-2 r}+\frac{2 r}{h_{c}-2 r} \\
& \quad=\frac{h_{a}-\left(h_{a}-2 r\right)}{h_{a}-2 r}+\frac{h_{b}-\left(h_{b}-2 r\right)}{h_{b}-2 r}+\frac{h_{c}-\left(h_{c}-2 r\right)}{h_{c}-2 r} \\
& \quad=\frac{h_{a}}{h_{a}-2 r}+\frac{h_{b}}{h_{b}-2 r}+\frac{h_{c}}{h_{c}-2 r}-3 \geq 9-3=6
\end{aligned}
$$
i.e.
$$
\frac{1}{h_{a}-2 r}+\frac{1}{h_{b}-2 r}+\frac{1}{h_{c}-2 r} \geq \frac{3}{r}
$$



Problem: Let $a, b, c$ be positive real numbers such that $a^2 + b^2 + c^2 = 3abc$. Find the largest constant $C$ such that the following inequality holds for all $a, b, c$ satisfying the given constraint:
$$
\frac{a}{b^2 c^2} + \frac{b}{c^2 a^2} + \frac{c}{a^2 b^2} \geq \frac{C}{a+b+c}
$$

Solution: The given inequality is equivalent to
$$
\left(a^{3}+b^{3}+c^{3}\right)(a+b+c) \geq 9 a^{2} b^{2} c^{2}
$$

Applying the Cauchy-Schwarz inequality we have
$$
\left(a^{3}+b^{3}+c^{3}\right)(a+b+c) \geq\left(a^{2}+b^{2}+c^{2}\right)^{2}
$$

Since $a^{2}+b^{2}+c^{2}=3 a b c$ we obtain
$$
\left(a^{3}+b^{3}+c^{3}\right)(a+b+c) \geq\left(a^{2}+b^{2}+c^{2}\right)^{2}=(3 a b c)^{2}=9 a^{2} b^{2} c^{2}
$$

Equality holds if and only if $a=b=c=1$.



Problem: Let $a, b, c$ be positive real numbers such that $a b c = 1$. Find the largest constant $C$ such that the following inequality holds for all $a, b, c$ satisfying the given constraint:
$$
\frac{b+c}{\sqrt{a}}+\frac{c+a}{\sqrt{b}}+\frac{a+b}{\sqrt{c}} \geq \sqrt{a}+\sqrt{b}+\sqrt{c}+C
$$

Solution: [Solution 1]
From the AM-GM Inequality, we have

$$
\begin{aligned}
& \frac{b+c}{\sqrt{a}}+\frac{c+a}{\sqrt{b}}+\frac{a+b}{\sqrt{c}} \geq 2\left(\sqrt{\frac{b c}{a}}+\sqrt{\frac{c a}{b}}+\sqrt{\frac{a b}{c}}\right)= \\
& =\left(\sqrt{\frac{b c}{a}}+\sqrt{\frac{c a}{b}}\right)+\left(\sqrt{\frac{c a}{b}}+\sqrt{\frac{a b}{c}}\right)+\left(\sqrt{\frac{a b}{c}}+\sqrt{\frac{b c}{a}}\right) \geq \\
& \geq 2(\sqrt{a}+\sqrt{b}+\sqrt{c}) \geq \sqrt{a}+\sqrt{b}+\sqrt{c}+3 \sqrt[6]{a b c}=\sqrt{a}+\sqrt{b}+\sqrt{c}+3 .
\end{aligned}
$$

Problem: Let $x, y, z$ be real numbers such that $x+y+z=xyz$. Find the largest constant $C$ such that the following inequality holds for all $x, y, z$ satisfying the given constraint:
$$
\frac{1}{1+x^2}+\frac{1}{1+y^2}+\frac{1}{1+z^2} \geq C.
$$

Solution:

## Response

To solve the problem, we start with the condition given: \( x + y + z = xyz \). We want to find the largest constant \( C \) such that the following inequality holds:

\[
\frac{1}{1+x^2} + \frac{1}{1+y^2} + \frac{1}{1+z^2} \geq C.
\]

### Step 1: Analyze the function \( f(t) = \frac{1}{1+t^2} \)

The function \( f(t) \) is decreasing for \( t \geq 0 \) because its derivative \( f'(t) = -\frac{2t}{(1+t^2)^2} \) is negative for \( t > 0 \). This means that larger values of \( t \) will yield smaller values of \( f(t) \).

### Step 2: Use the constraint

Given \( x + y + z = xyz \), we can express \( z \) in terms of \( x \) and \( y \):

\[
z = \frac{x + y}{xy - 1}.
\]

This expression is valid as long as \( xy > 1 \) (to avoid division by zero). 

### Step 3: Consider specific cases

To find the minimum value of the left-hand side, we can consider specific values for \( x, y, z \). A natural choice is to set \( x = y = z \). 

Let \( x = y = z = t \). Then the condition becomes:

\[
3t = t^3 \implies t^3 - 3t = 0 \implies t(t^2 - 3) = 0.
\]

Thus, \( t = 0 \) or \( t = \sqrt{3} \). We discard \( t = 0 \) since it leads to undefined terms in the inequality.

### Step 4: Evaluate the inequality at \( t = \sqrt{3} \)

Substituting \( t = \sqrt{3} \) into the left-hand side:

\[
\frac{1}{1+(\sqrt{3})^2} + \frac{1}{1+(\sqrt{3})^2} + \frac{1}{1+(\sqrt{3})^2} = 3 \cdot \frac{1}{1+3} = 3 \cdot \frac{1}{4} = \frac{3}{4}.
\]

### Step 5: Conclusion

Since we have found that for \( x = y = z = \sqrt{3} \), the left-hand side evaluates to \( \frac{3}{4} \), we can conclude that the largest constant \( C \) such that the inequality holds for all \( x, y, z \) satisfying \( x + y + z = xyz \) is:

\[
C = \frac{3}{4}.
\]

Thus, the final answer is:

The answer is \( C = \frac{3}{4} \).