## Problem

Let $a, b, c \geq 0$ and $a^2 + b + c^2 = 1$. Determine the largest constant $C$ such that the following inequality holds for all $a, b, c$:

$$
\frac{1}{1+a^2} + \frac{6}{5(1+b^2)} + \frac{1}{1+c^2} \geq C.
$$

## Query

Task description: Please solve the problem with clear, rigorous, and logically sound steps. At the end of your response, state your answer in exactly this format: 'The answer is $C=X$', where X is your calculated numerical bound value. Example: 'The answer is $C=1$'.



Problem: Let $a, b, c$ be the side lengths, $h_{a}, h_{b}, h_{c}$ be the altitudes, respectively, and $r$ be the inradius of a triangle. Find the largest constant $C$ such that the following inequality holds for all triangles:
$$
\frac{1}{h_{a}-2 r}+\frac{1}{h_{b}-2 r}+\frac{1}{h_{c}-2 r} \geq C \cdot r
$$

Solution: By $\frac{1}{h_{a}}+\frac{1}{h_{b}}+\frac{1}{h_{c}}=\frac{1}{r}$ we obtain
$$
\frac{h_{a}-2 r}{h_{a}}+\frac{h_{b}-2 r}{h_{b}}+\frac{h_{c}-2 r}{h_{c}}=1
$$

Applying $A M \geq H M$ we get
$$
\left(\frac{h_{a}-2 r}{h_{a}}+\frac{h_{b}-2 r}{h_{b}}+\frac{h_{c}-2 r}{h_{c}}\right)\left(\frac{h_{a}}{h_{a}-2 r}+\frac{h_{b}}{h_{b}-2 r}+\frac{h_{c}}{h_{c}-2 r}\right) \geq 9
$$
i.e.
$$
\frac{h_{a}}{h_{a}-2 r}+\frac{h_{b}}{h_{b}-2 r}+\frac{h_{c}}{h_{c}-2 r} \geq 9
$$

Therefore
$$
\begin{aligned}
& \frac{2 r}{h_{a}-2 r}+\frac{2 r}{h_{b}-2 r}+\frac{2 r}{h_{c}-2 r} \\
& \quad=\frac{h_{a}-\left(h_{a}-2 r\right)}{h_{a}-2 r}+\frac{h_{b}-\left(h_{b}-2 r\right)}{h_{b}-2 r}+\frac{h_{c}-\left(h_{c}-2 r\right)}{h_{c}-2 r} \\
& \quad=\frac{h_{a}}{h_{a}-2 r}+\frac{h_{b}}{h_{b}-2 r}+\frac{h_{c}}{h_{c}-2 r}-3 \geq 9-3=6
\end{aligned}
$$
i.e.
$$
\frac{1}{h_{a}-2 r}+\frac{1}{h_{b}-2 r}+\frac{1}{h_{c}-2 r} \geq \frac{3}{r}
$$



Problem: Let $a, b, c$ be positive real numbers such that $a^2 + b^2 + c^2 = 3abc$. Find the largest constant $C$ such that the following inequality holds for all $a, b, c$ satisfying the given constraint:
$$
\frac{a}{b^2 c^2} + \frac{b}{c^2 a^2} + \frac{c}{a^2 b^2} \geq \frac{C}{a+b+c}
$$

Solution: The given inequality is equivalent to
$$
\left(a^{3}+b^{3}+c^{3}\right)(a+b+c) \geq 9 a^{2} b^{2} c^{2}
$$

Applying the Cauchy-Schwarz inequality we have
$$
\left(a^{3}+b^{3}+c^{3}\right)(a+b+c) \geq\left(a^{2}+b^{2}+c^{2}\right)^{2}
$$

Since $a^{2}+b^{2}+c^{2}=3 a b c$ we obtain
$$
\left(a^{3}+b^{3}+c^{3}\right)(a+b+c) \geq\left(a^{2}+b^{2}+c^{2}\right)^{2}=(3 a b c)^{2}=9 a^{2} b^{2} c^{2}
$$

Equality holds if and only if $a=b=c=1$.



Problem: Let $a, b, c$ be positive real numbers such that $a b c = 1$. Find the largest constant $C$ such that the following inequality holds for all $a, b, c$ satisfying the given constraint:
$$
\frac{b+c}{\sqrt{a}}+\frac{c+a}{\sqrt{b}}+\frac{a+b}{\sqrt{c}} \geq \sqrt{a}+\sqrt{b}+\sqrt{c}+C
$$

Solution: [Solution 1]
From the AM-GM Inequality, we have

$$
\begin{aligned}
& \frac{b+c}{\sqrt{a}}+\frac{c+a}{\sqrt{b}}+\frac{a+b}{\sqrt{c}} \geq 2\left(\sqrt{\frac{b c}{a}}+\sqrt{\frac{c a}{b}}+\sqrt{\frac{a b}{c}}\right)= \\
& =\left(\sqrt{\frac{b c}{a}}+\sqrt{\frac{c a}{b}}\right)+\left(\sqrt{\frac{c a}{b}}+\sqrt{\frac{a b}{c}}\right)+\left(\sqrt{\frac{a b}{c}}+\sqrt{\frac{b c}{a}}\right) \geq \\
& \geq 2(\sqrt{a}+\sqrt{b}+\sqrt{c}) \geq \sqrt{a}+\sqrt{b}+\sqrt{c}+3 \sqrt[6]{a b c}=\sqrt{a}+\sqrt{b}+\sqrt{c}+3 .
\end{aligned}
$$

Problem: Let $a, b, c \geq 0$ and $a^2 + b + c^2 = 1$. Determine the largest constant $C$ such that the following inequality holds for all $a, b, c$:

$$
\frac{1}{1+a^2} + \frac{6}{5(1+b^2)} + \frac{1}{1+c^2} \geq C.
$$

Solution:

## Response

To solve the problem, we need to analyze the inequality 

\[
\frac{1}{1+a^2} + \frac{6}{5(1+b^2)} + \frac{1}{1+c^2} \geq C
\]

given the constraint \( a^2 + b + c^2 = 1 \) for non-negative \( a, b, c \).

### Step 1: Analyze the constraint

From the constraint \( a^2 + b + c^2 = 1 \), we can express \( b \) in terms of \( a \) and \( c \):

\[
b = 1 - a^2 - c^2.
\]

### Step 2: Substitute \( b \) into the inequality

We will substitute \( b \) into the inequality and analyze the behavior of the left-hand side as \( a \) and \( c \) vary.

### Step 3: Consider extreme cases

To find the largest constant \( C \), we can consider some extreme cases for \( a \) and \( c \):

1. **Case 1: \( a = 0, c = 0 \)**

   Then \( b = 1 \):
   \[
   \frac{1}{1+0^2} + \frac{6}{5(1+1^2)} + \frac{1}{1+0^2} = 1 + \frac{6}{10} + 1 = 1 + 0.6 + 1 = 2.6.
   \]

2. **Case 2: \( a = 1, b = 0, c = 0 \)**

   Then \( a^2 + b + c^2 = 1 + 0 + 0 = 1 \):
   \[
   \frac{1}{1+1^2} + \frac{6}{5(1+0^2)} + \frac{1}{1+0^2} = \frac{1}{2} + \frac{6}{5} + 1 = 0.5 + 1.2 + 1 = 2.7.
   \]

3. **Case 3: \( a = 0, b = 0, c = 1 \)**

   Then \( a^2 + b + c^2 = 0 + 0 + 1 = 1 \):
   \[
   \frac{1}{1+0^2} + \frac{6}{5(1+0^2)} + \frac{1}{1+1^2} = 1 + \frac{6}{5} + \frac{1}{2} = 1 + 1.2 + 0.5 = 2.7.
   \]

4. **Case 4: \( a = 0, b = 1, c = 0 \)**

   Then \( a^2 + b + c^2 = 0 + 1 + 0 = 1 \):
   \[
   \frac{1}{1+0^2} + \frac{6}{5(1+1^2)} + \frac{1}{1+0^2} = 1 + \frac{6}{10} + 1 = 1 + 0.6 + 1 = 2.6.
   \]

### Step 4: Determine the maximum value

From the cases analyzed, the maximum value of the left-hand side occurs in Case 2 and Case 3, yielding a value of \( 2.7 \).

### Conclusion

Thus, the largest constant \( C \) such that the inequality holds for all non-negative \( a, b, c \) satisfying \( a^2 + b + c^2 = 1 \) is 

\[
C = 2.7.
\]

Therefore, the final answer is:

The answer is \( C = 2.7 \).