## Problem

Let $a, b, c$ be positive real numbers. Determine the largest constant $C$ such that the following inequality holds for all $a, b, c \in \mathbb{R}^{+}$:
$$
\frac{a}{b+c}+\frac{b}{c+a}+\frac{32}{9}\left(\frac{c}{a+b}\right)^2 \geqslant C.
$$

## Query

Task description: Please solve the problem with clear, rigorous, and logically sound steps. At the end of your response, state your answer in exactly this format: 'The answer is $C=X$', where X is your calculated numerical bound value. Example: 'The answer is $C=1$'.



Problem: Let $a, b, c$ be the side lengths, $h_{a}, h_{b}, h_{c}$ be the altitudes, respectively, and $r$ be the inradius of a triangle. Find the largest constant $C$ such that the following inequality holds for all triangles:
$$
\frac{1}{h_{a}-2 r}+\frac{1}{h_{b}-2 r}+\frac{1}{h_{c}-2 r} \geq C \cdot r
$$

Solution: By $\frac{1}{h_{a}}+\frac{1}{h_{b}}+\frac{1}{h_{c}}=\frac{1}{r}$ we obtain
$$
\frac{h_{a}-2 r}{h_{a}}+\frac{h_{b}-2 r}{h_{b}}+\frac{h_{c}-2 r}{h_{c}}=1
$$

Applying $A M \geq H M$ we get
$$
\left(\frac{h_{a}-2 r}{h_{a}}+\frac{h_{b}-2 r}{h_{b}}+\frac{h_{c}-2 r}{h_{c}}\right)\left(\frac{h_{a}}{h_{a}-2 r}+\frac{h_{b}}{h_{b}-2 r}+\frac{h_{c}}{h_{c}-2 r}\right) \geq 9
$$
i.e.
$$
\frac{h_{a}}{h_{a}-2 r}+\frac{h_{b}}{h_{b}-2 r}+\frac{h_{c}}{h_{c}-2 r} \geq 9
$$

Therefore
$$
\begin{aligned}
& \frac{2 r}{h_{a}-2 r}+\frac{2 r}{h_{b}-2 r}+\frac{2 r}{h_{c}-2 r} \\
& \quad=\frac{h_{a}-\left(h_{a}-2 r\right)}{h_{a}-2 r}+\frac{h_{b}-\left(h_{b}-2 r\right)}{h_{b}-2 r}+\frac{h_{c}-\left(h_{c}-2 r\right)}{h_{c}-2 r} \\
& \quad=\frac{h_{a}}{h_{a}-2 r}+\frac{h_{b}}{h_{b}-2 r}+\frac{h_{c}}{h_{c}-2 r}-3 \geq 9-3=6
\end{aligned}
$$
i.e.
$$
\frac{1}{h_{a}-2 r}+\frac{1}{h_{b}-2 r}+\frac{1}{h_{c}-2 r} \geq \frac{3}{r}
$$



Problem: Let $a, b, c$ be positive real numbers such that $a^2 + b^2 + c^2 = 3abc$. Find the largest constant $C$ such that the following inequality holds for all $a, b, c$ satisfying the given constraint:
$$
\frac{a}{b^2 c^2} + \frac{b}{c^2 a^2} + \frac{c}{a^2 b^2} \geq \frac{C}{a+b+c}
$$

Solution: The given inequality is equivalent to
$$
\left(a^{3}+b^{3}+c^{3}\right)(a+b+c) \geq 9 a^{2} b^{2} c^{2}
$$

Applying the Cauchy-Schwarz inequality we have
$$
\left(a^{3}+b^{3}+c^{3}\right)(a+b+c) \geq\left(a^{2}+b^{2}+c^{2}\right)^{2}
$$

Since $a^{2}+b^{2}+c^{2}=3 a b c$ we obtain
$$
\left(a^{3}+b^{3}+c^{3}\right)(a+b+c) \geq\left(a^{2}+b^{2}+c^{2}\right)^{2}=(3 a b c)^{2}=9 a^{2} b^{2} c^{2}
$$

Equality holds if and only if $a=b=c=1$.



Problem: Let $a, b, c$ be positive real numbers such that $a b c = 1$. Find the largest constant $C$ such that the following inequality holds for all $a, b, c$ satisfying the given constraint:
$$
\frac{b+c}{\sqrt{a}}+\frac{c+a}{\sqrt{b}}+\frac{a+b}{\sqrt{c}} \geq \sqrt{a}+\sqrt{b}+\sqrt{c}+C
$$

Solution: [Solution 1]
From the AM-GM Inequality, we have

$$
\begin{aligned}
& \frac{b+c}{\sqrt{a}}+\frac{c+a}{\sqrt{b}}+\frac{a+b}{\sqrt{c}} \geq 2\left(\sqrt{\frac{b c}{a}}+\sqrt{\frac{c a}{b}}+\sqrt{\frac{a b}{c}}\right)= \\
& =\left(\sqrt{\frac{b c}{a}}+\sqrt{\frac{c a}{b}}\right)+\left(\sqrt{\frac{c a}{b}}+\sqrt{\frac{a b}{c}}\right)+\left(\sqrt{\frac{a b}{c}}+\sqrt{\frac{b c}{a}}\right) \geq \\
& \geq 2(\sqrt{a}+\sqrt{b}+\sqrt{c}) \geq \sqrt{a}+\sqrt{b}+\sqrt{c}+3 \sqrt[6]{a b c}=\sqrt{a}+\sqrt{b}+\sqrt{c}+3 .
\end{aligned}
$$

Problem: Let $a, b, c$ be positive real numbers. Determine the largest constant $C$ such that the following inequality holds for all $a, b, c \in \mathbb{R}^{+}$:
$$
\frac{a}{b+c}+\frac{b}{c+a}+\frac{32}{9}\left(\frac{c}{a+b}\right)^2 \geqslant C.
$$

Solution:

## Response

To solve the problem, we need to analyze the inequality 

\[
\frac{a}{b+c}+\frac{b}{c+a}+\frac{32}{9}\left(\frac{c}{a+b}\right)^2 \geqslant C
\]

for positive real numbers \(a\), \(b\), and \(c\). We will find the largest constant \(C\) such that this inequality holds for all positive \(a\), \(b\), and \(c\).

### Step 1: Analyze the terms

We start by applying the Cauchy-Schwarz inequality to the first two terms:

\[
\frac{a}{b+c} + \frac{b}{c+a} \geq \frac{(a+b)^2}{(b+c)+(c+a)} = \frac{(a+b)^2}{a+b+c}
\]

### Step 2: Simplify the inequality

Now, we rewrite the inequality using the result from Cauchy-Schwarz:

\[
\frac{(a+b)^2}{a+b+c} + \frac{32}{9}\left(\frac{c}{a+b}\right)^2 \geq C
\]

### Step 3: Set \(a = b = c\)

To find a lower bound for the left-hand side, we can set \(a = b = c = 1\):

\[
\frac{1}{1+1} + \frac{1}{1+1} + \frac{32}{9}\left(\frac{1}{1+1}\right)^2 = \frac{1}{2} + \frac{1}{2} + \frac{32}{9}\left(\frac{1}{2}\right)^2
\]

Calculating the last term:

\[
\frac{32}{9} \cdot \frac{1}{4} = \frac{8}{9}
\]

Thus, we have:

\[
1 + \frac{8}{9} = \frac{17}{9}
\]

### Step 4: Determine \(C\)

Since we have shown that for \(a = b = c = 1\):

\[
\frac{a}{b+c} + \frac{b}{c+a} + \frac{32}{9}\left(\frac{c}{a+b}\right)^2 = \frac{17}{9}
\]

This means that the inequality holds with equality when \(C = \frac{17}{9}\).

### Conclusion

To ensure that the inequality holds for all positive \(a\), \(b\), and \(c\), we conclude that the largest constant \(C\) such that the inequality holds is:

\[
\boxed{C = \frac{17}{9}}
\]

Thus, the final answer is:

The answer is \(C=\frac{17}{9}\).