## Problem

Let $a, b, c$ be positive real numbers. Find the largest constant $C$ such that the following inequality holds for all $a, b, c \in \mathbb{R}^{+}$:
$$
\frac{a}{b+C c}+\frac{b}{c+C a}+\frac{c}{a+C b} \geq 1.
$$

## Query

Task description: Please solve the problem with clear, rigorous, and logically sound steps. At the end of your response, state your answer in exactly this format: 'The answer is $C=X$', where X is your calculated numerical bound value. Example: 'The answer is $C=1$'.



Problem: Let $a, b, c$ be the side lengths, $h_{a}, h_{b}, h_{c}$ be the altitudes, respectively, and $r$ be the inradius of a triangle. Find the largest constant $C$ such that the following inequality holds for all triangles:
$$
\frac{1}{h_{a}-2 r}+\frac{1}{h_{b}-2 r}+\frac{1}{h_{c}-2 r} \geq C \cdot r
$$

Solution: By $\frac{1}{h_{a}}+\frac{1}{h_{b}}+\frac{1}{h_{c}}=\frac{1}{r}$ we obtain
$$
\frac{h_{a}-2 r}{h_{a}}+\frac{h_{b}-2 r}{h_{b}}+\frac{h_{c}-2 r}{h_{c}}=1
$$

Applying $A M \geq H M$ we get
$$
\left(\frac{h_{a}-2 r}{h_{a}}+\frac{h_{b}-2 r}{h_{b}}+\frac{h_{c}-2 r}{h_{c}}\right)\left(\frac{h_{a}}{h_{a}-2 r}+\frac{h_{b}}{h_{b}-2 r}+\frac{h_{c}}{h_{c}-2 r}\right) \geq 9
$$
i.e.
$$
\frac{h_{a}}{h_{a}-2 r}+\frac{h_{b}}{h_{b}-2 r}+\frac{h_{c}}{h_{c}-2 r} \geq 9
$$

Therefore
$$
\begin{aligned}
& \frac{2 r}{h_{a}-2 r}+\frac{2 r}{h_{b}-2 r}+\frac{2 r}{h_{c}-2 r} \\
& \quad=\frac{h_{a}-\left(h_{a}-2 r\right)}{h_{a}-2 r}+\frac{h_{b}-\left(h_{b}-2 r\right)}{h_{b}-2 r}+\frac{h_{c}-\left(h_{c}-2 r\right)}{h_{c}-2 r} \\
& \quad=\frac{h_{a}}{h_{a}-2 r}+\frac{h_{b}}{h_{b}-2 r}+\frac{h_{c}}{h_{c}-2 r}-3 \geq 9-3=6
\end{aligned}
$$
i.e.
$$
\frac{1}{h_{a}-2 r}+\frac{1}{h_{b}-2 r}+\frac{1}{h_{c}-2 r} \geq \frac{3}{r}
$$



Problem: Let $a, b, c$ be positive real numbers such that $a^2 + b^2 + c^2 = 3abc$. Find the largest constant $C$ such that the following inequality holds for all $a, b, c$ satisfying the given constraint:
$$
\frac{a}{b^2 c^2} + \frac{b}{c^2 a^2} + \frac{c}{a^2 b^2} \geq \frac{C}{a+b+c}
$$

Solution: The given inequality is equivalent to
$$
\left(a^{3}+b^{3}+c^{3}\right)(a+b+c) \geq 9 a^{2} b^{2} c^{2}
$$

Applying the Cauchy-Schwarz inequality we have
$$
\left(a^{3}+b^{3}+c^{3}\right)(a+b+c) \geq\left(a^{2}+b^{2}+c^{2}\right)^{2}
$$

Since $a^{2}+b^{2}+c^{2}=3 a b c$ we obtain
$$
\left(a^{3}+b^{3}+c^{3}\right)(a+b+c) \geq\left(a^{2}+b^{2}+c^{2}\right)^{2}=(3 a b c)^{2}=9 a^{2} b^{2} c^{2}
$$

Equality holds if and only if $a=b=c=1$.



Problem: Let $a, b, c$ be positive real numbers such that $a b c = 1$. Find the largest constant $C$ such that the following inequality holds for all $a, b, c$ satisfying the given constraint:
$$
\frac{b+c}{\sqrt{a}}+\frac{c+a}{\sqrt{b}}+\frac{a+b}{\sqrt{c}} \geq \sqrt{a}+\sqrt{b}+\sqrt{c}+C
$$

Solution: [Solution 1]
From the AM-GM Inequality, we have

$$
\begin{aligned}
& \frac{b+c}{\sqrt{a}}+\frac{c+a}{\sqrt{b}}+\frac{a+b}{\sqrt{c}} \geq 2\left(\sqrt{\frac{b c}{a}}+\sqrt{\frac{c a}{b}}+\sqrt{\frac{a b}{c}}\right)= \\
& =\left(\sqrt{\frac{b c}{a}}+\sqrt{\frac{c a}{b}}\right)+\left(\sqrt{\frac{c a}{b}}+\sqrt{\frac{a b}{c}}\right)+\left(\sqrt{\frac{a b}{c}}+\sqrt{\frac{b c}{a}}\right) \geq \\
& \geq 2(\sqrt{a}+\sqrt{b}+\sqrt{c}) \geq \sqrt{a}+\sqrt{b}+\sqrt{c}+3 \sqrt[6]{a b c}=\sqrt{a}+\sqrt{b}+\sqrt{c}+3 .
\end{aligned}
$$

Problem: Let $a, b, c$ be positive real numbers. Find the largest constant $C$ such that the following inequality holds for all $a, b, c \in \mathbb{R}^{+}$:
$$
\frac{a}{b+C c}+\frac{b}{c+C a}+\frac{c}{a+C b} \geq 1.
$$

Solution:

## Response

To solve the problem, we need to find the largest constant \( C \) such that the following inequality holds for all positive real numbers \( a, b, c \):

\[
\frac{a}{b + Cc} + \frac{b}{c + Ca} + \frac{c}{a + Cb} \geq 1.
\]

### Step 1: Analyze the inequality

We can use the method of substitution and symmetry. Let's assume \( a = b = c = 1 \). Then the inequality simplifies to:

\[
\frac{1}{1 + C} + \frac{1}{1 + C} + \frac{1}{1 + C} \geq 1.
\]

This simplifies to:

\[
\frac{3}{1 + C} \geq 1.
\]

### Step 2: Solve for \( C \)

From the inequality \( \frac{3}{1 + C} \geq 1 \), we can multiply both sides by \( 1 + C \) (which is positive since \( C \) is a constant and \( a, b, c \) are positive):

\[
3 \geq 1 + C.
\]

Rearranging gives:

\[
C \leq 2.
\]

### Step 3: Check if \( C = 2 \) works

Now we need to check if \( C = 2 \) satisfies the original inequality for all positive \( a, b, c \):

\[
\frac{a}{b + 2c} + \frac{b}{c + 2a} + \frac{c}{a + 2b} \geq 1.
\]

Using Titu's lemma (or Cauchy-Schwarz inequality), we can write:

\[
\frac{a^2}{ab + 2ac} + \frac{b^2}{bc + 2ba} + \frac{c^2}{ca + 2cb} \geq \frac{(a + b + c)^2}{ab + 2ac + bc + 2ba + ca + 2cb}.
\]

The denominator can be simplified as:

\[
ab + bc + ca + 2(ab + ac + bc) = 3(ab + ac + bc).
\]

Thus, we have:

\[
\frac{(a + b + c)^2}{3(ab + ac + bc)}.
\]

By the AM-GM inequality, we know that:

\[
ab + ac + bc \leq \frac{(a + b + c)^2}{3}.
\]

Substituting this into our inequality gives:

\[
\frac{(a + b + c)^2}{3 \cdot \frac{(a + b + c)^2}{3}} = 1.
\]

### Conclusion

Since we have shown that \( C = 2 \) satisfies the inequality, and we found that \( C \) cannot exceed 2, we conclude that the largest constant \( C \) for which the inequality holds for all positive \( a, b, c \) is:

\[
\boxed{2}.
\]

Thus, the final answer is:

The answer is \( C=2 \).