## Problem

Let $a_1, a_2, \ldots, a_n$ be non-negative real numbers such that $\prod a_1 = \lambda^n$. Determine the minimal constant $C$ such that the following inequality holds for all $a_1, a_2, \ldots, a_n$:

$$
\prod_{c y c}\left(a_1^2-a_1+1\right) \geq \sqrt{\left(\frac{1+\lambda^4}{C}\right)^n}.
$$

## Query

Task description: Please solve the problem with clear, rigorous, and logically sound steps. At the end of your response, state your answer in exactly this format: 'The answer is $C=X$', where X is your calculated numerical bound value. Example: 'The answer is $C=1$'.



Problem: Let $a, b, c$ be the side lengths, $h_{a}, h_{b}, h_{c}$ be the altitudes, respectively, and $r$ be the inradius of a triangle. Find the largest constant $C$ such that the following inequality holds for all triangles:
$$
\frac{1}{h_{a}-2 r}+\frac{1}{h_{b}-2 r}+\frac{1}{h_{c}-2 r} \geq C \cdot r
$$

Solution: By $\frac{1}{h_{a}}+\frac{1}{h_{b}}+\frac{1}{h_{c}}=\frac{1}{r}$ we obtain
$$
\frac{h_{a}-2 r}{h_{a}}+\frac{h_{b}-2 r}{h_{b}}+\frac{h_{c}-2 r}{h_{c}}=1
$$

Applying $A M \geq H M$ we get
$$
\left(\frac{h_{a}-2 r}{h_{a}}+\frac{h_{b}-2 r}{h_{b}}+\frac{h_{c}-2 r}{h_{c}}\right)\left(\frac{h_{a}}{h_{a}-2 r}+\frac{h_{b}}{h_{b}-2 r}+\frac{h_{c}}{h_{c}-2 r}\right) \geq 9
$$
i.e.
$$
\frac{h_{a}}{h_{a}-2 r}+\frac{h_{b}}{h_{b}-2 r}+\frac{h_{c}}{h_{c}-2 r} \geq 9
$$

Therefore
$$
\begin{aligned}
& \frac{2 r}{h_{a}-2 r}+\frac{2 r}{h_{b}-2 r}+\frac{2 r}{h_{c}-2 r} \\
& \quad=\frac{h_{a}-\left(h_{a}-2 r\right)}{h_{a}-2 r}+\frac{h_{b}-\left(h_{b}-2 r\right)}{h_{b}-2 r}+\frac{h_{c}-\left(h_{c}-2 r\right)}{h_{c}-2 r} \\
& \quad=\frac{h_{a}}{h_{a}-2 r}+\frac{h_{b}}{h_{b}-2 r}+\frac{h_{c}}{h_{c}-2 r}-3 \geq 9-3=6
\end{aligned}
$$
i.e.
$$
\frac{1}{h_{a}-2 r}+\frac{1}{h_{b}-2 r}+\frac{1}{h_{c}-2 r} \geq \frac{3}{r}
$$



Problem: Let $a, b, c$ be positive real numbers such that $a^2 + b^2 + c^2 = 3abc$. Find the largest constant $C$ such that the following inequality holds for all $a, b, c$ satisfying the given constraint:
$$
\frac{a}{b^2 c^2} + \frac{b}{c^2 a^2} + \frac{c}{a^2 b^2} \geq \frac{C}{a+b+c}
$$

Solution: The given inequality is equivalent to
$$
\left(a^{3}+b^{3}+c^{3}\right)(a+b+c) \geq 9 a^{2} b^{2} c^{2}
$$

Applying the Cauchy-Schwarz inequality we have
$$
\left(a^{3}+b^{3}+c^{3}\right)(a+b+c) \geq\left(a^{2}+b^{2}+c^{2}\right)^{2}
$$

Since $a^{2}+b^{2}+c^{2}=3 a b c$ we obtain
$$
\left(a^{3}+b^{3}+c^{3}\right)(a+b+c) \geq\left(a^{2}+b^{2}+c^{2}\right)^{2}=(3 a b c)^{2}=9 a^{2} b^{2} c^{2}
$$

Equality holds if and only if $a=b=c=1$.



Problem: Let $a, b, c$ be positive real numbers such that $a b c = 1$. Find the largest constant $C$ such that the following inequality holds for all $a, b, c$ satisfying the given constraint:
$$
\frac{b+c}{\sqrt{a}}+\frac{c+a}{\sqrt{b}}+\frac{a+b}{\sqrt{c}} \geq \sqrt{a}+\sqrt{b}+\sqrt{c}+C
$$

Solution: [Solution 1]
From the AM-GM Inequality, we have

$$
\begin{aligned}
& \frac{b+c}{\sqrt{a}}+\frac{c+a}{\sqrt{b}}+\frac{a+b}{\sqrt{c}} \geq 2\left(\sqrt{\frac{b c}{a}}+\sqrt{\frac{c a}{b}}+\sqrt{\frac{a b}{c}}\right)= \\
& =\left(\sqrt{\frac{b c}{a}}+\sqrt{\frac{c a}{b}}\right)+\left(\sqrt{\frac{c a}{b}}+\sqrt{\frac{a b}{c}}\right)+\left(\sqrt{\frac{a b}{c}}+\sqrt{\frac{b c}{a}}\right) \geq \\
& \geq 2(\sqrt{a}+\sqrt{b}+\sqrt{c}) \geq \sqrt{a}+\sqrt{b}+\sqrt{c}+3 \sqrt[6]{a b c}=\sqrt{a}+\sqrt{b}+\sqrt{c}+3 .
\end{aligned}
$$

Problem: Let $a_1, a_2, \ldots, a_n$ be non-negative real numbers such that $\prod a_1 = \lambda^n$. Determine the minimal constant $C$ such that the following inequality holds for all $a_1, a_2, \ldots, a_n$:

$$
\prod_{c y c}\left(a_1^2-a_1+1\right) \geq \sqrt{\left(\frac{1+\lambda^4}{C}\right)^n}.
$$

Solution:

## Response

To solve the problem, we need to analyze the inequality given:

$$
\prod_{i=1}^n (a_i^2 - a_i + 1) \geq \sqrt{\left(\frac{1+\lambda^4}{C}\right)^n}.
$$

We start by rewriting the left-hand side. The expression \( a_i^2 - a_i + 1 \) can be rewritten as:

$$
a_i^2 - a_i + 1 = \left(a_i - \frac{1}{2}\right)^2 + \frac{3}{4}.
$$

This shows that \( a_i^2 - a_i + 1 \) is always positive for all real \( a_i \) and achieves its minimum value of \( \frac{3}{4} \) when \( a_i = \frac{1}{2} \).

Next, we apply the AM-GM inequality to the terms \( a_i^2 - a_i + 1 \):

$$
\prod_{i=1}^n (a_i^2 - a_i + 1) \geq \left( \frac{(a_1^2 - a_1 + 1) + (a_2^2 - a_2 + 1) + \ldots + (a_n^2 - a_n + 1)}{n} \right)^n.
$$

Now, we need to find a suitable expression for the average of \( a_i^2 - a_i + 1 \). We know that:

$$
\sum_{i=1}^n (a_i^2 - a_i + 1) = \sum_{i=1}^n a_i^2 - \sum_{i=1}^n a_i + n.
$$

Using the condition \( \prod_{i=1}^n a_i = \lambda^n \), we can apply the AM-GM inequality to the \( a_i \):

$$
\frac{a_1 + a_2 + \ldots + a_n}{n} \geq \sqrt[n]{\prod_{i=1}^n a_i} = \lambda.
$$

Thus, we have:

$$
\sum_{i=1}^n a_i \geq n\lambda.
$$

Next, we also apply the Cauchy-Schwarz inequality to \( \sum_{i=1}^n a_i^2 \):

$$
\sum_{i=1}^n a_i^2 \geq \frac{(\sum_{i=1}^n a_i)^2}{n} \geq \frac{(n\lambda)^2}{n} = n\lambda^2.
$$

Combining these results, we can express the sum:

$$
\sum_{i=1}^n (a_i^2 - a_i + 1) \geq n\lambda^2 - n\lambda + n = n(\lambda^2 - \lambda + 1).
$$

Thus, we have:

$$
\prod_{i=1}^n (a_i^2 - a_i + 1) \geq \left( \lambda^2 - \lambda + 1 \right)^n.
$$

Now we need to relate this to the right-hand side of the original inequality:

$$
\sqrt{\left(\frac{1+\lambda^4}{C}\right)^n} = \left(\frac{1+\lambda^4}{C}\right)^{n/2}.
$$

Setting the two sides equal gives us:

$$
\left( \lambda^2 - \lambda + 1 \right)^n \geq \left(\frac{1+\lambda^4}{C}\right)^{n/2}.
$$

Taking the \( n \)-th root of both sides, we have:

$$
\lambda^2 - \lambda + 1 \geq \left(\frac{1+\lambda^4}{C}\right)^{1/2}.
$$

Squaring both sides yields:

$$
(\lambda^2 - \lambda + 1)^2 \geq \frac{1+\lambda^4}{C}.
$$

Rearranging gives:

$$
C \geq \frac{1+\lambda^4}{(\lambda^2 - \lambda + 1)^2}.
$$

To find the minimal constant \( C \), we need to minimize the right-hand side. The expression \( \lambda^2 - \lambda + 1 \) achieves its minimum value of \( \frac{3}{4} \) when \( \lambda = \frac{1}{2} \). Substituting \( \lambda = \frac{1}{2} \):

$$
C \geq \frac{1 + \left(\frac{1}{2}\right)^4}{\left(\frac{3}{4}\right)^2} = \frac{1 + \frac{1}{16}}{\frac{9}{16}} = \frac{\frac{17}{16}}{\frac{9}{16}} = \frac{17}{9}.
$$

Thus, the largest constant \( C \) such that the inequality holds for all \( a_1, a_2, \ldots, a_n \) is:

The answer is \( C = \frac{17}{9} \).