## Problem

Let $x, y, z$ be positive numbers such that $xy + yz + zx = 1$. Find the largest constant $C$ such that the following inequality holds for all $x, y, z$ satisfying the given constraint:
$$
\frac{x^3}{1+9y^2zx} + \frac{y^3}{1+9z^2xy} + \frac{z^3}{1+9x^2yz} \geq C(x+y+z)^3
$$

## Query

Task description: Please solve the problem with clear, rigorous, and logically sound steps. At the end of your response, state your answer in exactly this format: 'The answer is $C=X$', where X is your calculated numerical bound value. Example: 'The answer is $C=1$'.



Problem: Let $a, b, c$ be the side lengths, $h_{a}, h_{b}, h_{c}$ be the altitudes, respectively, and $r$ be the inradius of a triangle. Find the largest constant $C$ such that the following inequality holds for all triangles:
$$
\frac{1}{h_{a}-2 r}+\frac{1}{h_{b}-2 r}+\frac{1}{h_{c}-2 r} \geq C \cdot r
$$

Solution: By $\frac{1}{h_{a}}+\frac{1}{h_{b}}+\frac{1}{h_{c}}=\frac{1}{r}$ we obtain
$$
\frac{h_{a}-2 r}{h_{a}}+\frac{h_{b}-2 r}{h_{b}}+\frac{h_{c}-2 r}{h_{c}}=1
$$

Applying $A M \geq H M$ we get
$$
\left(\frac{h_{a}-2 r}{h_{a}}+\frac{h_{b}-2 r}{h_{b}}+\frac{h_{c}-2 r}{h_{c}}\right)\left(\frac{h_{a}}{h_{a}-2 r}+\frac{h_{b}}{h_{b}-2 r}+\frac{h_{c}}{h_{c}-2 r}\right) \geq 9
$$
i.e.
$$
\frac{h_{a}}{h_{a}-2 r}+\frac{h_{b}}{h_{b}-2 r}+\frac{h_{c}}{h_{c}-2 r} \geq 9
$$

Therefore
$$
\begin{aligned}
& \frac{2 r}{h_{a}-2 r}+\frac{2 r}{h_{b}-2 r}+\frac{2 r}{h_{c}-2 r} \\
& \quad=\frac{h_{a}-\left(h_{a}-2 r\right)}{h_{a}-2 r}+\frac{h_{b}-\left(h_{b}-2 r\right)}{h_{b}-2 r}+\frac{h_{c}-\left(h_{c}-2 r\right)}{h_{c}-2 r} \\
& \quad=\frac{h_{a}}{h_{a}-2 r}+\frac{h_{b}}{h_{b}-2 r}+\frac{h_{c}}{h_{c}-2 r}-3 \geq 9-3=6
\end{aligned}
$$
i.e.
$$
\frac{1}{h_{a}-2 r}+\frac{1}{h_{b}-2 r}+\frac{1}{h_{c}-2 r} \geq \frac{3}{r}
$$



Problem: Let $a, b, c$ be positive real numbers such that $a^2 + b^2 + c^2 = 3abc$. Find the largest constant $C$ such that the following inequality holds for all $a, b, c$ satisfying the given constraint:
$$
\frac{a}{b^2 c^2} + \frac{b}{c^2 a^2} + \frac{c}{a^2 b^2} \geq \frac{C}{a+b+c}
$$

Solution: The given inequality is equivalent to
$$
\left(a^{3}+b^{3}+c^{3}\right)(a+b+c) \geq 9 a^{2} b^{2} c^{2}
$$

Applying the Cauchy-Schwarz inequality we have
$$
\left(a^{3}+b^{3}+c^{3}\right)(a+b+c) \geq\left(a^{2}+b^{2}+c^{2}\right)^{2}
$$

Since $a^{2}+b^{2}+c^{2}=3 a b c$ we obtain
$$
\left(a^{3}+b^{3}+c^{3}\right)(a+b+c) \geq\left(a^{2}+b^{2}+c^{2}\right)^{2}=(3 a b c)^{2}=9 a^{2} b^{2} c^{2}
$$

Equality holds if and only if $a=b=c=1$.



Problem: Let $a, b, c$ be positive real numbers such that $a b c = 1$. Find the largest constant $C$ such that the following inequality holds for all $a, b, c$ satisfying the given constraint:
$$
\frac{b+c}{\sqrt{a}}+\frac{c+a}{\sqrt{b}}+\frac{a+b}{\sqrt{c}} \geq \sqrt{a}+\sqrt{b}+\sqrt{c}+C
$$

Solution: [Solution 1]
From the AM-GM Inequality, we have

$$
\begin{aligned}
& \frac{b+c}{\sqrt{a}}+\frac{c+a}{\sqrt{b}}+\frac{a+b}{\sqrt{c}} \geq 2\left(\sqrt{\frac{b c}{a}}+\sqrt{\frac{c a}{b}}+\sqrt{\frac{a b}{c}}\right)= \\
& =\left(\sqrt{\frac{b c}{a}}+\sqrt{\frac{c a}{b}}\right)+\left(\sqrt{\frac{c a}{b}}+\sqrt{\frac{a b}{c}}\right)+\left(\sqrt{\frac{a b}{c}}+\sqrt{\frac{b c}{a}}\right) \geq \\
& \geq 2(\sqrt{a}+\sqrt{b}+\sqrt{c}) \geq \sqrt{a}+\sqrt{b}+\sqrt{c}+3 \sqrt[6]{a b c}=\sqrt{a}+\sqrt{b}+\sqrt{c}+3 .
\end{aligned}
$$

Problem: Let $x, y, z$ be positive numbers such that $xy + yz + zx = 1$. Find the largest constant $C$ such that the following inequality holds for all $x, y, z$ satisfying the given constraint:
$$
\frac{x^3}{1+9y^2zx} + \frac{y^3}{1+9z^2xy} + \frac{z^3}{1+9x^2yz} \geq C(x+y+z)^3
$$

Solution:

## Response

To solve the problem, we need to find the largest constant \( C \) such that the following inequality holds for all positive numbers \( x, y, z \) satisfying \( xy + yz + zx = 1 \):

\[
\frac{x^3}{1+9y^2zx} + \frac{y^3}{1+9z^2xy} + \frac{z^3}{1+9x^2yz} \geq C(x+y+z)^3.
\]

### Step 1: Analyze the Denominator

Given the constraint \( xy + yz + zx = 1 \), we can express \( zx \) in terms of \( y \) and the other variables. Specifically, we can rewrite the denominator:

\[
1 + 9y^2zx = 1 + 9y^2 \cdot \frac{1 - y^2}{y} = 1 + 9y(1 - y^2).
\]

However, for simplicity, we will analyze the inequality directly without substituting.

### Step 2: Apply Cauchy-Schwarz Inequality

We can apply the Cauchy-Schwarz inequality to the left-hand side:

\[
\left( \frac{x^3}{1 + 9y^2zx} + \frac{y^3}{1 + 9z^2xy} + \frac{z^3}{1 + 9x^2yz} \right) \left( (1 + 9y^2zx) + (1 + 9z^2xy) + (1 + 9x^2yz) \right) \geq (x+y+z)^3.
\]

### Step 3: Simplify the Right-Hand Side

The right-hand side simplifies to:

\[
3 + 9(xy^2zx + yz^2xy + zx^2yz).
\]

### Step 4: Establish the Inequality

Thus, we have:

\[
\frac{x^3 + y^3 + z^3}{1 + 9y^2zx} + \frac{y^3 + z^3 + x^3}{1 + 9z^2xy} + \frac{z^3 + x^3 + y^3}{1 + 9x^2yz} \geq C(x+y+z)^3.
\]

### Step 5: Find the Constant \( C \)

To find the largest constant \( C \), we can test specific values of \( x, y, z \). A natural choice is to set \( x = y = z \). 

Let \( x = y = z = t \). Then:

\[
3t^2 = 1 \implies t = \frac{1}{\sqrt{3}}.
\]

Substituting back into the inequality gives:

\[
\frac{3\left(\frac{1}{\sqrt{3}}\right)^3}{1 + 9\left(\frac{1}{\sqrt{3}}\right)^2\left(\frac{1}{\sqrt{3}}\right)^2} = \frac{3 \cdot \frac{1}{3\sqrt{3}}}{1 + 9 \cdot \frac{1}{3} \cdot \frac{1}{3}} = \frac{1}{\sqrt{3}} \cdot \frac{1}{1 + 1} = \frac{1}{2\sqrt{3}}.
\]

The right-hand side becomes:

\[
C \cdot 3\left(\frac{1}{\sqrt{3}}\right)^3 = C \cdot \frac{1}{\sqrt{3}}.
\]

Setting these equal gives:

\[
\frac{1}{2\sqrt{3}} \geq C \cdot \frac{1}{\sqrt{3}} \implies C \leq \frac{1}{2}.
\]

### Conclusion

Thus, the largest constant \( C \) such that the inequality holds for all positive \( x, y, z \) satisfying \( xy + yz + zx = 1 \) is:

\[
\boxed{\frac{1}{2}}.
\]

The answer is \( C = \frac{1}{2} \).