## Problem

Let $a, b, c > 0$. Determine the largest constant $C$ such that the following inequality holds for all $a, b, c$:

$$
\frac{a+b+c}{\sqrt[3]{a b c}}+\frac{8 a b c}{(a+b)(b+c)(c+a)} \geq C.
$$

## Query

Task description: Please solve the problem with clear, rigorous, and logically sound steps. At the end of your response, state your answer in exactly this format: 'The answer is $C=X$', where X is your calculated numerical bound value. Example: 'The answer is $C=1$'.



Problem: Let $a, b, c$ be the side lengths, $h_{a}, h_{b}, h_{c}$ be the altitudes, respectively, and $r$ be the inradius of a triangle. Find the largest constant $C$ such that the following inequality holds for all triangles:
$$
\frac{1}{h_{a}-2 r}+\frac{1}{h_{b}-2 r}+\frac{1}{h_{c}-2 r} \geq C \cdot r
$$

Solution: By $\frac{1}{h_{a}}+\frac{1}{h_{b}}+\frac{1}{h_{c}}=\frac{1}{r}$ we obtain
$$
\frac{h_{a}-2 r}{h_{a}}+\frac{h_{b}-2 r}{h_{b}}+\frac{h_{c}-2 r}{h_{c}}=1
$$

Applying $A M \geq H M$ we get
$$
\left(\frac{h_{a}-2 r}{h_{a}}+\frac{h_{b}-2 r}{h_{b}}+\frac{h_{c}-2 r}{h_{c}}\right)\left(\frac{h_{a}}{h_{a}-2 r}+\frac{h_{b}}{h_{b}-2 r}+\frac{h_{c}}{h_{c}-2 r}\right) \geq 9
$$
i.e.
$$
\frac{h_{a}}{h_{a}-2 r}+\frac{h_{b}}{h_{b}-2 r}+\frac{h_{c}}{h_{c}-2 r} \geq 9
$$

Therefore
$$
\begin{aligned}
& \frac{2 r}{h_{a}-2 r}+\frac{2 r}{h_{b}-2 r}+\frac{2 r}{h_{c}-2 r} \\
& \quad=\frac{h_{a}-\left(h_{a}-2 r\right)}{h_{a}-2 r}+\frac{h_{b}-\left(h_{b}-2 r\right)}{h_{b}-2 r}+\frac{h_{c}-\left(h_{c}-2 r\right)}{h_{c}-2 r} \\
& \quad=\frac{h_{a}}{h_{a}-2 r}+\frac{h_{b}}{h_{b}-2 r}+\frac{h_{c}}{h_{c}-2 r}-3 \geq 9-3=6
\end{aligned}
$$
i.e.
$$
\frac{1}{h_{a}-2 r}+\frac{1}{h_{b}-2 r}+\frac{1}{h_{c}-2 r} \geq \frac{3}{r}
$$



Problem: Let $a, b, c$ be positive real numbers such that $a^2 + b^2 + c^2 = 3abc$. Find the largest constant $C$ such that the following inequality holds for all $a, b, c$ satisfying the given constraint:
$$
\frac{a}{b^2 c^2} + \frac{b}{c^2 a^2} + \frac{c}{a^2 b^2} \geq \frac{C}{a+b+c}
$$

Solution: The given inequality is equivalent to
$$
\left(a^{3}+b^{3}+c^{3}\right)(a+b+c) \geq 9 a^{2} b^{2} c^{2}
$$

Applying the Cauchy-Schwarz inequality we have
$$
\left(a^{3}+b^{3}+c^{3}\right)(a+b+c) \geq\left(a^{2}+b^{2}+c^{2}\right)^{2}
$$

Since $a^{2}+b^{2}+c^{2}=3 a b c$ we obtain
$$
\left(a^{3}+b^{3}+c^{3}\right)(a+b+c) \geq\left(a^{2}+b^{2}+c^{2}\right)^{2}=(3 a b c)^{2}=9 a^{2} b^{2} c^{2}
$$

Equality holds if and only if $a=b=c=1$.



Problem: Let $a, b, c$ be positive real numbers such that $a b c = 1$. Find the largest constant $C$ such that the following inequality holds for all $a, b, c$ satisfying the given constraint:
$$
\frac{b+c}{\sqrt{a}}+\frac{c+a}{\sqrt{b}}+\frac{a+b}{\sqrt{c}} \geq \sqrt{a}+\sqrt{b}+\sqrt{c}+C
$$

Solution: [Solution 1]
From the AM-GM Inequality, we have

$$
\begin{aligned}
& \frac{b+c}{\sqrt{a}}+\frac{c+a}{\sqrt{b}}+\frac{a+b}{\sqrt{c}} \geq 2\left(\sqrt{\frac{b c}{a}}+\sqrt{\frac{c a}{b}}+\sqrt{\frac{a b}{c}}\right)= \\
& =\left(\sqrt{\frac{b c}{a}}+\sqrt{\frac{c a}{b}}\right)+\left(\sqrt{\frac{c a}{b}}+\sqrt{\frac{a b}{c}}\right)+\left(\sqrt{\frac{a b}{c}}+\sqrt{\frac{b c}{a}}\right) \geq \\
& \geq 2(\sqrt{a}+\sqrt{b}+\sqrt{c}) \geq \sqrt{a}+\sqrt{b}+\sqrt{c}+3 \sqrt[6]{a b c}=\sqrt{a}+\sqrt{b}+\sqrt{c}+3 .
\end{aligned}
$$

Problem: Let $a, b, c > 0$. Determine the largest constant $C$ such that the following inequality holds for all $a, b, c$:

$$
\frac{a+b+c}{\sqrt[3]{a b c}}+\frac{8 a b c}{(a+b)(b+c)(c+a)} \geq C.
$$

Solution:

## Response

To solve the problem, we need to analyze the given inequality:

\[
\frac{a+b+c}{\sqrt[3]{abc}} + \frac{8abc}{(a+b)(b+c)(c+a)} \geq C.
\]

### Step 1: Analyze the first term

Using the AM-GM inequality, we have:

\[
\frac{a+b+c}{3} \geq \sqrt[3]{abc} \implies a+b+c \geq 3\sqrt[3]{abc}.
\]

Thus,

\[
\frac{a+b+c}{\sqrt[3]{abc}} \geq 3.
\]

### Step 2: Analyze the second term

Next, we need to analyze the term \(\frac{8abc}{(a+b)(b+c)(c+a)}\). We can use the AM-GM inequality again on the denominators:

\[
(a+b)(b+c)(c+a) \leq \left(\frac{(a+b) + (b+c) + (c+a)}{3}\right)^3 = \left(\frac{2(a+b+c)}{3}\right)^3.
\]

Thus,

\[
(a+b)(b+c)(c+a) \leq \frac{8(a+b+c)^3}{27}.
\]

### Step 3: Substitute the inequality into the second term

Now substituting this into our expression for the second term:

\[
\frac{8abc}{(a+b)(b+c)(c+a)} \geq \frac{8abc}{\frac{8(a+b+c)^3}{27}} = \frac{27abc}{(a+b+c)^3}.
\]

### Step 4: Combine the two terms

Now we combine the two results:

\[
\frac{a+b+c}{\sqrt[3]{abc}} + \frac{8abc}{(a+b)(b+c)(c+a)} \geq 3 + \frac{27abc}{(a+b+c)^3}.
\]

### Step 5: Find the minimum value of the combined expression

To find the largest constant \(C\), we need to analyze the minimum value of the expression \(3 + \frac{27abc}{(a+b+c)^3}\). 

Using the condition \(abc = 1\) (which can be achieved by setting \(a = b = c = 1\)), we have:

\[
\frac{27abc}{(a+b+c)^3} = \frac{27 \cdot 1}{(3)^3} = \frac{27}{27} = 1.
\]

Thus, the minimum value of the left-hand side is:

\[
3 + 1 = 4.
\]

### Conclusion

Therefore, the largest constant \(C\) such that the inequality holds for all positive \(a, b, c\) is:

\[
\boxed{4}.
\]

Thus, we can state the final answer as:

The answer is \(C=4\).