## Problem

Let $a, b, c \geq 0$ such that $a^2+b^2+c^2+abc=4$. Find the smallest constant $C$ such that the following inequality holds for all $a, b, c$ satisfying the given constraint:
$$
a+b+c+\sqrt{\frac{a^2+b^2+c^2}{3}} \leq C
$$

## Query

Task description: Please solve the problem with clear, rigorous, and logically sound steps. At the end of your response, state your answer in exactly this format: 'The answer is $C=X$', where X is your calculated numerical bound value. Example: 'The answer is $C=1$'.



Problem: Let $a, b, c$ be the side lengths, $h_{a}, h_{b}, h_{c}$ be the altitudes, respectively, and $r$ be the inradius of a triangle. Find the largest constant $C$ such that the following inequality holds for all triangles:
$$
\frac{1}{h_{a}-2 r}+\frac{1}{h_{b}-2 r}+\frac{1}{h_{c}-2 r} \geq C \cdot r
$$

Solution: By $\frac{1}{h_{a}}+\frac{1}{h_{b}}+\frac{1}{h_{c}}=\frac{1}{r}$ we obtain
$$
\frac{h_{a}-2 r}{h_{a}}+\frac{h_{b}-2 r}{h_{b}}+\frac{h_{c}-2 r}{h_{c}}=1
$$

Applying $A M \geq H M$ we get
$$
\left(\frac{h_{a}-2 r}{h_{a}}+\frac{h_{b}-2 r}{h_{b}}+\frac{h_{c}-2 r}{h_{c}}\right)\left(\frac{h_{a}}{h_{a}-2 r}+\frac{h_{b}}{h_{b}-2 r}+\frac{h_{c}}{h_{c}-2 r}\right) \geq 9
$$
i.e.
$$
\frac{h_{a}}{h_{a}-2 r}+\frac{h_{b}}{h_{b}-2 r}+\frac{h_{c}}{h_{c}-2 r} \geq 9
$$

Therefore
$$
\begin{aligned}
& \frac{2 r}{h_{a}-2 r}+\frac{2 r}{h_{b}-2 r}+\frac{2 r}{h_{c}-2 r} \\
& \quad=\frac{h_{a}-\left(h_{a}-2 r\right)}{h_{a}-2 r}+\frac{h_{b}-\left(h_{b}-2 r\right)}{h_{b}-2 r}+\frac{h_{c}-\left(h_{c}-2 r\right)}{h_{c}-2 r} \\
& \quad=\frac{h_{a}}{h_{a}-2 r}+\frac{h_{b}}{h_{b}-2 r}+\frac{h_{c}}{h_{c}-2 r}-3 \geq 9-3=6
\end{aligned}
$$
i.e.
$$
\frac{1}{h_{a}-2 r}+\frac{1}{h_{b}-2 r}+\frac{1}{h_{c}-2 r} \geq \frac{3}{r}
$$



Problem: Let $a, b, c$ be positive real numbers such that $a^2 + b^2 + c^2 = 3abc$. Find the largest constant $C$ such that the following inequality holds for all $a, b, c$ satisfying the given constraint:
$$
\frac{a}{b^2 c^2} + \frac{b}{c^2 a^2} + \frac{c}{a^2 b^2} \geq \frac{C}{a+b+c}
$$

Solution: The given inequality is equivalent to
$$
\left(a^{3}+b^{3}+c^{3}\right)(a+b+c) \geq 9 a^{2} b^{2} c^{2}
$$

Applying the Cauchy-Schwarz inequality we have
$$
\left(a^{3}+b^{3}+c^{3}\right)(a+b+c) \geq\left(a^{2}+b^{2}+c^{2}\right)^{2}
$$

Since $a^{2}+b^{2}+c^{2}=3 a b c$ we obtain
$$
\left(a^{3}+b^{3}+c^{3}\right)(a+b+c) \geq\left(a^{2}+b^{2}+c^{2}\right)^{2}=(3 a b c)^{2}=9 a^{2} b^{2} c^{2}
$$

Equality holds if and only if $a=b=c=1$.



Problem: Let $a, b, c$ be positive real numbers such that $a b c = 1$. Find the largest constant $C$ such that the following inequality holds for all $a, b, c$ satisfying the given constraint:
$$
\frac{b+c}{\sqrt{a}}+\frac{c+a}{\sqrt{b}}+\frac{a+b}{\sqrt{c}} \geq \sqrt{a}+\sqrt{b}+\sqrt{c}+C
$$

Solution: [Solution 1]
From the AM-GM Inequality, we have

$$
\begin{aligned}
& \frac{b+c}{\sqrt{a}}+\frac{c+a}{\sqrt{b}}+\frac{a+b}{\sqrt{c}} \geq 2\left(\sqrt{\frac{b c}{a}}+\sqrt{\frac{c a}{b}}+\sqrt{\frac{a b}{c}}\right)= \\
& =\left(\sqrt{\frac{b c}{a}}+\sqrt{\frac{c a}{b}}\right)+\left(\sqrt{\frac{c a}{b}}+\sqrt{\frac{a b}{c}}\right)+\left(\sqrt{\frac{a b}{c}}+\sqrt{\frac{b c}{a}}\right) \geq \\
& \geq 2(\sqrt{a}+\sqrt{b}+\sqrt{c}) \geq \sqrt{a}+\sqrt{b}+\sqrt{c}+3 \sqrt[6]{a b c}=\sqrt{a}+\sqrt{b}+\sqrt{c}+3 .
\end{aligned}
$$

Problem: Let $a, b, c \geq 0$ such that $a^2+b^2+c^2+abc=4$. Find the smallest constant $C$ such that the following inequality holds for all $a, b, c$ satisfying the given constraint:
$$
a+b+c+\sqrt{\frac{a^2+b^2+c^2}{3}} \leq C
$$

Solution:

## Response

To solve the problem, we start with the given constraint:

\[
a^2 + b^2 + c^2 + abc = 4.
\]

We need to find the smallest constant \( C \) such that the following inequality holds for all non-negative \( a, b, c \):

\[
a + b + c + \sqrt{\frac{a^2 + b^2 + c^2}{3}} \leq C.
\]

### Step 1: Analyze the constraint

From the constraint \( a^2 + b^2 + c^2 + abc = 4 \), we can express \( a^2 + b^2 + c^2 \) as:

\[
a^2 + b^2 + c^2 = 4 - abc.
\]

### Step 2: Substitute into the inequality

Substituting this into the inequality we want to analyze gives:

\[
a + b + c + \sqrt{\frac{4 - abc}{3}} \leq C.
\]

### Step 3: Find bounds for \( a + b + c \)

To find a suitable bound for \( a + b + c \), we can use the method of Lagrange multipliers or test specific cases. However, we can also use the AM-GM inequality to find a relationship between \( a + b + c \) and \( abc \).

### Step 4: Test specific cases

1. **Case 1: \( a = b = c = 1 \)**

   In this case, we have:

   \[
   a^2 + b^2 + c^2 = 1^2 + 1^2 + 1^2 = 3,
   \]
   and
   \[
   abc = 1 \cdot 1 \cdot 1 = 1.
   \]
   Thus, the constraint holds:

   \[
   3 + 1 = 4.
   \]

   Now, we compute:

   \[
   a + b + c + \sqrt{\frac{a^2 + b^2 + c^2}{3}} = 1 + 1 + 1 + \sqrt{\frac{3}{3}} = 3 + 1 = 4.
   \]

2. **Case 2: \( a = 2, b = 0, c = 0 \)**

   Here, we have:

   \[
   a^2 + b^2 + c^2 = 2^2 + 0^2 + 0^2 = 4,
   \]
   and
   \[
   abc = 2 \cdot 0 \cdot 0 = 0.
   \]
   Thus, the constraint holds:

   \[
   4 + 0 = 4.
   \]

   Now, we compute:

   \[
   a + b + c + \sqrt{\frac{a^2 + b^2 + c^2}{3}} = 2 + 0 + 0 + \sqrt{\frac{4}{3}} = 2 + \frac{2}{\sqrt{3}}.
   \]

   The value \( 2 + \frac{2}{\sqrt{3}} \) is approximately \( 2 + 1.1547 \approx 3.1547 \).

### Step 5: Find the maximum value

From the two cases, we see that the maximum value of \( a + b + c + \sqrt{\frac{a^2 + b^2 + c^2}{3}} \) occurs when \( a = b = c = 1 \), yielding a total of \( 4 \).

### Conclusion

Thus, the smallest constant \( C \) such that the inequality holds for all non-negative \( a, b, c \) satisfying the constraint is:

\[
C = 4.
\]

Therefore, the final answer is:

\[
\text{The answer is } C=4.
\]