## Problem

Find the smallest constant $C$ such that for all real numbers $x$ and $y$, the following inequality holds:
$$
x^2 + x + y^2 + y + C \geq x y
$$

## Query

Task description: Please solve the problem with clear, rigorous, and logically sound steps. At the end of your response, state your answer in exactly this format: 'The answer is $C=X$', where X is your calculated numerical bound value. Example: 'The answer is $C=1$'.



Problem: Let $a, b, c$ be the side lengths, $h_{a}, h_{b}, h_{c}$ be the altitudes, respectively, and $r$ be the inradius of a triangle. Find the largest constant $C$ such that the following inequality holds for all triangles:
$$
\frac{1}{h_{a}-2 r}+\frac{1}{h_{b}-2 r}+\frac{1}{h_{c}-2 r} \geq C \cdot r
$$

Solution: By $\frac{1}{h_{a}}+\frac{1}{h_{b}}+\frac{1}{h_{c}}=\frac{1}{r}$ we obtain
$$
\frac{h_{a}-2 r}{h_{a}}+\frac{h_{b}-2 r}{h_{b}}+\frac{h_{c}-2 r}{h_{c}}=1
$$

Applying $A M \geq H M$ we get
$$
\left(\frac{h_{a}-2 r}{h_{a}}+\frac{h_{b}-2 r}{h_{b}}+\frac{h_{c}-2 r}{h_{c}}\right)\left(\frac{h_{a}}{h_{a}-2 r}+\frac{h_{b}}{h_{b}-2 r}+\frac{h_{c}}{h_{c}-2 r}\right) \geq 9
$$
i.e.
$$
\frac{h_{a}}{h_{a}-2 r}+\frac{h_{b}}{h_{b}-2 r}+\frac{h_{c}}{h_{c}-2 r} \geq 9
$$

Therefore
$$
\begin{aligned}
& \frac{2 r}{h_{a}-2 r}+\frac{2 r}{h_{b}-2 r}+\frac{2 r}{h_{c}-2 r} \\
& \quad=\frac{h_{a}-\left(h_{a}-2 r\right)}{h_{a}-2 r}+\frac{h_{b}-\left(h_{b}-2 r\right)}{h_{b}-2 r}+\frac{h_{c}-\left(h_{c}-2 r\right)}{h_{c}-2 r} \\
& \quad=\frac{h_{a}}{h_{a}-2 r}+\frac{h_{b}}{h_{b}-2 r}+\frac{h_{c}}{h_{c}-2 r}-3 \geq 9-3=6
\end{aligned}
$$
i.e.
$$
\frac{1}{h_{a}-2 r}+\frac{1}{h_{b}-2 r}+\frac{1}{h_{c}-2 r} \geq \frac{3}{r}
$$



Problem: Let $a, b, c$ be positive real numbers such that $a^2 + b^2 + c^2 = 3abc$. Find the largest constant $C$ such that the following inequality holds for all $a, b, c$ satisfying the given constraint:
$$
\frac{a}{b^2 c^2} + \frac{b}{c^2 a^2} + \frac{c}{a^2 b^2} \geq \frac{C}{a+b+c}
$$

Solution: The given inequality is equivalent to
$$
\left(a^{3}+b^{3}+c^{3}\right)(a+b+c) \geq 9 a^{2} b^{2} c^{2}
$$

Applying the Cauchy-Schwarz inequality we have
$$
\left(a^{3}+b^{3}+c^{3}\right)(a+b+c) \geq\left(a^{2}+b^{2}+c^{2}\right)^{2}
$$

Since $a^{2}+b^{2}+c^{2}=3 a b c$ we obtain
$$
\left(a^{3}+b^{3}+c^{3}\right)(a+b+c) \geq\left(a^{2}+b^{2}+c^{2}\right)^{2}=(3 a b c)^{2}=9 a^{2} b^{2} c^{2}
$$

Equality holds if and only if $a=b=c=1$.



Problem: Let $a, b, c$ be positive real numbers such that $a b c = 1$. Find the largest constant $C$ such that the following inequality holds for all $a, b, c$ satisfying the given constraint:
$$
\frac{b+c}{\sqrt{a}}+\frac{c+a}{\sqrt{b}}+\frac{a+b}{\sqrt{c}} \geq \sqrt{a}+\sqrt{b}+\sqrt{c}+C
$$

Solution: [Solution 1]
From the AM-GM Inequality, we have

$$
\begin{aligned}
& \frac{b+c}{\sqrt{a}}+\frac{c+a}{\sqrt{b}}+\frac{a+b}{\sqrt{c}} \geq 2\left(\sqrt{\frac{b c}{a}}+\sqrt{\frac{c a}{b}}+\sqrt{\frac{a b}{c}}\right)= \\
& =\left(\sqrt{\frac{b c}{a}}+\sqrt{\frac{c a}{b}}\right)+\left(\sqrt{\frac{c a}{b}}+\sqrt{\frac{a b}{c}}\right)+\left(\sqrt{\frac{a b}{c}}+\sqrt{\frac{b c}{a}}\right) \geq \\
& \geq 2(\sqrt{a}+\sqrt{b}+\sqrt{c}) \geq \sqrt{a}+\sqrt{b}+\sqrt{c}+3 \sqrt[6]{a b c}=\sqrt{a}+\sqrt{b}+\sqrt{c}+3 .
\end{aligned}
$$

Problem: Find the smallest constant $C$ such that for all real numbers $x$ and $y$, the following inequality holds:
$$
x^2 + x + y^2 + y + C \geq x y
$$

Solution:

## Response

To find the smallest constant \( C \) such that the inequality 

\[
x^2 + x + y^2 + y + C \geq xy
\]

holds for all real numbers \( x \) and \( y \), we can rearrange the inequality as follows:

\[
x^2 - xy + y^2 + x + y + C \geq 0.
\]

This is a quadratic in \( x \):

\[
x^2 - xy + (y^2 + x + y + C) \geq 0.
\]

For this quadratic to be non-negative for all \( x \), the discriminant must be non-positive. The discriminant \( D \) of the quadratic \( ax^2 + bx + c \) is given by \( D = b^2 - 4ac \). Here, we have:

- \( a = 1 \)
- \( b = -y \)
- \( c = y^2 + x + y + C \)

Thus, the discriminant is:

\[
D = (-y)^2 - 4 \cdot 1 \cdot (y^2 + x + y + C) = y^2 - 4(y^2 + x + y + C).
\]

Simplifying this gives:

\[
D = y^2 - 4y^2 - 4x - 4y - 4C = -3y^2 - 4x - 4y - 4C.
\]

For the quadratic to be non-negative for all \( x \), we need \( D \leq 0 \):

\[
-3y^2 - 4x - 4y - 4C \leq 0.
\]

This must hold for all \( x \) and \( y \). To ensure this, we can analyze the case when \( y = 0 \):

\[
-4x - 4C \leq 0 \implies x + C \geq 0 \implies C \geq -x.
\]

Since \( x \) can be any real number, we need \( C \) to be at least \( 0 \) to satisfy this for all \( x \).

Next, we can analyze the case when \( y = 1 \):

\[
-3(1)^2 - 4x - 4(1) - 4C \leq 0 \implies -3 - 4x - 4 - 4C \leq 0 \implies -4x - 4C \leq 7.
\]

This gives us:

\[
C \leq -x + \frac{7}{4}.
\]

To find the smallest \( C \), we can set \( C = 0 \) and check if the inequality holds:

\[
x^2 + x + y^2 + y \geq xy.
\]

Rearranging gives:

\[
x^2 - xy + y^2 + x + y \geq 0.
\]

This is equivalent to:

\[
(x - \frac{y}{2})^2 + (y + \frac{1}{2})^2 \geq \frac{1}{4} \geq 0,
\]

which is always true.

Thus, the smallest constant \( C \) such that the inequality holds for all real numbers \( x \) and \( y \) is:

\[
\boxed{0}.
\]

The answer is \( C = 0 \).