## Problem

Let $x, y, z \in [0,1]$. Determine the minimal constant $C$ such that the following inequality holds for all $x, y, z$:
$$
x(x-y)(z-x) \leq C.
$$

## Query

Task description: Please solve the problem with clear, rigorous, and logically sound steps. At the end of your response, state your answer in exactly this format: 'The answer is $C=X$', where X is your calculated numerical bound value. Example: 'The answer is $C=1$'.



Problem: Let $a, b, c$ be the side lengths, $h_{a}, h_{b}, h_{c}$ be the altitudes, respectively, and $r$ be the inradius of a triangle. Find the largest constant $C$ such that the following inequality holds for all triangles:
$$
\frac{1}{h_{a}-2 r}+\frac{1}{h_{b}-2 r}+\frac{1}{h_{c}-2 r} \geq C \cdot r
$$

Solution: By $\frac{1}{h_{a}}+\frac{1}{h_{b}}+\frac{1}{h_{c}}=\frac{1}{r}$ we obtain
$$
\frac{h_{a}-2 r}{h_{a}}+\frac{h_{b}-2 r}{h_{b}}+\frac{h_{c}-2 r}{h_{c}}=1
$$

Applying $A M \geq H M$ we get
$$
\left(\frac{h_{a}-2 r}{h_{a}}+\frac{h_{b}-2 r}{h_{b}}+\frac{h_{c}-2 r}{h_{c}}\right)\left(\frac{h_{a}}{h_{a}-2 r}+\frac{h_{b}}{h_{b}-2 r}+\frac{h_{c}}{h_{c}-2 r}\right) \geq 9
$$
i.e.
$$
\frac{h_{a}}{h_{a}-2 r}+\frac{h_{b}}{h_{b}-2 r}+\frac{h_{c}}{h_{c}-2 r} \geq 9
$$

Therefore
$$
\begin{aligned}
& \frac{2 r}{h_{a}-2 r}+\frac{2 r}{h_{b}-2 r}+\frac{2 r}{h_{c}-2 r} \\
& \quad=\frac{h_{a}-\left(h_{a}-2 r\right)}{h_{a}-2 r}+\frac{h_{b}-\left(h_{b}-2 r\right)}{h_{b}-2 r}+\frac{h_{c}-\left(h_{c}-2 r\right)}{h_{c}-2 r} \\
& \quad=\frac{h_{a}}{h_{a}-2 r}+\frac{h_{b}}{h_{b}-2 r}+\frac{h_{c}}{h_{c}-2 r}-3 \geq 9-3=6
\end{aligned}
$$
i.e.
$$
\frac{1}{h_{a}-2 r}+\frac{1}{h_{b}-2 r}+\frac{1}{h_{c}-2 r} \geq \frac{3}{r}
$$



Problem: Let $a, b, c$ be positive real numbers such that $a^2 + b^2 + c^2 = 3abc$. Find the largest constant $C$ such that the following inequality holds for all $a, b, c$ satisfying the given constraint:
$$
\frac{a}{b^2 c^2} + \frac{b}{c^2 a^2} + \frac{c}{a^2 b^2} \geq \frac{C}{a+b+c}
$$

Solution: The given inequality is equivalent to
$$
\left(a^{3}+b^{3}+c^{3}\right)(a+b+c) \geq 9 a^{2} b^{2} c^{2}
$$

Applying the Cauchy-Schwarz inequality we have
$$
\left(a^{3}+b^{3}+c^{3}\right)(a+b+c) \geq\left(a^{2}+b^{2}+c^{2}\right)^{2}
$$

Since $a^{2}+b^{2}+c^{2}=3 a b c$ we obtain
$$
\left(a^{3}+b^{3}+c^{3}\right)(a+b+c) \geq\left(a^{2}+b^{2}+c^{2}\right)^{2}=(3 a b c)^{2}=9 a^{2} b^{2} c^{2}
$$

Equality holds if and only if $a=b=c=1$.



Problem: Let $a, b, c$ be positive real numbers such that $a b c = 1$. Find the largest constant $C$ such that the following inequality holds for all $a, b, c$ satisfying the given constraint:
$$
\frac{b+c}{\sqrt{a}}+\frac{c+a}{\sqrt{b}}+\frac{a+b}{\sqrt{c}} \geq \sqrt{a}+\sqrt{b}+\sqrt{c}+C
$$

Solution: [Solution 1]
From the AM-GM Inequality, we have

$$
\begin{aligned}
& \frac{b+c}{\sqrt{a}}+\frac{c+a}{\sqrt{b}}+\frac{a+b}{\sqrt{c}} \geq 2\left(\sqrt{\frac{b c}{a}}+\sqrt{\frac{c a}{b}}+\sqrt{\frac{a b}{c}}\right)= \\
& =\left(\sqrt{\frac{b c}{a}}+\sqrt{\frac{c a}{b}}\right)+\left(\sqrt{\frac{c a}{b}}+\sqrt{\frac{a b}{c}}\right)+\left(\sqrt{\frac{a b}{c}}+\sqrt{\frac{b c}{a}}\right) \geq \\
& \geq 2(\sqrt{a}+\sqrt{b}+\sqrt{c}) \geq \sqrt{a}+\sqrt{b}+\sqrt{c}+3 \sqrt[6]{a b c}=\sqrt{a}+\sqrt{b}+\sqrt{c}+3 .
\end{aligned}
$$

Problem: Let $x, y, z \in [0,1]$. Determine the minimal constant $C$ such that the following inequality holds for all $x, y, z$:
$$
x(x-y)(z-x) \leq C.
$$

Solution:

## Response

To solve the problem, we need to analyze the expression \( x(x-y)(z-x) \) for \( x, y, z \in [0, 1] \) and find the maximum value of this expression, which will give us the minimal constant \( C \) such that the inequality holds for all \( x, y, z \).

### Step 1: Analyze the expression

The expression \( x(x-y)(z-x) \) can be rewritten as:
\[
x \cdot (x - y) \cdot (z - x)
\]
This expression is a product of three factors: \( x \), \( (x - y) \), and \( (z - x) \).

### Step 2: Determine the ranges of the factors

1. **Factor \( x \)**: Since \( x \in [0, 1] \), we have \( x \geq 0 \).
2. **Factor \( (x - y) \)**: Since \( y \in [0, 1] \), the maximum value of \( (x - y) \) occurs when \( y \) is minimized (i.e., \( y = 0 \)). Thus, \( (x - y) \) can range from \( -1 \) (when \( x = 0 \) and \( y = 1 \)) to \( 1 \) (when \( x = 1 \) and \( y = 0 \)).
3. **Factor \( (z - x) \)**: Similarly, since \( z \in [0, 1] \), the maximum value of \( (z - x) \) occurs when \( z \) is maximized (i.e., \( z = 1 \)). Thus, \( (z - x) \) can range from \( -1 \) (when \( z = 0 \) and \( x = 1 \)) to \( 1 \) (when \( z = 1 \) and \( x = 0 \)).

### Step 3: Find critical points

To find the maximum of \( x(x-y)(z-x) \), we can consider the boundaries of the intervals for \( x, y, z \) and also check for critical points within the interval.

1. **Boundary cases**:
   - If \( x = 0 \): \( 0(0-y)(z-0) = 0 \).
   - If \( x = 1 \): \( 1(1-y)(z-1) = (1-y)(z-1) \). This can be \( 0 \) if \( z = 1 \) or \( y = 1 \).
   - If \( y = 0 \): \( x(x-0)(z-x) = x^2(z-x) \).
   - If \( z = 0 \): \( x(x-y)(0-x) = -x^2(x-y) \).

2. **Maximizing \( x^2(z-x) \)**:
   - Set \( z = 1 \) to maximize \( (z-x) \).
   - Then we have \( x^2(1-x) \).
   - The function \( f(x) = x^2(1-x) \) is a cubic function. To find its maximum, we can take the derivative:
     \[
     f'(x) = 2x(1-x) - x^2 = 2x - 3x^2
     \]
     Setting \( f'(x) = 0 \):
     \[
     2x - 3x^2 = 0 \implies x(2 - 3x) = 0 \implies x = 0 \text{ or } x = \frac{2}{3}
     \]
   - Evaluating \( f(x) \) at \( x = 0 \), \( x = 1 \), and \( x = \frac{2}{3} \):
     - \( f(0) = 0 \)
     - \( f(1) = 0 \)
     - \( f\left(\frac{2}{3}\right) = \left(\frac{2}{3}\right)^2\left(1 - \frac{2}{3}\right) = \frac{4}{9} \cdot \frac{1}{3} = \frac{4}{27} \).

### Step 4: Conclusion

The maximum value of \( x(x-y)(z-x) \) occurs at \( x = \frac{2}{3} \), \( y = 0 \), and \( z = 1 \), yielding \( \frac{4}{27} \).

Thus, the minimal constant \( C \) such that the inequality holds for all \( x, y, z \in [0, 1] \) is:
\[
\boxed{C = \frac{4}{27}}.
\]

The answer is \( C = \frac{4}{27} \).