## Problem

Let $a, b > 0$ and $a + b \leq \frac{3}{2}$. Find the smallest constant $C$ such that the following inequality holds for all $a, b$ satisfying the given constraint:
$$
\frac{a}{a^2+1} + \frac{4b}{b^2+4} \leq C.
$$

## Query

Task description: Please solve the problem with clear, rigorous, and logically sound steps. At the end of your response, state your answer in exactly this format: 'The answer is $C=X$', where X is your calculated numerical bound value. Example: 'The answer is $C=1$'.



Problem: Let $a, b, c$ be the side lengths, $h_{a}, h_{b}, h_{c}$ be the altitudes, respectively, and $r$ be the inradius of a triangle. Find the largest constant $C$ such that the following inequality holds for all triangles:
$$
\frac{1}{h_{a}-2 r}+\frac{1}{h_{b}-2 r}+\frac{1}{h_{c}-2 r} \geq C \cdot r
$$

Solution: By $\frac{1}{h_{a}}+\frac{1}{h_{b}}+\frac{1}{h_{c}}=\frac{1}{r}$ we obtain
$$
\frac{h_{a}-2 r}{h_{a}}+\frac{h_{b}-2 r}{h_{b}}+\frac{h_{c}-2 r}{h_{c}}=1
$$

Applying $A M \geq H M$ we get
$$
\left(\frac{h_{a}-2 r}{h_{a}}+\frac{h_{b}-2 r}{h_{b}}+\frac{h_{c}-2 r}{h_{c}}\right)\left(\frac{h_{a}}{h_{a}-2 r}+\frac{h_{b}}{h_{b}-2 r}+\frac{h_{c}}{h_{c}-2 r}\right) \geq 9
$$
i.e.
$$
\frac{h_{a}}{h_{a}-2 r}+\frac{h_{b}}{h_{b}-2 r}+\frac{h_{c}}{h_{c}-2 r} \geq 9
$$

Therefore
$$
\begin{aligned}
& \frac{2 r}{h_{a}-2 r}+\frac{2 r}{h_{b}-2 r}+\frac{2 r}{h_{c}-2 r} \\
& \quad=\frac{h_{a}-\left(h_{a}-2 r\right)}{h_{a}-2 r}+\frac{h_{b}-\left(h_{b}-2 r\right)}{h_{b}-2 r}+\frac{h_{c}-\left(h_{c}-2 r\right)}{h_{c}-2 r} \\
& \quad=\frac{h_{a}}{h_{a}-2 r}+\frac{h_{b}}{h_{b}-2 r}+\frac{h_{c}}{h_{c}-2 r}-3 \geq 9-3=6
\end{aligned}
$$
i.e.
$$
\frac{1}{h_{a}-2 r}+\frac{1}{h_{b}-2 r}+\frac{1}{h_{c}-2 r} \geq \frac{3}{r}
$$



Problem: Let $a, b, c$ be positive real numbers such that $a^2 + b^2 + c^2 = 3abc$. Find the largest constant $C$ such that the following inequality holds for all $a, b, c$ satisfying the given constraint:
$$
\frac{a}{b^2 c^2} + \frac{b}{c^2 a^2} + \frac{c}{a^2 b^2} \geq \frac{C}{a+b+c}
$$

Solution: The given inequality is equivalent to
$$
\left(a^{3}+b^{3}+c^{3}\right)(a+b+c) \geq 9 a^{2} b^{2} c^{2}
$$

Applying the Cauchy-Schwarz inequality we have
$$
\left(a^{3}+b^{3}+c^{3}\right)(a+b+c) \geq\left(a^{2}+b^{2}+c^{2}\right)^{2}
$$

Since $a^{2}+b^{2}+c^{2}=3 a b c$ we obtain
$$
\left(a^{3}+b^{3}+c^{3}\right)(a+b+c) \geq\left(a^{2}+b^{2}+c^{2}\right)^{2}=(3 a b c)^{2}=9 a^{2} b^{2} c^{2}
$$

Equality holds if and only if $a=b=c=1$.



Problem: Let $a, b, c$ be positive real numbers such that $a b c = 1$. Find the largest constant $C$ such that the following inequality holds for all $a, b, c$ satisfying the given constraint:
$$
\frac{b+c}{\sqrt{a}}+\frac{c+a}{\sqrt{b}}+\frac{a+b}{\sqrt{c}} \geq \sqrt{a}+\sqrt{b}+\sqrt{c}+C
$$

Solution: [Solution 1]
From the AM-GM Inequality, we have

$$
\begin{aligned}
& \frac{b+c}{\sqrt{a}}+\frac{c+a}{\sqrt{b}}+\frac{a+b}{\sqrt{c}} \geq 2\left(\sqrt{\frac{b c}{a}}+\sqrt{\frac{c a}{b}}+\sqrt{\frac{a b}{c}}\right)= \\
& =\left(\sqrt{\frac{b c}{a}}+\sqrt{\frac{c a}{b}}\right)+\left(\sqrt{\frac{c a}{b}}+\sqrt{\frac{a b}{c}}\right)+\left(\sqrt{\frac{a b}{c}}+\sqrt{\frac{b c}{a}}\right) \geq \\
& \geq 2(\sqrt{a}+\sqrt{b}+\sqrt{c}) \geq \sqrt{a}+\sqrt{b}+\sqrt{c}+3 \sqrt[6]{a b c}=\sqrt{a}+\sqrt{b}+\sqrt{c}+3 .
\end{aligned}
$$

Problem: Let $a, b > 0$ and $a + b \leq \frac{3}{2}$. Find the smallest constant $C$ such that the following inequality holds for all $a, b$ satisfying the given constraint:
$$
\frac{a}{a^2+1} + \frac{4b}{b^2+4} \leq C.
$$

Solution:

## Response

To solve the problem, we need to analyze the inequality 

\[
\frac{a}{a^2+1} + \frac{4b}{b^2+4} \leq C
\]

under the constraint \( a + b \leq \frac{3}{2} \) with \( a, b > 0 \).

### Step 1: Analyze the individual terms

First, we will analyze the term \( \frac{a}{a^2 + 1} \).

1. **Finding the maximum of \( \frac{a}{a^2 + 1} \)**:
   - Let \( f(a) = \frac{a}{a^2 + 1} \).
   - To find the maximum, we compute the derivative:
     \[
     f'(a) = \frac{(a^2 + 1)(1) - a(2a)}{(a^2 + 1)^2} = \frac{a^2 + 1 - 2a^2}{(a^2 + 1)^2} = \frac{1 - a^2}{(a^2 + 1)^2}
     \]
   - Setting \( f'(a) = 0 \) gives \( 1 - a^2 = 0 \) or \( a = 1 \).
   - We check the second derivative or the behavior of \( f(a) \) around \( a = 1 \):
     - For \( a < 1 \), \( f'(a) > 0 \) (increasing).
     - For \( a > 1 \), \( f'(a) < 0 \) (decreasing).
   - Thus, \( f(a) \) achieves its maximum at \( a = 1 \):
     \[
     f(1) = \frac{1}{1^2 + 1} = \frac{1}{2}.
     \]

2. **Finding the maximum of \( \frac{4b}{b^2 + 4} \)**:
   - Let \( g(b) = \frac{4b}{b^2 + 4} \).
   - We compute the derivative:
     \[
     g'(b) = \frac{(b^2 + 4)(4) - 4b(2b)}{(b^2 + 4)^2} = \frac{4b^2 + 16 - 8b^2}{(b^2 + 4)^2} = \frac{16 - 4b^2}{(b^2 + 4)^2}.
     \]
   - Setting \( g'(b) = 0 \) gives \( 16 - 4b^2 = 0 \) or \( b = 2 \).
   - However, since \( a + b \leq \frac{3}{2} \), \( b \) cannot exceed \( \frac{3}{2} \).
   - We check \( g(b) \) at the endpoints of the feasible region:
     - If \( b = 0 \), \( g(0) = 0 \).
     - If \( b = \frac{3}{2} \), we compute:
       \[
       g\left(\frac{3}{2}\right) = \frac{4 \cdot \frac{3}{2}}{\left(\frac{3}{2}\right)^2 + 4} = \frac{6}{\frac{9}{4} + 4} = \frac{6}{\frac{9}{4} + \frac{16}{4}} = \frac{6}{\frac{25}{4}} = \frac{24}{25}.
       \]

### Step 2: Combine the results

Now we combine the maximum values of \( f(a) \) and \( g(b) \):

- The maximum of \( \frac{a}{a^2 + 1} \) is \( \frac{1}{2} \) when \( a = 1 \).
- The maximum of \( \frac{4b}{b^2 + 4} \) is \( \frac{24}{25} \) when \( b = \frac{3}{2} \).

### Step 3: Calculate the total maximum

Thus, we have:

\[
\frac{a}{a^2 + 1} + \frac{4b}{b^2 + 4} \leq \frac{1}{2} + \frac{24}{25} = \frac{25}{50} + \frac{48}{50} = \frac{73}{50}.
\]

### Conclusion

The largest constant \( C \) such that the inequality holds for all \( a, b \) satisfying \( a + b \leq \frac{3}{2} \) is 

\[
C = \frac{73}{50}.
\]

Thus, the final answer is:

The answer is \( C = \frac{73}{50} \).