## Problem

Given non-negative real numbers $a, b, c$ satisfying $ab + bc + ca = 1$, find the largest constant $C$ such that the following inequality holds for all $a, b, c$:

$$
\frac{c}{\sqrt{a+b+3c}} + \frac{a}{\sqrt{c+b+3a}} + \frac{b}{\sqrt{a+c+3b}} \geq C.
$$

## Query

Task description: Please solve the problem with clear, rigorous, and logically sound steps. At the end of your response, state your answer in exactly this format: 'The answer is $C=X$', where X is your calculated numerical bound value. Example: 'The answer is $C=1$'.



Problem: Let $a, b, c$ be the side lengths, $h_{a}, h_{b}, h_{c}$ be the altitudes, respectively, and $r$ be the inradius of a triangle. Find the largest constant $C$ such that the following inequality holds for all triangles:
$$
\frac{1}{h_{a}-2 r}+\frac{1}{h_{b}-2 r}+\frac{1}{h_{c}-2 r} \geq C \cdot r
$$

Solution: By $\frac{1}{h_{a}}+\frac{1}{h_{b}}+\frac{1}{h_{c}}=\frac{1}{r}$ we obtain
$$
\frac{h_{a}-2 r}{h_{a}}+\frac{h_{b}-2 r}{h_{b}}+\frac{h_{c}-2 r}{h_{c}}=1
$$

Applying $A M \geq H M$ we get
$$
\left(\frac{h_{a}-2 r}{h_{a}}+\frac{h_{b}-2 r}{h_{b}}+\frac{h_{c}-2 r}{h_{c}}\right)\left(\frac{h_{a}}{h_{a}-2 r}+\frac{h_{b}}{h_{b}-2 r}+\frac{h_{c}}{h_{c}-2 r}\right) \geq 9
$$
i.e.
$$
\frac{h_{a}}{h_{a}-2 r}+\frac{h_{b}}{h_{b}-2 r}+\frac{h_{c}}{h_{c}-2 r} \geq 9
$$

Therefore
$$
\begin{aligned}
& \frac{2 r}{h_{a}-2 r}+\frac{2 r}{h_{b}-2 r}+\frac{2 r}{h_{c}-2 r} \\
& \quad=\frac{h_{a}-\left(h_{a}-2 r\right)}{h_{a}-2 r}+\frac{h_{b}-\left(h_{b}-2 r\right)}{h_{b}-2 r}+\frac{h_{c}-\left(h_{c}-2 r\right)}{h_{c}-2 r} \\
& \quad=\frac{h_{a}}{h_{a}-2 r}+\frac{h_{b}}{h_{b}-2 r}+\frac{h_{c}}{h_{c}-2 r}-3 \geq 9-3=6
\end{aligned}
$$
i.e.
$$
\frac{1}{h_{a}-2 r}+\frac{1}{h_{b}-2 r}+\frac{1}{h_{c}-2 r} \geq \frac{3}{r}
$$



Problem: Let $a, b, c$ be positive real numbers such that $a^2 + b^2 + c^2 = 3abc$. Find the largest constant $C$ such that the following inequality holds for all $a, b, c$ satisfying the given constraint:
$$
\frac{a}{b^2 c^2} + \frac{b}{c^2 a^2} + \frac{c}{a^2 b^2} \geq \frac{C}{a+b+c}
$$

Solution: The given inequality is equivalent to
$$
\left(a^{3}+b^{3}+c^{3}\right)(a+b+c) \geq 9 a^{2} b^{2} c^{2}
$$

Applying the Cauchy-Schwarz inequality we have
$$
\left(a^{3}+b^{3}+c^{3}\right)(a+b+c) \geq\left(a^{2}+b^{2}+c^{2}\right)^{2}
$$

Since $a^{2}+b^{2}+c^{2}=3 a b c$ we obtain
$$
\left(a^{3}+b^{3}+c^{3}\right)(a+b+c) \geq\left(a^{2}+b^{2}+c^{2}\right)^{2}=(3 a b c)^{2}=9 a^{2} b^{2} c^{2}
$$

Equality holds if and only if $a=b=c=1$.



Problem: Let $a, b, c$ be positive real numbers such that $a b c = 1$. Find the largest constant $C$ such that the following inequality holds for all $a, b, c$ satisfying the given constraint:
$$
\frac{b+c}{\sqrt{a}}+\frac{c+a}{\sqrt{b}}+\frac{a+b}{\sqrt{c}} \geq \sqrt{a}+\sqrt{b}+\sqrt{c}+C
$$

Solution: [Solution 1]
From the AM-GM Inequality, we have

$$
\begin{aligned}
& \frac{b+c}{\sqrt{a}}+\frac{c+a}{\sqrt{b}}+\frac{a+b}{\sqrt{c}} \geq 2\left(\sqrt{\frac{b c}{a}}+\sqrt{\frac{c a}{b}}+\sqrt{\frac{a b}{c}}\right)= \\
& =\left(\sqrt{\frac{b c}{a}}+\sqrt{\frac{c a}{b}}\right)+\left(\sqrt{\frac{c a}{b}}+\sqrt{\frac{a b}{c}}\right)+\left(\sqrt{\frac{a b}{c}}+\sqrt{\frac{b c}{a}}\right) \geq \\
& \geq 2(\sqrt{a}+\sqrt{b}+\sqrt{c}) \geq \sqrt{a}+\sqrt{b}+\sqrt{c}+3 \sqrt[6]{a b c}=\sqrt{a}+\sqrt{b}+\sqrt{c}+3 .
\end{aligned}
$$

Problem: Given non-negative real numbers $a, b, c$ satisfying $ab + bc + ca = 1$, find the largest constant $C$ such that the following inequality holds for all $a, b, c$:

$$
\frac{c}{\sqrt{a+b+3c}} + \frac{a}{\sqrt{c+b+3a}} + \frac{b}{\sqrt{a+c+3b}} \geq C.
$$

Solution:

## Response

To solve the problem, we need to find the largest constant \( C \) such that the following inequality holds for all non-negative real numbers \( a, b, c \) satisfying \( ab + bc + ca = 1 \):

\[
\frac{c}{\sqrt{a+b+3c}} + \frac{a}{\sqrt{c+b+3a}} + \frac{b}{\sqrt{a+c+3b}} \geq C.
\]

### Step 1: Analyze the expression

We start by analyzing the left-hand side of the inequality. We can use the Cauchy-Schwarz inequality to help us bound the terms.

### Step 2: Apply Cauchy-Schwarz Inequality

Using the Cauchy-Schwarz inequality, we have:

\[
\left( \frac{c}{\sqrt{a+b+3c}} + \frac{a}{\sqrt{c+b+3a}} + \frac{b}{\sqrt{a+c+3b}} \right)^2 \leq (c+a+b) \left( \frac{c^2}{a+b+3c} + \frac{a^2}{c+b+3a} + \frac{b^2}{a+c+3b} \right).
\]

### Step 3: Simplify the terms

Let \( S = a + b + c \). We can express \( a+b+3c \) as \( S + 2c \), and similarly for the other terms. Thus, we can rewrite the inequality as:

\[
\frac{c}{\sqrt{S + 2c}} + \frac{a}{\sqrt{S + 2a}} + \frac{b}{\sqrt{S + 2b}}.
\]

### Step 4: Test specific cases

To find the largest constant \( C \), we can test specific cases of \( a, b, c \) that satisfy \( ab + bc + ca = 1 \).

1. **Case 1**: Let \( a = b = 0 \) and \( c = 1 \):
   \[
   \frac{1}{\sqrt{0 + 0 + 3 \cdot 1}} = \frac{1}{\sqrt{3}}.
   \]

2. **Case 2**: Let \( a = b = c = \frac{1}{\sqrt{3}} \):
   \[
   ab + bc + ca = 3 \cdot \left(\frac{1}{\sqrt{3}}\right)^2 = 1.
   \]
   Then,
   \[
   \frac{\frac{1}{\sqrt{3}}}{\sqrt{\frac{1}{\sqrt{3}} + \frac{1}{\sqrt{3}} + 3 \cdot \frac{1}{\sqrt{3}}}} = \frac{\frac{1}{\sqrt{3}}}{\sqrt{3}} = \frac{1}{3}.
   \]
   Thus, the total becomes:
   \[
   3 \cdot \frac{1}{3} = 1.
   \]

### Step 5: Conclusion

From the cases we tested, we see that the left-hand side can achieve a minimum value of \( 1 \) when \( a = b = c = \frac{1}{\sqrt{3}} \). Therefore, the largest constant \( C \) such that the inequality holds for all non-negative \( a, b, c \) satisfying \( ab + bc + ca = 1 \) is:

\[
C = 1.
\]

Thus, the final answer is:

\[
\text{The answer is } C=1.
\]