## Problem

Let $a, b > 0$ such that $a + b = 1$. Determine the largest constant $C$ such that the following inequality holds for all $a, b$:

$$
\left(a+\frac{1}{a}\right)^2+\left(b+\frac{1}{b}\right)^2 \geq C.
$$

## Query

Task description: Please solve the problem with clear, rigorous, and logically sound steps. At the end of your response, state your answer in exactly this format: 'The answer is $C=X$', where X is your calculated numerical bound value. Example: 'The answer is $C=1$'.



Problem: Let $a, b, c$ be the side lengths, $h_{a}, h_{b}, h_{c}$ be the altitudes, respectively, and $r$ be the inradius of a triangle. Find the largest constant $C$ such that the following inequality holds for all triangles:
$$
\frac{1}{h_{a}-2 r}+\frac{1}{h_{b}-2 r}+\frac{1}{h_{c}-2 r} \geq C \cdot r
$$

Solution: By $\frac{1}{h_{a}}+\frac{1}{h_{b}}+\frac{1}{h_{c}}=\frac{1}{r}$ we obtain
$$
\frac{h_{a}-2 r}{h_{a}}+\frac{h_{b}-2 r}{h_{b}}+\frac{h_{c}-2 r}{h_{c}}=1
$$

Applying $A M \geq H M$ we get
$$
\left(\frac{h_{a}-2 r}{h_{a}}+\frac{h_{b}-2 r}{h_{b}}+\frac{h_{c}-2 r}{h_{c}}\right)\left(\frac{h_{a}}{h_{a}-2 r}+\frac{h_{b}}{h_{b}-2 r}+\frac{h_{c}}{h_{c}-2 r}\right) \geq 9
$$
i.e.
$$
\frac{h_{a}}{h_{a}-2 r}+\frac{h_{b}}{h_{b}-2 r}+\frac{h_{c}}{h_{c}-2 r} \geq 9
$$

Therefore
$$
\begin{aligned}
& \frac{2 r}{h_{a}-2 r}+\frac{2 r}{h_{b}-2 r}+\frac{2 r}{h_{c}-2 r} \\
& \quad=\frac{h_{a}-\left(h_{a}-2 r\right)}{h_{a}-2 r}+\frac{h_{b}-\left(h_{b}-2 r\right)}{h_{b}-2 r}+\frac{h_{c}-\left(h_{c}-2 r\right)}{h_{c}-2 r} \\
& \quad=\frac{h_{a}}{h_{a}-2 r}+\frac{h_{b}}{h_{b}-2 r}+\frac{h_{c}}{h_{c}-2 r}-3 \geq 9-3=6
\end{aligned}
$$
i.e.
$$
\frac{1}{h_{a}-2 r}+\frac{1}{h_{b}-2 r}+\frac{1}{h_{c}-2 r} \geq \frac{3}{r}
$$



Problem: Let $a, b, c$ be positive real numbers such that $a^2 + b^2 + c^2 = 3abc$. Find the largest constant $C$ such that the following inequality holds for all $a, b, c$ satisfying the given constraint:
$$
\frac{a}{b^2 c^2} + \frac{b}{c^2 a^2} + \frac{c}{a^2 b^2} \geq \frac{C}{a+b+c}
$$

Solution: The given inequality is equivalent to
$$
\left(a^{3}+b^{3}+c^{3}\right)(a+b+c) \geq 9 a^{2} b^{2} c^{2}
$$

Applying the Cauchy-Schwarz inequality we have
$$
\left(a^{3}+b^{3}+c^{3}\right)(a+b+c) \geq\left(a^{2}+b^{2}+c^{2}\right)^{2}
$$

Since $a^{2}+b^{2}+c^{2}=3 a b c$ we obtain
$$
\left(a^{3}+b^{3}+c^{3}\right)(a+b+c) \geq\left(a^{2}+b^{2}+c^{2}\right)^{2}=(3 a b c)^{2}=9 a^{2} b^{2} c^{2}
$$

Equality holds if and only if $a=b=c=1$.



Problem: Let $a, b, c$ be positive real numbers such that $a b c = 1$. Find the largest constant $C$ such that the following inequality holds for all $a, b, c$ satisfying the given constraint:
$$
\frac{b+c}{\sqrt{a}}+\frac{c+a}{\sqrt{b}}+\frac{a+b}{\sqrt{c}} \geq \sqrt{a}+\sqrt{b}+\sqrt{c}+C
$$

Solution: [Solution 1]
From the AM-GM Inequality, we have

$$
\begin{aligned}
& \frac{b+c}{\sqrt{a}}+\frac{c+a}{\sqrt{b}}+\frac{a+b}{\sqrt{c}} \geq 2\left(\sqrt{\frac{b c}{a}}+\sqrt{\frac{c a}{b}}+\sqrt{\frac{a b}{c}}\right)= \\
& =\left(\sqrt{\frac{b c}{a}}+\sqrt{\frac{c a}{b}}\right)+\left(\sqrt{\frac{c a}{b}}+\sqrt{\frac{a b}{c}}\right)+\left(\sqrt{\frac{a b}{c}}+\sqrt{\frac{b c}{a}}\right) \geq \\
& \geq 2(\sqrt{a}+\sqrt{b}+\sqrt{c}) \geq \sqrt{a}+\sqrt{b}+\sqrt{c}+3 \sqrt[6]{a b c}=\sqrt{a}+\sqrt{b}+\sqrt{c}+3 .
\end{aligned}
$$

Problem: Let $a, b > 0$ such that $a + b = 1$. Determine the largest constant $C$ such that the following inequality holds for all $a, b$:

$$
\left(a+\frac{1}{a}\right)^2+\left(b+\frac{1}{b}\right)^2 \geq C.
$$

Solution:

## Response

To solve the problem, we start with the given inequality:

\[
\left(a+\frac{1}{a}\right)^2+\left(b+\frac{1}{b}\right)^2 \geq C
\]

where \( a + b = 1 \) and \( a, b > 0 \).

First, we can express \( b \) in terms of \( a \):

\[
b = 1 - a
\]

Now, we rewrite the left-hand side of the inequality:

\[
\left(a + \frac{1}{a}\right)^2 + \left((1-a) + \frac{1}{1-a}\right)^2
\]

Next, we simplify each term. The first term is:

\[
\left(a + \frac{1}{a}\right)^2 = a^2 + 2 + \frac{1}{a^2}
\]

The second term is:

\[
\left((1-a) + \frac{1}{1-a}\right)^2 = (1-a)^2 + 2 + \frac{1}{(1-a)^2}
\]

Thus, we have:

\[
\left(a + \frac{1}{a}\right)^2 + \left((1-a) + \frac{1}{1-a}\right)^2 = \left(a^2 + \frac{1}{a^2} + 2\right) + \left((1-a)^2 + \frac{1}{(1-a)^2} + 2\right)
\]

Combining these, we get:

\[
= a^2 + (1-a)^2 + \frac{1}{a^2} + \frac{1}{(1-a)^2} + 4
\]

Now, we simplify \( a^2 + (1-a)^2 \):

\[
a^2 + (1-a)^2 = a^2 + (1 - 2a + a^2) = 2a^2 - 2a + 1
\]

Next, we need to analyze \( \frac{1}{a^2} + \frac{1}{(1-a)^2} \). Using the Cauchy-Schwarz inequality, we have:

\[
\left(\frac{1}{a^2} + \frac{1}{(1-a)^2}\right)(a^2 + (1-a)^2) \geq (1 + 1)^2 = 4
\]

Thus,

\[
\frac{1}{a^2} + \frac{1}{(1-a)^2} \geq \frac{4}{a^2 + (1-a)^2}
\]

Now, substituting \( a^2 + (1-a)^2 = 2a^2 - 2a + 1 \):

\[
\frac{1}{a^2} + \frac{1}{(1-a)^2} \geq \frac{4}{2a^2 - 2a + 1}
\]

To find the minimum value of \( \left(a + \frac{1}{a}\right)^2 + \left(b + \frac{1}{b}\right)^2 \), we can evaluate it at specific points. 

Letâ€™s consider \( a = b = \frac{1}{2} \):

\[
\left(\frac{1}{2} + 2\right)^2 + \left(\frac{1}{2} + 2\right)^2 = 2 \left(\frac{5}{2}\right)^2 = 2 \cdot \frac{25}{4} = \frac{50}{4} = 12.5
\]

Thus, we have:

\[
\left(a+\frac{1}{a}\right)^2+\left(b+\frac{1}{b}\right)^2 \geq 12.5
\]

This suggests that the largest constant \( C \) such that the inequality holds for all \( a, b > 0 \) with \( a + b = 1 \) is:

\[
C = 12.5
\]

Therefore, the final answer is:

\[
\text{The answer is } C = 12.5
\]