## Problem

Given four real numbers $a, b, c, d \geq 0$ satisfying $a \geq b + 7c + d$, find the largest constant $C$ such that the following inequality holds for all $a, b, c, d$:

$$
7(a+b)(b+c)(c+d)(d+a) \geq C a b c d
$$

## Query

Task description: Please solve the problem with clear, rigorous, and logically sound steps. At the end of your response, state your answer in exactly this format: 'The answer is $C=X$', where X is your calculated numerical bound value. Example: 'The answer is $C=1$'.



Problem: Let $a, b, c$ be the side lengths, $h_{a}, h_{b}, h_{c}$ be the altitudes, respectively, and $r$ be the inradius of a triangle. Find the largest constant $C$ such that the following inequality holds for all triangles:
$$
\frac{1}{h_{a}-2 r}+\frac{1}{h_{b}-2 r}+\frac{1}{h_{c}-2 r} \geq C \cdot r
$$

Solution: By $\frac{1}{h_{a}}+\frac{1}{h_{b}}+\frac{1}{h_{c}}=\frac{1}{r}$ we obtain
$$
\frac{h_{a}-2 r}{h_{a}}+\frac{h_{b}-2 r}{h_{b}}+\frac{h_{c}-2 r}{h_{c}}=1
$$

Applying $A M \geq H M$ we get
$$
\left(\frac{h_{a}-2 r}{h_{a}}+\frac{h_{b}-2 r}{h_{b}}+\frac{h_{c}-2 r}{h_{c}}\right)\left(\frac{h_{a}}{h_{a}-2 r}+\frac{h_{b}}{h_{b}-2 r}+\frac{h_{c}}{h_{c}-2 r}\right) \geq 9
$$
i.e.
$$
\frac{h_{a}}{h_{a}-2 r}+\frac{h_{b}}{h_{b}-2 r}+\frac{h_{c}}{h_{c}-2 r} \geq 9
$$

Therefore
$$
\begin{aligned}
& \frac{2 r}{h_{a}-2 r}+\frac{2 r}{h_{b}-2 r}+\frac{2 r}{h_{c}-2 r} \\
& \quad=\frac{h_{a}-\left(h_{a}-2 r\right)}{h_{a}-2 r}+\frac{h_{b}-\left(h_{b}-2 r\right)}{h_{b}-2 r}+\frac{h_{c}-\left(h_{c}-2 r\right)}{h_{c}-2 r} \\
& \quad=\frac{h_{a}}{h_{a}-2 r}+\frac{h_{b}}{h_{b}-2 r}+\frac{h_{c}}{h_{c}-2 r}-3 \geq 9-3=6
\end{aligned}
$$
i.e.
$$
\frac{1}{h_{a}-2 r}+\frac{1}{h_{b}-2 r}+\frac{1}{h_{c}-2 r} \geq \frac{3}{r}
$$



Problem: Let $a, b, c$ be positive real numbers such that $a^2 + b^2 + c^2 = 3abc$. Find the largest constant $C$ such that the following inequality holds for all $a, b, c$ satisfying the given constraint:
$$
\frac{a}{b^2 c^2} + \frac{b}{c^2 a^2} + \frac{c}{a^2 b^2} \geq \frac{C}{a+b+c}
$$

Solution: The given inequality is equivalent to
$$
\left(a^{3}+b^{3}+c^{3}\right)(a+b+c) \geq 9 a^{2} b^{2} c^{2}
$$

Applying the Cauchy-Schwarz inequality we have
$$
\left(a^{3}+b^{3}+c^{3}\right)(a+b+c) \geq\left(a^{2}+b^{2}+c^{2}\right)^{2}
$$

Since $a^{2}+b^{2}+c^{2}=3 a b c$ we obtain
$$
\left(a^{3}+b^{3}+c^{3}\right)(a+b+c) \geq\left(a^{2}+b^{2}+c^{2}\right)^{2}=(3 a b c)^{2}=9 a^{2} b^{2} c^{2}
$$

Equality holds if and only if $a=b=c=1$.



Problem: Let $a, b, c$ be positive real numbers such that $a b c = 1$. Find the largest constant $C$ such that the following inequality holds for all $a, b, c$ satisfying the given constraint:
$$
\frac{b+c}{\sqrt{a}}+\frac{c+a}{\sqrt{b}}+\frac{a+b}{\sqrt{c}} \geq \sqrt{a}+\sqrt{b}+\sqrt{c}+C
$$

Solution: [Solution 1]
From the AM-GM Inequality, we have

$$
\begin{aligned}
& \frac{b+c}{\sqrt{a}}+\frac{c+a}{\sqrt{b}}+\frac{a+b}{\sqrt{c}} \geq 2\left(\sqrt{\frac{b c}{a}}+\sqrt{\frac{c a}{b}}+\sqrt{\frac{a b}{c}}\right)= \\
& =\left(\sqrt{\frac{b c}{a}}+\sqrt{\frac{c a}{b}}\right)+\left(\sqrt{\frac{c a}{b}}+\sqrt{\frac{a b}{c}}\right)+\left(\sqrt{\frac{a b}{c}}+\sqrt{\frac{b c}{a}}\right) \geq \\
& \geq 2(\sqrt{a}+\sqrt{b}+\sqrt{c}) \geq \sqrt{a}+\sqrt{b}+\sqrt{c}+3 \sqrt[6]{a b c}=\sqrt{a}+\sqrt{b}+\sqrt{c}+3 .
\end{aligned}
$$

Problem: Given four real numbers $a, b, c, d \geq 0$ satisfying $a \geq b + 7c + d$, find the largest constant $C$ such that the following inequality holds for all $a, b, c, d$:

$$
7(a+b)(b+c)(c+d)(d+a) \geq C a b c d
$$

Solution:

## Response

To solve the problem, we start with the given inequality:

\[
7(a+b)(b+c)(c+d)(d+a) \geq C a b c d
\]

We need to find the largest constant \( C \) such that this inequality holds for all non-negative \( a, b, c, d \) satisfying \( a \geq b + 7c + d \).

### Step 1: Analyze the condition

The condition \( a \geq b + 7c + d \) suggests that \( a \) is significantly larger than \( b, c, \) and \( d \) when \( c \) is non-zero. This will help us in estimating the left-hand side of the inequality.

### Step 2: Simplify the left-hand side

We can express the left-hand side as follows:

\[
(a+b)(b+c)(c+d)(d+a)
\]

To analyze this, we can consider the case where \( b, c, d \) are small compared to \( a \). For simplicity, let’s set \( b = 0 \), \( c = 0 \), and \( d = 0 \). Then we have:

\[
7(a+0)(0+0)(0+0)(0+a) = 0
\]

This does not provide useful information since both sides are zero.

### Step 3: Consider specific values

Let’s consider a case where \( b, c, d \) are small but non-zero. Set \( b = 1 \), \( c = 1 \), and \( d = 1 \). Then, we have:

\[
a \geq 1 + 7 \cdot 1 + 1 = 9 \implies a \geq 9
\]

Now, substituting \( a = 9 \):

\[
7(9+1)(1+1)(1+1)(1+9) = 7 \cdot 10 \cdot 2 \cdot 2 \cdot 10 = 2800
\]

Now, we calculate \( C \cdot a b c d \):

\[
C \cdot 9 \cdot 1 \cdot 1 \cdot 1 = 9C
\]

Thus, we need:

\[
2800 \geq 9C \implies C \leq \frac{2800}{9} \approx 311.11
\]

### Step 4: Check if \( C = 311 \) holds

Let’s check if \( C = 311 \) satisfies the inequality for other values. We can try \( a = 9, b = 1, c = 1, d = 1 \):

\[
7(9+1)(1+1)(1+1)(1+9) = 2800
\]
\[
9 \cdot 311 = 2799
\]

Since \( 2800 \geq 2799 \), the inequality holds.

### Step 5: Check if \( C = 312 \) fails

Now, let’s check if \( C = 312 \) holds:

\[
9 \cdot 312 = 2808
\]

Since \( 2800 < 2808 \), the inequality does not hold.

### Conclusion

Thus, the largest constant \( C \) such that the inequality holds for all non-negative \( a, b, c, d \) satisfying \( a \geq b + 7c + d \) is:

\[
\boxed{311}
\]

The answer is \( C = 311 \).