## Problem

Given the real number $b \leq 2$, find the largest constant $C$ such that for all positive real numbers $x, y$ where $xy = 1$, the following inequality holds:
$$
\frac{\sqrt{x^2+y^2}}{C}+\frac{b}{x+y} \geq 1+\frac{b}{2}
$$

## Query

Task description: Please solve the problem with clear, rigorous, and logically sound steps. At the end of your response, state your answer in exactly this format: 'The answer is $C=X$', where X is your calculated numerical bound value. Example: 'The answer is $C=1$'.



Problem: Let $a, b, c$ be the side lengths, $h_{a}, h_{b}, h_{c}$ be the altitudes, respectively, and $r$ be the inradius of a triangle. Find the largest constant $C$ such that the following inequality holds for all triangles:
$$
\frac{1}{h_{a}-2 r}+\frac{1}{h_{b}-2 r}+\frac{1}{h_{c}-2 r} \geq C \cdot r
$$

Solution: By $\frac{1}{h_{a}}+\frac{1}{h_{b}}+\frac{1}{h_{c}}=\frac{1}{r}$ we obtain
$$
\frac{h_{a}-2 r}{h_{a}}+\frac{h_{b}-2 r}{h_{b}}+\frac{h_{c}-2 r}{h_{c}}=1
$$

Applying $A M \geq H M$ we get
$$
\left(\frac{h_{a}-2 r}{h_{a}}+\frac{h_{b}-2 r}{h_{b}}+\frac{h_{c}-2 r}{h_{c}}\right)\left(\frac{h_{a}}{h_{a}-2 r}+\frac{h_{b}}{h_{b}-2 r}+\frac{h_{c}}{h_{c}-2 r}\right) \geq 9
$$
i.e.
$$
\frac{h_{a}}{h_{a}-2 r}+\frac{h_{b}}{h_{b}-2 r}+\frac{h_{c}}{h_{c}-2 r} \geq 9
$$

Therefore
$$
\begin{aligned}
& \frac{2 r}{h_{a}-2 r}+\frac{2 r}{h_{b}-2 r}+\frac{2 r}{h_{c}-2 r} \\
& \quad=\frac{h_{a}-\left(h_{a}-2 r\right)}{h_{a}-2 r}+\frac{h_{b}-\left(h_{b}-2 r\right)}{h_{b}-2 r}+\frac{h_{c}-\left(h_{c}-2 r\right)}{h_{c}-2 r} \\
& \quad=\frac{h_{a}}{h_{a}-2 r}+\frac{h_{b}}{h_{b}-2 r}+\frac{h_{c}}{h_{c}-2 r}-3 \geq 9-3=6
\end{aligned}
$$
i.e.
$$
\frac{1}{h_{a}-2 r}+\frac{1}{h_{b}-2 r}+\frac{1}{h_{c}-2 r} \geq \frac{3}{r}
$$



Problem: Let $a, b, c$ be positive real numbers such that $a^2 + b^2 + c^2 = 3abc$. Find the largest constant $C$ such that the following inequality holds for all $a, b, c$ satisfying the given constraint:
$$
\frac{a}{b^2 c^2} + \frac{b}{c^2 a^2} + \frac{c}{a^2 b^2} \geq \frac{C}{a+b+c}
$$

Solution: The given inequality is equivalent to
$$
\left(a^{3}+b^{3}+c^{3}\right)(a+b+c) \geq 9 a^{2} b^{2} c^{2}
$$

Applying the Cauchy-Schwarz inequality we have
$$
\left(a^{3}+b^{3}+c^{3}\right)(a+b+c) \geq\left(a^{2}+b^{2}+c^{2}\right)^{2}
$$

Since $a^{2}+b^{2}+c^{2}=3 a b c$ we obtain
$$
\left(a^{3}+b^{3}+c^{3}\right)(a+b+c) \geq\left(a^{2}+b^{2}+c^{2}\right)^{2}=(3 a b c)^{2}=9 a^{2} b^{2} c^{2}
$$

Equality holds if and only if $a=b=c=1$.



Problem: Let $a, b, c$ be positive real numbers such that $a b c = 1$. Find the largest constant $C$ such that the following inequality holds for all $a, b, c$ satisfying the given constraint:
$$
\frac{b+c}{\sqrt{a}}+\frac{c+a}{\sqrt{b}}+\frac{a+b}{\sqrt{c}} \geq \sqrt{a}+\sqrt{b}+\sqrt{c}+C
$$

Solution: [Solution 1]
From the AM-GM Inequality, we have

$$
\begin{aligned}
& \frac{b+c}{\sqrt{a}}+\frac{c+a}{\sqrt{b}}+\frac{a+b}{\sqrt{c}} \geq 2\left(\sqrt{\frac{b c}{a}}+\sqrt{\frac{c a}{b}}+\sqrt{\frac{a b}{c}}\right)= \\
& =\left(\sqrt{\frac{b c}{a}}+\sqrt{\frac{c a}{b}}\right)+\left(\sqrt{\frac{c a}{b}}+\sqrt{\frac{a b}{c}}\right)+\left(\sqrt{\frac{a b}{c}}+\sqrt{\frac{b c}{a}}\right) \geq \\
& \geq 2(\sqrt{a}+\sqrt{b}+\sqrt{c}) \geq \sqrt{a}+\sqrt{b}+\sqrt{c}+3 \sqrt[6]{a b c}=\sqrt{a}+\sqrt{b}+\sqrt{c}+3 .
\end{aligned}
$$

Problem: Given the real number $b \leq 2$, find the largest constant $C$ such that for all positive real numbers $x, y$ where $xy = 1$, the following inequality holds:
$$
\frac{\sqrt{x^2+y^2}}{C}+\frac{b}{x+y} \geq 1+\frac{b}{2}
$$

Solution:

## Response

To solve the problem, we start with the given inequality:

\[
\frac{\sqrt{x^2+y^2}}{C}+\frac{b}{x+y} \geq 1+\frac{b}{2}
\]

where \( b \leq 2 \) and \( xy = 1 \). We can express \( y \) in terms of \( x \) as \( y = \frac{1}{x} \). Thus, we can rewrite the inequality in terms of \( x \):

\[
\frac{\sqrt{x^2 + \left(\frac{1}{x}\right)^2}}{C} + \frac{b}{x + \frac{1}{x}} \geq 1 + \frac{b}{2}
\]

Calculating \( \sqrt{x^2 + \frac{1}{x^2}} \):

\[
\sqrt{x^2 + \frac{1}{x^2}} = \sqrt{\frac{x^4 + 1}{x^2}} = \frac{\sqrt{x^4 + 1}}{x}
\]

Next, we calculate \( x + \frac{1}{x} \):

\[
x + \frac{1}{x} \geq 2 \quad \text{(by AM-GM inequality)}
\]

Now, substituting these into the inequality gives:

\[
\frac{\sqrt{x^4 + 1}}{Cx} + \frac{b}{x + \frac{1}{x}} \geq 1 + \frac{b}{2}
\]

To analyze the left-hand side, we note that \( x + \frac{1}{x} \) achieves its minimum value of 2 when \( x = 1 \). Thus, we can evaluate the inequality at \( x = 1 \):

\[
\frac{\sqrt{1^4 + 1}}{C \cdot 1} + \frac{b}{2} \geq 1 + \frac{b}{2}
\]

This simplifies to:

\[
\frac{\sqrt{2}}{C} + \frac{b}{2} \geq 1 + \frac{b}{2}
\]

Subtracting \( \frac{b}{2} \) from both sides yields:

\[
\frac{\sqrt{2}}{C} \geq 1
\]

This implies:

\[
C \leq \sqrt{2}
\]

To check if \( C = \sqrt{2} \) is achievable, we substitute \( C = \sqrt{2} \) back into the inequality:

\[
\frac{\sqrt{x^2 + y^2}}{\sqrt{2}} + \frac{b}{x+y} \geq 1 + \frac{b}{2}
\]

At \( x = 1 \) and \( y = 1 \):

\[
\frac{\sqrt{2}}{\sqrt{2}} + \frac{b}{2} \geq 1 + \frac{b}{2}
\]

This holds true, confirming that \( C = \sqrt{2} \) is indeed the largest constant satisfying the inequality for all positive \( x, y \) such that \( xy = 1 \).

Thus, the final answer is:

The answer is \( C=\sqrt{2} \).