## Problem

Let $a, b, c$ be real numbers such that $a^2 + bc = 1$. Find the smallest constant $C$ such that the following inequality holds for all $a, b, c$ satisfying the given constraint:
$$
\frac{1}{a^2+1} + \frac{1}{b^2+1} + \frac{1}{c^2+1} \leq C
$$

## Query

Task description: Please solve the problem with clear, rigorous, and logically sound steps. At the end of your response, state your answer in exactly this format: 'The answer is $C=X$', where X is your calculated numerical bound value. Example: 'The answer is $C=1$'.



Problem: Let $a, b, c$ be the side lengths, $h_{a}, h_{b}, h_{c}$ be the altitudes, respectively, and $r$ be the inradius of a triangle. Find the largest constant $C$ such that the following inequality holds for all triangles:
$$
\frac{1}{h_{a}-2 r}+\frac{1}{h_{b}-2 r}+\frac{1}{h_{c}-2 r} \geq C \cdot r
$$

Solution: By $\frac{1}{h_{a}}+\frac{1}{h_{b}}+\frac{1}{h_{c}}=\frac{1}{r}$ we obtain
$$
\frac{h_{a}-2 r}{h_{a}}+\frac{h_{b}-2 r}{h_{b}}+\frac{h_{c}-2 r}{h_{c}}=1
$$

Applying $A M \geq H M$ we get
$$
\left(\frac{h_{a}-2 r}{h_{a}}+\frac{h_{b}-2 r}{h_{b}}+\frac{h_{c}-2 r}{h_{c}}\right)\left(\frac{h_{a}}{h_{a}-2 r}+\frac{h_{b}}{h_{b}-2 r}+\frac{h_{c}}{h_{c}-2 r}\right) \geq 9
$$
i.e.
$$
\frac{h_{a}}{h_{a}-2 r}+\frac{h_{b}}{h_{b}-2 r}+\frac{h_{c}}{h_{c}-2 r} \geq 9
$$

Therefore
$$
\begin{aligned}
& \frac{2 r}{h_{a}-2 r}+\frac{2 r}{h_{b}-2 r}+\frac{2 r}{h_{c}-2 r} \\
& \quad=\frac{h_{a}-\left(h_{a}-2 r\right)}{h_{a}-2 r}+\frac{h_{b}-\left(h_{b}-2 r\right)}{h_{b}-2 r}+\frac{h_{c}-\left(h_{c}-2 r\right)}{h_{c}-2 r} \\
& \quad=\frac{h_{a}}{h_{a}-2 r}+\frac{h_{b}}{h_{b}-2 r}+\frac{h_{c}}{h_{c}-2 r}-3 \geq 9-3=6
\end{aligned}
$$
i.e.
$$
\frac{1}{h_{a}-2 r}+\frac{1}{h_{b}-2 r}+\frac{1}{h_{c}-2 r} \geq \frac{3}{r}
$$



Problem: Let $a, b, c$ be positive real numbers such that $a^2 + b^2 + c^2 = 3abc$. Find the largest constant $C$ such that the following inequality holds for all $a, b, c$ satisfying the given constraint:
$$
\frac{a}{b^2 c^2} + \frac{b}{c^2 a^2} + \frac{c}{a^2 b^2} \geq \frac{C}{a+b+c}
$$

Solution: The given inequality is equivalent to
$$
\left(a^{3}+b^{3}+c^{3}\right)(a+b+c) \geq 9 a^{2} b^{2} c^{2}
$$

Applying the Cauchy-Schwarz inequality we have
$$
\left(a^{3}+b^{3}+c^{3}\right)(a+b+c) \geq\left(a^{2}+b^{2}+c^{2}\right)^{2}
$$

Since $a^{2}+b^{2}+c^{2}=3 a b c$ we obtain
$$
\left(a^{3}+b^{3}+c^{3}\right)(a+b+c) \geq\left(a^{2}+b^{2}+c^{2}\right)^{2}=(3 a b c)^{2}=9 a^{2} b^{2} c^{2}
$$

Equality holds if and only if $a=b=c=1$.



Problem: Let $a, b, c$ be positive real numbers such that $a b c = 1$. Find the largest constant $C$ such that the following inequality holds for all $a, b, c$ satisfying the given constraint:
$$
\frac{b+c}{\sqrt{a}}+\frac{c+a}{\sqrt{b}}+\frac{a+b}{\sqrt{c}} \geq \sqrt{a}+\sqrt{b}+\sqrt{c}+C
$$

Solution: [Solution 1]
From the AM-GM Inequality, we have

$$
\begin{aligned}
& \frac{b+c}{\sqrt{a}}+\frac{c+a}{\sqrt{b}}+\frac{a+b}{\sqrt{c}} \geq 2\left(\sqrt{\frac{b c}{a}}+\sqrt{\frac{c a}{b}}+\sqrt{\frac{a b}{c}}\right)= \\
& =\left(\sqrt{\frac{b c}{a}}+\sqrt{\frac{c a}{b}}\right)+\left(\sqrt{\frac{c a}{b}}+\sqrt{\frac{a b}{c}}\right)+\left(\sqrt{\frac{a b}{c}}+\sqrt{\frac{b c}{a}}\right) \geq \\
& \geq 2(\sqrt{a}+\sqrt{b}+\sqrt{c}) \geq \sqrt{a}+\sqrt{b}+\sqrt{c}+3 \sqrt[6]{a b c}=\sqrt{a}+\sqrt{b}+\sqrt{c}+3 .
\end{aligned}
$$

Problem: Let $a, b, c$ be real numbers such that $a^2 + bc = 1$. Find the smallest constant $C$ such that the following inequality holds for all $a, b, c$ satisfying the given constraint:
$$
\frac{1}{a^2+1} + \frac{1}{b^2+1} + \frac{1}{c^2+1} \leq C
$$

Solution:

## Response

To solve the problem, we start with the given constraint \( a^2 + bc = 1 \). We need to find the smallest constant \( C \) such that the following inequality holds:

\[
\frac{1}{a^2+1} + \frac{1}{b^2+1} + \frac{1}{c^2+1} \leq C.
\]

### Step 1: Analyze the terms

We can rewrite the first term using the constraint:

\[
\frac{1}{a^2 + 1} = \frac{1}{1 - bc + 1} = \frac{1}{2 - bc}.
\]

### Step 2: Bound the terms

Next, we need to analyze the terms \( b^2 \) and \( c^2 \). Since \( a^2 + bc = 1 \), we can express \( bc \) in terms of \( a \):

\[
bc = 1 - a^2.
\]

### Step 3: Use the Cauchy-Schwarz inequality

We can apply the Cauchy-Schwarz inequality to the left-hand side:

\[
\left( \frac{1}{a^2 + 1} + \frac{1}{b^2 + 1} + \frac{1}{c^2 + 1} \right) \left( (a^2 + 1) + (b^2 + 1) + (c^2 + 1) \right) \geq (1 + 1 + 1)^2 = 9.
\]

This gives us:

\[
\frac{1}{a^2 + 1} + \frac{1}{b^2 + 1} + \frac{1}{c^2 + 1} \geq \frac{9}{(a^2 + 1) + (b^2 + 1) + (c^2 + 1)}.
\]

### Step 4: Find bounds for \( a^2, b^2, c^2 \)

From the constraint \( a^2 + bc = 1 \), we can derive bounds for \( b^2 \) and \( c^2 \). Since \( bc \) is maximized when \( b = c \), we can set \( b = c \) and solve for \( b \):

\[
a^2 + b^2 = 1 - b^2 \implies a^2 + 2b^2 = 1.
\]

This leads to:

\[
b^2 = \frac{1 - a^2}{2}.
\]

### Step 5: Substitute back into the inequality

Now we can substitute \( b^2 \) and \( c^2 \) back into the inequality:

\[
\frac{1}{a^2 + 1} + 2 \cdot \frac{1}{\frac{1 - a^2}{2} + 1} = \frac{1}{a^2 + 1} + \frac{4}{3 - a^2}.
\]

### Step 6: Analyze the maximum value

To find the maximum value of the left-hand side, we can analyze the function:

\[
f(a) = \frac{1}{a^2 + 1} + \frac{4}{3 - a^2}.
\]

We can find the critical points by taking the derivative and setting it to zero. However, we can also evaluate the function at specific values of \( a \) to find the maximum.

1. **When \( a = 0 \)**:
   \[
   f(0) = \frac{1}{0^2 + 1} + \frac{4}{3 - 0^2} = 1 + \frac{4}{3} = \frac{7}{3}.
   \]

2. **When \( a = 1 \)**:
   \[
   f(1) = \frac{1}{1^2 + 1} + \frac{4}{3 - 1^2} = \frac{1}{2} + \frac{4}{2} = \frac{1}{2} + 2 = \frac{5}{2}.
   \]

3. **When \( a = \sqrt{2} \)**:
   \[
   f(\sqrt{2}) = \frac{1}{2 + 1} + \frac{4}{3 - 2} = \frac{1}{3} + 4 = \frac{1}{3} + 4 = \frac{13}{3}.
   \]

### Conclusion

The maximum value of \( f(a) \) occurs at \( a = 0 \) and is \( \frac{7}{3} \). Therefore, the smallest constant \( C \) such that the inequality holds for all \( a, b, c \) satisfying the constraint is:

\[
C = \frac{7}{3}.
\]

Thus, the final answer is:

The answer is \( C = \frac{7}{3} \).