## Problem

Let $x, y, z \in [-1, 3]$ such that $x + y + z = 3$. Find the smallest constant $C$ such that the following inequality holds for all $x, y, z$:
$$
x^2 + y^2 + z^2 \leq C.
$$

## Query

Task description: Please solve the problem with clear, rigorous, and logically sound steps. At the end of your response, state your answer in exactly this format: 'The answer is $C=X$', where X is your calculated numerical bound value. Example: 'The answer is $C=1$'.



Problem: Let $a, b, c$ be the side lengths, $h_{a}, h_{b}, h_{c}$ be the altitudes, respectively, and $r$ be the inradius of a triangle. Find the largest constant $C$ such that the following inequality holds for all triangles:
$$
\frac{1}{h_{a}-2 r}+\frac{1}{h_{b}-2 r}+\frac{1}{h_{c}-2 r} \geq C \cdot r
$$

Solution: By $\frac{1}{h_{a}}+\frac{1}{h_{b}}+\frac{1}{h_{c}}=\frac{1}{r}$ we obtain
$$
\frac{h_{a}-2 r}{h_{a}}+\frac{h_{b}-2 r}{h_{b}}+\frac{h_{c}-2 r}{h_{c}}=1
$$

Applying $A M \geq H M$ we get
$$
\left(\frac{h_{a}-2 r}{h_{a}}+\frac{h_{b}-2 r}{h_{b}}+\frac{h_{c}-2 r}{h_{c}}\right)\left(\frac{h_{a}}{h_{a}-2 r}+\frac{h_{b}}{h_{b}-2 r}+\frac{h_{c}}{h_{c}-2 r}\right) \geq 9
$$
i.e.
$$
\frac{h_{a}}{h_{a}-2 r}+\frac{h_{b}}{h_{b}-2 r}+\frac{h_{c}}{h_{c}-2 r} \geq 9
$$

Therefore
$$
\begin{aligned}
& \frac{2 r}{h_{a}-2 r}+\frac{2 r}{h_{b}-2 r}+\frac{2 r}{h_{c}-2 r} \\
& \quad=\frac{h_{a}-\left(h_{a}-2 r\right)}{h_{a}-2 r}+\frac{h_{b}-\left(h_{b}-2 r\right)}{h_{b}-2 r}+\frac{h_{c}-\left(h_{c}-2 r\right)}{h_{c}-2 r} \\
& \quad=\frac{h_{a}}{h_{a}-2 r}+\frac{h_{b}}{h_{b}-2 r}+\frac{h_{c}}{h_{c}-2 r}-3 \geq 9-3=6
\end{aligned}
$$
i.e.
$$
\frac{1}{h_{a}-2 r}+\frac{1}{h_{b}-2 r}+\frac{1}{h_{c}-2 r} \geq \frac{3}{r}
$$



Problem: Let $a, b, c$ be positive real numbers such that $a^2 + b^2 + c^2 = 3abc$. Find the largest constant $C$ such that the following inequality holds for all $a, b, c$ satisfying the given constraint:
$$
\frac{a}{b^2 c^2} + \frac{b}{c^2 a^2} + \frac{c}{a^2 b^2} \geq \frac{C}{a+b+c}
$$

Solution: The given inequality is equivalent to
$$
\left(a^{3}+b^{3}+c^{3}\right)(a+b+c) \geq 9 a^{2} b^{2} c^{2}
$$

Applying the Cauchy-Schwarz inequality we have
$$
\left(a^{3}+b^{3}+c^{3}\right)(a+b+c) \geq\left(a^{2}+b^{2}+c^{2}\right)^{2}
$$

Since $a^{2}+b^{2}+c^{2}=3 a b c$ we obtain
$$
\left(a^{3}+b^{3}+c^{3}\right)(a+b+c) \geq\left(a^{2}+b^{2}+c^{2}\right)^{2}=(3 a b c)^{2}=9 a^{2} b^{2} c^{2}
$$

Equality holds if and only if $a=b=c=1$.



Problem: Let $a, b, c$ be positive real numbers such that $a b c = 1$. Find the largest constant $C$ such that the following inequality holds for all $a, b, c$ satisfying the given constraint:
$$
\frac{b+c}{\sqrt{a}}+\frac{c+a}{\sqrt{b}}+\frac{a+b}{\sqrt{c}} \geq \sqrt{a}+\sqrt{b}+\sqrt{c}+C
$$

Solution: [Solution 1]
From the AM-GM Inequality, we have

$$
\begin{aligned}
& \frac{b+c}{\sqrt{a}}+\frac{c+a}{\sqrt{b}}+\frac{a+b}{\sqrt{c}} \geq 2\left(\sqrt{\frac{b c}{a}}+\sqrt{\frac{c a}{b}}+\sqrt{\frac{a b}{c}}\right)= \\
& =\left(\sqrt{\frac{b c}{a}}+\sqrt{\frac{c a}{b}}\right)+\left(\sqrt{\frac{c a}{b}}+\sqrt{\frac{a b}{c}}\right)+\left(\sqrt{\frac{a b}{c}}+\sqrt{\frac{b c}{a}}\right) \geq \\
& \geq 2(\sqrt{a}+\sqrt{b}+\sqrt{c}) \geq \sqrt{a}+\sqrt{b}+\sqrt{c}+3 \sqrt[6]{a b c}=\sqrt{a}+\sqrt{b}+\sqrt{c}+3 .
\end{aligned}
$$

Problem: Let $x, y, z \in [-1, 3]$ such that $x + y + z = 3$. Find the smallest constant $C$ such that the following inequality holds for all $x, y, z$:
$$
x^2 + y^2 + z^2 \leq C.
$$

Solution:

## Response

To solve the problem, we start with the given conditions: \( x, y, z \in [-1, 3] \) and \( x + y + z = 3 \). We need to find the smallest constant \( C \) such that the inequality 

\[
x^2 + y^2 + z^2 \leq C
\]

holds for all \( x, y, z \) satisfying these conditions.

First, we can use the identity that relates the sum of squares to the square of the sum:

\[
x^2 + y^2 + z^2 = (x + y + z)^2 - 2(xy + xz + yz).
\]

Since \( x + y + z = 3 \), we have:

\[
x^2 + y^2 + z^2 = 3^2 - 2(xy + xz + yz) = 9 - 2(xy + xz + yz).
\]

To maximize \( x^2 + y^2 + z^2 \), we need to minimize \( xy + xz + yz \). 

Next, we will analyze the possible values of \( x, y, z \) under the constraints \( x, y, z \in [-1, 3] \).

### Step 1: Finding the minimum of \( xy + xz + yz \)

To minimize \( xy + xz + yz \), we can consider the extreme values of \( x, y, z \) within the given bounds. 

1. **Case 1**: Let \( x = 3 \), \( y = 3 \), and \( z = -3 \) (not valid since \( z \) must be in \([-1, 3]\)).
2. **Case 2**: Let \( x = 3 \), \( y = 1 \), and \( z = -1 \):
   - Here, \( x + y + z = 3 + 1 - 1 = 3 \).
   - Calculate \( xy + xz + yz = 3 \cdot 1 + 3 \cdot (-1) + 1 \cdot (-1) = 3 - 3 - 1 = -1 \).

3. **Case 3**: Let \( x = 1 \), \( y = 1 \), and \( z = 1 \):
   - Here, \( x + y + z = 1 + 1 + 1 = 3 \).
   - Calculate \( xy + xz + yz = 1 \cdot 1 + 1 \cdot 1 + 1 \cdot 1 = 3 \).

4. **Case 4**: Let \( x = -1 \), \( y = -1 \), and \( z = 5 \) (not valid since \( z \) must be in \([-1, 3]\)).
5. **Case 5**: Let \( x = -1 \), \( y = 3 \), and \( z = 1 \):
   - Here, \( x + y + z = -1 + 3 + 1 = 3 \).
   - Calculate \( xy + xz + yz = (-1) \cdot 3 + (-1) \cdot 1 + 3 \cdot 1 = -3 - 1 + 3 = -1 \).

### Step 2: Calculate \( x^2 + y^2 + z^2 \)

Now we can calculate \( x^2 + y^2 + z^2 \) for the cases we found:

1. For \( (3, 1, -1) \):
   \[
   x^2 + y^2 + z^2 = 3^2 + 1^2 + (-1)^2 = 9 + 1 + 1 = 11.
   \]

2. For \( (1, 1, 1) \):
   \[
   x^2 + y^2 + z^2 = 1^2 + 1^2 + 1^2 = 1 + 1 + 1 = 3.
   \]

3. For \( (-1, 3, 1) \):
   \[
   x^2 + y^2 + z^2 = (-1)^2 + 3^2 + 1^2 = 1 + 9 + 1 = 11.
   \]

### Conclusion

The maximum value of \( x^2 + y^2 + z^2 \) we found is \( 11 \). Therefore, the smallest constant \( C \) such that 

\[
x^2 + y^2 + z^2 \leq C
\]

for all \( x, y, z \) satisfying the given conditions is 

\[
C = 11.
\]

Thus, the final answer is:

The answer is \( C=11 \).