## Problem

Let $a, b, c > 0$ such that $a+b+c=2$ and $a^2+b^2+c^2=2$. Determine the minimal constant $C$ such that the following inequality holds for all $a, b, c$ satisfying the given constraints:
$$
a b c \leq C.
$$

## Query

Task description: Please solve the problem with clear, rigorous, and logically sound steps. At the end of your response, state your answer in exactly this format: 'The answer is $C=X$', where X is your calculated numerical bound value. Example: 'The answer is $C=1$'.



Problem: Let $a, b, c$ be the side lengths, $h_{a}, h_{b}, h_{c}$ be the altitudes, respectively, and $r$ be the inradius of a triangle. Find the largest constant $C$ such that the following inequality holds for all triangles:
$$
\frac{1}{h_{a}-2 r}+\frac{1}{h_{b}-2 r}+\frac{1}{h_{c}-2 r} \geq C \cdot r
$$

Solution: By $\frac{1}{h_{a}}+\frac{1}{h_{b}}+\frac{1}{h_{c}}=\frac{1}{r}$ we obtain
$$
\frac{h_{a}-2 r}{h_{a}}+\frac{h_{b}-2 r}{h_{b}}+\frac{h_{c}-2 r}{h_{c}}=1
$$

Applying $A M \geq H M$ we get
$$
\left(\frac{h_{a}-2 r}{h_{a}}+\frac{h_{b}-2 r}{h_{b}}+\frac{h_{c}-2 r}{h_{c}}\right)\left(\frac{h_{a}}{h_{a}-2 r}+\frac{h_{b}}{h_{b}-2 r}+\frac{h_{c}}{h_{c}-2 r}\right) \geq 9
$$
i.e.
$$
\frac{h_{a}}{h_{a}-2 r}+\frac{h_{b}}{h_{b}-2 r}+\frac{h_{c}}{h_{c}-2 r} \geq 9
$$

Therefore
$$
\begin{aligned}
& \frac{2 r}{h_{a}-2 r}+\frac{2 r}{h_{b}-2 r}+\frac{2 r}{h_{c}-2 r} \\
& \quad=\frac{h_{a}-\left(h_{a}-2 r\right)}{h_{a}-2 r}+\frac{h_{b}-\left(h_{b}-2 r\right)}{h_{b}-2 r}+\frac{h_{c}-\left(h_{c}-2 r\right)}{h_{c}-2 r} \\
& \quad=\frac{h_{a}}{h_{a}-2 r}+\frac{h_{b}}{h_{b}-2 r}+\frac{h_{c}}{h_{c}-2 r}-3 \geq 9-3=6
\end{aligned}
$$
i.e.
$$
\frac{1}{h_{a}-2 r}+\frac{1}{h_{b}-2 r}+\frac{1}{h_{c}-2 r} \geq \frac{3}{r}
$$



Problem: Let $a, b, c$ be positive real numbers such that $a^2 + b^2 + c^2 = 3abc$. Find the largest constant $C$ such that the following inequality holds for all $a, b, c$ satisfying the given constraint:
$$
\frac{a}{b^2 c^2} + \frac{b}{c^2 a^2} + \frac{c}{a^2 b^2} \geq \frac{C}{a+b+c}
$$

Solution: The given inequality is equivalent to
$$
\left(a^{3}+b^{3}+c^{3}\right)(a+b+c) \geq 9 a^{2} b^{2} c^{2}
$$

Applying the Cauchy-Schwarz inequality we have
$$
\left(a^{3}+b^{3}+c^{3}\right)(a+b+c) \geq\left(a^{2}+b^{2}+c^{2}\right)^{2}
$$

Since $a^{2}+b^{2}+c^{2}=3 a b c$ we obtain
$$
\left(a^{3}+b^{3}+c^{3}\right)(a+b+c) \geq\left(a^{2}+b^{2}+c^{2}\right)^{2}=(3 a b c)^{2}=9 a^{2} b^{2} c^{2}
$$

Equality holds if and only if $a=b=c=1$.



Problem: Let $a, b, c$ be positive real numbers such that $a b c = 1$. Find the largest constant $C$ such that the following inequality holds for all $a, b, c$ satisfying the given constraint:
$$
\frac{b+c}{\sqrt{a}}+\frac{c+a}{\sqrt{b}}+\frac{a+b}{\sqrt{c}} \geq \sqrt{a}+\sqrt{b}+\sqrt{c}+C
$$

Solution: [Solution 1]
From the AM-GM Inequality, we have

$$
\begin{aligned}
& \frac{b+c}{\sqrt{a}}+\frac{c+a}{\sqrt{b}}+\frac{a+b}{\sqrt{c}} \geq 2\left(\sqrt{\frac{b c}{a}}+\sqrt{\frac{c a}{b}}+\sqrt{\frac{a b}{c}}\right)= \\
& =\left(\sqrt{\frac{b c}{a}}+\sqrt{\frac{c a}{b}}\right)+\left(\sqrt{\frac{c a}{b}}+\sqrt{\frac{a b}{c}}\right)+\left(\sqrt{\frac{a b}{c}}+\sqrt{\frac{b c}{a}}\right) \geq \\
& \geq 2(\sqrt{a}+\sqrt{b}+\sqrt{c}) \geq \sqrt{a}+\sqrt{b}+\sqrt{c}+3 \sqrt[6]{a b c}=\sqrt{a}+\sqrt{b}+\sqrt{c}+3 .
\end{aligned}
$$

Problem: Let $a, b, c > 0$ such that $a+b+c=2$ and $a^2+b^2+c^2=2$. Determine the minimal constant $C$ such that the following inequality holds for all $a, b, c$ satisfying the given constraints:
$$
a b c \leq C.
$$

Solution:

## Response

To solve the problem, we start with the given conditions:

1. \( a + b + c = 2 \)
2. \( a^2 + b^2 + c^2 = 2 \)

From the second condition, we can use the identity:

\[
a^2 + b^2 + c^2 = (a + b + c)^2 - 2(ab + ac + bc)
\]

Substituting the first condition into this identity gives:

\[
2 = 2^2 - 2(ab + ac + bc)
\]

This simplifies to:

\[
2 = 4 - 2(ab + ac + bc) \implies 2(ab + ac + bc) = 2 \implies ab + ac + bc = 1
\]

Now we have the following relationships:

- \( a + b + c = 2 \)
- \( ab + ac + bc = 1 \)

Next, we want to find the maximum value of \( abc \). We can use the method of Lagrange multipliers or apply the AM-GM inequality. However, we will use the symmetric nature of the problem and the relationships we have derived.

Using the identity for the product of the roots of a cubic polynomial, we can express \( abc \) in terms of \( a + b + c \) and \( ab + ac + bc \). The polynomial whose roots are \( a, b, c \) can be expressed as:

\[
x^3 - (a+b+c)x^2 + (ab+ac+bc)x - abc = 0
\]

Substituting our known values:

\[
x^3 - 2x^2 + x - abc = 0
\]

To find the maximum value of \( abc \), we can apply the AM-GM inequality directly to \( a, b, c \):

\[
\frac{a + b + c}{3} \geq \sqrt[3]{abc}
\]

Substituting \( a + b + c = 2 \):

\[
\frac{2}{3} \geq \sqrt[3]{abc} \implies abc \leq \left(\frac{2}{3}\right)^3 = \frac{8}{27}
\]

Now we need to check if this maximum can be achieved under the constraints. 

Assume \( a = b \) and \( c = 2 - 2a \). Then we have:

\[
a^2 + a^2 + (2 - 2a)^2 = 2
\]

This simplifies to:

\[
2a^2 + (4 - 8a + 4a^2) = 2 \implies 6a^2 - 8a + 2 = 0
\]

Using the quadratic formula:

\[
a = \frac{8 \pm \sqrt{(-8)^2 - 4 \cdot 6 \cdot 2}}{2 \cdot 6} = \frac{8 \pm \sqrt{64 - 48}}{12} = \frac{8 \pm \sqrt{16}}{12} = \frac{8 \pm 4}{12}
\]

This gives us:

\[
a = 1 \quad \text{or} \quad a = \frac{1}{3}
\]

If \( a = 1 \), then \( b = 1 \) and \( c = 0 \), which does not satisfy \( a, b, c > 0 \).

If \( a = \frac{1}{3} \), then \( b = \frac{1}{3} \) and \( c = \frac{4}{3} \). We can calculate \( abc \):

\[
abc = \frac{1}{3} \cdot \frac{1}{3} \cdot \frac{4}{3} = \frac{4}{27}
\]

This value is less than \( \frac{8}{27} \). 

To check if \( abc = \frac{8}{27} \) can be achieved, we can set \( a = b = c = \frac{2}{3} \):

\[
abc = \left(\frac{2}{3}\right)^3 = \frac{8}{27}
\]

This satisfies both conditions:

1. \( a + b + c = 2 \)
2. \( a^2 + b^2 + c^2 = 2 \)

Thus, the maximum value of \( abc \) is \( \frac{8}{27} \).

Therefore, the largest constant \( C \) such that \( abc \leq C \) for all \( a, b, c \) satisfying the given constraints is:

\[
\text{The answer is } C = \frac{8}{27}.
\]