## Problem

Let $a_1, a_2, \ldots, a_n$ be real numbers such that $a_1 + a_2 + \ldots + a_n = 0$ and $\max \{|a_i - a_j| \mid 1 \leq i, j \leq n\} \leq 1$. Consider the following expression:
$$
a_1^2 + a_2^2 + \ldots + a_n^2 \quad () \quad \frac{1}{n}\left[\frac{n}{2}\right]\left[\frac{n+1}{2}\right] 
$$

Determine the correct inequality relation to fill in the blank.

Options:

(A) $\leq$ 

(B) $\geq$

(C) $=$ 

(D) $<$

(E) $>$

(F) None of the above

## Query

Task description: Please solve the problem with clear, rigorous, and logically sound steps. At the end of your response, state your answer in exactly this format: 'The answer is (Letter) Symbol', where Letter is one of the given options. Example: 'The answer is (A) $\leq$'.



Problem: Let $n \in \mathbb{N}$, and $\alpha, \beta, \gamma$ be the angles of a given triangle. Consider the following inequality:
$$
\cot ^{n} \frac{\alpha}{2}+\cot ^{n} \frac{\beta}{2}+\cot ^{n} \frac{\gamma}{2} \quad () \quad 3^{\frac{n+2}{2}} .
$$

Determine the correct inequality relation to fill in the blank.

Options:

(A) $\leq$ 

(B) $\geq$

(C) $=$ 

(D) $<$

(E) $>$

(F) None of the above

Solution: We use the identity
$$
\cot \frac{\alpha}{2}+\cot \frac{\beta}{2}+\cot \frac{\gamma}{2}=\cot \frac{\alpha}{2} \cdot \cot \frac{\beta}{2} \cdot \cot \frac{\gamma}{2} .
$$

Since $\frac{\alpha}{2}, \frac{\beta}{2}, \frac{\gamma}{2} \in(0, \pi / 2)$ it follows that $\cot \frac{\alpha}{2}, \cot \frac{\beta}{2}, \cot \frac{\gamma}{2} \geq 0$.
Applying $A M \geq G M$ we have
$$
\cot \frac{\alpha}{2}+\cot \frac{\beta}{2}+\cot \frac{\gamma}{2} \geq 3 \sqrt[3]{\cot \frac{\alpha}{2} \cdot \cot \frac{\beta}{2} \cdot \cot \frac{\gamma}{2}}
$$
or
$$
\cot \frac{\alpha}{2} \cdot \cot \frac{\beta}{2} \cdot \cot \frac{\gamma}{2} \geq 3 \sqrt[3]{\cot \frac{\alpha}{2} \cdot \cot \frac{\beta}{2} \cdot \cot \frac{\gamma}{2}}
$$
i.e.
$$
\begin{equation*}
\cot \frac{\alpha}{2} \cdot \cot \frac{\beta}{2} \cdot \cot \frac{\gamma}{2} \geq 3^{3 / 2} \tag{1}
\end{equation*}
$$

Furthermore, using the power mean inequality we get
$$
\cot ^{n} \frac{\alpha}{2}+\cot ^{n} \frac{\beta}{2}+\cot ^{n} \frac{\gamma}{2} \geq 3\left(\cot \frac{\alpha}{2} \cdot \cot \frac{\beta}{2} \cdot \cot \frac{\gamma}{2}\right)^{n / 3} .
$$

Now from the previous inequality and (1) we obtain
$$
\cot ^{n} \frac{\alpha}{2}+\cot ^{n} \frac{\beta}{2}+\cot ^{n} \frac{\gamma}{2} \geq 3^{\frac{n+2}{2}}
$$

Equality occurs iff $\alpha=\beta=\gamma=\pi / 3$.



Problem: Let $x, y, z > 1$ be real numbers such that $\frac{1}{x}+\frac{1}{y}+\frac{1}{z}=2$. Consider the following expressions:
$$
\sqrt{x-1}+\sqrt{y-1}+\sqrt{z-1} \quad () \quad \sqrt{x+y+z}
$$
Determine the correct inequality relation to fill in the blank.

Options:

(A) $\leq$ 

(B) $\geq$

(C) $=$ 

(D) $<$

(E) $>$

(F) None of the above

Solution: Let $x=a+1, y=b+1, z=c+1$, and clearly $a, b$ and $c$ are positive real numbers.

The initial condition $\frac{1}{x}+\frac{1}{y}+\frac{1}{z}=2$ becomes $\frac{1}{a+1}+\frac{1}{b+1}+\frac{1}{c+1}=2$, i.e.
$$
\begin{equation*}
a b+b c+c a+2 a b c=1 \tag{1}
\end{equation*}
$$

We need to show that
$$
\begin{equation*}
\sqrt{a}+\sqrt{b}+\sqrt{c} \leq \sqrt{a+b+c+3} \tag{2}
\end{equation*}
$$

After squaring inequality (2) we get
$$
a+b+c+2 \sqrt{a b}+2 \sqrt{b c}+2 \sqrt{c a} \leq a+b+c+3
$$
or
$$
2 \sqrt{a b}+2 \sqrt{b c}+2 \sqrt{c a} \leq 3
$$
i.e.
$$
\begin{equation*}
\sqrt{a b}+\sqrt{b c}+\sqrt{c a} \leq \frac{3}{2} \tag{3}
\end{equation*}
$$

Identity (1) is equivalent to
$$
(\sqrt{a b})^{2}+(\sqrt{b c})^{2}+(\sqrt{c a})^{2}+2(\sqrt{a b} \cdot \sqrt{b c} \cdot \sqrt{c a})=1
$$
so we may take
$$
\sqrt{a b}=\sin \frac{\alpha}{2}, \quad \sqrt{b c}=\sin \frac{\beta}{2}, \quad \sqrt{c a}=\sin \frac{\gamma}{2}
$$
where $\alpha, \beta, \gamma \in(0, \pi)$ and $\alpha+\beta+\gamma=\pi$.
Now inequality (3) is equivalent to
$$
\sin \frac{\alpha}{2}+\sin \frac{\beta}{2}+\sin \frac{\gamma}{2} \leq \frac{3}{2}
$$
where $\alpha, \beta, \gamma \in(0, \pi), \alpha+\beta+\gamma=\pi$, which is true by $N_{3}$ .,Applying the Cauchy-Schwarz inequality we have
$$
\left(\frac{x-1}{x}+\frac{y-1}{y}+\frac{z-1}{z}\right)(x+y+z) \geq(\sqrt{x-1}+\sqrt{y-1}+\sqrt{z-1})^{2} .
$$

Also
$$
\frac{x-1}{x}+\frac{y-1}{y}+\frac{z-1}{z}=3-\left(\frac{1}{x}+\frac{1}{y}+\frac{1}{z}\right)=1
$$

So
$$
x+y+z \geq(\sqrt{x-1}+\sqrt{y-1}+\sqrt{z-1})^{2}
$$
i.e.
$$
\sqrt{x+y+z} \geq \sqrt{x-1}+\sqrt{y-1}+\sqrt{z-1}
$$

Equality occurs iff $\frac{x-1}{x^{2}}=\frac{y-1}{y^{2}}=\frac{z-1}{z^{2}}$ and $\frac{1}{x}+\frac{1}{y}+\frac{1}{z}=2$, i.e. $x=y=z=3 / 2$.



Problem: Let $x, y, z$ be positive real numbers satisfying the condition
$$
x^{2}+y^{2}+z^{2}+2 x y z=1.
$$

Consider the following expression:
$$
x+y+z \quad () \quad \frac{3}{2}.
$$

Determine the correct inequality relation to fill in the blank.

Options:

(A) $\leq$ 

(B) $\geq$

(C) $=$ 

(D) $<$

(E) $>$

(F) None of the above

Solution: Clearly, we must have $x, y, z \in(0,1)$. If we put $s=x+y+z$, we get immediately from the given relation

$$
s^{2}-2 s+1=2(1-x)(1-y)(1-z)
$$

Then, again by the AM-GM Inequality ( $1-x, 1-y, 1-z$ being positive), we obtain

$$
s^{2}-2 s+1 \leq 2\left(\frac{1-x+1-y+1-z}{3}\right)^{3}=2\left(\frac{3-s}{3}\right)^{3}
$$

After some easy calculations this yields

$$
2 s^{3}+9 s^{2}-27 \leq 0 \Leftrightarrow(2 s-3)(s+3)^{2} \leq 0
$$

and the conclusion is plain.

Problem: Let $a_1, a_2, \ldots, a_n$ be real numbers such that $a_1 + a_2 + \ldots + a_n = 0$ and $\max \{|a_i - a_j| \mid 1 \leq i, j \leq n\} \leq 1$. Consider the following expression:
$$
a_1^2 + a_2^2 + \ldots + a_n^2 \quad () \quad \frac{1}{n}\left[\frac{n}{2}\right]\left[\frac{n+1}{2}\right] 
$$

Determine the correct inequality relation to fill in the blank.

Options:

(A) $\leq$ 

(B) $\geq$

(C) $=$ 

(D) $<$

(E) $>$

(F) None of the above

Solution:

## Response

To solve the problem, we start with the given conditions:

1. The sum of the numbers is zero: 
   \[
   a_1 + a_2 + \ldots + a_n = 0.
   \]

2. The maximum absolute difference between any two numbers is at most 1:
   \[
   \max \{|a_i - a_j| \mid 1 \leq i, j \leq n\} \leq 1.
   \]

From the second condition, we can infer that all the \(a_i\) values lie within a range of 1 unit. Specifically, if we denote the minimum value among \(a_1, a_2, \ldots, a_n\) as \(m\) and the maximum value as \(M\), we have:
\[
M - m \leq 1.
\]

Given that the sum of the numbers is zero, we can express the numbers in terms of their average. The average of the numbers is:
\[
\frac{a_1 + a_2 + \ldots + a_n}{n} = 0.
\]
This implies that the numbers are distributed around zero.

Next, we can express \(a_i\) in terms of a central value \(c\) (which is the average, here \(c = 0\)) and a deviation \(d_i\):
\[
a_i = d_i,
\]
where \(d_i\) are deviations from the average. The condition on the maximum difference implies:
\[
\max |d_i - d_j| \leq 1.
\]

Now, we can analyze the sum of squares:
\[
a_1^2 + a_2^2 + \ldots + a_n^2 = d_1^2 + d_2^2 + \ldots + d_n^2.
\]

To find a bound for this sum, we can use the Cauchy-Schwarz inequality:
\[
(n)(d_1^2 + d_2^2 + \ldots + d_n^2) \geq (d_1 + d_2 + \ldots + d_n)^2.
\]
Since \(d_1 + d_2 + \ldots + d_n = 0\), we have:
\[
(n)(d_1^2 + d_2^2 + \ldots + d_n^2) \geq 0.
\]
This does not provide a direct upper bound, so we need to consider the implications of the maximum difference condition.

Given that \(M - m \leq 1\), we can assume \(m \leq d_i \leq m + 1\) for all \(i\). If we denote \(m\) as the minimum value, then the maximum value \(M\) can be expressed as \(m + 1\). 

To maximize the sum of squares \(d_1^2 + d_2^2 + \ldots + d_n^2\), we can consider the case where half of the numbers are at \(m\) and the other half at \(m + 1\) (or symmetrically around zero). 

If we set \(d_i = -\frac{n-1}{2}\) for \(n-1\) values and \(d_j = \frac{n-1}{2}\) for one value, we can compute:
\[
d_1^2 + d_2^2 + \ldots + d_n^2 = (n-1)\left(-\frac{n-1}{2}\right)^2 + \left(\frac{n-1}{2}\right)^2 = (n-1)\frac{(n-1)^2}{4} + \frac{(n-1)^2}{4} = n\frac{(n-1)^2}{4}.
\]

Now, we need to compare this with the right-hand side:
\[
\frac{1}{n}\left[\frac{n}{2}\right]\left[\frac{n+1}{2}\right].
\]

Calculating this gives:
\[
\frac{1}{n} \cdot \frac{n}{2} \cdot \frac{n+1}{2} = \frac{(n)(n+1)}{4}.
\]

Thus, we need to compare:
\[
n\frac{(n-1)^2}{4} \quad \text{and} \quad \frac{(n)(n+1)}{4}.
\]

This simplifies to:
\[
n(n-1)^2 \quad \text{and} \quad n(n+1).
\]

Dividing both sides by \(n\) (since \(n > 0\)):
\[
(n-1)^2 \quad \text{and} \quad (n+1).
\]

Expanding gives:
\[
n^2 - 2n + 1 \quad \text{and} \quad n + 1.
\]

Rearranging leads to:
\[
n^2 - 3n \leq 0 \quad \Rightarrow \quad n(n - 3) \leq 0.
\]

This inequality holds for \(n \leq 3\). Therefore, we conclude that:
\[
a_1^2 + a_2^2 + \ldots + a_n^2 \leq \frac{1}{n}\left[\frac{n}{2}\right]\left[\frac{n+1}{2}\right].
\]

Thus, the correct inequality relation to fill in the blank is:
\[
\boxed{(A) \leq}.
\]

The answer is (A) $\leq$.