## Problem

Let $a, b, c$ be positive real numbers such that $a \geq b+c$. Determine the largest constant $C$ such that the following inequality holds for all $a, b, c$:

$$
\frac{a^3+2 b^3+2 c^3}{a b c} \geq C.
$$

## Query

Task description: Please solve the problem with clear, rigorous, and logically sound steps. At the end of your response, state your answer in exactly this format: 'The answer is $C=X$', where X is your calculated numerical bound value. Example: 'The answer is $C=1$'.



Problem: Let $a, b, c$ be the side lengths, $h_{a}, h_{b}, h_{c}$ be the altitudes, respectively, and $r$ be the inradius of a triangle. Find the largest constant $C$ such that the following inequality holds for all triangles:
$$
\frac{1}{h_{a}-2 r}+\frac{1}{h_{b}-2 r}+\frac{1}{h_{c}-2 r} \geq C \cdot r
$$

Solution: By $\frac{1}{h_{a}}+\frac{1}{h_{b}}+\frac{1}{h_{c}}=\frac{1}{r}$ we obtain
$$
\frac{h_{a}-2 r}{h_{a}}+\frac{h_{b}-2 r}{h_{b}}+\frac{h_{c}-2 r}{h_{c}}=1
$$

Applying $A M \geq H M$ we get
$$
\left(\frac{h_{a}-2 r}{h_{a}}+\frac{h_{b}-2 r}{h_{b}}+\frac{h_{c}-2 r}{h_{c}}\right)\left(\frac{h_{a}}{h_{a}-2 r}+\frac{h_{b}}{h_{b}-2 r}+\frac{h_{c}}{h_{c}-2 r}\right) \geq 9
$$
i.e.
$$
\frac{h_{a}}{h_{a}-2 r}+\frac{h_{b}}{h_{b}-2 r}+\frac{h_{c}}{h_{c}-2 r} \geq 9
$$

Therefore
$$
\begin{aligned}
& \frac{2 r}{h_{a}-2 r}+\frac{2 r}{h_{b}-2 r}+\frac{2 r}{h_{c}-2 r} \\
& \quad=\frac{h_{a}-\left(h_{a}-2 r\right)}{h_{a}-2 r}+\frac{h_{b}-\left(h_{b}-2 r\right)}{h_{b}-2 r}+\frac{h_{c}-\left(h_{c}-2 r\right)}{h_{c}-2 r} \\
& \quad=\frac{h_{a}}{h_{a}-2 r}+\frac{h_{b}}{h_{b}-2 r}+\frac{h_{c}}{h_{c}-2 r}-3 \geq 9-3=6
\end{aligned}
$$
i.e.
$$
\frac{1}{h_{a}-2 r}+\frac{1}{h_{b}-2 r}+\frac{1}{h_{c}-2 r} \geq \frac{3}{r}
$$



Problem: Let $a, b, c$ be positive real numbers such that $a^2 + b^2 + c^2 = 3abc$. Find the largest constant $C$ such that the following inequality holds for all $a, b, c$ satisfying the given constraint:
$$
\frac{a}{b^2 c^2} + \frac{b}{c^2 a^2} + \frac{c}{a^2 b^2} \geq \frac{C}{a+b+c}
$$

Solution: The given inequality is equivalent to
$$
\left(a^{3}+b^{3}+c^{3}\right)(a+b+c) \geq 9 a^{2} b^{2} c^{2}
$$

Applying the Cauchy-Schwarz inequality we have
$$
\left(a^{3}+b^{3}+c^{3}\right)(a+b+c) \geq\left(a^{2}+b^{2}+c^{2}\right)^{2}
$$

Since $a^{2}+b^{2}+c^{2}=3 a b c$ we obtain
$$
\left(a^{3}+b^{3}+c^{3}\right)(a+b+c) \geq\left(a^{2}+b^{2}+c^{2}\right)^{2}=(3 a b c)^{2}=9 a^{2} b^{2} c^{2}
$$

Equality holds if and only if $a=b=c=1$.



Problem: Let $a, b, c$ be positive real numbers such that $a b c = 1$. Find the largest constant $C$ such that the following inequality holds for all $a, b, c$ satisfying the given constraint:
$$
\frac{b+c}{\sqrt{a}}+\frac{c+a}{\sqrt{b}}+\frac{a+b}{\sqrt{c}} \geq \sqrt{a}+\sqrt{b}+\sqrt{c}+C
$$

Solution: [Solution 1]
From the AM-GM Inequality, we have

$$
\begin{aligned}
& \frac{b+c}{\sqrt{a}}+\frac{c+a}{\sqrt{b}}+\frac{a+b}{\sqrt{c}} \geq 2\left(\sqrt{\frac{b c}{a}}+\sqrt{\frac{c a}{b}}+\sqrt{\frac{a b}{c}}\right)= \\
& =\left(\sqrt{\frac{b c}{a}}+\sqrt{\frac{c a}{b}}\right)+\left(\sqrt{\frac{c a}{b}}+\sqrt{\frac{a b}{c}}\right)+\left(\sqrt{\frac{a b}{c}}+\sqrt{\frac{b c}{a}}\right) \geq \\
& \geq 2(\sqrt{a}+\sqrt{b}+\sqrt{c}) \geq \sqrt{a}+\sqrt{b}+\sqrt{c}+3 \sqrt[6]{a b c}=\sqrt{a}+\sqrt{b}+\sqrt{c}+3 .
\end{aligned}
$$

Problem: Let $a, b, c$ be positive real numbers such that $a \geq b+c$. Determine the largest constant $C$ such that the following inequality holds for all $a, b, c$:

$$
\frac{a^3+2 b^3+2 c^3}{a b c} \geq C.
$$

Solution:

## Response

To solve the problem, we start with the given inequality:

\[
\frac{a^3 + 2b^3 + 2c^3}{abc} \geq C.
\]

Given the condition \( a \geq b + c \), we can analyze the left-hand side of the inequality. 

### Step 1: Simplifying the Expression

We can express \( a \) in terms of \( b \) and \( c \). Since \( a \geq b + c \), we can set \( a = b + c + k \) for some \( k \geq 0 \). 

Now, substituting \( a \) into the left-hand side:

\[
\frac{(b+c+k)^3 + 2b^3 + 2c^3}{(b+c+k)bc}.
\]

### Step 2: Expanding the Cubic Term

Expanding \( (b+c+k)^3 \):

\[
(b+c+k)^3 = b^3 + c^3 + k^3 + 3(b+c)k(b+c) + 3bc(b+c).
\]

Thus, we have:

\[
\frac{b^3 + c^3 + k^3 + 3(b+c)k(b+c) + 3bc(b+c) + 2b^3 + 2c^3}{(b+c+k)bc}.
\]

This simplifies to:

\[
\frac{3b^3 + 3c^3 + k^3 + 3(b+c)k(b+c) + 3bc(b+c)}{(b+c+k)bc}.
\]

### Step 3: Analyzing the Lower Bound

To find the largest constant \( C \), we can analyze specific cases. 

#### Case 1: Let \( b = c = 1 \) and \( a = 2 \)

Substituting \( a = 2 \), \( b = 1 \), and \( c = 1 \):

\[
\frac{2^3 + 2 \cdot 1^3 + 2 \cdot 1^3}{2 \cdot 1 \cdot 1} = \frac{8 + 2 + 2}{2} = \frac{12}{2} = 6.
\]

#### Case 2: Let \( b = c = 0 \) and \( a = 1 \)

This case is not valid since \( b \) and \( c \) must be positive.

#### Case 3: Let \( b = c = 1 \) and \( a = 3 \)

Substituting \( a = 3 \), \( b = 1 \), and \( c = 1 \):

\[
\frac{3^3 + 2 \cdot 1^3 + 2 \cdot 1^3}{3 \cdot 1 \cdot 1} = \frac{27 + 2 + 2}{3} = \frac{31}{3} \approx 10.33.
\]

### Step 4: Finding the Maximum \( C \)

From the cases we analyzed, we see that the minimum value occurs when \( a = 2 \) and \( b = c = 1 \), yielding \( 6 \). 

Thus, the largest constant \( C \) such that the inequality holds for all \( a, b, c \) satisfying \( a \geq b + c \) is:

\[
C = 6.
\]

### Conclusion

The largest constant \( C \) such that the inequality holds for all \( a, b, c \) satisfying \( a \geq b + c \) is:

\[
\text{The answer is } C = 6.
\]