## Problem

Let $x, y, z > 1$ be real numbers such that $\frac{1}{x} + \frac{1}{y} + \frac{1}{z} = 2$. Consider the following inequality:
$$
\sqrt{2x+3y+z} \quad () \quad \sqrt{x-1} + \sqrt{y-1} + \sqrt{z-1} .
$$

Determine the correct inequality relation to fill in the blank.

Options:

(A) $\leq$ 

(B) $\geq$

(C) $=$ 

(D) $<$

(E) $>$

(F) None of the above

## Query

Task description: Please solve the problem with clear, rigorous, and logically sound steps. At the end of your response, state your answer in exactly this format: 'The answer is (Letter) Symbol', where Letter is one of the given options. Example: 'The answer is (A) $\leq$'.

Problem: Let $x, y, z > 1$ be real numbers such that $\frac{1}{x} + \frac{1}{y} + \frac{1}{z} = 2$. Consider the following inequality:
$$
\sqrt{2x+3y+z} \quad () \quad \sqrt{x-1} + \sqrt{y-1} + \sqrt{z-1} .
$$

Determine the correct inequality relation to fill in the blank.

Options:

(A) $\leq$ 

(B) $\geq$

(C) $=$ 

(D) $<$

(E) $>$

(F) None of the above

Please use some of the following theorems to solve the problem:
Theorem 1 (Category: Inequality Between Means, Nicknames: mean inequalities): Let $a_{1}, a_{2}, \ldots, a_{n}$ be positive real numbers. The numbers
$$
\begin{aligned}
& Q M=\sqrt{\frac{a_{1}^{2}+a_{2}^{2}+\cdots+a_{n}^{2}}{n}}, \quad A M=\frac{a_{1}+a_{2}+\cdots+a_{n}}{n} \\
& G M=\sqrt[n]{a_{1} a_{2} \cdots a_{n}} \quad \text { and } \quad H M=\frac{n}{\frac{1}{a_{1}}+\frac{1}{a_{2}}+\cdots+\frac{1}{a_{n}}}
\end{aligned}
$$
are called the quadratic, arithmetic, geometric and harmonic mean for the numbers $a_{1}, a_{2}, \ldots, a_{n}$, respectively, and we have
$$
Q M \geq A M \geq G M \geq H M
$$

Equalities occur if and only if $a_{1}=a_{2}=\cdots=a_{n}$.

Theorem 2 (Category: Cauchy-Schwarz Inequality, Nicknames: cauchy-schwarz inequality): Let $a_{1}, a_{2}, \ldots, a_{n}$ and $b_{1}, b_{2}$, $\ldots, b_{n}$ be real numbers. Then we have
$$
\left(\sum_{i=1}^{n} a_{i}^{2}\right)\left(\sum_{i=1}^{n} b_{i}^{2}\right) \geq\left(\sum_{i=1}^{n} a_{i} b_{i}\right)^{2}
$$
i.e.
$$
\left(a_{1}^{2}+a_{2}^{2}+\cdots+a_{n}^{2}\right)\left(b_{1}^{2}+b_{2}^{2}+\cdots+b_{n}^{2}\right) \geq\left(a_{1} b_{1}+a_{2} b_{2}+\cdots+a_{n} b_{n}\right)^{2}
$$

Equality occurs if and only if the sequences $\left(a_{1}, a_{2}, \ldots, a_{n}\right)$ and $\left(b_{1}, b_{2}\right.$, $\ldots, b_{n}$ ) are proportional, i.e. $\frac{a_{1}}{b_{1}}=\frac{a_{2}}{b_{2}}=\cdots=\frac{a_{n}}{b_{n}}$.

Theorem 3 (Category: Inequality Between Means, Nicknames: am-gm (arithmetic mean-geometric mean) inequality, am-gm): If $a_{1}, a_{2}, \ldots, a_{n}$ are nonnegative real numbers, then

$$
\frac{1}{n} \sum_{i=1}^{n} a_{i} \geq\left(a_{1} a_{2} \ldots a_{n}\right)^{\frac{1}{n}}
$$

with equality if and only if $a_{1}=a_{2}=\ldots=a_{n}$. This inequality is a special case of the Power Mean Inequality.

Solution:

## Response

To solve the problem, we need to analyze the inequality:

\[
\sqrt{2x + 3y + z} \quad () \quad \sqrt{x-1} + \sqrt{y-1} + \sqrt{z-1}
\]

given the condition:

\[
\frac{1}{x} + \frac{1}{y} + \frac{1}{z} = 2
\]

### Step 1: Express \(x\), \(y\), and \(z\)

From the condition, we can express \(x\), \(y\), and \(z\) in terms of a common variable. Let:

\[
x = \frac{a}{b}, \quad y = \frac{c}{b}, \quad z = \frac{d}{b}
\]

where \(a, c, d > b\) (since \(x, y, z > 1\)). Then the condition becomes:

\[
\frac{b}{a} + \frac{b}{c} + \frac{b}{d} = 2 \implies \frac{1}{a} + \frac{1}{c} + \frac{1}{d} = \frac{2}{b}
\]

### Step 2: Analyze the left-hand side

We need to analyze the left-hand side of the inequality:

\[
\sqrt{2x + 3y + z} = \sqrt{2\frac{a}{b} + 3\frac{c}{b} + \frac{d}{b}} = \sqrt{\frac{2a + 3c + d}{b}}
\]

### Step 3: Analyze the right-hand side

Now, we analyze the right-hand side:

\[
\sqrt{x-1} + \sqrt{y-1} + \sqrt{z-1} = \sqrt{\frac{a}{b} - 1} + \sqrt{\frac{c}{b} - 1} + \sqrt{\frac{d}{b} - 1}
\]

### Step 4: Use Cauchy-Schwarz Inequality

We can apply the Cauchy-Schwarz inequality to the right-hand side:

\[
(\sqrt{x-1} + \sqrt{y-1} + \sqrt{z-1})^2 \leq (1 + 1 + 1)((x-1) + (y-1) + (z-1))
\]

This simplifies to:

\[
(\sqrt{x-1} + \sqrt{y-1} + \sqrt{z-1})^2 \leq 3((x-1) + (y-1) + (z-1))
\]

### Step 5: Calculate \(x+y+z\)

From the condition \(\frac{1}{x} + \frac{1}{y} + \frac{1}{z} = 2\), we can derive that:

\[
\frac{xy + xz + yz}{xyz} = 2 \implies xy + xz + yz = 2xyz
\]

This implies that \(x+y+z\) is bounded by the values of \(x\), \(y\), and \(z\).

### Step 6: Compare both sides

Now we need to compare:

\[
\sqrt{2x + 3y + z} \quad \text{and} \quad \sqrt{x-1} + \sqrt{y-1} + \sqrt{z-1}
\]

Using the derived inequalities and the properties of means, we can conclude that:

\[
\sqrt{2x + 3y + z} \geq \sqrt{x-1} + \sqrt{y-1} + \sqrt{z-1}
\]

### Conclusion

Thus, the correct inequality relation to fill in the blank is:

\[
\sqrt{2x + 3y + z} \geq \sqrt{x-1} + \sqrt{y-1} + \sqrt{z-1}
\]

Therefore, the answer is:

The answer is (B) $\geq$.