## Problem

Let $a_1, a_2, \ldots, a_n > 0$ be positive real numbers such that $a_1 + a_2 + \ldots + a_n < 1$. Consider the following inequality:
$$
\frac{a_1 \cdot a_2 \ldots a_n\left(1-a_1-a_2-\ldots-a_n\right)}{\left(a_1+a_2+\ldots+a_n\right)\left(1-a_1\right)\left(1-a_2\right) \ldots\left(1-a_n\right)} \quad () \quad \frac{1}{n^{n-1}}.
$$

Determine the correct inequality relation to fill in the blank.

Options:

(A) $\leq$ 

(B) $\geq$

(C) $=$ 

(D) $<$

(E) $>$

(F) None of the above

## Query

Task description: Please solve the problem with clear, rigorous, and logically sound steps. At the end of your response, state your answer in exactly this format: 'The answer is (Letter) Symbol', where Letter is one of the given options. Example: 'The answer is (A) $\leq$'.

Problem: Let $a_1, a_2, \ldots, a_n > 0$ be positive real numbers such that $a_1 + a_2 + \ldots + a_n < 1$. Consider the following inequality:
$$
\frac{a_1 \cdot a_2 \ldots a_n\left(1-a_1-a_2-\ldots-a_n\right)}{\left(a_1+a_2+\ldots+a_n\right)\left(1-a_1\right)\left(1-a_2\right) \ldots\left(1-a_n\right)} \quad () \quad \frac{1}{n^{n-1}}.
$$

Determine the correct inequality relation to fill in the blank.

Options:

(A) $\leq$ 

(B) $\geq$

(C) $=$ 

(D) $<$

(E) $>$

(F) None of the above

Please use some of the following theorems to solve the problem:
Theorem 1 (Category: Inequality Between Means, Nicknames: mean inequalities): Let $a_{1}, a_{2}, \ldots, a_{n}$ be positive real numbers. The numbers
$$
\begin{aligned}
& Q M=\sqrt{\frac{a_{1}^{2}+a_{2}^{2}+\cdots+a_{n}^{2}}{n}}, \quad A M=\frac{a_{1}+a_{2}+\cdots+a_{n}}{n} \\
& G M=\sqrt[n]{a_{1} a_{2} \cdots a_{n}} \quad \text { and } \quad H M=\frac{n}{\frac{1}{a_{1}}+\frac{1}{a_{2}}+\cdots+\frac{1}{a_{n}}}
\end{aligned}
$$
are called the quadratic, arithmetic, geometric and harmonic mean for the numbers $a_{1}, a_{2}, \ldots, a_{n}$, respectively, and we have
$$
Q M \geq A M \geq G M \geq H M
$$

Equalities occur if and only if $a_{1}=a_{2}=\cdots=a_{n}$.

Theorem 2 (Category: Cauchy-Schwarz Inequality, Nicknames: cauchy-schwarz inequality): Let $a_{1}, a_{2}, \ldots, a_{n}$ and $b_{1}, b_{2}$, $\ldots, b_{n}$ be real numbers. Then we have
$$
\left(\sum_{i=1}^{n} a_{i}^{2}\right)\left(\sum_{i=1}^{n} b_{i}^{2}\right) \geq\left(\sum_{i=1}^{n} a_{i} b_{i}\right)^{2}
$$
i.e.
$$
\left(a_{1}^{2}+a_{2}^{2}+\cdots+a_{n}^{2}\right)\left(b_{1}^{2}+b_{2}^{2}+\cdots+b_{n}^{2}\right) \geq\left(a_{1} b_{1}+a_{2} b_{2}+\cdots+a_{n} b_{n}\right)^{2}
$$

Equality occurs if and only if the sequences $\left(a_{1}, a_{2}, \ldots, a_{n}\right)$ and $\left(b_{1}, b_{2}\right.$, $\ldots, b_{n}$ ) are proportional, i.e. $\frac{a_{1}}{b_{1}}=\frac{a_{2}}{b_{2}}=\cdots=\frac{a_{n}}{b_{n}}$.

Theorem 3 (Category: Inequality Between Means, Nicknames: am-gm (arithmetic mean-geometric mean) inequality, am-gm): If $a_{1}, a_{2}, \ldots, a_{n}$ are nonnegative real numbers, then

$$
\frac{1}{n} \sum_{i=1}^{n} a_{i} \geq\left(a_{1} a_{2} \ldots a_{n}\right)^{\frac{1}{n}}
$$

with equality if and only if $a_{1}=a_{2}=\ldots=a_{n}$. This inequality is a special case of the Power Mean Inequality.

Solution:

## Response

To solve the problem, we need to analyze the given inequality:

$$
\frac{a_1 \cdot a_2 \ldots a_n\left(1-a_1-a_2-\ldots-a_n\right)}{\left(a_1+a_2+\ldots+a_n\right)\left(1-a_1\right)\left(1-a_2\right) \ldots\left(1-a_n\right)} \quad () \quad \frac{1}{n^{n-1}}.
$$

Let \( S = a_1 + a_2 + \ldots + a_n \). Given that \( S < 1 \), we can denote \( T = 1 - S \), which is positive since \( S < 1 \).

We can rewrite the left-hand side of the inequality as:

$$
\frac{a_1 a_2 \ldots a_n T}{S (1 - a_1)(1 - a_2) \ldots (1 - a_n)}.
$$

### Step 1: Apply the AM-GM Inequality

Using the AM-GM inequality on the terms \( a_1, a_2, \ldots, a_n \):

$$
\frac{a_1 + a_2 + \ldots + a_n}{n} \geq (a_1 a_2 \ldots a_n)^{\frac{1}{n}}.
$$

This implies:

$$
S \geq n (a_1 a_2 \ldots a_n)^{\frac{1}{n}}.
$$

### Step 2: Analyze the Denominator

Next, we analyze the terms \( 1 - a_i \):

Using the fact that \( 1 - a_i = T + S - a_i \), we can apply the AM-GM inequality again:

$$
1 - a_i \geq \frac{T + S - a_i}{n-1} \text{ for each } i.
$$

However, a more straightforward approach is to note that since \( S < 1 \), we have \( 1 - a_i > 0 \) for all \( i \).

### Step 3: Combine Results

Now, we can combine our results. We know:

1. \( S \geq n (a_1 a_2 \ldots a_n)^{\frac{1}{n}} \)
2. Each \( 1 - a_i \) is positive.

Thus, we can express the left-hand side in terms of \( S \) and \( T \):

$$
\frac{a_1 a_2 \ldots a_n T}{S (1 - a_1)(1 - a_2) \ldots (1 - a_n)}.
$$

### Step 4: Compare with \( \frac{1}{n^{n-1}} \)

To compare this with \( \frac{1}{n^{n-1}} \), we can use the fact that the product \( a_1 a_2 \ldots a_n \) is maximized when all \( a_i \) are equal (by AM-GM). 

Let \( a_i = x \) for all \( i \), then \( S = nx < 1 \) implies \( x < \frac{1}{n} \). Thus, we can express:

$$
a_1 a_2 \ldots a_n = x^n,
$$

and \( T = 1 - nx \).

### Step 5: Final Comparison

The left-hand side becomes:

$$
\frac{x^n (1 - nx)}{nx (1 - x)^{n}}.
$$

As \( n \) increases, the left-hand side tends to decrease due to the \( n \) in the denominator and the nature of the product terms. 

### Conclusion

After analyzing the behavior of the left-hand side and comparing it with \( \frac{1}{n^{n-1}} \), we conclude that:

$$
\frac{a_1 a_2 \ldots a_n (1 - S)}{S (1 - a_1)(1 - a_2) \ldots (1 - a_n)} < \frac{1}{n^{n-1}}.
$$

Thus, the correct inequality to fill in the blank is:

The answer is (D) $<$.