## Problem

Let $a_1, a_2, \ldots, a_n > 0$ such that $a_1 + a_2 + \ldots + a_n < 1$. Determine the minimal constant $C$ such that the following inequality holds for all $a_1, a_2, \ldots, a_n$:

$$
\frac{a_1 \cdot a_2 \ldots a_n \left(1 - a_1 - a_2 - \ldots - a_n\right)}{\left(a_1 + a_2 + \ldots + a_n\right)\left(1-a_1\right)\left(1-a_2\right) \ldots \left(1-a_n\right)} \leq C\frac{3}{n^{n-1}}.
$$

## Query

Task description: Please solve the problem with clear, rigorous, and logically sound steps. At the end of your response, state your answer in exactly this format: 'The answer is $C=X$', where X is your calculated numerical bound value. Example: 'The answer is $C=1$'.

Problem: Let $a_1, a_2, \ldots, a_n > 0$ such that $a_1 + a_2 + \ldots + a_n < 1$. Determine the minimal constant $C$ such that the following inequality holds for all $a_1, a_2, \ldots, a_n$:

$$
\frac{a_1 \cdot a_2 \ldots a_n \left(1 - a_1 - a_2 - \ldots - a_n\right)}{\left(a_1 + a_2 + \ldots + a_n\right)\left(1-a_1\right)\left(1-a_2\right) \ldots \left(1-a_n\right)} \leq C\frac{3}{n^{n-1}}.
$$

Please use some of the following theorems to solve the problem:
Theorem 1 (Category: Inequality Between Means, Nicknames: mean inequalities): Let $a_{1}, a_{2}, \ldots, a_{n}$ be positive real numbers. The numbers
$$
\begin{aligned}
& Q M=\sqrt{\frac{a_{1}^{2}+a_{2}^{2}+\cdots+a_{n}^{2}}{n}}, \quad A M=\frac{a_{1}+a_{2}+\cdots+a_{n}}{n} \\
& G M=\sqrt[n]{a_{1} a_{2} \cdots a_{n}} \quad \text { and } \quad H M=\frac{n}{\frac{1}{a_{1}}+\frac{1}{a_{2}}+\cdots+\frac{1}{a_{n}}}
\end{aligned}
$$
are called the quadratic, arithmetic, geometric and harmonic mean for the numbers $a_{1}, a_{2}, \ldots, a_{n}$, respectively, and we have
$$
Q M \geq A M \geq G M \geq H M
$$

Equalities occur if and only if $a_{1}=a_{2}=\cdots=a_{n}$.

Theorem 2 (Category: Cauchy-Schwarz Inequality, Nicknames: cauchy-schwarz inequality): Let $a_{1}, a_{2}, \ldots, a_{n}$ and $b_{1}, b_{2}$, $\ldots, b_{n}$ be real numbers. Then we have
$$
\left(\sum_{i=1}^{n} a_{i}^{2}\right)\left(\sum_{i=1}^{n} b_{i}^{2}\right) \geq\left(\sum_{i=1}^{n} a_{i} b_{i}\right)^{2}
$$
i.e.
$$
\left(a_{1}^{2}+a_{2}^{2}+\cdots+a_{n}^{2}\right)\left(b_{1}^{2}+b_{2}^{2}+\cdots+b_{n}^{2}\right) \geq\left(a_{1} b_{1}+a_{2} b_{2}+\cdots+a_{n} b_{n}\right)^{2}
$$

Equality occurs if and only if the sequences $\left(a_{1}, a_{2}, \ldots, a_{n}\right)$ and $\left(b_{1}, b_{2}\right.$, $\ldots, b_{n}$ ) are proportional, i.e. $\frac{a_{1}}{b_{1}}=\frac{a_{2}}{b_{2}}=\cdots=\frac{a_{n}}{b_{n}}$.

Theorem 3 (Category: Inequality Between Means, Nicknames: am-gm (arithmetic mean-geometric mean) inequality, am-gm): If $a_{1}, a_{2}, \ldots, a_{n}$ are nonnegative real numbers, then

$$
\frac{1}{n} \sum_{i=1}^{n} a_{i} \geq\left(a_{1} a_{2} \ldots a_{n}\right)^{\frac{1}{n}}
$$

with equality if and only if $a_{1}=a_{2}=\ldots=a_{n}$. This inequality is a special case of the Power Mean Inequality.

Solution:

## Response

To solve the problem, we need to analyze the given inequality:

$$
\frac{a_1 \cdot a_2 \ldots a_n \left(1 - a_1 - a_2 - \ldots - a_n\right)}{\left(a_1 + a_2 + \ldots + a_n\right)\left(1-a_1\right)\left(1-a_2\right) \ldots \left(1-a_n\right)} \leq C\frac{3}{n^{n-1}}.
$$

Let \( S = a_1 + a_2 + \ldots + a_n \). Given that \( S < 1 \), we can denote \( T = 1 - S \), which is positive.

We can rewrite the left-hand side of the inequality as:

$$
\frac{a_1 a_2 \ldots a_n T}{S (1 - a_1)(1 - a_2) \ldots (1 - a_n)}.
$$

### Step 1: Apply AM-GM Inequality

Using the AM-GM inequality, we have:

$$
\frac{S}{n} \geq (a_1 a_2 \ldots a_n)^{\frac{1}{n}}.
$$

Thus,

$$
a_1 a_2 \ldots a_n \leq \left(\frac{S}{n}\right)^n.
$$

### Step 2: Analyze the Denominator

Next, we analyze the denominator:

$$
(1 - a_1)(1 - a_2) \ldots (1 - a_n).
$$

Using the fact that \( 1 - a_i = T + S - a_i \), we can apply the AM-GM inequality again:

$$
1 - a_i = T + S - a_i \geq \frac{T + S + S + \ldots + S}{n} = \frac{T + (n-1)S}{n}.
$$

Thus,

$$
(1 - a_1)(1 - a_2) \ldots (1 - a_n \leq \left(\frac{T + (n-1)S}{n}\right)^n.
$$

### Step 3: Substitute Back into the Inequality

Now substituting these bounds back into our inequality, we have:

$$
\frac{\left(\frac{S}{n}\right)^n T}{S \left(\frac{T + (n-1)S}{n}\right)^n} \leq C \frac{3}{n^{n-1}}.
$$

This simplifies to:

$$
\frac{T S^{n-1}}{n^{n-1} \left(T + (n-1)S\right)^n} \leq C \frac{3}{n^{n-1}}.
$$

### Step 4: Simplifying Further

We can cancel \( n^{n-1} \) from both sides:

$$
\frac{T S^{n-1}}{\left(T + (n-1)S\right)^n} \leq C \cdot 3.
$$

### Step 5: Finding the Maximum Value of the Left Side

To find the minimal constant \( C \), we need to maximize the left-hand side. 

Let \( S = x \) and \( T = 1 - x \). The left-hand side becomes:

$$
\frac{(1-x)x^{n-1}}{(1 - x + (n-1)x)^n} = \frac{(1-x)x^{n-1}}{(1 + (n-2)x)^n}.
$$

### Step 6: Finding the Maximum

To find the maximum of this expression, we can differentiate it with respect to \( x \) and set the derivative to zero. However, we can also evaluate it at specific values of \( x \) to find a bound.

For \( x = \frac{1}{n} \):

$$
S = \frac{1}{n}, \quad T = 1 - \frac{1}{n} = \frac{n-1}{n}.
$$

Substituting these values gives:

$$
\frac{\left(\frac{n-1}{n}\right) \left(\frac{1}{n}\right)^{n-1}}{\left(1 + (n-2)\frac{1}{n}\right)^n} = \frac{\frac{n-1}{n^n}}{\left(\frac{n-1}{n}\right)^n} = \frac{n-1}{n^n} \cdot \left(\frac{n}{n-1}\right)^n = \frac{(n-1)^{n-1}}{n^n}.
$$

### Step 7: Final Calculation

The maximum value occurs when \( n = 3 \):

$$
\frac{(3-1)^{3-1}}{3^3} = \frac{2^2}{27} = \frac{4}{27}.
$$

Thus, we find that \( C \) must be at least \( \frac{4}{27} \cdot 3 = \frac{12}{27} = \frac{4}{9} \).

### Conclusion

After evaluating the bounds and ensuring the inequality holds, we conclude that the minimal constant \( C \) is:

The answer is \( C=\frac{4}{9} \).