## Problem

Let $a, b, c, x, y, z \in \mathbb{R}$ be real numbers such that $a + b + c = 1$ and $x^2 + y^2 + z^2 = 1$. Consider the following expression:
$$
a(x+b) + b(y+c) + c(z+a)  \quad () \quad 1.
$$

Determine the correct inequality relation to fill in the blank.

Options:

(A) $\leq$ 

(B) $\geq$

(C) $=$ 

(D) $<$

(E) $>$

(F) None of the above

## Query

Task description: Please solve the problem with clear, rigorous, and logically sound steps. At the end of your response, state your answer in exactly this format: 'The answer is (Letter) Symbol', where Letter is one of the given options. Example: 'The answer is (A) $\leq$'.

Problem: Let $a, b, c, x, y, z \in \mathbb{R}$ be real numbers such that $a + b + c = 1$ and $x^2 + y^2 + z^2 = 1$. Consider the following expression:
$$
a(x+b) + b(y+c) + c(z+a)  \quad () \quad 1.
$$

Determine the correct inequality relation to fill in the blank.

Options:

(A) $\leq$ 

(B) $\geq$

(C) $=$ 

(D) $<$

(E) $>$

(F) None of the above

Please use some of the following theorems to solve the problem:
Theorem 1 (Category: Inequality Between Means, Nicknames: mean inequalities): Let $a_{1}, a_{2}, \ldots, a_{n}$ be positive real numbers. The numbers
$$
\begin{aligned}
& Q M=\sqrt{\frac{a_{1}^{2}+a_{2}^{2}+\cdots+a_{n}^{2}}{n}}, \quad A M=\frac{a_{1}+a_{2}+\cdots+a_{n}}{n} \\
& G M=\sqrt[n]{a_{1} a_{2} \cdots a_{n}} \quad \text { and } \quad H M=\frac{n}{\frac{1}{a_{1}}+\frac{1}{a_{2}}+\cdots+\frac{1}{a_{n}}}
\end{aligned}
$$
are called the quadratic, arithmetic, geometric and harmonic mean for the numbers $a_{1}, a_{2}, \ldots, a_{n}$, respectively, and we have
$$
Q M \geq A M \geq G M \geq H M
$$

Equalities occur if and only if $a_{1}=a_{2}=\cdots=a_{n}$.

Theorem 2 (Category: Cauchy-Schwarz Inequality, Nicknames: cauchy-schwarz inequality): Let $a_{1}, a_{2}, \ldots, a_{n}$ and $b_{1}, b_{2}$, $\ldots, b_{n}$ be real numbers. Then we have
$$
\left(\sum_{i=1}^{n} a_{i}^{2}\right)\left(\sum_{i=1}^{n} b_{i}^{2}\right) \geq\left(\sum_{i=1}^{n} a_{i} b_{i}\right)^{2}
$$
i.e.
$$
\left(a_{1}^{2}+a_{2}^{2}+\cdots+a_{n}^{2}\right)\left(b_{1}^{2}+b_{2}^{2}+\cdots+b_{n}^{2}\right) \geq\left(a_{1} b_{1}+a_{2} b_{2}+\cdots+a_{n} b_{n}\right)^{2}
$$

Equality occurs if and only if the sequences $\left(a_{1}, a_{2}, \ldots, a_{n}\right)$ and $\left(b_{1}, b_{2}\right.$, $\ldots, b_{n}$ ) are proportional, i.e. $\frac{a_{1}}{b_{1}}=\frac{a_{2}}{b_{2}}=\cdots=\frac{a_{n}}{b_{n}}$.

Theorem 3 (Category: Inequality Between Means, Nicknames: am-gm (arithmetic mean-geometric mean) inequality, am-gm): If $a_{1}, a_{2}, \ldots, a_{n}$ are nonnegative real numbers, then

$$
\frac{1}{n} \sum_{i=1}^{n} a_{i} \geq\left(a_{1} a_{2} \ldots a_{n}\right)^{\frac{1}{n}}
$$

with equality if and only if $a_{1}=a_{2}=\ldots=a_{n}$. This inequality is a special case of the Power Mean Inequality.

Solution:

## Response

To solve the problem, we need to analyze the expression given:

\[
E = a(x+b) + b(y+c) + c(z+a)
\]

We can expand this expression:

\[
E = ax + ab + by + bc + cz + ca
\]

Rearranging the terms, we have:

\[
E = ax + by + cz + ab + bc + ca
\]

Next, we will use the conditions provided in the problem: \( a + b + c = 1 \) and \( x^2 + y^2 + z^2 = 1 \).

### Step 1: Analyze the terms \( ax + by + cz \)

Using the Cauchy-Schwarz inequality, we can relate \( ax + by + cz \) to the sums of squares:

\[
(ax + by + cz)^2 \leq (a^2 + b^2 + c^2)(x^2 + y^2 + z^2)
\]

Since \( x^2 + y^2 + z^2 = 1 \), we have:

\[
(ax + by + cz)^2 \leq (a^2 + b^2 + c^2)
\]

### Step 2: Use the condition \( a + b + c = 1 \)

By the Cauchy-Schwarz inequality, we also know that:

\[
a^2 + b^2 + c^2 \geq \frac{(a + b + c)^2}{3} = \frac{1^2}{3} = \frac{1}{3}
\]

Thus, we can conclude:

\[
(ax + by + cz)^2 \leq a^2 + b^2 + c^2 \leq \frac{1}{3}
\]

Taking the square root gives:

\[
|ax + by + cz| \leq \sqrt{\frac{1}{3}} \implies ax + by + cz \leq \sqrt{\frac{1}{3}}
\]

### Step 3: Analyze the constant terms \( ab + bc + ca \)

The terms \( ab + bc + ca \) can be expressed in terms of \( a, b, c \):

Using the identity:

\[
ab + bc + ca = \frac{(a+b+c)^2 - (a^2 + b^2 + c^2)}{2} = \frac{1 - (a^2 + b^2 + c^2)}{2}
\]

Since \( a^2 + b^2 + c^2 \geq \frac{1}{3} \), we have:

\[
ab + bc + ca \leq \frac{1 - \frac{1}{3}}{2} = \frac{1}{3}
\]

### Step 4: Combine the results

Now we can combine our results:

\[
E = ax + by + cz + ab + bc + ca
\]

From our previous steps, we know:

1. \( ax + by + cz \leq \sqrt{\frac{1}{3}} \)
2. \( ab + bc + ca \leq \frac{1}{3} \)

Thus, we can conclude:

\[
E \leq \sqrt{\frac{1}{3}} + \frac{1}{3}
\]

### Step 5: Compare with 1

Now we need to check if \( E < 1 \):

Since \( \sqrt{\frac{1}{3}} \approx 0.577 \) and \( \frac{1}{3} \approx 0.333 \), we have:

\[
E \leq 0.577 + 0.333 = 0.91 < 1
\]

### Conclusion

Thus, we conclude that:

\[
E < 1
\]

Therefore, the correct inequality relation to fill in the blank is:

The answer is (D) $<$.