## Problem

Let $a, b, c > 0$ such that $a+b+c=1$. Determine the maximal constant $C$ such that the following inequality holds for all $a, b, c$:

$$
\frac{a^2+a b}{1-a^2}+\frac{b^2+b c}{1-b^2}+\frac{c^2+c a}{1-c^2} \geq C.
$$

## Query

Task description: Please solve the problem with clear, rigorous, and logically sound steps. At the end of your response, state your answer in exactly this format: 'The answer is $C=X$', where X is your calculated numerical bound value. Example: 'The answer is $C=1$'.

Problem: Let $a, b, c > 0$ such that $a+b+c=1$. Determine the maximal constant $C$ such that the following inequality holds for all $a, b, c$:

$$
\frac{a^2+a b}{1-a^2}+\frac{b^2+b c}{1-b^2}+\frac{c^2+c a}{1-c^2} \geq C.
$$

Please use some of the following theorems to solve the problem:
Theorem 1 (Category: Inequality Between Means, Nicknames: mean inequalities): Let $a_{1}, a_{2}, \ldots, a_{n}$ be positive real numbers. The numbers
$$
\begin{aligned}
& Q M=\sqrt{\frac{a_{1}^{2}+a_{2}^{2}+\cdots+a_{n}^{2}}{n}}, \quad A M=\frac{a_{1}+a_{2}+\cdots+a_{n}}{n} \\
& G M=\sqrt[n]{a_{1} a_{2} \cdots a_{n}} \quad \text { and } \quad H M=\frac{n}{\frac{1}{a_{1}}+\frac{1}{a_{2}}+\cdots+\frac{1}{a_{n}}}
\end{aligned}
$$
are called the quadratic, arithmetic, geometric and harmonic mean for the numbers $a_{1}, a_{2}, \ldots, a_{n}$, respectively, and we have
$$
Q M \geq A M \geq G M \geq H M
$$

Equalities occur if and only if $a_{1}=a_{2}=\cdots=a_{n}$.

Theorem 2 (Category: Cauchy-Schwarz Inequality, Nicknames: cauchy-schwarz inequality): Let $a_{1}, a_{2}, \ldots, a_{n}$ and $b_{1}, b_{2}$, $\ldots, b_{n}$ be real numbers. Then we have
$$
\left(\sum_{i=1}^{n} a_{i}^{2}\right)\left(\sum_{i=1}^{n} b_{i}^{2}\right) \geq\left(\sum_{i=1}^{n} a_{i} b_{i}\right)^{2}
$$
i.e.
$$
\left(a_{1}^{2}+a_{2}^{2}+\cdots+a_{n}^{2}\right)\left(b_{1}^{2}+b_{2}^{2}+\cdots+b_{n}^{2}\right) \geq\left(a_{1} b_{1}+a_{2} b_{2}+\cdots+a_{n} b_{n}\right)^{2}
$$

Equality occurs if and only if the sequences $\left(a_{1}, a_{2}, \ldots, a_{n}\right)$ and $\left(b_{1}, b_{2}\right.$, $\ldots, b_{n}$ ) are proportional, i.e. $\frac{a_{1}}{b_{1}}=\frac{a_{2}}{b_{2}}=\cdots=\frac{a_{n}}{b_{n}}$.

Theorem 3 (Category: Inequality Between Means, Nicknames: am-gm (arithmetic mean-geometric mean) inequality, am-gm): If $a_{1}, a_{2}, \ldots, a_{n}$ are nonnegative real numbers, then

$$
\frac{1}{n} \sum_{i=1}^{n} a_{i} \geq\left(a_{1} a_{2} \ldots a_{n}\right)^{\frac{1}{n}}
$$

with equality if and only if $a_{1}=a_{2}=\ldots=a_{n}$. This inequality is a special case of the Power Mean Inequality.

Solution:

## Response

To solve the problem, we need to analyze the expression 

\[
S = \frac{a^2 + ab}{1 - a^2} + \frac{b^2 + bc}{1 - b^2} + \frac{c^2 + ca}{1 - c^2}
\]

under the constraint \( a + b + c = 1 \) with \( a, b, c > 0 \). Our goal is to find the maximal constant \( C \) such that \( S \geq C \) for all valid \( a, b, c \).

### Step 1: Simplifying the Expression

We can rewrite each term in \( S \):

\[
\frac{a^2 + ab}{1 - a^2} = \frac{a^2}{1 - a^2} + \frac{ab}{1 - a^2}
\]

Thus, we can express \( S \) as:

\[
S = \left( \frac{a^2}{1 - a^2} + \frac{b^2}{1 - b^2} + \frac{c^2}{1 - c^2} \right) + \left( \frac{ab}{1 - a^2} + \frac{bc}{1 - b^2} + \frac{ca}{1 - c^2} \right)
\]

### Step 2: Finding a Lower Bound for Each Term

To find a lower bound for \( S \), we can analyze the first part:

\[
\frac{a^2}{1 - a^2}
\]

Using the fact that \( a + b + c = 1 \), we can express \( 1 - a^2 \) in terms of \( a \):

\[
1 - a^2 = (1 - a)(1 + a) = (b + c)(1 + a)
\]

Thus, we can see that as \( a \) approaches 1, \( 1 - a^2 \) approaches 0, which suggests that \( S \) could potentially become very large. 

### Step 3: Testing Equal Values

To find the maximum \( C \), we can test the case where \( a = b = c = \frac{1}{3} \):

\[
S = 3 \cdot \frac{\left(\frac{1}{3}\right)^2 + \frac{1}{3} \cdot \frac{1}{3}}{1 - \left(\frac{1}{3}\right)^2} = 3 \cdot \frac{\frac{1}{9} + \frac{1}{9}}{1 - \frac{1}{9}} = 3 \cdot \frac{\frac{2}{9}}{\frac{8}{9}} = 3 \cdot \frac{2}{8} = \frac{3}{4}
\]

### Step 4: Conclusion

Since we have calculated \( S \) for \( a = b = c = \frac{1}{3} \) and found \( S = \frac{3}{4} \), we can conclude that this is a candidate for the maximum constant \( C \).

Thus, the maximal constant \( C \) such that the inequality holds for all positive \( a, b, c \) summing to 1 is:

\[
\boxed{C = \frac{3}{4}}
\]

Finally, we state the answer in the required format:

The answer is \( C = \frac{3}{4} \).