## Problem

Let $x, y, z > 0$ be positive real numbers such that $x + y + z = xyz$. Consider the following inequality:
$$
(x-1)(y-1)(z-1) \quad () \quad 6\sqrt{3} - 8.
$$

Determine the correct inequality relation to fill in the blank.

Options:

(A) $\leq$ 

(B) $\geq$

(C) $=$ 

(D) $<$

(E) $>$

(F) None of the above

## Query

Task description: Please solve the problem with clear, rigorous, and logically sound steps. At the end of your response, state your answer in exactly this format: 'The answer is (Letter) Symbol', where Letter is one of the given options. Example: 'The answer is (A) $\leq$'.

Problem: Let $x, y, z > 0$ be positive real numbers such that $x + y + z = xyz$. Consider the following inequality:
$$
(x-1)(y-1)(z-1) \quad () \quad 6\sqrt{3} - 8.
$$

Determine the correct inequality relation to fill in the blank.

Options:

(A) $\leq$ 

(B) $\geq$

(C) $=$ 

(D) $<$

(E) $>$

(F) None of the above

Please use some of the following theorems to solve the problem:
Theorem 1 (Category: Inequality Between Means, Nicknames: mean inequalities): Let $a_{1}, a_{2}, \ldots, a_{n}$ be positive real numbers. The numbers
$$
\begin{aligned}
& Q M=\sqrt{\frac{a_{1}^{2}+a_{2}^{2}+\cdots+a_{n}^{2}}{n}}, \quad A M=\frac{a_{1}+a_{2}+\cdots+a_{n}}{n} \\
& G M=\sqrt[n]{a_{1} a_{2} \cdots a_{n}} \quad \text { and } \quad H M=\frac{n}{\frac{1}{a_{1}}+\frac{1}{a_{2}}+\cdots+\frac{1}{a_{n}}}
\end{aligned}
$$
are called the quadratic, arithmetic, geometric and harmonic mean for the numbers $a_{1}, a_{2}, \ldots, a_{n}$, respectively, and we have
$$
Q M \geq A M \geq G M \geq H M
$$

Equalities occur if and only if $a_{1}=a_{2}=\cdots=a_{n}$.

Theorem 2 (Category: Cauchy-Schwarz Inequality, Nicknames: cauchy-schwarz inequality): Let $a_{1}, a_{2}, \ldots, a_{n}$ and $b_{1}, b_{2}$, $\ldots, b_{n}$ be real numbers. Then we have
$$
\left(\sum_{i=1}^{n} a_{i}^{2}\right)\left(\sum_{i=1}^{n} b_{i}^{2}\right) \geq\left(\sum_{i=1}^{n} a_{i} b_{i}\right)^{2}
$$
i.e.
$$
\left(a_{1}^{2}+a_{2}^{2}+\cdots+a_{n}^{2}\right)\left(b_{1}^{2}+b_{2}^{2}+\cdots+b_{n}^{2}\right) \geq\left(a_{1} b_{1}+a_{2} b_{2}+\cdots+a_{n} b_{n}\right)^{2}
$$

Equality occurs if and only if the sequences $\left(a_{1}, a_{2}, \ldots, a_{n}\right)$ and $\left(b_{1}, b_{2}\right.$, $\ldots, b_{n}$ ) are proportional, i.e. $\frac{a_{1}}{b_{1}}=\frac{a_{2}}{b_{2}}=\cdots=\frac{a_{n}}{b_{n}}$.

Theorem 3 (Category: Inequality Between Means, Nicknames: am-gm (arithmetic mean-geometric mean) inequality, am-gm): If $a_{1}, a_{2}, \ldots, a_{n}$ are nonnegative real numbers, then

$$
\frac{1}{n} \sum_{i=1}^{n} a_{i} \geq\left(a_{1} a_{2} \ldots a_{n}\right)^{\frac{1}{n}}
$$

with equality if and only if $a_{1}=a_{2}=\ldots=a_{n}$. This inequality is a special case of the Power Mean Inequality.

Solution:

## Response

To solve the problem, we start with the condition given: \( x + y + z = xyz \). We can manipulate this condition to express \( (x-1)(y-1)(z-1) \).

First, we expand \( (x-1)(y-1)(z-1) \):

\[
(x-1)(y-1)(z-1) = xyz - (xy + xz + yz) + (x + y + z) - 1
\]

Substituting \( x + y + z = xyz \) into the equation gives:

\[
(x-1)(y-1)(z-1) = xyz - (xy + xz + yz) + xyz - 1
\]
\[
= 2xyz - (xy + xz + yz) - 1
\]

Next, we need to analyze the expression \( 2xyz - (xy + xz + yz) - 1 \) in relation to \( 6\sqrt{3} - 8 \).

To proceed, we can use the substitution \( x = \frac{a}{b}, y = \frac{b}{c}, z = \frac{c}{a} \) where \( a, b, c > 0 \). This substitution is useful because it maintains the symmetry of the problem and allows us to express \( xyz \) and \( xy + xz + yz \) in terms of \( a, b, c \).

Calculating \( xyz \):

\[
xyz = \frac{a}{b} \cdot \frac{b}{c} \cdot \frac{c}{a} = 1
\]

Now, we need to find \( xy + xz + yz \):

\[
xy = \frac{a}{b} \cdot \frac{b}{c} = \frac{a}{c}, \quad xz = \frac{a}{b} \cdot \frac{c}{a} = \frac{c}{b}, \quad yz = \frac{b}{c} \cdot \frac{c}{a} = \frac{b}{a}
\]

Thus,

\[
xy + xz + yz = \frac{a}{c} + \frac{c}{b} + \frac{b}{a}
\]

Now substituting back into our expression for \( (x-1)(y-1)(z-1) \):

\[
(x-1)(y-1)(z-1) = 2 \cdot 1 - \left( \frac{a}{c} + \frac{c}{b} + \frac{b}{a} \right) - 1
\]
\[
= 1 - \left( \frac{a}{c} + \frac{c}{b} + \frac{b}{a} \right)
\]

Next, we apply the AM-GM inequality to \( \frac{a}{c}, \frac{c}{b}, \frac{b}{a} \):

\[
\frac{\frac{a}{c} + \frac{c}{b} + \frac{b}{a}}{3} \geq \sqrt[3]{\frac{a}{c} \cdot \frac{c}{b} \cdot \frac{b}{a}} = 1
\]

This implies:

\[
\frac{a}{c} + \frac{c}{b} + \frac{b}{a} \geq 3
\]

Thus,

\[
1 - \left( \frac{a}{c} + \frac{c}{b} + \frac{b}{a} \right) \leq 1 - 3 = -2
\]

Now we need to compare \( -2 \) with \( 6\sqrt{3} - 8 \). We calculate \( 6\sqrt{3} - 8 \):

\[
6\sqrt{3} \approx 6 \cdot 1.732 = 10.392
\]
\[
6\sqrt{3} - 8 \approx 10.392 - 8 = 2.392
\]

Since \( -2 < 2.392 \), we conclude that:

\[
(x-1)(y-1)(z-1) < 6\sqrt{3} - 8
\]

Thus, the correct inequality relation to fill in the blank is:

The answer is (D) $<$.