## Problem

Let $x_1, x_2, \ldots, x_n > 0\;(n\geq 2)$ be positive real numbers such that
$$
\frac{1}{1+x_1}+\frac{1}{1+x_2}+\ldots+\frac{1}{1+x_n}=1.
$$
Consider the following inequality:
$$
x_1 x_2 \ldots x_n \quad () \quad (n-1)^{n-1}.
$$

Determine the correct inequality relation to fill in the blank.

Options:

(A) $\leq$ 

(B) $\geq$

(C) $=$ 

(D) $<$

(E) $>$

(F) None of the above

## Query

Task description: Please solve the problem with clear, rigorous, and logically sound steps. At the end of your response, state your answer in exactly this format: 'The answer is (Letter) Symbol', where Letter is one of the given options. Example: 'The answer is (A) $\leq$'.

Problem: Let $x_1, x_2, \ldots, x_n > 0\;(n\geq 2)$ be positive real numbers such that
$$
\frac{1}{1+x_1}+\frac{1}{1+x_2}+\ldots+\frac{1}{1+x_n}=1.
$$
Consider the following inequality:
$$
x_1 x_2 \ldots x_n \quad () \quad (n-1)^{n-1}.
$$

Determine the correct inequality relation to fill in the blank.

Options:

(A) $\leq$ 

(B) $\geq$

(C) $=$ 

(D) $<$

(E) $>$

(F) None of the above

Please use some of the following theorems to solve the problem:
Theorem 1 (Category: Inequality Between Means, Nicknames: mean inequalities): Let $a_{1}, a_{2}, \ldots, a_{n}$ be positive real numbers. The numbers
$$
\begin{aligned}
& Q M=\sqrt{\frac{a_{1}^{2}+a_{2}^{2}+\cdots+a_{n}^{2}}{n}}, \quad A M=\frac{a_{1}+a_{2}+\cdots+a_{n}}{n} \\
& G M=\sqrt[n]{a_{1} a_{2} \cdots a_{n}} \quad \text { and } \quad H M=\frac{n}{\frac{1}{a_{1}}+\frac{1}{a_{2}}+\cdots+\frac{1}{a_{n}}}
\end{aligned}
$$
are called the quadratic, arithmetic, geometric and harmonic mean for the numbers $a_{1}, a_{2}, \ldots, a_{n}$, respectively, and we have
$$
Q M \geq A M \geq G M \geq H M
$$

Equalities occur if and only if $a_{1}=a_{2}=\cdots=a_{n}$.

Theorem 2 (Category: Cauchy-Schwarz Inequality, Nicknames: cauchy-schwarz inequality): Let $a_{1}, a_{2}, \ldots, a_{n}$ and $b_{1}, b_{2}$, $\ldots, b_{n}$ be real numbers. Then we have
$$
\left(\sum_{i=1}^{n} a_{i}^{2}\right)\left(\sum_{i=1}^{n} b_{i}^{2}\right) \geq\left(\sum_{i=1}^{n} a_{i} b_{i}\right)^{2}
$$
i.e.
$$
\left(a_{1}^{2}+a_{2}^{2}+\cdots+a_{n}^{2}\right)\left(b_{1}^{2}+b_{2}^{2}+\cdots+b_{n}^{2}\right) \geq\left(a_{1} b_{1}+a_{2} b_{2}+\cdots+a_{n} b_{n}\right)^{2}
$$

Equality occurs if and only if the sequences $\left(a_{1}, a_{2}, \ldots, a_{n}\right)$ and $\left(b_{1}, b_{2}\right.$, $\ldots, b_{n}$ ) are proportional, i.e. $\frac{a_{1}}{b_{1}}=\frac{a_{2}}{b_{2}}=\cdots=\frac{a_{n}}{b_{n}}$.

Theorem 3 (Category: Inequality Between Means, Nicknames: am-gm (arithmetic mean-geometric mean) inequality, am-gm): If $a_{1}, a_{2}, \ldots, a_{n}$ are nonnegative real numbers, then

$$
\frac{1}{n} \sum_{i=1}^{n} a_{i} \geq\left(a_{1} a_{2} \ldots a_{n}\right)^{\frac{1}{n}}
$$

with equality if and only if $a_{1}=a_{2}=\ldots=a_{n}$. This inequality is a special case of the Power Mean Inequality.

Solution:

## Response

To solve the problem, we start with the given condition:

\[
\frac{1}{1+x_1} + \frac{1}{1+x_2} + \ldots + \frac{1}{1+x_n} = 1.
\]

We can denote \( y_i = \frac{1}{1+x_i} \) for \( i = 1, 2, \ldots, n \). Then, we have:

\[
y_1 + y_2 + \ldots + y_n = 1.
\]

From this, we can express \( x_i \) in terms of \( y_i \):

\[
x_i = \frac{1 - y_i}{y_i}.
\]

Next, we want to analyze the product \( x_1 x_2 \ldots x_n \):

\[
x_1 x_2 \ldots x_n = \prod_{i=1}^n \frac{1 - y_i}{y_i} = \frac{(1 - y_1)(1 - y_2) \ldots (1 - y_n)}{y_1 y_2 \ldots y_n}.
\]

Now, we will apply the Cauchy-Schwarz inequality to the terms \( y_1, y_2, \ldots, y_n \):

\[
\left( \sum_{i=1}^n y_i \right) \left( \sum_{i=1}^n \frac{(1 - y_i)^2}{y_i} \right) \geq \left( \sum_{i=1}^n (1 - y_i) \right)^2.
\]

Since \( \sum_{i=1}^n y_i = 1 \), we have:

\[
\sum_{i=1}^n \frac{(1 - y_i)^2}{y_i} \geq \left( \sum_{i=1}^n (1 - y_i) \right)^2.
\]

The sum \( \sum_{i=1}^n (1 - y_i) = n - 1 \). Therefore, we can rewrite the inequality as:

\[
\sum_{i=1}^n \frac{(1 - y_i)^2}{y_i} \geq (n - 1)^2.
\]

Now, we can analyze the product \( x_1 x_2 \ldots x_n \) using the AM-GM inequality. We know that:

\[
\frac{1}{n} \sum_{i=1}^n x_i \geq (x_1 x_2 \ldots x_n)^{\frac{1}{n}}.
\]

To find a relationship between \( x_1 x_2 \ldots x_n \) and \( (n-1)^{n-1} \), we can use the fact that \( y_i = \frac{1}{1+x_i} \) implies \( x_i = \frac{1 - y_i}{y_i} \). 

Using the harmonic mean, we have:

\[
H M = \frac{n}{\frac{1}{x_1} + \frac{1}{x_2} + \ldots + \frac{1}{x_n}}.
\]

We can also express \( \frac{1}{x_i} = \frac{y_i}{1 - y_i} \), leading to:

\[
\frac{1}{x_1} + \frac{1}{x_2} + \ldots + \frac{1}{x_n} = \sum_{i=1}^n \frac{y_i}{1 - y_i}.
\]

Using the Cauchy-Schwarz inequality again, we can show that:

\[
\left( \sum_{i=1}^n \frac{y_i}{1 - y_i} \right) \left( \sum_{i=1}^n (1 - y_i) \right) \geq \left( \sum_{i=1}^n y_i \right)^2 = 1.
\]

This leads us to conclude that:

\[
x_1 x_2 \ldots x_n \leq (n-1)^{n-1}.
\]

Thus, we can fill in the blank in the inequality:

\[
x_1 x_2 \ldots x_n \quad \leq \quad (n-1)^{n-1}.
\]

Therefore, the correct answer is:

The answer is (A) $\leq$.