## Problem

Let $x, y, z \geq -\frac{3}{4}$ be real numbers such that $x + y + z = 1$. Consider the following inequality:
$$
\frac{x}{2x^2+1} + \frac{y}{y^2+3} + \frac{z}{z^2+1} \quad () \quad 1.
$$

Determine the correct inequality relation to fill in the blank.

Options:

(A) $\leq$ 

(B) $\geq$

(C) $=$ 

(D) $<$

(E) $>$

(F) None of the above

## Query

Task description: Please solve the problem with clear, rigorous, and logically sound steps. At the end of your response, state your answer in exactly this format: 'The answer is (Letter) Symbol', where Letter is one of the given options. Example: 'The answer is (A) $\leq$'.

Problem: Let $x, y, z \geq -\frac{3}{4}$ be real numbers such that $x + y + z = 1$. Consider the following inequality:
$$
\frac{x}{2x^2+1} + \frac{y}{y^2+3} + \frac{z}{z^2+1} \quad () \quad 1.
$$

Determine the correct inequality relation to fill in the blank.

Options:

(A) $\leq$ 

(B) $\geq$

(C) $=$ 

(D) $<$

(E) $>$

(F) None of the above

Please use some of the following theorems to solve the problem:
Theorem 1 (Category: Inequality Between Means, Nicknames: mean inequalities): Let $a_{1}, a_{2}, \ldots, a_{n}$ be positive real numbers. The numbers
$$
\begin{aligned}
& Q M=\sqrt{\frac{a_{1}^{2}+a_{2}^{2}+\cdots+a_{n}^{2}}{n}}, \quad A M=\frac{a_{1}+a_{2}+\cdots+a_{n}}{n} \\
& G M=\sqrt[n]{a_{1} a_{2} \cdots a_{n}} \quad \text { and } \quad H M=\frac{n}{\frac{1}{a_{1}}+\frac{1}{a_{2}}+\cdots+\frac{1}{a_{n}}}
\end{aligned}
$$
are called the quadratic, arithmetic, geometric and harmonic mean for the numbers $a_{1}, a_{2}, \ldots, a_{n}$, respectively, and we have
$$
Q M \geq A M \geq G M \geq H M
$$

Equalities occur if and only if $a_{1}=a_{2}=\cdots=a_{n}$.

Theorem 2 (Category: Cauchy-Schwarz Inequality, Nicknames: cauchy-schwarz inequality): Let $a_{1}, a_{2}, \ldots, a_{n}$ and $b_{1}, b_{2}$, $\ldots, b_{n}$ be real numbers. Then we have
$$
\left(\sum_{i=1}^{n} a_{i}^{2}\right)\left(\sum_{i=1}^{n} b_{i}^{2}\right) \geq\left(\sum_{i=1}^{n} a_{i} b_{i}\right)^{2}
$$
i.e.
$$
\left(a_{1}^{2}+a_{2}^{2}+\cdots+a_{n}^{2}\right)\left(b_{1}^{2}+b_{2}^{2}+\cdots+b_{n}^{2}\right) \geq\left(a_{1} b_{1}+a_{2} b_{2}+\cdots+a_{n} b_{n}\right)^{2}
$$

Equality occurs if and only if the sequences $\left(a_{1}, a_{2}, \ldots, a_{n}\right)$ and $\left(b_{1}, b_{2}\right.$, $\ldots, b_{n}$ ) are proportional, i.e. $\frac{a_{1}}{b_{1}}=\frac{a_{2}}{b_{2}}=\cdots=\frac{a_{n}}{b_{n}}$.

Theorem 3 (Category: Inequality Between Means, Nicknames: am-gm (arithmetic mean-geometric mean) inequality, am-gm): If $a_{1}, a_{2}, \ldots, a_{n}$ are nonnegative real numbers, then

$$
\frac{1}{n} \sum_{i=1}^{n} a_{i} \geq\left(a_{1} a_{2} \ldots a_{n}\right)^{\frac{1}{n}}
$$

with equality if and only if $a_{1}=a_{2}=\ldots=a_{n}$. This inequality is a special case of the Power Mean Inequality.

Solution:

## Response

To solve the inequality 

\[
\frac{x}{2x^2+1} + \frac{y}{y^2+3} + \frac{z}{z^2+1} \quad () \quad 1
\]

given the constraints \(x, y, z \geq -\frac{3}{4}\) and \(x + y + z = 1\), we will analyze each term in the sum separately and then combine the results.

### Step 1: Analyze Each Term

1. **For the term \(\frac{x}{2x^2 + 1}\)**:
   - The denominator \(2x^2 + 1\) is always positive for \(x \geq -\frac{3}{4}\).
   - We can find the maximum of \(\frac{x}{2x^2 + 1}\) by differentiating:
     \[
     f(x) = \frac{x}{2x^2 + 1}
     \]
     Using the quotient rule:
     \[
     f'(x) = \frac{(2x^2 + 1)(1) - x(4x)}{(2x^2 + 1)^2} = \frac{2x^2 + 1 - 4x^2}{(2x^2 + 1)^2} = \frac{1 - 2x^2}{(2x^2 + 1)^2}
     \]
     Setting \(f'(x) = 0\) gives \(1 - 2x^2 = 0\) or \(x^2 = \frac{1}{2}\), thus \(x = \frac{1}{\sqrt{2}}\) or \(x = -\frac{1}{\sqrt{2}}\). Since \(x \geq -\frac{3}{4}\), we only consider \(x = \frac{1}{\sqrt{2}}\).
   - Evaluating \(f\) at \(x = \frac{1}{\sqrt{2}}\):
     \[
     f\left(\frac{1}{\sqrt{2}}\right) = \frac{\frac{1}{\sqrt{2}}}{2\left(\frac{1}{2}\right) + 1} = \frac{\frac{1}{\sqrt{2}}}{2} = \frac{1}{2\sqrt{2}} \approx 0.3535
     \]

2. **For the term \(\frac{y}{y^2 + 3}\)**:
   - The denominator \(y^2 + 3\) is always positive.
   - The maximum occurs at \(y = 1\) (since \(y\) can be at most 1 when \(x + y + z = 1\)):
     \[
     f(1) = \frac{1}{1 + 3} = \frac{1}{4} = 0.25
     \]

3. **For the term \(\frac{z}{z^2 + 1}\)**:
   - The maximum occurs at \(z = 1\) (similar reasoning as above):
     \[
     f(1) = \frac{1}{1 + 1} = \frac{1}{2} = 0.5
     \]

### Step 2: Combine the Results

Now we can combine the maximum values of each term:
- The maximum of \(\frac{x}{2x^2 + 1}\) is approximately \(0.3535\).
- The maximum of \(\frac{y}{y^2 + 3}\) is \(0.25\).
- The maximum of \(\frac{z}{z^2 + 1}\) is \(0.5\).

Adding these maximum values together:
\[
0.3535 + 0.25 + 0.5 = 1.1035
\]

### Step 3: Conclusion

Since the maximum sum of the left-hand side exceeds 1, we can conclude that:

\[
\frac{x}{2x^2 + 1} + \frac{y}{y^2 + 3} + \frac{z}{z^2 + 1} \geq 1
\]

Thus, the correct inequality to fill in the blank is:

\[
\frac{x}{2x^2 + 1} + \frac{y}{y^2 + 3} + \frac{z}{z^2 + 1} \geq 1
\]

Therefore, the answer is:

The answer is (B) $\geq$.