## Problem

For all real numbers $x, y, z$, consider the following expression:
$$
\frac{x^2-y^2}{2 x^2+1}+\frac{y^2-z^2}{2 y^2+2}+\frac{z^2-x^2}{2 z^2+1}\quad () \quad 0.
$$

Determine the correct inequality relation between the expression and 0.

Options:

(A) $\leq$ 

(B) $\geq$

(C) $=$ 

(D) $<$

(E) $>$

(F) None of the above

## Query

Task description: Please solve the problem with clear, rigorous, and logically sound steps. At the end of your response, state your answer in exactly this format: 'The answer is (Letter) Symbol', where Letter is one of the given options. Example: 'The answer is (A) $\leq$'.

Problem: For all real numbers $x, y, z$, consider the following expression:
$$
\frac{x^2-y^2}{2 x^2+1}+\frac{y^2-z^2}{2 y^2+2}+\frac{z^2-x^2}{2 z^2+1}\quad () \quad 0.
$$

Determine the correct inequality relation between the expression and 0.

Options:

(A) $\leq$ 

(B) $\geq$

(C) $=$ 

(D) $<$

(E) $>$

(F) None of the above

Please use some of the following theorems to solve the problem:
Theorem 1 (Category: Inequality Between Means, Nicknames: mean inequalities): Let $a_{1}, a_{2}, \ldots, a_{n}$ be positive real numbers. The numbers
$$
\begin{aligned}
& Q M=\sqrt{\frac{a_{1}^{2}+a_{2}^{2}+\cdots+a_{n}^{2}}{n}}, \quad A M=\frac{a_{1}+a_{2}+\cdots+a_{n}}{n} \\
& G M=\sqrt[n]{a_{1} a_{2} \cdots a_{n}} \quad \text { and } \quad H M=\frac{n}{\frac{1}{a_{1}}+\frac{1}{a_{2}}+\cdots+\frac{1}{a_{n}}}
\end{aligned}
$$
are called the quadratic, arithmetic, geometric and harmonic mean for the numbers $a_{1}, a_{2}, \ldots, a_{n}$, respectively, and we have
$$
Q M \geq A M \geq G M \geq H M
$$

Equalities occur if and only if $a_{1}=a_{2}=\cdots=a_{n}$.

Theorem 2 (Category: Cauchy-Schwarz Inequality, Nicknames: cauchy-schwarz inequality): Let $a_{1}, a_{2}, \ldots, a_{n}$ and $b_{1}, b_{2}$, $\ldots, b_{n}$ be real numbers. Then we have
$$
\left(\sum_{i=1}^{n} a_{i}^{2}\right)\left(\sum_{i=1}^{n} b_{i}^{2}\right) \geq\left(\sum_{i=1}^{n} a_{i} b_{i}\right)^{2}
$$
i.e.
$$
\left(a_{1}^{2}+a_{2}^{2}+\cdots+a_{n}^{2}\right)\left(b_{1}^{2}+b_{2}^{2}+\cdots+b_{n}^{2}\right) \geq\left(a_{1} b_{1}+a_{2} b_{2}+\cdots+a_{n} b_{n}\right)^{2}
$$

Equality occurs if and only if the sequences $\left(a_{1}, a_{2}, \ldots, a_{n}\right)$ and $\left(b_{1}, b_{2}\right.$, $\ldots, b_{n}$ ) are proportional, i.e. $\frac{a_{1}}{b_{1}}=\frac{a_{2}}{b_{2}}=\cdots=\frac{a_{n}}{b_{n}}$.

Theorem 3 (Category: Inequality Between Means, Nicknames: am-gm (arithmetic mean-geometric mean) inequality, am-gm): If $a_{1}, a_{2}, \ldots, a_{n}$ are nonnegative real numbers, then

$$
\frac{1}{n} \sum_{i=1}^{n} a_{i} \geq\left(a_{1} a_{2} \ldots a_{n}\right)^{\frac{1}{n}}
$$

with equality if and only if $a_{1}=a_{2}=\ldots=a_{n}$. This inequality is a special case of the Power Mean Inequality.

Solution:

## Response

To analyze the expression 

\[
E = \frac{x^2 - y^2}{2x^2 + 1} + \frac{y^2 - z^2}{2y^2 + 2} + \frac{z^2 - x^2}{2z^2 + 1},
\]

we will evaluate each term and their contributions to the overall expression.

### Step 1: Analyze Each Term

1. **First Term:**
   \[
   \frac{x^2 - y^2}{2x^2 + 1}
   \]
   This term can be rewritten as:
   \[
   \frac{(x-y)(x+y)}{2x^2 + 1}.
   \]
   The sign of this term depends on the sign of \(x^2 - y^2\). If \(x^2 > y^2\), the term is positive; if \(x^2 < y^2\), it is negative.

2. **Second Term:**
   \[
   \frac{y^2 - z^2}{2y^2 + 2}
   \]
   This term can be rewritten as:
   \[
   \frac{(y-z)(y+z)}{2(y^2 + 1)}.
   \]
   Similar to the first term, the sign depends on \(y^2 - z^2\).

3. **Third Term:**
   \[
   \frac{z^2 - x^2}{2z^2 + 1}
   \]
   This term can be rewritten as:
   \[
   \frac{(z-x)(z+x)}{2z^2 + 1}.
   \]
   Again, the sign depends on \(z^2 - x^2\).

### Step 2: Combine the Terms

The overall expression \(E\) is a sum of three terms, each of which can be positive or negative depending on the relationships between \(x^2\), \(y^2\), and \(z^2\). 

### Step 3: Consider Special Cases

To understand the behavior of \(E\), we can consider specific cases:

1. **Case 1: \(x = y = z\)**
   \[
   E = \frac{x^2 - x^2}{2x^2 + 1} + \frac{x^2 - x^2}{2x^2 + 2} + \frac{x^2 - x^2}{2x^2 + 1} = 0.
   \]

2. **Case 2: \(x = 1, y = 0, z = 0\)**
   \[
   E = \frac{1^2 - 0^2}{2 \cdot 1^2 + 1} + \frac{0^2 - 0^2}{2 \cdot 0^2 + 2} + \frac{0^2 - 1^2}{2 \cdot 0^2 + 1} = \frac{1}{3} + 0 - 1 = \frac{1}{3} - 1 = -\frac{2}{3}.
   \]

3. **Case 3: \(x = 0, y = 1, z = 0\)**
   \[
   E = \frac{0^2 - 1^2}{2 \cdot 0^2 + 1} + \frac{1^2 - 0^2}{2 \cdot 1^2 + 2} + \frac{0^2 - 0^2}{2 \cdot 0^2 + 1} = -1 + \frac{1}{4} + 0 = -1 + 0.25 = -0.75.
   \]

### Step 4: General Behavior

From the special cases, we see that \(E\) can be negative. However, we also found that \(E = 0\) when \(x = y = z\). 

### Conclusion

Since we can find values of \(x, y, z\) such that \(E < 0\) and also values such that \(E = 0\), we conclude that the expression can be less than or equal to zero. 

Thus, the correct inequality relation is:

\[
E \leq 0.
\]

Therefore, the answer is:

The answer is (A) $\leq$.