## Problem

Let $a_1, a_2, a_3, \ldots, a_n$ be real numbers with $n > 1$. Consider the following expression:
$$
\sqrt{a_1^2+(1-a_2)^2} + \sqrt{a_2^2+(1-a_3)^2} + \ldots + \sqrt{a_n^2+(1-a_1)^2} \quad () \quad \frac{n}{2}.
$$

Determine the correct inequality relation to fill in the blank.

Options:

(A) $\leq$ 

(B) $\geq$

(C) $=$ 

(D) $<$

(E) $>$

(F) None of the above

## Query

Task description: Please solve the problem with clear, rigorous, and logically sound steps. At the end of your response, state your answer in exactly this format: 'The answer is (Letter) Symbol', where Letter is one of the given options. Example: 'The answer is (A) $\leq$'.

Problem: Let $a_1, a_2, a_3, \ldots, a_n$ be real numbers with $n > 1$. Consider the following expression:
$$
\sqrt{a_1^2+(1-a_2)^2} + \sqrt{a_2^2+(1-a_3)^2} + \ldots + \sqrt{a_n^2+(1-a_1)^2} \quad () \quad \frac{n}{2}.
$$

Determine the correct inequality relation to fill in the blank.

Options:

(A) $\leq$ 

(B) $\geq$

(C) $=$ 

(D) $<$

(E) $>$

(F) None of the above

Please use some of the following theorems to solve the problem:
Theorem 1 (Category: Inequality Between Means, Nicknames: mean inequalities): Let $a_{1}, a_{2}, \ldots, a_{n}$ be positive real numbers. The numbers
$$
\begin{aligned}
& Q M=\sqrt{\frac{a_{1}^{2}+a_{2}^{2}+\cdots+a_{n}^{2}}{n}}, \quad A M=\frac{a_{1}+a_{2}+\cdots+a_{n}}{n} \\
& G M=\sqrt[n]{a_{1} a_{2} \cdots a_{n}} \quad \text { and } \quad H M=\frac{n}{\frac{1}{a_{1}}+\frac{1}{a_{2}}+\cdots+\frac{1}{a_{n}}}
\end{aligned}
$$
are called the quadratic, arithmetic, geometric and harmonic mean for the numbers $a_{1}, a_{2}, \ldots, a_{n}$, respectively, and we have
$$
Q M \geq A M \geq G M \geq H M
$$

Equalities occur if and only if $a_{1}=a_{2}=\cdots=a_{n}$.

Theorem 2 (Category: Cauchy-Schwarz Inequality, Nicknames: cauchy-schwarz inequality): Let $a_{1}, a_{2}, \ldots, a_{n}$ and $b_{1}, b_{2}$, $\ldots, b_{n}$ be real numbers. Then we have
$$
\left(\sum_{i=1}^{n} a_{i}^{2}\right)\left(\sum_{i=1}^{n} b_{i}^{2}\right) \geq\left(\sum_{i=1}^{n} a_{i} b_{i}\right)^{2}
$$
i.e.
$$
\left(a_{1}^{2}+a_{2}^{2}+\cdots+a_{n}^{2}\right)\left(b_{1}^{2}+b_{2}^{2}+\cdots+b_{n}^{2}\right) \geq\left(a_{1} b_{1}+a_{2} b_{2}+\cdots+a_{n} b_{n}\right)^{2}
$$

Equality occurs if and only if the sequences $\left(a_{1}, a_{2}, \ldots, a_{n}\right)$ and $\left(b_{1}, b_{2}\right.$, $\ldots, b_{n}$ ) are proportional, i.e. $\frac{a_{1}}{b_{1}}=\frac{a_{2}}{b_{2}}=\cdots=\frac{a_{n}}{b_{n}}$.

Theorem 3 (Category: Inequality Between Means, Nicknames: am-gm (arithmetic mean-geometric mean) inequality, am-gm): If $a_{1}, a_{2}, \ldots, a_{n}$ are nonnegative real numbers, then

$$
\frac{1}{n} \sum_{i=1}^{n} a_{i} \geq\left(a_{1} a_{2} \ldots a_{n}\right)^{\frac{1}{n}}
$$

with equality if and only if $a_{1}=a_{2}=\ldots=a_{n}$. This inequality is a special case of the Power Mean Inequality.

Solution:

## Response

To solve the problem, we need to analyze the expression 

\[
S = \sqrt{a_1^2 + (1 - a_2)^2} + \sqrt{a_2^2 + (1 - a_3)^2} + \ldots + \sqrt{a_n^2 + (1 - a_1)^2}
\]

and compare it to \(\frac{n}{2}\).

### Step 1: Understanding the Terms

Each term in the sum \(S\) can be interpreted geometrically. The term \(\sqrt{a_i^2 + (1 - a_{i+1})^2}\) represents the distance from the point \((a_i, 1 - a_{i+1})\) to the origin \((0, 0)\) in the Cartesian plane.

### Step 2: Applying the Cauchy-Schwarz Inequality

We can apply the Cauchy-Schwarz inequality to the sum \(S\). According to the Cauchy-Schwarz inequality:

\[
\left(\sum_{i=1}^{n} x_i^2\right)\left(\sum_{i=1}^{n} y_i^2\right) \geq \left(\sum_{i=1}^{n} x_i y_i\right)^2
\]

Let \(x_i = \sqrt{a_i^2 + (1 - a_{i+1})^2}\) and \(y_i = 1\) for all \(i\). Then we have:

\[
S^2 = \left(\sum_{i=1}^{n} \sqrt{a_i^2 + (1 - a_{i+1})^2}\right)^2 \leq n \sum_{i=1}^{n} (a_i^2 + (1 - a_{i+1})^2)
\]

### Step 3: Simplifying the Right Side

Now, we need to simplify the right-hand side:

\[
\sum_{i=1}^{n} (a_i^2 + (1 - a_{i+1})^2) = \sum_{i=1}^{n} a_i^2 + \sum_{i=1}^{n} (1 - a_{i+1})^2
\]

The second term can be rewritten as:

\[
\sum_{i=1}^{n} (1 - a_{i+1})^2 = \sum_{i=1}^{n} (1 - 2a_{i+1} + a_{i+1}^2) = n - 2\sum_{i=1}^{n} a_{i+1} + \sum_{i=1}^{n} a_{i+1}^2
\]

Thus, we have:

\[
S^2 \leq n \left(\sum_{i=1}^{n} a_i^2 + n - 2\sum_{i=1}^{n} a_{i+1} + \sum_{i=1}^{n} a_{i+1}^2\right)
\]

### Step 4: Analyzing the Result

To analyze the inequality \(S \geq \frac{n}{2}\), we can consider the case when all \(a_i\) are equal. If \(a_i = \frac{1}{2}\) for all \(i\), then:

\[
S = n \cdot \sqrt{\left(\frac{1}{2}\right)^2 + \left(1 - \frac{1}{2}\right)^2} = n \cdot \sqrt{\frac{1}{4} + \frac{1}{4}} = n \cdot \sqrt{\frac{1}{2}} = n \cdot \frac{1}{\sqrt{2}} \approx 0.707n
\]

This value is less than \(\frac{n}{2}\) for \(n > 1\).

### Conclusion

From the analysis, we can conclude that the sum \(S\) is generally less than \(\frac{n}{2}\) for \(n > 1\). Therefore, the correct inequality to fill in the blank is:

\[
\sqrt{a_1^2 + (1 - a_2)^2} + \sqrt{a_2^2 + (1 - a_3)^2} + \ldots + \sqrt{a_n^2 + (1 - a_1)^2} < \frac{n}{2}
\]

Thus, the answer is:

The answer is (D) $<$.