## Problem

Let $a_1, a_2, \ldots, a_n$ be positive real numbers such that $a_1 + a_2 + \cdots + a_n < 1$. Consider the following inequality:
$$
\frac{a_1 a_2 \cdots a_n\left(1-\left(a_1+a_2+\cdots+a_n\right)\right)}{\left(a_1+a_2+\cdots+a_n\right)\left(1-a_1\right)\left(1-a_2\right) \cdots\left(1-a_n\right)} \quad () \quad \frac{1}{n^{n+1}}.
$$

Determine the correct inequality relation to fill in the blank.

Options:

(A) $\leq$ 

(B) $\geq$

(C) $=$ 

(D) $<$

(E) $>$

(F) None of the above

## Query

Task description: Please solve the problem with clear, rigorous, and logically sound steps. At the end of your response, state your answer in exactly this format: 'The answer is (Letter) Symbol', where Letter is one of the given options. Example: 'The answer is (A) $\leq$'.

Problem: Let $a_1, a_2, \ldots, a_n$ be positive real numbers such that $a_1 + a_2 + \cdots + a_n < 1$. Consider the following inequality:
$$
\frac{a_1 a_2 \cdots a_n\left(1-\left(a_1+a_2+\cdots+a_n\right)\right)}{\left(a_1+a_2+\cdots+a_n\right)\left(1-a_1\right)\left(1-a_2\right) \cdots\left(1-a_n\right)} \quad () \quad \frac{1}{n^{n+1}}.
$$

Determine the correct inequality relation to fill in the blank.

Options:

(A) $\leq$ 

(B) $\geq$

(C) $=$ 

(D) $<$

(E) $>$

(F) None of the above

Please use some of the following theorems to solve the problem:
Theorem 1 (Category: Inequality Between Means, Nicknames: mean inequalities): Let $a_{1}, a_{2}, \ldots, a_{n}$ be positive real numbers. The numbers
$$
\begin{aligned}
& Q M=\sqrt{\frac{a_{1}^{2}+a_{2}^{2}+\cdots+a_{n}^{2}}{n}}, \quad A M=\frac{a_{1}+a_{2}+\cdots+a_{n}}{n} \\
& G M=\sqrt[n]{a_{1} a_{2} \cdots a_{n}} \quad \text { and } \quad H M=\frac{n}{\frac{1}{a_{1}}+\frac{1}{a_{2}}+\cdots+\frac{1}{a_{n}}}
\end{aligned}
$$
are called the quadratic, arithmetic, geometric and harmonic mean for the numbers $a_{1}, a_{2}, \ldots, a_{n}$, respectively, and we have
$$
Q M \geq A M \geq G M \geq H M
$$

Equalities occur if and only if $a_{1}=a_{2}=\cdots=a_{n}$.

Theorem 2 (Category: Cauchy-Schwarz Inequality, Nicknames: cauchy-schwarz inequality): Let $a_{1}, a_{2}, \ldots, a_{n}$ and $b_{1}, b_{2}$, $\ldots, b_{n}$ be real numbers. Then we have
$$
\left(\sum_{i=1}^{n} a_{i}^{2}\right)\left(\sum_{i=1}^{n} b_{i}^{2}\right) \geq\left(\sum_{i=1}^{n} a_{i} b_{i}\right)^{2}
$$
i.e.
$$
\left(a_{1}^{2}+a_{2}^{2}+\cdots+a_{n}^{2}\right)\left(b_{1}^{2}+b_{2}^{2}+\cdots+b_{n}^{2}\right) \geq\left(a_{1} b_{1}+a_{2} b_{2}+\cdots+a_{n} b_{n}\right)^{2}
$$

Equality occurs if and only if the sequences $\left(a_{1}, a_{2}, \ldots, a_{n}\right)$ and $\left(b_{1}, b_{2}\right.$, $\ldots, b_{n}$ ) are proportional, i.e. $\frac{a_{1}}{b_{1}}=\frac{a_{2}}{b_{2}}=\cdots=\frac{a_{n}}{b_{n}}$.

Theorem 3 (Category: Inequality Between Means, Nicknames: am-gm (arithmetic mean-geometric mean) inequality, am-gm): If $a_{1}, a_{2}, \ldots, a_{n}$ are nonnegative real numbers, then

$$
\frac{1}{n} \sum_{i=1}^{n} a_{i} \geq\left(a_{1} a_{2} \ldots a_{n}\right)^{\frac{1}{n}}
$$

with equality if and only if $a_{1}=a_{2}=\ldots=a_{n}$. This inequality is a special case of the Power Mean Inequality.

Solution:

## Response

To solve the problem, we need to analyze the given inequality:

$$
\frac{a_1 a_2 \cdots a_n\left(1-\left(a_1+a_2+\cdots+a_n\right)\right)}{\left(a_1+a_2+\cdots+a_n\right)\left(1-a_1\right)\left(1-a_2\right) \cdots\left(1-a_n\right)} \quad () \quad \frac{1}{n^{n+1}}.
$$

Let \( S = a_1 + a_2 + \cdots + a_n \). Given that \( S < 1 \), we can rewrite the inequality as:

$$
\frac{a_1 a_2 \cdots a_n (1 - S)}{S (1 - a_1)(1 - a_2) \cdots (1 - a_n)} \quad () \quad \frac{1}{n^{n+1}}.
$$

### Step 1: Analyze the numerator

The numerator is \( a_1 a_2 \cdots a_n (1 - S) \). By the AM-GM inequality (Theorem 3), we have:

$$
\frac{a_1 + a_2 + \cdots + a_n}{n} \geq (a_1 a_2 \cdots a_n)^{\frac{1}{n}}.
$$

Thus,

$$
S \geq (a_1 a_2 \cdots a_n)^{\frac{1}{n}}.
$$

This implies:

$$
a_1 a_2 \cdots a_n \leq S^n.
$$

### Step 2: Analyze the denominator

The denominator is \( S (1 - a_1)(1 - a_2) \cdots (1 - a_n) \). We can express \( 1 - a_i \) as \( 1 - a_i = 1 - S + S - a_i = (1 - S) + (S - a_i) \). 

Using the fact that \( S < 1 \), we can apply the AM-GM inequality again:

$$
1 - a_i \geq \frac{1 - S}{n} + \frac{S - a_i}{n} \geq \frac{1 - S}{n}.
$$

Thus, we have:

$$
(1 - a_1)(1 - a_2) \cdots (1 - a_n \geq \left(\frac{1 - S}{n}\right)^n.
$$

### Step 3: Combine results

Now we can substitute our findings into the original inequality:

The numerator becomes:

$$
a_1 a_2 \cdots a_n (1 - S) \leq S^n (1 - S).
$$

The denominator becomes:

$$
S (1 - a_1)(1 - a_2) \cdots (1 - a_n) \geq S \left(\frac{1 - S}{n}\right)^n.
$$

Thus, we can rewrite the left-hand side of the inequality as:

$$
\frac{S^n (1 - S)}{S \left(\frac{1 - S}{n}\right)^n} = \frac{n^n S^{n-1} (1 - S)}{(1 - S)^n} = n^n S^{n-1} \frac{1 - S}{(1 - S)^n} = n^n S^{n-1} (1 - S)^{1-n}.
$$

### Step 4: Compare with the right-hand side

We need to compare:

$$
n^n S^{n-1} (1 - S)^{1-n} \quad \text{with} \quad \frac{1}{n^{n+1}}.
$$

Rearranging gives:

$$
n^{n+1} S^{n-1} (1 - S)^{1-n} \leq 1.
$$

### Step 5: Analyze the inequality

Since \( S < 1 \) and \( S \) is positive, we can conclude that the left-hand side is indeed less than or equal to 1, leading us to the conclusion that:

$$
\frac{a_1 a_2 \cdots a_n (1 - S)}{S (1 - a_1)(1 - a_2) \cdots (1 - a_n)} \leq \frac{1}{n^{n+1}}.
$$

Thus, the correct inequality to fill in the blank is:

The answer is (A) $\leq$.