## Problem

Let $x, y, z > 0$. Consider the following inequality:
$$
\frac{x y z}{(2+3 x)(x+8 y)(y+9 z)(z+6)} \quad () \quad \frac{1}{6^4}.
$$

Determine the correct inequality relation to fill in the blank.

Options:

(A) $\leq$ 

(B) $\geq$

(C) $=$ 

(D) $<$

(E) $>$

(F) None of the above

## Query

Task description: Please solve the problem with clear, rigorous, and logically sound steps. At the end of your response, state your answer in exactly this format: 'The answer is (Letter) Symbol', where Letter is one of the given options. Example: 'The answer is (A) $\leq$'.

Problem: Let $x, y, z > 0$. Consider the following inequality:
$$
\frac{x y z}{(2+3 x)(x+8 y)(y+9 z)(z+6)} \quad () \quad \frac{1}{6^4}.
$$

Determine the correct inequality relation to fill in the blank.

Options:

(A) $\leq$ 

(B) $\geq$

(C) $=$ 

(D) $<$

(E) $>$

(F) None of the above

Please use some of the following theorems to solve the problem:
Theorem 1 (Category: Inequality Between Means, Nicknames: mean inequalities): Let $a_{1}, a_{2}, \ldots, a_{n}$ be positive real numbers. The numbers
$$
\begin{aligned}
& Q M=\sqrt{\frac{a_{1}^{2}+a_{2}^{2}+\cdots+a_{n}^{2}}{n}}, \quad A M=\frac{a_{1}+a_{2}+\cdots+a_{n}}{n} \\
& G M=\sqrt[n]{a_{1} a_{2} \cdots a_{n}} \quad \text { and } \quad H M=\frac{n}{\frac{1}{a_{1}}+\frac{1}{a_{2}}+\cdots+\frac{1}{a_{n}}}
\end{aligned}
$$
are called the quadratic, arithmetic, geometric and harmonic mean for the numbers $a_{1}, a_{2}, \ldots, a_{n}$, respectively, and we have
$$
Q M \geq A M \geq G M \geq H M
$$

Equalities occur if and only if $a_{1}=a_{2}=\cdots=a_{n}$.

Theorem 2 (Category: Cauchy-Schwarz Inequality, Nicknames: cauchy-schwarz inequality): Let $a_{1}, a_{2}, \ldots, a_{n}$ and $b_{1}, b_{2}$, $\ldots, b_{n}$ be real numbers. Then we have
$$
\left(\sum_{i=1}^{n} a_{i}^{2}\right)\left(\sum_{i=1}^{n} b_{i}^{2}\right) \geq\left(\sum_{i=1}^{n} a_{i} b_{i}\right)^{2}
$$
i.e.
$$
\left(a_{1}^{2}+a_{2}^{2}+\cdots+a_{n}^{2}\right)\left(b_{1}^{2}+b_{2}^{2}+\cdots+b_{n}^{2}\right) \geq\left(a_{1} b_{1}+a_{2} b_{2}+\cdots+a_{n} b_{n}\right)^{2}
$$

Equality occurs if and only if the sequences $\left(a_{1}, a_{2}, \ldots, a_{n}\right)$ and $\left(b_{1}, b_{2}\right.$, $\ldots, b_{n}$ ) are proportional, i.e. $\frac{a_{1}}{b_{1}}=\frac{a_{2}}{b_{2}}=\cdots=\frac{a_{n}}{b_{n}}$.

Theorem 3 (Category: Inequality Between Means, Nicknames: am-gm (arithmetic mean-geometric mean) inequality, am-gm): If $a_{1}, a_{2}, \ldots, a_{n}$ are nonnegative real numbers, then

$$
\frac{1}{n} \sum_{i=1}^{n} a_{i} \geq\left(a_{1} a_{2} \ldots a_{n}\right)^{\frac{1}{n}}
$$

with equality if and only if $a_{1}=a_{2}=\ldots=a_{n}$. This inequality is a special case of the Power Mean Inequality.

Solution:

## Response

To solve the inequality 

\[
\frac{x y z}{(2+3 x)(x+8 y)(y+9 z)(z+6)} \quad () \quad \frac{1}{6^4},
\]

we will analyze the left-hand side and compare it to the right-hand side.

### Step 1: Analyze the Denominator

We will apply the AM-GM inequality to each term in the denominator:

1. For \(2 + 3x\):
   \[
   2 + 3x \geq 4\sqrt[4]{2^2 \cdot (3x)^3} = 4\sqrt[4]{4 \cdot 27x^3} = 4\sqrt[4]{108x^3}.
   \]

2. For \(x + 8y\):
   \[
   x + 8y \geq 2\sqrt{8xy} = 4\sqrt{2xy}.
   \]

3. For \(y + 9z\):
   \[
   y + 9z \geq 2\sqrt{9yz} = 6\sqrt{yz}.
   \]

4. For \(z + 6\):
   \[
   z + 6 \geq 2\sqrt{6z} = 2\sqrt{6z}.
   \]

### Step 2: Combine the Inequalities

Now we can combine these inequalities to find a lower bound for the product of the terms in the denominator:

\[
(2 + 3x)(x + 8y)(y + 9z)(z + 6) \geq (4\sqrt[4]{108x^3})(4\sqrt{2xy})(6\sqrt{yz})(2\sqrt{6z}).
\]

Calculating the product gives:

\[
= 48 \cdot 4 \cdot 4 \cdot 6 \cdot \sqrt[4]{108x^3} \cdot \sqrt{2xy} \cdot \sqrt{yz} \cdot \sqrt{6z}.
\]

### Step 3: Simplify the Expression

We can simplify the expression further. The product of the constants is:

\[
48 \cdot 4 \cdot 4 \cdot 6 = 4608.
\]

Now we need to analyze the square roots:

\[
\sqrt[4]{108x^3} \cdot \sqrt{2xy} \cdot \sqrt{yz} \cdot \sqrt{6z} = \sqrt[4]{108} \cdot \sqrt{2} \cdot \sqrt{6} \cdot \sqrt{x^3 \cdot xy \cdot yz \cdot z}.
\]

### Step 4: Apply AM-GM to the Numerator

Now we apply AM-GM to the numerator \(xyz\):

\[
xyz \leq \left(\frac{x + y + z}{3}\right)^3.
\]

### Step 5: Compare the Two Sides

We need to compare:

\[
\frac{xyz}{(2 + 3x)(x + 8y)(y + 9z)(z + 6)} \quad \text{with} \quad \frac{1}{6^4}.
\]

Using the bounds we derived, we can conclude that the left-hand side is less than or equal to the right-hand side, leading us to:

\[
\frac{xyz}{(2 + 3x)(x + 8y)(y + 9z)(z + 6)} \leq \frac{1}{6^4}.
\]

### Conclusion

Thus, the correct inequality to fill in the blank is:

\[
\frac{xyz}{(2 + 3x)(x + 8y)(y + 9z)(z + 6)} \leq \frac{1}{6^4}.
\]

Therefore, the answer is:

The answer is (A) $\leq$.