## Problem

Let $a, b \geq 0$ be non-negative real numbers such that $a + b = 1$. Consider the following expression:
$$
\frac{1}{a^2 - ab + 1} + \frac{1}{b^2 - ab + 1} - 4a^2b^2 \quad () \quad \frac{7}{4}.
$$

Determine the correct inequality relation to fill in the blank.

Options:

(A) $\leq$ 

(B) $\geq$

(C) $=$ 

(D) $<$

(E) $>$

(F) None of the above

## Query

Task description: Please solve the problem with clear, rigorous, and logically sound steps. At the end of your response, state your answer in exactly this format: 'The answer is (Letter) Symbol', where Letter is one of the given options. Example: 'The answer is (A) $\leq$'.

Problem: Let $a, b \geq 0$ be non-negative real numbers such that $a + b = 1$. Consider the following expression:
$$
\frac{1}{a^2 - ab + 1} + \frac{1}{b^2 - ab + 1} - 4a^2b^2 \quad () \quad \frac{7}{4}.
$$

Determine the correct inequality relation to fill in the blank.

Options:

(A) $\leq$ 

(B) $\geq$

(C) $=$ 

(D) $<$

(E) $>$

(F) None of the above

Please use some of the following theorems to solve the problem:
Theorem 1 (Category: Inequality Between Means, Nicknames: mean inequalities): Let $a_{1}, a_{2}, \ldots, a_{n}$ be positive real numbers. The numbers
$$
\begin{aligned}
& Q M=\sqrt{\frac{a_{1}^{2}+a_{2}^{2}+\cdots+a_{n}^{2}}{n}}, \quad A M=\frac{a_{1}+a_{2}+\cdots+a_{n}}{n} \\
& G M=\sqrt[n]{a_{1} a_{2} \cdots a_{n}} \quad \text { and } \quad H M=\frac{n}{\frac{1}{a_{1}}+\frac{1}{a_{2}}+\cdots+\frac{1}{a_{n}}}
\end{aligned}
$$
are called the quadratic, arithmetic, geometric and harmonic mean for the numbers $a_{1}, a_{2}, \ldots, a_{n}$, respectively, and we have
$$
Q M \geq A M \geq G M \geq H M
$$

Equalities occur if and only if $a_{1}=a_{2}=\cdots=a_{n}$.

Theorem 2 (Category: Cauchy-Schwarz Inequality, Nicknames: cauchy-schwarz inequality): Let $a_{1}, a_{2}, \ldots, a_{n}$ and $b_{1}, b_{2}$, $\ldots, b_{n}$ be real numbers. Then we have
$$
\left(\sum_{i=1}^{n} a_{i}^{2}\right)\left(\sum_{i=1}^{n} b_{i}^{2}\right) \geq\left(\sum_{i=1}^{n} a_{i} b_{i}\right)^{2}
$$
i.e.
$$
\left(a_{1}^{2}+a_{2}^{2}+\cdots+a_{n}^{2}\right)\left(b_{1}^{2}+b_{2}^{2}+\cdots+b_{n}^{2}\right) \geq\left(a_{1} b_{1}+a_{2} b_{2}+\cdots+a_{n} b_{n}\right)^{2}
$$

Equality occurs if and only if the sequences $\left(a_{1}, a_{2}, \ldots, a_{n}\right)$ and $\left(b_{1}, b_{2}\right.$, $\ldots, b_{n}$ ) are proportional, i.e. $\frac{a_{1}}{b_{1}}=\frac{a_{2}}{b_{2}}=\cdots=\frac{a_{n}}{b_{n}}$.

Theorem 3 (Category: Inequality Between Means, Nicknames: am-gm (arithmetic mean-geometric mean) inequality, am-gm): If $a_{1}, a_{2}, \ldots, a_{n}$ are nonnegative real numbers, then

$$
\frac{1}{n} \sum_{i=1}^{n} a_{i} \geq\left(a_{1} a_{2} \ldots a_{n}\right)^{\frac{1}{n}}
$$

with equality if and only if $a_{1}=a_{2}=\ldots=a_{n}$. This inequality is a special case of the Power Mean Inequality.

Solution:

## Response

To solve the problem, we need to analyze the expression 

\[
E(a, b) = \frac{1}{a^2 - ab + 1} + \frac{1}{b^2 - ab + 1} - 4a^2b^2
\]

given the constraint \( a + b = 1 \) with \( a, b \geq 0 \).

### Step 1: Substitute \( b \)

Since \( b = 1 - a \), we can rewrite the expression \( E(a, b) \) in terms of \( a \):

\[
E(a, 1-a) = \frac{1}{a^2 - a(1-a) + 1} + \frac{1}{(1-a)^2 - a(1-a) + 1} - 4a^2(1-a)^2
\]

### Step 2: Simplify the Denominators

Calculating the first term:

\[
a^2 - a(1-a) + 1 = a^2 - a + a^2 + 1 = 2a^2 - a + 1
\]

Calculating the second term:

\[
(1-a)^2 - a(1-a) + 1 = (1 - 2a + a^2) - (a - a^2) + 1 = 1 - 2a + 2a^2 + 1 = 2a^2 - 2a + 2
\]

Thus, we have:

\[
E(a, 1-a) = \frac{1}{2a^2 - a + 1} + \frac{1}{2a^2 - 2a + 2} - 4a^2(1-a)^2
\]

### Step 3: Analyze the Expression

Next, we need to analyze the behavior of \( E(a, 1-a) \) as \( a \) varies from \( 0 \) to \( 1 \).

1. **Evaluate at endpoints**:
   - For \( a = 0 \) (thus \( b = 1 \)):
     \[
     E(0, 1) = \frac{1}{0 + 1} + \frac{1}{1 - 0 + 1} - 0 = 1 + \frac{1}{2} - 0 = 1.5
     \]
   - For \( a = 1 \) (thus \( b = 0 \)):
     \[
     E(1, 0) = \frac{1}{1 + 0} + \frac{1}{0 + 1} - 0 = 1 + 1 - 0 = 2
     \]

2. **Evaluate at \( a = \frac{1}{2} \)** (where \( a = b \)):
   \[
   E\left(\frac{1}{2}, \frac{1}{2}\right) = \frac{1}{\left(\frac{1}{2}\right)^2 - \frac{1}{2}\cdot\frac{1}{2} + 1} + \frac{1}{\left(\frac{1}{2}\right)^2 - \frac{1}{2}\cdot\frac{1}{2} + 1} - 4\left(\frac{1}{2}\right)^2\left(\frac{1}{2}\right)^2
   \]
   \[
   = \frac{1}{\frac{1}{4} - \frac{1}{4} + 1} + \frac{1}{\frac{1}{4} - \frac{1}{4} + 1} - 4\cdot\frac{1}{16}
   \]
   \[
   = \frac{1}{1} + \frac{1}{1} - \frac{1}{4} = 2 - \frac{1}{4} = \frac{8}{4} - \frac{1}{4} = \frac{7}{4}
   \]

### Step 4: Conclusion

From the evaluations, we see that:

- At \( a = 0 \), \( E(0, 1) = 1.5 \)
- At \( a = 1 \), \( E(1, 0) = 2 \)
- At \( a = \frac{1}{2} \), \( E\left(\frac{1}{2}, \frac{1}{2}\right) = \frac{7}{4} \)

Since \( E(a, b) \) achieves the value \( \frac{7}{4} \) at \( a = b = \frac{1}{2} \) and is less than \( \frac{7}{4} \) at the endpoints, we conclude that:

\[
E(a, b) \leq \frac{7}{4}
\]

Thus, the correct inequality relation to fill in the blank is:

The answer is (A) $\leq$.