## Problem

For $a, b > 0$, find the minimal constant $C$ such that the following inequality holds for all $a, b$:
$$
\frac{1}{2}(a+b)^2 + C(a+b) \geq a \sqrt{b} + b \sqrt{a}.
$$

## Query

Task description: Please solve the problem with clear, rigorous, and logically sound steps. At the end of your response, state your answer in exactly this format: 'The answer is $C=X$', where X is your calculated numerical bound value. Example: 'The answer is $C=1$'.

Problem: For $a, b > 0$, find the minimal constant $C$ such that the following inequality holds for all $a, b$:
$$
\frac{1}{2}(a+b)^2 + C(a+b) \geq a \sqrt{b} + b \sqrt{a}.
$$

Please use some of the following theorems to solve the problem:
Theorem 1 (Category: Inequality Between Means, Nicknames: mean inequalities): Let $a_{1}, a_{2}, \ldots, a_{n}$ be positive real numbers. The numbers
$$
\begin{aligned}
& Q M=\sqrt{\frac{a_{1}^{2}+a_{2}^{2}+\cdots+a_{n}^{2}}{n}}, \quad A M=\frac{a_{1}+a_{2}+\cdots+a_{n}}{n} \\
& G M=\sqrt[n]{a_{1} a_{2} \cdots a_{n}} \quad \text { and } \quad H M=\frac{n}{\frac{1}{a_{1}}+\frac{1}{a_{2}}+\cdots+\frac{1}{a_{n}}}
\end{aligned}
$$
are called the quadratic, arithmetic, geometric and harmonic mean for the numbers $a_{1}, a_{2}, \ldots, a_{n}$, respectively, and we have
$$
Q M \geq A M \geq G M \geq H M
$$

Equalities occur if and only if $a_{1}=a_{2}=\cdots=a_{n}$.

Theorem 2 (Category: Cauchy-Schwarz Inequality, Nicknames: cauchy-schwarz inequality): Let $a_{1}, a_{2}, \ldots, a_{n}$ and $b_{1}, b_{2}$, $\ldots, b_{n}$ be real numbers. Then we have
$$
\left(\sum_{i=1}^{n} a_{i}^{2}\right)\left(\sum_{i=1}^{n} b_{i}^{2}\right) \geq\left(\sum_{i=1}^{n} a_{i} b_{i}\right)^{2}
$$
i.e.
$$
\left(a_{1}^{2}+a_{2}^{2}+\cdots+a_{n}^{2}\right)\left(b_{1}^{2}+b_{2}^{2}+\cdots+b_{n}^{2}\right) \geq\left(a_{1} b_{1}+a_{2} b_{2}+\cdots+a_{n} b_{n}\right)^{2}
$$

Equality occurs if and only if the sequences $\left(a_{1}, a_{2}, \ldots, a_{n}\right)$ and $\left(b_{1}, b_{2}\right.$, $\ldots, b_{n}$ ) are proportional, i.e. $\frac{a_{1}}{b_{1}}=\frac{a_{2}}{b_{2}}=\cdots=\frac{a_{n}}{b_{n}}$.

Theorem 3 (Category: Inequality Between Means, Nicknames: am-gm (arithmetic mean-geometric mean) inequality, am-gm): If $a_{1}, a_{2}, \ldots, a_{n}$ are nonnegative real numbers, then

$$
\frac{1}{n} \sum_{i=1}^{n} a_{i} \geq\left(a_{1} a_{2} \ldots a_{n}\right)^{\frac{1}{n}}
$$

with equality if and only if $a_{1}=a_{2}=\ldots=a_{n}$. This inequality is a special case of the Power Mean Inequality.

Solution:

## Response

To find the minimal constant \( C \) such that the inequality 

\[
\frac{1}{2}(a+b)^2 + C(a+b) \geq a \sqrt{b} + b \sqrt{a}
\]

holds for all \( a, b > 0 \), we will analyze the inequality step by step.

First, we can rewrite the right-hand side using the Cauchy-Schwarz inequality. According to Cauchy-Schwarz, we have:

\[
(a+b)(\sqrt{b} + \sqrt{a}) \geq a \sqrt{b} + b \sqrt{a}.
\]

This implies:

\[
a \sqrt{b} + b \sqrt{a} \leq (a+b) \sqrt{a+b}.
\]

Now, we can express the inequality we want to satisfy as:

\[
\frac{1}{2}(a+b)^2 + C(a+b) \geq (a+b) \sqrt{a+b}.
\]

Dividing both sides by \( a+b \) (which is positive since \( a, b > 0 \)), we get:

\[
\frac{1}{2}(a+b) + C \geq \sqrt{a+b}.
\]

Let \( s = a + b \). The inequality simplifies to:

\[
\frac{1}{2}s + C \geq \sqrt{s}.
\]

Rearranging gives:

\[
C \geq \sqrt{s} - \frac{1}{2}s.
\]

To find the minimal \( C \), we need to analyze the expression \( \sqrt{s} - \frac{1}{2}s \). We can define a function:

\[
f(s) = \sqrt{s} - \frac{1}{2}s.
\]

Next, we will find the critical points of \( f(s) \) by taking its derivative:

\[
f'(s) = \frac{1}{2\sqrt{s}} - \frac{1}{2}.
\]

Setting the derivative to zero to find critical points:

\[
\frac{1}{2\sqrt{s}} - \frac{1}{2} = 0 \implies \frac{1}{2\sqrt{s}} = \frac{1}{2} \implies \sqrt{s} = 1 \implies s = 1.
\]

Now we evaluate \( f(s) \) at \( s = 1 \):

\[
f(1) = \sqrt{1} - \frac{1}{2} \cdot 1 = 1 - \frac{1}{2} = \frac{1}{2}.
\]

Next, we check the behavior of \( f(s) \) as \( s \to 0 \) and \( s \to \infty \):

- As \( s \to 0 \), \( f(s) \to 0 - 0 = 0 \).
- As \( s \to \infty \), \( f(s) \to \infty - \infty = -\infty \).

Thus, the minimum value of \( f(s) \) occurs at \( s = 1 \) and is \( \frac{1}{2} \). Therefore, the minimal constant \( C \) that satisfies the inequality for all \( a, b > 0 \) is:

\[
C = \frac{1}{2}.
\]

Thus, the final answer is:

\[
\text{The answer is } C = \frac{1}{2}.
\]