## Problem

Let $x, y, z > 0$ such that $x + y + z = xyz$. Find the smallest constant $C$ such that the following inequality holds for all $x, y, z$ satisfying the given constraint:
$$
(x-1)(y-1)(z-1) \leq C
$$

## Query

Task description: Please solve the problem with clear, rigorous, and logically sound steps. At the end of your response, state your answer in exactly this format: 'The answer is $C=X$', where X is your calculated numerical bound value. Example: 'The answer is $C=1$'.

Problem: Let $x, y, z > 0$ such that $x + y + z = xyz$. Find the smallest constant $C$ such that the following inequality holds for all $x, y, z$ satisfying the given constraint:
$$
(x-1)(y-1)(z-1) \leq C
$$

Please use some of the following theorems to solve the problem:
Theorem 1 (Category: Inequality Between Means, Nicknames: mean inequalities): Let $a_{1}, a_{2}, \ldots, a_{n}$ be positive real numbers. The numbers
$$
\begin{aligned}
& Q M=\sqrt{\frac{a_{1}^{2}+a_{2}^{2}+\cdots+a_{n}^{2}}{n}}, \quad A M=\frac{a_{1}+a_{2}+\cdots+a_{n}}{n} \\
& G M=\sqrt[n]{a_{1} a_{2} \cdots a_{n}} \quad \text { and } \quad H M=\frac{n}{\frac{1}{a_{1}}+\frac{1}{a_{2}}+\cdots+\frac{1}{a_{n}}}
\end{aligned}
$$
are called the quadratic, arithmetic, geometric and harmonic mean for the numbers $a_{1}, a_{2}, \ldots, a_{n}$, respectively, and we have
$$
Q M \geq A M \geq G M \geq H M
$$

Equalities occur if and only if $a_{1}=a_{2}=\cdots=a_{n}$.

Theorem 2 (Category: Cauchy-Schwarz Inequality, Nicknames: cauchy-schwarz inequality): Let $a_{1}, a_{2}, \ldots, a_{n}$ and $b_{1}, b_{2}$, $\ldots, b_{n}$ be real numbers. Then we have
$$
\left(\sum_{i=1}^{n} a_{i}^{2}\right)\left(\sum_{i=1}^{n} b_{i}^{2}\right) \geq\left(\sum_{i=1}^{n} a_{i} b_{i}\right)^{2}
$$
i.e.
$$
\left(a_{1}^{2}+a_{2}^{2}+\cdots+a_{n}^{2}\right)\left(b_{1}^{2}+b_{2}^{2}+\cdots+b_{n}^{2}\right) \geq\left(a_{1} b_{1}+a_{2} b_{2}+\cdots+a_{n} b_{n}\right)^{2}
$$

Equality occurs if and only if the sequences $\left(a_{1}, a_{2}, \ldots, a_{n}\right)$ and $\left(b_{1}, b_{2}\right.$, $\ldots, b_{n}$ ) are proportional, i.e. $\frac{a_{1}}{b_{1}}=\frac{a_{2}}{b_{2}}=\cdots=\frac{a_{n}}{b_{n}}$.

Theorem 3 (Category: Inequality Between Means, Nicknames: am-gm (arithmetic mean-geometric mean) inequality, am-gm): If $a_{1}, a_{2}, \ldots, a_{n}$ are nonnegative real numbers, then

$$
\frac{1}{n} \sum_{i=1}^{n} a_{i} \geq\left(a_{1} a_{2} \ldots a_{n}\right)^{\frac{1}{n}}
$$

with equality if and only if $a_{1}=a_{2}=\ldots=a_{n}$. This inequality is a special case of the Power Mean Inequality.

Solution:

## Response

To solve the problem, we start with the condition given: \( x + y + z = xyz \). We want to find the smallest constant \( C \) such that the inequality 

\[
(x-1)(y-1)(z-1) \leq C
\]

holds for all positive \( x, y, z \) satisfying the condition.

First, we can rewrite the expression \( (x-1)(y-1)(z-1) \):

\[
(x-1)(y-1)(z-1) = xyz - (xy + xz + yz) + (x + y + z) - 1
\]

Using the condition \( x + y + z = xyz \), we substitute this into our expression:

\[
(x-1)(y-1)(z-1) = xyz - (xy + xz + yz) + xyz - 1 = 2xyz - (xy + xz + yz) - 1
\]

Next, we need to analyze the values of \( x, y, z \) under the constraint \( x + y + z = xyz \). A common substitution for this type of problem is to set \( x = \frac{a}{b}, y = \frac{b}{c}, z = \frac{c}{a} \) for positive \( a, b, c \). This substitution satisfies the condition because:

\[
\frac{a}{b} + \frac{b}{c} + \frac{c}{a} = \frac{a^2c + b^2a + c^2b}{abc} = \frac{abc}{abc} = 1
\]

Thus, we can express \( x, y, z \) in terms of \( a, b, c \) and analyze the product \( (x-1)(y-1)(z-1) \).

To find the maximum value of \( (x-1)(y-1)(z-1) \), we can use symmetry and the AM-GM inequality. By the AM-GM inequality, we have:

\[
\frac{x + y + z}{3} \geq \sqrt[3]{xyz}
\]

Given \( x + y + z = xyz \), we can set \( t = xyz \). Then:

\[
\frac{t}{3} \geq \sqrt[3]{t^3} \implies t \geq 3
\]

Now, we can analyze the case when \( x = y = z \). Let \( x = y = z = k \). Then:

\[
3k = k^3 \implies k^3 - 3k = 0 \implies k(k^2 - 3) = 0
\]

Since \( k > 0 \), we have \( k = \sqrt{3} \). Thus, substituting back, we find:

\[
(x-1)(y-1)(z-1) = (k-1)^3 = (\sqrt{3} - 1)^3
\]

Calculating \( (\sqrt{3} - 1)^3 \):

\[
(\sqrt{3} - 1)^3 = 3\sqrt{3} - 3\sqrt{3} + 3 - 1 = 2\sqrt{3} - 3
\]

To find the numerical value of \( 2\sqrt{3} - 3 \):

\[
\sqrt{3} \approx 1.732 \implies 2\sqrt{3} \approx 3.464 \implies 2\sqrt{3} - 3 \approx 0.464
\]

Thus, the maximum value of \( (x-1)(y-1)(z-1) \) is \( 2\sqrt{3} - 3 \).

Finally, we conclude that the smallest constant \( C \) such that the inequality holds for all positive \( x, y, z \) satisfying \( x + y + z = xyz \) is:

\[
C = 2\sqrt{3} - 3
\]

Therefore, the answer is:

\[
\text{The answer is } C = 2\sqrt{3} - 3
\]