## Problem

Let $a, b, c \geq 0$ satisfy $ab + bc + ca = 1$. Determine the minimal constant $C$ such that the following inequality holds for all $a, b, c$:

$$
\sum \frac{ab}{(a+b)(c^2+1)} \leq \frac{C}{a+b+c}.
$$

## Query

Task description: Please solve the problem with clear, rigorous, and logically sound steps. At the end of your response, state your answer in exactly this format: 'The answer is $C=X$', where X is your calculated numerical bound value. Example: 'The answer is $C=1$'.

Problem: Let $a, b, c \geq 0$ satisfy $ab + bc + ca = 1$. Determine the minimal constant $C$ such that the following inequality holds for all $a, b, c$:

$$
\sum \frac{ab}{(a+b)(c^2+1)} \leq \frac{C}{a+b+c}.
$$

Please use some of the following theorems to solve the problem:
Theorem 1 (Category: Inequality Between Means, Nicknames: mean inequalities): Let $a_{1}, a_{2}, \ldots, a_{n}$ be positive real numbers. The numbers
$$
\begin{aligned}
& Q M=\sqrt{\frac{a_{1}^{2}+a_{2}^{2}+\cdots+a_{n}^{2}}{n}}, \quad A M=\frac{a_{1}+a_{2}+\cdots+a_{n}}{n} \\
& G M=\sqrt[n]{a_{1} a_{2} \cdots a_{n}} \quad \text { and } \quad H M=\frac{n}{\frac{1}{a_{1}}+\frac{1}{a_{2}}+\cdots+\frac{1}{a_{n}}}
\end{aligned}
$$
are called the quadratic, arithmetic, geometric and harmonic mean for the numbers $a_{1}, a_{2}, \ldots, a_{n}$, respectively, and we have
$$
Q M \geq A M \geq G M \geq H M
$$

Equalities occur if and only if $a_{1}=a_{2}=\cdots=a_{n}$.

Theorem 2 (Category: Cauchy-Schwarz Inequality, Nicknames: cauchy-schwarz inequality): Let $a_{1}, a_{2}, \ldots, a_{n}$ and $b_{1}, b_{2}$, $\ldots, b_{n}$ be real numbers. Then we have
$$
\left(\sum_{i=1}^{n} a_{i}^{2}\right)\left(\sum_{i=1}^{n} b_{i}^{2}\right) \geq\left(\sum_{i=1}^{n} a_{i} b_{i}\right)^{2}
$$
i.e.
$$
\left(a_{1}^{2}+a_{2}^{2}+\cdots+a_{n}^{2}\right)\left(b_{1}^{2}+b_{2}^{2}+\cdots+b_{n}^{2}\right) \geq\left(a_{1} b_{1}+a_{2} b_{2}+\cdots+a_{n} b_{n}\right)^{2}
$$

Equality occurs if and only if the sequences $\left(a_{1}, a_{2}, \ldots, a_{n}\right)$ and $\left(b_{1}, b_{2}\right.$, $\ldots, b_{n}$ ) are proportional, i.e. $\frac{a_{1}}{b_{1}}=\frac{a_{2}}{b_{2}}=\cdots=\frac{a_{n}}{b_{n}}$.

Theorem 3 (Category: Inequality Between Means, Nicknames: am-gm (arithmetic mean-geometric mean) inequality, am-gm): If $a_{1}, a_{2}, \ldots, a_{n}$ are nonnegative real numbers, then

$$
\frac{1}{n} \sum_{i=1}^{n} a_{i} \geq\left(a_{1} a_{2} \ldots a_{n}\right)^{\frac{1}{n}}
$$

with equality if and only if $a_{1}=a_{2}=\ldots=a_{n}$. This inequality is a special case of the Power Mean Inequality.

Solution:

## Response

To solve the problem, we need to analyze the inequality 

\[
\sum \frac{ab}{(a+b)(c^2+1)} \leq \frac{C}{a+b+c}
\]

given the constraint \( ab + bc + ca = 1 \) for non-negative \( a, b, c \).

### Step 1: Analyze the left-hand side

We can rewrite the left-hand side as:

\[
\sum \frac{ab}{(a+b)(c^2+1)} = \frac{ab}{(a+b)(c^2+1)} + \frac{bc}{(b+c)(a^2+1)} + \frac{ca}{(c+a)(b^2+1)}
\]

### Step 2: Apply Cauchy-Schwarz Inequality

Using the Cauchy-Schwarz inequality, we can estimate each term. For the first term, we have:

\[
\frac{ab}{(a+b)(c^2+1)} \leq \frac{ab}{(a+b)(1)} = \frac{ab}{a+b}
\]

Thus, we can write:

\[
\sum \frac{ab}{(a+b)(c^2+1)} \leq \sum \frac{ab}{a+b}
\]

### Step 3: Simplify the sum

Now we need to analyze \( \sum \frac{ab}{a+b} \). By applying the Cauchy-Schwarz inequality again, we have:

\[
\sum \frac{ab}{a+b} \leq \frac{(ab + bc + ca)^2}{\sum (a+b)} = \frac{1^2}{a+b+c} = \frac{1}{a+b+c}
\]

### Step 4: Combine results

Thus, we have:

\[
\sum \frac{ab}{(a+b)(c^2+1)} \leq \frac{1}{a+b+c}
\]

This implies that:

\[
\frac{C}{a+b+c} \geq \frac{1}{a+b+c}
\]

### Step 5: Determine the constant \( C \)

From the above inequality, we can conclude that:

\[
C \geq 1
\]

### Step 6: Check if \( C = 1 \) is achievable

To check if \( C = 1 \) is achievable, we can consider the case when \( a = b = c \). If we set \( a = b = c = \frac{1}{\sqrt{3}} \), we have:

\[
ab + bc + ca = 3 \cdot \left(\frac{1}{\sqrt{3}} \cdot \frac{1}{\sqrt{3}}\right) = 1
\]

Calculating the left-hand side:

\[
\sum \frac{ab}{(a+b)(c^2+1)} = 3 \cdot \frac{\left(\frac{1}{\sqrt{3}} \cdot \frac{1}{\sqrt{3}}\right)}{\left(\frac{2}{\sqrt{3}}\right)\left(\left(\frac{1}{\sqrt{3}}\right)^2 + 1\right)} = 3 \cdot \frac{\frac{1}{3}}{\frac{2}{\sqrt{3}} \cdot \left(\frac{1}{3} + 1\right)} = 3 \cdot \frac{\frac{1}{3}}{\frac{2}{\sqrt{3}} \cdot \frac{4}{3}} = \frac{3\sqrt{3}}{8}
\]

And the right-hand side:

\[
\frac{1}{a+b+c} = \frac{1}{\sqrt{3}} = \frac{\sqrt{3}}{3}
\]

Since \( \frac{3\sqrt{3}}{8} \leq \frac{\sqrt{3}}{3} \) holds true, we conclude that \( C = 1 \) is indeed achievable.

### Conclusion

Thus, the minimal constant \( C \) such that the inequality holds for all non-negative \( a, b, c \) satisfying \( ab + bc + ca = 1 \) is:

\[
\boxed{1}
\]

The answer is \( C=1 \).