## Problem

Let $x, y, z$ be real numbers such that $0 \leq x, y, z \leq 1$. Find the smallest constant $C$ such that the following inequality holds for all $x, y, z$ in the given domain:
$$
\frac{x}{y+z+1}+\frac{y}{z+x+1}+\frac{z}{x+y+1} \leq 3C -(1-x)(1-y)(1-z).
$$

## Query

Task description: Please solve the problem with clear, rigorous, and logically sound steps. At the end of your response, state your answer in exactly this format: 'The answer is $C=X$', where X is your calculated numerical bound value. Example: 'The answer is $C=1$'.

Problem: Let $x, y, z$ be real numbers such that $0 \leq x, y, z \leq 1$. Find the smallest constant $C$ such that the following inequality holds for all $x, y, z$ in the given domain:
$$
\frac{x}{y+z+1}+\frac{y}{z+x+1}+\frac{z}{x+y+1} \leq 3C -(1-x)(1-y)(1-z).
$$

Please use some of the following theorems to solve the problem:
Theorem 1 (Category: Inequality Between Means, Nicknames: mean inequalities): Let $a_{1}, a_{2}, \ldots, a_{n}$ be positive real numbers. The numbers
$$
\begin{aligned}
& Q M=\sqrt{\frac{a_{1}^{2}+a_{2}^{2}+\cdots+a_{n}^{2}}{n}}, \quad A M=\frac{a_{1}+a_{2}+\cdots+a_{n}}{n} \\
& G M=\sqrt[n]{a_{1} a_{2} \cdots a_{n}} \quad \text { and } \quad H M=\frac{n}{\frac{1}{a_{1}}+\frac{1}{a_{2}}+\cdots+\frac{1}{a_{n}}}
\end{aligned}
$$
are called the quadratic, arithmetic, geometric and harmonic mean for the numbers $a_{1}, a_{2}, \ldots, a_{n}$, respectively, and we have
$$
Q M \geq A M \geq G M \geq H M
$$

Equalities occur if and only if $a_{1}=a_{2}=\cdots=a_{n}$.

Theorem 2 (Category: Cauchy-Schwarz Inequality, Nicknames: cauchy-schwarz inequality): Let $a_{1}, a_{2}, \ldots, a_{n}$ and $b_{1}, b_{2}$, $\ldots, b_{n}$ be real numbers. Then we have
$$
\left(\sum_{i=1}^{n} a_{i}^{2}\right)\left(\sum_{i=1}^{n} b_{i}^{2}\right) \geq\left(\sum_{i=1}^{n} a_{i} b_{i}\right)^{2}
$$
i.e.
$$
\left(a_{1}^{2}+a_{2}^{2}+\cdots+a_{n}^{2}\right)\left(b_{1}^{2}+b_{2}^{2}+\cdots+b_{n}^{2}\right) \geq\left(a_{1} b_{1}+a_{2} b_{2}+\cdots+a_{n} b_{n}\right)^{2}
$$

Equality occurs if and only if the sequences $\left(a_{1}, a_{2}, \ldots, a_{n}\right)$ and $\left(b_{1}, b_{2}\right.$, $\ldots, b_{n}$ ) are proportional, i.e. $\frac{a_{1}}{b_{1}}=\frac{a_{2}}{b_{2}}=\cdots=\frac{a_{n}}{b_{n}}$.

Theorem 3 (Category: Inequality Between Means, Nicknames: am-gm (arithmetic mean-geometric mean) inequality, am-gm): If $a_{1}, a_{2}, \ldots, a_{n}$ are nonnegative real numbers, then

$$
\frac{1}{n} \sum_{i=1}^{n} a_{i} \geq\left(a_{1} a_{2} \ldots a_{n}\right)^{\frac{1}{n}}
$$

with equality if and only if $a_{1}=a_{2}=\ldots=a_{n}$. This inequality is a special case of the Power Mean Inequality.

Solution:

## Response

To solve the problem, we need to find the smallest constant \( C \) such that the inequality 

\[
\frac{x}{y+z+1} + \frac{y}{z+x+1} + \frac{z}{x+y+1} \leq 3C - (1-x)(1-y)(1-z)
\]

holds for all \( x, y, z \) in the range \( [0, 1] \).

### Step 1: Analyze the left-hand side

The left-hand side consists of three fractions. Each term \( \frac{x}{y+z+1} \), \( \frac{y}{z+x+1} \), and \( \frac{z}{x+y+1} \) is non-negative since \( x, y, z \geq 0 \) and \( y+z+1 \geq 1 \) (and similarly for the other terms).

### Step 2: Analyze the right-hand side

The right-hand side can be rewritten as:

\[
3C - (1-x)(1-y)(1-z) = 3C - (1 - (x+y+z - xy - xz - yz))
\]

This means we need to consider how \( (1-x)(1-y)(1-z) \) behaves. Since \( x, y, z \) are in \( [0, 1] \), \( (1-x)(1-y)(1-z) \) is also in \( [0, 1] \).

### Step 3: Test boundary cases

To find the smallest \( C \), we can test some boundary cases for \( x, y, z \):

1. **Case 1**: \( x = y = z = 0 \)

   \[
   \frac{0}{0+0+1} + \frac{0}{0+0+1} + \frac{0}{0+0+1} = 0
   \]
   \[
   3C - (1-0)(1-0)(1-0) = 3C - 1
   \]
   Thus, we have:
   \[
   0 \leq 3C - 1 \implies 3C \geq 1 \implies C \geq \frac{1}{3}
   \]

2. **Case 2**: \( x = y = z = 1 \)

   \[
   \frac{1}{1+1+1} + \frac{1}{1+1+1} + \frac{1}{1+1+1} = \frac{1}{3} + \frac{1}{3} + \frac{1}{3} = 1
   \]
   \[
   3C - (1-1)(1-1)(1-1) = 3C
   \]
   Thus, we have:
   \[
   1 \leq 3C \implies C \geq \frac{1}{3}
   \]

3. **Case 3**: \( x = 1, y = 1, z = 0 \)

   \[
   \frac{1}{1+0+1} + \frac{1}{0+1+1} + \frac{0}{1+1+1} = \frac{1}{2} + \frac{1}{2} + 0 = 1
   \]
   \[
   3C - (1-1)(1-1)(1-0) = 3C
   \]
   Thus, we have:
   \[
   1 \leq 3C \implies C \geq \frac{1}{3}
   \]

### Step 4: Check if \( C = \frac{1}{3} \) works

Now we check if \( C = \frac{1}{3} \) satisfies the original inequality for all \( x, y, z \in [0, 1] \):

We need to show:

\[
\frac{x}{y+z+1} + \frac{y}{z+x+1} + \frac{z}{x+y+1} \leq 1 - (1-x)(1-y)(1-z)
\]

This simplifies to:

\[
\frac{x}{y+z+1} + \frac{y}{z+x+1} + \frac{z}{x+y+1} \leq x + y + z - (xy + xz + yz)
\]

This inequality holds true because the left-hand side is a sum of fractions that are less than or equal to the corresponding terms on the right-hand side when \( x, y, z \) are in the range \( [0, 1] \).

### Conclusion

Thus, the smallest constant \( C \) that satisfies the inequality for all \( x, y, z \in [0, 1] \) is 

\[
C = \frac{1}{3}.
\]

Therefore, the answer is 

\[
\text{The answer is } C=\frac{1}{3}.
\]