## Problem

Let $a, b, c$ be positive real numbers greater than 1. Find the smallest constant $C$ such that the following inequality holds for all $a, b, c > 1$:
$$
\sqrt{a-1} + \sqrt{b-1} + \sqrt{c-1} \leq 3C \sqrt{c(ab+1)}
$$

## Query

Task description: Please solve the problem with clear, rigorous, and logically sound steps. At the end of your response, state your answer in exactly this format: 'The answer is $C=X$', where X is your calculated numerical bound value. Example: 'The answer is $C=1$'.

Problem: Let $a, b, c$ be positive real numbers greater than 1. Find the smallest constant $C$ such that the following inequality holds for all $a, b, c > 1$:
$$
\sqrt{a-1} + \sqrt{b-1} + \sqrt{c-1} \leq 3C \sqrt{c(ab+1)}
$$

Please use some of the following theorems to solve the problem:
Theorem 1 (Category: Inequality Between Means, Nicknames: mean inequalities): Let $a_{1}, a_{2}, \ldots, a_{n}$ be positive real numbers. The numbers
$$
\begin{aligned}
& Q M=\sqrt{\frac{a_{1}^{2}+a_{2}^{2}+\cdots+a_{n}^{2}}{n}}, \quad A M=\frac{a_{1}+a_{2}+\cdots+a_{n}}{n} \\
& G M=\sqrt[n]{a_{1} a_{2} \cdots a_{n}} \quad \text { and } \quad H M=\frac{n}{\frac{1}{a_{1}}+\frac{1}{a_{2}}+\cdots+\frac{1}{a_{n}}}
\end{aligned}
$$
are called the quadratic, arithmetic, geometric and harmonic mean for the numbers $a_{1}, a_{2}, \ldots, a_{n}$, respectively, and we have
$$
Q M \geq A M \geq G M \geq H M
$$

Equalities occur if and only if $a_{1}=a_{2}=\cdots=a_{n}$.

Theorem 2 (Category: Cauchy-Schwarz Inequality, Nicknames: cauchy-schwarz inequality): Let $a_{1}, a_{2}, \ldots, a_{n}$ and $b_{1}, b_{2}$, $\ldots, b_{n}$ be real numbers. Then we have
$$
\left(\sum_{i=1}^{n} a_{i}^{2}\right)\left(\sum_{i=1}^{n} b_{i}^{2}\right) \geq\left(\sum_{i=1}^{n} a_{i} b_{i}\right)^{2}
$$
i.e.
$$
\left(a_{1}^{2}+a_{2}^{2}+\cdots+a_{n}^{2}\right)\left(b_{1}^{2}+b_{2}^{2}+\cdots+b_{n}^{2}\right) \geq\left(a_{1} b_{1}+a_{2} b_{2}+\cdots+a_{n} b_{n}\right)^{2}
$$

Equality occurs if and only if the sequences $\left(a_{1}, a_{2}, \ldots, a_{n}\right)$ and $\left(b_{1}, b_{2}\right.$, $\ldots, b_{n}$ ) are proportional, i.e. $\frac{a_{1}}{b_{1}}=\frac{a_{2}}{b_{2}}=\cdots=\frac{a_{n}}{b_{n}}$.

Theorem 3 (Category: Inequality Between Means, Nicknames: am-gm (arithmetic mean-geometric mean) inequality, am-gm): If $a_{1}, a_{2}, \ldots, a_{n}$ are nonnegative real numbers, then

$$
\frac{1}{n} \sum_{i=1}^{n} a_{i} \geq\left(a_{1} a_{2} \ldots a_{n}\right)^{\frac{1}{n}}
$$

with equality if and only if $a_{1}=a_{2}=\ldots=a_{n}$. This inequality is a special case of the Power Mean Inequality.

Solution:

## Response

To solve the inequality 

\[
\sqrt{a-1} + \sqrt{b-1} + \sqrt{c-1} \leq 3C \sqrt{c(ab+1)}
\]

for positive real numbers \(a, b, c > 1\), we will analyze both sides of the inequality and find the smallest constant \(C\) that satisfies it for all \(a, b, c\).

### Step 1: Analyze the left-hand side

We start with the left-hand side:

\[
\sqrt{a-1} + \sqrt{b-1} + \sqrt{c-1}
\]

Using the substitution \(x = \sqrt{a-1}\), \(y = \sqrt{b-1}\), and \(z = \sqrt{c-1}\), we can express \(a\), \(b\), and \(c\) in terms of \(x\), \(y\), and \(z\):

\[
a = x^2 + 1, \quad b = y^2 + 1, \quad c = z^2 + 1
\]

Thus, we can rewrite the left-hand side as:

\[
x + y + z
\]

### Step 2: Analyze the right-hand side

Now, we analyze the right-hand side:

\[
3C \sqrt{c(ab+1)} = 3C \sqrt{(z^2 + 1)((x^2 + 1)(y^2 + 1) + 1)}
\]

Calculating \(ab + 1\):

\[
ab = (x^2 + 1)(y^2 + 1) = x^2y^2 + x^2 + y^2 + 1
\]

Thus,

\[
ab + 1 = x^2y^2 + x^2 + y^2 + 2
\]

Now, substituting this into the right-hand side gives:

\[
3C \sqrt{(z^2 + 1)(x^2y^2 + x^2 + y^2 + 2)}
\]

### Step 3: Use Cauchy-Schwarz Inequality

To find a suitable bound for \(C\), we can apply the Cauchy-Schwarz inequality:

\[
(x + y + z)^2 \leq 3(x^2 + y^2 + z^2)
\]

This implies:

\[
x + y + z \leq \sqrt{3} \sqrt{x^2 + y^2 + z^2}
\]

### Step 4: Find a suitable \(C\)

We need to find \(C\) such that:

\[
\sqrt{3} \sqrt{x^2 + y^2 + z^2} \leq 3C \sqrt{(z^2 + 1)(x^2y^2 + x^2 + y^2 + 2)}
\]

To simplify our analysis, we can consider the case when \(a = b = c\). Let \(a = b = c = t\) where \(t > 1\):

\[
3\sqrt{t-1} \leq 3C \sqrt{t(t^2 + 1)}
\]

Dividing both sides by 3 gives:

\[
\sqrt{t-1} \leq C \sqrt{t(t^2 + 1)}
\]

Squaring both sides results in:

\[
t - 1 \leq C^2 t(t^2 + 1)
\]

Rearranging gives:

\[
C^2 t^3 + C^2 t - t + 1 \geq 0
\]

### Step 5: Find the minimum \(C\)

To find the minimum \(C\), we can analyze the behavior of the function as \(t\) approaches 1. As \(t \to 1\):

\[
C^2(1^3 + 1) - 1 + 1 \geq 0 \implies 2C^2 \geq 0
\]

This is always true. Now, we can test specific values of \(t\) to find the smallest \(C\). 

Testing \(t = 2\):

\[
C^2(2^3 + 2) - 2 + 1 \geq 0 \implies 10C^2 - 1 \geq 0 \implies C^2 \geq \frac{1}{10} \implies C \geq \frac{1}{\sqrt{10}}
\]

Testing \(t = 3\):

\[
C^2(3^3 + 3) - 3 + 1 \geq 0 \implies 30C^2 - 2 \geq 0 \implies C^2 \geq \frac{1}{15} \implies C \geq \frac{1}{\sqrt{15}}
\]

The minimum value occurs at \(C = \frac{1}{\sqrt{10}}\).

### Conclusion

Thus, the smallest constant \(C\) such that the inequality holds for all \(a, b, c > 1\) is:

\[
\boxed{C = \frac{1}{\sqrt{10}}}
\]

In the required format:

The answer is \(C=\frac{1}{\sqrt{10}}\).