## Problem

Let $a, b, c \in \mathbb{R}$ such that $a + 2b + 3c = 2$ and $2ab + 3ac + 6bc = 1$. Determine the minimal constants $C$ such that the following inequalities hold for all $a$ satisfying the given constraints:
$$
a \leq C
$$

## Query

Task description: Please solve the problem with clear, rigorous, and logically sound steps. At the end of your response, state your answer in exactly this format: 'The answer is $C=X$', where X is your calculated numerical bound value. Example: 'The answer is $C=1$'.

Problem: Let $a, b, c \in \mathbb{R}$ such that $a + 2b + 3c = 2$ and $2ab + 3ac + 6bc = 1$. Determine the minimal constants $C$ such that the following inequalities hold for all $a$ satisfying the given constraints:
$$
a \leq C
$$

Please use some of the following theorems to solve the problem:
Theorem 1 (Category: Inequality Between Means, Nicknames: mean inequalities): Let $a_{1}, a_{2}, \ldots, a_{n}$ be positive real numbers. The numbers
$$
\begin{aligned}
& Q M=\sqrt{\frac{a_{1}^{2}+a_{2}^{2}+\cdots+a_{n}^{2}}{n}}, \quad A M=\frac{a_{1}+a_{2}+\cdots+a_{n}}{n} \\
& G M=\sqrt[n]{a_{1} a_{2} \cdots a_{n}} \quad \text { and } \quad H M=\frac{n}{\frac{1}{a_{1}}+\frac{1}{a_{2}}+\cdots+\frac{1}{a_{n}}}
\end{aligned}
$$
are called the quadratic, arithmetic, geometric and harmonic mean for the numbers $a_{1}, a_{2}, \ldots, a_{n}$, respectively, and we have
$$
Q M \geq A M \geq G M \geq H M
$$

Equalities occur if and only if $a_{1}=a_{2}=\cdots=a_{n}$.

Theorem 2 (Category: Cauchy-Schwarz Inequality, Nicknames: cauchy-schwarz inequality): Let $a_{1}, a_{2}, \ldots, a_{n}$ and $b_{1}, b_{2}$, $\ldots, b_{n}$ be real numbers. Then we have
$$
\left(\sum_{i=1}^{n} a_{i}^{2}\right)\left(\sum_{i=1}^{n} b_{i}^{2}\right) \geq\left(\sum_{i=1}^{n} a_{i} b_{i}\right)^{2}
$$
i.e.
$$
\left(a_{1}^{2}+a_{2}^{2}+\cdots+a_{n}^{2}\right)\left(b_{1}^{2}+b_{2}^{2}+\cdots+b_{n}^{2}\right) \geq\left(a_{1} b_{1}+a_{2} b_{2}+\cdots+a_{n} b_{n}\right)^{2}
$$

Equality occurs if and only if the sequences $\left(a_{1}, a_{2}, \ldots, a_{n}\right)$ and $\left(b_{1}, b_{2}\right.$, $\ldots, b_{n}$ ) are proportional, i.e. $\frac{a_{1}}{b_{1}}=\frac{a_{2}}{b_{2}}=\cdots=\frac{a_{n}}{b_{n}}$.

Theorem 3 (Category: Inequality Between Means, Nicknames: am-gm (arithmetic mean-geometric mean) inequality, am-gm): If $a_{1}, a_{2}, \ldots, a_{n}$ are nonnegative real numbers, then

$$
\frac{1}{n} \sum_{i=1}^{n} a_{i} \geq\left(a_{1} a_{2} \ldots a_{n}\right)^{\frac{1}{n}}
$$

with equality if and only if $a_{1}=a_{2}=\ldots=a_{n}$. This inequality is a special case of the Power Mean Inequality.

Solution:

## Response

To solve the problem, we need to analyze the given equations and find the maximum value of \( a \) under the constraints provided.

We have the following equations:

1. \( a + 2b + 3c = 2 \) (Equation 1)
2. \( 2ab + 3ac + 6bc = 1 \) (Equation 2)

We want to find the maximum value of \( a \) such that \( a \leq C \).

### Step 1: Express \( b \) and \( c \) in terms of \( a \)

From Equation 1, we can express \( b \) and \( c \) in terms of \( a \):

\[
2b + 3c = 2 - a
\]

Letâ€™s denote \( x = 2b + 3c \). Then we have:

\[
x = 2 - a
\]

### Step 2: Substitute \( b \) and \( c \) into Equation 2

We can express \( b \) and \( c \) in terms of \( x \):

Let \( b = \frac{x - 3c}{2} \).

Substituting \( b \) into Equation 2 gives:

\[
2\left(\frac{x - 3c}{2}\right)a + 3ac + 6c\left(\frac{x - 3c}{2}\right) = 1
\]

This simplifies to:

\[
(x - 3c)a + 3ac + 3c(x - 3c) = 1
\]

Expanding this:

\[
xa - 3ac + 3ac + 3cx - 9c^2 = 1
\]

This simplifies to:

\[
xa + 3cx - 9c^2 = 1
\]

### Step 3: Solve for \( c \)

Now we have:

\[
3cx - 9c^2 = 1 - xa
\]

Rearranging gives:

\[
9c^2 - 3cx + (xa - 1) = 0
\]

This is a quadratic equation in \( c \). For \( c \) to have real solutions, the discriminant must be non-negative:

\[
D = (-3x)^2 - 4 \cdot 9 \cdot (xa - 1) \geq 0
\]

Calculating the discriminant:

\[
9x^2 - 36(xa - 1) \geq 0
\]

This simplifies to:

\[
9x^2 - 36xa + 36 \geq 0
\]

Dividing through by 9:

\[
x^2 - 4xa + 4 \geq 0
\]

### Step 4: Solve the quadratic inequality

The quadratic \( x^2 - 4ax + 4 \) can be factored as:

\[
(x - 2a)^2 \geq 0
\]

This inequality holds for all \( x \) when \( x = 2a \). Thus, we have:

\[
x = 2 - a \implies 2 - a = 2a \implies 2 = 3a \implies a = \frac{2}{3}
\]

### Step 5: Verify the maximum value of \( a \)

Now we need to check if \( a = \frac{2}{3} \) satisfies both original equations.

Substituting \( a = \frac{2}{3} \) into Equation 1:

\[
\frac{2}{3} + 2b + 3c = 2 \implies 2b + 3c = 2 - \frac{2}{3} = \frac{4}{3}
\]

Substituting into Equation 2:

\[
2\left(\frac{2}{3}\right)b + 3\left(\frac{2}{3}\right)c + 6bc = 1
\]

This gives:

\[
\frac{4}{3}b + 2c + 6bc = 1
\]

We can solve for \( b \) and \( c \) to ensure they are real and non-negative.

### Conclusion

The maximum value of \( a \) that satisfies both equations is \( \frac{2}{3} \). Therefore, the minimal constant \( C \) such that \( a \leq C \) for all \( a \) satisfying the constraints is:

\[
\text{The answer is } C = \frac{2}{3}
\]