## Problem

Let $0 \leq x \leq 1$ and $n \in \mathbb{N}$. Find the smallest constant $C$ such that the following inequality holds for all $x$ and $n$:
$$
\left(1-x+\frac{x^2}{2}\right)^n-(1-x)^n \leq Cx.
$$

## Query

Task description: Please solve the problem with clear, rigorous, and logically sound steps. At the end of your response, state your answer in exactly this format: 'The answer is $C=X$', where X is your calculated numerical bound value. Example: 'The answer is $C=1$'.

Problem: Let $0 \leq x \leq 1$ and $n \in \mathbb{N}$. Find the smallest constant $C$ such that the following inequality holds for all $x$ and $n$:
$$
\left(1-x+\frac{x^2}{2}\right)^n-(1-x)^n \leq Cx.
$$

Please use some of the following theorems to solve the problem:
Theorem 1 (Category: Inequality Between Means, Nicknames: mean inequalities): Let $a_{1}, a_{2}, \ldots, a_{n}$ be positive real numbers. The numbers
$$
\begin{aligned}
& Q M=\sqrt{\frac{a_{1}^{2}+a_{2}^{2}+\cdots+a_{n}^{2}}{n}}, \quad A M=\frac{a_{1}+a_{2}+\cdots+a_{n}}{n} \\
& G M=\sqrt[n]{a_{1} a_{2} \cdots a_{n}} \quad \text { and } \quad H M=\frac{n}{\frac{1}{a_{1}}+\frac{1}{a_{2}}+\cdots+\frac{1}{a_{n}}}
\end{aligned}
$$
are called the quadratic, arithmetic, geometric and harmonic mean for the numbers $a_{1}, a_{2}, \ldots, a_{n}$, respectively, and we have
$$
Q M \geq A M \geq G M \geq H M
$$

Equalities occur if and only if $a_{1}=a_{2}=\cdots=a_{n}$.

Theorem 2 (Category: Cauchy-Schwarz Inequality, Nicknames: cauchy-schwarz inequality): Let $a_{1}, a_{2}, \ldots, a_{n}$ and $b_{1}, b_{2}$, $\ldots, b_{n}$ be real numbers. Then we have
$$
\left(\sum_{i=1}^{n} a_{i}^{2}\right)\left(\sum_{i=1}^{n} b_{i}^{2}\right) \geq\left(\sum_{i=1}^{n} a_{i} b_{i}\right)^{2}
$$
i.e.
$$
\left(a_{1}^{2}+a_{2}^{2}+\cdots+a_{n}^{2}\right)\left(b_{1}^{2}+b_{2}^{2}+\cdots+b_{n}^{2}\right) \geq\left(a_{1} b_{1}+a_{2} b_{2}+\cdots+a_{n} b_{n}\right)^{2}
$$

Equality occurs if and only if the sequences $\left(a_{1}, a_{2}, \ldots, a_{n}\right)$ and $\left(b_{1}, b_{2}\right.$, $\ldots, b_{n}$ ) are proportional, i.e. $\frac{a_{1}}{b_{1}}=\frac{a_{2}}{b_{2}}=\cdots=\frac{a_{n}}{b_{n}}$.

Theorem 3 (Category: Inequality Between Means, Nicknames: am-gm (arithmetic mean-geometric mean) inequality, am-gm): If $a_{1}, a_{2}, \ldots, a_{n}$ are nonnegative real numbers, then

$$
\frac{1}{n} \sum_{i=1}^{n} a_{i} \geq\left(a_{1} a_{2} \ldots a_{n}\right)^{\frac{1}{n}}
$$

with equality if and only if $a_{1}=a_{2}=\ldots=a_{n}$. This inequality is a special case of the Power Mean Inequality.

Solution:

## Response

To solve the problem, we need to analyze the expression 

\[
\left(1 - x + \frac{x^2}{2}\right)^n - (1 - x)^n
\]

and find the smallest constant \( C \) such that 

\[
\left(1 - x + \frac{x^2}{2}\right)^n - (1 - x)^n \leq Cx
\]

for all \( x \) in the interval \( [0, 1] \) and for all \( n \in \mathbb{N} \).

### Step 1: Simplifying the Expression

Let \( a = 1 - x \). Then, we can rewrite the expression as:

\[
\left(a + \frac{(1-a)^2}{2}\right)^n - a^n
\]

This simplifies to:

\[
\left(a + \frac{(1 - 2a + a^2)}{2}\right)^n - a^n = \left(a + \frac{1 - 2a + a^2}{2}\right)^n - a^n
\]

### Step 2: Analyzing the Difference

We can denote:

\[
f(x) = \left(1 - x + \frac{x^2}{2}\right)^n - (1 - x)^n
\]

We will analyze \( f(x) \) as \( x \) approaches 0 and 1.

### Step 3: Taylor Expansion

To understand the behavior of \( f(x) \) near \( x = 0 \), we can use Taylor expansion. 

1. **At \( x = 0 \)**:
   \[
   f(0) = \left(1 - 0 + 0\right)^n - (1 - 0)^n = 1 - 1 = 0
   \]

2. **At \( x = 1 \)**:
   \[
   f(1) = \left(1 - 1 + \frac{1^2}{2}\right)^n - (1 - 1)^n = \left(0 + \frac{1}{2}\right)^n - 0 = \left(\frac{1}{2}\right)^n
   \]

### Step 4: Derivative Analysis

To find the maximum of \( f(x) \) in \( (0, 1) \), we can compute the derivative \( f'(x) \):

\[
f'(x) = n\left(1 - x + \frac{x^2}{2}\right)^{n-1}\left(-1 + x\right) - n(1 - x)^{n-1}(-1)
\]

Setting \( f'(x) = 0 \) will help us find critical points. However, this can be complex, so we will evaluate \( f(x) \) at specific points.

### Step 5: Evaluating at Specific Points

1. **At \( x = 0 \)**: \( f(0) = 0 \)
2. **At \( x = 1 \)**: \( f(1) = \left(\frac{1}{2}\right)^n \)

### Step 6: Finding the Constant \( C \)

To find \( C \), we need to ensure that:

\[
\left(1 - x + \frac{x^2}{2}\right)^n - (1 - x)^n \leq Cx
\]

For small \( x \), we can approximate:

\[
\left(1 - x + \frac{x^2}{2}\right)^n \approx 1 - nx + O(x^2)
\]
\[
(1 - x)^n \approx 1 - nx + O(x^2)
\]

Thus, the leading term in the difference is \( O(x^2) \). Therefore, we can conclude that:

\[
f(x) \approx O(x^2)
\]

This suggests that \( C \) must be at least 1 to satisfy the inequality for small \( x \).

### Conclusion

After evaluating the behavior of \( f(x) \) and considering the maximum value at \( x = 1 \), we find that the smallest constant \( C \) that satisfies the inequality for all \( x \) in \( [0, 1] \) is:

\[
C = 1
\]

Thus, the final answer is:

\[
\text{The answer is } C=1
\]