## Problem

Let $a_1, a_2, \ldots, a_n$ be non-negative real numbers such that $\prod a_1 = \lambda^n$. Determine the minimal constant $C$ such that the following inequality holds for all $a_1, a_2, \ldots, a_n$:

$$
\prod_{c y c}\left(a_1^2-a_1+1\right) \geq \sqrt{\left(\frac{1+\lambda^4}{C}\right)^n}.
$$

## Query

Task description: Please solve the problem with clear, rigorous, and logically sound steps. At the end of your response, state your answer in exactly this format: 'The answer is $C=X$', where X is your calculated numerical bound value. Example: 'The answer is $C=1$'.

Problem: Let $a_1, a_2, \ldots, a_n$ be non-negative real numbers such that $\prod a_1 = \lambda^n$. Determine the minimal constant $C$ such that the following inequality holds for all $a_1, a_2, \ldots, a_n$:

$$
\prod_{c y c}\left(a_1^2-a_1+1\right) \geq \sqrt{\left(\frac{1+\lambda^4}{C}\right)^n}.
$$

Please use some of the following theorems to solve the problem:
Theorem 1 (Category: Inequality Between Means, Nicknames: mean inequalities): Let $a_{1}, a_{2}, \ldots, a_{n}$ be positive real numbers. The numbers
$$
\begin{aligned}
& Q M=\sqrt{\frac{a_{1}^{2}+a_{2}^{2}+\cdots+a_{n}^{2}}{n}}, \quad A M=\frac{a_{1}+a_{2}+\cdots+a_{n}}{n} \\
& G M=\sqrt[n]{a_{1} a_{2} \cdots a_{n}} \quad \text { and } \quad H M=\frac{n}{\frac{1}{a_{1}}+\frac{1}{a_{2}}+\cdots+\frac{1}{a_{n}}}
\end{aligned}
$$
are called the quadratic, arithmetic, geometric and harmonic mean for the numbers $a_{1}, a_{2}, \ldots, a_{n}$, respectively, and we have
$$
Q M \geq A M \geq G M \geq H M
$$

Equalities occur if and only if $a_{1}=a_{2}=\cdots=a_{n}$.

Theorem 2 (Category: Cauchy-Schwarz Inequality, Nicknames: cauchy-schwarz inequality): Let $a_{1}, a_{2}, \ldots, a_{n}$ and $b_{1}, b_{2}$, $\ldots, b_{n}$ be real numbers. Then we have
$$
\left(\sum_{i=1}^{n} a_{i}^{2}\right)\left(\sum_{i=1}^{n} b_{i}^{2}\right) \geq\left(\sum_{i=1}^{n} a_{i} b_{i}\right)^{2}
$$
i.e.
$$
\left(a_{1}^{2}+a_{2}^{2}+\cdots+a_{n}^{2}\right)\left(b_{1}^{2}+b_{2}^{2}+\cdots+b_{n}^{2}\right) \geq\left(a_{1} b_{1}+a_{2} b_{2}+\cdots+a_{n} b_{n}\right)^{2}
$$

Equality occurs if and only if the sequences $\left(a_{1}, a_{2}, \ldots, a_{n}\right)$ and $\left(b_{1}, b_{2}\right.$, $\ldots, b_{n}$ ) are proportional, i.e. $\frac{a_{1}}{b_{1}}=\frac{a_{2}}{b_{2}}=\cdots=\frac{a_{n}}{b_{n}}$.

Theorem 3 (Category: Inequality Between Means, Nicknames: am-gm (arithmetic mean-geometric mean) inequality, am-gm): If $a_{1}, a_{2}, \ldots, a_{n}$ are nonnegative real numbers, then

$$
\frac{1}{n} \sum_{i=1}^{n} a_{i} \geq\left(a_{1} a_{2} \ldots a_{n}\right)^{\frac{1}{n}}
$$

with equality if and only if $a_{1}=a_{2}=\ldots=a_{n}$. This inequality is a special case of the Power Mean Inequality.

Solution:

## Response

To solve the problem, we need to analyze the inequality given:

$$
\prod_{i=1}^{n}\left(a_i^2 - a_i + 1\right) \geq \sqrt{\left(\frac{1+\lambda^4}{C}\right)^n}.
$$

We start by rewriting the left-hand side. The expression \( a_i^2 - a_i + 1 \) can be rewritten as:

$$
a_i^2 - a_i + 1 = \left(a_i - \frac{1}{2}\right)^2 + \frac{3}{4}.
$$

This shows that \( a_i^2 - a_i + 1 \) is always positive for all \( a_i \) and achieves its minimum value of \( \frac{3}{4} \) when \( a_i = \frac{1}{2} \).

Next, we apply the AM-GM inequality to the terms \( a_i^2 - a_i + 1 \):

$$
\prod_{i=1}^{n} (a_i^2 - a_i + 1) \geq \left( \frac{1}{n} \sum_{i=1}^{n} (a_i^2 - a_i + 1) \right)^n.
$$

Now, we need to compute \( \sum_{i=1}^{n} (a_i^2 - a_i + 1) \):

$$
\sum_{i=1}^{n} (a_i^2 - a_i + 1) = \sum_{i=1}^{n} a_i^2 - \sum_{i=1}^{n} a_i + n.
$$

Using the Cauchy-Schwarz inequality, we have:

$$
\left( \sum_{i=1}^{n} a_i \right)^2 \leq n \sum_{i=1}^{n} a_i^2.
$$

Let \( S = \sum_{i=1}^{n} a_i \) and \( P = \prod_{i=1}^{n} a_i \). By the AM-GM inequality, we know:

$$
\frac{S}{n} \geq \sqrt[n]{P} \implies S^2 \geq nP.
$$

Given that \( P = \lambda^n \), we have:

$$
S^2 \geq n \lambda^n.
$$

Now, we can express \( \sum_{i=1}^{n} a_i^2 \) in terms of \( S \):

$$
\sum_{i=1}^{n} a_i^2 \geq \frac{S^2}{n} \geq \lambda^n.
$$

Thus, we can write:

$$
\sum_{i=1}^{n} (a_i^2 - a_i + 1) \geq \lambda^n - S + n.
$$

To find a suitable \( C \), we need to ensure that:

$$
\prod_{i=1}^{n} (a_i^2 - a_i + 1) \geq \sqrt{\left(\frac{1+\lambda^4}{C}\right)^n}.
$$

We can set \( C \) such that:

$$
\left( \frac{1}{n} \sum_{i=1}^{n} (a_i^2 - a_i + 1) \right) \geq \frac{1+\lambda^4}{C}.
$$

To minimize \( C \), we can consider the case when all \( a_i \) are equal, say \( a_i = \lambda \). In this case:

$$
\prod_{i=1}^{n} (a_i^2 - a_i + 1) = n \left( \lambda^2 - \lambda + 1 \right).
$$

We need to find \( C \) such that:

$$
n \left( \lambda^2 - \lambda + 1 \right) \geq \sqrt{\left(\frac{1+\lambda^4}{C}\right)^n}.
$$

Taking the \( n \)-th root on both sides gives:

$$
\lambda^2 - \lambda + 1 \geq \sqrt{\frac{1+\lambda^4}{C}}.
$$

Squaring both sides leads to:

$$
(\lambda^2 - \lambda + 1)^2 \geq \frac{1+\lambda^4}{C}.
$$

Rearranging gives:

$$
C \geq \frac{1+\lambda^4}{(\lambda^2 - \lambda + 1)^2}.
$$

To find the minimum value of \( C \), we can evaluate this expression for specific values of \( \lambda \). For \( \lambda = 1 \):

$$
C \geq \frac{1 + 1^4}{(1^2 - 1 + 1)^2} = \frac{2}{1} = 2.
$$

Thus, the minimal constant \( C \) that satisfies the inequality for all non-negative \( a_i \) is:

The answer is \( C=2 \).