## Problem

Let $a, b, c > 0$ be positive real numbers such that $a + b + c = 1$. Consider the following inequality:
$$
\frac{1+a+b}{2+c} + \frac{1+b+c}{2+a} + \frac{1+c+a}{2+b} \quad () \quad 2.
$$

Determine the correct inequality relation to fill in the blank.

Options:

(A) $\leq$ 

(B) $\geq$

(C) $=$ 

(D) $<$

(E) $>$

(F) None of the above

## Query

Task description: Please solve the problem with clear, rigorous, and logically sound steps. At the end of your response, state your answer in exactly this format: 'The answer is (Letter) Symbol', where Letter is one of the given options. Example: 'The answer is (A) $\leq$'.

Problem: Let $a, b, c > 0$ be positive real numbers such that $a + b + c = 1$. Consider the following inequality:
$$
\frac{1+a+b}{2+c} + \frac{1+b+c}{2+a} + \frac{1+c+a}{2+b} \quad () \quad 2.
$$

Determine the correct inequality relation to fill in the blank.

Options:

(A) $\leq$ 

(B) $\geq$

(C) $=$ 

(D) $<$

(E) $>$

(F) None of the above

Please use some of the following theorems to solve the problem:
Theorem 1 (Category: Inequality Between Means, Nicknames: mean inequalities): Let $a_{1}, a_{2}, \ldots, a_{n}$ be positive real numbers. The numbers
$$
\begin{aligned}
& Q M=\sqrt{\frac{a_{1}^{2}+a_{2}^{2}+\cdots+a_{n}^{2}}{n}}, \quad A M=\frac{a_{1}+a_{2}+\cdots+a_{n}}{n} \\
& G M=\sqrt[n]{a_{1} a_{2} \cdots a_{n}} \quad \text { and } \quad H M=\frac{n}{\frac{1}{a_{1}}+\frac{1}{a_{2}}+\cdots+\frac{1}{a_{n}}}
\end{aligned}
$$
are called the quadratic, arithmetic, geometric and harmonic mean for the numbers $a_{1}, a_{2}, \ldots, a_{n}$, respectively, and we have
$$
Q M \geq A M \geq G M \geq H M
$$

Equalities occur if and only if $a_{1}=a_{2}=\cdots=a_{n}$.

Theorem 2 (Category: Cauchy-Schwarz Inequality, Nicknames: cauchy-schwarz inequality): Let $a_{1}, a_{2}, \ldots, a_{n}$ and $b_{1}, b_{2}$, $\ldots, b_{n}$ be real numbers. Then we have
$$
\left(\sum_{i=1}^{n} a_{i}^{2}\right)\left(\sum_{i=1}^{n} b_{i}^{2}\right) \geq\left(\sum_{i=1}^{n} a_{i} b_{i}\right)^{2}
$$
i.e.
$$
\left(a_{1}^{2}+a_{2}^{2}+\cdots+a_{n}^{2}\right)\left(b_{1}^{2}+b_{2}^{2}+\cdots+b_{n}^{2}\right) \geq\left(a_{1} b_{1}+a_{2} b_{2}+\cdots+a_{n} b_{n}\right)^{2}
$$

Equality occurs if and only if the sequences $\left(a_{1}, a_{2}, \ldots, a_{n}\right)$ and $\left(b_{1}, b_{2}\right.$, $\ldots, b_{n}$ ) are proportional, i.e. $\frac{a_{1}}{b_{1}}=\frac{a_{2}}{b_{2}}=\cdots=\frac{a_{n}}{b_{n}}$.

Theorem 3 (Category: Inequality Between Means, Nicknames: am-gm (arithmetic mean-geometric mean) inequality, am-gm): If $a_{1}, a_{2}, \ldots, a_{n}$ are nonnegative real numbers, then

$$
\frac{1}{n} \sum_{i=1}^{n} a_{i} \geq\left(a_{1} a_{2} \ldots a_{n}\right)^{\frac{1}{n}}
$$

with equality if and only if $a_{1}=a_{2}=\ldots=a_{n}$. This inequality is a special case of the Power Mean Inequality.

Solution:

## Response

To solve the inequality 

\[
\frac{1+a+b}{2+c} + \frac{1+b+c}{2+a} + \frac{1+c+a}{2+b} \quad () \quad 2,
\]

given that \( a, b, c > 0 \) and \( a + b + c = 1 \), we will analyze the left-hand side of the inequality.

First, we can rewrite each term in the sum:

1. The first term is 

\[
\frac{1 + a + b}{2 + c} = \frac{1 + (a + b)}{2 + c} = \frac{1 + (1 - c)}{2 + c} = \frac{2 - c}{2 + c}.
\]

2. The second term is 

\[
\frac{1 + b + c}{2 + a} = \frac{1 + (b + c)}{2 + a} = \frac{1 + (1 - a)}{2 + a} = \frac{2 - a}{2 + a}.
\]

3. The third term is 

\[
\frac{1 + c + a}{2 + b} = \frac{1 + (c + a)}{2 + b} = \frac{1 + (1 - b)}{2 + b} = \frac{2 - b}{2 + b}.
\]

Thus, we can rewrite the entire expression as:

\[
\frac{2 - c}{2 + c} + \frac{2 - a}{2 + a} + \frac{2 - b}{2 + b}.
\]

Next, we will analyze the sum:

\[
S = \frac{2 - a}{2 + a} + \frac{2 - b}{2 + b} + \frac{2 - c}{2 + c}.
\]

To simplify our analysis, we can use the Cauchy-Schwarz inequality. We apply it to the sums:

\[
\left( \sum_{cyc} (2 - a) \right) \left( \sum_{cyc} \frac{1}{2 + a} \right) \geq \left( \sum_{cyc} 1 \right)^2 = 3^2 = 9.
\]

Calculating the left-hand side:

\[
\sum_{cyc} (2 - a) = 6 - (a + b + c) = 6 - 1 = 5.
\]

Thus, we have:

\[
5 \left( \sum_{cyc} \frac{1}{2 + a} \right) \geq 9 \implies \sum_{cyc} \frac{1}{2 + a} \geq \frac{9}{5}.
\]

Now, we can analyze \( S \):

\[
S = \sum_{cyc} \frac{2 - a}{2 + a} = 3 - \sum_{cyc} \frac{a}{2 + a}.
\]

Next, we need to find \( \sum_{cyc} \frac{a}{2 + a} \). Using the fact that \( a + b + c = 1 \), we can estimate:

\[
\sum_{cyc} \frac{a}{2 + a} \leq \sum_{cyc} \frac{a}{2} = \frac{1}{2} \sum_{cyc} a = \frac{1}{2}.
\]

Thus, we have:

\[
S \geq 3 - \frac{1}{2} = \frac{5}{2}.
\]

Since \( \frac{5}{2} > 2 \), we conclude that:

\[
S > 2.
\]

Therefore, the correct inequality relation to fill in the blank is:

\[
\frac{1+a+b}{2+c} + \frac{1+b+c}{2+a} + \frac{1+c+a}{2+b} > 2.
\]

Thus, the answer is:

The answer is (E) $>$.