## Problem

Let $a, b, c, d > 0$ such that $a \leq b \leq c \leq d$ and $abcd = 1$. Determine the minimal constant $C$ such that the following inequality holds for all $a, b, c, d$:

$$(a + 1)(d + 1)-\frac {3}{4d^3} \geq 2C.$$

## Query

Task description: Please solve the problem with clear, rigorous, and logically sound steps. At the end of your response, state your answer in exactly this format: 'The answer is $C=X$', where X is your calculated numerical bound value. Example: 'The answer is $C=1$'.

Problem: Let $a, b, c, d > 0$ such that $a \leq b \leq c \leq d$ and $abcd = 1$. Determine the minimal constant $C$ such that the following inequality holds for all $a, b, c, d$:

$$(a + 1)(d + 1)-\frac {3}{4d^3} \geq 2C.$$

Solution:

## Response

To solve this problem, we need to find the minimal constant \( C \) such that the inequality

\[
(a + 1)(d + 1) - \frac{3}{4d^3} \geq 2C
\]

holds for all positive \( a, b, c, d \) satisfying \( a \leq b \leq c \leq d \) and \( abcd = 1 \).

### Step 1: Simplify the Problem

Given \( abcd = 1 \), we can express \( a \) in terms of \( b, c, \) and \( d \):

\[
a = \frac{1}{bcd}.
\]

Substituting \( a = \frac{1}{bcd} \) into the inequality, we have:

\[
\left(\frac{1}{bcd} + 1\right)(d + 1) - \frac{3}{4d^3} \geq 2C.
\]

Simplifying the left-hand side:

\[
\left(\frac{1}{bcd} + 1\right)(d + 1) = \frac{d + 1}{bcd} + d + 1.
\]

Thus, the inequality becomes:

\[
\frac{d + 1}{bcd} + d + 1 - \frac{3}{4d^3} \geq 2C.
\]

### Step 2: Analyze the Expression

To find the minimal \( C \), consider the case where \( a = b = c = d = 1 \). This satisfies \( abcd = 1 \) and \( a \leq b \leq c \leq d \).

Substitute \( a = b = c = d = 1 \) into the inequality:

\[
(a + 1)(d + 1) - \frac{3}{4d^3} = (1 + 1)(1 + 1) - \frac{3}{4 \cdot 1^3} = 2 \cdot 2 - \frac{3}{4} = 4 - \frac{3}{4} = \frac{16}{4} - \frac{3}{4} = \frac{13}{4}.
\]

Thus, the inequality becomes:

\[
\frac{13}{4} \geq 2C.
\]

Solving for \( C \):

\[
2C \leq \frac{13}{4} \implies C \leq \frac{13}{8}.
\]

### Step 3: Verify the Bound

To ensure that \( C = \frac{13}{8} \) is indeed the minimal constant, consider the behavior of the inequality as \( d \to \infty \). In this case, \( a = \frac{1}{bcd} \to 0 \), and the expression simplifies to:

\[
(a + 1)(d + 1) \approx d + 1.
\]

The term \(-\frac{3}{4d^3}\) becomes negligible, and the inequality becomes:

\[
d + 1 \geq 2C.
\]

As \( d \to \infty \), this inequality holds for any finite \( C \). Therefore, the critical case is when \( a = b = c = d = 1 \), which we have already checked.

Thus, the minimal constant \( C \) such that the inequality holds for all \( a, b, c, d \) is:

\[
\boxed{\frac{13}{8}}
\]

The answer is \(\boxed{C = \frac{13}{8}}\).