## Problem

Let $a, b, c$ be positive real numbers. Find the largest positive constant $C$ such that the inequality below holds for all $a, b, c \in \mathbb{R}^{+}$:
$$
\frac{a}{(b+c)^2}+\frac{b}{(c+a)^2}+\frac{c}{(a+b)^2} \geq \frac{C}{a+b+c}
$$

## Query

Task description: Please solve the problem with clear, rigorous, and logically sound steps. At the end of your response, state your answer in exactly this format: 'The answer is $C=X$', where X is your calculated numerical bound value. Example: 'The answer is $C=1$'.

Problem: Let $a, b, c$ be positive real numbers. Find the largest positive constant $C$ such that the inequality below holds for all $a, b, c \in \mathbb{R}^{+}$:
$$
\frac{a}{(b+c)^2}+\frac{b}{(c+a)^2}+\frac{c}{(a+b)^2} \geq \frac{C}{a+b+c}
$$

Solution:

## Response

To solve this problem, we need to find the largest constant \( C \) such that the inequality

\[
\frac{a}{(b+c)^2} + \frac{b}{(c+a)^2} + \frac{c}{(a+b)^2} \geq \frac{C}{a+b+c}
\]

holds for all positive real numbers \( a, b, c \).

### Step 1: Analyze the Symmetry and Homogeneity

The inequality is symmetric in \( a, b, c \) and homogeneous of degree \(-1\). This suggests that the inequality should hold for any positive scaling of \( a, b, c \). Therefore, without loss of generality, we can assume \( a + b + c = 1 \) to simplify the problem. Under this assumption, the inequality becomes:

\[
\frac{a}{(b+c)^2} + \frac{b}{(c+a)^2} + \frac{c}{(a+b)^2} \geq C
\]

### Step 2: Test Simple Cases

Let's test the inequality for simple cases to get an idea of what \( C \) might be.

#### Case 1: \( a = b = c = \frac{1}{3} \)

In this case, \( b+c = c+a = a+b = \frac{2}{3} \). The left-hand side becomes:

\[
3 \cdot \frac{\frac{1}{3}}{\left(\frac{2}{3}\right)^2} = 3 \cdot \frac{\frac{1}{3}}{\frac{4}{9}} = 3 \cdot \frac{3}{4} = \frac{9}{4}
\]

Thus, for \( a = b = c = \frac{1}{3} \), the inequality becomes:

\[
\frac{9}{4} \geq C
\]

#### Case 2: \( a = 1, b = c = 0 \)

In this case, the left-hand side becomes:

\[
\frac{1}{0^2} + 0 + 0 = \infty
\]

This case doesn't provide a finite bound for \( C \), but it shows that the inequality holds trivially.

### Step 3: Use Known Inequalities

Consider the AM-GM inequality:

\[
b+c \leq 2\sqrt{bc}
\]

Thus,

\[
(b+c)^2 \leq 4bc
\]

This implies:

\[
\frac{a}{(b+c)^2} \geq \frac{a}{4bc}
\]

Applying this to each term, we have:

\[
\frac{a}{(b+c)^2} + \frac{b}{(c+a)^2} + \frac{c}{(a+b)^2} \geq \frac{a}{4bc} + \frac{b}{4ca} + \frac{c}{4ab}
\]

This is equivalent to:

\[
\frac{1}{4} \left( \frac{a}{bc} + \frac{b}{ca} + \frac{c}{ab} \right)
\]

By AM-GM, we know:

\[
\frac{a}{bc} + \frac{b}{ca} + \frac{c}{ab} \geq 3\sqrt[3]{\frac{a}{bc} \cdot \frac{b}{ca} \cdot \frac{c}{ab}} = 3
\]

Thus:

\[
\frac{1}{4} \left( \frac{a}{bc} + \frac{b}{ca} + \frac{c}{ab} \right) \geq \frac{3}{4}
\]

### Conclusion

From the above analysis, the largest constant \( C \) that satisfies the inequality for all positive \( a, b, c \) is \( \frac{9}{4} \). Therefore, the answer is:

\[
\text{The answer is } C = \frac{9}{4}
\]