## Problem

Let $a, b, c$ be side lengths of a triangle, and $\beta$ is the angle between $a$ and $c$. Consider the following expressions:
$$
\frac{b^2+c^2}{a^2} \quad () \quad \frac{2 \sqrt{3} c \sin \beta - a}{b+c} 
$$

Determine the correct inequality relation to fill in the blank.

Options:

(A) $\leq$ 

(B) $\geq$

(C) $=$ 

(D) $<$

(E) $>$

(F) None of the above

## Query

Task description: Please solve the problem with clear, rigorous, and logically sound steps. At the end of your response, state your answer in exactly this format: 'The answer is (Letter) Symbol', where Letter is one of the given options. Example: 'The answer is (A) $\leq$'.

Problem: Let $a, b, c$ be side lengths of a triangle, and $\beta$ is the angle between $a$ and $c$. Consider the following expressions:
$$
\frac{b^2+c^2}{a^2} \quad () \quad \frac{2 \sqrt{3} c \sin \beta - a}{b+c} 
$$

Determine the correct inequality relation to fill in the blank.

Options:

(A) $\leq$ 

(B) $\geq$

(C) $=$ 

(D) $<$

(E) $>$

(F) None of the above

Solution:

## Response

To solve this problem, we need to compare the two expressions given:

1. \(\frac{b^2 + c^2}{a^2}\)
2. \(\frac{2 \sqrt{3} c \sin \beta - a}{b+c}\)

We know that \(a\), \(b\), and \(c\) are the side lengths of a triangle, and \(\beta\) is the angle between sides \(a\) and \(c\). By the triangle inequality, we have:
- \(a + b > c\)
- \(b + c > a\)
- \(c + a > b\)

Additionally, by the law of cosines, we have:
\[ b^2 = a^2 + c^2 - 2ac \cos \beta \]

Let's analyze each expression:

### Expression 1: \(\frac{b^2 + c^2}{a^2}\)

Using the law of cosines, we can express \(b^2\) as:
\[ b^2 = a^2 + c^2 - 2ac \cos \beta \]

Thus:
\[ b^2 + c^2 = a^2 + c^2 - 2ac \cos \beta + c^2 = a^2 + 2c^2 - 2ac \cos \beta \]

So:
\[ \frac{b^2 + c^2}{a^2} = \frac{a^2 + 2c^2 - 2ac \cos \beta}{a^2} = 1 + \frac{2c^2 - 2ac \cos \beta}{a^2} \]

### Expression 2: \(\frac{2 \sqrt{3} c \sin \beta - a}{b+c}\)

This expression involves the sine of the angle \(\beta\). We know from the law of sines:
\[ \frac{a}{\sin \alpha} = \frac{b}{\sin \beta} = \frac{c}{\sin \gamma} = 2R \]
where \(R\) is the circumradius of the triangle.

### Comparison

To compare these expressions, consider the following:

1. **Expression 1** is always positive because \(b^2 + c^2 > 0\) and \(a^2 > 0\).

2. **Expression 2** can be positive, negative, or zero depending on the values of \(a\), \(b\), \(c\), and \(\beta\).

To find a specific relationship, consider a special case where the triangle is equilateral. In this case, \(a = b = c\) and \(\beta = 60^\circ\).

- For an equilateral triangle, \(\cos \beta = \frac{1}{2}\) and \(\sin \beta = \frac{\sqrt{3}}{2}\).

- **Expression 1** becomes:
  \[
  \frac{b^2 + c^2}{a^2} = \frac{2a^2}{a^2} = 2
  \]

- **Expression 2** becomes:
  \[
  \frac{2 \sqrt{3} c \sin \beta - a}{b+c} = \frac{2 \sqrt{3} \cdot a \cdot \frac{\sqrt{3}}{2} - a}{2a} = \frac{3a - a}{2a} = 1
  \]

In this special case, \(\frac{b^2 + c^2}{a^2} = 2\) and \(\frac{2 \sqrt{3} c \sin \beta - a}{b+c} = 1\).

Thus, \(\frac{b^2 + c^2}{a^2} > \frac{2 \sqrt{3} c \sin \beta - a}{b+c}\).

Therefore, the correct inequality relation is:

The answer is (E) $>$.