## Problem

Let $a_1, a_2, \ldots, a_n > 0$ such that $a_1 + a_2 + \ldots + a_n < 1$. Determine the minimal constant $C$ such that the following inequality holds for all $a_1, a_2, \ldots, a_n$:

$$
\frac{a_1 \cdot a_2 \ldots a_n \left(1 - a_1 - a_2 - \ldots - a_n\right)}{\left(a_1 + a_2 + \ldots + a_n\right)\left(1-a_1\right)\left(1-a_2\right) \ldots \left(1-a_n\right)} \leq C\frac{3}{n^{n-1}}.
$$

## Query

Task description: Please solve the problem with clear, rigorous, and logically sound steps. At the end of your response, state your answer in exactly this format: 'The answer is $C=X$', where X is your calculated numerical bound value. Example: 'The answer is $C=1$'.

Problem: Let $a_1, a_2, \ldots, a_n > 0$ such that $a_1 + a_2 + \ldots + a_n < 1$. Determine the minimal constant $C$ such that the following inequality holds for all $a_1, a_2, \ldots, a_n$:

$$
\frac{a_1 \cdot a_2 \ldots a_n \left(1 - a_1 - a_2 - \ldots - a_n\right)}{\left(a_1 + a_2 + \ldots + a_n\right)\left(1-a_1\right)\left(1-a_2\right) \ldots \left(1-a_n\right)} \leq C\frac{3}{n^{n-1}}.
$$

Solution:

## Response

To solve this problem, we need to find the minimal constant \( C \) such that the given inequality holds for all positive \( a_1, a_2, \ldots, a_n \) with the condition \( a_1 + a_2 + \ldots + a_n < 1 \).

The inequality is:

\[
\frac{a_1 \cdot a_2 \ldots a_n \left(1 - a_1 - a_2 - \ldots - a_n\right)}{\left(a_1 + a_2 + \ldots + a_n\right)\left(1-a_1\right)\left(1-a_2\right) \ldots \left(1-a_n\right)} \leq C\frac{3}{n^{n-1}}.
\]

### Step 1: Simplify the Problem

First, consider the expression:

\[
E = \frac{a_1 \cdot a_2 \ldots a_n \left(1 - a_1 - a_2 - \ldots - a_n\right)}{\left(a_1 + a_2 + \ldots + a_n\right)\left(1-a_1\right)\left(1-a_2\right) \ldots \left(1-a_n\right)}.
\]

We need to find the maximum value of \( E \) under the constraint \( a_1 + a_2 + \ldots + a_n < 1 \).

### Step 2: Analyze the Expression

The numerator \( a_1 \cdot a_2 \ldots a_n \left(1 - a_1 - a_2 - \ldots - a_n\right) \) is maximized when each \( a_i \) is equal, due to the AM-GM inequality. Let \( a_1 = a_2 = \ldots = a_n = x \). Then:

\[
nx < 1 \implies x < \frac{1}{n}.
\]

The expression becomes:

\[
E = \frac{x^n \left(1 - nx\right)}{nx(1-x)^n}.
\]

### Step 3: Simplify Further

Substitute \( x = \frac{1}{n} \) to check the behavior:

\[
E = \frac{\left(\frac{1}{n}\right)^n \left(1 - 1\right)}{\frac{1}{n} \left(1 - \frac{1}{n}\right)^n} = 0.
\]

This suggests that the maximum does not occur at \( x = \frac{1}{n} \). Instead, consider the derivative of the function to find critical points.

### Step 4: Use AM-GM Inequality

By AM-GM, the product \( a_1 a_2 \ldots a_n \) is maximized when all \( a_i \) are equal, but since \( a_1 + a_2 + \ldots + a_n < 1 \), the maximum occurs when \( a_i \to 0 \) for all but one \( a_i \).

### Step 5: Evaluate the Bound

If \( a_1 = 1 - \epsilon \) and \( a_2 = a_3 = \ldots = a_n = \frac{\epsilon}{n-1} \), then:

\[
E \approx \frac{\left(\frac{\epsilon}{n-1}\right)^{n-1} (1 - \epsilon)}{\epsilon (1 - (1-\epsilon))(1 - \frac{\epsilon}{n-1})^{n-1}}.
\]

Simplifying, as \( \epsilon \to 0 \), the expression approaches:

\[
E \approx \frac{1}{n^{n-1}}.
\]

### Conclusion

The maximum value of \( E \) is \( \frac{1}{n^{n-1}} \), and thus the minimal constant \( C \) such that the inequality holds is:

\[
C = 1.
\]

Therefore, the answer is \(\boxed{C=1}\).