## Problem

Let $x, y, z$ be vectors in $\mathbb{R}^n$. Consider the following expressions:
$$
|x+y+z| + |x| + |2y| + |2z|  \quad () \quad |x+y| + |y+z| + |z+x|.
$$

Determine the correct inequality relation to fill in the blank.

Options:

(A) $\leq$ 

(B) $\geq$

(C) $=$ 

(D) $<$

(E) $>$

(F) None of the above

## Query

Task description: Please solve the problem with clear, rigorous, and logically sound steps. At the end of your response, state your answer in exactly this format: 'The answer is (Letter) Symbol', where Letter is one of the given options. Example: 'The answer is (A) $\leq$'.

Problem: Let $x, y, z$ be vectors in $\mathbb{R}^n$. Consider the following expressions:
$$
|x+y+z| + |x| + |2y| + |2z|  \quad () \quad |x+y| + |y+z| + |z+x|.
$$

Determine the correct inequality relation to fill in the blank.

Options:

(A) $\leq$ 

(B) $\geq$

(C) $=$ 

(D) $<$

(E) $>$

(F) None of the above

Solution:

## Response

To solve this problem, we need to compare the two expressions:

1. \( |x+y+z| + |x| + |2y| + |2z| \)
2. \( |x+y| + |y+z| + |z+x| \)

We will use the triangle inequality, which states that for any vectors \( a \) and \( b \) in \(\mathbb{R}^n\), \( |a + b| \leq |a| + |b| \).

Let's analyze each part of the expressions:

### Expression 1: \( |x+y+z| + |x| + |2y| + |2z| \)

- \( |x+y+z| \) is the norm of the vector sum of \( x, y, \) and \( z \).
- \( |x| \) is the norm of vector \( x \).
- \( |2y| = 2|y| \) is twice the norm of vector \( y \).
- \( |2z| = 2|z| \) is twice the norm of vector \( z \).

### Expression 2: \( |x+y| + |y+z| + |z+x| \)

- \( |x+y| \) is the norm of the vector sum of \( x \) and \( y \).
- \( |y+z| \) is the norm of the vector sum of \( y \) and \( z \).
- \( |z+x| \) is the norm of the vector sum of \( z \) and \( x \).

### Applying the Triangle Inequality

1. **For \( |x+y+z| \):**
   \[
   |x+y+z| \leq |x+y| + |z|
   \]
   \[
   |x+y+z| \leq |x+z| + |y|
   \]
   \[
   |x+y+z| \leq |y+z| + |x|
   \]

2. **For \( |x+y| + |y+z| + |z+x| \):**
   By the triangle inequality, each term is less than or equal to the sum of the norms of its components:
   \[
   |x+y| \leq |x| + |y|
   \]
   \[
   |y+z| \leq |y| + |z|
   \]
   \[
   |z+x| \leq |z| + |x|
   \]

   Adding these inequalities gives:
   \[
   |x+y| + |y+z| + |z+x| \leq 2(|x| + |y| + |z|)
   \]

### Comparing the Two Expressions

Now, let's compare the two expressions:

- **Expression 1:** \( |x+y+z| + |x| + 2|y| + 2|z| \)
- **Expression 2:** \( |x+y| + |y+z| + |z+x| \)

From the triangle inequality, we have:
\[
|x+y+z| \leq |x+y| + |z|
\]
\[
|x+y+z| \leq |y+z| + |x|
\]
\[
|x+y+z| \leq |z+x| + |y|
\]

Thus, \( |x+y+z| \) is less than or equal to any of the sums of two terms from Expression 2. Therefore, Expression 1 is generally less than or equal to Expression 2, but not necessarily equal.

Therefore, the correct inequality relation is:

The answer is (A) \(\leq\).