## Problem

Let $a, b, c, x, y, z \in \mathbb{R}$ be real numbers such that $a + b + c = 1$ and $x^2 + y^2 + z^2 = 1$. Consider the following expression:
$$
a(x+b) + b(y+c) + c(z+a)  \quad () \quad 1.
$$

Determine the correct inequality relation to fill in the blank.

Options:

(A) $\leq$ 

(B) $\geq$

(C) $=$ 

(D) $<$

(E) $>$

(F) None of the above

## Query

Task description: Please solve the problem with clear, rigorous, and logically sound steps. At the end of your response, state your answer in exactly this format: 'The answer is (Letter) Symbol', where Letter is one of the given options. Example: 'The answer is (A) $\leq$'.

Problem: Let $a, b, c, x, y, z \in \mathbb{R}$ be real numbers such that $a + b + c = 1$ and $x^2 + y^2 + z^2 = 1$. Consider the following expression:
$$
a(x+b) + b(y+c) + c(z+a)  \quad () \quad 1.
$$

Determine the correct inequality relation to fill in the blank.

Options:

(A) $\leq$ 

(B) $\geq$

(C) $=$ 

(D) $<$

(E) $>$

(F) None of the above

Solution:

## Response

To solve this problem, we need to analyze the expression:

\[
a(x+b) + b(y+c) + c(z+a)
\]

Given the conditions \(a + b + c = 1\) and \(x^2 + y^2 + z^2 = 1\), we want to determine the relationship between this expression and the number 1.

First, let's expand the expression:

\[
a(x+b) + b(y+c) + c(z+a) = ax + ab + by + bc + cz + ca
\]

Rearranging terms, we have:

\[
ax + by + cz + ab + bc + ca
\]

Now, consider the expression \(ax + by + cz\). By the Cauchy-Schwarz inequality, we have:

\[
(ax + by + cz)^2 \leq (a^2 + b^2 + c^2)(x^2 + y^2 + z^2)
\]

Since \(x^2 + y^2 + z^2 = 1\), this simplifies to:

\[
(ax + by + cz)^2 \leq a^2 + b^2 + c^2
\]

Next, we use the identity:

\[
a^2 + b^2 + c^2 = (a + b + c)^2 - 2(ab + bc + ca) = 1 - 2(ab + bc + ca)
\]

Thus, we have:

\[
(ax + by + cz)^2 \leq 1 - 2(ab + bc + ca)
\]

Taking the square root on both sides, we get:

\[
|ax + by + cz| \leq \sqrt{1 - 2(ab + bc + ca)}
\]

Now, consider the full expression:

\[
ax + by + cz + ab + bc + ca
\]

We want to compare this to 1. Notice that:

\[
ab + bc + ca \leq \frac{(a+b+c)^2}{3} = \frac{1}{3}
\]

Thus, the maximum value of \(ab + bc + ca\) is \(\frac{1}{3}\).

Now, let's consider the maximum possible value of \(ax + by + cz\). Since:

\[
|ax + by + cz| \leq \sqrt{1 - 2(ab + bc + ca)}
\]

The maximum value of \(\sqrt{1 - 2(ab + bc + ca)}\) occurs when \(ab + bc + ca\) is minimized. The minimum value of \(ab + bc + ca\) is 0 (when two of \(a, b, c\) are 0 and the other is 1), giving:

\[
|ax + by + cz| \leq 1
\]

Therefore, the maximum value of \(ax + by + cz + ab + bc + ca\) is:

\[
1 + \frac{1}{3} = \frac{4}{3}
\]

However, this is not necessarily achievable due to the constraints on \(a, b, c\) and \(x, y, z\). The expression can be equal to 1 when \(ax + by + cz = 1\) and \(ab + bc + ca = 0\), which is possible when one of \(a, b, c\) is 1 and the others are 0, and similarly for \(x, y, z\).

Thus, the expression can be equal to 1, but it cannot exceed 1. Therefore, the correct inequality is:

\[
a(x+b) + b(y+c) + c(z+a) \leq 1
\]

The answer is (A) \(\leq\).