## Problem

Let $a, b, c > 0$ such that $a+b+c=1$. Determine the maximal constant $C$ such that the following inequality holds for all $a, b, c$:

$$
\frac{a^2+a b}{1-a^2}+\frac{b^2+b c}{1-b^2}+\frac{c^2+c a}{1-c^2} \geq C.
$$

## Query

Task description: Please solve the problem with clear, rigorous, and logically sound steps. At the end of your response, state your answer in exactly this format: 'The answer is $C=X$', where X is your calculated numerical bound value. Example: 'The answer is $C=1$'.

Problem: Let $a, b, c > 0$ such that $a+b+c=1$. Determine the maximal constant $C$ such that the following inequality holds for all $a, b, c$:

$$
\frac{a^2+a b}{1-a^2}+\frac{b^2+b c}{1-b^2}+\frac{c^2+c a}{1-c^2} \geq C.
$$

Solution:

## Response

To solve this problem, we need to find the maximal constant \( C \) such that the inequality

\[
\frac{a^2 + ab}{1-a^2} + \frac{b^2 + bc}{1-b^2} + \frac{c^2 + ca}{1-c^2} \geq C
\]

holds for all positive \( a, b, c \) with \( a + b + c = 1 \).

### Step 1: Simplify the Expression

First, consider the expression for each term:

\[
\frac{a^2 + ab}{1-a^2} = \frac{a^2 + ab}{(1-a)(1+a)} = \frac{a^2 + ab}{1-a^2}
\]

Similarly, for the other terms:

\[
\frac{b^2 + bc}{1-b^2} = \frac{b^2 + bc}{(1-b)(1+b)}
\]

\[
\frac{c^2 + ca}{1-c^2} = \frac{c^2 + ca}{(1-c)(1+c)}
\]

### Step 2: Consider Symmetric Case

To find a lower bound, consider the symmetric case where \( a = b = c = \frac{1}{3} \). Then:

\[
\frac{a^2 + ab}{1-a^2} = \frac{\left(\frac{1}{3}\right)^2 + \frac{1}{3} \cdot \frac{1}{3}}{1-\left(\frac{1}{3}\right)^2} = \frac{\frac{1}{9} + \frac{1}{9}}{\frac{8}{9}} = \frac{2}{8} = \frac{1}{4}
\]

Similarly, for the other terms:

\[
\frac{b^2 + bc}{1-b^2} = \frac{1}{4}, \quad \frac{c^2 + ca}{1-c^2} = \frac{1}{4}
\]

Thus, the sum is:

\[
\frac{1}{4} + \frac{1}{4} + \frac{1}{4} = \frac{3}{4}
\]

### Step 3: Check for Other Configurations

To ensure that \( C = \frac{3}{4} \) is indeed the maximal constant, consider the case where one variable approaches 1 and the others approach 0. For instance, let \( a \to 1 \) and \( b, c \to 0 \). Then:

\[
\frac{a^2 + ab}{1-a^2} \to \frac{1^2 + 0}{1-1^2} \to \infty
\]

The other terms:

\[
\frac{b^2 + bc}{1-b^2} \to 0, \quad \frac{c^2 + ca}{1-c^2} \to 0
\]

Thus, the expression can become arbitrarily large, confirming that \( C = \frac{3}{4} \) is indeed the maximal constant that satisfies the inequality for all \( a, b, c > 0 \) with \( a + b + c = 1 \).

Therefore, the answer is \(\boxed{C = \frac{3}{4}}\).