## Problem

Let $x, y, z > 0$ be positive real numbers such that $x + y + z = xyz$. Consider the following inequality:
$$
(x-1)(y-1)(z-1) \quad () \quad 6\sqrt{3} - 8.
$$

Determine the correct inequality relation to fill in the blank.

Options:

(A) $\leq$ 

(B) $\geq$

(C) $=$ 

(D) $<$

(E) $>$

(F) None of the above

## Query

Task description: Please solve the problem with clear, rigorous, and logically sound steps. At the end of your response, state your answer in exactly this format: 'The answer is (Letter) Symbol', where Letter is one of the given options. Example: 'The answer is (A) $\leq$'.

Problem: Let $x, y, z > 0$ be positive real numbers such that $x + y + z = xyz$. Consider the following inequality:
$$
(x-1)(y-1)(z-1) \quad () \quad 6\sqrt{3} - 8.
$$

Determine the correct inequality relation to fill in the blank.

Options:

(A) $\leq$ 

(B) $\geq$

(C) $=$ 

(D) $<$

(E) $>$

(F) None of the above

Solution:

## Response

To solve this problem, we need to analyze the inequality \((x-1)(y-1)(z-1) \quad () \quad 6\sqrt{3} - 8\) given the condition \(x + y + z = xyz\) with \(x, y, z > 0\).

First, let's explore the condition \(x + y + z = xyz\). This condition is reminiscent of the identity for the sides of a triangle with angles of \(60^\circ\), which suggests that \(x = \cot A\), \(y = \cot B\), and \(z = \cot C\) for a triangle with angles \(A, B, C\) summing to \(180^\circ\). In particular, if \(A = B = C = 60^\circ\), then \(x = y = z = \sqrt{3}\).

Let's verify this:
- If \(x = y = z = \sqrt{3}\), then \(x + y + z = 3\sqrt{3}\).
- Also, \(xyz = (\sqrt{3})^3 = 3\sqrt{3}\).

Thus, \(x + y + z = xyz\) holds true for \(x = y = z = \sqrt{3}\).

Now, calculate \((x-1)(y-1)(z-1)\) for \(x = y = z = \sqrt{3}\):
\[
(x-1)(y-1)(z-1) = (\sqrt{3} - 1)^3.
\]

Calculate \((\sqrt{3} - 1)^3\):
\[
(\sqrt{3} - 1)^3 = (\sqrt{3} - 1)(\sqrt{3} - 1)(\sqrt{3} - 1).
\]

First, find \((\sqrt{3} - 1)^2\):
\[
(\sqrt{3} - 1)^2 = (\sqrt{3})^2 - 2\sqrt{3} \cdot 1 + 1^2 = 3 - 2\sqrt{3} + 1 = 4 - 2\sqrt{3}.
\]

Now, multiply by \((\sqrt{3} - 1)\):
\[
(\sqrt{3} - 1)^3 = (4 - 2\sqrt{3})(\sqrt{3} - 1).
\]

Expand this product:
\[
= 4\sqrt{3} - 4 - 2\sqrt{3} \cdot \sqrt{3} + 2\sqrt{3}.
\]

Simplify:
\[
= 4\sqrt{3} - 4 - 6 + 2\sqrt{3} = 6\sqrt{3} - 10.
\]

Now, compare \(6\sqrt{3} - 10\) with \(6\sqrt{3} - 8\):
\[
6\sqrt{3} - 10 < 6\sqrt{3} - 8.
\]

Thus, \((x-1)(y-1)(z-1) < 6\sqrt{3} - 8\) when \(x = y = z = \sqrt{3}\).

Since the condition \(x + y + z = xyz\) is symmetric and holds for \(x = y = z = \sqrt{3}\), and the inequality is strict, the correct relation is:
\[
(x-1)(y-1)(z-1) < 6\sqrt{3} - 8.
\]

Therefore, the answer is \((D) <\). 

The answer is (D) $<$.