## Problem

Let $x_1, x_2, \ldots, x_n > 0\;(n\geq 2)$ be positive real numbers such that
$$
\frac{1}{1+x_1}+\frac{1}{1+x_2}+\ldots+\frac{1}{1+x_n}=1.
$$
Consider the following inequality:
$$
x_1 x_2 \ldots x_n \quad () \quad (n-1)^{n-1}.
$$

Determine the correct inequality relation to fill in the blank.

Options:

(A) $\leq$ 

(B) $\geq$

(C) $=$ 

(D) $<$

(E) $>$

(F) None of the above

## Query

Task description: Please solve the problem with clear, rigorous, and logically sound steps. At the end of your response, state your answer in exactly this format: 'The answer is (Letter) Symbol', where Letter is one of the given options. Example: 'The answer is (A) $\leq$'.

Problem: Let $x_1, x_2, \ldots, x_n > 0\;(n\geq 2)$ be positive real numbers such that
$$
\frac{1}{1+x_1}+\frac{1}{1+x_2}+\ldots+\frac{1}{1+x_n}=1.
$$
Consider the following inequality:
$$
x_1 x_2 \ldots x_n \quad () \quad (n-1)^{n-1}.
$$

Determine the correct inequality relation to fill in the blank.

Options:

(A) $\leq$ 

(B) $\geq$

(C) $=$ 

(D) $<$

(E) $>$

(F) None of the above

Solution:

## Response

To solve this problem, we need to analyze the given condition and determine the relationship between the product \( x_1 x_2 \ldots x_n \) and \( (n-1)^{n-1} \).

We are given that:

\[
\frac{1}{1+x_1} + \frac{1}{1+x_2} + \ldots + \frac{1}{1+x_n} = 1.
\]

Let's rewrite each term:

\[
\frac{1}{1+x_i} = 1 - \frac{x_i}{1+x_i}.
\]

Thus, the condition becomes:

\[
n - \left( \frac{x_1}{1+x_1} + \frac{x_2}{1+x_2} + \ldots + \frac{x_n}{1+x_n} \right) = 1.
\]

This simplifies to:

\[
\frac{x_1}{1+x_1} + \frac{x_2}{1+x_2} + \ldots + \frac{x_n}{1+x_n} = n - 1.
\]

Now, consider the function \( f(x) = \frac{x}{1+x} \). This function is increasing for \( x > 0 \) because its derivative \( f'(x) = \frac{1}{(1+x)^2} > 0 \).

By the AM-GM inequality, we have:

\[
\frac{x_1}{1+x_1} + \frac{x_2}{1+x_2} + \ldots + \frac{x_n}{1+x_n} \geq n \sqrt[n]{\frac{x_1 x_2 \ldots x_n}{(1+x_1)(1+x_2)\ldots(1+x_n)}}.
\]

Given that:

\[
\frac{x_1}{1+x_1} + \frac{x_2}{1+x_2} + \ldots + \frac{x_n}{1+x_n} = n - 1,
\]

we have:

\[
n - 1 \geq n \sqrt[n]{\frac{x_1 x_2 \ldots x_n}{(1+x_1)(1+x_2)\ldots(1+x_n)}}.
\]

This implies:

\[
\frac{n-1}{n} \geq \sqrt[n]{\frac{x_1 x_2 \ldots x_n}{(1+x_1)(1+x_2)\ldots(1+x_n)}}.
\]

Raising both sides to the power of \( n \), we get:

\[
\left(\frac{n-1}{n}\right)^n \geq \frac{x_1 x_2 \ldots x_n}{(1+x_1)(1+x_2)\ldots(1+x_n)}.
\]

Thus:

\[
x_1 x_2 \ldots x_n \leq \left(\frac{n-1}{n}\right)^n (1+x_1)(1+x_2)\ldots(1+x_n).
\]

Now, consider the case when all \( x_i \) are equal. Let \( x_1 = x_2 = \ldots = x_n = x \). Then:

\[
\frac{n}{1+x} = 1 \implies 1+x = n \implies x = n-1.
\]

In this case, \( x_1 x_2 \ldots x_n = (n-1)^n \).

Thus, the inequality becomes:

\[
(n-1)^n \leq \left(\frac{n-1}{n}\right)^n n^n = (n-1)^n.
\]

This shows that the inequality holds with equality when all \( x_i = n-1 \).

Therefore, the correct inequality relation is:

\[
x_1 x_2 \ldots x_n \leq (n-1)^{n-1}.
\]

The answer is (A) \(\leq\).