## Problem

Let $x, y, z \geq -\frac{3}{4}$ be real numbers such that $x + y + z = 1$. Consider the following inequality:
$$
\frac{x}{2x^2+1} + \frac{y}{y^2+3} + \frac{z}{z^2+1} \quad () \quad 1.
$$

Determine the correct inequality relation to fill in the blank.

Options:

(A) $\leq$ 

(B) $\geq$

(C) $=$ 

(D) $<$

(E) $>$

(F) None of the above

## Query

Task description: Please solve the problem with clear, rigorous, and logically sound steps. At the end of your response, state your answer in exactly this format: 'The answer is (Letter) Symbol', where Letter is one of the given options. Example: 'The answer is (A) $\leq$'.

Problem: Let $x, y, z \geq -\frac{3}{4}$ be real numbers such that $x + y + z = 1$. Consider the following inequality:
$$
\frac{x}{2x^2+1} + \frac{y}{y^2+3} + \frac{z}{z^2+1} \quad () \quad 1.
$$

Determine the correct inequality relation to fill in the blank.

Options:

(A) $\leq$ 

(B) $\geq$

(C) $=$ 

(D) $<$

(E) $>$

(F) None of the above

Solution:

## Response

To solve this problem, we need to analyze the given inequality:

\[
\frac{x}{2x^2+1} + \frac{y}{y^2+3} + \frac{z}{z^2+1} \quad () \quad 1
\]

where \(x, y, z \geq -\frac{3}{4}\) and \(x + y + z = 1\).

### Step 1: Analyze each term

1. **Term \(\frac{x}{2x^2+1}\):**

   For \(x \geq -\frac{3}{4}\), we need to check the behavior of the function \(f(x) = \frac{x}{2x^2+1}\).

   - At \(x = 0\), \(f(0) = 0\).
   - As \(x \to \infty\), \(f(x) \to 0\).
   - As \(x \to -\frac{3}{4}\), \(f(x) = \frac{-\frac{3}{4}}{2\left(-\frac{3}{4}\right)^2 + 1} = \frac{-\frac{3}{4}}{\frac{9}{8} + 1} = \frac{-\frac{3}{4}}{\frac{17}{8}} = -\frac{3}{17}\).

   The function \(f(x)\) is continuous and differentiable, and it is bounded between \(-\frac{3}{17}\) and some positive value less than 1.

2. **Term \(\frac{y}{y^2+3}\):**

   For \(y \geq -\frac{3}{4}\), consider \(g(y) = \frac{y}{y^2+3}\).

   - At \(y = 0\), \(g(0) = 0\).
   - As \(y \to \infty\), \(g(y) \to 0\).
   - As \(y \to -\frac{3}{4}\), \(g(y) = \frac{-\frac{3}{4}}{\left(-\frac{3}{4}\right)^2 + 3} = \frac{-\frac{3}{4}}{\frac{9}{16} + 3} = \frac{-\frac{3}{4}}{\frac{57}{16}} = -\frac{12}{57} = -\frac{4}{19}\).

   The function \(g(y)\) is also continuous and differentiable, and it is bounded between \(-\frac{4}{19}\) and some positive value less than 1.

3. **Term \(\frac{z}{z^2+1}\):**

   For \(z \geq -\frac{3}{4}\), consider \(h(z) = \frac{z}{z^2+1}\).

   - At \(z = 0\), \(h(0) = 0\).
   - As \(z \to \infty\), \(h(z) \to 0\).
   - As \(z \to -\frac{3}{4}\), \(h(z) = \frac{-\frac{3}{4}}{\left(-\frac{3}{4}\right)^2 + 1} = \frac{-\frac{3}{4}}{\frac{9}{16} + 1} = \frac{-\frac{3}{4}}{\frac{25}{16}} = -\frac{12}{25}\).

   The function \(h(z)\) is continuous and differentiable, and it is bounded between \(-\frac{12}{25}\) and some positive value less than 1.

### Step 2: Combine the terms

We need to evaluate:

\[
\frac{x}{2x^2+1} + \frac{y}{y^2+3} + \frac{z}{z^2+1}
\]

Given that \(x + y + z = 1\), we want to determine if this sum is less than, greater than, or equal to 1.

### Step 3: Consider special cases

1. **Case \(x = y = z = \frac{1}{3}\):**

   - \(\frac{x}{2x^2+1} = \frac{\frac{1}{3}}{2\left(\frac{1}{3}\right)^2 + 1} = \frac{\frac{1}{3}}{\frac{2}{9} + 1} = \frac{\frac{1}{3}}{\frac{11}{9}} = \frac{3}{11}\).
   - \(\frac{y}{y^2+3} = \frac{\frac{1}{3}}{\left(\frac{1}{3}\right)^2 + 3} = \frac{\frac{1}{3}}{\frac{1}{9} + 3} = \frac{\frac{1}{3}}{\frac{28}{9}} = \frac{3}{28}\).
   - \(\frac{z}{z^2+1} = \frac{\frac{1}{3}}{\left(\frac{1}{3}\right)^2 + 1} = \frac{\frac{1}{3}}{\frac{1}{9} + 1} = \frac{\frac{1}{3}}{\frac{10}{9}} = \frac{3}{10}\).

   Sum: \(\frac{3}{11} + \frac{3}{28} + \frac{3}{10}\).

   - Common denominator: 3080.
   - \(\frac{3}{11} = \frac{840}{3080}\).
   - \(\frac{3}{28} = \frac{330}{3080}\).
   - \(\frac{3}{10} = \frac{924}{3080}\).

   Total: \(\frac{840 + 330 + 924}{3080} = \frac{2094}{3080} \approx 0.68\).

This sum is less than 1.

### Conclusion

The inequality is:

\[
\frac{x}{2x^2+1} + \frac{y}{y^2+3} + \frac{z}{z^2+1} < 1
\]

Thus, the correct option is:

The answer is (D) $<$.