## Problem

Suppose $a, b, x, y$ are all real numbers and $x^2 + y^2 = 1$. Consider the following inequality:
$$
\sqrt{a^2 x^2 + b^2 y^2} + \sqrt{a^2 y^2 + b^2 x^2} \quad () \quad a + b .
$$

Determine the correct inequality relation to fill in the blank.

Options:

(A) $\leq$ 

(B) $\geq$

(C) $=$ 

(D) $<$

(E) $>$

(F) None of the above

## Query

Task description: Please solve the problem with clear, rigorous, and logically sound steps. At the end of your response, state your answer in exactly this format: 'The answer is (Letter) Symbol', where Letter is one of the given options. Example: 'The answer is (A) $\leq$'.

Problem: Suppose $a, b, x, y$ are all real numbers and $x^2 + y^2 = 1$. Consider the following inequality:
$$
\sqrt{a^2 x^2 + b^2 y^2} + \sqrt{a^2 y^2 + b^2 x^2} \quad () \quad a + b .
$$

Determine the correct inequality relation to fill in the blank.

Options:

(A) $\leq$ 

(B) $\geq$

(C) $=$ 

(D) $<$

(E) $>$

(F) None of the above

Solution:

## Response

To solve this problem, we need to analyze the given inequality:

\[
\sqrt{a^2 x^2 + b^2 y^2} + \sqrt{a^2 y^2 + b^2 x^2} \quad () \quad a + b
\]

where \(x^2 + y^2 = 1\).

### Step 1: Simplify the Expression

First, observe that \(x^2 + y^2 = 1\) implies that \((x, y)\) lies on the unit circle. We can parameterize \(x\) and \(y\) as \(x = \cos \theta\) and \(y = \sin \theta\) for some angle \(\theta\).

Substitute these into the expression:

\[
\sqrt{a^2 \cos^2 \theta + b^2 \sin^2 \theta} + \sqrt{a^2 \sin^2 \theta + b^2 \cos^2 \theta}
\]

### Step 2: Use Trigonometric Identities

Using the identity \(\cos^2 \theta + \sin^2 \theta = 1\), we can rewrite the terms inside the square roots:

1. \(a^2 \cos^2 \theta + b^2 \sin^2 \theta = (a^2 - b^2) \cos^2 \theta + b^2\)
2. \(a^2 \sin^2 \theta + b^2 \cos^2 \theta = (a^2 - b^2) \sin^2 \theta + b^2\)

### Step 3: Analyze the Expression

The expression becomes:

\[
\sqrt{(a^2 - b^2) \cos^2 \theta + b^2} + \sqrt{(a^2 - b^2) \sin^2 \theta + b^2}
\]

### Step 4: Consider Special Cases

1. **Case \(a = b\):**

   If \(a = b\), then the expression simplifies to:

   \[
   \sqrt{a^2} + \sqrt{a^2} = a + a = 2a
   \]

   Since \(a + b = 2a\), the expression equals \(a + b\).

2. **Case \(a \neq b\):**

   Without loss of generality, assume \(a > b\). Then:

   \[
   \sqrt{(a^2 - b^2) \cos^2 \theta + b^2} \leq \sqrt{a^2}
   \]
   \[
   \sqrt{(a^2 - b^2) \sin^2 \theta + b^2} \leq \sqrt{a^2}
   \]

   Adding these inequalities gives:

   \[
   \sqrt{(a^2 - b^2) \cos^2 \theta + b^2} + \sqrt{(a^2 - b^2) \sin^2 \theta + b^2} \leq 2a
   \]

   Since \(a + b \leq 2a\), the expression is generally less than or equal to \(a + b\).

### Step 5: Conclusion

The expression \(\sqrt{a^2 x^2 + b^2 y^2} + \sqrt{a^2 y^2 + b^2 x^2}\) is always less than or equal to \(a + b\), and it equals \(a + b\) when \(a = b\).

Thus, the correct inequality relation is:

\[
\sqrt{a^2 x^2 + b^2 y^2} + \sqrt{a^2 y^2 + b^2 x^2} \leq a + b
\]

The answer is \((A) \leq\).