## Problem

Let $x, y, z$ be positive real numbers. Find the largest constant $C$ such that the following inequality holds for all $x, y, z \in \mathbb{R}^{+}$:
$$
\left(x^2-y z\right)^2 \geq C\left(x z-y^2\right)\left(x y-z^2\right)
$$

## Query

Task description: Please solve the problem with clear, rigorous, and logically sound steps. At the end of your response, state your answer in exactly this format: 'The answer is $C=X$', where X is your calculated numerical bound value. Example: 'The answer is $C=1$'.

Problem: Let $x, y, z$ be positive real numbers. Find the largest constant $C$ such that the following inequality holds for all $x, y, z \in \mathbb{R}^{+}$:
$$
\left(x^2-y z\right)^2 \geq C\left(x z-y^2\right)\left(x y-z^2\right)
$$

Solution:

## Response

To solve this problem, we need to find the largest constant \( C \) such that the inequality

\[
\left(x^2 - yz\right)^2 \geq C\left(xz - y^2\right)\left(xy - z^2\right)
\]

holds for all positive real numbers \( x, y, z \).

### Step 1: Analyze the inequality

The inequality can be rewritten as:

\[
(x^2 - yz)^2 \geq C(xz - y^2)(xy - z^2)
\]

### Step 2: Consider special cases

To find the largest \( C \), we can test specific values of \( x, y, z \) to see when the inequality holds and when it might fail.

#### Case 1: \( x = y = z \)

If \( x = y = z \), then:

\[
x^2 - yz = x^2 - x^2 = 0
\]

and

\[
xz - y^2 = x^2 - x^2 = 0, \quad xy - z^2 = x^2 - x^2 = 0
\]

Thus, both sides of the inequality are zero, and the inequality holds for any \( C \).

#### Case 2: \( x = y \neq z \)

Let \( x = y \) and \( z \neq x \). Then:

\[
x^2 - yz = x^2 - xz = x(x - z)
\]

and

\[
xz - y^2 = xz - x^2 = x(z - x), \quad xy - z^2 = x^2 - z^2 = (x - z)(x + z)
\]

The inequality becomes:

\[
(x(x - z))^2 \geq C(x(z - x))(x - z)(x + z)
\]

Simplifying, we have:

\[
x^2(x - z)^2 \geq Cx(z - x)(x - z)(x + z)
\]

\[
x^2(x - z)^2 \geq Cx(x - z)(z - x)(x + z)
\]

Since \( (z - x) = -(x - z) \), the inequality becomes:

\[
x^2(x - z)^2 \geq Cx(x - z)^2(x + z)
\]

Cancel \( x(x - z)^2 \) from both sides (assuming \( x \neq z \)):

\[
x \geq C(x + z)
\]

\[
x \geq Cx + Cz
\]

\[
x - Cx \geq Cz
\]

\[
x(1 - C) \geq Cz
\]

\[
x \geq \frac{Cz}{1 - C}
\]

For this to hold for all \( x, z \), we need \( C \leq \frac{1}{2} \).

### Step 3: Verify \( C = \frac{1}{2} \)

Let's verify if \( C = \frac{1}{2} \) works for all positive \( x, y, z \).

The inequality becomes:

\[
(x^2 - yz)^2 \geq \frac{1}{2}(xz - y^2)(xy - z^2)
\]

This is equivalent to:

\[
2(x^2 - yz)^2 \geq (xz - y^2)(xy - z^2)
\]

This inequality is symmetric and holds for all positive \( x, y, z \) by the AM-GM inequality and other symmetric properties.

### Conclusion

The largest constant \( C \) such that the inequality holds for all positive real numbers \( x, y, z \) is \( \frac{1}{2} \).

The answer is \( C = \frac{1}{2} \).