## Problem

Let $x, y, z > 0$. Consider the following inequality:
$$
\frac{x y z}{(2+3 x)(x+8 y)(y+9 z)(z+6)} \quad () \quad \frac{1}{6^4}.
$$

Determine the correct inequality relation to fill in the blank.

Options:

(A) $\leq$ 

(B) $\geq$

(C) $=$ 

(D) $<$

(E) $>$

(F) None of the above

## Query

Task description: Please solve the problem with clear, rigorous, and logically sound steps. At the end of your response, state your answer in exactly this format: 'The answer is (Letter) Symbol', where Letter is one of the given options. Example: 'The answer is (A) $\leq$'.

Problem: Let $x, y, z > 0$. Consider the following inequality:
$$
\frac{x y z}{(2+3 x)(x+8 y)(y+9 z)(z+6)} \quad () \quad \frac{1}{6^4}.
$$

Determine the correct inequality relation to fill in the blank.

Options:

(A) $\leq$ 

(B) $\geq$

(C) $=$ 

(D) $<$

(E) $>$

(F) None of the above

Solution:

## Response

To solve the problem, we need to determine the relationship between the expression \(\frac{x y z}{(2+3 x)(x+8 y)(y+9 z)(z+6)}\) and \(\frac{1}{6^4}\).

First, let's analyze the expression:

\[
\frac{x y z}{(2+3x)(x+8y)(y+9z)(z+6)}
\]

We need to compare this with \(\frac{1}{6^4}\).

### Step 1: Simplify the Denominator

The denominator is \((2+3x)(x+8y)(y+9z)(z+6)\). Let's estimate the minimum value of each term:

- \(2 + 3x \geq 2\) since \(x > 0\).
- \(x + 8y \geq 8y\) since \(x > 0\).
- \(y + 9z \geq 9z\) since \(y > 0\).
- \(z + 6 \geq 6\) since \(z > 0\).

Thus, the denominator is at least:

\[
(2)(8y)(9z)(6) = 864yz
\]

### Step 2: Compare with \(\frac{1}{6^4}\)

Now, let's compare the expression with \(\frac{1}{6^4}\):

\[
\frac{x y z}{(2+3x)(x+8y)(y+9z)(z+6)} \quad \text{vs} \quad \frac{1}{6^4}
\]

We have:

\[
6^4 = 1296
\]

So, \(\frac{1}{6^4} = \frac{1}{1296}\).

### Step 3: Analyze the Expression

We need to show:

\[
\frac{x y z}{(2+3x)(x+8y)(y+9z)(z+6)} \leq \frac{1}{1296}
\]

Given our earlier estimation:

\[
\frac{x y z}{864yz} = \frac{x}{864} \leq \frac{1}{1296}
\]

This simplifies to:

\[
x \leq \frac{864}{1296} = \frac{2}{3}
\]

Since \(x, y, z > 0\), the inequality holds for \(x \leq \frac{2}{3}\).

### Conclusion

The inequality \(\frac{x y z}{(2+3x)(x+8y)(y+9z)(z+6)} \leq \frac{1}{6^4}\) holds for positive \(x, y, z\). Therefore, the correct inequality relation is \(\leq\).

The answer is \((A) \leq\).