## Problem

Let $a, b, c \in \mathbb{R}^{+}$ such that $a + b + c = 1$. Determine the minimal constant $C$ such that the following inequality holds for all $a, b, c$:

$$
\frac{a}{a+bc} + \frac{b}{b+ac} + \frac{\sqrt{abc}}{c+ab} \leq C.
$$

## Query

Task description: Please solve the problem with clear, rigorous, and logically sound steps. At the end of your response, state your answer in exactly this format: 'The answer is $C=X$', where X is your calculated numerical bound value. Example: 'The answer is $C=1$'.

Problem: Let $a, b, c \in \mathbb{R}^{+}$ such that $a + b + c = 1$. Determine the minimal constant $C$ such that the following inequality holds for all $a, b, c$:

$$
\frac{a}{a+bc} + \frac{b}{b+ac} + \frac{\sqrt{abc}}{c+ab} \leq C.
$$

Solution:

## Response

To solve this problem, we need to find the minimal constant \( C \) such that the inequality

\[
\frac{a}{a+bc} + \frac{b}{b+ac} + \frac{\sqrt{abc}}{c+ab} \leq C
\]

holds for all positive real numbers \( a, b, c \) satisfying \( a + b + c = 1 \).

### Step 1: Analyze the terms

First, consider the term \(\frac{a}{a+bc}\). Since \( a + b + c = 1 \), we have \( bc \leq \frac{(b+c)^2}{4} = \frac{(1-a)^2}{4} \). Therefore, \( a + bc \leq a + \frac{(1-a)^2}{4} \).

Similarly, for the term \(\frac{b}{b+ac}\), we have \( ac \leq \frac{(a+c)^2}{4} = \frac{(1-b)^2}{4} \), so \( b + ac \leq b + \frac{(1-b)^2}{4} \).

For the term \(\frac{\sqrt{abc}}{c+ab}\), note that \( ab \leq \frac{(a+b)^2}{4} = \frac{(1-c)^2}{4} \), so \( c + ab \leq c + \frac{(1-c)^2}{4} \).

### Step 2: Consider special cases

#### Case 1: \( a = b = c = \frac{1}{3} \)

In this case, the expression becomes:

\[
\frac{\frac{1}{3}}{\frac{1}{3} + \left(\frac{1}{3}\right)^2} + \frac{\frac{1}{3}}{\frac{1}{3} + \left(\frac{1}{3}\right)^2} + \frac{\sqrt{\left(\frac{1}{3}\right)^3}}{\frac{1}{3} + \left(\frac{1}{3}\right)^2}
\]

Each term simplifies to:

\[
\frac{\frac{1}{3}}{\frac{1}{3} + \frac{1}{9}} = \frac{\frac{1}{3}}{\frac{4}{9}} = \frac{3}{4}
\]

And the third term:

\[
\frac{\sqrt{\frac{1}{27}}}{\frac{1}{3} + \frac{1}{9}} = \frac{\frac{1}{3\sqrt{3}}}{\frac{4}{9}} = \frac{3\sqrt{3}}{12} = \frac{\sqrt{3}}{4}
\]

Adding these, we get:

\[
\frac{3}{4} + \frac{3}{4} + \frac{\sqrt{3}}{4} = \frac{6 + \sqrt{3}}{4}
\]

#### Case 2: \( a = 1, b = c = 0 \)

The expression becomes:

\[
\frac{1}{1+0} + \frac{0}{0+0} + \frac{0}{0+0} = 1
\]

### Step 3: Determine the minimal \( C \)

From the above cases, the expression achieves a maximum of 1 when \( a = 1, b = c = 0 \). Therefore, the minimal constant \( C \) such that the inequality holds for all \( a, b, c \) is:

\[
C = 1
\]

Thus, the answer is \(\boxed{1}\).

The answer is \( C = 1 \).