## Problem

Let $a, b, c \geq 0$ such that $a + b + c = 2$. Consider the following inequality:
$$
\sum \frac{bc}{2a^2+1} \quad () \quad \frac{3}{2}.
$$

Determine the correct inequality relation to fill in the blank.

Options:

(A) $\leq$ 

(B) $\geq$

(C) $=$ 

(D) $<$

(E) $>$

(F) None of the above

## Query

Task description: Please solve the problem with clear, rigorous, and logically sound steps. At the end of your response, state your answer in exactly this format: 'The answer is (Letter) Symbol', where Letter is one of the given options. Example: 'The answer is (A) $\leq$'.

Problem: Let $a, b, c \geq 0$ such that $a + b + c = 2$. Consider the following inequality:
$$
\sum \frac{bc}{2a^2+1} \quad () \quad \frac{3}{2}.
$$

Determine the correct inequality relation to fill in the blank.

Options:

(A) $\leq$ 

(B) $\geq$

(C) $=$ 

(D) $<$

(E) $>$

(F) None of the above

Solution:

## Response

To solve this problem, we need to analyze the inequality:

\[
\sum \frac{bc}{2a^2+1} \quad () \quad \frac{3}{2}
\]

where \( a, b, c \geq 0 \) and \( a + b + c = 2 \).

First, let's consider the symmetry and possible equality cases. A natural case to consider is when \( a = b = c \). If \( a = b = c \), then \( 3a = 2 \), so \( a = \frac{2}{3} \).

Substituting \( a = b = c = \frac{2}{3} \) into the left-hand side of the inequality, we have:

\[
\sum \frac{bc}{2a^2+1} = 3 \cdot \frac{\left(\frac{2}{3}\right)\left(\frac{2}{3}\right)}{2\left(\frac{2}{3}\right)^2 + 1}
\]

Calculating the denominator:

\[
2\left(\frac{2}{3}\right)^2 + 1 = 2 \cdot \frac{4}{9} + 1 = \frac{8}{9} + 1 = \frac{17}{9}
\]

Thus, each term in the sum is:

\[
\frac{\left(\frac{2}{3}\right)^2}{\frac{17}{9}} = \frac{\frac{4}{9}}{\frac{17}{9}} = \frac{4}{17}
\]

Therefore, the sum is:

\[
3 \cdot \frac{4}{17} = \frac{12}{17}
\]

Now, compare \(\frac{12}{17}\) with \(\frac{3}{2}\):

\[
\frac{12}{17} \approx 0.7059 \quad \text{and} \quad \frac{3}{2} = 1.5
\]

Clearly, \(\frac{12}{17} < \frac{3}{2}\).

To further verify, consider the extreme case where two variables are zero, say \( a = 2 \) and \( b = c = 0 \). Then:

\[
\sum \frac{bc}{2a^2+1} = \frac{0 \cdot 0}{2 \cdot 2^2 + 1} = 0
\]

This is also less than \(\frac{3}{2}\).

Thus, in all tested cases, the sum is less than \(\frac{3}{2}\). Therefore, the correct inequality relation is:

\[
\sum \frac{bc}{2a^2+1} < \frac{3}{2}
\]

The answer is (D) $<$.