## Problem

Let $a, b, c$ be positive real numbers such that $a b c = 1$. Consider the following expression:
$$
\frac{a^2 b^2}{2a^7+b^7+2a^2 b^2}+\frac{b^2 c^2}{b^7+3c^7+b^2 c^2}+\frac{c^2 a^2}{c^7+a^7+c^2 a^2} \quad () \quad 1.
$$

Determine the correct inequality relation to fill in the blank.

Options:

(A) $\leq$ 

(B) $\geq$

(C) $=$ 

(D) $<$

(E) $>$

(F) None of the above

## Query

Task description: Please solve the problem with clear, rigorous, and logically sound steps. At the end of your response, state your answer in exactly this format: 'The answer is (Letter) Symbol', where Letter is one of the given options. Example: 'The answer is (A) $\leq$'.

Problem: Let $a, b, c$ be positive real numbers such that $a b c = 1$. Consider the following expression:
$$
\frac{a^2 b^2}{2a^7+b^7+2a^2 b^2}+\frac{b^2 c^2}{b^7+3c^7+b^2 c^2}+\frac{c^2 a^2}{c^7+a^7+c^2 a^2} \quad () \quad 1.
$$

Determine the correct inequality relation to fill in the blank.

Options:

(A) $\leq$ 

(B) $\geq$

(C) $=$ 

(D) $<$

(E) $>$

(F) None of the above

Solution:

## Response

To solve this problem, we need to analyze the given expression:

\[
S = \frac{a^2 b^2}{2a^7+b^7+2a^2 b^2}+\frac{b^2 c^2}{b^7+3c^7+b^2 c^2}+\frac{c^2 a^2}{c^7+a^7+c^2 a^2}
\]

and determine its relationship to 1, given that \(abc = 1\).

### Step 1: Simplify the Expression

Since \(abc = 1\), we can use this condition to simplify the expression. Notice that each term in the expression has the form:

\[
\frac{x^2 y^2}{kx^7 + ly^7 + x^2 y^2}
\]

where \(x, y\) are cyclic permutations of \(a, b, c\) and \(k, l\) are constants. 

### Step 2: Analyze Each Term

Consider the first term:

\[
\frac{a^2 b^2}{2a^7 + b^7 + 2a^2 b^2}
\]

Since \(a, b, c\) are positive and \(abc = 1\), we can use the AM-GM inequality:

\[
2a^7 + b^7 + 2a^2 b^2 \geq 3 \sqrt[3]{2a^7 \cdot b^7 \cdot 2a^2 b^2} = 3 \sqrt[3]{4a^9 b^9} = 3 \cdot 2ab = 6ab
\]

Thus,

\[
\frac{a^2 b^2}{2a^7 + b^7 + 2a^2 b^2} \leq \frac{a^2 b^2}{6ab} = \frac{ab}{6}
\]

Similarly, for the second term:

\[
\frac{b^2 c^2}{b^7 + 3c^7 + b^2 c^2} \leq \frac{bc}{5}
\]

And for the third term:

\[
\frac{c^2 a^2}{c^7 + a^7 + c^2 a^2} \leq \frac{ca}{3}
\]

### Step 3: Sum the Inequalities

Summing these inequalities, we have:

\[
S \leq \frac{ab}{6} + \frac{bc}{5} + \frac{ca}{3}
\]

### Step 4: Use AM-GM on the Sum

Since \(abc = 1\), we can apply AM-GM inequality:

\[
\frac{ab}{6} + \frac{bc}{5} + \frac{ca}{3} \leq \frac{ab + bc + ca}{3}
\]

By AM-GM, \(ab + bc + ca \geq 3\sqrt[3]{(abc)^2} = 3\), so:

\[
\frac{ab + bc + ca}{3} \geq 1
\]

Thus, \(S \leq 1\).

### Conclusion

The expression \(S\) is less than or equal to 1. Therefore, the correct inequality relation is:

\[
\boxed{\leq}
\]

The answer is \((A) \leq\).