## Problem

Let $a, b \geq 0$ be non-negative real numbers such that $a + b = 1$. Consider the following expression:
$$
\frac{1}{a^2 - ab + 1} + \frac{1}{b^2 - ab + 1} - 4a^2b^2 \quad () \quad \frac{7}{4}.
$$

Determine the correct inequality relation to fill in the blank.

Options:

(A) $\leq$ 

(B) $\geq$

(C) $=$ 

(D) $<$

(E) $>$

(F) None of the above

## Query

Task description: Please solve the problem with clear, rigorous, and logically sound steps. At the end of your response, state your answer in exactly this format: 'The answer is (Letter) Symbol', where Letter is one of the given options. Example: 'The answer is (A) $\leq$'.

Problem: Let $a, b \geq 0$ be non-negative real numbers such that $a + b = 1$. Consider the following expression:
$$
\frac{1}{a^2 - ab + 1} + \frac{1}{b^2 - ab + 1} - 4a^2b^2 \quad () \quad \frac{7}{4}.
$$

Determine the correct inequality relation to fill in the blank.

Options:

(A) $\leq$ 

(B) $\geq$

(C) $=$ 

(D) $<$

(E) $>$

(F) None of the above

Solution:

## Response

To solve this problem, we need to analyze the expression:

\[
E = \frac{1}{a^2 - ab + 1} + \frac{1}{b^2 - ab + 1} - 4a^2b^2
\]

and compare it to \(\frac{7}{4}\).

Given that \(a + b = 1\), we can express \(b\) as \(b = 1 - a\). Substituting \(b = 1 - a\) into the expression, we have:

\[
E = \frac{1}{a^2 - a(1-a) + 1} + \frac{1}{(1-a)^2 - a(1-a) + 1} - 4a^2(1-a)^2
\]

Simplifying the terms inside the denominators:

1. For the first term:
   \[
   a^2 - a(1-a) + 1 = a^2 - a + a^2 + 1 = 2a^2 - a + 1
   \]

2. For the second term:
   \[
   (1-a)^2 - a(1-a) + 1 = 1 - 2a + a^2 - a + a^2 + 1 = 2a^2 - 3a + 2
   \]

Thus, the expression becomes:

\[
E = \frac{1}{2a^2 - a + 1} + \frac{1}{2a^2 - 3a + 2} - 4a^2(1-a)^2
\]

Now, let's analyze the expression for specific values of \(a\) and \(b\).

### Case 1: \(a = 0\), \(b = 1\)

\[
E = \frac{1}{1} + \frac{1}{1} - 0 = 2
\]

### Case 2: \(a = 1\), \(b = 0\)

\[
E = \frac{1}{1} + \frac{1}{1} - 0 = 2
\]

### Case 3: \(a = \frac{1}{2}\), \(b = \frac{1}{2}\)

\[
E = \frac{1}{2\left(\frac{1}{2}\right)^2 - \frac{1}{2} + 1} + \frac{1}{2\left(\frac{1}{2}\right)^2 - \frac{3}{2}\left(\frac{1}{2}\right) + 2} - 4\left(\frac{1}{2}\right)^2\left(\frac{1}{2}\right)^2
\]

Calculating each term:

- First term:
  \[
  2\left(\frac{1}{2}\right)^2 - \frac{1}{2} + 1 = \frac{1}{2} - \frac{1}{2} + 1 = 1
  \]
  \[
  \frac{1}{1} = 1
  \]

- Second term:
  \[
  2\left(\frac{1}{2}\right)^2 - \frac{3}{2}\left(\frac{1}{2}\right) + 2 = \frac{1}{2} - \frac{3}{4} + 2 = \frac{7}{4}
  \]
  \[
  \frac{1}{\frac{7}{4}} = \frac{4}{7}
  \]

- Third term:
  \[
  4\left(\frac{1}{2}\right)^4 = \frac{1}{4}
  \]

Thus, for \(a = \frac{1}{2}\), \(b = \frac{1}{2}\):

\[
E = 1 + \frac{4}{7} - \frac{1}{4} = \frac{28}{28} + \frac{16}{28} - \frac{7}{28} = \frac{37}{28}
\]

Now, compare \(\frac{37}{28}\) to \(\frac{7}{4}\):

\[
\frac{7}{4} = \frac{49}{28}
\]

Since \(\frac{37}{28} < \frac{49}{28}\), we have:

\[
E < \frac{7}{4}
\]

Thus, the expression is less than \(\frac{7}{4}\) for \(a = \frac{1}{2}\), \(b = \frac{1}{2}\), and it is equal to 2 for the boundary cases \(a = 0\) or \(a = 1\). Therefore, the inequality that holds for all \(a, b \geq 0\) with \(a + b = 1\) is:

\[
E \leq \frac{7}{4}
\]

The answer is \((A) \leq\).