## Problem

Let \( a_1, a_2, \ldots, a_n, x_1, x_2, \ldots, x_n \) be positive real numbers. Consider the following expression:
$$
a_1 a_2 \cdots a_n \left( \frac{a_1}{x_1} + \frac{a_2}{x_2} + \cdots + \frac{a_n}{x_n} - n \right) + x_1 x_2 \cdots x_n \left( \frac{x_1}{a_1} + \frac{x_2}{a_2} + \cdots + \frac{x_n}{a_n} - n \right) \quad () \quad 1
$$

Determine the correct inequality relation to fill in the blank.

Options:

(A) $\leq$ 

(B) $\geq$

(C) $=$ 

(D) $<$

(E) $>$

(F) None of the above

## Query

Task description: Please solve the problem with clear, rigorous, and logically sound steps. At the end of your response, state your answer in exactly this format: 'The answer is (Letter) Symbol', where Letter is one of the given options. Example: 'The answer is (A) $\leq$'.

Problem: Let \( a_1, a_2, \ldots, a_n, x_1, x_2, \ldots, x_n \) be positive real numbers. Consider the following expression:
$$
a_1 a_2 \cdots a_n \left( \frac{a_1}{x_1} + \frac{a_2}{x_2} + \cdots + \frac{a_n}{x_n} - n \right) + x_1 x_2 \cdots x_n \left( \frac{x_1}{a_1} + \frac{x_2}{a_2} + \cdots + \frac{x_n}{a_n} - n \right) \quad () \quad 1
$$

Determine the correct inequality relation to fill in the blank.

Options:

(A) $\leq$ 

(B) $\geq$

(C) $=$ 

(D) $<$

(E) $>$

(F) None of the above

Solution:

## Response

To solve this problem, we need to analyze the given expression:

\[
a_1 a_2 \cdots a_n \left( \frac{a_1}{x_1} + \frac{a_2}{x_2} + \cdots + \frac{a_n}{x_n} - n \right) + x_1 x_2 \cdots x_n \left( \frac{x_1}{a_1} + \frac{x_2}{a_2} + \cdots + \frac{x_n}{a_n} - n \right)
\]

We will use the AM-GM inequality, which states that for any non-negative real numbers \( y_1, y_2, \ldots, y_n \), the following holds:

\[
\frac{y_1 + y_2 + \cdots + y_n}{n} \geq \sqrt[n]{y_1 y_2 \cdots y_n}
\]

with equality if and only if \( y_1 = y_2 = \cdots = y_n \).

First, consider the term:

\[
\frac{a_1}{x_1} + \frac{a_2}{x_2} + \cdots + \frac{a_n}{x_n} \geq n \sqrt[n]{\frac{a_1 a_2 \cdots a_n}{x_1 x_2 \cdots x_n}}
\]

Thus:

\[
\frac{a_1}{x_1} + \frac{a_2}{x_2} + \cdots + \frac{a_n}{x_n} - n \geq n \left( \sqrt[n]{\frac{a_1 a_2 \cdots a_n}{x_1 x_2 \cdots x_n}} - 1 \right)
\]

Similarly, for the other term:

\[
\frac{x_1}{a_1} + \frac{x_2}{a_2} + \cdots + \frac{x_n}{a_n} \geq n \sqrt[n]{\frac{x_1 x_2 \cdots x_n}{a_1 a_2 \cdots a_n}}
\]

Thus:

\[
\frac{x_1}{a_1} + \frac{x_2}{a_2} + \cdots + \frac{x_n}{a_n} - n \geq n \left( \sqrt[n]{\frac{x_1 x_2 \cdots x_n}{a_1 a_2 \cdots a_n}} - 1 \right)
\]

Now, consider the entire expression:

\[
a_1 a_2 \cdots a_n \left( \frac{a_1}{x_1} + \frac{a_2}{x_2} + \cdots + \frac{a_n}{x_n} - n \right) + x_1 x_2 \cdots x_n \left( \frac{x_1}{a_1} + \frac{x_2}{a_2} + \cdots + \frac{x_n}{a_n} - n \right)
\]

Substituting the inequalities derived:

\[
\geq a_1 a_2 \cdots a_n \cdot n \left( \sqrt[n]{\frac{a_1 a_2 \cdots a_n}{x_1 x_2 \cdots x_n}} - 1 \right) + x_1 x_2 \cdots x_n \cdot n \left( \sqrt[n]{\frac{x_1 x_2 \cdots x_n}{a_1 a_2 \cdots a_n}} - 1 \right)
\]

Simplifying, we have:

\[
= n \left( a_1 a_2 \cdots a_n \cdot \sqrt[n]{\frac{a_1 a_2 \cdots a_n}{x_1 x_2 \cdots x_n}} + x_1 x_2 \cdots x_n \cdot \sqrt[n]{\frac{x_1 x_2 \cdots x_n}{a_1 a_2 \cdots a_n}} - a_1 a_2 \cdots a_n - x_1 x_2 \cdots x_n \right)
\]

By AM-GM, we know:

\[
a_1 a_2 \cdots a_n \cdot \sqrt[n]{\frac{a_1 a_2 \cdots a_n}{x_1 x_2 \cdots x_n}} \geq a_1 a_2 \cdots a_n
\]

\[
x_1 x_2 \cdots x_n \cdot \sqrt[n]{\frac{x_1 x_2 \cdots x_n}{a_1 a_2 \cdots a_n}} \geq x_1 x_2 \cdots x_n
\]

Thus, the entire expression is non-negative:

\[
\geq 0
\]

Equality holds if and only if \( \frac{a_1}{x_1} = \frac{a_2}{x_2} = \cdots = \frac{a_n}{x_n} = 1 \), i.e., \( a_i = x_i \) for all \( i \).

Therefore, the correct inequality relation is:

\[
\geq 0
\]

The answer is (B) $\geq$.