## Problem

Let $x_1, x_2, \ldots, x_n$ be positive real numbers such that $x_1 + x_2 + \cdots + x_n = 1$. Consider the following expression:
$$
\sum_{i=1}^n \frac{\min \left\{x_{i-1}, x_i\right\} \cdot \max \left\{x_i, x_{i+1}\right\}}{x_i} \quad () \quad 1
$$
where we denote $x_0 = x_n$ and $x_{n+1} = x_1$.

Determine the correct inequality relation to fill in the blank.

Options:

(A) $\leq$ 

(B) $\geq$

(C) $=$ 

(D) $<$

(E) $>$

(F) None of the above

## Query

Task description: Please solve the problem with clear, rigorous, and logically sound steps. At the end of your response, state your answer in exactly this format: 'The answer is (Letter) Symbol', where Letter is one of the given options. Example: 'The answer is (A) $\leq$'.

Problem: Let $x_1, x_2, \ldots, x_n$ be positive real numbers such that $x_1 + x_2 + \cdots + x_n = 1$. Consider the following expression:
$$
\sum_{i=1}^n \frac{\min \left\{x_{i-1}, x_i\right\} \cdot \max \left\{x_i, x_{i+1}\right\}}{x_i} \quad () \quad 1
$$
where we denote $x_0 = x_n$ and $x_{n+1} = x_1$.

Determine the correct inequality relation to fill in the blank.

Options:

(A) $\leq$ 

(B) $\geq$

(C) $=$ 

(D) $<$

(E) $>$

(F) None of the above

Solution:

## Response

To solve this problem, we need to analyze the given expression:

\[
\sum_{i=1}^n \frac{\min \left\{x_{i-1}, x_i\right\} \cdot \max \left\{x_i, x_{i+1}\right\}}{x_i}
\]

where \(x_0 = x_n\) and \(x_{n+1} = x_1\), and \(x_1 + x_2 + \cdots + x_n = 1\).

### Step-by-step Analysis:

1. **Understanding the Expression:**

   For each term in the sum, we have:
   \[
   \frac{\min \{x_{i-1}, x_i\} \cdot \max \{x_i, x_{i+1}\}}{x_i}
   \]

   - **Case 1:** If \(x_{i-1} \leq x_i\), then \(\min \{x_{i-1}, x_i\} = x_{i-1}\).
   - **Case 2:** If \(x_{i-1} > x_i\), then \(\min \{x_{i-1}, x_i\} = x_i\).

   - **Case 1:** If \(x_i \geq x_{i+1}\), then \(\max \{x_i, x_{i+1}\} = x_i\).
   - **Case 2:** If \(x_i < x_{i+1}\), then \(\max \{x_i, x_{i+1}\} = x_{i+1}\).

2. **Simplifying the Expression:**

   - If \(x_{i-1} \leq x_i\) and \(x_i \geq x_{i+1}\), the term becomes:
     \[
     \frac{x_{i-1} \cdot x_i}{x_i} = x_{i-1}
     \]

   - If \(x_{i-1} \leq x_i\) and \(x_i < x_{i+1}\), the term becomes:
     \[
     \frac{x_{i-1} \cdot x_{i+1}}{x_i}
     \]

   - If \(x_{i-1} > x_i\) and \(x_i \geq x_{i+1}\), the term becomes:
     \[
     \frac{x_i \cdot x_i}{x_i} = x_i
     \]

   - If \(x_{i-1} > x_i\) and \(x_i < x_{i+1}\), the term becomes:
     \[
     \frac{x_i \cdot x_{i+1}}{x_i} = x_{i+1}
     \]

3. **Bounding the Expression:**

   Each term in the sum is either \(x_{i-1}\), \(x_i\), \(x_{i+1}\), or \(\frac{x_{i-1} \cdot x_{i+1}}{x_i}\). Since \(x_1 + x_2 + \cdots + x_n = 1\), the sum of all terms \(x_i\) is 1.

   The expression can be bounded by considering the maximum possible value of each term. Since each \(x_i\) is a positive real number and the sum of all \(x_i\) is 1, the maximum value of any term \(\frac{x_{i-1} \cdot x_{i+1}}{x_i}\) is constrained by the fact that \(x_{i-1}, x_i, x_{i+1} \leq 1\).

4. **Conclusion:**

   The expression is a sum of terms that are each less than or equal to 1, and since the sum of all \(x_i\) is 1, the entire expression is bounded by 1. Therefore, the inequality relation that holds is:

   \[
   \sum_{i=1}^n \frac{\min \left\{x_{i-1}, x_i\right\} \cdot \max \left\{x_i, x_{i+1}\right\}}{x_i} \leq 1
   \]

Thus, the correct inequality relation to fill in the blank is:

The answer is (A) \(\leq\).