## Problem

Let $a, b, c$ be positive real numbers such that $abc = 1$. Consider the following inequality:
$$
\frac{2}{b(a+b)} + \frac{1}{c(b+c)} + \frac{1}{a(c+a)} \quad () \quad \frac{4}{3}.
$$

Determine the correct inequality relation to fill in the blank.

Options:

(A) $\leq$ 

(B) $\geq$

(C) $=$ 

(D) $<$

(E) $>$

(F) None of the above

## Query

Task description: Please solve the problem with clear, rigorous, and logically sound steps. At the end of your response, state your answer in exactly this format: 'The answer is (Letter) Symbol', where Letter is one of the given options. Example: 'The answer is (A) $\leq$'.

Problem: Let $a, b, c$ be positive real numbers such that $abc = 1$. Consider the following inequality:
$$
\frac{2}{b(a+b)} + \frac{1}{c(b+c)} + \frac{1}{a(c+a)} \quad () \quad \frac{4}{3}.
$$

Determine the correct inequality relation to fill in the blank.

Options:

(A) $\leq$ 

(B) $\geq$

(C) $=$ 

(D) $<$

(E) $>$

(F) None of the above

Solution:

## Response

To solve this problem, we need to analyze the given inequality:

\[
\frac{2}{b(a+b)} + \frac{1}{c(b+c)} + \frac{1}{a(c+a)} \quad () \quad \frac{4}{3}.
\]

We are given that \(abc = 1\) and \(a, b, c\) are positive real numbers. We need to determine the correct inequality relation to fill in the blank.

First, let's consider the expression on the left-hand side:

\[
\frac{2}{b(a+b)} + \frac{1}{c(b+c)} + \frac{1}{a(c+a)}.
\]

To simplify this, we can use the AM-GM inequality, which states that for non-negative numbers, the arithmetic mean is greater than or equal to the geometric mean. Applying AM-GM to each term, we have:

1. For the first term:
   \[
   b(a+b) \geq 2\sqrt{ab^2} = 2b\sqrt{a}.
   \]
   Thus,
   \[
   \frac{2}{b(a+b)} \leq \frac{1}{b\sqrt{a}}.
   \]

2. For the second term:
   \[
   c(b+c) \geq 2\sqrt{bc^2} = 2c\sqrt{b}.
   \]
   Thus,
   \[
   \frac{1}{c(b+c)} \leq \frac{1}{2c\sqrt{b}}.
   \]

3. For the third term:
   \[
   a(c+a) \geq 2\sqrt{a^2c} = 2a\sqrt{c}.
   \]
   Thus,
   \[
   \frac{1}{a(c+a)} \leq \frac{1}{2a\sqrt{c}}.
   \]

Now, let's sum these inequalities:

\[
\frac{2}{b(a+b)} + \frac{1}{c(b+c)} + \frac{1}{a(c+a)} \leq \frac{1}{b\sqrt{a}} + \frac{1}{2c\sqrt{b}} + \frac{1}{2a\sqrt{c}}.
\]

To further analyze this, we can use the condition \(abc = 1\). This implies that \(a = \frac{x}{y}\), \(b = \frac{y}{z}\), \(c = \frac{z}{x}\) for some positive \(x, y, z\). Substituting these into the inequality, we get:

\[
\frac{2}{\frac{y}{z} \left(\frac{x}{y} + \frac{y}{z}\right)} + \frac{1}{\frac{z}{x} \left(\frac{y}{z} + \frac{z}{x}\right)} + \frac{1}{\frac{x}{y} \left(\frac{z}{x} + \frac{x}{y}\right)}.
\]

Simplifying each term:

1. \(\frac{2}{\frac{y}{z} \left(\frac{x}{y} + \frac{y}{z}\right)} = \frac{2z}{y \left(\frac{x}{y} + \frac{y}{z}\right)} = \frac{2z}{x + y}\).

2. \(\frac{1}{\frac{z}{x} \left(\frac{y}{z} + \frac{z}{x}\right)} = \frac{x}{z \left(\frac{y}{z} + \frac{z}{x}\right)} = \frac{x}{y + z}\).

3. \(\frac{1}{\frac{x}{y} \left(\frac{z}{x} + \frac{x}{y}\right)} = \frac{y}{x \left(\frac{z}{x} + \frac{x}{y}\right)} = \frac{y}{z + x}\).

Thus, the inequality becomes:

\[
\frac{2z}{x+y} + \frac{x}{y+z} + \frac{y}{z+x}.
\]

By the Nesbitt's inequality, we know that:

\[
\frac{x}{y+z} + \frac{y}{z+x} + \frac{z}{x+y} \geq \frac{3}{2}.
\]

However, we have an extra factor of 2 in the first term, which suggests that the inequality is actually greater than \(\frac{4}{3}\).

Therefore, the correct inequality relation is:

\[
\frac{2}{b(a+b)} + \frac{1}{c(b+c)} + \frac{1}{a(c+a)} > \frac{4}{3}.
\]

The answer is (E) $>$.