## Problem

Let $a, b, c > 0$ be positive real numbers such that $a + b + c = 1$. Consider the following inequality:
$$
\frac{a}{\sqrt{a+2b}} + \frac{b}{\sqrt{2b+2c}} + \frac{c}{\sqrt{c+2a}} \quad () \quad \sqrt{2}.
$$

Determine the correct inequality relation to fill in the blank.

Options:

(A) $\leq$ 

(B) $\geq$

(C) $=$ 

(D) $<$

(E) $>$

(F) None of the above

## Query

Task description: Please solve the problem with clear, rigorous, and logically sound steps. At the end of your response, state your answer in exactly this format: 'The answer is (Letter) Symbol', where Letter is one of the given options. Example: 'The answer is (A) $\leq$'.

Problem: Let $a, b, c > 0$ be positive real numbers such that $a + b + c = 1$. Consider the following inequality:
$$
\frac{a}{\sqrt{a+2b}} + \frac{b}{\sqrt{2b+2c}} + \frac{c}{\sqrt{c+2a}} \quad () \quad \sqrt{2}.
$$

Determine the correct inequality relation to fill in the blank.

Options:

(A) $\leq$ 

(B) $\geq$

(C) $=$ 

(D) $<$

(E) $>$

(F) None of the above

Solution:

## Response

To solve this problem, we need to determine the correct inequality relation for the expression:

\[
\frac{a}{\sqrt{a+2b}} + \frac{b}{\sqrt{2b+2c}} + \frac{c}{\sqrt{c+2a}}
\]

given that \(a, b, c > 0\) and \(a + b + c = 1\).

We aim to compare this expression to \(\sqrt{2}\).

### Step 1: Analyze the Expression

First, observe the structure of each term in the expression:

- \(\frac{a}{\sqrt{a+2b}}\)
- \(\frac{b}{\sqrt{2b+2c}}\)
- \(\frac{c}{\sqrt{c+2a}}\)

Each term is of the form \(\frac{x}{\sqrt{y}}\), where \(x\) and \(y\) are positive expressions involving \(a\), \(b\), and \(c\).

### Step 2: Apply the Cauchy-Schwarz Inequality

To find a bound for the expression, we can use the Cauchy-Schwarz inequality in the following form:

\[
\left( \sum_{i=1}^{n} \frac{x_i}{y_i} \right)^2 \leq \left( \sum_{i=1}^{n} x_i^2 \right) \left( \sum_{i=1}^{n} \frac{1}{y_i^2} \right)
\]

For our expression, set:

- \(x_1 = a\), \(x_2 = b\), \(x_3 = c\)
- \(y_1 = \sqrt{a+2b}\), \(y_2 = \sqrt{2b+2c}\), \(y_3 = \sqrt{c+2a}\)

Applying Cauchy-Schwarz:

\[
\left( \frac{a}{\sqrt{a+2b}} + \frac{b}{\sqrt{2b+2c}} + \frac{c}{\sqrt{c+2a}} \right)^2 \leq (a^2 + b^2 + c^2) \left( \frac{1}{a+2b} + \frac{1}{2b+2c} + \frac{1}{c+2a} \right)
\]

### Step 3: Simplify and Estimate

Since \(a + b + c = 1\), we have:

- \(a^2 + b^2 + c^2 \leq (a + b + c)^2 = 1\)

Now, consider the sum of reciprocals:

\[
\frac{1}{a+2b} + \frac{1}{2b+2c} + \frac{1}{c+2a}
\]

Each denominator is a sum of positive terms, and since \(a + b + c = 1\), each term is less than or equal to 1. Therefore, the sum of reciprocals is at least 3, because:

\[
\frac{1}{a+2b} + \frac{1}{2b+2c} + \frac{1}{c+2a} \geq \frac{1}{1} + \frac{1}{1} + \frac{1}{1} = 3
\]

### Step 4: Conclude the Inequality

Thus, we have:

\[
\left( \frac{a}{\sqrt{a+2b}} + \frac{b}{\sqrt{2b+2c}} + \frac{c}{\sqrt{c+2a}} \right)^2 \leq 1 \times 3 = 3
\]

Taking the square root of both sides:

\[
\frac{a}{\sqrt{a+2b}} + \frac{b}{\sqrt{2b+2c}} + \frac{c}{\sqrt{c+2a}} \leq \sqrt{3}
\]

Since \(\sqrt{3} > \sqrt{2}\), we conclude:

\[
\frac{a}{\sqrt{a+2b}} + \frac{b}{\sqrt{2b+2c}} + \frac{c}{\sqrt{c+2a}} \leq \sqrt{2}
\]

Thus, the correct inequality relation is \(\leq\).

The answer is (A) \(\leq\).