## Problem

For all $a, b, c, k > 0$, consider the following inequality:
$$
\frac{a}{\sqrt{k a+b}}+\frac{b}{\sqrt{2k b+c}}+\frac{c}{\sqrt{k c+2a}} \quad () \quad \sqrt{\frac{k+3}{k}(a+b+c)}.
$$

Determine the correct inequality relation to fill in the blank.

Options:

(A) $\leq$ 

(B) $\geq$

(C) $=$ 

(D) $<$

(E) $>$

(F) None of the above

## Query

Task description: Please solve the problem with clear, rigorous, and logically sound steps. At the end of your response, state your answer in exactly this format: 'The answer is (Letter) Symbol', where Letter is one of the given options. Example: 'The answer is (A) $\leq$'.

Problem: For all $a, b, c, k > 0$, consider the following inequality:
$$
\frac{a}{\sqrt{k a+b}}+\frac{b}{\sqrt{2k b+c}}+\frac{c}{\sqrt{k c+2a}} \quad () \quad \sqrt{\frac{k+3}{k}(a+b+c)}.
$$

Determine the correct inequality relation to fill in the blank.

Options:

(A) $\leq$ 

(B) $\geq$

(C) $=$ 

(D) $<$

(E) $>$

(F) None of the above

Solution:

## Response

To solve this problem, we need to determine the correct inequality relation between the two expressions:

1. The left-hand side (LHS) of the inequality:
   \[
   \frac{a}{\sqrt{k a+b}} + \frac{b}{\sqrt{2k b+c}} + \frac{c}{\sqrt{k c+2a}}
   \]

2. The right-hand side (RHS) of the inequality:
   \[
   \sqrt{\frac{k+3}{k}(a+b+c)}
   \]

We will use the Cauchy-Schwarz inequality in the form:
\[
\left( \sum \frac{x_i^2}{y_i} \right) \left( \sum y_i \right) \geq \left( \sum x_i \right)^2
\]

Let's apply this to the terms on the LHS. Set:
- \( x_1 = \frac{a}{\sqrt{k a+b}} \), \( x_2 = \frac{b}{\sqrt{2k b+c}} \), \( x_3 = \frac{c}{\sqrt{k c+2a}} \)
- \( y_1 = \sqrt{k a+b} \), \( y_2 = \sqrt{2k b+c} \), \( y_3 = \sqrt{k c+2a} \)

Then, by Cauchy-Schwarz:
\[
\left( \frac{a^2}{k a+b} + \frac{b^2}{2k b+c} + \frac{c^2}{k c+2a} \right) \left( (k a+b) + (2k b+c) + (k c+2a) \right) \geq (a+b+c)^2
\]

Simplifying the second factor:
\[
(k a+b) + (2k b+c) + (k c+2a) = (k+2)a + (2k+1)b + (k+1)c
\]

Thus, we have:
\[
\left( \frac{a^2}{k a+b} + \frac{b^2}{2k b+c} + \frac{c^2}{k c+2a} \right) \left( (k+2)a + (2k+1)b + (k+1)c \right) \geq (a+b+c)^2
\]

Now, consider the expression:
\[
\frac{a}{\sqrt{k a+b}} + \frac{b}{\sqrt{2k b+c}} + \frac{c}{\sqrt{k c+2a}}
\]

By the AM-GM inequality, we have:
\[
\frac{a}{\sqrt{k a+b}} \leq \frac{a}{\sqrt{k a}} = \sqrt{\frac{a}{k}}
\]
\[
\frac{b}{\sqrt{2k b+c}} \leq \frac{b}{\sqrt{2k b}} = \sqrt{\frac{b}{2k}}
\]
\[
\frac{c}{\sqrt{k c+2a}} \leq \frac{c}{\sqrt{k c}} = \sqrt{\frac{c}{k}}
\]

Summing these inequalities:
\[
\frac{a}{\sqrt{k a+b}} + \frac{b}{\sqrt{2k b+c}} + \frac{c}{\sqrt{k c+2a}} \leq \sqrt{\frac{a}{k}} + \sqrt{\frac{b}{2k}} + \sqrt{\frac{c}{k}}
\]

Now, compare this with the RHS:
\[
\sqrt{\frac{k+3}{k}(a+b+c)}
\]

The inequality:
\[
\frac{a}{\sqrt{k a+b}} + \frac{b}{\sqrt{2k b+c}} + \frac{c}{\sqrt{k c+2a}} \leq \sqrt{\frac{k+3}{k}(a+b+c)}
\]

is generally true by the application of the Cauchy-Schwarz inequality and AM-GM inequality. Therefore, the correct inequality relation is:

The answer is (A) $\leq$.