## Problem

Let $x, y, z$ be positive numbers such that $xy + yz + zx = 1$. Consider the following inequality:
$$
\frac{x^3}{1+9y^2zx} + \frac{y^3}{1+9z^2xy} + \frac{z^3}{1+9x^2yz} \quad () \quad \frac{(x+y+z)^3}{20}.
$$

Determine the correct inequality relation to fill in the blank.

Options:

(A) $\leq$ 

(B) $\geq$

(C) $=$ 

(D) $<$

(E) $>$

(F) None of the above

## Query

Task description: Please solve the problem with clear, rigorous, and logically sound steps. At the end of your response, state your answer in exactly this format: 'The answer is (Letter) Symbol', where Letter is one of the given options. Example: 'The answer is (A) $\leq$'.

Problem: Let $x, y, z$ be positive numbers such that $xy + yz + zx = 1$. Consider the following inequality:
$$
\frac{x^3}{1+9y^2zx} + \frac{y^3}{1+9z^2xy} + \frac{z^3}{1+9x^2yz} \quad () \quad \frac{(x+y+z)^3}{20}.
$$

Determine the correct inequality relation to fill in the blank.

Options:

(A) $\leq$ 

(B) $\geq$

(C) $=$ 

(D) $<$

(E) $>$

(F) None of the above

Solution:

## Response

To solve this problem, we need to determine the correct inequality relation between the two expressions:

1. \(\frac{x^3}{1+9y^2zx} + \frac{y^3}{1+9z^2xy} + \frac{z^3}{1+9x^2yz}\)
2. \(\frac{(x+y+z)^3}{20}\)

given the condition \(xy + yz + zx = 1\).

### Step 1: Analyze the Left-Hand Side

The left-hand side of the inequality is:

\[
\frac{x^3}{1+9y^2zx} + \frac{y^3}{1+9z^2xy} + \frac{z^3}{1+9x^2yz}
\]

Each term \(\frac{x^3}{1+9y^2zx}\), \(\frac{y^3}{1+9z^2xy}\), and \(\frac{z^3}{1+9x^2yz}\) is a fraction where the numerator is a cube of one of the variables and the denominator is a linear function of the product of the other two variables, scaled by 9.

### Step 2: Analyze the Right-Hand Side

The right-hand side of the inequality is:

\[
\frac{(x+y+z)^3}{20}
\]

This is a cubic expression in \(x, y, z\) divided by 20.

### Step 3: Use Symmetry and Homogeneity

The problem is symmetric in \(x, y, z\), and the condition \(xy + yz + zx = 1\) is homogeneous of degree 2. We can assume without loss of generality that \(x = y = z\) to simplify the analysis, as the inequality should hold for all positive \(x, y, z\) satisfying the condition.

Assume \(x = y = z = t\). Then:

\[
3t^2 = 1 \implies t^2 = \frac{1}{3} \implies t = \frac{1}{\sqrt{3}}
\]

Substitute \(x = y = z = \frac{1}{\sqrt{3}}\) into both sides:

**Left-Hand Side:**

\[
3 \cdot \frac{\left(\frac{1}{\sqrt{3}}\right)^3}{1 + 9 \left(\frac{1}{\sqrt{3}}\right)^5} = 3 \cdot \frac{\frac{1}{3\sqrt{3}}}{1 + \frac{9}{27\sqrt{3}}} = 3 \cdot \frac{\frac{1}{3\sqrt{3}}}{1 + \frac{1}{3\sqrt{3}}}
\]

Simplifying the denominator:

\[
1 + \frac{1}{3\sqrt{3}} = \frac{3\sqrt{3} + 1}{3\sqrt{3}}
\]

Thus, the left-hand side becomes:

\[
3 \cdot \frac{\frac{1}{3\sqrt{3}}}{\frac{3\sqrt{3} + 1}{3\sqrt{3}}} = 3 \cdot \frac{1}{3\sqrt{3} + 1} = \frac{3}{3\sqrt{3} + 1}
\]

**Right-Hand Side:**

\[
\frac{(3 \cdot \frac{1}{\sqrt{3}})^3}{20} = \frac{3^3 \cdot \frac{1}{3\sqrt{3}}}{20} = \frac{27}{20\sqrt{3}}
\]

### Step 4: Compare the Two Sides

We need to compare:

\[
\frac{3}{3\sqrt{3} + 1} \quad \text{and} \quad \frac{27}{20\sqrt{3}}
\]

To compare these, we can cross-multiply:

\[
3 \cdot 20\sqrt{3} \quad \text{vs} \quad 27 \cdot (3\sqrt{3} + 1)
\]

Calculate each:

- Left: \(60\sqrt{3}\)
- Right: \(81\sqrt{3} + 27\)

Clearly, \(60\sqrt{3} < 81\sqrt{3} + 27\).

Thus, the left-hand side is less than the right-hand side.

### Conclusion

The inequality is:

\[
\frac{x^3}{1+9y^2zx} + \frac{y^3}{1+9z^2xy} + \frac{z^3}{1+9x^2yz} < \frac{(x+y+z)^3}{20}
\]

The answer is \((D) <\).