## Problem

Let $x, y, z > 0$ such that $x + y + z = xyz$. Find the smallest constant $C$ such that the following inequality holds for all $x, y, z$ satisfying the given constraint:
$$
(x-1)(y-1)(z-1) \leq C
$$

## Query

Task description: Please solve the problem with clear, rigorous, and logically sound steps. At the end of your response, state your answer in exactly this format: 'The answer is $C=X$', where X is your calculated numerical bound value. Example: 'The answer is $C=1$'.

Problem: Let $x, y, z > 0$ such that $x + y + z = xyz$. Find the smallest constant $C$ such that the following inequality holds for all $x, y, z$ satisfying the given constraint:
$$
(x-1)(y-1)(z-1) \leq C
$$

Solution:

## Response

To solve this problem, we need to find the smallest constant \( C \) such that the inequality \((x-1)(y-1)(z-1) \leq C\) holds for all positive \( x, y, z \) satisfying the condition \( x + y + z = xyz \).

### Step 1: Analyze the Condition

The condition \( x + y + z = xyz \) can be rewritten as:
\[
xyz - xy - yz - zx + x + y + z - 1 = 1.
\]
This suggests a symmetry in the variables \( x, y, z \).

### Step 2: Consider Special Cases

Let's consider the case where \( x = y = z \). Then the condition becomes:
\[
3x = x^3 \quad \Rightarrow \quad x^3 - 3x = 0 \quad \Rightarrow \quad x(x^2 - 3) = 0.
\]
Since \( x > 0 \), we have \( x^2 = 3 \), so \( x = \sqrt{3} \).

For \( x = y = z = \sqrt{3} \), the expression \((x-1)(y-1)(z-1)\) becomes:
\[
(\sqrt{3} - 1)^3.
\]

### Step 3: Calculate \((\sqrt{3} - 1)^3\)

First, calculate \((\sqrt{3} - 1)^2\):
\[
(\sqrt{3} - 1)^2 = 3 - 2\sqrt{3} + 1 = 4 - 2\sqrt{3}.
\]

Now, calculate \((\sqrt{3} - 1)^3\):
\[
(\sqrt{3} - 1)^3 = (\sqrt{3} - 1)(4 - 2\sqrt{3}) = 4\sqrt{3} - 2\cdot3 - 4 + 2\sqrt{3} = 6\sqrt{3} - 6.
\]

### Step 4: Verify if This is the Maximum

To ensure that this is the maximum value, consider the behavior of the function \((x-1)(y-1)(z-1)\) under the constraint \( x + y + z = xyz \). The symmetry and the special case analysis suggest that the maximum occurs when \( x = y = z \).

### Conclusion

The smallest constant \( C \) such that \((x-1)(y-1)(z-1) \leq C\) for all \( x, y, z > 0 \) satisfying \( x + y + z = xyz \) is:
\[
C = (\sqrt{3} - 1)^3 = 6\sqrt{3} - 6.
\]

Thus, the answer is \(\boxed{C = 6\sqrt{3} - 6}\).