## Problem

Find the largest constant $C$ such that for all real numbers $x, y, z$, the following inequality holds:
$$
\frac{x^2-y^2}{2 x^2+1}+\frac{y^2-z^2}{2 y^2+1}+\frac{z^2-x^2}{2 z^2+1} \geq C
$$

## Query

Task description: Please solve the problem with clear, rigorous, and logically sound steps. At the end of your response, state your answer in exactly this format: 'The answer is $C=X$', where X is your calculated numerical bound value. Example: 'The answer is $C=1$'.

Problem: Find the largest constant $C$ such that for all real numbers $x, y, z$, the following inequality holds:
$$
\frac{x^2-y^2}{2 x^2+1}+\frac{y^2-z^2}{2 y^2+1}+\frac{z^2-x^2}{2 z^2+1} \geq C
$$

Solution:

## Response

To solve this problem, we need to find the largest constant \( C \) such that the inequality

\[
\frac{x^2-y^2}{2x^2+1} + \frac{y^2-z^2}{2y^2+1} + \frac{z^2-x^2}{2z^2+1} \geq C
\]

holds for all real numbers \( x, y, z \).

First, observe that the expression is cyclic in \( x, y, z \). This suggests that symmetry might play a role in simplifying the problem. Let's consider some specific cases to gain insight.

### Case 1: \( x = y = z \)

If \( x = y = z \), then each term in the sum becomes zero:

\[
\frac{x^2-x^2}{2x^2+1} = 0
\]

Thus, the entire expression evaluates to 0. Therefore, for \( C \) to satisfy the inequality for all \( x, y, z \), it must be that \( C \leq 0 \).

### Case 2: \( x = y \neq z \)

Consider \( x = y \) and \( z = 0 \). The expression becomes:

\[
\frac{x^2-x^2}{2x^2+1} + \frac{x^2-0^2}{2x^2+1} + \frac{0^2-x^2}{1} = 0 + \frac{x^2}{2x^2+1} - x^2
\]

Simplifying, we have:

\[
\frac{x^2}{2x^2+1} - x^2 = \frac{x^2 - x^2(2x^2+1)}{2x^2+1} = \frac{x^2 - 2x^4 - x^2}{2x^2+1} = \frac{-2x^4}{2x^2+1}
\]

For large \( x \), this expression approaches \(-x^2\), which can be made arbitrarily large negative. Thus, \( C \) cannot be positive.

### Case 3: \( x = 1, y = 0, z = -1 \)

Evaluate the expression:

\[
\frac{1^2-0^2}{2 \cdot 1^2 + 1} + \frac{0^2 - (-1)^2}{2 \cdot 0^2 + 1} + \frac{(-1)^2 - 1^2}{2 \cdot (-1)^2 + 1}
\]

This simplifies to:

\[
\frac{1}{3} + \frac{-1}{1} + \frac{0}{3} = \frac{1}{3} - 1 = -\frac{2}{3}
\]

This shows that the expression can be as low as \(-\frac{2}{3}\).

### Conclusion

From the above cases, the expression can be zero or negative, and it can reach as low as \(-\frac{2}{3}\). Therefore, the largest constant \( C \) such that the inequality holds for all real numbers \( x, y, z \) is \(-\frac{2}{3}\).

Thus, the answer is \(\boxed{C = -\frac{2}{3}}\).