## Problem

Let $a_1, a_2, \ldots, a_n$ be real numbers and $S$ be a non-empty subset of $\{1,2, \ldots, n\}$. Find the largest constant $C$ such that the following inequality holds for all $a_1, a_2, \ldots, a_n$ and $S$:
$$
2C \left(\sum_{i \in S} a_i\right)^2 \leq \sum_{1 \leq i \leq j \leq n}\left(a_i+\cdots+a_j\right)^2
$$

## Query

Task description: Please solve the problem with clear, rigorous, and logically sound steps. At the end of your response, state your answer in exactly this format: 'The answer is $C=X$', where X is your calculated numerical bound value. Example: 'The answer is $C=1$'.

Problem: Let $a_1, a_2, \ldots, a_n$ be real numbers and $S$ be a non-empty subset of $\{1,2, \ldots, n\}$. Find the largest constant $C$ such that the following inequality holds for all $a_1, a_2, \ldots, a_n$ and $S$:
$$
2C \left(\sum_{i \in S} a_i\right)^2 \leq \sum_{1 \leq i \leq j \leq n}\left(a_i+\cdots+a_j\right)^2
$$

Solution:

## Response

To solve this problem, we need to find the largest constant \( C \) such that the inequality

\[
2C \left(\sum_{i \in S} a_i\right)^2 \leq \sum_{1 \leq i \leq j \leq n}\left(a_i+\cdots+a_j\right)^2
\]

holds for all real numbers \( a_1, a_2, \ldots, a_n \) and all non-empty subsets \( S \subseteq \{1, 2, \ldots, n\} \).

### Step 1: Understand the Right-Hand Side

The right-hand side of the inequality is a sum over all subarrays of the sequence \( a_1, a_2, \ldots, a_n \). For each pair \( (i, j) \) with \( 1 \leq i \leq j \leq n \), the term \((a_i + a_{i+1} + \cdots + a_j)^2\) is included.

### Step 2: Simplify the Right-Hand Side

The sum \(\sum_{1 \leq i \leq j \leq n} (a_i + \cdots + a_j)^2\) can be expanded and simplified. Consider the contribution of each \( a_k \) to this sum. Each \( a_k \) appears in several subarrays, specifically in all subarrays starting at or before \( k \) and ending at or after \( k \).

The number of such subarrays is \( k \times (n-k+1) \). Therefore, the contribution of \( a_k \) to the sum is:

\[
a_k^2 \cdot k \cdot (n-k+1)
\]

Additionally, there are cross terms involving \( a_k a_l \) for \( k \neq l \), but these will cancel out when considering symmetry and the fact that the inequality must hold for all choices of \( a_1, a_2, \ldots, a_n \).

### Step 3: Consider the Left-Hand Side

The left-hand side is \( 2C \left(\sum_{i \in S} a_i\right)^2 \). This is a quadratic form in the \( a_i \)'s, specifically focusing on the subset \( S \).

### Step 4: Find the Largest \( C \)

To find the largest \( C \), consider the case where \( S = \{1, 2, \ldots, n\} \). Then the left-hand side becomes:

\[
2C \left(\sum_{i=1}^n a_i\right)^2
\]

The right-hand side, as simplified, becomes:

\[
\sum_{1 \leq i \leq j \leq n} (a_i + \cdots + a_j)^2 = \sum_{k=1}^n a_k^2 \cdot k \cdot (n-k+1)
\]

For the inequality to hold for all \( a_1, a_2, \ldots, a_n \), we need:

\[
2C \left(\sum_{i=1}^n a_i\right)^2 \leq \sum_{k=1}^n a_k^2 \cdot k \cdot (n-k+1)
\]

### Step 5: Test with Specific Values

Consider \( a_1 = a_2 = \cdots = a_n = 1 \). Then:

- The left-hand side becomes \( 2C n^2 \).
- The right-hand side becomes:

\[
\sum_{k=1}^n k(n-k+1) = \sum_{k=1}^n (kn - k^2 + k) = n \sum_{k=1}^n k - \sum_{k=1}^n k^2 + \sum_{k=1}^n k
\]

Using the formulas for sums of integers and squares:

\[
\sum_{k=1}^n k = \frac{n(n+1)}{2}, \quad \sum_{k=1}^n k^2 = \frac{n(n+1)(2n+1)}{6}
\]

The right-hand side simplifies to:

\[
n \cdot \frac{n(n+1)}{2} - \frac{n(n+1)(2n+1)}{6} + \frac{n(n+1)}{2}
\]

Simplifying further, this becomes:

\[
\frac{n(n+1)(3n+2)}{6}
\]

For the inequality to hold, we need:

\[
2C n^2 \leq \frac{n(n+1)(3n+2)}{6}
\]

Solving for \( C \), we find:

\[
C \leq \frac{(n+1)(3n+2)}{12n}
\]

As \( n \to \infty \), this expression approaches \(\frac{3}{4}\).

### Conclusion

The largest constant \( C \) such that the inequality holds for all \( a_1, a_2, \ldots, a_n \) and all non-empty subsets \( S \) is:

\[
\boxed{\frac{3}{4}}
\]

Thus, the answer is \( C = \frac{3}{4} \).

The answer is \( C = \frac{3}{4} \).