## Problem

Let $x, y, z > 0$ such that $x+y+z=1$. Determine the minimal constant $C$ such that the following inequality holds for all $x, y, z$:

$$
x y(y+4 z)+y z(z+4 x)+z x(x+4 y) \leq C.
$$

## Query

Task description: Please solve the problem with clear, rigorous, and logically sound steps. At the end of your response, state your answer in exactly this format: 'The answer is $C=X$', where X is your calculated numerical bound value. Example: 'The answer is $C=1$'.

Problem: Let $x, y, z > 0$ such that $x+y+z=1$. Determine the minimal constant $C$ such that the following inequality holds for all $x, y, z$:

$$
x y(y+4 z)+y z(z+4 x)+z x(x+4 y) \leq C.
$$

Solution:

## Response

To solve this problem, we need to find the minimal constant \( C \) such that the inequality

\[
x y(y+4 z) + y z(z+4 x) + z x(x+4 y) \leq C
\]

holds for all positive \( x, y, z \) with \( x + y + z = 1 \).

First, let's expand each term in the inequality:

1. \( x y(y + 4z) = xy^2 + 4xyz \)
2. \( y z(z + 4x) = yz^2 + 4xyz \)
3. \( z x(x + 4y) = zx^2 + 4xyz \)

Adding these, we have:

\[
xy^2 + yz^2 + zx^2 + 12xyz
\]

Thus, the inequality becomes:

\[
xy^2 + yz^2 + zx^2 + 12xyz \leq C
\]

To find the minimal \( C \), we consider specific cases and use symmetry and the condition \( x + y + z = 1 \).

### Case 1: \( x = y = z = \frac{1}{3} \)

Substitute \( x = y = z = \frac{1}{3} \) into the expression:

\[
xy^2 + yz^2 + zx^2 + 12xyz = \left(\frac{1}{3}\right)\left(\frac{1}{3}\right)^2 + \left(\frac{1}{3}\right)\left(\frac{1}{3}\right)^2 + \left(\frac{1}{3}\right)\left(\frac{1}{3}\right)^2 + 12\left(\frac{1}{3}\right)^3
\]

Calculating each term:

- \( xy^2 = \frac{1}{3} \cdot \frac{1}{9} = \frac{1}{27} \)
- \( yz^2 = \frac{1}{3} \cdot \frac{1}{9} = \frac{1}{27} \)
- \( zx^2 = \frac{1}{3} \cdot \frac{1}{9} = \frac{1}{27} \)
- \( 12xyz = 12 \cdot \frac{1}{27} = \frac{12}{27} = \frac{4}{9} \)

Summing these:

\[
3 \cdot \frac{1}{27} + \frac{4}{9} = \frac{3}{27} + \frac{12}{27} = \frac{15}{27} = \frac{5}{9}
\]

### Case 2: \( x = \frac{1}{2}, y = \frac{1}{2}, z = 0 \)

Substitute \( x = \frac{1}{2}, y = \frac{1}{2}, z = 0 \):

\[
xy^2 + yz^2 + zx^2 + 12xyz = \frac{1}{2} \cdot \left(\frac{1}{2}\right)^2 + 0 + 0 + 0 = \frac{1}{2} \cdot \frac{1}{4} = \frac{1}{8}
\]

### Case 3: \( x = 1, y = z = 0 \)

Substitute \( x = 1, y = 0, z = 0 \):

\[
xy^2 + yz^2 + zx^2 + 12xyz = 0 + 0 + 0 + 0 = 0
\]

From these cases, the maximum value of the expression is \(\frac{5}{9}\).

Thus, the minimal constant \( C \) such that the inequality holds for all \( x, y, z > 0 \) with \( x + y + z = 1 \) is \(\frac{5}{9}\).

The answer is \(\boxed{C = \frac{5}{9}}\).