## Problem

Given $a, b, c > 0$ such that $ab + bc + ca = abc$, find the smallest constant $C$ such that the following inequality holds for all $a, b, c$:
$$
\frac{1}{a+3b+2c} + \frac{1}{b+3c+2a} + \frac{1}{c+3a+2b} \leq C.
$$

## Query

Task description: Please solve the problem with clear, rigorous, and logically sound steps. At the end of your response, state your answer in exactly this format: 'The answer is $C=X$', where X is your calculated numerical bound value. Example: 'The answer is $C=1$'.

Problem: Given $a, b, c > 0$ such that $ab + bc + ca = abc$, find the smallest constant $C$ such that the following inequality holds for all $a, b, c$:
$$
\frac{1}{a+3b+2c} + \frac{1}{b+3c+2a} + \frac{1}{c+3a+2b} \leq C.
$$

Solution:

## Response

To solve this problem, we need to find the smallest constant \( C \) such that the inequality

\[
\frac{1}{a+3b+2c} + \frac{1}{b+3c+2a} + \frac{1}{c+3a+2b} \leq C
\]

holds for all positive \( a, b, c \) satisfying \( ab + bc + ca = abc \).

First, let's explore the condition \( ab + bc + ca = abc \). We can rewrite this as:

\[
abc = ab + bc + ca.
\]

This condition is symmetric in \( a, b, c \). A natural substitution to simplify the problem is to set \( a = \frac{x+y+z}{x}, b = \frac{x+y+z}{y}, c = \frac{x+y+z}{z} \) for some positive \( x, y, z \). This substitution satisfies the condition:

\[
ab + bc + ca = \left(\frac{x+y+z}{x}\right)\left(\frac{x+y+z}{y}\right) + \left(\frac{x+y+z}{y}\right)\left(\frac{x+y+z}{z}\right) + \left(\frac{x+y+z}{z}\right)\left(\frac{x+y+z}{x}\right) = \frac{(x+y+z)^2}{xy} + \frac{(x+y+z)^2}{yz} + \frac{(x+y+z)^2}{zx}.
\]

This simplifies to:

\[
abc = \frac{(x+y+z)^3}{xyz} = \frac{(x+y+z)^2}{xy} + \frac{(x+y+z)^2}{yz} + \frac{(x+y+z)^2}{zx} = ab + bc + ca.
\]

Now, let's evaluate the expression:

\[
\frac{1}{a+3b+2c} + \frac{1}{b+3c+2a} + \frac{1}{c+3a+2b}.
\]

Substituting \( a = \frac{x+y+z}{x}, b = \frac{x+y+z}{y}, c = \frac{x+y+z}{z} \), we have:

\[
a + 3b + 2c = \frac{x+y+z}{x} + 3\frac{x+y+z}{y} + 2\frac{x+y+z}{z} = (x+y+z)\left(\frac{1}{x} + \frac{3}{y} + \frac{2}{z}\right).
\]

Similarly, we find:

\[
b + 3c + 2a = (x+y+z)\left(\frac{1}{y} + \frac{3}{z} + \frac{2}{x}\right),
\]
\[
c + 3a + 2b = (x+y+z)\left(\frac{1}{z} + \frac{3}{x} + \frac{2}{y}\right).
\]

Thus, the expression becomes:

\[
\frac{1}{(x+y+z)\left(\frac{1}{x} + \frac{3}{y} + \frac{2}{z}\right)} + \frac{1}{(x+y+z)\left(\frac{1}{y} + \frac{3}{z} + \frac{2}{x}\right)} + \frac{1}{(x+y+z)\left(\frac{1}{z} + \frac{3}{x} + \frac{2}{y}\right)}.
\]

This simplifies to:

\[
\frac{1}{x+y+z}\left(\frac{1}{\frac{1}{x} + \frac{3}{y} + \frac{2}{z}} + \frac{1}{\frac{1}{y} + \frac{3}{z} + \frac{2}{x}} + \frac{1}{\frac{1}{z} + \frac{3}{x} + \frac{2}{y}}\right).
\]

To find the maximum value of this expression, we can use the AM-HM inequality:

\[
\frac{1}{\frac{1}{x} + \frac{3}{y} + \frac{2}{z}} \leq \frac{x}{6}, \quad \frac{1}{\frac{1}{y} + \frac{3}{z} + \frac{2}{x}} \leq \frac{y}{6}, \quad \frac{1}{\frac{1}{z} + \frac{3}{x} + \frac{2}{y}} \leq \frac{z}{6}.
\]

Thus, the sum is bounded by:

\[
\frac{x}{6} + \frac{y}{6} + \frac{z}{6} = \frac{x+y+z}{6}.
\]

Therefore, the entire expression is bounded by:

\[
\frac{1}{x+y+z} \cdot \frac{x+y+z}{6} = \frac{1}{6}.
\]

Thus, the smallest constant \( C \) such that the inequality holds for all \( a, b, c \) is:

\[
\boxed{\frac{1}{6}}.
\]

The answer is \( C = \frac{1}{6} \).