## Problem

Let $a, b, c$ be positive real numbers. Determine the minimal constant $C$ such that the following inequality holds for all $a, b, c \in \mathbb{R}^{+}$:
$$
a+b+c+\sqrt{a^2+b^2+c^2} \leq C \cdot \left(\frac{1}{a}+\frac{1}{b}+\frac{1}{c}\right) \cdot \left(a^2+b^2+c^2\right)
$$

## Query

Task description: Please solve the problem with clear, rigorous, and logically sound steps. At the end of your response, state your answer in exactly this format: 'The answer is $C=X$', where X is your calculated numerical bound value. Example: 'The answer is $C=1$'.

Problem: Let $a, b, c$ be positive real numbers. Determine the minimal constant $C$ such that the following inequality holds for all $a, b, c \in \mathbb{R}^{+}$:
$$
a+b+c+\sqrt{a^2+b^2+c^2} \leq C \cdot \left(\frac{1}{a}+\frac{1}{b}+\frac{1}{c}\right) \cdot \left(a^2+b^2+c^2\right)
$$

Solution:

## Response

To solve this problem, we need to find the minimal constant \( C \) such that the inequality

\[
a + b + c + \sqrt{a^2 + b^2 + c^2} \leq C \cdot \left(\frac{1}{a} + \frac{1}{b} + \frac{1}{c}\right) \cdot \left(a^2 + b^2 + c^2\right)
\]

holds for all positive real numbers \( a, b, c \).

### Step 1: Simplify the Right-Hand Side

The right-hand side of the inequality is:

\[
C \cdot \left(\frac{1}{a} + \frac{1}{b} + \frac{1}{c}\right) \cdot \left(a^2 + b^2 + c^2\right)
\]

This can be rewritten as:

\[
C \cdot \left(\frac{a^2 + b^2 + c^2}{a} + \frac{a^2 + b^2 + c^2}{b} + \frac{a^2 + b^2 + c^2}{c}\right)
\]

\[
= C \cdot \left((b^2 + c^2) + (a^2 + c^2) + (a^2 + b^2)\right)
\]

\[
= C \cdot (2a^2 + 2b^2 + 2c^2)
\]

\[
= 2C \cdot (a^2 + b^2 + c^2)
\]

### Step 2: Analyze the Left-Hand Side

The left-hand side is:

\[
a + b + c + \sqrt{a^2 + b^2 + c^2}
\]

### Step 3: Consider Special Cases

To find the minimal \( C \), consider the case where \( a = b = c = t \). Then:

- The left-hand side becomes:
  \[
  3t + \sqrt{3t^2} = 3t + \sqrt{3}t = (3 + \sqrt{3})t
  \]

- The right-hand side becomes:
  \[
  2C \cdot 3t^2 = 6Ct^2
  \]

The inequality becomes:

\[
(3 + \sqrt{3})t \leq 6Ct^2
\]

Dividing both sides by \( t \) (assuming \( t > 0 \)):

\[
3 + \sqrt{3} \leq 6Ct
\]

Solving for \( C \), we get:

\[
C \geq \frac{3 + \sqrt{3}}{6t}
\]

As \( t \to 0^+ \), the right-hand side approaches infinity, so this does not provide a bound. Instead, consider \( t = 1 \):

\[
C \geq \frac{3 + \sqrt{3}}{6}
\]

### Step 4: Verify the Bound

To verify, substitute \( C = \frac{3 + \sqrt{3}}{6} \) into the inequality:

- For \( a = b = c = 1 \), the left-hand side is:
  \[
  3 + \sqrt{3}
  \]

- The right-hand side is:
  \[
  6 \cdot \frac{3 + \sqrt{3}}{6} = 3 + \sqrt{3}
  \]

Thus, the inequality holds with equality for \( a = b = c = 1 \).

### Conclusion

The minimal constant \( C \) such that the inequality holds for all positive real numbers \( a, b, c \) is:

\[
\boxed{\frac{3 + \sqrt{3}}{6}}
\]

The answer is \( C = \frac{3 + \sqrt{3}}{6} \).