## Problem

Let $x, y, z$ be real numbers such that $0 \leq x, y, z \leq 1$. Find the smallest constant $C$ such that the following inequality holds for all $x, y, z$ in the given domain:
$$
\frac{x}{y+z+1}+\frac{y}{z+x+1}+\frac{z}{x+y+1} \leq 3C -(1-x)(1-y)(1-z).
$$

## Query

Task description: Please solve the problem with clear, rigorous, and logically sound steps. At the end of your response, state your answer in exactly this format: 'The answer is $C=X$', where X is your calculated numerical bound value. Example: 'The answer is $C=1$'.

Problem: Let $x, y, z$ be real numbers such that $0 \leq x, y, z \leq 1$. Find the smallest constant $C$ such that the following inequality holds for all $x, y, z$ in the given domain:
$$
\frac{x}{y+z+1}+\frac{y}{z+x+1}+\frac{z}{x+y+1} \leq 3C -(1-x)(1-y)(1-z).
$$

Solution:

## Response

To solve this problem, we need to find the smallest constant \( C \) such that the inequality

\[
\frac{x}{y+z+1} + \frac{y}{z+x+1} + \frac{z}{x+y+1} \leq 3C - (1-x)(1-y)(1-z)
\]

holds for all \( x, y, z \) in the interval \([0, 1]\).

### Step 1: Analyze the Left-Hand Side

The left-hand side of the inequality is:

\[
\frac{x}{y+z+1} + \frac{y}{z+x+1} + \frac{z}{x+y+1}.
\]

Each term \(\frac{x}{y+z+1}\), \(\frac{y}{z+x+1}\), and \(\frac{z}{x+y+1}\) is non-negative and less than or equal to \(x\), \(y\), and \(z\) respectively, since \(y+z+1 \geq 1\), \(z+x+1 \geq 1\), and \(x+y+1 \geq 1\).

### Step 2: Analyze the Right-Hand Side

The right-hand side is:

\[
3C - (1-x)(1-y)(1-z).
\]

The term \((1-x)(1-y)(1-z)\) is non-negative and reaches its maximum value of 1 when \(x = y = z = 0\).

### Step 3: Consider Boundary Cases

1. **Case \(x = y = z = 0\):**

   \[
   \text{LHS} = 0, \quad \text{RHS} = 3C - 1.
   \]

   For the inequality to hold, we need:

   \[
   0 \leq 3C - 1 \implies C \geq \frac{1}{3}.
   \]

2. **Case \(x = y = z = 1\):**

   \[
   \text{LHS} = \frac{1}{2} + \frac{1}{2} + \frac{1}{2} = \frac{3}{2}, \quad \text{RHS} = 3C.
   \]

   For the inequality to hold, we need:

   \[
   \frac{3}{2} \leq 3C \implies C \geq \frac{1}{2}.
   \]

### Step 4: Check Intermediate Values

To ensure \(C = \frac{1}{2}\) works for all \(x, y, z \in [0, 1]\), consider:

- **Case \(x = 1, y = z = 0\):**

  \[
  \text{LHS} = \frac{1}{1} + 0 + 0 = 1, \quad \text{RHS} = 3C - 1.
  \]

  For the inequality to hold, we need:

  \[
  1 \leq 3C - 1 \implies 3C \geq 2 \implies C \geq \frac{2}{3}.
  \]

### Conclusion

The smallest \( C \) that satisfies all these conditions is \( C = \frac{2}{3} \). Therefore, the inequality holds for all \( x, y, z \in [0, 1] \) when \( C = \frac{2}{3} \).

The answer is \(\boxed{C = \frac{2}{3}}\).