## Problem

Let $a, b, c$ be real numbers such that $a+b+c=1$. Find the smallest constant $C$ such that the following inequality holds for all $a, b, c$ satisfying the given constraint:
$$
\frac{11 a-2}{1+a^2}+\frac{11 b-2}{1+b^2}+\frac{11 c-2}{1+c^2} \leq C.
$$

## Query

Task description: Please solve the problem with clear, rigorous, and logically sound steps. At the end of your response, state your answer in exactly this format: 'The answer is $C=X$', where X is your calculated numerical bound value. Example: 'The answer is $C=1$'.

Problem: Let $a, b, c$ be real numbers such that $a+b+c=1$. Find the smallest constant $C$ such that the following inequality holds for all $a, b, c$ satisfying the given constraint:
$$
\frac{11 a-2}{1+a^2}+\frac{11 b-2}{1+b^2}+\frac{11 c-2}{1+c^2} \leq C.
$$

Solution:

## Response

To solve this problem, we need to find the smallest constant \( C \) such that the inequality

\[
\frac{11a - 2}{1 + a^2} + \frac{11b - 2}{1 + b^2} + \frac{11c - 2}{1 + c^2} \leq C
\]

holds for all real numbers \( a, b, c \) satisfying \( a + b + c = 1 \).

### Step 1: Analyze the function

Consider the function \( f(x) = \frac{11x - 2}{1 + x^2} \). We need to understand its behavior to find the maximum possible value of the sum.

#### Derivative and Critical Points

First, compute the derivative of \( f(x) \):

\[
f'(x) = \frac{(1 + x^2)(11) - (11x - 2)(2x)}{(1 + x^2)^2} = \frac{11 + 11x^2 - 22x^2 + 4x}{(1 + x^2)^2} = \frac{11 - 11x^2 + 4x}{(1 + x^2)^2}
\]

Set \( f'(x) = 0 \) to find critical points:

\[
11 - 11x^2 + 4x = 0 \quad \Rightarrow \quad 11x^2 - 4x - 11 = 0
\]

Using the quadratic formula, \( x = \frac{-b \pm \sqrt{b^2 - 4ac}}{2a} \), we find:

\[
x = \frac{4 \pm \sqrt{16 + 484}}{22} = \frac{4 \pm \sqrt{500}}{22} = \frac{4 \pm 10\sqrt{5}}{22} = \frac{2 \pm 5\sqrt{5}}{11}
\]

These are the critical points. Evaluate \( f(x) \) at these points and at the boundaries as \( x \to \pm \infty \).

#### Behavior at Infinity

As \( x \to \pm \infty \), \( f(x) \to 0 \).

#### Evaluate at Critical Points

Calculate \( f(x) \) at \( x = \frac{2 + 5\sqrt{5}}{11} \) and \( x = \frac{2 - 5\sqrt{5}}{11} \).

### Step 2: Symmetry and Simplification

Since \( a + b + c = 1 \), consider symmetric cases like \( a = b = c = \frac{1}{3} \).

\[
f\left(\frac{1}{3}\right) = \frac{11 \cdot \frac{1}{3} - 2}{1 + \left(\frac{1}{3}\right)^2} = \frac{\frac{11}{3} - 2}{1 + \frac{1}{9}} = \frac{\frac{5}{3}}{\frac{10}{9}} = \frac{5}{3} \cdot \frac{9}{10} = \frac{3}{2}
\]

Thus, the sum is:

\[
3 \cdot \frac{3}{2} = \frac{9}{2} = 4.5
\]

### Step 3: Conclusion

The maximum value of the sum \( \frac{11a - 2}{1 + a^2} + \frac{11b - 2}{1 + b^2} + \frac{11c - 2}{1 + c^2} \) is achieved when \( a = b = c = \frac{1}{3} \), and it equals \( 4.5 \).

Thus, the smallest constant \( C \) such that the inequality holds for all \( a, b, c \) satisfying \( a + b + c = 1 \) is:

\[
\boxed{4.5}
\]

The answer is \( C = 4.5 \).