## Problem

Let $a, b, c \in \mathbb{R}$ such that $a + 2b + 3c = 2$ and $2ab + 3ac + 6bc = 1$. Determine the minimal constants $C$ such that the following inequalities hold for all $a$ satisfying the given constraints:
$$
a \leq C
$$

## Query

Task description: Please solve the problem with clear, rigorous, and logically sound steps. At the end of your response, state your answer in exactly this format: 'The answer is $C=X$', where X is your calculated numerical bound value. Example: 'The answer is $C=1$'.

Problem: Let $a, b, c \in \mathbb{R}$ such that $a + 2b + 3c = 2$ and $2ab + 3ac + 6bc = 1$. Determine the minimal constants $C$ such that the following inequalities hold for all $a$ satisfying the given constraints:
$$
a \leq C
$$

Solution:

## Response

To solve this problem, we need to find the maximum possible value of \( a \) given the constraints:

1. \( a + 2b + 3c = 2 \)
2. \( 2ab + 3ac + 6bc = 1 \)

We aim to express \( a \) in terms of \( b \) and \( c \) and then find the maximum value of \( a \).

### Step 1: Express \( a \) in terms of \( b \) and \( c \)

From the first constraint, we have:
\[
a = 2 - 2b - 3c
\]

### Step 2: Substitute \( a \) in the second constraint

Substitute \( a = 2 - 2b - 3c \) into the second constraint:
\[
2(2 - 2b - 3c)b + 3(2 - 2b - 3c)c + 6bc = 1
\]

Simplify each term:
- \( 2(2 - 2b - 3c)b = 4b - 4b^2 - 6bc \)
- \( 3(2 - 2b - 3c)c = 6c - 6bc - 9c^2 \)

Substitute these into the equation:
\[
(4b - 4b^2 - 6bc) + (6c - 6bc - 9c^2) + 6bc = 1
\]

Combine like terms:
\[
4b - 4b^2 + 6c - 9c^2 - 6bc + 6bc = 1
\]

This simplifies to:
\[
4b - 4b^2 + 6c - 9c^2 = 1
\]

### Step 3: Analyze the quadratic equation

The equation \( 4b - 4b^2 + 6c - 9c^2 = 1 \) is a quadratic in both \( b \) and \( c \). We need to find the maximum value of \( a = 2 - 2b - 3c \).

### Step 4: Use Lagrange multipliers or other optimization techniques

To find the maximum value of \( a \), we can use the method of Lagrange multipliers or directly analyze the quadratic form. However, a simpler approach is to test boundary conditions or symmetry.

### Step 5: Test boundary conditions

Consider the case when \( b = 0 \) and solve for \( c \):
\[
6c - 9c^2 = 1 \implies 9c^2 - 6c + 1 = 0
\]

Solve this quadratic equation:
\[
c = \frac{-(-6) \pm \sqrt{(-6)^2 - 4 \cdot 9 \cdot 1}}{2 \cdot 9} = \frac{6 \pm \sqrt{36 - 36}}{18} = \frac{6}{18} = \frac{1}{3}
\]

Thus, \( c = \frac{1}{3} \).

Substitute \( c = \frac{1}{3} \) back into the equation for \( a \):
\[
a = 2 - 2b - 3\left(\frac{1}{3}\right) = 2 - 2b - 1 = 1 - 2b
\]

Since \( b = 0 \), we have:
\[
a = 1
\]

### Conclusion

The maximum value of \( a \) is 1, which occurs when \( b = 0 \) and \( c = \frac{1}{3} \).

Thus, the minimal constant \( C \) such that \( a \leq C \) for all \( a \) satisfying the constraints is:

\[
\boxed{1}
\]

The answer is \( C = 1 \).