## Problem

Let $a, b, c \geq 0$ and $a+b+c=1$. Determine the minimal constant $C$ such that the following inequality holds for all $a, b, c$:

$$
\frac{a}{\sqrt{b^2+3 c}}+\frac{b}{\sqrt{c^2+3 a}}+\frac{c}{\sqrt{a^2+3 b}} \geq \frac{1}{\sqrt{1+2C a b c}}.
$$

## Query

Task description: Please solve the problem with clear, rigorous, and logically sound steps. At the end of your response, state your answer in exactly this format: 'The answer is $C=X$', where X is your calculated numerical bound value. Example: 'The answer is $C=1$'.

Problem: Let $a, b, c \geq 0$ and $a+b+c=1$. Determine the minimal constant $C$ such that the following inequality holds for all $a, b, c$:

$$
\frac{a}{\sqrt{b^2+3 c}}+\frac{b}{\sqrt{c^2+3 a}}+\frac{c}{\sqrt{a^2+3 b}} \geq \frac{1}{\sqrt{1+2C a b c}}.
$$

Solution:

## Response

To solve this problem, we need to find the minimal constant \( C \) such that the inequality

\[
\frac{a}{\sqrt{b^2+3c}} + \frac{b}{\sqrt{c^2+3a}} + \frac{c}{\sqrt{a^2+3b}} \geq \frac{1}{\sqrt{1+2Cabc}}
\]

holds for all non-negative \( a, b, c \) with \( a + b + c = 1 \).

### Step 1: Analyze the inequality

First, consider the case where one of the variables is zero, say \( c = 0 \). Then \( a + b = 1 \) and the inequality becomes:

\[
\frac{a}{\sqrt{b^2}} + \frac{b}{\sqrt{3a}} \geq 1.
\]

This simplifies to:

\[
\frac{a}{b} + \frac{b}{\sqrt{3a}} \geq 1.
\]

### Step 2: Test specific cases

#### Case 1: \( a = 1, b = 0, c = 0 \)

The left-hand side becomes:

\[
\frac{1}{\sqrt{0^2 + 3 \cdot 0}} = \infty,
\]

which trivially satisfies the inequality for any \( C \).

#### Case 2: \( a = b = \frac{1}{2}, c = 0 \)

The left-hand side becomes:

\[
\frac{\frac{1}{2}}{\left(\frac{1}{2}\right)} + \frac{\frac{1}{2}}{\sqrt{3 \cdot \frac{1}{2}}} = 1 + \frac{1}{\sqrt{\frac{3}{2}}} = 1 + \sqrt{\frac{2}{3}}.
\]

The right-hand side is:

\[
\frac{1}{\sqrt{1 + 0}} = 1.
\]

Since \( 1 + \sqrt{\frac{2}{3}} > 1 \), the inequality holds.

### Step 3: Consider the symmetric case

For \( a = b = c = \frac{1}{3} \), the left-hand side becomes:

\[
3 \cdot \frac{\frac{1}{3}}{\sqrt{\left(\frac{1}{3}\right)^2 + 3 \cdot \frac{1}{3}}} = \frac{1}{\sqrt{\frac{1}{9} + 1}} = \frac{1}{\sqrt{\frac{10}{9}}} = \frac{3}{\sqrt{10}}.
\]

The right-hand side is:

\[
\frac{1}{\sqrt{1 + 2C \left(\frac{1}{3}\right)^3}} = \frac{1}{\sqrt{1 + \frac{2C}{27}}}.
\]

We need:

\[
\frac{3}{\sqrt{10}} \geq \frac{1}{\sqrt{1 + \frac{2C}{27}}}.
\]

Squaring both sides:

\[
\frac{9}{10} \geq \frac{1}{1 + \frac{2C}{27}}.
\]

Cross-multiplying gives:

\[
9 + \frac{18C}{27} \leq 10.
\]

Simplifying:

\[
\frac{18C}{27} \leq 1 \quad \Rightarrow \quad \frac{2C}{3} \leq 1 \quad \Rightarrow \quad C \leq \frac{3}{2}.
\]

### Conclusion

The minimal constant \( C \) such that the inequality holds for all non-negative \( a, b, c \) with \( a + b + c = 1 \) is \( C = \frac{3}{2} \).

The answer is \( C = \frac{3}{2} \).