## Problem

Find the smallest constant $C$ such that for all non-negative real numbers $a, b, c$, the following inequality holds:
$$
\sqrt{\frac{a b+b c+c a}{3}} \leq C \cdot \sqrt[3]{\frac{(a+b)(b+c)(c+a)}{2}}
$$

## Query

Task description: Please solve the problem with clear, rigorous, and logically sound steps. At the end of your response, state your answer in exactly this format: 'The answer is $C=X$', where X is your calculated numerical bound value. Example: 'The answer is $C=1$'.

Problem: Find the smallest constant $C$ such that for all non-negative real numbers $a, b, c$, the following inequality holds:
$$
\sqrt{\frac{a b+b c+c a}{3}} \leq C \cdot \sqrt[3]{\frac{(a+b)(b+c)(c+a)}{2}}
$$

Solution:

## Response

To solve this problem, we need to find the smallest constant \( C \) such that the inequality

\[
\sqrt{\frac{ab + bc + ca}{3}} \leq C \cdot \sqrt[3]{\frac{(a+b)(b+c)(c+a)}{2}}
\]

holds for all non-negative real numbers \( a, b, c \).

### Step 1: Analyze the inequality

First, let's rewrite the inequality in a more manageable form:

\[
\frac{ab + bc + ca}{3} \leq C^2 \cdot \left(\frac{(a+b)(b+c)(c+a)}{2}\right)^{2/3}
\]

### Step 2: Consider special cases

#### Case 1: \( a = b = c \)

If \( a = b = c \), then both sides of the inequality become equal:

- Left side: \(\frac{ab + bc + ca}{3} = \frac{3a^2}{3} = a^2\).
- Right side: \(\left(\frac{(a+a)(a+a)(a+a)}{2}\right)^{2/3} = \left(\frac{8a^3}{2}\right)^{2/3} = (4a^3)^{2/3} = 4^{2/3}a^2\).

Thus, the inequality becomes:

\[
a^2 \leq C^2 \cdot 4^{2/3} a^2
\]

This simplifies to:

\[
1 \leq C^2 \cdot 4^{2/3}
\]

So, \( C^2 \geq 4^{-2/3} \).

#### Case 2: \( a = 1, b = 1, c = 0 \)

- Left side: \(\frac{ab + bc + ca}{3} = \frac{1 \cdot 1 + 1 \cdot 0 + 0 \cdot 1}{3} = \frac{1}{3}\).
- Right side: \(\left(\frac{(1+1)(1+0)(0+1)}{2}\right)^{2/3} = \left(\frac{2 \cdot 1 \cdot 1}{2}\right)^{2/3} = 1^{2/3} = 1\).

The inequality becomes:

\[
\frac{1}{3} \leq C^2
\]

So, \( C^2 \geq \frac{1}{3} \).

### Step 3: Determine the smallest \( C \)

From the two cases, we have:

- \( C^2 \geq 4^{-2/3} \)
- \( C^2 \geq \frac{1}{3} \)

Calculate \( 4^{-2/3} \):

\[
4^{-2/3} = \left(2^2\right)^{-2/3} = 2^{-4/3} = \frac{1}{2^{4/3}}
\]

Now, compare \( \frac{1}{2^{4/3}} \) and \( \frac{1}{3} \):

- \( 2^{4/3} \approx 2.5198421 \)
- \( \frac{1}{2^{4/3}} \approx 0.39685026 \)
- \( \frac{1}{3} \approx 0.33333333 \)

Since \( \frac{1}{3} < \frac{1}{2^{4/3}} \), the larger bound is \( \frac{1}{3} \).

Thus, the smallest \( C \) is:

\[
C = \sqrt{\frac{1}{3}}
\]

Therefore, the smallest constant \( C \) is:

\[
C = \frac{1}{\sqrt{3}}
\]

The answer is \(\boxed{C = \frac{1}{\sqrt{3}}}\).