## Problem

Let $a, b, c > 0$ satisfy $a + b + c = 3$. Find the largest constant $C$ such that the following inequality holds for all $a, b, c$:
$$
\sqrt[3]{a^2 + ab + bc} + \sqrt[3]{b^2 + bc + ca} + \sqrt[3]{c^2 + ca + ab} \geq C(ab + bc + ca).
$$

## Query

Task description: Please solve the problem with clear, rigorous, and logically sound steps. At the end of your response, state your answer in exactly this format: 'The answer is $C=X$', where X is your calculated numerical bound value. Example: 'The answer is $C=1$'.

Problem: Let $a, b, c > 0$ satisfy $a + b + c = 3$. Find the largest constant $C$ such that the following inequality holds for all $a, b, c$:
$$
\sqrt[3]{a^2 + ab + bc} + \sqrt[3]{b^2 + bc + ca} + \sqrt[3]{c^2 + ca + ab} \geq C(ab + bc + ca).
$$

Solution:

## Response

To solve this problem, we need to find the largest constant \( C \) such that the inequality

\[
\sqrt[3]{a^2 + ab + bc} + \sqrt[3]{b^2 + bc + ca} + \sqrt[3]{c^2 + ca + ab} \geq C(ab + bc + ca)
\]

holds for all positive \( a, b, c \) satisfying \( a + b + c = 3 \).

### Step 1: Analyze the Expression

First, consider the expression inside each cube root:

- \( a^2 + ab + bc \)
- \( b^2 + bc + ca \)
- \( c^2 + ca + ab \)

These expressions are symmetric in nature and involve combinations of squares and products of the variables.

### Step 2: Test Simple Cases

Let's test the inequality with simple cases to gain insight into the possible value of \( C \).

#### Case 1: \( a = b = c = 1 \)

In this case, \( a + b + c = 3 \) and \( ab + bc + ca = 3 \).

The left-hand side becomes:

\[
\sqrt[3]{1^2 + 1 \cdot 1 + 1 \cdot 1} + \sqrt[3]{1^2 + 1 \cdot 1 + 1 \cdot 1} + \sqrt[3]{1^2 + 1 \cdot 1 + 1 \cdot 1} = 3 \sqrt[3]{3}
\]

The right-hand side is:

\[
C \cdot 3
\]

For the inequality to hold, we need:

\[
3 \sqrt[3]{3} \geq 3C \quad \Rightarrow \quad \sqrt[3]{3} \geq C
\]

#### Case 2: \( a = 2, b = 1, c = 0 \)

In this case, \( a + b + c = 3 \) and \( ab + bc + ca = 2 \).

The left-hand side becomes:

\[
\sqrt[3]{2^2 + 2 \cdot 1 + 1 \cdot 0} + \sqrt[3]{1^2 + 1 \cdot 0 + 0 \cdot 2} + \sqrt[3]{0^2 + 0 \cdot 2 + 2 \cdot 1} = \sqrt[3]{6} + 1 + \sqrt[3]{2}
\]

The right-hand side is:

\[
2C
\]

For the inequality to hold, we need:

\[
\sqrt[3]{6} + 1 + \sqrt[3]{2} \geq 2C
\]

### Step 3: Determine the Largest \( C \)

From the first case, we have \( C \leq \sqrt[3]{3} \).

From the second case, we need to check if \( C = \sqrt[3]{3} \) satisfies the inequality:

\[
\sqrt[3]{6} + 1 + \sqrt[3]{2} \geq 2 \sqrt[3]{3}
\]

Numerically, we find:

- \( \sqrt[3]{6} \approx 1.817 \)
- \( \sqrt[3]{2} \approx 1.260 \)
- \( \sqrt[3]{3} \approx 1.442 \)

Thus:

\[
1.817 + 1 + 1.260 \approx 4.077
\]

And:

\[
2 \times 1.442 \approx 2.884
\]

Since \( 4.077 \geq 2.884 \), the inequality holds for \( C = \sqrt[3]{3} \).

### Conclusion

The largest constant \( C \) such that the inequality holds for all positive \( a, b, c \) with \( a + b + c = 3 \) is:

\[
\boxed{\sqrt[3]{3}}
\]

Thus, the answer is \( C = \sqrt[3]{3} \).