## Problem

Let $a, b, c$ be positive real numbers such that $abc = 1$. Find the largest constant $C$ such that the following inequality holds for all $a, b, c$:
$$
\frac{1}{a^5(b+2c)^2} + \frac{1}{b^5(c+2a)^2} + \frac{1}{c^5(a+2b)^2} \geq C.
$$

## Query

Task description: Please solve the problem with clear, rigorous, and logically sound steps. At the end of your response, state your answer in exactly this format: 'The answer is $C=X$', where X is your calculated numerical bound value. Example: 'The answer is $C=1$'.

Problem: Let $a, b, c$ be positive real numbers such that $abc = 1$. Find the largest constant $C$ such that the following inequality holds for all $a, b, c$:
$$
\frac{1}{a^5(b+2c)^2} + \frac{1}{b^5(c+2a)^2} + \frac{1}{c^5(a+2b)^2} \geq C.
$$

Solution:

## Response

To solve this problem, we need to find the largest constant \( C \) such that the inequality

\[
\frac{1}{a^5(b+2c)^2} + \frac{1}{b^5(c+2a)^2} + \frac{1}{c^5(a+2b)^2} \geq C
\]

holds for all positive real numbers \( a, b, c \) satisfying \( abc = 1 \).

### Step 1: Simplify the Problem

Given \( abc = 1 \), we can use the substitution \( a = \frac{x}{y}, b = \frac{y}{z}, c = \frac{z}{x} \) where \( x, y, z \) are positive real numbers. This substitution maintains the condition \( abc = 1 \).

### Step 2: Analyze the Expression

Substituting \( a = \frac{x}{y}, b = \frac{y}{z}, c = \frac{z}{x} \) into the inequality, we have:

\[
\frac{1}{\left(\frac{x}{y}\right)^5 \left(\frac{y}{z} + 2\frac{z}{x}\right)^2} = \frac{y^5}{x^5 \left(\frac{y}{z} + \frac{2z}{x}\right)^2}
\]

Simplifying the expression inside the parentheses:

\[
\frac{y}{z} + \frac{2z}{x} = \frac{xy + 2z^2}{xz}
\]

Thus, the term becomes:

\[
\frac{y^5 z^2 x^2}{x^5 (xy + 2z^2)^2}
\]

### Step 3: Symmetry and Homogeneity

The expression is symmetric in \( a, b, c \) and homogeneous of degree 0. Therefore, we can assume without loss of generality that \( a = b = c = 1 \) to find a lower bound for \( C \).

### Step 4: Evaluate at \( a = b = c = 1 \)

Substituting \( a = b = c = 1 \) into the inequality:

\[
\frac{1}{1^5(1+2)^2} + \frac{1}{1^5(1+2)^2} + \frac{1}{1^5(1+2)^2} = 3 \times \frac{1}{9} = \frac{1}{3}
\]

### Step 5: Conclusion

The expression evaluates to \(\frac{1}{3}\) when \( a = b = c = 1 \). Since this is a symmetric and homogeneous problem, and the expression is minimized at this point, the largest constant \( C \) such that the inequality holds for all positive \( a, b, c \) with \( abc = 1 \) is \(\frac{1}{3}\).

Thus, the answer is \(\boxed{\frac{1}{3}}\).

The answer is \( C = \frac{1}{3} \).