## Problem

Let $a, b, c > 0$ such that $abc = 1$. Determine the minimal constant $C$ such that the following inequality holds for all $a, b, c$:

$$
\left(\frac{a+b+c}{3}\right)^{C} \geq \frac{a^2+b^2+c^2}{3}
$$

## Query

Task description: Please solve the problem with clear, rigorous, and logically sound steps. At the end of your response, state your answer in exactly this format: 'The answer is $C=X$', where X is your calculated numerical bound value. Example: 'The answer is $C=1$'.

Problem: Let $a, b, c > 0$ such that $abc = 1$. Determine the minimal constant $C$ such that the following inequality holds for all $a, b, c$:

$$
\left(\frac{a+b+c}{3}\right)^{C} \geq \frac{a^2+b^2+c^2}{3}
$$

Solution:

## Response

To solve this problem, we need to find the minimal constant \( C \) such that the inequality

\[
\left(\frac{a+b+c}{3}\right)^{C} \geq \frac{a^2+b^2+c^2}{3}
\]

holds for all positive \( a, b, c \) with the condition \( abc = 1 \).

### Step 1: Analyze the inequality

First, note that by the AM-GM inequality, we have:

\[
\frac{a+b+c}{3} \geq \sqrt[3]{abc} = 1
\]

Thus, \(\left(\frac{a+b+c}{3}\right)^{C} \geq 1\).

### Step 2: Consider equality conditions

The equality in AM-GM occurs when \( a = b = c = 1 \). In this case, both sides of the inequality become:

\[
\left(\frac{1+1+1}{3}\right)^{C} = 1 \quad \text{and} \quad \frac{1^2 + 1^2 + 1^2}{3} = 1
\]

Thus, the inequality holds with equality when \( a = b = c = 1 \).

### Step 3: Test specific values

To find the minimal \( C \), consider the case where two variables are equal and the third is determined by the condition \( abc = 1 \). Let \( a = b = t \) and \( c = \frac{1}{t^2} \).

Then:

\[
a + b + c = 2t + \frac{1}{t^2}
\]

\[
a^2 + b^2 + c^2 = 2t^2 + \frac{1}{t^4}
\]

The inequality becomes:

\[
\left(\frac{2t + \frac{1}{t^2}}{3}\right)^{C} \geq \frac{2t^2 + \frac{1}{t^4}}{3}
\]

### Step 4: Simplify and analyze

For large \( t \), the left side behaves as \(\left(\frac{2t}{3}\right)^{C}\) and the right side as \(\frac{2t^2}{3}\). We need:

\[
\left(\frac{2t}{3}\right)^{C} \geq \frac{2t^2}{3}
\]

Taking logarithms and simplifying, we find:

\[
C \log\left(\frac{2t}{3}\right) \geq \log\left(\frac{2t^2}{3}\right)
\]

\[
C \log(2t) - C \log(3) \geq \log(2) + 2\log(t) - \log(3)
\]

For large \( t \), the dominant term is \( C \log(t) \geq 2 \log(t) \), which implies \( C \geq 2 \).

### Step 5: Verify \( C = 2 \)

If \( C = 2 \), the inequality becomes:

\[
\left(\frac{a+b+c}{3}\right)^{2} \geq \frac{a^2+b^2+c^2}{3}
\]

This is equivalent to:

\[
(a+b+c)^2 \geq 3(a^2+b^2+c^2)
\]

Expanding both sides:

\[
a^2 + b^2 + c^2 + 2(ab + bc + ca) \geq 3(a^2 + b^2 + c^2)
\]

Simplifying:

\[
2(ab + bc + ca) \geq 2(a^2 + b^2 + c^2)
\]

\[
ab + bc + ca \geq a^2 + b^2 + c^2
\]

This inequality holds by the rearrangement inequality or by AM-GM, confirming that \( C = 2 \) is valid.

Thus, the minimal constant \( C \) is:

\[
\boxed{2}
\]

The answer is \( C = 2 \).