## Problem

Let $0 < a < b$ and $x_i \in [a, b]$. Determine the largest constant $C$ such that the following inequality holds for all $x_i$:

$$
\left(x_1+x_2+\ldots+x_n\right)\left(\frac{1}{x_1}+\frac{1}{x_2}+\ldots+\frac{1}{x_n}\right) \leq \frac{n^2(a+b)^2}{Cab}.
$$

## Query

Task description: Please solve the problem with clear, rigorous, and logically sound steps. At the end of your response, state your answer in exactly this format: 'The answer is $C=X$', where X is your calculated numerical bound value. Example: 'The answer is $C=1$'.

Problem: Let $0 < a < b$ and $x_i \in [a, b]$. Determine the largest constant $C$ such that the following inequality holds for all $x_i$:

$$
\left(x_1+x_2+\ldots+x_n\right)\left(\frac{1}{x_1}+\frac{1}{x_2}+\ldots+\frac{1}{x_n}\right) \leq \frac{n^2(a+b)^2}{Cab}.
$$

Solution:

## Response

To solve this problem, we need to find the largest constant \( C \) such that the inequality

\[
\left(x_1 + x_2 + \ldots + x_n\right)\left(\frac{1}{x_1} + \frac{1}{x_2} + \ldots + \frac{1}{x_n}\right) \leq \frac{n^2(a+b)^2}{Cab}
\]

holds for all \( x_i \in [a, b] \).

### Step 1: Analyze the Left-Hand Side

The left-hand side of the inequality is:

\[
S = \left(x_1 + x_2 + \ldots + x_n\right)\left(\frac{1}{x_1} + \frac{1}{x_2} + \ldots + \frac{1}{x_n}\right).
\]

By the Cauchy-Schwarz inequality, we have:

\[
\left(x_1 + x_2 + \ldots + x_n\right)\left(\frac{1}{x_1} + \frac{1}{x_2} + \ldots + \frac{1}{x_n}\right) \geq n^2.
\]

This gives us a lower bound for \( S \).

### Step 2: Find the Upper Bound for \( S \)

To find the maximum value of \( S \), consider the case where \( x_1 = x_2 = \ldots = x_n = a \) and \( x_1 = x_2 = \ldots = x_n = b \).

1. **Case \( x_1 = x_2 = \ldots = x_n = a \):**

   \[
   S = n \cdot a \cdot \frac{n}{a} = n^2.
   \]

2. **Case \( x_1 = x_2 = \ldots = x_n = b \):**

   \[
   S = n \cdot b \cdot \frac{n}{b} = n^2.
   \]

3. **Mixed Case:**

   Consider \( x_1 = a \) and \( x_2 = x_3 = \ldots = x_n = b \):

   \[
   S = (a + (n-1)b)\left(\frac{1}{a} + \frac{n-1}{b}\right).
   \]

   Simplifying, we get:

   \[
   S = (a + (n-1)b)\left(\frac{b + (n-1)a}{ab}\right) = \frac{(a + (n-1)b)(b + (n-1)a)}{ab}.
   \]

   Expanding the terms:

   \[
   (a + (n-1)b)(b + (n-1)a) = ab + (n-1)a^2 + (n-1)b^2 + (n-1)^2ab.
   \]

   Simplifying further:

   \[
   = ab + (n-1)(a^2 + b^2) + (n-1)^2ab.
   \]

   \[
   = ab(1 + (n-1)^2) + (n-1)(a^2 + b^2).
   \]

   The maximum value of \( S \) occurs when \( x_i \) are at the extremes \( a \) and \( b \).

### Step 3: Determine the Constant \( C \)

The inequality we want to satisfy is:

\[
n^2 \leq \frac{n^2(a+b)^2}{Cab}.
\]

Rearranging gives:

\[
Cab \leq (a+b)^2.
\]

Thus, the largest \( C \) is:

\[
C = \frac{(a+b)^2}{ab}.
\]

Therefore, the answer is \(\boxed{C = \frac{(a+b)^2}{ab}}\).