## Problem

Let $x \geq y \geq z \geq 0$. Find the largest constant $C$ such that the following inequality holds for all $x, y, z$:
$$
\frac{x^2 y}{z}+\frac{y^2 z}{x}+\frac{z^2 x}{y} \geq C(x^2+y^2+z^2)
$$

## Query

Task description: Please solve the problem with clear, rigorous, and logically sound steps. At the end of your response, state your answer in exactly this format: 'The answer is $C=X$', where X is your calculated numerical bound value. Example: 'The answer is $C=1$'.

Problem: Let $x \geq y \geq z \geq 0$. Find the largest constant $C$ such that the following inequality holds for all $x, y, z$:
$$
\frac{x^2 y}{z}+\frac{y^2 z}{x}+\frac{z^2 x}{y} \geq C(x^2+y^2+z^2)
$$

Solution:

## Response

To solve this problem, we need to find the largest constant \( C \) such that the inequality

\[
\frac{x^2 y}{z} + \frac{y^2 z}{x} + \frac{z^2 x}{y} \geq C(x^2 + y^2 + z^2)
\]

holds for all \( x \geq y \geq z \geq 0 \).

### Step 1: Analyze the inequality

First, let's consider the case where \( x = y = z \). In this scenario, the inequality becomes:

\[
\frac{x^3}{x} + \frac{x^3}{x} + \frac{x^3}{x} = 3x^2 \geq C(3x^2)
\]

This simplifies to \( 3 \geq 3C \), which implies \( C \leq 1 \).

### Step 2: Consider extreme cases

To find the largest possible \( C \), consider the case where \( x \) is much larger than \( y \) and \( z \), specifically \( x \to \infty \) and \( y, z \to 0 \). In this case, the left-hand side of the inequality becomes:

\[
\frac{x^2 y}{z} + \frac{y^2 z}{x} + \frac{z^2 x}{y} \approx \frac{x^2 y}{z}
\]

The right-hand side becomes:

\[
C(x^2 + y^2 + z^2) \approx Cx^2
\]

For the inequality to hold, we need:

\[
\frac{x^2 y}{z} \geq Cx^2
\]

This simplifies to:

\[
\frac{y}{z} \geq C
\]

Since \( y \geq z \), we have \( \frac{y}{z} \geq 1 \). Therefore, \( C \leq 1 \).

### Step 3: Verify \( C = 1 \)

Now, let's verify if \( C = 1 \) satisfies the inequality for all \( x \geq y \geq z \geq 0 \). The inequality becomes:

\[
\frac{x^2 y}{z} + \frac{y^2 z}{x} + \frac{z^2 x}{y} \geq x^2 + y^2 + z^2
\]

Rearranging gives:

\[
\frac{x^2 y}{z} + \frac{y^2 z}{x} + \frac{z^2 x}{y} - x^2 - y^2 - z^2 \geq 0
\]

This can be rewritten as:

\[
\frac{x^2 y}{z} - x^2 + \frac{y^2 z}{x} - y^2 + \frac{z^2 x}{y} - z^2 \geq 0
\]

Or:

\[
x^2 \left(\frac{y}{z} - 1\right) + y^2 \left(\frac{z}{x} - 1\right) + z^2 \left(\frac{x}{y} - 1\right) \geq 0
\]

Since \( x \geq y \geq z \), we have \( \frac{y}{z} \geq 1 \), \( \frac{z}{x} \leq 1 \), and \( \frac{x}{y} \geq 1 \). Therefore, each term is non-negative, and the inequality holds.

Thus, the largest constant \( C \) for which the inequality holds for all \( x \geq y \geq z \geq 0 \) is indeed \( C = 1 \).

The answer is \(\boxed{C=1}\).