## Problem

Let $0 \leq x \leq 1$ and $n \in \mathbb{N}$. Find the smallest constant $C$ such that the following inequality holds for all $x$ and $n$:
$$
\left(1-x+\frac{x^2}{2}\right)^n-(1-x)^n \leq Cx.
$$

## Query

Task description: Please solve the problem with clear, rigorous, and logically sound steps. At the end of your response, state your answer in exactly this format: 'The answer is $C=X$', where X is your calculated numerical bound value. Example: 'The answer is $C=1$'.

Problem: Let $0 \leq x \leq 1$ and $n \in \mathbb{N}$. Find the smallest constant $C$ such that the following inequality holds for all $x$ and $n$:
$$
\left(1-x+\frac{x^2}{2}\right)^n-(1-x)^n \leq Cx.
$$

Solution:

## Response

To solve this problem, we need to find the smallest constant \( C \) such that the inequality

\[
\left(1-x+\frac{x^2}{2}\right)^n-(1-x)^n \leq Cx
\]

holds for all \( 0 \leq x \leq 1 \) and \( n \in \mathbb{N} \).

### Step 1: Expand the expressions

First, consider the binomial expansions of both terms:

1. \((1-x)^n\) can be expanded using the binomial theorem:

\[
(1-x)^n = \sum_{k=0}^{n} \binom{n}{k} (-x)^k = \sum_{k=0}^{n} \binom{n}{k} (-1)^k x^k.
\]

2. \(\left(1-x+\frac{x^2}{2}\right)^n\) can also be expanded using the binomial theorem:

\[
\left(1-x+\frac{x^2}{2}\right)^n = \sum_{k=0}^{n} \binom{n}{k} \left(-x+\frac{x^2}{2}\right)^k.
\]

### Step 2: Simplify the difference

We are interested in the difference:

\[
\left(1-x+\frac{x^2}{2}\right)^n - (1-x)^n.
\]

For small \( x \), we can approximate the terms:

- \((1-x)^n \approx 1 - nx + \frac{n(n-1)}{2}x^2\).
- \(\left(1-x+\frac{x^2}{2}\right)^n \approx 1 - nx + \frac{n(n-1)}{2}x^2 + \frac{n}{2}x^2\).

The difference is:

\[
\left(1-x+\frac{x^2}{2}\right)^n - (1-x)^n \approx \frac{n}{2}x^2.
\]

### Step 3: Bound the difference

We need to ensure:

\[
\frac{n}{2}x^2 \leq Cx.
\]

This simplifies to:

\[
\frac{n}{2}x \leq C.
\]

For the inequality to hold for all \( 0 \leq x \leq 1 \), the worst-case scenario is when \( x = 1 \). Thus, we have:

\[
\frac{n}{2} \leq C.
\]

### Step 4: Determine the smallest \( C \)

The smallest \( C \) that satisfies this inequality for all \( n \) is:

\[
C = \frac{n}{2}.
\]

However, since \( n \) can be any natural number, we need a constant \( C \) that works for all \( n \). Therefore, the smallest \( C \) that works for all \( n \) is:

\[
C = \frac{1}{2}.
\]

Thus, the smallest constant \( C \) such that the inequality holds for all \( x \) and \( n \) is:

\[
\boxed{\frac{1}{2}}
\]

The answer is \( C = \frac{1}{2} \).