## Problem

Let $a_1, \ldots, a_n, b_1, \ldots, b_n > 0$. Find the smallest constant $C$ such that the following inequality holds for all positive $a_i$ and $b_i$:
$$
\sum_{i=1}^n \frac{a_i b_i}{a_i+b_i} \leq C \cdot \frac{\left(\sum_{i=1}^n a_i\right)\left(\sum_{i=1}^n b_i\right)}{\sum_{i=1}^n\left(a_i+b_i\right)}
$$

## Query

Task description: Please solve the problem with clear, rigorous, and logically sound steps. At the end of your response, state your answer in exactly this format: 'The answer is $C=X$', where X is your calculated numerical bound value. Example: 'The answer is $C=1$'.

Problem: Let $a_1, \ldots, a_n, b_1, \ldots, b_n > 0$. Find the smallest constant $C$ such that the following inequality holds for all positive $a_i$ and $b_i$:
$$
\sum_{i=1}^n \frac{a_i b_i}{a_i+b_i} \leq C \cdot \frac{\left(\sum_{i=1}^n a_i\right)\left(\sum_{i=1}^n b_i\right)}{\sum_{i=1}^n\left(a_i+b_i\right)}
$$

Solution:

## Response

To solve this problem, we need to find the smallest constant \( C \) such that the inequality

\[
\sum_{i=1}^n \frac{a_i b_i}{a_i + b_i} \leq C \cdot \frac{\left(\sum_{i=1}^n a_i\right)\left(\sum_{i=1}^n b_i\right)}{\sum_{i=1}^n (a_i + b_i)}
\]

holds for all positive \( a_i \) and \( b_i \).

### Step 1: Simplify the Problem

First, consider the case when \( n = 1 \). The inequality becomes:

\[
\frac{a_1 b_1}{a_1 + b_1} \leq C \cdot \frac{a_1 b_1}{a_1 + b_1}
\]

This simplifies to \( 1 \leq C \), so \( C \geq 1 \).

### Step 2: Consider the General Case

For \( n \geq 1 \), we need to show that the inequality holds for \( C = 1 \). We want to prove:

\[
\sum_{i=1}^n \frac{a_i b_i}{a_i + b_i} \leq \frac{\left(\sum_{i=1}^n a_i\right)\left(\sum_{i=1}^n b_i\right)}{\sum_{i=1}^n (a_i + b_i)}
\]

### Step 3: Use Cauchy-Schwarz Inequality

Apply the Cauchy-Schwarz inequality in the form:

\[
\left( \sum_{i=1}^n \frac{a_i b_i}{a_i + b_i} \right) \left( \sum_{i=1}^n (a_i + b_i) \right) \geq \left( \sum_{i=1}^n \sqrt{\frac{a_i b_i}{a_i + b_i} \cdot (a_i + b_i)} \right)^2
\]

Simplifying the right side, we have:

\[
\sum_{i=1}^n \sqrt{a_i b_i} = \sum_{i=1}^n \sqrt{a_i} \sqrt{b_i}
\]

By the Cauchy-Schwarz inequality again:

\[
\left( \sum_{i=1}^n \sqrt{a_i} \sqrt{b_i} \right)^2 \leq \left( \sum_{i=1}^n a_i \right) \left( \sum_{i=1}^n b_i \right)
\]

Thus, we have:

\[
\left( \sum_{i=1}^n \frac{a_i b_i}{a_i + b_i} \right) \left( \sum_{i=1}^n (a_i + b_i) \right) \geq \left( \sum_{i=1}^n \sqrt{a_i} \sqrt{b_i} \right)^2 \leq \left( \sum_{i=1}^n a_i \right) \left( \sum_{i=1}^n b_i \right)
\]

This implies:

\[
\sum_{i=1}^n \frac{a_i b_i}{a_i + b_i} \leq \frac{\left( \sum_{i=1}^n a_i \right) \left( \sum_{i=1}^n b_i \right)}{\sum_{i=1}^n (a_i + b_i)}
\]

### Conclusion

The inequality holds for \( C = 1 \), and since we showed \( C \geq 1 \) in the base case, the smallest such constant \( C \) is indeed 1.

The answer is \(\boxed{C=1}\).