## Problem

Let $a, b, c \in \left[\frac{1}{3}, 3\right]$. Find the largest constant $C$ such that the following inequality holds for all $a, b, c$ in the given range:
$$
\frac{a}{a+b}+\frac{b}{b+c}+\frac{c}{c+a} \geq C.
$$

## Query

Task description: Please solve the problem with clear, rigorous, and logically sound steps. At the end of your response, state your answer in exactly this format: 'The answer is $C=X$', where X is your calculated numerical bound value. Example: 'The answer is $C=1$'.

Problem: Let $a, b, c \in \left[\frac{1}{3}, 3\right]$. Find the largest constant $C$ such that the following inequality holds for all $a, b, c$ in the given range:
$$
\frac{a}{a+b}+\frac{b}{b+c}+\frac{c}{c+a} \geq C.
$$

Solution:

## Response

To solve this problem, we need to find the largest constant \( C \) such that the inequality

\[
\frac{a}{a+b} + \frac{b}{b+c} + \frac{c}{c+a} \geq C
\]

holds for all \( a, b, c \in \left[\frac{1}{3}, 3\right] \).

### Step 1: Analyze the Expression

First, observe that each term in the sum is of the form \(\frac{x}{x+y}\), which is always less than 1. Therefore, the sum of the three terms is less than 3. We need to find the minimum value of this sum over the given range.

### Step 2: Consider Symmetric Cases

Consider the symmetric case where \( a = b = c \). In this case, the expression simplifies to:

\[
\frac{a}{a+a} + \frac{a}{a+a} + \frac{a}{a+a} = \frac{1}{2} + \frac{1}{2} + \frac{1}{2} = \frac{3}{2}.
\]

This suggests that the expression can be at least \(\frac{3}{2}\).

### Step 3: Consider Boundary Cases

To ensure that \(\frac{3}{2}\) is indeed the minimum, consider the boundary values of the range. 

1. **Case 1**: \( a = \frac{1}{3}, b = \frac{1}{3}, c = \frac{1}{3} \)

   \[
   \frac{\frac{1}{3}}{\frac{1}{3} + \frac{1}{3}} + \frac{\frac{1}{3}}{\frac{1}{3} + \frac{1}{3}} + \frac{\frac{1}{3}}{\frac{1}{3} + \frac{1}{3}} = \frac{1}{2} + \frac{1}{2} + \frac{1}{2} = \frac{3}{2}.
   \]

2. **Case 2**: \( a = 3, b = 3, c = 3 \)

   \[
   \frac{3}{3+3} + \frac{3}{3+3} + \frac{3}{3+3} = \frac{1}{2} + \frac{1}{2} + \frac{1}{2} = \frac{3}{2}.
   \]

3. **Case 3**: \( a = \frac{1}{3}, b = 3, c = 3 \)

   \[
   \frac{\frac{1}{3}}{\frac{1}{3} + 3} + \frac{3}{3 + 3} + \frac{3}{3 + \frac{1}{3}} = \frac{\frac{1}{3}}{\frac{10}{3}} + \frac{1}{2} + \frac{3}{\frac{10}{3}} = \frac{1}{10} + \frac{1}{2} + \frac{9}{10} = \frac{1}{10} + \frac{5}{10} + \frac{9}{10} = \frac{15}{10} = \frac{3}{2}.
   \]

### Step 4: Conclusion

In all these cases, the expression evaluates to \(\frac{3}{2}\). Since we have checked both symmetric and boundary cases, and the expression does not drop below \(\frac{3}{2}\), we conclude that the largest constant \( C \) for which the inequality holds for all \( a, b, c \in \left[\frac{1}{3}, 3\right] \) is \(\frac{3}{2}\).

Thus, the answer is \(\boxed{\frac{3}{2}}\).

The answer is \( C = \frac{3}{2} \).