## Problem

Let $x, y, z$ be real numbers such that $x+y+z=xyz$. Find the largest constant $C$ such that the following inequality holds for all $x, y, z$ satisfying the given constraint:
$$
\frac{1}{1+x^2}+\frac{1}{1+y^2}+\frac{1}{1+z^2} \geq C.
$$

## Query

Task description: Please solve the problem with clear, rigorous, and logically sound steps. At the end of your response, state your answer in exactly this format: 'The answer is $C=X$', where X is your calculated numerical bound value. Example: 'The answer is $C=1$'.

Problem: Let $x, y, z$ be real numbers such that $x+y+z=xyz$. Find the largest constant $C$ such that the following inequality holds for all $x, y, z$ satisfying the given constraint:
$$
\frac{1}{1+x^2}+\frac{1}{1+y^2}+\frac{1}{1+z^2} \geq C.
$$

Solution:

## Response

To solve this problem, we need to find the largest constant \( C \) such that the inequality

\[
\frac{1}{1+x^2} + \frac{1}{1+y^2} + \frac{1}{1+z^2} \geq C
\]

holds for all real numbers \( x, y, z \) satisfying \( x+y+z = xyz \).

### Step 1: Analyze the Constraint

The condition \( x+y+z = xyz \) can be rewritten as:

\[
xyz - x - y - z = 0.
\]

This equation is symmetric in \( x, y, z \).

### Step 2: Consider Special Cases

Let's consider the case where \( x = y = z \). Then the condition becomes:

\[
3x = x^3 \quad \Rightarrow \quad x^3 - 3x = 0 \quad \Rightarrow \quad x(x^2 - 3) = 0.
\]

This gives solutions \( x = 0 \) or \( x = \pm\sqrt{3} \).

#### Case 1: \( x = y = z = 0 \)

Substituting into the inequality:

\[
\frac{1}{1+0^2} + \frac{1}{1+0^2} + \frac{1}{1+0^2} = 3.
\]

#### Case 2: \( x = y = z = \sqrt{3} \)

Substituting into the inequality:

\[
\frac{1}{1+(\sqrt{3})^2} + \frac{1}{1+(\sqrt{3})^2} + \frac{1}{1+(\sqrt{3})^2} = 3 \cdot \frac{1}{1+3} = \frac{3}{4}.
\]

#### Case 3: \( x = y = z = -\sqrt{3} \)

This is similar to Case 2, yielding:

\[
\frac{1}{1+(-\sqrt{3})^2} + \frac{1}{1+(-\sqrt{3})^2} + \frac{1}{1+(-\sqrt{3})^2} = \frac{3}{4}.
\]

### Step 3: Consider Other Configurations

Consider \( x = 0, y = 1, z = -1 \). Then:

\[
x+y+z = 0 = xyz.
\]

Substituting into the inequality:

\[
\frac{1}{1+0^2} + \frac{1}{1+1^2} + \frac{1}{1+(-1)^2} = 1 + \frac{1}{2} + \frac{1}{2} = 2.
\]

### Step 4: Determine the Largest \( C \)

From the cases considered, the smallest value of the sum is \(\frac{3}{4}\) when \( x = y = z = \pm\sqrt{3} \). Therefore, the largest constant \( C \) such that the inequality holds for all \( x, y, z \) satisfying the constraint is:

\[
C = \frac{3}{4}.
\]

Thus, the answer is \(\boxed{\frac{3}{4}}\).

The answer is \( C = \frac{3}{4} \).