## Problem

Find the largest constant $C$ such that for all real numbers $x$, the following inequality holds:
$$
x^2+\frac{1}{6(1+|x-2|)} \geq C
$$

## Query

Task description: Please solve the problem with clear, rigorous, and logically sound steps. At the end of your response, state your answer in exactly this format: 'The answer is $C=X$', where X is your calculated numerical bound value. Example: 'The answer is $C=1$'.

Problem: Find the largest constant $C$ such that for all real numbers $x$, the following inequality holds:
$$
x^2+\frac{1}{6(1+|x-2|)} \geq C
$$

Solution:

## Response

To solve this problem, we need to find the largest constant \( C \) such that the inequality

\[
x^2 + \frac{1}{6(1+|x-2|)} \geq C
\]

holds for all real numbers \( x \).

### Step 1: Analyze the expression

The expression consists of two parts: \( x^2 \) and \(\frac{1}{6(1+|x-2|)}\).

- The term \( x^2 \) is non-negative and increases as \( |x| \) increases.
- The term \(\frac{1}{6(1+|x-2|)}\) is positive and decreases as \( |x-2| \) increases.

### Step 2: Consider the behavior of the expression at \( x = 2 \)

At \( x = 2 \), the expression simplifies to:

\[
x^2 + \frac{1}{6(1+|x-2|)} = 2^2 + \frac{1}{6(1+0)} = 4 + \frac{1}{6} = \frac{25}{6}
\]

### Step 3: Consider the behavior as \( x \to \infty \) and \( x \to -\infty \)

As \( x \to \infty \) or \( x \to -\infty \), the term \( x^2 \) dominates, and the expression tends to infinity. Therefore, the minimum value of the expression is not at infinity.

### Step 4: Consider the behavior around \( x = 2 \)

Since the expression is continuous and differentiable, we can check for local minima around \( x = 2 \).

Define the function:

\[
f(x) = x^2 + \frac{1}{6(1+|x-2|)}
\]

For \( x \geq 2 \), \( |x-2| = x-2 \), so:

\[
f(x) = x^2 + \frac{1}{6(1+x-2)} = x^2 + \frac{1}{6x-6}
\]

For \( x < 2 \), \( |x-2| = 2-x \), so:

\[
f(x) = x^2 + \frac{1}{6(1+2-x)} = x^2 + \frac{1}{8-x}
\]

### Step 5: Check for local minima

**For \( x \geq 2 \):**

The derivative of \( f(x) = x^2 + \frac{1}{6x-6} \) is:

\[
f'(x) = 2x - \frac{1}{(6x-6)^2}
\]

Setting \( f'(x) = 0 \):

\[
2x = \frac{1}{(6x-6)^2}
\]

This equation is complex to solve analytically, but we know \( f(x) \) is increasing for \( x > 2 \) because \( x^2 \) grows faster than the decrease in \(\frac{1}{6x-6}\).

**For \( x < 2 \):**

The derivative of \( f(x) = x^2 + \frac{1}{8-x} \) is:

\[
f'(x) = 2x + \frac{1}{(8-x)^2}
\]

Setting \( f'(x) = 0 \):

\[
2x = -\frac{1}{(8-x)^2}
\]

This equation is also complex to solve analytically, but \( f(x) \) is increasing for \( x < 2 \) because \( x^2 \) grows faster than the decrease in \(\frac{1}{8-x}\).

### Conclusion

The minimum value of the expression occurs at \( x = 2 \), where we calculated:

\[
f(2) = \frac{25}{6}
\]

Thus, the largest constant \( C \) such that the inequality holds for all \( x \) is:

\[
\boxed{\frac{25}{6}}
\]

The answer is \( C = \frac{25}{6} \).