## Problem

Let $x, y, z$ be complex numbers such that $|x+2y+3z| = 1$. Determine the largest constant $C$ such that the following inequality holds for all $x, y, z$:

$$
x^2 + y^2 + z^2 + \left|x^2 + y^2 + z^2\right| \geq C.
$$

## Query

Task description: Please solve the problem with clear, rigorous, and logically sound steps. At the end of your response, state your answer in exactly this format: 'The answer is $C=X$', where X is your calculated numerical bound value. Example: 'The answer is $C=1$'.

Problem: Let $x, y, z$ be complex numbers such that $|x+2y+3z| = 1$. Determine the largest constant $C$ such that the following inequality holds for all $x, y, z$:

$$
x^2 + y^2 + z^2 + \left|x^2 + y^2 + z^2\right| \geq C.
$$

Solution:

## Response

To solve this problem, we need to find the largest constant \( C \) such that the inequality

\[
x^2 + y^2 + z^2 + \left|x^2 + y^2 + z^2\right| \geq C
\]

holds for all complex numbers \( x, y, z \) satisfying \( |x + 2y + 3z| = 1 \).

### Step 1: Analyze the expression

The expression \( x^2 + y^2 + z^2 + \left|x^2 + y^2 + z^2\right| \) can be simplified based on the value of \( x^2 + y^2 + z^2 \):

- If \( x^2 + y^2 + z^2 \) is non-negative, then \( \left|x^2 + y^2 + z^2\right| = x^2 + y^2 + z^2 \), and the expression becomes \( 2(x^2 + y^2 + z^2) \).
- If \( x^2 + y^2 + z^2 \) is negative, then \( \left|x^2 + y^2 + z^2\right| = -(x^2 + y^2 + z^2) \), and the expression becomes \( 0 \).

Thus, the expression is always non-negative, and the minimum value occurs when \( x^2 + y^2 + z^2 = 0 \).

### Step 2: Find conditions for \( x^2 + y^2 + z^2 = 0 \)

For complex numbers, \( x^2 + y^2 + z^2 = 0 \) implies that each of the terms \( x^2, y^2, z^2 \) must cancel each other out. This is possible if \( x, y, z \) are chosen such that their squares sum to zero.

### Step 3: Check if \( x^2 + y^2 + z^2 = 0 \) is possible under the constraint

Given \( |x + 2y + 3z| = 1 \), we need to check if there exist complex numbers \( x, y, z \) such that both \( x^2 + y^2 + z^2 = 0 \) and \( |x + 2y + 3z| = 1 \).

Consider the case where \( x = 0 \), \( y = 0 \), and \( z = 0 \). Clearly, \( x^2 + y^2 + z^2 = 0 \) holds, but \( |x + 2y + 3z| = 0 \neq 1 \).

Now, consider non-zero values. Suppose \( x = 1 \), \( y = i \), and \( z = -\frac{1}{3} - \frac{2i}{3} \). Then:

\[
x^2 = 1, \quad y^2 = -1, \quad z^2 = \left(-\frac{1}{3} - \frac{2i}{3}\right)^2 = \frac{1}{9} - \frac{4}{9}i - \frac{4}{9} = -\frac{1}{3} - \frac{4}{9}i
\]

Summing these:

\[
x^2 + y^2 + z^2 = 1 - 1 - \frac{1}{3} - \frac{4}{9}i = -\frac{1}{3} - \frac{4}{9}i
\]

This does not satisfy \( x^2 + y^2 + z^2 = 0 \).

### Step 4: Conclusion

The minimum value of \( x^2 + y^2 + z^2 + \left|x^2 + y^2 + z^2\right| \) is \( 0 \), which occurs when \( x^2 + y^2 + z^2 = 0 \). However, under the constraint \( |x + 2y + 3z| = 1 \), achieving \( x^2 + y^2 + z^2 = 0 \) is not possible.

Thus, the minimum value of the expression is actually greater than zero, and the largest constant \( C \) such that the inequality holds for all \( x, y, z \) is:

\[
\boxed{0}
\]

The answer is \( C = 0 \).