## Problem

Let $a_1, a_2, \ldots, a_n$ be non-negative real numbers such that $\prod a_1 = \lambda^n$. Determine the minimal constant $C$ such that the following inequality holds for all $a_1, a_2, \ldots, a_n$:

$$
\prod_{c y c}\left(a_1^2-a_1+1\right) \geq \sqrt{\left(\frac{1+\lambda^4}{C}\right)^n}.
$$

## Query

Task description: Please solve the problem with clear, rigorous, and logically sound steps. At the end of your response, state your answer in exactly this format: 'The answer is $C=X$', where X is your calculated numerical bound value. Example: 'The answer is $C=1$'.

Problem: Let $a_1, a_2, \ldots, a_n$ be non-negative real numbers such that $\prod a_1 = \lambda^n$. Determine the minimal constant $C$ such that the following inequality holds for all $a_1, a_2, \ldots, a_n$:

$$
\prod_{c y c}\left(a_1^2-a_1+1\right) \geq \sqrt{\left(\frac{1+\lambda^4}{C}\right)^n}.
$$

Solution:

## Response

To solve this problem, we need to find the minimal constant \( C \) such that the inequality

\[
\prod_{i=1}^n \left(a_i^2 - a_i + 1\right) \geq \sqrt{\left(\frac{1+\lambda^4}{C}\right)^n}
\]

holds for all non-negative real numbers \( a_1, a_2, \ldots, a_n \) satisfying \(\prod_{i=1}^n a_i = \lambda^n\).

### Step 1: Simplify the Right-Hand Side

The right-hand side of the inequality can be rewritten as:

\[
\sqrt{\left(\frac{1+\lambda^4}{C}\right)^n} = \left(\frac{1+\lambda^4}{C}\right)^{n/2}
\]

### Step 2: Analyze the Function \( f(a) = a^2 - a + 1 \)

The function \( f(a) = a^2 - a + 1 \) is a quadratic function. We can complete the square to find its minimum value:

\[
f(a) = a^2 - a + 1 = \left(a - \frac{1}{2}\right)^2 + \frac{3}{4}
\]

The minimum value of \( f(a) \) is \(\frac{3}{4}\), which occurs at \( a = \frac{1}{2} \).

### Step 3: Use AM-GM Inequality

We apply the AM-GM inequality to the product \(\prod_{i=1}^n \left(a_i^2 - a_i + 1\right)\):

\[
\prod_{i=1}^n \left(a_i^2 - a_i + 1\right) \geq \left(\frac{1}{n} \sum_{i=1}^n (a_i^2 - a_i + 1)\right)^n
\]

### Step 4: Relate to the Given Condition

Given \(\prod_{i=1}^n a_i = \lambda^n\), we use the AM-GM inequality again:

\[
\frac{1}{n} \sum_{i=1}^n a_i \geq \sqrt[n]{\prod_{i=1}^n a_i} = \lambda
\]

### Step 5: Find the Minimum Value of the Product

To find the minimum value of \(\prod_{i=1}^n \left(a_i^2 - a_i + 1\right)\), consider the case where all \( a_i = \lambda \). Then:

\[
a_i^2 - a_i + 1 = \lambda^2 - \lambda + 1
\]

Thus, the product becomes:

\[
\prod_{i=1}^n \left(\lambda^2 - \lambda + 1\right) = \left(\lambda^2 - \lambda + 1\right)^n
\]

### Step 6: Equate and Solve for \( C \)

We want:

\[
\left(\lambda^2 - \lambda + 1\right)^n \geq \left(\frac{1+\lambda^4}{C}\right)^{n/2}
\]

Taking the \( n \)-th root on both sides:

\[
\lambda^2 - \lambda + 1 \geq \left(\frac{1+\lambda^4}{C}\right)^{1/2}
\]

Squaring both sides:

\[
(\lambda^2 - \lambda + 1)^2 \geq \frac{1+\lambda^4}{C}
\]

Solving for \( C \):

\[
C \geq \frac{1+\lambda^4}{(\lambda^2 - \lambda + 1)^2}
\]

### Conclusion

The minimal constant \( C \) is:

\[
C = \frac{1+\lambda^4}{(\lambda^2 - \lambda + 1)^2}
\]

Thus, the answer is \(\boxed{C = \frac{1+\lambda^4}{(\lambda^2 - \lambda + 1)^2}}\).