## Problem

Let $x, y, z$ be positive numbers such that $xy + yz + zx = 1$. Find the largest constant $C$ such that the following inequality holds for all $x, y, z$ satisfying the given constraint:
$$
\frac{x^3}{1+9y^2zx} + \frac{y^3}{1+9z^2xy} + \frac{z^3}{1+9x^2yz} \geq C(x+y+z)^3
$$

## Query

Task description: Please solve the problem with clear, rigorous, and logically sound steps. At the end of your response, state your answer in exactly this format: 'The answer is $C=X$', where X is your calculated numerical bound value. Example: 'The answer is $C=1$'.

Problem: Let $x, y, z$ be positive numbers such that $xy + yz + zx = 1$. Find the largest constant $C$ such that the following inequality holds for all $x, y, z$ satisfying the given constraint:
$$
\frac{x^3}{1+9y^2zx} + \frac{y^3}{1+9z^2xy} + \frac{z^3}{1+9x^2yz} \geq C(x+y+z)^3
$$

Solution:

## Response

To solve this problem, we need to find the largest constant \( C \) such that the inequality

\[
\frac{x^3}{1+9y^2zx} + \frac{y^3}{1+9z^2xy} + \frac{z^3}{1+9x^2yz} \geq C(x+y+z)^3
\]

holds for all positive \( x, y, z \) satisfying \( xy + yz + zx = 1 \).

### Step 1: Simplify the Problem

First, observe that the constraint \( xy + yz + zx = 1 \) is symmetric in \( x, y, z \). This suggests that the inequality might be easier to analyze if we assume some symmetry in \( x, y, z \).

### Step 2: Test Symmetric Case

Consider the symmetric case where \( x = y = z \). Then, \( 3x^2 = 1 \), so \( x = \frac{1}{\sqrt{3}} \).

Substitute \( x = y = z = \frac{1}{\sqrt{3}} \) into the left-hand side of the inequality:

\[
\frac{x^3}{1+9y^2zx} = \frac{\left(\frac{1}{\sqrt{3}}\right)^3}{1 + 9\left(\frac{1}{\sqrt{3}}\right)^2\left(\frac{1}{\sqrt{3}}\right)} = \frac{\frac{1}{3\sqrt{3}}}{1 + 3} = \frac{\frac{1}{3\sqrt{3}}}{4} = \frac{1}{12\sqrt{3}}
\]

Since the expression is symmetric, the total contribution from all three terms is:

\[
3 \times \frac{1}{12\sqrt{3}} = \frac{1}{4\sqrt{3}}
\]

Now, calculate the right-hand side:

\[
C(x+y+z)^3 = C\left(3 \times \frac{1}{\sqrt{3}}\right)^3 = C \times 3\sqrt{3}
\]

Set the inequality:

\[
\frac{1}{4\sqrt{3}} \geq C \times 3\sqrt{3}
\]

Simplify:

\[
\frac{1}{4\sqrt{3}} \geq 3C\sqrt{3}
\]

\[
\frac{1}{12} \geq C
\]

Thus, \( C \leq \frac{1}{12} \).

### Step 3: Check if \( C = \frac{1}{12} \) is Achievable

To verify if \( C = \frac{1}{12} \) is achievable, consider the case where \( x = y = z = \frac{1}{\sqrt{3}} \) again. We have already shown that:

\[
\frac{1}{4\sqrt{3}} = \frac{1}{12}
\]

Thus, the inequality holds with equality when \( C = \frac{1}{12} \).

### Conclusion

The largest constant \( C \) such that the inequality holds for all positive \( x, y, z \) satisfying \( xy + yz + zx = 1 \) is:

\[
\boxed{\frac{1}{12}}
\]

The answer is \( C = \frac{1}{12} \).