## Problem

Let $a, b, c > 0$ be positive real numbers such that $a + b + c = 1$. Consider the following inequality:
$$
\frac{1+a+b}{2+c} + \frac{1+b+c}{2+a} + \frac{1+c+a}{2+b} \quad () \quad 2.
$$

Determine the correct inequality relation to fill in the blank.

Options:

(A) $\leq$ 

(B) $\geq$

(C) $=$ 

(D) $<$

(E) $>$

(F) None of the above

## Query

Task description: Please solve the problem with clear, rigorous, and logically sound steps. At the end of your response, state your answer in exactly this format: 'The answer is (Letter) Symbol', where Letter is one of the given options. Example: 'The answer is (A) $\leq$'.

Problem: Let $a, b, c > 0$ be positive real numbers such that $a + b + c = 1$. Consider the following inequality:
$$
\frac{1+a+b}{2+c} + \frac{1+b+c}{2+a} + \frac{1+c+a}{2+b} \quad () \quad 2.
$$

Determine the correct inequality relation to fill in the blank.

Options:

(A) $\leq$ 

(B) $\geq$

(C) $=$ 

(D) $<$

(E) $>$

(F) None of the above

Solution:

## Response

To solve this problem, we need to analyze the given inequality:

\[
\frac{1+a+b}{2+c} + \frac{1+b+c}{2+a} + \frac{1+c+a}{2+b} \quad () \quad 2.
\]

We are given that \(a, b, c > 0\) and \(a + b + c = 1\). We need to determine the correct inequality relation to fill in the blank.

First, let's rewrite the terms in the inequality:

1. \(\frac{1+a+b}{2+c} = \frac{1 + (a+b)}{2+c}\).
2. \(\frac{1+b+c}{2+a} = \frac{1 + (b+c)}{2+a}\).
3. \(\frac{1+c+a}{2+b} = \frac{1 + (c+a)}{2+b}\).

Since \(a + b + c = 1\), we have:

- \(a + b = 1 - c\),
- \(b + c = 1 - a\),
- \(c + a = 1 - b\).

Substituting these into the fractions, we get:

\[
\frac{1 + (1-c)}{2+c} = \frac{2-c}{2+c},
\]
\[
\frac{1 + (1-a)}{2+a} = \frac{2-a}{2+a},
\]
\[
\frac{1 + (1-b)}{2+b} = \frac{2-b}{2+b}.
\]

Thus, the inequality becomes:

\[
\frac{2-c}{2+c} + \frac{2-a}{2+a} + \frac{2-b}{2+b} \quad () \quad 2.
\]

Now, let's consider the function \(f(x) = \frac{2-x}{2+x}\). This function is decreasing because its derivative \(f'(x) = -\frac{4}{(2+x)^2}\) is negative for \(x > 0\).

Since \(f(x)\) is decreasing, we can apply Jensen's inequality for the convex function \(-f(x)\) (since \(f(x)\) is concave):

\[
f(a) + f(b) + f(c) \leq 3f\left(\frac{a+b+c}{3}\right) = 3f\left(\frac{1}{3}\right).
\]

Calculating \(f\left(\frac{1}{3}\right)\):

\[
f\left(\frac{1}{3}\right) = \frac{2-\frac{1}{3}}{2+\frac{1}{3}} = \frac{\frac{5}{3}}{\frac{7}{3}} = \frac{5}{7}.
\]

Thus, we have:

\[
f(a) + f(b) + f(c) \leq 3 \times \frac{5}{7} = \frac{15}{7}.
\]

However, we need to compare this sum to 2. Notice that:

\[
\frac{15}{7} \approx 2.14 > 2.
\]

Therefore, the inequality:

\[
\frac{2-c}{2+c} + \frac{2-a}{2+a} + \frac{2-b}{2+b} \geq 2
\]

holds true. Thus, the correct relation is \(\geq\).

The answer is (B) \(\geq\).