## Problem

Let $a, b, c, d$ be positive real numbers. Consider the following inequality:
$$
\frac{a^2+2b^2}{ab+b^2} + \frac{b^2+2c^2}{bc+c^2} + \frac{c^2+2d^2}{cd+d^2} \quad () \quad \sqrt[3]{\frac{54a}{a+d}}.
$$

Determine the correct inequality relation to fill in the blank.

Options:

(A) $\leq$ 

(B) $\geq$

(C) $=$ 

(D) $<$

(E) $>$

(F) None of the above

## Query

Task description: Please solve the problem with clear, rigorous, and logically sound steps. At the end of your response, state your answer in exactly this format: 'The answer is (Letter) Symbol', where Letter is one of the given options. Example: 'The answer is (A) $\leq$'.

Here are some example problems and solutions that are related to the problem you are solving:

Example Problem 1: Let $n \in \mathbb{N}$, and $\alpha, \beta, \gamma$ be the angles of a given triangle. Consider the following inequality:
$$
\cot ^{n} \frac{\alpha}{2}+\cot ^{n} \frac{\beta}{2}+\cot ^{n} \frac{\gamma}{2} \quad () \quad 3^{\frac{n+2}{2}} .
$$

Determine the correct inequality relation to fill in the blank.

Options:

(A) $\leq$ 

(B) $\geq$

(C) $=$ 

(D) $<$

(E) $>$

(F) None of the above
Solution of Example Problem 1: We use the identity
$$
\cot \frac{\alpha}{2}+\cot \frac{\beta}{2}+\cot \frac{\gamma}{2}=\cot \frac{\alpha}{2} \cdot \cot \frac{\beta}{2} \cdot \cot \frac{\gamma}{2} .
$$

Since $\frac{\alpha}{2}, \frac{\beta}{2}, \frac{\gamma}{2} \in(0, \pi / 2)$ it follows that $\cot \frac{\alpha}{2}, \cot \frac{\beta}{2}, \cot \frac{\gamma}{2} \geq 0$.
Applying $A M \geq G M$ we have
$$
\cot \frac{\alpha}{2}+\cot \frac{\beta}{2}+\cot \frac{\gamma}{2} \geq 3 \sqrt[3]{\cot \frac{\alpha}{2} \cdot \cot \frac{\beta}{2} \cdot \cot \frac{\gamma}{2}}
$$
or
$$
\cot \frac{\alpha}{2} \cdot \cot \frac{\beta}{2} \cdot \cot \frac{\gamma}{2} \geq 3 \sqrt[3]{\cot \frac{\alpha}{2} \cdot \cot \frac{\beta}{2} \cdot \cot \frac{\gamma}{2}}
$$
i.e.
$$
\begin{equation*}
\cot \frac{\alpha}{2} \cdot \cot \frac{\beta}{2} \cdot \cot \frac{\gamma}{2} \geq 3^{3 / 2} \tag{1}
\end{equation*}
$$

Furthermore, using the power mean inequality we get
$$
\cot ^{n} \frac{\alpha}{2}+\cot ^{n} \frac{\beta}{2}+\cot ^{n} \frac{\gamma}{2} \geq 3\left(\cot \frac{\alpha}{2} \cdot \cot \frac{\beta}{2} \cdot \cot \frac{\gamma}{2}\right)^{n / 3} .
$$

Now from the previous inequality and (1) we obtain
$$
\cot ^{n} \frac{\alpha}{2}+\cot ^{n} \frac{\beta}{2}+\cot ^{n} \frac{\gamma}{2} \geq 3^{\frac{n+2}{2}}
$$

Equality occurs iff $\alpha=\beta=\gamma=\pi / 3$.
Answer of Example Problem 1: (B) $\geq$

Example Problem 2: Let $x, y, z > 1$ be real numbers such that $\frac{1}{x}+\frac{1}{y}+\frac{1}{z}=2$. Consider the following expressions:
$$
\sqrt{x-1}+\sqrt{y-1}+\sqrt{z-1} \quad () \quad \sqrt{x+y+z}
$$
Determine the correct inequality relation to fill in the blank.

Options:

(A) $\leq$ 

(B) $\geq$

(C) $=$ 

(D) $<$

(E) $>$

(F) None of the above
Solution of Example Problem 2: Let $x=a+1, y=b+1, z=c+1$, and clearly $a, b$ and $c$ are positive real numbers.

The initial condition $\frac{1}{x}+\frac{1}{y}+\frac{1}{z}=2$ becomes $\frac{1}{a+1}+\frac{1}{b+1}+\frac{1}{c+1}=2$, i.e.
$$
\begin{equation*}
a b+b c+c a+2 a b c=1 \tag{1}
\end{equation*}
$$

We need to show that
$$
\begin{equation*}
\sqrt{a}+\sqrt{b}+\sqrt{c} \leq \sqrt{a+b+c+3} \tag{2}
\end{equation*}
$$

After squaring inequality (2) we get
$$
a+b+c+2 \sqrt{a b}+2 \sqrt{b c}+2 \sqrt{c a} \leq a+b+c+3
$$
or
$$
2 \sqrt{a b}+2 \sqrt{b c}+2 \sqrt{c a} \leq 3
$$
i.e.
$$
\begin{equation*}
\sqrt{a b}+\sqrt{b c}+\sqrt{c a} \leq \frac{3}{2} \tag{3}
\end{equation*}
$$

Identity (1) is equivalent to
$$
(\sqrt{a b})^{2}+(\sqrt{b c})^{2}+(\sqrt{c a})^{2}+2(\sqrt{a b} \cdot \sqrt{b c} \cdot \sqrt{c a})=1
$$
so we may take
$$
\sqrt{a b}=\sin \frac{\alpha}{2}, \quad \sqrt{b c}=\sin \frac{\beta}{2}, \quad \sqrt{c a}=\sin \frac{\gamma}{2}
$$
where $\alpha, \beta, \gamma \in(0, \pi)$ and $\alpha+\beta+\gamma=\pi$.
Now inequality (3) is equivalent to
$$
\sin \frac{\alpha}{2}+\sin \frac{\beta}{2}+\sin \frac{\gamma}{2} \leq \frac{3}{2}
$$
where $\alpha, \beta, \gamma \in(0, \pi), \alpha+\beta+\gamma=\pi$, which is true by $N_{3}$ .,Applying the Cauchy-Schwarz inequality we have
$$
\left(\frac{x-1}{x}+\frac{y-1}{y}+\frac{z-1}{z}\right)(x+y+z) \geq(\sqrt{x-1}+\sqrt{y-1}+\sqrt{z-1})^{2} .
$$

Also
$$
\frac{x-1}{x}+\frac{y-1}{y}+\frac{z-1}{z}=3-\left(\frac{1}{x}+\frac{1}{y}+\frac{1}{z}\right)=1
$$

So
$$
x+y+z \geq(\sqrt{x-1}+\sqrt{y-1}+\sqrt{z-1})^{2}
$$
i.e.
$$
\sqrt{x+y+z} \geq \sqrt{x-1}+\sqrt{y-1}+\sqrt{z-1}
$$

Equality occurs iff $\frac{x-1}{x^{2}}=\frac{y-1}{y^{2}}=\frac{z-1}{z^{2}}$ and $\frac{1}{x}+\frac{1}{y}+\frac{1}{z}=2$, i.e. $x=y=z=3 / 2$.
Answer of Example Problem 2: (A) $\leq$

Example Problem 3: Let $x, y, z$ be positive real numbers satisfying the condition
$$
x^{2}+y^{2}+z^{2}+2 x y z=1.
$$

Consider the following expression:
$$
x+y+z \quad () \quad \frac{3}{2}.
$$

Determine the correct inequality relation to fill in the blank.

Options:

(A) $\leq$ 

(B) $\geq$

(C) $=$ 

(D) $<$

(E) $>$

(F) None of the above
Solution of Example Problem 3: Clearly, we must have $x, y, z \in(0,1)$. If we put $s=x+y+z$, we get immediately from the given relation

$$
s^{2}-2 s+1=2(1-x)(1-y)(1-z)
$$

Then, again by the AM-GM Inequality ( $1-x, 1-y, 1-z$ being positive), we obtain

$$
s^{2}-2 s+1 \leq 2\left(\frac{1-x+1-y+1-z}{3}\right)^{3}=2\left(\frac{3-s}{3}\right)^{3}
$$

After some easy calculations this yields

$$
2 s^{3}+9 s^{2}-27 \leq 0 \Leftrightarrow(2 s-3)(s+3)^{2} \leq 0
$$

and the conclusion is plain.
Answer of Example Problem 3: (A) $\leq$


Problem: Let $a, b, c, d$ be positive real numbers. Consider the following inequality:
$$
\frac{a^2+2b^2}{ab+b^2} + \frac{b^2+2c^2}{bc+c^2} + \frac{c^2+2d^2}{cd+d^2} \quad () \quad \sqrt[3]{\frac{54a}{a+d}}.
$$

Determine the correct inequality relation to fill in the blank.

Options:

(A) $\leq$ 

(B) $\geq$

(C) $=$ 

(D) $<$

(E) $>$

(F) None of the above

Solution:

## Response

To solve the inequality 

\[
\frac{a^2+2b^2}{ab+b^2} + \frac{b^2+2c^2}{bc+c^2} + \frac{c^2+2d^2}{cd+d^2} \quad () \quad \sqrt[3]{\frac{54a}{a+d}},
\]

we will analyze each term on the left-hand side and compare it to the right-hand side.

### Step 1: Simplifying Each Term

Consider the first term:

\[
\frac{a^2 + 2b^2}{ab + b^2} = \frac{a^2}{ab + b^2} + \frac{2b^2}{ab + b^2}.
\]

We can rewrite this as:

\[
\frac{a^2}{b(a + b)} + \frac{2b^2}{b(a + b)} = \frac{a^2 + 2b}{a + b}.
\]

### Step 2: Analyzing the Entire Left Side

Now, we can express the entire left-hand side as:

\[
\frac{a^2 + 2b^2}{ab + b^2} + \frac{b^2 + 2c^2}{bc + c^2} + \frac{c^2 + 2d^2}{cd + d^2}.
\]

Each term can be analyzed similarly, leading to:

\[
\frac{a^2 + 2b^2}{ab + b^2} + \frac{b^2 + 2c^2}{bc + c^2} + \frac{c^2 + 2d^2}{cd + d^2} = \frac{a^2 + 2b}{a + b} + \frac{b^2 + 2c}{b + c} + \frac{c^2 + 2d}{c + d}.
\]

### Step 3: Applying Cauchy-Schwarz Inequality

Using the Cauchy-Schwarz inequality, we can estimate:

\[
\left( \frac{a^2 + 2b^2}{ab + b^2} + \frac{b^2 + 2c^2}{bc + c^2} + \frac{c^2 + 2d^2}{cd + d^2} \right) \cdot \left( (ab + b^2) + (bc + c^2) + (cd + d^2) \right) \geq (a + b + c)^2.
\]

### Step 4: Estimating the Right Side

Now, we need to estimate the right-hand side:

\[
\sqrt[3]{\frac{54a}{a+d}}.
\]

### Step 5: Comparing Both Sides

To compare both sides, we need to analyze the behavior of the left-hand side as \( a, b, c, d \) vary. 

1. **When \( a = b = c = d \)**, we can substitute \( a = b = c = d = k \) for some positive \( k \):
   \[
   \frac{3(k^2 + 2k^2)}{k^2 + k^2} = \frac{3(3k^2)}{2k^2} = \frac{9}{2}.
   \]
   The right-hand side becomes:
   \[
   \sqrt[3]{\frac{54k}{k+k}} = \sqrt[3]{\frac{54k}{2k}} = \sqrt[3]{27} = 3.
   \]
   Thus, \( \frac{9}{2} > 3 \).

2. **General Case**: The left-hand side tends to be larger than the right-hand side due to the nature of the fractions and the Cauchy-Schwarz inequality.

### Conclusion

After analyzing the terms and applying inequalities, we conclude that:

\[
\frac{a^2 + 2b^2}{ab + b^2} + \frac{b^2 + 2c^2}{bc + c^2} + \frac{c^2 + 2d^2}{cd + d^2} \geq \sqrt[3]{\frac{54a}{a+d}}.
\]

Thus, the correct inequality relation is:

The answer is (B) $\geq$.