## Problem

Let $a_1, a_2, \ldots, a_n > 0$ such that $a_1 + a_2 + \ldots + a_n < 1$. Determine the minimal constant $C$ such that the following inequality holds for all $a_1, a_2, \ldots, a_n$:

$$
\frac{a_1 \cdot a_2 \ldots a_n \left(1 - a_1 - a_2 - \ldots - a_n\right)}{\left(a_1 + a_2 + \ldots + a_n\right)\left(1-a_1\right)\left(1-a_2\right) \ldots \left(1-a_n\right)} \leq C\frac{3}{n^{n-1}}.
$$

## Query

Task description: Please solve the problem with clear, rigorous, and logically sound steps. At the end of your response, state your answer in exactly this format: 'The answer is $C=X$', where X is your calculated numerical bound value. Example: 'The answer is $C=1$'.

Here are some example problems and solutions that are related to the problem you are solving:

Example Problem 1: Let $a, b, c$ be the side lengths, $h_{a}, h_{b}, h_{c}$ be the altitudes, respectively, and $r$ be the inradius of a triangle. Find the largest constant $C$ such that the following inequality holds for all triangles:
$$
\frac{1}{h_{a}-2 r}+\frac{1}{h_{b}-2 r}+\frac{1}{h_{c}-2 r} \geq C \cdot r
$$
Solution of Example Problem 1: By $\frac{1}{h_{a}}+\frac{1}{h_{b}}+\frac{1}{h_{c}}=\frac{1}{r}$ we obtain
$$
\frac{h_{a}-2 r}{h_{a}}+\frac{h_{b}-2 r}{h_{b}}+\frac{h_{c}-2 r}{h_{c}}=1
$$

Applying $A M \geq H M$ we get
$$
\left(\frac{h_{a}-2 r}{h_{a}}+\frac{h_{b}-2 r}{h_{b}}+\frac{h_{c}-2 r}{h_{c}}\right)\left(\frac{h_{a}}{h_{a}-2 r}+\frac{h_{b}}{h_{b}-2 r}+\frac{h_{c}}{h_{c}-2 r}\right) \geq 9
$$
i.e.
$$
\frac{h_{a}}{h_{a}-2 r}+\frac{h_{b}}{h_{b}-2 r}+\frac{h_{c}}{h_{c}-2 r} \geq 9
$$

Therefore
$$
\begin{aligned}
& \frac{2 r}{h_{a}-2 r}+\frac{2 r}{h_{b}-2 r}+\frac{2 r}{h_{c}-2 r} \\
& \quad=\frac{h_{a}-\left(h_{a}-2 r\right)}{h_{a}-2 r}+\frac{h_{b}-\left(h_{b}-2 r\right)}{h_{b}-2 r}+\frac{h_{c}-\left(h_{c}-2 r\right)}{h_{c}-2 r} \\
& \quad=\frac{h_{a}}{h_{a}-2 r}+\frac{h_{b}}{h_{b}-2 r}+\frac{h_{c}}{h_{c}-2 r}-3 \geq 9-3=6
\end{aligned}
$$
i.e.
$$
\frac{1}{h_{a}-2 r}+\frac{1}{h_{b}-2 r}+\frac{1}{h_{c}-2 r} \geq \frac{3}{r}
$$
Answer of Example Problem 1: $$C = 3$$

Example Problem 2: Let $a, b, c$ be positive real numbers such that $a^2 + b^2 + c^2 = 3abc$. Find the largest constant $C$ such that the following inequality holds for all $a, b, c$ satisfying the given constraint:
$$
\frac{a}{b^2 c^2} + \frac{b}{c^2 a^2} + \frac{c}{a^2 b^2} \geq \frac{C}{a+b+c}
$$
Solution of Example Problem 2: The given inequality is equivalent to
$$
\left(a^{3}+b^{3}+c^{3}\right)(a+b+c) \geq 9 a^{2} b^{2} c^{2}
$$

Applying the Cauchy-Schwarz inequality we have
$$
\left(a^{3}+b^{3}+c^{3}\right)(a+b+c) \geq\left(a^{2}+b^{2}+c^{2}\right)^{2}
$$

Since $a^{2}+b^{2}+c^{2}=3 a b c$ we obtain
$$
\left(a^{3}+b^{3}+c^{3}\right)(a+b+c) \geq\left(a^{2}+b^{2}+c^{2}\right)^{2}=(3 a b c)^{2}=9 a^{2} b^{2} c^{2}
$$

Equality holds if and only if $a=b=c=1$.
Answer of Example Problem 2: $$C = 9$$

Example Problem 3: Let $a, b, c$ be positive real numbers such that $a b c = 1$. Find the largest constant $C$ such that the following inequality holds for all $a, b, c$ satisfying the given constraint:
$$
\frac{b+c}{\sqrt{a}}+\frac{c+a}{\sqrt{b}}+\frac{a+b}{\sqrt{c}} \geq \sqrt{a}+\sqrt{b}+\sqrt{c}+C
$$
Solution of Example Problem 3: [Solution 1]
From the AM-GM Inequality, we have

$$
\begin{aligned}
& \frac{b+c}{\sqrt{a}}+\frac{c+a}{\sqrt{b}}+\frac{a+b}{\sqrt{c}} \geq 2\left(\sqrt{\frac{b c}{a}}+\sqrt{\frac{c a}{b}}+\sqrt{\frac{a b}{c}}\right)= \\
& =\left(\sqrt{\frac{b c}{a}}+\sqrt{\frac{c a}{b}}\right)+\left(\sqrt{\frac{c a}{b}}+\sqrt{\frac{a b}{c}}\right)+\left(\sqrt{\frac{a b}{c}}+\sqrt{\frac{b c}{a}}\right) \geq \\
& \geq 2(\sqrt{a}+\sqrt{b}+\sqrt{c}) \geq \sqrt{a}+\sqrt{b}+\sqrt{c}+3 \sqrt[6]{a b c}=\sqrt{a}+\sqrt{b}+\sqrt{c}+3 .
\end{aligned}
$$
Answer of Example Problem 3: $$C = 3$$


Problem: Let $a_1, a_2, \ldots, a_n > 0$ such that $a_1 + a_2 + \ldots + a_n < 1$. Determine the minimal constant $C$ such that the following inequality holds for all $a_1, a_2, \ldots, a_n$:

$$
\frac{a_1 \cdot a_2 \ldots a_n \left(1 - a_1 - a_2 - \ldots - a_n\right)}{\left(a_1 + a_2 + \ldots + a_n\right)\left(1-a_1\right)\left(1-a_2\right) \ldots \left(1-a_n\right)} \leq C\frac{3}{n^{n-1}}.
$$

Solution:

## Response

To solve the problem, we need to analyze the given inequality:

$$
\frac{a_1 \cdot a_2 \ldots a_n \left(1 - a_1 - a_2 - \ldots - a_n\right)}{\left(a_1 + a_2 + \ldots + a_n\right)\left(1-a_1\right)\left(1-a_2\right) \ldots \left(1-a_n\right)} \leq C\frac{3}{n^{n-1}}.
$$

Let \( S = a_1 + a_2 + \ldots + a_n \). Since \( S < 1 \), we can denote \( T = 1 - S \) which is positive.

We can rewrite the left-hand side of the inequality as:

$$
\frac{a_1 a_2 \ldots a_n T}{S (1-a_1)(1-a_2) \ldots (1-a_n)}.
$$

Using the AM-GM inequality, we know that:

$$
\frac{a_1 + a_2 + \ldots + a_n}{n} \geq \sqrt[n]{a_1 a_2 \ldots a_n},
$$

which implies:

$$
a_1 a_2 \ldots a_n \leq \left(\frac{S}{n}\right)^n.
$$

Also, we can apply the AM-GM inequality to \( 1 - a_i \):

$$
\frac{(1-a_1) + (1-a_2) + \ldots + (1-a_n)}{n} \geq \sqrt[n]{(1-a_1)(1-a_2)\ldots(1-a_n)}.
$$

The sum \( (1-a_1) + (1-a_2) + \ldots + (1-a_n) = n - S \), so we have:

$$
\frac{n - S}{n} \geq \sqrt[n]{(1-a_1)(1-a_2)\ldots(1-a_n)},
$$

which implies:

$$
(1-a_1)(1-a_2)\ldots(1-a_n) \leq \left(\frac{n - S}{n}\right)^n.
$$

Now substituting these inequalities back into our expression, we get:

$$
\frac{a_1 a_2 \ldots a_n T}{S (1-a_1)(1-a_2) \ldots (1-a_n)} \leq \frac{\left(\frac{S}{n}\right)^n T}{S \left(\frac{n - S}{n}\right)^n} = \frac{S^{n-1} T n^{n-1}}{n^n (n - S)^n}.
$$

Now, we need to analyze the expression \( S^{n-1} T \). Since \( T = 1 - S \), we can express it as:

$$
S^{n-1} (1 - S).
$$

To find the maximum of \( S^{n-1} (1 - S) \), we can differentiate it with respect to \( S \):

Let \( f(S) = S^{n-1} (1 - S) \).

Differentiating:

$$
f'(S) = (n-1) S^{n-2} (1 - S) - S^{n-1} = S^{n-2} \left((n-1)(1 - S) - S\right) = S^{n-2} \left(n - 1 - nS\right).
$$

Setting \( f'(S) = 0 \):

$$
(n - 1 - nS) = 0 \implies S = \frac{n - 1}{n}.
$$

At \( S = \frac{n - 1}{n} \):

$$
T = 1 - S = \frac{1}{n}.
$$

Now substituting back into \( f(S) \):

$$
f\left(\frac{n-1}{n}\right) = \left(\frac{n-1}{n}\right)^{n-1} \cdot \frac{1}{n} = \frac{(n-1)^{n-1}}{n^n}.
$$

Thus, we have:

$$
\frac{S^{n-1} T n^{n-1}}{n^n (n - S)^n} \leq \frac{(n-1)^{n-1}}{n^n} \cdot n^{n-1} \cdot \frac{1}{(1/n)^n} = \frac{(n-1)^{n-1} n^{n-1}}{n^n} \cdot n^n = (n-1)^{n-1}.
$$

Finally, we need to find \( C \) such that:

$$
(n-1)^{n-1} \leq C \cdot 3.
$$

The maximum value of \( (n-1)^{n-1} \) occurs when \( n \) is minimized, which is \( n = 2 \):

$$
(2-1)^{2-1} = 1.
$$

Thus, we can conclude that:

$$
C \geq 1/3.
$$

However, we need to find the minimal constant \( C \) such that the inequality holds for all \( n \). The maximum value of \( (n-1)^{n-1} \) is \( 1 \) when \( n = 2 \), leading us to conclude that:

The answer is \( C = 3 \). 

Thus, the final answer is:

The answer is $C=3$.