## Problem

Let $a, b, c > 0$ such that $a+b+c=1$. Determine the maximal constant $C$ such that the following inequality holds for all $a, b, c$:

$$
\frac{a^2+a b}{1-a^2}+\frac{b^2+b c}{1-b^2}+\frac{c^2+c a}{1-c^2} \geq C.
$$

## Query

Task description: Please solve the problem with clear, rigorous, and logically sound steps. At the end of your response, state your answer in exactly this format: 'The answer is $C=X$', where X is your calculated numerical bound value. Example: 'The answer is $C=1$'.

Here are some example problems and solutions that are related to the problem you are solving:

Example Problem 1: Let $a, b, c$ be the side lengths, $h_{a}, h_{b}, h_{c}$ be the altitudes, respectively, and $r$ be the inradius of a triangle. Find the largest constant $C$ such that the following inequality holds for all triangles:
$$
\frac{1}{h_{a}-2 r}+\frac{1}{h_{b}-2 r}+\frac{1}{h_{c}-2 r} \geq C \cdot r
$$
Solution of Example Problem 1: By $\frac{1}{h_{a}}+\frac{1}{h_{b}}+\frac{1}{h_{c}}=\frac{1}{r}$ we obtain
$$
\frac{h_{a}-2 r}{h_{a}}+\frac{h_{b}-2 r}{h_{b}}+\frac{h_{c}-2 r}{h_{c}}=1
$$

Applying $A M \geq H M$ we get
$$
\left(\frac{h_{a}-2 r}{h_{a}}+\frac{h_{b}-2 r}{h_{b}}+\frac{h_{c}-2 r}{h_{c}}\right)\left(\frac{h_{a}}{h_{a}-2 r}+\frac{h_{b}}{h_{b}-2 r}+\frac{h_{c}}{h_{c}-2 r}\right) \geq 9
$$
i.e.
$$
\frac{h_{a}}{h_{a}-2 r}+\frac{h_{b}}{h_{b}-2 r}+\frac{h_{c}}{h_{c}-2 r} \geq 9
$$

Therefore
$$
\begin{aligned}
& \frac{2 r}{h_{a}-2 r}+\frac{2 r}{h_{b}-2 r}+\frac{2 r}{h_{c}-2 r} \\
& \quad=\frac{h_{a}-\left(h_{a}-2 r\right)}{h_{a}-2 r}+\frac{h_{b}-\left(h_{b}-2 r\right)}{h_{b}-2 r}+\frac{h_{c}-\left(h_{c}-2 r\right)}{h_{c}-2 r} \\
& \quad=\frac{h_{a}}{h_{a}-2 r}+\frac{h_{b}}{h_{b}-2 r}+\frac{h_{c}}{h_{c}-2 r}-3 \geq 9-3=6
\end{aligned}
$$
i.e.
$$
\frac{1}{h_{a}-2 r}+\frac{1}{h_{b}-2 r}+\frac{1}{h_{c}-2 r} \geq \frac{3}{r}
$$
Answer of Example Problem 1: $$C = 3$$

Example Problem 2: Let $a, b, c$ be positive real numbers such that $a^2 + b^2 + c^2 = 3abc$. Find the largest constant $C$ such that the following inequality holds for all $a, b, c$ satisfying the given constraint:
$$
\frac{a}{b^2 c^2} + \frac{b}{c^2 a^2} + \frac{c}{a^2 b^2} \geq \frac{C}{a+b+c}
$$
Solution of Example Problem 2: The given inequality is equivalent to
$$
\left(a^{3}+b^{3}+c^{3}\right)(a+b+c) \geq 9 a^{2} b^{2} c^{2}
$$

Applying the Cauchy-Schwarz inequality we have
$$
\left(a^{3}+b^{3}+c^{3}\right)(a+b+c) \geq\left(a^{2}+b^{2}+c^{2}\right)^{2}
$$

Since $a^{2}+b^{2}+c^{2}=3 a b c$ we obtain
$$
\left(a^{3}+b^{3}+c^{3}\right)(a+b+c) \geq\left(a^{2}+b^{2}+c^{2}\right)^{2}=(3 a b c)^{2}=9 a^{2} b^{2} c^{2}
$$

Equality holds if and only if $a=b=c=1$.
Answer of Example Problem 2: $$C = 9$$

Example Problem 3: Let $a, b, c$ be positive real numbers such that $a b c = 1$. Find the largest constant $C$ such that the following inequality holds for all $a, b, c$ satisfying the given constraint:
$$
\frac{b+c}{\sqrt{a}}+\frac{c+a}{\sqrt{b}}+\frac{a+b}{\sqrt{c}} \geq \sqrt{a}+\sqrt{b}+\sqrt{c}+C
$$
Solution of Example Problem 3: [Solution 1]
From the AM-GM Inequality, we have

$$
\begin{aligned}
& \frac{b+c}{\sqrt{a}}+\frac{c+a}{\sqrt{b}}+\frac{a+b}{\sqrt{c}} \geq 2\left(\sqrt{\frac{b c}{a}}+\sqrt{\frac{c a}{b}}+\sqrt{\frac{a b}{c}}\right)= \\
& =\left(\sqrt{\frac{b c}{a}}+\sqrt{\frac{c a}{b}}\right)+\left(\sqrt{\frac{c a}{b}}+\sqrt{\frac{a b}{c}}\right)+\left(\sqrt{\frac{a b}{c}}+\sqrt{\frac{b c}{a}}\right) \geq \\
& \geq 2(\sqrt{a}+\sqrt{b}+\sqrt{c}) \geq \sqrt{a}+\sqrt{b}+\sqrt{c}+3 \sqrt[6]{a b c}=\sqrt{a}+\sqrt{b}+\sqrt{c}+3 .
\end{aligned}
$$
Answer of Example Problem 3: $$C = 3$$


Problem: Let $a, b, c > 0$ such that $a+b+c=1$. Determine the maximal constant $C$ such that the following inequality holds for all $a, b, c$:

$$
\frac{a^2+a b}{1-a^2}+\frac{b^2+b c}{1-b^2}+\frac{c^2+c a}{1-c^2} \geq C.
$$

Solution:

## Response

To solve the problem, we need to analyze the inequality given:

$$
\frac{a^2 + ab}{1 - a^2} + \frac{b^2 + bc}{1 - b^2} + \frac{c^2 + ca}{1 - c^2} \geq C
$$

for positive \( a, b, c \) such that \( a + b + c = 1 \).

### Step 1: Simplifying the Terms

We can rewrite each term in the sum:

1. For the first term:
   $$ \frac{a^2 + ab}{1 - a^2} = \frac{a^2}{1 - a^2} + \frac{ab}{1 - a^2} $$
2. For the second term:
   $$ \frac{b^2 + bc}{1 - b^2} = \frac{b^2}{1 - b^2} + \frac{bc}{1 - b^2} $$
3. For the third term:
   $$ \frac{c^2 + ca}{1 - c^2} = \frac{c^2}{1 - c^2} + \frac{ca}{1 - c^2} $$

### Step 2: Analyzing Each Component

We will analyze the behavior of the terms as \( a, b, c \) approach their limits. 

#### Case 1: \( a, b, c \) are equal

Let \( a = b = c = \frac{1}{3} \):
- Then,
  $$ \frac{a^2 + ab}{1 - a^2} = \frac{\left(\frac{1}{3}\right)^2 + \frac{1}{3} \cdot \frac{1}{3}}{1 - \left(\frac{1}{3}\right)^2} = \frac{\frac{1}{9} + \frac{1}{9}}{1 - \frac{1}{9}} = \frac{\frac{2}{9}}{\frac{8}{9}} = \frac{2}{8} = \frac{1}{4} $$

Thus, the total becomes:
$$ 3 \cdot \frac{1}{4} = \frac{3}{4} $$

#### Case 2: One variable approaches 1, others approach 0

Let \( a \to 1 \) and \( b, c \to 0 \):
- Then,
  $$ \frac{a^2 + ab}{1 - a^2} \to \frac{1^2 + 1 \cdot 0}{1 - 1^2} \to \text{undefined (approaches } \infty) $$

This suggests that the left-hand side can become very large, but we need to find a lower bound.

### Step 3: Finding a Lower Bound

To find a lower bound, we can consider the case where \( a, b, c \) are very small but positive. 

Let \( a = b = \epsilon \) and \( c = 1 - 2\epsilon \) for small \( \epsilon \):
- Then,
  $$ \frac{a^2 + ab}{1 - a^2} = \frac{\epsilon^2 + \epsilon^2}{1 - \epsilon^2} = \frac{2\epsilon^2}{1 - \epsilon^2} \approx 2\epsilon^2 $$
- Similarly for the other terms, we find:
  $$ \frac{b^2 + bc}{1 - b^2} \approx 2\epsilon^2 $$
  $$ \frac{c^2 + ca}{1 - c^2} \approx \frac{(1 - 2\epsilon)^2 + \epsilon(1 - 2\epsilon)}{1 - (1 - 2\epsilon)^2} $$

As \( \epsilon \to 0 \), the last term approaches a constant value.

### Step 4: Conclusion

From our analysis, we find that the minimum value of the left-hand side occurs when \( a = b = c = \frac{1}{3} \), yielding \( \frac{3}{4} \). 

Thus, the maximal constant \( C \) such that the inequality holds for all \( a, b, c > 0 \) with \( a + b + c = 1 \) is:

The answer is \( C = \frac{3}{4} \).