## Problem

Let $\left(a_n\right)_{n \geq 0}$ be a sequence of real numbers such that for all $n \geq 0$,

$$
a_{n+1} \geq a_n^2+\frac{1}{5}
$$

Consider the following inequality for all $n \geq 5$:
$$
\sqrt{a_{n+5}} \quad () \quad a_{n-5}^2.
$$

Determine the correct inequality relation to fill in the blank.

Options:

(A) $\leq$ 

(B) $\geq$

(C) $=$ 

(D) $<$

(E) $>$

(F) None of the above

## Query

Task description: Please solve the problem with clear, rigorous, and logically sound steps. At the end of your response, state your answer in exactly this format: 'The answer is (Letter) Symbol', where Letter is one of the given options. Example: 'The answer is (A) $\leq$'.

Here are some example problems and solutions that are related to the problem you are solving:

Example Problem 1: Let $n \in \mathbb{N}$, and $\alpha, \beta, \gamma$ be the angles of a given triangle. Consider the following inequality:
$$
\cot ^{n} \frac{\alpha}{2}+\cot ^{n} \frac{\beta}{2}+\cot ^{n} \frac{\gamma}{2} \quad () \quad 3^{\frac{n+2}{2}} .
$$

Determine the correct inequality relation to fill in the blank.

Options:

(A) $\leq$ 

(B) $\geq$

(C) $=$ 

(D) $<$

(E) $>$

(F) None of the above
Solution of Example Problem 1: We use the identity
$$
\cot \frac{\alpha}{2}+\cot \frac{\beta}{2}+\cot \frac{\gamma}{2}=\cot \frac{\alpha}{2} \cdot \cot \frac{\beta}{2} \cdot \cot \frac{\gamma}{2} .
$$

Since $\frac{\alpha}{2}, \frac{\beta}{2}, \frac{\gamma}{2} \in(0, \pi / 2)$ it follows that $\cot \frac{\alpha}{2}, \cot \frac{\beta}{2}, \cot \frac{\gamma}{2} \geq 0$.
Applying $A M \geq G M$ we have
$$
\cot \frac{\alpha}{2}+\cot \frac{\beta}{2}+\cot \frac{\gamma}{2} \geq 3 \sqrt[3]{\cot \frac{\alpha}{2} \cdot \cot \frac{\beta}{2} \cdot \cot \frac{\gamma}{2}}
$$
or
$$
\cot \frac{\alpha}{2} \cdot \cot \frac{\beta}{2} \cdot \cot \frac{\gamma}{2} \geq 3 \sqrt[3]{\cot \frac{\alpha}{2} \cdot \cot \frac{\beta}{2} \cdot \cot \frac{\gamma}{2}}
$$
i.e.
$$
\begin{equation*}
\cot \frac{\alpha}{2} \cdot \cot \frac{\beta}{2} \cdot \cot \frac{\gamma}{2} \geq 3^{3 / 2} \tag{1}
\end{equation*}
$$

Furthermore, using the power mean inequality we get
$$
\cot ^{n} \frac{\alpha}{2}+\cot ^{n} \frac{\beta}{2}+\cot ^{n} \frac{\gamma}{2} \geq 3\left(\cot \frac{\alpha}{2} \cdot \cot \frac{\beta}{2} \cdot \cot \frac{\gamma}{2}\right)^{n / 3} .
$$

Now from the previous inequality and (1) we obtain
$$
\cot ^{n} \frac{\alpha}{2}+\cot ^{n} \frac{\beta}{2}+\cot ^{n} \frac{\gamma}{2} \geq 3^{\frac{n+2}{2}}
$$

Equality occurs iff $\alpha=\beta=\gamma=\pi / 3$.
Answer of Example Problem 1: (B) $\geq$

Example Problem 2: Let $x, y, z > 1$ be real numbers such that $\frac{1}{x}+\frac{1}{y}+\frac{1}{z}=2$. Consider the following expressions:
$$
\sqrt{x-1}+\sqrt{y-1}+\sqrt{z-1} \quad () \quad \sqrt{x+y+z}
$$
Determine the correct inequality relation to fill in the blank.

Options:

(A) $\leq$ 

(B) $\geq$

(C) $=$ 

(D) $<$

(E) $>$

(F) None of the above
Solution of Example Problem 2: Let $x=a+1, y=b+1, z=c+1$, and clearly $a, b$ and $c$ are positive real numbers.

The initial condition $\frac{1}{x}+\frac{1}{y}+\frac{1}{z}=2$ becomes $\frac{1}{a+1}+\frac{1}{b+1}+\frac{1}{c+1}=2$, i.e.
$$
\begin{equation*}
a b+b c+c a+2 a b c=1 \tag{1}
\end{equation*}
$$

We need to show that
$$
\begin{equation*}
\sqrt{a}+\sqrt{b}+\sqrt{c} \leq \sqrt{a+b+c+3} \tag{2}
\end{equation*}
$$

After squaring inequality (2) we get
$$
a+b+c+2 \sqrt{a b}+2 \sqrt{b c}+2 \sqrt{c a} \leq a+b+c+3
$$
or
$$
2 \sqrt{a b}+2 \sqrt{b c}+2 \sqrt{c a} \leq 3
$$
i.e.
$$
\begin{equation*}
\sqrt{a b}+\sqrt{b c}+\sqrt{c a} \leq \frac{3}{2} \tag{3}
\end{equation*}
$$

Identity (1) is equivalent to
$$
(\sqrt{a b})^{2}+(\sqrt{b c})^{2}+(\sqrt{c a})^{2}+2(\sqrt{a b} \cdot \sqrt{b c} \cdot \sqrt{c a})=1
$$
so we may take
$$
\sqrt{a b}=\sin \frac{\alpha}{2}, \quad \sqrt{b c}=\sin \frac{\beta}{2}, \quad \sqrt{c a}=\sin \frac{\gamma}{2}
$$
where $\alpha, \beta, \gamma \in(0, \pi)$ and $\alpha+\beta+\gamma=\pi$.
Now inequality (3) is equivalent to
$$
\sin \frac{\alpha}{2}+\sin \frac{\beta}{2}+\sin \frac{\gamma}{2} \leq \frac{3}{2}
$$
where $\alpha, \beta, \gamma \in(0, \pi), \alpha+\beta+\gamma=\pi$, which is true by $N_{3}$ .,Applying the Cauchy-Schwarz inequality we have
$$
\left(\frac{x-1}{x}+\frac{y-1}{y}+\frac{z-1}{z}\right)(x+y+z) \geq(\sqrt{x-1}+\sqrt{y-1}+\sqrt{z-1})^{2} .
$$

Also
$$
\frac{x-1}{x}+\frac{y-1}{y}+\frac{z-1}{z}=3-\left(\frac{1}{x}+\frac{1}{y}+\frac{1}{z}\right)=1
$$

So
$$
x+y+z \geq(\sqrt{x-1}+\sqrt{y-1}+\sqrt{z-1})^{2}
$$
i.e.
$$
\sqrt{x+y+z} \geq \sqrt{x-1}+\sqrt{y-1}+\sqrt{z-1}
$$

Equality occurs iff $\frac{x-1}{x^{2}}=\frac{y-1}{y^{2}}=\frac{z-1}{z^{2}}$ and $\frac{1}{x}+\frac{1}{y}+\frac{1}{z}=2$, i.e. $x=y=z=3 / 2$.
Answer of Example Problem 2: (A) $\leq$

Example Problem 3: Let $x, y, z$ be positive real numbers satisfying the condition
$$
x^{2}+y^{2}+z^{2}+2 x y z=1.
$$

Consider the following expression:
$$
x+y+z \quad () \quad \frac{3}{2}.
$$

Determine the correct inequality relation to fill in the blank.

Options:

(A) $\leq$ 

(B) $\geq$

(C) $=$ 

(D) $<$

(E) $>$

(F) None of the above
Solution of Example Problem 3: Clearly, we must have $x, y, z \in(0,1)$. If we put $s=x+y+z$, we get immediately from the given relation

$$
s^{2}-2 s+1=2(1-x)(1-y)(1-z)
$$

Then, again by the AM-GM Inequality ( $1-x, 1-y, 1-z$ being positive), we obtain

$$
s^{2}-2 s+1 \leq 2\left(\frac{1-x+1-y+1-z}{3}\right)^{3}=2\left(\frac{3-s}{3}\right)^{3}
$$

After some easy calculations this yields

$$
2 s^{3}+9 s^{2}-27 \leq 0 \Leftrightarrow(2 s-3)(s+3)^{2} \leq 0
$$

and the conclusion is plain.
Answer of Example Problem 3: (A) $\leq$


Problem: Let $\left(a_n\right)_{n \geq 0}$ be a sequence of real numbers such that for all $n \geq 0$,

$$
a_{n+1} \geq a_n^2+\frac{1}{5}
$$

Consider the following inequality for all $n \geq 5$:
$$
\sqrt{a_{n+5}} \quad () \quad a_{n-5}^2.
$$

Determine the correct inequality relation to fill in the blank.

Options:

(A) $\leq$ 

(B) $\geq$

(C) $=$ 

(D) $<$

(E) $>$

(F) None of the above

Solution:

## Response

To solve the problem, we start with the given recursive inequality for the sequence \( (a_n)_{n \geq 0} \):

\[
a_{n+1} \geq a_n^2 + \frac{1}{5}
\]

We need to analyze the behavior of the sequence as \( n \) increases, particularly for \( n \geq 5 \), and compare \( \sqrt{a_{n+5}} \) with \( a_{n-5}^2 \).

### Step 1: Establish a lower bound for \( a_n \)

We can use the recursive inequality to derive a lower bound for \( a_n \). Starting from an initial value \( a_0 \), we can express subsequent terms:

\[
a_1 \geq a_0^2 + \frac{1}{5}
\]
\[
a_2 \geq a_1^2 + \frac{1}{5} \geq (a_0^2 + \frac{1}{5})^2 + \frac{1}{5}
\]

Continuing this process, we can see that each term is at least as large as the square of the previous term plus a constant. This suggests that the sequence grows rapidly.

### Step 2: Analyze the growth of the sequence

Assuming \( a_n \) is sufficiently large, we can approximate the growth. If \( a_n \) is large, then \( a_n^2 \) will dominate the constant \( \frac{1}{5} \). Thus, we can expect:

\[
a_{n+1} \approx a_n^2
\]

This suggests that \( a_n \) grows at least exponentially. More formally, if we denote \( a_n \) as \( b_n = \log(a_n) \), we can see that:

\[
b_{n+1} \geq 2b_n + \log\left(1 + \frac{1}{5a_n^2}\right)
\]

For large \( n \), the term \( \log\left(1 + \frac{1}{5a_n^2}\right) \) becomes negligible, and we can approximate:

\[
b_{n+1} \approx 2b_n
\]

This indicates that \( b_n \) (and thus \( a_n \)) grows very quickly.

### Step 3: Compare \( \sqrt{a_{n+5}} \) and \( a_{n-5}^2 \)

Now we need to compare \( \sqrt{a_{n+5}} \) and \( a_{n-5}^2 \). Using the recursive inequality, we can express \( a_{n+5} \):

\[
a_{n+5} \geq a_{n+4}^2 + \frac{1}{5} \geq (a_{n+3}^2 + \frac{1}{5})^2 + \frac{1}{5} \geq \ldots
\]

Continuing this process, we can see that \( a_{n+5} \) is significantly larger than \( a_{n-5}^2 \) for large \( n \).

### Step 4: Establish the inequality

Given the rapid growth of \( a_n \), we can conclude that:

\[
\sqrt{a_{n+5}} \geq a_{n-5}
\]

Squaring both sides gives:

\[
a_{n+5} \geq a_{n-5}^2
\]

Thus, we can conclude that:

\[
\sqrt{a_{n+5}} \geq a_{n-5}
\]

Since \( a_{n-5} \) is also growing, we can assert that:

\[
\sqrt{a_{n+5}} \geq a_{n-5}^2
\]

### Conclusion

Thus, the correct inequality relation to fill in the blank is:

The answer is (B) $\geq$.