## Problem

Given sides of a triangle $a, b, c$, consider the following inequality:
$$
\frac{a}{2b}+\frac{b}{4c}+\frac{c}{a} \quad () \quad \frac{3a}{b+c}+\frac{2b}{c+a}+\frac{3c}{a+b}.
$$

Determine the correct inequality relation to fill in the blank.

Options:

(A) $\leq$ 

(B) $\geq$

(C) $=$ 

(D) $<$

(E) $>$

(F) None of the above

## Query

Task description: Please solve the problem with clear, rigorous, and logically sound steps. At the end of your response, state your answer in exactly this format: 'The answer is (Letter) Symbol', where Letter is one of the given options. Example: 'The answer is (A) $\leq$'.

Here are some example problems and solutions that are related to the problem you are solving:

Example Problem 1: Let $n \in \mathbb{N}$, and $\alpha, \beta, \gamma$ be the angles of a given triangle. Consider the following inequality:
$$
\cot ^{n} \frac{\alpha}{2}+\cot ^{n} \frac{\beta}{2}+\cot ^{n} \frac{\gamma}{2} \quad () \quad 3^{\frac{n+2}{2}} .
$$

Determine the correct inequality relation to fill in the blank.

Options:

(A) $\leq$ 

(B) $\geq$

(C) $=$ 

(D) $<$

(E) $>$

(F) None of the above
Solution of Example Problem 1: We use the identity
$$
\cot \frac{\alpha}{2}+\cot \frac{\beta}{2}+\cot \frac{\gamma}{2}=\cot \frac{\alpha}{2} \cdot \cot \frac{\beta}{2} \cdot \cot \frac{\gamma}{2} .
$$

Since $\frac{\alpha}{2}, \frac{\beta}{2}, \frac{\gamma}{2} \in(0, \pi / 2)$ it follows that $\cot \frac{\alpha}{2}, \cot \frac{\beta}{2}, \cot \frac{\gamma}{2} \geq 0$.
Applying $A M \geq G M$ we have
$$
\cot \frac{\alpha}{2}+\cot \frac{\beta}{2}+\cot \frac{\gamma}{2} \geq 3 \sqrt[3]{\cot \frac{\alpha}{2} \cdot \cot \frac{\beta}{2} \cdot \cot \frac{\gamma}{2}}
$$
or
$$
\cot \frac{\alpha}{2} \cdot \cot \frac{\beta}{2} \cdot \cot \frac{\gamma}{2} \geq 3 \sqrt[3]{\cot \frac{\alpha}{2} \cdot \cot \frac{\beta}{2} \cdot \cot \frac{\gamma}{2}}
$$
i.e.
$$
\begin{equation*}
\cot \frac{\alpha}{2} \cdot \cot \frac{\beta}{2} \cdot \cot \frac{\gamma}{2} \geq 3^{3 / 2} \tag{1}
\end{equation*}
$$

Furthermore, using the power mean inequality we get
$$
\cot ^{n} \frac{\alpha}{2}+\cot ^{n} \frac{\beta}{2}+\cot ^{n} \frac{\gamma}{2} \geq 3\left(\cot \frac{\alpha}{2} \cdot \cot \frac{\beta}{2} \cdot \cot \frac{\gamma}{2}\right)^{n / 3} .
$$

Now from the previous inequality and (1) we obtain
$$
\cot ^{n} \frac{\alpha}{2}+\cot ^{n} \frac{\beta}{2}+\cot ^{n} \frac{\gamma}{2} \geq 3^{\frac{n+2}{2}}
$$

Equality occurs iff $\alpha=\beta=\gamma=\pi / 3$.
Answer of Example Problem 1: (B) $\geq$

Example Problem 2: Let $x, y, z > 1$ be real numbers such that $\frac{1}{x}+\frac{1}{y}+\frac{1}{z}=2$. Consider the following expressions:
$$
\sqrt{x-1}+\sqrt{y-1}+\sqrt{z-1} \quad () \quad \sqrt{x+y+z}
$$
Determine the correct inequality relation to fill in the blank.

Options:

(A) $\leq$ 

(B) $\geq$

(C) $=$ 

(D) $<$

(E) $>$

(F) None of the above
Solution of Example Problem 2: Let $x=a+1, y=b+1, z=c+1$, and clearly $a, b$ and $c$ are positive real numbers.

The initial condition $\frac{1}{x}+\frac{1}{y}+\frac{1}{z}=2$ becomes $\frac{1}{a+1}+\frac{1}{b+1}+\frac{1}{c+1}=2$, i.e.
$$
\begin{equation*}
a b+b c+c a+2 a b c=1 \tag{1}
\end{equation*}
$$

We need to show that
$$
\begin{equation*}
\sqrt{a}+\sqrt{b}+\sqrt{c} \leq \sqrt{a+b+c+3} \tag{2}
\end{equation*}
$$

After squaring inequality (2) we get
$$
a+b+c+2 \sqrt{a b}+2 \sqrt{b c}+2 \sqrt{c a} \leq a+b+c+3
$$
or
$$
2 \sqrt{a b}+2 \sqrt{b c}+2 \sqrt{c a} \leq 3
$$
i.e.
$$
\begin{equation*}
\sqrt{a b}+\sqrt{b c}+\sqrt{c a} \leq \frac{3}{2} \tag{3}
\end{equation*}
$$

Identity (1) is equivalent to
$$
(\sqrt{a b})^{2}+(\sqrt{b c})^{2}+(\sqrt{c a})^{2}+2(\sqrt{a b} \cdot \sqrt{b c} \cdot \sqrt{c a})=1
$$
so we may take
$$
\sqrt{a b}=\sin \frac{\alpha}{2}, \quad \sqrt{b c}=\sin \frac{\beta}{2}, \quad \sqrt{c a}=\sin \frac{\gamma}{2}
$$
where $\alpha, \beta, \gamma \in(0, \pi)$ and $\alpha+\beta+\gamma=\pi$.
Now inequality (3) is equivalent to
$$
\sin \frac{\alpha}{2}+\sin \frac{\beta}{2}+\sin \frac{\gamma}{2} \leq \frac{3}{2}
$$
where $\alpha, \beta, \gamma \in(0, \pi), \alpha+\beta+\gamma=\pi$, which is true by $N_{3}$ .,Applying the Cauchy-Schwarz inequality we have
$$
\left(\frac{x-1}{x}+\frac{y-1}{y}+\frac{z-1}{z}\right)(x+y+z) \geq(\sqrt{x-1}+\sqrt{y-1}+\sqrt{z-1})^{2} .
$$

Also
$$
\frac{x-1}{x}+\frac{y-1}{y}+\frac{z-1}{z}=3-\left(\frac{1}{x}+\frac{1}{y}+\frac{1}{z}\right)=1
$$

So
$$
x+y+z \geq(\sqrt{x-1}+\sqrt{y-1}+\sqrt{z-1})^{2}
$$
i.e.
$$
\sqrt{x+y+z} \geq \sqrt{x-1}+\sqrt{y-1}+\sqrt{z-1}
$$

Equality occurs iff $\frac{x-1}{x^{2}}=\frac{y-1}{y^{2}}=\frac{z-1}{z^{2}}$ and $\frac{1}{x}+\frac{1}{y}+\frac{1}{z}=2$, i.e. $x=y=z=3 / 2$.
Answer of Example Problem 2: (A) $\leq$

Example Problem 3: Let $x, y, z$ be positive real numbers satisfying the condition
$$
x^{2}+y^{2}+z^{2}+2 x y z=1.
$$

Consider the following expression:
$$
x+y+z \quad () \quad \frac{3}{2}.
$$

Determine the correct inequality relation to fill in the blank.

Options:

(A) $\leq$ 

(B) $\geq$

(C) $=$ 

(D) $<$

(E) $>$

(F) None of the above
Solution of Example Problem 3: Clearly, we must have $x, y, z \in(0,1)$. If we put $s=x+y+z$, we get immediately from the given relation

$$
s^{2}-2 s+1=2(1-x)(1-y)(1-z)
$$

Then, again by the AM-GM Inequality ( $1-x, 1-y, 1-z$ being positive), we obtain

$$
s^{2}-2 s+1 \leq 2\left(\frac{1-x+1-y+1-z}{3}\right)^{3}=2\left(\frac{3-s}{3}\right)^{3}
$$

After some easy calculations this yields

$$
2 s^{3}+9 s^{2}-27 \leq 0 \Leftrightarrow(2 s-3)(s+3)^{2} \leq 0
$$

and the conclusion is plain.
Answer of Example Problem 3: (A) $\leq$


Problem: Given sides of a triangle $a, b, c$, consider the following inequality:
$$
\frac{a}{2b}+\frac{b}{4c}+\frac{c}{a} \quad () \quad \frac{3a}{b+c}+\frac{2b}{c+a}+\frac{3c}{a+b}.
$$

Determine the correct inequality relation to fill in the blank.

Options:

(A) $\leq$ 

(B) $\geq$

(C) $=$ 

(D) $<$

(E) $>$

(F) None of the above

Solution:

## Response

To solve the problem, we need to analyze the inequality:

$$
\frac{a}{2b}+\frac{b}{4c}+\frac{c}{a} \quad () \quad \frac{3a}{b+c}+\frac{2b}{c+a}+\frac{3c}{a+b}.
$$

We will denote the left-hand side as \( L \) and the right-hand side as \( R \):

- \( L = \frac{a}{2b} + \frac{b}{4c} + \frac{c}{a} \)
- \( R = \frac{3a}{b+c} + \frac{2b}{c+a} + \frac{3c}{a+b} \)

### Step 1: Analyze \( L \)

We can rewrite \( L \) in a more manageable form. To do this, we will find a common denominator for the fractions:

The common denominator for \( L \) is \( 4abc \):

\[
L = \frac{2a^2c + b^2a + 4c^2b}{4abc}
\]

### Step 2: Analyze \( R \)

Next, we analyze \( R \). The common denominator for \( R \) is \( (b+c)(c+a)(a+b) \). However, for simplicity, we will analyze the terms separately and use the Cauchy-Schwarz inequality.

Using Cauchy-Schwarz inequality, we can estimate \( R \):

\[
R = \frac{3a}{b+c} + \frac{2b}{c+a} + \frac{3c}{a+b} \geq \frac{(3a + 2b + 3c)^2}{3(b+c) + 2(c+a) + 3(a+b)}
\]

Calculating the denominator:

\[
3(b+c) + 2(c+a) + 3(a+b) = 3b + 3c + 2c + 2a + 3a + 3b = 5a + 6b + 5c
\]

Thus, we have:

\[
R \geq \frac{(3a + 2b + 3c)^2}{5a + 6b + 5c}
\]

### Step 3: Compare \( L \) and \( R \)

Now we need to compare \( L \) and \( R \). We can use specific values for \( a, b, c \) to test the inequality.

Letâ€™s take \( a = 1, b = 1, c = 1 \):

Calculating \( L \):

\[
L = \frac{1}{2 \cdot 1} + \frac{1}{4 \cdot 1} + \frac{1}{1} = \frac{1}{2} + \frac{1}{4} + 1 = \frac{2}{4} + \frac{1}{4} + \frac{4}{4} = \frac{7}{4}
\]

Calculating \( R \):

\[
R = \frac{3 \cdot 1}{1 + 1} + \frac{2 \cdot 1}{1 + 1} + \frac{3 \cdot 1}{1 + 1} = \frac{3}{2} + \frac{2}{2} + \frac{3}{2} = \frac{3}{2} + 1 + \frac{3}{2} = \frac{8}{2} = 4
\]

### Conclusion

Since \( L = \frac{7}{4} \) and \( R = 4 \), we have:

\[
\frac{7}{4} < 4
\]

Thus, we conclude that:

\[
L < R
\]

Therefore, the correct inequality relation is:

The answer is (D) $<$.