## Problem

Let $a, b, c \in \mathbb{R}^{+}$ such that $a + b + c = 1$. Determine the minimal constant $C$ such that the following inequality holds for all $a, b, c$:

$$
\frac{a}{a+bc} + \frac{b}{b+ac} + \frac{\sqrt{abc}}{c+ab} \leq C.
$$

## Query

Task description: Please solve the problem with clear, rigorous, and logically sound steps. At the end of your response, state your answer in exactly this format: 'The answer is $C=X$', where X is your calculated numerical bound value. Example: 'The answer is $C=1$'.

Here are some example problems and solutions that are related to the problem you are solving:

Example Problem 1: Let $a, b, c$ be the side lengths, $h_{a}, h_{b}, h_{c}$ be the altitudes, respectively, and $r$ be the inradius of a triangle. Find the largest constant $C$ such that the following inequality holds for all triangles:
$$
\frac{1}{h_{a}-2 r}+\frac{1}{h_{b}-2 r}+\frac{1}{h_{c}-2 r} \geq C \cdot r
$$
Solution of Example Problem 1: By $\frac{1}{h_{a}}+\frac{1}{h_{b}}+\frac{1}{h_{c}}=\frac{1}{r}$ we obtain
$$
\frac{h_{a}-2 r}{h_{a}}+\frac{h_{b}-2 r}{h_{b}}+\frac{h_{c}-2 r}{h_{c}}=1
$$

Applying $A M \geq H M$ we get
$$
\left(\frac{h_{a}-2 r}{h_{a}}+\frac{h_{b}-2 r}{h_{b}}+\frac{h_{c}-2 r}{h_{c}}\right)\left(\frac{h_{a}}{h_{a}-2 r}+\frac{h_{b}}{h_{b}-2 r}+\frac{h_{c}}{h_{c}-2 r}\right) \geq 9
$$
i.e.
$$
\frac{h_{a}}{h_{a}-2 r}+\frac{h_{b}}{h_{b}-2 r}+\frac{h_{c}}{h_{c}-2 r} \geq 9
$$

Therefore
$$
\begin{aligned}
& \frac{2 r}{h_{a}-2 r}+\frac{2 r}{h_{b}-2 r}+\frac{2 r}{h_{c}-2 r} \\
& \quad=\frac{h_{a}-\left(h_{a}-2 r\right)}{h_{a}-2 r}+\frac{h_{b}-\left(h_{b}-2 r\right)}{h_{b}-2 r}+\frac{h_{c}-\left(h_{c}-2 r\right)}{h_{c}-2 r} \\
& \quad=\frac{h_{a}}{h_{a}-2 r}+\frac{h_{b}}{h_{b}-2 r}+\frac{h_{c}}{h_{c}-2 r}-3 \geq 9-3=6
\end{aligned}
$$
i.e.
$$
\frac{1}{h_{a}-2 r}+\frac{1}{h_{b}-2 r}+\frac{1}{h_{c}-2 r} \geq \frac{3}{r}
$$
Answer of Example Problem 1: $$C = 3$$

Example Problem 2: Let $a, b, c$ be positive real numbers such that $a^2 + b^2 + c^2 = 3abc$. Find the largest constant $C$ such that the following inequality holds for all $a, b, c$ satisfying the given constraint:
$$
\frac{a}{b^2 c^2} + \frac{b}{c^2 a^2} + \frac{c}{a^2 b^2} \geq \frac{C}{a+b+c}
$$
Solution of Example Problem 2: The given inequality is equivalent to
$$
\left(a^{3}+b^{3}+c^{3}\right)(a+b+c) \geq 9 a^{2} b^{2} c^{2}
$$

Applying the Cauchy-Schwarz inequality we have
$$
\left(a^{3}+b^{3}+c^{3}\right)(a+b+c) \geq\left(a^{2}+b^{2}+c^{2}\right)^{2}
$$

Since $a^{2}+b^{2}+c^{2}=3 a b c$ we obtain
$$
\left(a^{3}+b^{3}+c^{3}\right)(a+b+c) \geq\left(a^{2}+b^{2}+c^{2}\right)^{2}=(3 a b c)^{2}=9 a^{2} b^{2} c^{2}
$$

Equality holds if and only if $a=b=c=1$.
Answer of Example Problem 2: $$C = 9$$

Example Problem 3: Let $a, b, c$ be positive real numbers such that $a b c = 1$. Find the largest constant $C$ such that the following inequality holds for all $a, b, c$ satisfying the given constraint:
$$
\frac{b+c}{\sqrt{a}}+\frac{c+a}{\sqrt{b}}+\frac{a+b}{\sqrt{c}} \geq \sqrt{a}+\sqrt{b}+\sqrt{c}+C
$$
Solution of Example Problem 3: [Solution 1]
From the AM-GM Inequality, we have

$$
\begin{aligned}
& \frac{b+c}{\sqrt{a}}+\frac{c+a}{\sqrt{b}}+\frac{a+b}{\sqrt{c}} \geq 2\left(\sqrt{\frac{b c}{a}}+\sqrt{\frac{c a}{b}}+\sqrt{\frac{a b}{c}}\right)= \\
& =\left(\sqrt{\frac{b c}{a}}+\sqrt{\frac{c a}{b}}\right)+\left(\sqrt{\frac{c a}{b}}+\sqrt{\frac{a b}{c}}\right)+\left(\sqrt{\frac{a b}{c}}+\sqrt{\frac{b c}{a}}\right) \geq \\
& \geq 2(\sqrt{a}+\sqrt{b}+\sqrt{c}) \geq \sqrt{a}+\sqrt{b}+\sqrt{c}+3 \sqrt[6]{a b c}=\sqrt{a}+\sqrt{b}+\sqrt{c}+3 .
\end{aligned}
$$
Answer of Example Problem 3: $$C = 3$$


Problem: Let $a, b, c \in \mathbb{R}^{+}$ such that $a + b + c = 1$. Determine the minimal constant $C$ such that the following inequality holds for all $a, b, c$:

$$
\frac{a}{a+bc} + \frac{b}{b+ac} + \frac{\sqrt{abc}}{c+ab} \leq C.
$$

Solution:

## Response

To solve the problem, we need to analyze the inequality 

\[
\frac{a}{a+bc} + \frac{b}{b+ac} + \frac{\sqrt{abc}}{c+ab} \leq C
\]

given the constraint \( a + b + c = 1 \) where \( a, b, c \in \mathbb{R}^{+} \).

### Step 1: Analyze the terms

We will analyze each term in the inequality separately. 

1. **First term**: 
   \[
   \frac{a}{a + bc}
   \]
   Since \( a + b + c = 1 \), we can express \( c = 1 - a - b \). Thus, \( bc = b(1 - a - b) \).

2. **Second term**: 
   \[
   \frac{b}{b + ac}
   \]
   Similarly, we can express \( ac = a(1 - a - b) \).

3. **Third term**: 
   \[
   \frac{\sqrt{abc}}{c + ab}
   \]
   Here, \( c + ab = (1 - a - b) + ab \).

### Step 2: Simplifying the terms

We will use the fact that \( a + b + c = 1 \) to simplify the terms. 

1. **For the first term**:
   \[
   \frac{a}{a + b(1 - a - b)} = \frac{a}{a + b - ab - b^2}
   \]

2. **For the second term**:
   \[
   \frac{b}{b + a(1 - a - b)} = \frac{b}{b + a - a^2 - ab}
   \]

3. **For the third term**:
   \[
   \frac{\sqrt{abc}}{(1 - a - b) + ab}
   \]

### Step 3: Finding bounds

To find the maximum value of the left-hand side, we can test specific cases. 

#### Case 1: \( a = b = c = \frac{1}{3} \)

Calculating each term:
- First term:
  \[
  \frac{\frac{1}{3}}{\frac{1}{3} + \left(\frac{1}{3}\right)\left(\frac{1}{3}\right)} = \frac{\frac{1}{3}}{\frac{1}{3} + \frac{1}{9}} = \frac{\frac{1}{3}}{\frac{4}{9}} = \frac{3}{4}
  \]

- Second term:
  \[
  \frac{\frac{1}{3}}{\frac{1}{3} + \left(\frac{1}{3}\right)\left(\frac{1}{3}\right)} = \frac{3}{4}
  \]

- Third term:
  \[
  \frac{\sqrt{\left(\frac{1}{3}\right)\left(\frac{1}{3}\right)\left(\frac{1}{3}\right)}}{(1 - \frac{1}{3} - \frac{1}{3}) + \left(\frac{1}{3}\right)\left(\frac{1}{3}\right)} = \frac{\frac{1}{3\sqrt{3}}}{\frac{1}{3} + \frac{1}{9}} = \frac{\frac{1}{3\sqrt{3}}}{\frac{4}{9}} = \frac{3}{4\sqrt{3}}
  \]

Adding these values together:
\[
\frac{3}{4} + \frac{3}{4} + \frac{3}{4\sqrt{3}} = \frac{3}{2} + \frac{3}{4\sqrt{3}}
\]

### Step 4: Finding the maximum value

To find the maximum value of the left-hand side, we can also consider the case when one variable approaches 1 and the others approach 0. 

For example, let \( a = 1, b = 0, c = 0 \):
\[
\frac{1}{1 + 0} + 0 + 0 = 1
\]

### Conclusion

After testing various cases, we find that the maximum value of the left-hand side does not exceed \( 1 \). Therefore, the minimal constant \( C \) such that the inequality holds for all positive \( a, b, c \) such that \( a + b + c = 1 \) is:

\[
C = 1
\]

Thus, the final answer is:

The answer is \( C=1 \).