## Problem

For $a, b > 0$, find the minimal constant $C$ such that the following inequality holds for all $a, b$:
$$
\frac{1}{2}(a+b)^2 + C(a+b) \geq a \sqrt{b} + b \sqrt{a}.
$$

## Query

Task description: Please solve the problem with clear, rigorous, and logically sound steps. At the end of your response, state your answer in exactly this format: 'The answer is $C=X$', where X is your calculated numerical bound value. Example: 'The answer is $C=1$'.

Here are some example problems and solutions that are related to the problem you are solving:

Example Problem 1: Let $a, b, c$ be the side lengths, $h_{a}, h_{b}, h_{c}$ be the altitudes, respectively, and $r$ be the inradius of a triangle. Find the largest constant $C$ such that the following inequality holds for all triangles:
$$
\frac{1}{h_{a}-2 r}+\frac{1}{h_{b}-2 r}+\frac{1}{h_{c}-2 r} \geq C \cdot r
$$
Solution of Example Problem 1: By $\frac{1}{h_{a}}+\frac{1}{h_{b}}+\frac{1}{h_{c}}=\frac{1}{r}$ we obtain
$$
\frac{h_{a}-2 r}{h_{a}}+\frac{h_{b}-2 r}{h_{b}}+\frac{h_{c}-2 r}{h_{c}}=1
$$

Applying $A M \geq H M$ we get
$$
\left(\frac{h_{a}-2 r}{h_{a}}+\frac{h_{b}-2 r}{h_{b}}+\frac{h_{c}-2 r}{h_{c}}\right)\left(\frac{h_{a}}{h_{a}-2 r}+\frac{h_{b}}{h_{b}-2 r}+\frac{h_{c}}{h_{c}-2 r}\right) \geq 9
$$
i.e.
$$
\frac{h_{a}}{h_{a}-2 r}+\frac{h_{b}}{h_{b}-2 r}+\frac{h_{c}}{h_{c}-2 r} \geq 9
$$

Therefore
$$
\begin{aligned}
& \frac{2 r}{h_{a}-2 r}+\frac{2 r}{h_{b}-2 r}+\frac{2 r}{h_{c}-2 r} \\
& \quad=\frac{h_{a}-\left(h_{a}-2 r\right)}{h_{a}-2 r}+\frac{h_{b}-\left(h_{b}-2 r\right)}{h_{b}-2 r}+\frac{h_{c}-\left(h_{c}-2 r\right)}{h_{c}-2 r} \\
& \quad=\frac{h_{a}}{h_{a}-2 r}+\frac{h_{b}}{h_{b}-2 r}+\frac{h_{c}}{h_{c}-2 r}-3 \geq 9-3=6
\end{aligned}
$$
i.e.
$$
\frac{1}{h_{a}-2 r}+\frac{1}{h_{b}-2 r}+\frac{1}{h_{c}-2 r} \geq \frac{3}{r}
$$
Answer of Example Problem 1: $$C = 3$$

Example Problem 2: Let $a, b, c$ be positive real numbers such that $a^2 + b^2 + c^2 = 3abc$. Find the largest constant $C$ such that the following inequality holds for all $a, b, c$ satisfying the given constraint:
$$
\frac{a}{b^2 c^2} + \frac{b}{c^2 a^2} + \frac{c}{a^2 b^2} \geq \frac{C}{a+b+c}
$$
Solution of Example Problem 2: The given inequality is equivalent to
$$
\left(a^{3}+b^{3}+c^{3}\right)(a+b+c) \geq 9 a^{2} b^{2} c^{2}
$$

Applying the Cauchy-Schwarz inequality we have
$$
\left(a^{3}+b^{3}+c^{3}\right)(a+b+c) \geq\left(a^{2}+b^{2}+c^{2}\right)^{2}
$$

Since $a^{2}+b^{2}+c^{2}=3 a b c$ we obtain
$$
\left(a^{3}+b^{3}+c^{3}\right)(a+b+c) \geq\left(a^{2}+b^{2}+c^{2}\right)^{2}=(3 a b c)^{2}=9 a^{2} b^{2} c^{2}
$$

Equality holds if and only if $a=b=c=1$.
Answer of Example Problem 2: $$C = 9$$

Example Problem 3: Let $a, b, c$ be positive real numbers such that $a b c = 1$. Find the largest constant $C$ such that the following inequality holds for all $a, b, c$ satisfying the given constraint:
$$
\frac{b+c}{\sqrt{a}}+\frac{c+a}{\sqrt{b}}+\frac{a+b}{\sqrt{c}} \geq \sqrt{a}+\sqrt{b}+\sqrt{c}+C
$$
Solution of Example Problem 3: [Solution 1]
From the AM-GM Inequality, we have

$$
\begin{aligned}
& \frac{b+c}{\sqrt{a}}+\frac{c+a}{\sqrt{b}}+\frac{a+b}{\sqrt{c}} \geq 2\left(\sqrt{\frac{b c}{a}}+\sqrt{\frac{c a}{b}}+\sqrt{\frac{a b}{c}}\right)= \\
& =\left(\sqrt{\frac{b c}{a}}+\sqrt{\frac{c a}{b}}\right)+\left(\sqrt{\frac{c a}{b}}+\sqrt{\frac{a b}{c}}\right)+\left(\sqrt{\frac{a b}{c}}+\sqrt{\frac{b c}{a}}\right) \geq \\
& \geq 2(\sqrt{a}+\sqrt{b}+\sqrt{c}) \geq \sqrt{a}+\sqrt{b}+\sqrt{c}+3 \sqrt[6]{a b c}=\sqrt{a}+\sqrt{b}+\sqrt{c}+3 .
\end{aligned}
$$
Answer of Example Problem 3: $$C = 3$$


Problem: For $a, b > 0$, find the minimal constant $C$ such that the following inequality holds for all $a, b$:
$$
\frac{1}{2}(a+b)^2 + C(a+b) \geq a \sqrt{b} + b \sqrt{a}.
$$

Solution:

## Response

To solve the inequality 

\[
\frac{1}{2}(a+b)^2 + C(a+b) \geq a \sqrt{b} + b \sqrt{a}
\]

for all positive \(a\) and \(b\), we start by rewriting the left-hand side:

\[
\frac{1}{2}(a+b)^2 + C(a+b) = \frac{1}{2}(a^2 + 2ab + b^2) + C(a+b) = \frac{1}{2}a^2 + ab + \frac{1}{2}b^2 + Ca + Cb.
\]

Now, we need to analyze the right-hand side:

\[
a \sqrt{b} + b \sqrt{a}.
\]

To find the minimal constant \(C\), we will consider specific cases for \(a\) and \(b\). 

### Case 1: Let \(a = b\)

Set \(a = b = x\). Then the inequality becomes:

\[
\frac{1}{2}(2x)^2 + C(2x) \geq x \sqrt{x} + x \sqrt{x}.
\]

This simplifies to:

\[
\frac{1}{2}(4x^2) + 2Cx \geq 2x^{3/2}.
\]

Thus, we have:

\[
2x^2 + 2Cx \geq 2x^{3/2}.
\]

Dividing through by 2 gives:

\[
x^2 + Cx \geq x^{3/2}.
\]

Rearranging yields:

\[
x^2 - x^{3/2} + Cx \geq 0.
\]

Factoring out \(x^{3/2}\):

\[
x^{3/2} - Cx - x^2 \leq 0.
\]

### Case 2: Let \(b = 1\)

Now, let \(b = 1\) and \(a = x\). The inequality becomes:

\[
\frac{1}{2}(x + 1)^2 + C(x + 1) \geq x.
\]

Expanding the left-hand side:

\[
\frac{1}{2}(x^2 + 2x + 1) + C(x + 1) \geq x.
\]

This simplifies to:

\[
\frac{1}{2}x^2 + (1 + C)x + \frac{1}{2} \geq x.
\]

Rearranging gives:

\[
\frac{1}{2}x^2 + (C)x + \frac{1}{2} \geq 0.
\]

### Finding the Minimum \(C\)

To ensure the quadratic \( \frac{1}{2}x^2 + Cx + \frac{1}{2} \geq 0 \) has no real roots, the discriminant must be non-positive:

\[
C^2 - 4 \cdot \frac{1}{2} \cdot \frac{1}{2} \leq 0.
\]

Calculating the discriminant:

\[
C^2 - 1 \leq 0 \implies C^2 \leq 1 \implies |C| \leq 1.
\]

Thus, the maximum value of \(C\) is \(1\). 

### Conclusion

To satisfy the inequality for all positive \(a\) and \(b\), the minimal constant \(C\) must be:

\[
C = 1.
\]

Thus, the answer is:

\[
\text{The answer is } C=1.
\]