## Problem

Let $a_1, a_2, \ldots, a_n$ be positive real numbers. Determine the minimal constant $C$ such that the following inequality holds for all $a_1, a_2, \ldots, a_n$:

$$
\left(a_1+\ldots+a_n\right)^2 \leq C\left(1^2 a_1^2+2^2 a_2^2+\ldots+n^2 a_n^2\right)
$$

## Query

Task description: Please solve the problem with clear, rigorous, and logically sound steps. At the end of your response, state your answer in exactly this format: 'The answer is $C=X$', where X is your calculated numerical bound value. Example: 'The answer is $C=1$'.

Here are some example problems and solutions that are related to the problem you are solving:

Example Problem 1: Let $a, b, c$ be the side lengths, $h_{a}, h_{b}, h_{c}$ be the altitudes, respectively, and $r$ be the inradius of a triangle. Find the largest constant $C$ such that the following inequality holds for all triangles:
$$
\frac{1}{h_{a}-2 r}+\frac{1}{h_{b}-2 r}+\frac{1}{h_{c}-2 r} \geq C \cdot r
$$
Solution of Example Problem 1: By $\frac{1}{h_{a}}+\frac{1}{h_{b}}+\frac{1}{h_{c}}=\frac{1}{r}$ we obtain
$$
\frac{h_{a}-2 r}{h_{a}}+\frac{h_{b}-2 r}{h_{b}}+\frac{h_{c}-2 r}{h_{c}}=1
$$

Applying $A M \geq H M$ we get
$$
\left(\frac{h_{a}-2 r}{h_{a}}+\frac{h_{b}-2 r}{h_{b}}+\frac{h_{c}-2 r}{h_{c}}\right)\left(\frac{h_{a}}{h_{a}-2 r}+\frac{h_{b}}{h_{b}-2 r}+\frac{h_{c}}{h_{c}-2 r}\right) \geq 9
$$
i.e.
$$
\frac{h_{a}}{h_{a}-2 r}+\frac{h_{b}}{h_{b}-2 r}+\frac{h_{c}}{h_{c}-2 r} \geq 9
$$

Therefore
$$
\begin{aligned}
& \frac{2 r}{h_{a}-2 r}+\frac{2 r}{h_{b}-2 r}+\frac{2 r}{h_{c}-2 r} \\
& \quad=\frac{h_{a}-\left(h_{a}-2 r\right)}{h_{a}-2 r}+\frac{h_{b}-\left(h_{b}-2 r\right)}{h_{b}-2 r}+\frac{h_{c}-\left(h_{c}-2 r\right)}{h_{c}-2 r} \\
& \quad=\frac{h_{a}}{h_{a}-2 r}+\frac{h_{b}}{h_{b}-2 r}+\frac{h_{c}}{h_{c}-2 r}-3 \geq 9-3=6
\end{aligned}
$$
i.e.
$$
\frac{1}{h_{a}-2 r}+\frac{1}{h_{b}-2 r}+\frac{1}{h_{c}-2 r} \geq \frac{3}{r}
$$
Answer of Example Problem 1: $$C = 3$$

Example Problem 2: Let $a, b, c$ be positive real numbers such that $a^2 + b^2 + c^2 = 3abc$. Find the largest constant $C$ such that the following inequality holds for all $a, b, c$ satisfying the given constraint:
$$
\frac{a}{b^2 c^2} + \frac{b}{c^2 a^2} + \frac{c}{a^2 b^2} \geq \frac{C}{a+b+c}
$$
Solution of Example Problem 2: The given inequality is equivalent to
$$
\left(a^{3}+b^{3}+c^{3}\right)(a+b+c) \geq 9 a^{2} b^{2} c^{2}
$$

Applying the Cauchy-Schwarz inequality we have
$$
\left(a^{3}+b^{3}+c^{3}\right)(a+b+c) \geq\left(a^{2}+b^{2}+c^{2}\right)^{2}
$$

Since $a^{2}+b^{2}+c^{2}=3 a b c$ we obtain
$$
\left(a^{3}+b^{3}+c^{3}\right)(a+b+c) \geq\left(a^{2}+b^{2}+c^{2}\right)^{2}=(3 a b c)^{2}=9 a^{2} b^{2} c^{2}
$$

Equality holds if and only if $a=b=c=1$.
Answer of Example Problem 2: $$C = 9$$

Example Problem 3: Let $a, b, c$ be positive real numbers such that $a b c = 1$. Find the largest constant $C$ such that the following inequality holds for all $a, b, c$ satisfying the given constraint:
$$
\frac{b+c}{\sqrt{a}}+\frac{c+a}{\sqrt{b}}+\frac{a+b}{\sqrt{c}} \geq \sqrt{a}+\sqrt{b}+\sqrt{c}+C
$$
Solution of Example Problem 3: [Solution 1]
From the AM-GM Inequality, we have

$$
\begin{aligned}
& \frac{b+c}{\sqrt{a}}+\frac{c+a}{\sqrt{b}}+\frac{a+b}{\sqrt{c}} \geq 2\left(\sqrt{\frac{b c}{a}}+\sqrt{\frac{c a}{b}}+\sqrt{\frac{a b}{c}}\right)= \\
& =\left(\sqrt{\frac{b c}{a}}+\sqrt{\frac{c a}{b}}\right)+\left(\sqrt{\frac{c a}{b}}+\sqrt{\frac{a b}{c}}\right)+\left(\sqrt{\frac{a b}{c}}+\sqrt{\frac{b c}{a}}\right) \geq \\
& \geq 2(\sqrt{a}+\sqrt{b}+\sqrt{c}) \geq \sqrt{a}+\sqrt{b}+\sqrt{c}+3 \sqrt[6]{a b c}=\sqrt{a}+\sqrt{b}+\sqrt{c}+3 .
\end{aligned}
$$
Answer of Example Problem 3: $$C = 3$$


Problem: Let $a_1, a_2, \ldots, a_n$ be positive real numbers. Determine the minimal constant $C$ such that the following inequality holds for all $a_1, a_2, \ldots, a_n$:

$$
\left(a_1+\ldots+a_n\right)^2 \leq C\left(1^2 a_1^2+2^2 a_2^2+\ldots+n^2 a_n^2\right)
$$

Solution:

## Response

To solve the problem, we need to find the minimal constant \( C \) such that the following inequality holds for all positive real numbers \( a_1, a_2, \ldots, a_n \):

\[
\left(a_1 + a_2 + \ldots + a_n\right)^2 \leq C\left(1^2 a_1^2 + 2^2 a_2^2 + \ldots + n^2 a_n^2\right).
\]

We can apply the Cauchy-Schwarz inequality to the left-hand side and the right-hand side of the inequality. The Cauchy-Schwarz inequality states that for any sequences of real numbers \( x_1, x_2, \ldots, x_n \) and \( y_1, y_2, \ldots, y_n \):

\[
(x_1^2 + x_2^2 + \ldots + x_n^2)(y_1^2 + y_2^2 + \ldots + y_n^2) \geq (x_1y_1 + x_2y_2 + \ldots + x_ny_n)^2.
\]

In our case, we can set:

- \( x_i = i a_i \) for \( i = 1, 2, \ldots, n \)
- \( y_i = 1 \) for all \( i \)

Then, we have:

\[
\left(1^2 + 2^2 + \ldots + n^2\right)\left(a_1^2 + a_2^2 + \ldots + a_n^2\right) \geq \left(a_1 + a_2 + \ldots + a_n\right)^2.
\]

This can be rewritten as:

\[
\left(1^2 + 2^2 + \ldots + n^2\right) \cdot \left(a_1^2 + a_2^2 + \ldots + a_n^2\right) \geq \left(a_1 + a_2 + \ldots + a_n\right)^2.
\]

Now, we denote \( S = a_1 + a_2 + \ldots + a_n \) and \( T = 1^2 a_1^2 + 2^2 a_2^2 + \ldots + n^2 a_n^2 \). The inequality we derived gives us:

\[
S^2 \leq (1^2 + 2^2 + \ldots + n^2) T.
\]

Thus, we can express \( C \) as:

\[
C \geq \frac{S^2}{T} \cdot \frac{1}{1^2 + 2^2 + \ldots + n^2}.
\]

To find the minimal \( C \), we need to evaluate \( 1^2 + 2^2 + \ldots + n^2 \). The formula for the sum of squares is:

\[
1^2 + 2^2 + \ldots + n^2 = \frac{n(n+1)(2n+1)}{6}.
\]

Now, we can set \( a_i = 1 \) for all \( i \) (i.e., \( a_1 = a_2 = \ldots = a_n = 1 \)). Then:

\[
S = n,
\]
and

\[
T = 1^2 + 2^2 + \ldots + n^2 = \frac{n(n+1)(2n+1)}{6}.
\]

Substituting these into our inequality gives:

\[
n^2 \leq C \cdot \frac{n(n+1)(2n+1)}{6}.
\]

Dividing both sides by \( n \) (since \( n > 0 \)):

\[
n \leq C \cdot \frac{(n+1)(2n+1)}{6}.
\]

Rearranging gives:

\[
C \geq \frac{6n}{(n+1)(2n+1)}.
\]

To find the minimum value of \( C \), we can analyze the limit as \( n \to \infty \):

\[
\lim_{n \to \infty} \frac{6n}{(n+1)(2n+1)} = \lim_{n \to \infty} \frac{6}{2} = 3.
\]

Thus, the minimal constant \( C \) that satisfies the inequality for all positive real numbers \( a_1, a_2, \ldots, a_n \) is:

\[
C = 3.
\]

Therefore, the answer is:

The answer is \( C=3 \).