## Problem

Let $a, b, c$ be the side lengths of a triangle. Determine the largest constant $C$ such that the following inequality holds for all $a, b, c$ satisfying the triangle inequality:
$$
\frac{b+c}{a}+\frac{c+a}{b}+\frac{a+b}{c}+\frac{(b+c-a)(c+a-b)(a+b-c)}{a b c} \geq C.
$$

## Query

Task description: Please solve the problem with clear, rigorous, and logically sound steps. At the end of your response, state your answer in exactly this format: 'The answer is $C=X$', where X is your calculated numerical bound value. Example: 'The answer is $C=1$'.

Here are some example problems and solutions that are related to the problem you are solving:

Example Problem 1: Let $a, b, c$ be the side lengths, $h_{a}, h_{b}, h_{c}$ be the altitudes, respectively, and $r$ be the inradius of a triangle. Find the largest constant $C$ such that the following inequality holds for all triangles:
$$
\frac{1}{h_{a}-2 r}+\frac{1}{h_{b}-2 r}+\frac{1}{h_{c}-2 r} \geq C \cdot r
$$
Solution of Example Problem 1: By $\frac{1}{h_{a}}+\frac{1}{h_{b}}+\frac{1}{h_{c}}=\frac{1}{r}$ we obtain
$$
\frac{h_{a}-2 r}{h_{a}}+\frac{h_{b}-2 r}{h_{b}}+\frac{h_{c}-2 r}{h_{c}}=1
$$

Applying $A M \geq H M$ we get
$$
\left(\frac{h_{a}-2 r}{h_{a}}+\frac{h_{b}-2 r}{h_{b}}+\frac{h_{c}-2 r}{h_{c}}\right)\left(\frac{h_{a}}{h_{a}-2 r}+\frac{h_{b}}{h_{b}-2 r}+\frac{h_{c}}{h_{c}-2 r}\right) \geq 9
$$
i.e.
$$
\frac{h_{a}}{h_{a}-2 r}+\frac{h_{b}}{h_{b}-2 r}+\frac{h_{c}}{h_{c}-2 r} \geq 9
$$

Therefore
$$
\begin{aligned}
& \frac{2 r}{h_{a}-2 r}+\frac{2 r}{h_{b}-2 r}+\frac{2 r}{h_{c}-2 r} \\
& \quad=\frac{h_{a}-\left(h_{a}-2 r\right)}{h_{a}-2 r}+\frac{h_{b}-\left(h_{b}-2 r\right)}{h_{b}-2 r}+\frac{h_{c}-\left(h_{c}-2 r\right)}{h_{c}-2 r} \\
& \quad=\frac{h_{a}}{h_{a}-2 r}+\frac{h_{b}}{h_{b}-2 r}+\frac{h_{c}}{h_{c}-2 r}-3 \geq 9-3=6
\end{aligned}
$$
i.e.
$$
\frac{1}{h_{a}-2 r}+\frac{1}{h_{b}-2 r}+\frac{1}{h_{c}-2 r} \geq \frac{3}{r}
$$
Answer of Example Problem 1: $$C = 3$$

Example Problem 2: Let $a, b, c$ be positive real numbers such that $a^2 + b^2 + c^2 = 3abc$. Find the largest constant $C$ such that the following inequality holds for all $a, b, c$ satisfying the given constraint:
$$
\frac{a}{b^2 c^2} + \frac{b}{c^2 a^2} + \frac{c}{a^2 b^2} \geq \frac{C}{a+b+c}
$$
Solution of Example Problem 2: The given inequality is equivalent to
$$
\left(a^{3}+b^{3}+c^{3}\right)(a+b+c) \geq 9 a^{2} b^{2} c^{2}
$$

Applying the Cauchy-Schwarz inequality we have
$$
\left(a^{3}+b^{3}+c^{3}\right)(a+b+c) \geq\left(a^{2}+b^{2}+c^{2}\right)^{2}
$$

Since $a^{2}+b^{2}+c^{2}=3 a b c$ we obtain
$$
\left(a^{3}+b^{3}+c^{3}\right)(a+b+c) \geq\left(a^{2}+b^{2}+c^{2}\right)^{2}=(3 a b c)^{2}=9 a^{2} b^{2} c^{2}
$$

Equality holds if and only if $a=b=c=1$.
Answer of Example Problem 2: $$C = 9$$

Example Problem 3: Let $a, b, c$ be positive real numbers such that $a b c = 1$. Find the largest constant $C$ such that the following inequality holds for all $a, b, c$ satisfying the given constraint:
$$
\frac{b+c}{\sqrt{a}}+\frac{c+a}{\sqrt{b}}+\frac{a+b}{\sqrt{c}} \geq \sqrt{a}+\sqrt{b}+\sqrt{c}+C
$$
Solution of Example Problem 3: [Solution 1]
From the AM-GM Inequality, we have

$$
\begin{aligned}
& \frac{b+c}{\sqrt{a}}+\frac{c+a}{\sqrt{b}}+\frac{a+b}{\sqrt{c}} \geq 2\left(\sqrt{\frac{b c}{a}}+\sqrt{\frac{c a}{b}}+\sqrt{\frac{a b}{c}}\right)= \\
& =\left(\sqrt{\frac{b c}{a}}+\sqrt{\frac{c a}{b}}\right)+\left(\sqrt{\frac{c a}{b}}+\sqrt{\frac{a b}{c}}\right)+\left(\sqrt{\frac{a b}{c}}+\sqrt{\frac{b c}{a}}\right) \geq \\
& \geq 2(\sqrt{a}+\sqrt{b}+\sqrt{c}) \geq \sqrt{a}+\sqrt{b}+\sqrt{c}+3 \sqrt[6]{a b c}=\sqrt{a}+\sqrt{b}+\sqrt{c}+3 .
\end{aligned}
$$
Answer of Example Problem 3: $$C = 3$$


Problem: Let $a, b, c$ be the side lengths of a triangle. Determine the largest constant $C$ such that the following inequality holds for all $a, b, c$ satisfying the triangle inequality:
$$
\frac{b+c}{a}+\frac{c+a}{b}+\frac{a+b}{c}+\frac{(b+c-a)(c+a-b)(a+b-c)}{a b c} \geq C.
$$

Solution:

## Response

To solve the problem, we start with the given inequality:

\[
\frac{b+c}{a}+\frac{c+a}{b}+\frac{a+b}{c}+\frac{(b+c-a)(c+a-b)(a+b-c)}{abc} \geq C.
\]

### Step 1: Simplifying the Left Side

We can rewrite the first three terms using the triangle inequality. For any triangle with sides \(a\), \(b\), and \(c\), we know that:

\[
\frac{b+c}{a} \geq 1, \quad \frac{c+a}{b} \geq 1, \quad \frac{a+b}{c} \geq 1.
\]

Thus, we have:

\[
\frac{b+c}{a} + \frac{c+a}{b} + \frac{a+b}{c} \geq 3.
\]

### Step 2: Analyzing the Second Term

Next, we need to analyze the term \(\frac{(b+c-a)(c+a-b)(a+b-c)}{abc}\). 

Let \(x = b+c-a\), \(y = c+a-b\), and \(z = a+b-c\). By the triangle inequality, \(x\), \(y\), and \(z\) are all positive. We can express \(x\), \(y\), and \(z\) in terms of \(a\), \(b\), and \(c\):

- \(x = b+c-a\)
- \(y = c+a-b\)
- \(z = a+b-c\)

### Step 3: Finding a Lower Bound for the Product

The product \(xyz\) can be expressed as:

\[
xyz = (b+c-a)(c+a-b)(a+b-c).
\]

Using the AM-GM inequality, we can find a lower bound for \(xyz\):

\[
xyz \leq \left(\frac{(b+c) + (c+a) + (a+b)}{3} - \frac{a+b+c}{3}\right)^3 = \left(\frac{2(a+b+c)}{3} - \frac{a+b+c}{3}\right)^3 = \left(\frac{(a+b+c)}{3}\right)^3.
\]

However, we need to find a more direct approach to evaluate the term \(\frac{xyz}{abc}\).

### Step 4: Evaluating the Expression

We can evaluate the expression \(\frac{(b+c-a)(c+a-b)(a+b-c)}{abc}\) at specific values of \(a\), \(b\), and \(c\). 

Letâ€™s consider the case where \(a = b = c = 1\):

\[
\frac{(1+1-1)(1+1-1)(1+1-1)}{1 \cdot 1 \cdot 1} = \frac{1 \cdot 1 \cdot 1}{1} = 1.
\]

Thus, we have:

\[
\frac{b+c}{a} + \frac{c+a}{b} + \frac{a+b}{c} = 3 + 1 = 4.
\]

### Step 5: Generalizing the Result

Now, we need to check if this holds for other triangles. The minimum value of \(\frac{(b+c-a)(c+a-b)(a+b-c)}{abc}\) is indeed \(1\) when \(a = b = c\). 

Thus, we can conclude that:

\[
\frac{b+c}{a} + \frac{c+a}{b} + \frac{a+b}{c} + 1 \geq 4.
\]

### Conclusion

Therefore, the largest constant \(C\) such that the inequality holds for all triangles is:

\[
C = 4.
\]

Thus, the final answer is:

The answer is \(C=4\).