## Problem

Let $x, y, z \in \mathbb{R}$ satisfy the following constraints:
$$
\left\{\begin{array}{r}
x^2+x y+y^2=16 ; \\
y^2+y z+z^2=3 ;
\end{array}\right.
$$

Find the smallest constant $C$ such that the following inequality holds for all $x, y, z$ satisfying the constraints:
$$
x y+y z+z x \leq C.
$$

## Query

Task description: Please solve the problem with clear, rigorous, and logically sound steps. At the end of your response, state your answer in exactly this format: 'The answer is $C=X$', where X is your calculated numerical bound value. Example: 'The answer is $C=1$'.

Here are some example problems and solutions that are related to the problem you are solving:

Example Problem 1: Let $a, b, c$ be the side lengths, $h_{a}, h_{b}, h_{c}$ be the altitudes, respectively, and $r$ be the inradius of a triangle. Find the largest constant $C$ such that the following inequality holds for all triangles:
$$
\frac{1}{h_{a}-2 r}+\frac{1}{h_{b}-2 r}+\frac{1}{h_{c}-2 r} \geq C \cdot r
$$
Solution of Example Problem 1: By $\frac{1}{h_{a}}+\frac{1}{h_{b}}+\frac{1}{h_{c}}=\frac{1}{r}$ we obtain
$$
\frac{h_{a}-2 r}{h_{a}}+\frac{h_{b}-2 r}{h_{b}}+\frac{h_{c}-2 r}{h_{c}}=1
$$

Applying $A M \geq H M$ we get
$$
\left(\frac{h_{a}-2 r}{h_{a}}+\frac{h_{b}-2 r}{h_{b}}+\frac{h_{c}-2 r}{h_{c}}\right)\left(\frac{h_{a}}{h_{a}-2 r}+\frac{h_{b}}{h_{b}-2 r}+\frac{h_{c}}{h_{c}-2 r}\right) \geq 9
$$
i.e.
$$
\frac{h_{a}}{h_{a}-2 r}+\frac{h_{b}}{h_{b}-2 r}+\frac{h_{c}}{h_{c}-2 r} \geq 9
$$

Therefore
$$
\begin{aligned}
& \frac{2 r}{h_{a}-2 r}+\frac{2 r}{h_{b}-2 r}+\frac{2 r}{h_{c}-2 r} \\
& \quad=\frac{h_{a}-\left(h_{a}-2 r\right)}{h_{a}-2 r}+\frac{h_{b}-\left(h_{b}-2 r\right)}{h_{b}-2 r}+\frac{h_{c}-\left(h_{c}-2 r\right)}{h_{c}-2 r} \\
& \quad=\frac{h_{a}}{h_{a}-2 r}+\frac{h_{b}}{h_{b}-2 r}+\frac{h_{c}}{h_{c}-2 r}-3 \geq 9-3=6
\end{aligned}
$$
i.e.
$$
\frac{1}{h_{a}-2 r}+\frac{1}{h_{b}-2 r}+\frac{1}{h_{c}-2 r} \geq \frac{3}{r}
$$
Answer of Example Problem 1: $$C = 3$$

Example Problem 2: Let $a, b, c$ be positive real numbers such that $a^2 + b^2 + c^2 = 3abc$. Find the largest constant $C$ such that the following inequality holds for all $a, b, c$ satisfying the given constraint:
$$
\frac{a}{b^2 c^2} + \frac{b}{c^2 a^2} + \frac{c}{a^2 b^2} \geq \frac{C}{a+b+c}
$$
Solution of Example Problem 2: The given inequality is equivalent to
$$
\left(a^{3}+b^{3}+c^{3}\right)(a+b+c) \geq 9 a^{2} b^{2} c^{2}
$$

Applying the Cauchy-Schwarz inequality we have
$$
\left(a^{3}+b^{3}+c^{3}\right)(a+b+c) \geq\left(a^{2}+b^{2}+c^{2}\right)^{2}
$$

Since $a^{2}+b^{2}+c^{2}=3 a b c$ we obtain
$$
\left(a^{3}+b^{3}+c^{3}\right)(a+b+c) \geq\left(a^{2}+b^{2}+c^{2}\right)^{2}=(3 a b c)^{2}=9 a^{2} b^{2} c^{2}
$$

Equality holds if and only if $a=b=c=1$.
Answer of Example Problem 2: $$C = 9$$

Example Problem 3: Let $a, b, c$ be positive real numbers such that $a b c = 1$. Find the largest constant $C$ such that the following inequality holds for all $a, b, c$ satisfying the given constraint:
$$
\frac{b+c}{\sqrt{a}}+\frac{c+a}{\sqrt{b}}+\frac{a+b}{\sqrt{c}} \geq \sqrt{a}+\sqrt{b}+\sqrt{c}+C
$$
Solution of Example Problem 3: [Solution 1]
From the AM-GM Inequality, we have

$$
\begin{aligned}
& \frac{b+c}{\sqrt{a}}+\frac{c+a}{\sqrt{b}}+\frac{a+b}{\sqrt{c}} \geq 2\left(\sqrt{\frac{b c}{a}}+\sqrt{\frac{c a}{b}}+\sqrt{\frac{a b}{c}}\right)= \\
& =\left(\sqrt{\frac{b c}{a}}+\sqrt{\frac{c a}{b}}\right)+\left(\sqrt{\frac{c a}{b}}+\sqrt{\frac{a b}{c}}\right)+\left(\sqrt{\frac{a b}{c}}+\sqrt{\frac{b c}{a}}\right) \geq \\
& \geq 2(\sqrt{a}+\sqrt{b}+\sqrt{c}) \geq \sqrt{a}+\sqrt{b}+\sqrt{c}+3 \sqrt[6]{a b c}=\sqrt{a}+\sqrt{b}+\sqrt{c}+3 .
\end{aligned}
$$
Answer of Example Problem 3: $$C = 3$$


Problem: Let $x, y, z \in \mathbb{R}$ satisfy the following constraints:
$$
\left\{\begin{array}{r}
x^2+x y+y^2=16 ; \\
y^2+y z+z^2=3 ;
\end{array}\right.
$$

Find the smallest constant $C$ such that the following inequality holds for all $x, y, z$ satisfying the constraints:
$$
x y+y z+z x \leq C.
$$

Solution:

## Response

To solve the problem, we need to analyze the given constraints and find the maximum value of the expression \( xy + yz + zx \).

We have the following constraints:

1. \( x^2 + xy + y^2 = 16 \)
2. \( y^2 + yz + z^2 = 3 \)

We will express \( xy + yz + zx \) in terms of \( y \) and the other variables.

### Step 1: Express \( x \) in terms of \( y \)

From the first constraint, we can rearrange it to express \( x \):

\[
x^2 + xy + y^2 = 16 \implies x^2 + xy = 16 - y^2
\]

This is a quadratic equation in \( x \):

\[
x^2 + xy - (16 - y^2) = 0
\]

Using the quadratic formula, we find:

\[
x = \frac{-y \pm \sqrt{y^2 + 4(16 - y^2)}}{2} = \frac{-y \pm \sqrt{64 - 3y^2}}{2}
\]

### Step 2: Express \( z \) in terms of \( y \)

From the second constraint, we can express \( z \):

\[
y^2 + yz + z^2 = 3 \implies z^2 + yz = 3 - y^2
\]

This is also a quadratic equation in \( z \):

\[
z^2 + yz - (3 - y^2) = 0
\]

Using the quadratic formula, we find:

\[
z = \frac{-y \pm \sqrt{y^2 + 4(3 - y^2)}}{2} = \frac{-y \pm \sqrt{12 - 3y^2}}{2}
\]

### Step 3: Analyze \( xy + yz + zx \)

Now we can express \( xy + yz + zx \):

\[
xy + yz + zx = yx + y \left( \frac{-y \pm \sqrt{12 - 3y^2}}{2} \right) + \left( \frac{-y \pm \sqrt{64 - 3y^2}}{2} \right) z
\]

However, this expression is quite complex. Instead, we can use the constraints to find bounds for \( xy + yz + zx \).

### Step 4: Use the constraints to find bounds

1. From \( x^2 + xy + y^2 = 16 \), we can deduce that \( x \) and \( y \) cannot be too large. Specifically, if we set \( y = 0 \), we find \( x^2 = 16 \) which gives \( x = 4 \) or \( x = -4 \).

2. From \( y^2 + yz + z^2 = 3 \), if we set \( y = 0 \), we find \( z^2 = 3 \) which gives \( z = \sqrt{3} \) or \( z = -\sqrt{3} \).

### Step 5: Calculate \( xy + yz + zx \) for boundary cases

- If \( y = 0 \), then \( xy + yz + zx = 0 \).
- If \( y = 2 \) (which is a reasonable value since \( 2^2 + 2z + z^2 = 3 \) gives \( z = -1 \)), we can calculate:

\[
x^2 + 2x + 4 = 16 \implies x^2 + 2x - 12 = 0 \implies (x - 4)(x + 3) = 0 \implies x = 4 \text{ or } x = -3
\]

Calculating \( xy + yz + zx \):

- For \( x = 4, y = 2, z = -1 \):

\[
xy + yz + zx = 4 \cdot 2 + 2 \cdot (-1) + 4 \cdot (-1) = 8 - 2 - 4 = 2
\]

- For \( x = -3, y = 2, z = -1 \):

\[
xy + yz + zx = -3 \cdot 2 + 2 \cdot (-1) + (-3) \cdot (-1) = -6 - 2 + 3 = -5
\]

### Conclusion

The maximum value of \( xy + yz + zx \) we found is \( 2 \). Therefore, the smallest constant \( C \) such that \( xy + yz + zx \leq C \) for all \( x, y, z \) satisfying the constraints is:

\[
\boxed{2}
\]

Thus, the final answer is:

The answer is \( C=2 \).