## Problem

Let $a, b, c$ be positive real numbers greater than 1. Find the smallest constant $C$ such that the following inequality holds for all $a, b, c > 1$:
$$
\sqrt{a-1} + \sqrt{b-1} + \sqrt{c-1} \leq 3C \sqrt{c(ab+1)}
$$

## Query

Task description: Please solve the problem with clear, rigorous, and logically sound steps. At the end of your response, state your answer in exactly this format: 'The answer is $C=X$', where X is your calculated numerical bound value. Example: 'The answer is $C=1$'.

Here are some example problems and solutions that are related to the problem you are solving:

Example Problem 1: Let $a, b, c$ be the side lengths, $h_{a}, h_{b}, h_{c}$ be the altitudes, respectively, and $r$ be the inradius of a triangle. Find the largest constant $C$ such that the following inequality holds for all triangles:
$$
\frac{1}{h_{a}-2 r}+\frac{1}{h_{b}-2 r}+\frac{1}{h_{c}-2 r} \geq C \cdot r
$$
Solution of Example Problem 1: By $\frac{1}{h_{a}}+\frac{1}{h_{b}}+\frac{1}{h_{c}}=\frac{1}{r}$ we obtain
$$
\frac{h_{a}-2 r}{h_{a}}+\frac{h_{b}-2 r}{h_{b}}+\frac{h_{c}-2 r}{h_{c}}=1
$$

Applying $A M \geq H M$ we get
$$
\left(\frac{h_{a}-2 r}{h_{a}}+\frac{h_{b}-2 r}{h_{b}}+\frac{h_{c}-2 r}{h_{c}}\right)\left(\frac{h_{a}}{h_{a}-2 r}+\frac{h_{b}}{h_{b}-2 r}+\frac{h_{c}}{h_{c}-2 r}\right) \geq 9
$$
i.e.
$$
\frac{h_{a}}{h_{a}-2 r}+\frac{h_{b}}{h_{b}-2 r}+\frac{h_{c}}{h_{c}-2 r} \geq 9
$$

Therefore
$$
\begin{aligned}
& \frac{2 r}{h_{a}-2 r}+\frac{2 r}{h_{b}-2 r}+\frac{2 r}{h_{c}-2 r} \\
& \quad=\frac{h_{a}-\left(h_{a}-2 r\right)}{h_{a}-2 r}+\frac{h_{b}-\left(h_{b}-2 r\right)}{h_{b}-2 r}+\frac{h_{c}-\left(h_{c}-2 r\right)}{h_{c}-2 r} \\
& \quad=\frac{h_{a}}{h_{a}-2 r}+\frac{h_{b}}{h_{b}-2 r}+\frac{h_{c}}{h_{c}-2 r}-3 \geq 9-3=6
\end{aligned}
$$
i.e.
$$
\frac{1}{h_{a}-2 r}+\frac{1}{h_{b}-2 r}+\frac{1}{h_{c}-2 r} \geq \frac{3}{r}
$$
Answer of Example Problem 1: $$C = 3$$

Example Problem 2: Let $a, b, c$ be positive real numbers such that $a^2 + b^2 + c^2 = 3abc$. Find the largest constant $C$ such that the following inequality holds for all $a, b, c$ satisfying the given constraint:
$$
\frac{a}{b^2 c^2} + \frac{b}{c^2 a^2} + \frac{c}{a^2 b^2} \geq \frac{C}{a+b+c}
$$
Solution of Example Problem 2: The given inequality is equivalent to
$$
\left(a^{3}+b^{3}+c^{3}\right)(a+b+c) \geq 9 a^{2} b^{2} c^{2}
$$

Applying the Cauchy-Schwarz inequality we have
$$
\left(a^{3}+b^{3}+c^{3}\right)(a+b+c) \geq\left(a^{2}+b^{2}+c^{2}\right)^{2}
$$

Since $a^{2}+b^{2}+c^{2}=3 a b c$ we obtain
$$
\left(a^{3}+b^{3}+c^{3}\right)(a+b+c) \geq\left(a^{2}+b^{2}+c^{2}\right)^{2}=(3 a b c)^{2}=9 a^{2} b^{2} c^{2}
$$

Equality holds if and only if $a=b=c=1$.
Answer of Example Problem 2: $$C = 9$$

Example Problem 3: Let $a, b, c$ be positive real numbers such that $a b c = 1$. Find the largest constant $C$ such that the following inequality holds for all $a, b, c$ satisfying the given constraint:
$$
\frac{b+c}{\sqrt{a}}+\frac{c+a}{\sqrt{b}}+\frac{a+b}{\sqrt{c}} \geq \sqrt{a}+\sqrt{b}+\sqrt{c}+C
$$
Solution of Example Problem 3: [Solution 1]
From the AM-GM Inequality, we have

$$
\begin{aligned}
& \frac{b+c}{\sqrt{a}}+\frac{c+a}{\sqrt{b}}+\frac{a+b}{\sqrt{c}} \geq 2\left(\sqrt{\frac{b c}{a}}+\sqrt{\frac{c a}{b}}+\sqrt{\frac{a b}{c}}\right)= \\
& =\left(\sqrt{\frac{b c}{a}}+\sqrt{\frac{c a}{b}}\right)+\left(\sqrt{\frac{c a}{b}}+\sqrt{\frac{a b}{c}}\right)+\left(\sqrt{\frac{a b}{c}}+\sqrt{\frac{b c}{a}}\right) \geq \\
& \geq 2(\sqrt{a}+\sqrt{b}+\sqrt{c}) \geq \sqrt{a}+\sqrt{b}+\sqrt{c}+3 \sqrt[6]{a b c}=\sqrt{a}+\sqrt{b}+\sqrt{c}+3 .
\end{aligned}
$$
Answer of Example Problem 3: $$C = 3$$


Problem: Let $a, b, c$ be positive real numbers greater than 1. Find the smallest constant $C$ such that the following inequality holds for all $a, b, c > 1$:
$$
\sqrt{a-1} + \sqrt{b-1} + \sqrt{c-1} \leq 3C \sqrt{c(ab+1)}
$$

Solution:

## Response

To solve the problem, we need to find the smallest constant \( C \) such that the inequality 

\[
\sqrt{a-1} + \sqrt{b-1} + \sqrt{c-1} \leq 3C \sqrt{c(ab+1)}
\]

holds for all positive real numbers \( a, b, c > 1 \).

### Step 1: Analyze the left-hand side

We start with the left-hand side:

\[
\sqrt{a-1} + \sqrt{b-1} + \sqrt{c-1}
\]

Since \( a, b, c > 1 \), we can express \( a-1, b-1, c-1 \) as positive quantities. 

### Step 2: Analyze the right-hand side

Now, consider the right-hand side:

\[
3C \sqrt{c(ab+1)}
\]

We need to find a relationship between the left-hand side and the right-hand side. 

### Step 3: Test specific values

To find \( C \), we can test specific values of \( a, b, c \). A natural choice is to set \( a = b = c \). Let \( a = b = c = x \) where \( x > 1 \).

Then the inequality becomes:

\[
3\sqrt{x-1} \leq 3C \sqrt{x(x^2 + 1)}
\]

Dividing both sides by 3 gives:

\[
\sqrt{x-1} \leq C \sqrt{x(x^2 + 1)}
\]

### Step 4: Square both sides

Squaring both sides results in:

\[
x - 1 \leq C^2 x(x^2 + 1)
\]

This simplifies to:

\[
x - 1 \leq C^2 (x^3 + x)
\]

Rearranging gives:

\[
x - C^2 x^3 - C^2 x + 1 \leq 0
\]

This can be rewritten as:

\[
-C^2 x^3 + (1 - C^2)x + 1 \leq 0
\]

### Step 5: Analyze the cubic polynomial

The cubic polynomial \( -C^2 x^3 + (1 - C^2)x + 1 \) must be non-positive for all \( x > 1 \). 

To ensure this, we can analyze the behavior of the polynomial as \( x \to 1 \):

Substituting \( x = 1 \):

\[
-C^2(1)^3 + (1 - C^2)(1) + 1 = -C^2 + (1 - C^2) + 1 = 2 - 2C^2
\]

For this to be non-positive:

\[
2 - 2C^2 \leq 0 \implies C^2 \geq 1 \implies C \geq 1
\]

### Step 6: Check if \( C = 1 \) works

Now we check if \( C = 1 \) satisfies the original inequality:

\[
\sqrt{a-1} + \sqrt{b-1} + \sqrt{c-1} \leq 3\sqrt{c(ab+1)}
\]

Testing \( a = b = c = 2 \):

\[
\sqrt{2-1} + \sqrt{2-1} + \sqrt{2-1} = 3 \leq 3\sqrt{2(2 \cdot 2 + 1)} = 3\sqrt{10}
\]

This holds true since \( 3 \leq 3\sqrt{10} \).

### Conclusion

Thus, the smallest constant \( C \) such that the inequality holds for all \( a, b, c > 1 \) is:

\[
\boxed{1}
\]

Therefore, the final answer is:

The answer is \( C=1 \).