## Problem

Let $a, b, c \in \mathbb{R}$ such that $a + 2b + 3c = 2$ and $2ab + 3ac + 6bc = 1$. Determine the minimal constants $C$ such that the following inequalities hold for all $a$ satisfying the given constraints:
$$
a \leq C
$$

## Query

Task description: Please solve the problem with clear, rigorous, and logically sound steps. At the end of your response, state your answer in exactly this format: 'The answer is $C=X$', where X is your calculated numerical bound value. Example: 'The answer is $C=1$'.

Here are some example problems and solutions that are related to the problem you are solving:

Example Problem 1: Let $a, b, c$ be the side lengths, $h_{a}, h_{b}, h_{c}$ be the altitudes, respectively, and $r$ be the inradius of a triangle. Find the largest constant $C$ such that the following inequality holds for all triangles:
$$
\frac{1}{h_{a}-2 r}+\frac{1}{h_{b}-2 r}+\frac{1}{h_{c}-2 r} \geq C \cdot r
$$
Solution of Example Problem 1: By $\frac{1}{h_{a}}+\frac{1}{h_{b}}+\frac{1}{h_{c}}=\frac{1}{r}$ we obtain
$$
\frac{h_{a}-2 r}{h_{a}}+\frac{h_{b}-2 r}{h_{b}}+\frac{h_{c}-2 r}{h_{c}}=1
$$

Applying $A M \geq H M$ we get
$$
\left(\frac{h_{a}-2 r}{h_{a}}+\frac{h_{b}-2 r}{h_{b}}+\frac{h_{c}-2 r}{h_{c}}\right)\left(\frac{h_{a}}{h_{a}-2 r}+\frac{h_{b}}{h_{b}-2 r}+\frac{h_{c}}{h_{c}-2 r}\right) \geq 9
$$
i.e.
$$
\frac{h_{a}}{h_{a}-2 r}+\frac{h_{b}}{h_{b}-2 r}+\frac{h_{c}}{h_{c}-2 r} \geq 9
$$

Therefore
$$
\begin{aligned}
& \frac{2 r}{h_{a}-2 r}+\frac{2 r}{h_{b}-2 r}+\frac{2 r}{h_{c}-2 r} \\
& \quad=\frac{h_{a}-\left(h_{a}-2 r\right)}{h_{a}-2 r}+\frac{h_{b}-\left(h_{b}-2 r\right)}{h_{b}-2 r}+\frac{h_{c}-\left(h_{c}-2 r\right)}{h_{c}-2 r} \\
& \quad=\frac{h_{a}}{h_{a}-2 r}+\frac{h_{b}}{h_{b}-2 r}+\frac{h_{c}}{h_{c}-2 r}-3 \geq 9-3=6
\end{aligned}
$$
i.e.
$$
\frac{1}{h_{a}-2 r}+\frac{1}{h_{b}-2 r}+\frac{1}{h_{c}-2 r} \geq \frac{3}{r}
$$
Answer of Example Problem 1: $$C = 3$$

Example Problem 2: Let $a, b, c$ be positive real numbers such that $a^2 + b^2 + c^2 = 3abc$. Find the largest constant $C$ such that the following inequality holds for all $a, b, c$ satisfying the given constraint:
$$
\frac{a}{b^2 c^2} + \frac{b}{c^2 a^2} + \frac{c}{a^2 b^2} \geq \frac{C}{a+b+c}
$$
Solution of Example Problem 2: The given inequality is equivalent to
$$
\left(a^{3}+b^{3}+c^{3}\right)(a+b+c) \geq 9 a^{2} b^{2} c^{2}
$$

Applying the Cauchy-Schwarz inequality we have
$$
\left(a^{3}+b^{3}+c^{3}\right)(a+b+c) \geq\left(a^{2}+b^{2}+c^{2}\right)^{2}
$$

Since $a^{2}+b^{2}+c^{2}=3 a b c$ we obtain
$$
\left(a^{3}+b^{3}+c^{3}\right)(a+b+c) \geq\left(a^{2}+b^{2}+c^{2}\right)^{2}=(3 a b c)^{2}=9 a^{2} b^{2} c^{2}
$$

Equality holds if and only if $a=b=c=1$.
Answer of Example Problem 2: $$C = 9$$

Example Problem 3: Let $a, b, c$ be positive real numbers such that $a b c = 1$. Find the largest constant $C$ such that the following inequality holds for all $a, b, c$ satisfying the given constraint:
$$
\frac{b+c}{\sqrt{a}}+\frac{c+a}{\sqrt{b}}+\frac{a+b}{\sqrt{c}} \geq \sqrt{a}+\sqrt{b}+\sqrt{c}+C
$$
Solution of Example Problem 3: [Solution 1]
From the AM-GM Inequality, we have

$$
\begin{aligned}
& \frac{b+c}{\sqrt{a}}+\frac{c+a}{\sqrt{b}}+\frac{a+b}{\sqrt{c}} \geq 2\left(\sqrt{\frac{b c}{a}}+\sqrt{\frac{c a}{b}}+\sqrt{\frac{a b}{c}}\right)= \\
& =\left(\sqrt{\frac{b c}{a}}+\sqrt{\frac{c a}{b}}\right)+\left(\sqrt{\frac{c a}{b}}+\sqrt{\frac{a b}{c}}\right)+\left(\sqrt{\frac{a b}{c}}+\sqrt{\frac{b c}{a}}\right) \geq \\
& \geq 2(\sqrt{a}+\sqrt{b}+\sqrt{c}) \geq \sqrt{a}+\sqrt{b}+\sqrt{c}+3 \sqrt[6]{a b c}=\sqrt{a}+\sqrt{b}+\sqrt{c}+3 .
\end{aligned}
$$
Answer of Example Problem 3: $$C = 3$$


Problem: Let $a, b, c \in \mathbb{R}$ such that $a + 2b + 3c = 2$ and $2ab + 3ac + 6bc = 1$. Determine the minimal constants $C$ such that the following inequalities hold for all $a$ satisfying the given constraints:
$$
a \leq C
$$

Solution:

## Response

To solve the problem, we start with the constraints given:

1. \( a + 2b + 3c = 2 \)
2. \( 2ab + 3ac + 6bc = 1 \)

We need to find the maximum value of \( a \) under these constraints.

### Step 1: Express \( b \) and \( c \) in terms of \( a \)

From the first equation, we can express \( b \) and \( c \) in terms of \( a \):

\[
2b + 3c = 2 - a \quad \text{(1)}
\]

From equation (1), we can express \( b \) in terms of \( c \):

\[
b = \frac{2 - a - 3c}{2} \quad \text{(2)}
\]

### Step 2: Substitute \( b \) into the second equation

Now we substitute equation (2) into the second constraint:

\[
2ab + 3ac + 6bc = 1
\]

Substituting \( b \):

\[
2a\left(\frac{2 - a - 3c}{2}\right) + 3ac + 6\left(\frac{2 - a - 3c}{2}\right)c = 1
\]

This simplifies to:

\[
a(2 - a - 3c) + 3ac + 3(2 - a - 3c)c = 1
\]

Expanding this gives:

\[
2a - a^2 - 3ac + 3ac + 6c - 3ac - 9c^2 = 1
\]

This simplifies to:

\[
2a - a^2 + 6c - 9c^2 = 1
\]

Rearranging gives:

\[
-a^2 + 2a + 6c - 9c^2 = 1
\]

### Step 3: Solve for \( c \)

Rearranging the equation gives:

\[
9c^2 - 6c + (a^2 - 2a + 1) = 0
\]

This is a quadratic in \( c \). For \( c \) to have real solutions, the discriminant must be non-negative:

\[
D = (-6)^2 - 4 \cdot 9 \cdot (a^2 - 2a + 1) \geq 0
\]

Calculating the discriminant:

\[
36 - 36(a^2 - 2a + 1) \geq 0
\]

This simplifies to:

\[
36 - 36a^2 + 72a - 36 \geq 0
\]

Thus:

\[
-36a^2 + 72a \geq 0
\]

Factoring out \( -36 \):

\[
a(2 - a) \geq 0
\]

### Step 4: Determine the bounds for \( a \)

The inequality \( a(2 - a) \geq 0 \) holds when:

1. \( a \leq 0 \)
2. \( a \geq 2 \)

However, since \( a \) must be non-negative (as it is part of a linear combination that sums to 2), we only consider:

\[
0 \leq a \leq 2
\]

### Step 5: Conclusion

The maximum value of \( a \) that satisfies both constraints is \( 2 \). Therefore, the largest constant \( C \) such that \( a \leq C \) for all \( a \) satisfying the given constraints is:

\[
\text{The answer is } C=2.
\]