## Problem

Find the smallest constant $C$ such that for all non-negative real numbers $a, b, c$, the following inequality holds:
$$
\sqrt{\frac{a b+b c+c a}{3}} \leq C \cdot \sqrt[3]{\frac{(a+b)(b+c)(c+a)}{2}}
$$

## Query

Task description: Please solve the problem with clear, rigorous, and logically sound steps. At the end of your response, state your answer in exactly this format: 'The answer is $C=X$', where X is your calculated numerical bound value. Example: 'The answer is $C=1$'.

Here are some example problems and solutions that are related to the problem you are solving:

Example Problem 1: Let $a, b, c$ be the side lengths, $h_{a}, h_{b}, h_{c}$ be the altitudes, respectively, and $r$ be the inradius of a triangle. Find the largest constant $C$ such that the following inequality holds for all triangles:
$$
\frac{1}{h_{a}-2 r}+\frac{1}{h_{b}-2 r}+\frac{1}{h_{c}-2 r} \geq C \cdot r
$$
Solution of Example Problem 1: By $\frac{1}{h_{a}}+\frac{1}{h_{b}}+\frac{1}{h_{c}}=\frac{1}{r}$ we obtain
$$
\frac{h_{a}-2 r}{h_{a}}+\frac{h_{b}-2 r}{h_{b}}+\frac{h_{c}-2 r}{h_{c}}=1
$$

Applying $A M \geq H M$ we get
$$
\left(\frac{h_{a}-2 r}{h_{a}}+\frac{h_{b}-2 r}{h_{b}}+\frac{h_{c}-2 r}{h_{c}}\right)\left(\frac{h_{a}}{h_{a}-2 r}+\frac{h_{b}}{h_{b}-2 r}+\frac{h_{c}}{h_{c}-2 r}\right) \geq 9
$$
i.e.
$$
\frac{h_{a}}{h_{a}-2 r}+\frac{h_{b}}{h_{b}-2 r}+\frac{h_{c}}{h_{c}-2 r} \geq 9
$$

Therefore
$$
\begin{aligned}
& \frac{2 r}{h_{a}-2 r}+\frac{2 r}{h_{b}-2 r}+\frac{2 r}{h_{c}-2 r} \\
& \quad=\frac{h_{a}-\left(h_{a}-2 r\right)}{h_{a}-2 r}+\frac{h_{b}-\left(h_{b}-2 r\right)}{h_{b}-2 r}+\frac{h_{c}-\left(h_{c}-2 r\right)}{h_{c}-2 r} \\
& \quad=\frac{h_{a}}{h_{a}-2 r}+\frac{h_{b}}{h_{b}-2 r}+\frac{h_{c}}{h_{c}-2 r}-3 \geq 9-3=6
\end{aligned}
$$
i.e.
$$
\frac{1}{h_{a}-2 r}+\frac{1}{h_{b}-2 r}+\frac{1}{h_{c}-2 r} \geq \frac{3}{r}
$$
Answer of Example Problem 1: $$C = 3$$

Example Problem 2: Let $a, b, c$ be positive real numbers such that $a^2 + b^2 + c^2 = 3abc$. Find the largest constant $C$ such that the following inequality holds for all $a, b, c$ satisfying the given constraint:
$$
\frac{a}{b^2 c^2} + \frac{b}{c^2 a^2} + \frac{c}{a^2 b^2} \geq \frac{C}{a+b+c}
$$
Solution of Example Problem 2: The given inequality is equivalent to
$$
\left(a^{3}+b^{3}+c^{3}\right)(a+b+c) \geq 9 a^{2} b^{2} c^{2}
$$

Applying the Cauchy-Schwarz inequality we have
$$
\left(a^{3}+b^{3}+c^{3}\right)(a+b+c) \geq\left(a^{2}+b^{2}+c^{2}\right)^{2}
$$

Since $a^{2}+b^{2}+c^{2}=3 a b c$ we obtain
$$
\left(a^{3}+b^{3}+c^{3}\right)(a+b+c) \geq\left(a^{2}+b^{2}+c^{2}\right)^{2}=(3 a b c)^{2}=9 a^{2} b^{2} c^{2}
$$

Equality holds if and only if $a=b=c=1$.
Answer of Example Problem 2: $$C = 9$$

Example Problem 3: Let $a, b, c$ be positive real numbers such that $a b c = 1$. Find the largest constant $C$ such that the following inequality holds for all $a, b, c$ satisfying the given constraint:
$$
\frac{b+c}{\sqrt{a}}+\frac{c+a}{\sqrt{b}}+\frac{a+b}{\sqrt{c}} \geq \sqrt{a}+\sqrt{b}+\sqrt{c}+C
$$
Solution of Example Problem 3: [Solution 1]
From the AM-GM Inequality, we have

$$
\begin{aligned}
& \frac{b+c}{\sqrt{a}}+\frac{c+a}{\sqrt{b}}+\frac{a+b}{\sqrt{c}} \geq 2\left(\sqrt{\frac{b c}{a}}+\sqrt{\frac{c a}{b}}+\sqrt{\frac{a b}{c}}\right)= \\
& =\left(\sqrt{\frac{b c}{a}}+\sqrt{\frac{c a}{b}}\right)+\left(\sqrt{\frac{c a}{b}}+\sqrt{\frac{a b}{c}}\right)+\left(\sqrt{\frac{a b}{c}}+\sqrt{\frac{b c}{a}}\right) \geq \\
& \geq 2(\sqrt{a}+\sqrt{b}+\sqrt{c}) \geq \sqrt{a}+\sqrt{b}+\sqrt{c}+3 \sqrt[6]{a b c}=\sqrt{a}+\sqrt{b}+\sqrt{c}+3 .
\end{aligned}
$$
Answer of Example Problem 3: $$C = 3$$


Problem: Find the smallest constant $C$ such that for all non-negative real numbers $a, b, c$, the following inequality holds:
$$
\sqrt{\frac{a b+b c+c a}{3}} \leq C \cdot \sqrt[3]{\frac{(a+b)(b+c)(c+a)}{2}}
$$

Solution:

## Response

To solve the problem, we need to find the smallest constant \( C \) such that the following inequality holds for all non-negative real numbers \( a, b, c \):

\[
\sqrt{\frac{ab + bc + ca}{3}} \leq C \cdot \sqrt[3]{\frac{(a+b)(b+c)(c+a)}{2}}.
\]

### Step 1: Analyze the left-hand side

The left-hand side of the inequality is:

\[
L = \sqrt{\frac{ab + bc + ca}{3}}.
\]

### Step 2: Analyze the right-hand side

The right-hand side of the inequality is:

\[
R = C \cdot \sqrt[3]{\frac{(a+b)(b+c)(c+a)}{2}}.
\]

### Step 3: Test specific cases

To find the smallest \( C \), we can test specific cases of \( a, b, c \).

#### Case 1: \( a = b = c = 1 \)

In this case:

\[
L = \sqrt{\frac{1 \cdot 1 + 1 \cdot 1 + 1 \cdot 1}{3}} = \sqrt{1} = 1,
\]

and

\[
R = C \cdot \sqrt[3]{\frac{(1+1)(1+1)(1+1)}{2}} = C \cdot \sqrt[3]{\frac{2 \cdot 2 \cdot 2}{2}} = C \cdot \sqrt[3]{4} = C \cdot 2^{2/3}.
\]

Thus, we have:

\[
1 \leq C \cdot 2^{2/3} \implies C \geq \frac{1}{2^{2/3}}.
\]

#### Case 2: \( a = 1, b = 1, c = 0 \)

In this case:

\[
L = \sqrt{\frac{1 \cdot 1 + 1 \cdot 0 + 0 \cdot 1}{3}} = \sqrt{\frac{1}{3}} = \frac{1}{\sqrt{3}},
\]

and

\[
R = C \cdot \sqrt[3]{\frac{(1+1)(1+0)(0+1)}{2}} = C \cdot \sqrt[3]{\frac{2 \cdot 1 \cdot 1}{2}} = C \cdot \sqrt[3]{1} = C.
\]

Thus, we have:

\[
\frac{1}{\sqrt{3}} \leq C \implies C \geq \frac{1}{\sqrt{3}}.
\]

### Step 4: Compare the bounds

Now we have two bounds for \( C \):

1. \( C \geq \frac{1}{2^{2/3}} \)
2. \( C \geq \frac{1}{\sqrt{3}} \)

Next, we need to compare \( \frac{1}{2^{2/3}} \) and \( \frac{1}{\sqrt{3}} \).

Calculating these values:

- \( 2^{2/3} \approx 1.5874 \) implies \( \frac{1}{2^{2/3}} \approx 0.6299 \).
- \( \sqrt{3} \approx 1.732 \) implies \( \frac{1}{\sqrt{3}} \approx 0.5774 \).

Since \( \frac{1}{2^{2/3}} \approx 0.6299 > \frac{1}{\sqrt{3}} \approx 0.5774 \), the tighter bound is:

\[
C \geq \frac{1}{2^{2/3}}.
\]

### Step 5: Conclusion

Thus, the smallest constant \( C \) that satisfies the inequality for all non-negative real numbers \( a, b, c \) is:

\[
C = \frac{1}{2^{2/3}}.
\]

Therefore, the answer is:

\[
\text{The answer is } C = \frac{1}{2^{2/3}}.
\]