## Problem

For positive reals $x, y, z$, determine the largest constant $C$ such that the following inequality holds for all $x, y, z \in \mathbb{R}^{+}$:

$$
\sum_{cyc} \frac{x(y+z)^2}{2x+y+z} + \frac{9}{2}\left(\frac{x+y+z}{xy+yz+zx}\right)^2 \geq C + \frac{9}{2(xy+yz+zx)}
$$

## Query

Task description: Please solve the problem with clear, rigorous, and logically sound steps. At the end of your response, state your answer in exactly this format: 'The answer is $C=X$', where X is your calculated numerical bound value. Example: 'The answer is $C=1$'.

Here are some example problems and solutions that are related to the problem you are solving:

Example Problem 1: Let $a, b, c$ be the side lengths, $h_{a}, h_{b}, h_{c}$ be the altitudes, respectively, and $r$ be the inradius of a triangle. Find the largest constant $C$ such that the following inequality holds for all triangles:
$$
\frac{1}{h_{a}-2 r}+\frac{1}{h_{b}-2 r}+\frac{1}{h_{c}-2 r} \geq C \cdot r
$$
Solution of Example Problem 1: By $\frac{1}{h_{a}}+\frac{1}{h_{b}}+\frac{1}{h_{c}}=\frac{1}{r}$ we obtain
$$
\frac{h_{a}-2 r}{h_{a}}+\frac{h_{b}-2 r}{h_{b}}+\frac{h_{c}-2 r}{h_{c}}=1
$$

Applying $A M \geq H M$ we get
$$
\left(\frac{h_{a}-2 r}{h_{a}}+\frac{h_{b}-2 r}{h_{b}}+\frac{h_{c}-2 r}{h_{c}}\right)\left(\frac{h_{a}}{h_{a}-2 r}+\frac{h_{b}}{h_{b}-2 r}+\frac{h_{c}}{h_{c}-2 r}\right) \geq 9
$$
i.e.
$$
\frac{h_{a}}{h_{a}-2 r}+\frac{h_{b}}{h_{b}-2 r}+\frac{h_{c}}{h_{c}-2 r} \geq 9
$$

Therefore
$$
\begin{aligned}
& \frac{2 r}{h_{a}-2 r}+\frac{2 r}{h_{b}-2 r}+\frac{2 r}{h_{c}-2 r} \\
& \quad=\frac{h_{a}-\left(h_{a}-2 r\right)}{h_{a}-2 r}+\frac{h_{b}-\left(h_{b}-2 r\right)}{h_{b}-2 r}+\frac{h_{c}-\left(h_{c}-2 r\right)}{h_{c}-2 r} \\
& \quad=\frac{h_{a}}{h_{a}-2 r}+\frac{h_{b}}{h_{b}-2 r}+\frac{h_{c}}{h_{c}-2 r}-3 \geq 9-3=6
\end{aligned}
$$
i.e.
$$
\frac{1}{h_{a}-2 r}+\frac{1}{h_{b}-2 r}+\frac{1}{h_{c}-2 r} \geq \frac{3}{r}
$$
Answer of Example Problem 1: $$C = 3$$

Example Problem 2: Let $a, b, c$ be positive real numbers such that $a^2 + b^2 + c^2 = 3abc$. Find the largest constant $C$ such that the following inequality holds for all $a, b, c$ satisfying the given constraint:
$$
\frac{a}{b^2 c^2} + \frac{b}{c^2 a^2} + \frac{c}{a^2 b^2} \geq \frac{C}{a+b+c}
$$
Solution of Example Problem 2: The given inequality is equivalent to
$$
\left(a^{3}+b^{3}+c^{3}\right)(a+b+c) \geq 9 a^{2} b^{2} c^{2}
$$

Applying the Cauchy-Schwarz inequality we have
$$
\left(a^{3}+b^{3}+c^{3}\right)(a+b+c) \geq\left(a^{2}+b^{2}+c^{2}\right)^{2}
$$

Since $a^{2}+b^{2}+c^{2}=3 a b c$ we obtain
$$
\left(a^{3}+b^{3}+c^{3}\right)(a+b+c) \geq\left(a^{2}+b^{2}+c^{2}\right)^{2}=(3 a b c)^{2}=9 a^{2} b^{2} c^{2}
$$

Equality holds if and only if $a=b=c=1$.
Answer of Example Problem 2: $$C = 9$$

Example Problem 3: Let $a, b, c$ be positive real numbers such that $a b c = 1$. Find the largest constant $C$ such that the following inequality holds for all $a, b, c$ satisfying the given constraint:
$$
\frac{b+c}{\sqrt{a}}+\frac{c+a}{\sqrt{b}}+\frac{a+b}{\sqrt{c}} \geq \sqrt{a}+\sqrt{b}+\sqrt{c}+C
$$
Solution of Example Problem 3: [Solution 1]
From the AM-GM Inequality, we have

$$
\begin{aligned}
& \frac{b+c}{\sqrt{a}}+\frac{c+a}{\sqrt{b}}+\frac{a+b}{\sqrt{c}} \geq 2\left(\sqrt{\frac{b c}{a}}+\sqrt{\frac{c a}{b}}+\sqrt{\frac{a b}{c}}\right)= \\
& =\left(\sqrt{\frac{b c}{a}}+\sqrt{\frac{c a}{b}}\right)+\left(\sqrt{\frac{c a}{b}}+\sqrt{\frac{a b}{c}}\right)+\left(\sqrt{\frac{a b}{c}}+\sqrt{\frac{b c}{a}}\right) \geq \\
& \geq 2(\sqrt{a}+\sqrt{b}+\sqrt{c}) \geq \sqrt{a}+\sqrt{b}+\sqrt{c}+3 \sqrt[6]{a b c}=\sqrt{a}+\sqrt{b}+\sqrt{c}+3 .
\end{aligned}
$$
Answer of Example Problem 3: $$C = 3$$


Problem: For positive reals $x, y, z$, determine the largest constant $C$ such that the following inequality holds for all $x, y, z \in \mathbb{R}^{+}$:

$$
\sum_{cyc} \frac{x(y+z)^2}{2x+y+z} + \frac{9}{2}\left(\frac{x+y+z}{xy+yz+zx}\right)^2 \geq C + \frac{9}{2(xy+yz+zx)}
$$

Solution:

## Response

To solve the problem, we need to analyze the given inequality:

\[
\sum_{cyc} \frac{x(y+z)^2}{2x+y+z} + \frac{9}{2}\left(\frac{x+y+z}{xy+yz+zx}\right)^2 \geq C + \frac{9}{2(xy+yz+zx)}
\]

We will start by simplifying the left-hand side and exploring the terms involved.

### Step 1: Analyze the cyclic sum

The cyclic sum can be expanded as follows:

\[
\sum_{cyc} \frac{x(y+z)^2}{2x+y+z} = \frac{x(y^2 + 2yz + z^2)}{2x + y + z} + \frac{y(z^2 + 2zx + x^2)}{2y + z + x} + \frac{z(x^2 + 2xy + y^2)}{2z + x + y}
\]

This expression is symmetric in \(x, y, z\) and can be analyzed for specific cases, such as when \(x = y = z\).

### Step 2: Test with \(x = y = z\)

Let \(x = y = z = t\). Then we have:

\[
xy + yz + zx = 3t^2
\]

Substituting into the inequality gives:

\[
\sum_{cyc} \frac{t(2t)^2}{2t + 2t} + \frac{9}{2}\left(\frac{3t}{3t^2}\right)^2 \geq C + \frac{9}{2(3t^2)}
\]

Calculating the left-hand side:

\[
\sum_{cyc} \frac{t(4t^2)}{4t} = \sum_{cyc} t^2 = 3t^2
\]

And for the second term:

\[
\frac{9}{2}\left(\frac{3t}{3t^2}\right)^2 = \frac{9}{2}\left(\frac{1}{t}\right)^2 = \frac{9}{2t^2}
\]

Thus, the left-hand side becomes:

\[
3t^2 + \frac{9}{2t^2}
\]

### Step 3: Combine and simplify

Now we need to analyze:

\[
3t^2 + \frac{9}{2t^2} \geq C + \frac{3}{2t^2}
\]

Rearranging gives:

\[
3t^2 + \frac{9}{2t^2} - \frac{3}{2t^2} \geq C
\]

This simplifies to:

\[
3t^2 + \frac{6}{2t^2} \geq C
\]

### Step 4: Find the minimum value

To find the minimum value of \(3t^2 + \frac{6}{2t^2}\), we can use calculus or the AM-GM inequality. 

Using AM-GM:

\[
3t^2 + 3t^2 + 3t^2 + \frac{6}{2t^2} \geq 4\sqrt[4]{(3t^2)^3 \cdot \frac{6}{2t^2}} = 4\sqrt[4]{\frac{54t^6}{2t^2}} = 4\sqrt[4]{27t^4} = 12\sqrt{3}t
\]

Setting \(t = 1\) gives:

\[
3 + 3 = 6
\]

Thus, the minimum value occurs at \(t = 1\) and is equal to \(6\).

### Conclusion

The largest constant \(C\) such that the inequality holds for all positive reals \(x, y, z\) is:

\[
C = 6
\]

Thus, the final answer is:

The answer is \(C=6\).