## Problem

Let $a$ and $b$ be non-negative real numbers such that $a \geq b$. Determine the largest constant $C$ such that the following inequality holds for all $a \geq b \geq 0$:
$$
a + \frac{1}{b(a-b)} \geq C.
$$

## Query

Task description: Please solve the problem with clear, rigorous, and logically sound steps. At the end of your response, state your answer in exactly this format: 'The answer is $C=X$', where X is your calculated numerical bound value. Example: 'The answer is $C=1$'.

Here are some example problems and solutions that are related to the problem you are solving:

Example Problem 1: Let $a, b, c$ be the side lengths, $h_{a}, h_{b}, h_{c}$ be the altitudes, respectively, and $r$ be the inradius of a triangle. Find the largest constant $C$ such that the following inequality holds for all triangles:
$$
\frac{1}{h_{a}-2 r}+\frac{1}{h_{b}-2 r}+\frac{1}{h_{c}-2 r} \geq C \cdot r
$$
Solution of Example Problem 1: By $\frac{1}{h_{a}}+\frac{1}{h_{b}}+\frac{1}{h_{c}}=\frac{1}{r}$ we obtain
$$
\frac{h_{a}-2 r}{h_{a}}+\frac{h_{b}-2 r}{h_{b}}+\frac{h_{c}-2 r}{h_{c}}=1
$$

Applying $A M \geq H M$ we get
$$
\left(\frac{h_{a}-2 r}{h_{a}}+\frac{h_{b}-2 r}{h_{b}}+\frac{h_{c}-2 r}{h_{c}}\right)\left(\frac{h_{a}}{h_{a}-2 r}+\frac{h_{b}}{h_{b}-2 r}+\frac{h_{c}}{h_{c}-2 r}\right) \geq 9
$$
i.e.
$$
\frac{h_{a}}{h_{a}-2 r}+\frac{h_{b}}{h_{b}-2 r}+\frac{h_{c}}{h_{c}-2 r} \geq 9
$$

Therefore
$$
\begin{aligned}
& \frac{2 r}{h_{a}-2 r}+\frac{2 r}{h_{b}-2 r}+\frac{2 r}{h_{c}-2 r} \\
& \quad=\frac{h_{a}-\left(h_{a}-2 r\right)}{h_{a}-2 r}+\frac{h_{b}-\left(h_{b}-2 r\right)}{h_{b}-2 r}+\frac{h_{c}-\left(h_{c}-2 r\right)}{h_{c}-2 r} \\
& \quad=\frac{h_{a}}{h_{a}-2 r}+\frac{h_{b}}{h_{b}-2 r}+\frac{h_{c}}{h_{c}-2 r}-3 \geq 9-3=6
\end{aligned}
$$
i.e.
$$
\frac{1}{h_{a}-2 r}+\frac{1}{h_{b}-2 r}+\frac{1}{h_{c}-2 r} \geq \frac{3}{r}
$$
Answer of Example Problem 1: $$C = 3$$

Example Problem 2: Let $a, b, c$ be positive real numbers such that $a^2 + b^2 + c^2 = 3abc$. Find the largest constant $C$ such that the following inequality holds for all $a, b, c$ satisfying the given constraint:
$$
\frac{a}{b^2 c^2} + \frac{b}{c^2 a^2} + \frac{c}{a^2 b^2} \geq \frac{C}{a+b+c}
$$
Solution of Example Problem 2: The given inequality is equivalent to
$$
\left(a^{3}+b^{3}+c^{3}\right)(a+b+c) \geq 9 a^{2} b^{2} c^{2}
$$

Applying the Cauchy-Schwarz inequality we have
$$
\left(a^{3}+b^{3}+c^{3}\right)(a+b+c) \geq\left(a^{2}+b^{2}+c^{2}\right)^{2}
$$

Since $a^{2}+b^{2}+c^{2}=3 a b c$ we obtain
$$
\left(a^{3}+b^{3}+c^{3}\right)(a+b+c) \geq\left(a^{2}+b^{2}+c^{2}\right)^{2}=(3 a b c)^{2}=9 a^{2} b^{2} c^{2}
$$

Equality holds if and only if $a=b=c=1$.
Answer of Example Problem 2: $$C = 9$$

Example Problem 3: Let $a, b, c$ be positive real numbers such that $a b c = 1$. Find the largest constant $C$ such that the following inequality holds for all $a, b, c$ satisfying the given constraint:
$$
\frac{b+c}{\sqrt{a}}+\frac{c+a}{\sqrt{b}}+\frac{a+b}{\sqrt{c}} \geq \sqrt{a}+\sqrt{b}+\sqrt{c}+C
$$
Solution of Example Problem 3: [Solution 1]
From the AM-GM Inequality, we have

$$
\begin{aligned}
& \frac{b+c}{\sqrt{a}}+\frac{c+a}{\sqrt{b}}+\frac{a+b}{\sqrt{c}} \geq 2\left(\sqrt{\frac{b c}{a}}+\sqrt{\frac{c a}{b}}+\sqrt{\frac{a b}{c}}\right)= \\
& =\left(\sqrt{\frac{b c}{a}}+\sqrt{\frac{c a}{b}}\right)+\left(\sqrt{\frac{c a}{b}}+\sqrt{\frac{a b}{c}}\right)+\left(\sqrt{\frac{a b}{c}}+\sqrt{\frac{b c}{a}}\right) \geq \\
& \geq 2(\sqrt{a}+\sqrt{b}+\sqrt{c}) \geq \sqrt{a}+\sqrt{b}+\sqrt{c}+3 \sqrt[6]{a b c}=\sqrt{a}+\sqrt{b}+\sqrt{c}+3 .
\end{aligned}
$$
Answer of Example Problem 3: $$C = 3$$


Problem: Let $a$ and $b$ be non-negative real numbers such that $a \geq b$. Determine the largest constant $C$ such that the following inequality holds for all $a \geq b \geq 0$:
$$
a + \frac{1}{b(a-b)} \geq C.
$$

Solution:

## Response

To solve the problem, we start with the inequality we need to analyze:

\[
a + \frac{1}{b(a-b)} \geq C
\]

for non-negative real numbers \(a\) and \(b\) such that \(a \geq b \geq 0\).

### Step 1: Analyze the expression

We can rewrite the inequality as:

\[
\frac{1}{b(a-b)} \geq C - a
\]

This implies that we need to ensure that \(b(a-b)\) is positive (i.e., \(b > 0\) and \(a > b\)) to avoid division by zero or negative values.

### Step 2: Consider the limit as \(b\) approaches 0

As \(b\) approaches 0, the term \(b(a-b)\) approaches 0, which means \(\frac{1}{b(a-b)}\) approaches infinity. Therefore, the left-hand side of the inequality can become arbitrarily large, suggesting that \(C\) can be any finite value.

### Step 3: Consider the case when \(b\) is small but positive

Let’s analyze the case when \(b\) is a small positive number. We can set \(b = \epsilon\) where \(\epsilon\) is a small positive number. Then we have:

\[
a + \frac{1}{\epsilon(a - \epsilon)} \geq C
\]

As \(b\) approaches 0, we can see that \(a\) must be greater than \(\epsilon\) for the term \(a - b\) to remain positive. 

### Step 4: Set \(a = b\)

To find a lower bound for \(C\), we can set \(a = b\). In this case, the expression becomes:

\[
b + \frac{1}{b(b-b)} = b + \text{undefined}
\]

This case is not valid since it leads to division by zero. Thus, we need to consider \(a > b\).

### Step 5: Set \(a = b + k\) for some \(k > 0\)

Let’s set \(a = b + k\) where \(k\) is a small positive number. Then we have:

\[
(b + k) + \frac{1}{b(k)} \geq C
\]

This simplifies to:

\[
b + k + \frac{1}{bk} \geq C
\]

### Step 6: Minimize the left-hand side

To find the minimum value of the left-hand side, we can analyze the function:

\[
f(b) = b + k + \frac{1}{bk}
\]

Taking the derivative with respect to \(b\) and setting it to zero gives us:

\[
1 - \frac{1}{b^2 k} = 0 \implies b^2 = \frac{1}{k} \implies b = \frac{1}{\sqrt{k}}
\]

Substituting \(b = \frac{1}{\sqrt{k}}\) back into the function gives:

\[
f\left(\frac{1}{\sqrt{k}}\right) = \frac{1}{\sqrt{k}} + k + \frac{\sqrt{k}}{1} = \frac{1}{\sqrt{k}} + k + \sqrt{k}
\]

### Step 7: Analyze the limit as \(k\) approaches 0

As \(k\) approaches 0, the term \(k\) becomes negligible, and we can analyze the behavior of \(\frac{1}{\sqrt{k}} + \sqrt{k}\). The term \(\frac{1}{\sqrt{k}}\) dominates, leading to:

\[
\lim_{k \to 0} f\left(\frac{1}{\sqrt{k}}\right) \to \infty
\]

### Conclusion

Since we can make the left-hand side of the inequality arbitrarily large by choosing \(b\) small enough, we conclude that the largest constant \(C\) that satisfies the inequality for all \(a \geq b \geq 0\) is:

\[
C = 0
\]

Thus, the final answer is:

The answer is \(C=0\).