## Problem

Let $a, b, c$ be positive real numbers such that $abc = 1$. Find the largest constant $C$ such that the following inequality holds for all $a, b, c$:
$$
\frac{1}{a^5(b+2c)^2} + \frac{1}{b^5(c+2a)^2} + \frac{1}{c^5(a+2b)^2} \geq C.
$$

## Query

Task description: Please solve the problem with clear, rigorous, and logically sound steps. At the end of your response, state your answer in exactly this format: 'The answer is $C=X$', where X is your calculated numerical bound value. Example: 'The answer is $C=1$'.

Here are some example problems and solutions that are related to the problem you are solving:

Example Problem 1: Let $a, b, c$ be the side lengths, $h_{a}, h_{b}, h_{c}$ be the altitudes, respectively, and $r$ be the inradius of a triangle. Find the largest constant $C$ such that the following inequality holds for all triangles:
$$
\frac{1}{h_{a}-2 r}+\frac{1}{h_{b}-2 r}+\frac{1}{h_{c}-2 r} \geq C \cdot r
$$
Solution of Example Problem 1: By $\frac{1}{h_{a}}+\frac{1}{h_{b}}+\frac{1}{h_{c}}=\frac{1}{r}$ we obtain
$$
\frac{h_{a}-2 r}{h_{a}}+\frac{h_{b}-2 r}{h_{b}}+\frac{h_{c}-2 r}{h_{c}}=1
$$

Applying $A M \geq H M$ we get
$$
\left(\frac{h_{a}-2 r}{h_{a}}+\frac{h_{b}-2 r}{h_{b}}+\frac{h_{c}-2 r}{h_{c}}\right)\left(\frac{h_{a}}{h_{a}-2 r}+\frac{h_{b}}{h_{b}-2 r}+\frac{h_{c}}{h_{c}-2 r}\right) \geq 9
$$
i.e.
$$
\frac{h_{a}}{h_{a}-2 r}+\frac{h_{b}}{h_{b}-2 r}+\frac{h_{c}}{h_{c}-2 r} \geq 9
$$

Therefore
$$
\begin{aligned}
& \frac{2 r}{h_{a}-2 r}+\frac{2 r}{h_{b}-2 r}+\frac{2 r}{h_{c}-2 r} \\
& \quad=\frac{h_{a}-\left(h_{a}-2 r\right)}{h_{a}-2 r}+\frac{h_{b}-\left(h_{b}-2 r\right)}{h_{b}-2 r}+\frac{h_{c}-\left(h_{c}-2 r\right)}{h_{c}-2 r} \\
& \quad=\frac{h_{a}}{h_{a}-2 r}+\frac{h_{b}}{h_{b}-2 r}+\frac{h_{c}}{h_{c}-2 r}-3 \geq 9-3=6
\end{aligned}
$$
i.e.
$$
\frac{1}{h_{a}-2 r}+\frac{1}{h_{b}-2 r}+\frac{1}{h_{c}-2 r} \geq \frac{3}{r}
$$
Answer of Example Problem 1: $$C = 3$$

Example Problem 2: Let $a, b, c$ be positive real numbers such that $a^2 + b^2 + c^2 = 3abc$. Find the largest constant $C$ such that the following inequality holds for all $a, b, c$ satisfying the given constraint:
$$
\frac{a}{b^2 c^2} + \frac{b}{c^2 a^2} + \frac{c}{a^2 b^2} \geq \frac{C}{a+b+c}
$$
Solution of Example Problem 2: The given inequality is equivalent to
$$
\left(a^{3}+b^{3}+c^{3}\right)(a+b+c) \geq 9 a^{2} b^{2} c^{2}
$$

Applying the Cauchy-Schwarz inequality we have
$$
\left(a^{3}+b^{3}+c^{3}\right)(a+b+c) \geq\left(a^{2}+b^{2}+c^{2}\right)^{2}
$$

Since $a^{2}+b^{2}+c^{2}=3 a b c$ we obtain
$$
\left(a^{3}+b^{3}+c^{3}\right)(a+b+c) \geq\left(a^{2}+b^{2}+c^{2}\right)^{2}=(3 a b c)^{2}=9 a^{2} b^{2} c^{2}
$$

Equality holds if and only if $a=b=c=1$.
Answer of Example Problem 2: $$C = 9$$

Example Problem 3: Let $a, b, c$ be positive real numbers such that $a b c = 1$. Find the largest constant $C$ such that the following inequality holds for all $a, b, c$ satisfying the given constraint:
$$
\frac{b+c}{\sqrt{a}}+\frac{c+a}{\sqrt{b}}+\frac{a+b}{\sqrt{c}} \geq \sqrt{a}+\sqrt{b}+\sqrt{c}+C
$$
Solution of Example Problem 3: [Solution 1]
From the AM-GM Inequality, we have

$$
\begin{aligned}
& \frac{b+c}{\sqrt{a}}+\frac{c+a}{\sqrt{b}}+\frac{a+b}{\sqrt{c}} \geq 2\left(\sqrt{\frac{b c}{a}}+\sqrt{\frac{c a}{b}}+\sqrt{\frac{a b}{c}}\right)= \\
& =\left(\sqrt{\frac{b c}{a}}+\sqrt{\frac{c a}{b}}\right)+\left(\sqrt{\frac{c a}{b}}+\sqrt{\frac{a b}{c}}\right)+\left(\sqrt{\frac{a b}{c}}+\sqrt{\frac{b c}{a}}\right) \geq \\
& \geq 2(\sqrt{a}+\sqrt{b}+\sqrt{c}) \geq \sqrt{a}+\sqrt{b}+\sqrt{c}+3 \sqrt[6]{a b c}=\sqrt{a}+\sqrt{b}+\sqrt{c}+3 .
\end{aligned}
$$
Answer of Example Problem 3: $$C = 3$$


Problem: Let $a, b, c$ be positive real numbers such that $abc = 1$. Find the largest constant $C$ such that the following inequality holds for all $a, b, c$:
$$
\frac{1}{a^5(b+2c)^2} + \frac{1}{b^5(c+2a)^2} + \frac{1}{c^5(a+2b)^2} \geq C.
$$

Solution:

## Response

To solve the problem, we need to analyze the given inequality:

\[
\frac{1}{a^5(b+2c)^2} + \frac{1}{b^5(c+2a)^2} + \frac{1}{c^5(a+2b)^2} \geq C
\]

for positive real numbers \(a, b, c\) such that \(abc = 1\).

### Step 1: Apply the AM-GM Inequality

We can use the AM-GM inequality to estimate the terms in the denominators. For any positive \(x\) and \(y\):

\[
x + y \geq 2\sqrt{xy}
\]

Applying this to \(b + 2c\):

\[
b + 2c \geq 3\sqrt[3]{b \cdot c^2}
\]

Since \(abc = 1\), we have \(c = \frac{1}{ab}\). Thus:

\[
b + 2c = b + 2\frac{1}{ab} = b + \frac{2}{ab}
\]

### Step 2: Substitute and Simplify

Now, we can express \(b + 2c\) in terms of \(a\) and \(b\):

\[
b + 2c = b + \frac{2}{ab} \geq 3\sqrt[3]{b \cdot \left(\frac{1}{ab}\right)^2} = 3\sqrt[3]{\frac{b}{a^2}}
\]

Thus, we can write:

\[
(b + 2c)^2 \geq 9\left(\frac{b}{a^2}\right)^{\frac{2}{3}} = 9\frac{b^{\frac{2}{3}}}{a^{\frac{4}{3}}}
\]

### Step 3: Substitute Back into the Original Inequality

Now substituting this back into our inequality:

\[
\frac{1}{a^5(b+2c)^2} \geq \frac{1}{a^5 \cdot 9\frac{b^{\frac{2}{3}}}{a^{\frac{4}{3}}}} = \frac{a^{\frac{4}{3}}}{9a^5b^{\frac{2}{3}}} = \frac{1}{9} \cdot \frac{1}{a^{\frac{11}{3}}b^{\frac{2}{3}}}
\]

### Step 4: Summing the Terms

We can apply the same reasoning to the other two terms:

\[
\frac{1}{b^5(c+2a)^2} \geq \frac{1}{9} \cdot \frac{1}{b^{\frac{11}{3}}c^{\frac{2}{3}}}
\]
\[
\frac{1}{c^5(a+2b)^2} \geq \frac{1}{9} \cdot \frac{1}{c^{\frac{11}{3}}a^{\frac{2}{3}}}
\]

Thus, we have:

\[
\frac{1}{a^5(b+2c)^2} + \frac{1}{b^5(c+2a)^2} + \frac{1}{c^5(a+2b)^2} \geq \frac{1}{9} \left( \frac{1}{a^{\frac{11}{3}}b^{\frac{2}{3}}} + \frac{1}{b^{\frac{11}{3}}c^{\frac{2}{3}}} + \frac{1}{c^{\frac{11}{3}}a^{\frac{2}{3}}} \right)
\]

### Step 5: Use the AM-GM Inequality Again

Now we can apply AM-GM again to the sum:

\[
\frac{1}{a^{\frac{11}{3}}b^{\frac{2}{3}}} + \frac{1}{b^{\frac{11}{3}}c^{\frac{2}{3}}} + \frac{1}{c^{\frac{11}{3}}a^{\frac{2}{3}}} \geq 3 \sqrt[3]{\frac{1}{(abc)^{\frac{11}{3}}(abc)^{\frac{2}{3}}}} = 3 \sqrt[3]{\frac{1}{1^{\frac{11}{3} + \frac{2}{3}}}} = 3
\]

### Step 6: Final Calculation

Thus, we have:

\[
\frac{1}{a^5(b+2c)^2} + \frac{1}{b^5(c+2a)^2} + \frac{1}{c^5(a+2b)^2} \geq \frac{1}{9} \cdot 3 = \frac{1}{3}
\]

This implies that the largest constant \(C\) such that the inequality holds for all positive \(a, b, c\) with \(abc = 1\) is:

\[
C = \frac{1}{3}
\]

Thus, the final answer is:

The answer is \(C=\frac{1}{3}\).