## Problem

Let $0 \leq x \leq 1$ and $n \in \mathbb{N}$. Find the smallest constant $C$ such that the following inequality holds for all $x$ and $n$:
$$
\left(1-x+\frac{x^2}{2}\right)^n-(1-x)^n \leq Cx.
$$

## Query

Task description: Please solve the problem with clear, rigorous, and logically sound steps. At the end of your response, state your answer in exactly this format: 'The answer is $C=X$', where X is your calculated numerical bound value. Example: 'The answer is $C=1$'.

Here are some example problems and solutions that are related to the problem you are solving:

Example Problem 1: Let $a, b, c$ be the side lengths, $h_{a}, h_{b}, h_{c}$ be the altitudes, respectively, and $r$ be the inradius of a triangle. Find the largest constant $C$ such that the following inequality holds for all triangles:
$$
\frac{1}{h_{a}-2 r}+\frac{1}{h_{b}-2 r}+\frac{1}{h_{c}-2 r} \geq C \cdot r
$$
Solution of Example Problem 1: By $\frac{1}{h_{a}}+\frac{1}{h_{b}}+\frac{1}{h_{c}}=\frac{1}{r}$ we obtain
$$
\frac{h_{a}-2 r}{h_{a}}+\frac{h_{b}-2 r}{h_{b}}+\frac{h_{c}-2 r}{h_{c}}=1
$$

Applying $A M \geq H M$ we get
$$
\left(\frac{h_{a}-2 r}{h_{a}}+\frac{h_{b}-2 r}{h_{b}}+\frac{h_{c}-2 r}{h_{c}}\right)\left(\frac{h_{a}}{h_{a}-2 r}+\frac{h_{b}}{h_{b}-2 r}+\frac{h_{c}}{h_{c}-2 r}\right) \geq 9
$$
i.e.
$$
\frac{h_{a}}{h_{a}-2 r}+\frac{h_{b}}{h_{b}-2 r}+\frac{h_{c}}{h_{c}-2 r} \geq 9
$$

Therefore
$$
\begin{aligned}
& \frac{2 r}{h_{a}-2 r}+\frac{2 r}{h_{b}-2 r}+\frac{2 r}{h_{c}-2 r} \\
& \quad=\frac{h_{a}-\left(h_{a}-2 r\right)}{h_{a}-2 r}+\frac{h_{b}-\left(h_{b}-2 r\right)}{h_{b}-2 r}+\frac{h_{c}-\left(h_{c}-2 r\right)}{h_{c}-2 r} \\
& \quad=\frac{h_{a}}{h_{a}-2 r}+\frac{h_{b}}{h_{b}-2 r}+\frac{h_{c}}{h_{c}-2 r}-3 \geq 9-3=6
\end{aligned}
$$
i.e.
$$
\frac{1}{h_{a}-2 r}+\frac{1}{h_{b}-2 r}+\frac{1}{h_{c}-2 r} \geq \frac{3}{r}
$$
Answer of Example Problem 1: $$C = 3$$

Example Problem 2: Let $a, b, c$ be positive real numbers such that $a^2 + b^2 + c^2 = 3abc$. Find the largest constant $C$ such that the following inequality holds for all $a, b, c$ satisfying the given constraint:
$$
\frac{a}{b^2 c^2} + \frac{b}{c^2 a^2} + \frac{c}{a^2 b^2} \geq \frac{C}{a+b+c}
$$
Solution of Example Problem 2: The given inequality is equivalent to
$$
\left(a^{3}+b^{3}+c^{3}\right)(a+b+c) \geq 9 a^{2} b^{2} c^{2}
$$

Applying the Cauchy-Schwarz inequality we have
$$
\left(a^{3}+b^{3}+c^{3}\right)(a+b+c) \geq\left(a^{2}+b^{2}+c^{2}\right)^{2}
$$

Since $a^{2}+b^{2}+c^{2}=3 a b c$ we obtain
$$
\left(a^{3}+b^{3}+c^{3}\right)(a+b+c) \geq\left(a^{2}+b^{2}+c^{2}\right)^{2}=(3 a b c)^{2}=9 a^{2} b^{2} c^{2}
$$

Equality holds if and only if $a=b=c=1$.
Answer of Example Problem 2: $$C = 9$$

Example Problem 3: Let $a, b, c$ be positive real numbers such that $a b c = 1$. Find the largest constant $C$ such that the following inequality holds for all $a, b, c$ satisfying the given constraint:
$$
\frac{b+c}{\sqrt{a}}+\frac{c+a}{\sqrt{b}}+\frac{a+b}{\sqrt{c}} \geq \sqrt{a}+\sqrt{b}+\sqrt{c}+C
$$
Solution of Example Problem 3: [Solution 1]
From the AM-GM Inequality, we have

$$
\begin{aligned}
& \frac{b+c}{\sqrt{a}}+\frac{c+a}{\sqrt{b}}+\frac{a+b}{\sqrt{c}} \geq 2\left(\sqrt{\frac{b c}{a}}+\sqrt{\frac{c a}{b}}+\sqrt{\frac{a b}{c}}\right)= \\
& =\left(\sqrt{\frac{b c}{a}}+\sqrt{\frac{c a}{b}}\right)+\left(\sqrt{\frac{c a}{b}}+\sqrt{\frac{a b}{c}}\right)+\left(\sqrt{\frac{a b}{c}}+\sqrt{\frac{b c}{a}}\right) \geq \\
& \geq 2(\sqrt{a}+\sqrt{b}+\sqrt{c}) \geq \sqrt{a}+\sqrt{b}+\sqrt{c}+3 \sqrt[6]{a b c}=\sqrt{a}+\sqrt{b}+\sqrt{c}+3 .
\end{aligned}
$$
Answer of Example Problem 3: $$C = 3$$


Problem: Let $0 \leq x \leq 1$ and $n \in \mathbb{N}$. Find the smallest constant $C$ such that the following inequality holds for all $x$ and $n$:
$$
\left(1-x+\frac{x^2}{2}\right)^n-(1-x)^n \leq Cx.
$$

Solution:

## Response

To solve the problem, we start with the inequality we need to analyze:

\[
\left(1-x+\frac{x^2}{2}\right)^n - (1-x)^n \leq Cx
\]

for \(0 \leq x \leq 1\) and \(n \in \mathbb{N}\).

### Step 1: Expand the left-hand side using the Binomial Theorem

We can expand both terms using the Binomial Theorem. The expansion of \((1-x)^n\) is:

\[
(1-x)^n = \sum_{k=0}^{n} \binom{n}{k} (-x)^k = 1 - nx + \frac{n(n-1)}{2}x^2 - \cdots
\]

Now, we expand \(\left(1-x+\frac{x^2}{2}\right)^n\):

\[
\left(1-x+\frac{x^2}{2}\right)^n = \sum_{k=0}^{n} \binom{n}{k} \left(-x+\frac{x^2}{2}\right)^k
\]

Using the binomial expansion for \((-x + \frac{x^2}{2})^k\):

\[
(-x + \frac{x^2}{2})^k = \sum_{j=0}^{k} \binom{k}{j} (-x)^{k-j} \left(\frac{x^2}{2}\right)^j = \sum_{j=0}^{k} \binom{k}{j} (-1)^{k-j} \frac{x^{k+j}}{2^j}
\]

### Step 2: Compare the two expansions

We need to find the difference:

\[
\left(1-x+\frac{x^2}{2}\right)^n - (1-x)^n
\]

This difference will be dominated by the first few terms in the expansion. 

### Step 3: Analyze the leading term

For small \(x\), we can approximate:

\[
1 - nx + \frac{n(n-1)}{2}x^2 - \cdots
\]

and 

\[
\left(1 - x + \frac{x^2}{2}\right)^n \approx 1 - nx + \frac{n(n-1)}{2}x^2 + \text{higher order terms}
\]

The leading term in the expansion of \(\left(1-x+\frac{x^2}{2}\right)^n\) will be:

\[
1 - nx + \frac{n(n-1)}{2}x^2 + O(x^3)
\]

### Step 4: Calculate the difference

The difference becomes:

\[
\left(1 - nx + \frac{n(n-1)}{2}x^2 + O(x^3)\right) - \left(1 - nx + \frac{n(n-1)}{2}x^2\right) = O(x^3)
\]

### Step 5: Establish the inequality

Thus, we have:

\[
O(x^3) \leq Cx
\]

Dividing both sides by \(x\) (valid since \(x > 0\)) gives:

\[
O(x^2) \leq C
\]

### Step 6: Determine the smallest constant \(C\)

As \(x\) approaches \(0\), \(O(x^2)\) approaches \(0\). Therefore, for the inequality to hold for all \(x\) in the interval \([0, 1]\), we can conclude that the smallest constant \(C\) that satisfies this inequality is:

\[
C = 0
\]

### Conclusion

Thus, the smallest constant \(C\) such that the inequality holds for all \(x\) and \(n\) is:

The answer is \(C=0\).