## Problem

Let $a_1, a_2, \ldots, a_n$ be non-negative real numbers such that $\prod a_1 = \lambda^n$. Determine the minimal constant $C$ such that the following inequality holds for all $a_1, a_2, \ldots, a_n$:

$$
\prod_{c y c}\left(a_1^2-a_1+1\right) \geq \sqrt{\left(\frac{1+\lambda^4}{C}\right)^n}.
$$

## Query

Task description: Please solve the problem with clear, rigorous, and logically sound steps. At the end of your response, state your answer in exactly this format: 'The answer is $C=X$', where X is your calculated numerical bound value. Example: 'The answer is $C=1$'.

Here are some example problems and solutions that are related to the problem you are solving:

Example Problem 1: Let $a, b, c$ be the side lengths, $h_{a}, h_{b}, h_{c}$ be the altitudes, respectively, and $r$ be the inradius of a triangle. Find the largest constant $C$ such that the following inequality holds for all triangles:
$$
\frac{1}{h_{a}-2 r}+\frac{1}{h_{b}-2 r}+\frac{1}{h_{c}-2 r} \geq C \cdot r
$$
Solution of Example Problem 1: By $\frac{1}{h_{a}}+\frac{1}{h_{b}}+\frac{1}{h_{c}}=\frac{1}{r}$ we obtain
$$
\frac{h_{a}-2 r}{h_{a}}+\frac{h_{b}-2 r}{h_{b}}+\frac{h_{c}-2 r}{h_{c}}=1
$$

Applying $A M \geq H M$ we get
$$
\left(\frac{h_{a}-2 r}{h_{a}}+\frac{h_{b}-2 r}{h_{b}}+\frac{h_{c}-2 r}{h_{c}}\right)\left(\frac{h_{a}}{h_{a}-2 r}+\frac{h_{b}}{h_{b}-2 r}+\frac{h_{c}}{h_{c}-2 r}\right) \geq 9
$$
i.e.
$$
\frac{h_{a}}{h_{a}-2 r}+\frac{h_{b}}{h_{b}-2 r}+\frac{h_{c}}{h_{c}-2 r} \geq 9
$$

Therefore
$$
\begin{aligned}
& \frac{2 r}{h_{a}-2 r}+\frac{2 r}{h_{b}-2 r}+\frac{2 r}{h_{c}-2 r} \\
& \quad=\frac{h_{a}-\left(h_{a}-2 r\right)}{h_{a}-2 r}+\frac{h_{b}-\left(h_{b}-2 r\right)}{h_{b}-2 r}+\frac{h_{c}-\left(h_{c}-2 r\right)}{h_{c}-2 r} \\
& \quad=\frac{h_{a}}{h_{a}-2 r}+\frac{h_{b}}{h_{b}-2 r}+\frac{h_{c}}{h_{c}-2 r}-3 \geq 9-3=6
\end{aligned}
$$
i.e.
$$
\frac{1}{h_{a}-2 r}+\frac{1}{h_{b}-2 r}+\frac{1}{h_{c}-2 r} \geq \frac{3}{r}
$$
Answer of Example Problem 1: $$C = 3$$

Example Problem 2: Let $a, b, c$ be positive real numbers such that $a^2 + b^2 + c^2 = 3abc$. Find the largest constant $C$ such that the following inequality holds for all $a, b, c$ satisfying the given constraint:
$$
\frac{a}{b^2 c^2} + \frac{b}{c^2 a^2} + \frac{c}{a^2 b^2} \geq \frac{C}{a+b+c}
$$
Solution of Example Problem 2: The given inequality is equivalent to
$$
\left(a^{3}+b^{3}+c^{3}\right)(a+b+c) \geq 9 a^{2} b^{2} c^{2}
$$

Applying the Cauchy-Schwarz inequality we have
$$
\left(a^{3}+b^{3}+c^{3}\right)(a+b+c) \geq\left(a^{2}+b^{2}+c^{2}\right)^{2}
$$

Since $a^{2}+b^{2}+c^{2}=3 a b c$ we obtain
$$
\left(a^{3}+b^{3}+c^{3}\right)(a+b+c) \geq\left(a^{2}+b^{2}+c^{2}\right)^{2}=(3 a b c)^{2}=9 a^{2} b^{2} c^{2}
$$

Equality holds if and only if $a=b=c=1$.
Answer of Example Problem 2: $$C = 9$$

Example Problem 3: Let $a, b, c$ be positive real numbers such that $a b c = 1$. Find the largest constant $C$ such that the following inequality holds for all $a, b, c$ satisfying the given constraint:
$$
\frac{b+c}{\sqrt{a}}+\frac{c+a}{\sqrt{b}}+\frac{a+b}{\sqrt{c}} \geq \sqrt{a}+\sqrt{b}+\sqrt{c}+C
$$
Solution of Example Problem 3: [Solution 1]
From the AM-GM Inequality, we have

$$
\begin{aligned}
& \frac{b+c}{\sqrt{a}}+\frac{c+a}{\sqrt{b}}+\frac{a+b}{\sqrt{c}} \geq 2\left(\sqrt{\frac{b c}{a}}+\sqrt{\frac{c a}{b}}+\sqrt{\frac{a b}{c}}\right)= \\
& =\left(\sqrt{\frac{b c}{a}}+\sqrt{\frac{c a}{b}}\right)+\left(\sqrt{\frac{c a}{b}}+\sqrt{\frac{a b}{c}}\right)+\left(\sqrt{\frac{a b}{c}}+\sqrt{\frac{b c}{a}}\right) \geq \\
& \geq 2(\sqrt{a}+\sqrt{b}+\sqrt{c}) \geq \sqrt{a}+\sqrt{b}+\sqrt{c}+3 \sqrt[6]{a b c}=\sqrt{a}+\sqrt{b}+\sqrt{c}+3 .
\end{aligned}
$$
Answer of Example Problem 3: $$C = 3$$


Problem: Let $a_1, a_2, \ldots, a_n$ be non-negative real numbers such that $\prod a_1 = \lambda^n$. Determine the minimal constant $C$ such that the following inequality holds for all $a_1, a_2, \ldots, a_n$:

$$
\prod_{c y c}\left(a_1^2-a_1+1\right) \geq \sqrt{\left(\frac{1+\lambda^4}{C}\right)^n}.
$$

Solution:

## Response

To solve the problem, we need to analyze the given inequality:

\[
\prod_{i=1}^n (a_i^2 - a_i + 1) \geq \sqrt{\left(\frac{1+\lambda^4}{C}\right)^n}.
\]

First, we will simplify the left-hand side. The expression \(a_i^2 - a_i + 1\) can be rewritten as:

\[
a_i^2 - a_i + 1 = \left(a_i - \frac{1}{2}\right)^2 + \frac{3}{4}.
\]

This shows that \(a_i^2 - a_i + 1\) is always positive for all real \(a_i\) and achieves its minimum value of \(\frac{3}{4}\) when \(a_i = \frac{1}{2}\).

Next, we will apply the AM-GM inequality to the terms \(a_i^2 - a_i + 1\):

\[
\prod_{i=1}^n (a_i^2 - a_i + 1) \geq \left(\frac{(a_1^2 - a_1 + 1) + (a_2^2 - a_2 + 1) + \ldots + (a_n^2 - a_n + 1)}{n}\right)^n.
\]

Now, we need to find a suitable expression for the average of \(a_i^2 - a_i + 1\). We can express this average as:

\[
\frac{1}{n} \sum_{i=1}^n (a_i^2 - a_i + 1) = \frac{1}{n} \left(\sum_{i=1}^n a_i^2 - \sum_{i=1}^n a_i + n\right).
\]

Using the Cauchy-Schwarz inequality, we have:

\[
\left(\sum_{i=1}^n a_i\right)^2 \leq n \sum_{i=1}^n a_i^2.
\]

Let \(S = \sum_{i=1}^n a_i\) and \(Q = \sum_{i=1}^n a_i^2\). Then, we can express \(Q\) in terms of \(S\):

\[
Q \geq \frac{S^2}{n}.
\]

Now, substituting this back into our average, we get:

\[
\frac{1}{n} \left(Q - S + n\right) \geq \frac{1}{n} \left(\frac{S^2}{n} - S + n\right).
\]

To find the minimum value of the product, we need to analyze the case when all \(a_i\) are equal, say \(a_i = \lambda\). In this case, we have:

\[
\prod_{i=1}^n (a_i^2 - a_i + 1) = (n(\lambda^2 - \lambda + 1))^n.
\]

Now, we need to find \(C\) such that:

\[
(n(\lambda^2 - \lambda + 1))^n \geq \sqrt{\left(\frac{1+\lambda^4}{C}\right)^n}.
\]

Taking the \(n\)-th root on both sides gives:

\[
n(\lambda^2 - \lambda + 1) \geq \sqrt{\frac{1+\lambda^4}{C}}.
\]

Squaring both sides results in:

\[
n^2(\lambda^2 - \lambda + 1)^2 \geq \frac{1+\lambda^4}{C}.
\]

Rearranging gives:

\[
C \geq \frac{1+\lambda^4}{n^2(\lambda^2 - \lambda + 1)^2}.
\]

To find the minimal constant \(C\), we need to minimize the right-hand side. The expression \(n^2(\lambda^2 - \lambda + 1)^2\) achieves its minimum when \(\lambda = 1\), yielding:

\[
C \geq \frac{1 + 1^4}{n^2(1^2 - 1 + 1)^2} = \frac{2}{n^2}.
\]

Thus, the minimal constant \(C\) that satisfies the inequality for all non-negative \(a_1, a_2, \ldots, a_n\) such that \(\prod a_i = \lambda^n\) is:

\[
C = 2.
\]

Therefore, the final answer is:

The answer is \(C=2\).