## Problem

Let $x$ and $y$ be two positive real numbers such that $x + y = 1$. Determine the largest constant $C$ such that the following inequality holds for all $x, y$:

$$
\left(1+\frac{1}{x}\right)\left(1+\frac{1}{y}\right) \geq C.
$$

## Query

Task description: Please solve the problem with clear, rigorous, and logically sound steps. At the end of your response, state your answer in exactly this format: 'The answer is $C=X$', where X is your calculated numerical bound value. Example: 'The answer is $C=1$'.

Here are some example problems and solutions that are related to the problem you are solving:

Example Problem 1: Let $a, b, c$ be the side lengths, $h_{a}, h_{b}, h_{c}$ be the altitudes, respectively, and $r$ be the inradius of a triangle. Find the largest constant $C$ such that the following inequality holds for all triangles:
$$
\frac{1}{h_{a}-2 r}+\frac{1}{h_{b}-2 r}+\frac{1}{h_{c}-2 r} \geq C \cdot r
$$
Solution of Example Problem 1: By $\frac{1}{h_{a}}+\frac{1}{h_{b}}+\frac{1}{h_{c}}=\frac{1}{r}$ we obtain
$$
\frac{h_{a}-2 r}{h_{a}}+\frac{h_{b}-2 r}{h_{b}}+\frac{h_{c}-2 r}{h_{c}}=1
$$

Applying $A M \geq H M$ we get
$$
\left(\frac{h_{a}-2 r}{h_{a}}+\frac{h_{b}-2 r}{h_{b}}+\frac{h_{c}-2 r}{h_{c}}\right)\left(\frac{h_{a}}{h_{a}-2 r}+\frac{h_{b}}{h_{b}-2 r}+\frac{h_{c}}{h_{c}-2 r}\right) \geq 9
$$
i.e.
$$
\frac{h_{a}}{h_{a}-2 r}+\frac{h_{b}}{h_{b}-2 r}+\frac{h_{c}}{h_{c}-2 r} \geq 9
$$

Therefore
$$
\begin{aligned}
& \frac{2 r}{h_{a}-2 r}+\frac{2 r}{h_{b}-2 r}+\frac{2 r}{h_{c}-2 r} \\
& \quad=\frac{h_{a}-\left(h_{a}-2 r\right)}{h_{a}-2 r}+\frac{h_{b}-\left(h_{b}-2 r\right)}{h_{b}-2 r}+\frac{h_{c}-\left(h_{c}-2 r\right)}{h_{c}-2 r} \\
& \quad=\frac{h_{a}}{h_{a}-2 r}+\frac{h_{b}}{h_{b}-2 r}+\frac{h_{c}}{h_{c}-2 r}-3 \geq 9-3=6
\end{aligned}
$$
i.e.
$$
\frac{1}{h_{a}-2 r}+\frac{1}{h_{b}-2 r}+\frac{1}{h_{c}-2 r} \geq \frac{3}{r}
$$
Answer of Example Problem 1: $$C = 3$$

Example Problem 2: Let $a, b, c$ be positive real numbers such that $a^2 + b^2 + c^2 = 3abc$. Find the largest constant $C$ such that the following inequality holds for all $a, b, c$ satisfying the given constraint:
$$
\frac{a}{b^2 c^2} + \frac{b}{c^2 a^2} + \frac{c}{a^2 b^2} \geq \frac{C}{a+b+c}
$$
Solution of Example Problem 2: The given inequality is equivalent to
$$
\left(a^{3}+b^{3}+c^{3}\right)(a+b+c) \geq 9 a^{2} b^{2} c^{2}
$$

Applying the Cauchy-Schwarz inequality we have
$$
\left(a^{3}+b^{3}+c^{3}\right)(a+b+c) \geq\left(a^{2}+b^{2}+c^{2}\right)^{2}
$$

Since $a^{2}+b^{2}+c^{2}=3 a b c$ we obtain
$$
\left(a^{3}+b^{3}+c^{3}\right)(a+b+c) \geq\left(a^{2}+b^{2}+c^{2}\right)^{2}=(3 a b c)^{2}=9 a^{2} b^{2} c^{2}
$$

Equality holds if and only if $a=b=c=1$.
Answer of Example Problem 2: $$C = 9$$

Example Problem 3: Let $a, b, c$ be positive real numbers such that $a b c = 1$. Find the largest constant $C$ such that the following inequality holds for all $a, b, c$ satisfying the given constraint:
$$
\frac{b+c}{\sqrt{a}}+\frac{c+a}{\sqrt{b}}+\frac{a+b}{\sqrt{c}} \geq \sqrt{a}+\sqrt{b}+\sqrt{c}+C
$$
Solution of Example Problem 3: [Solution 1]
From the AM-GM Inequality, we have

$$
\begin{aligned}
& \frac{b+c}{\sqrt{a}}+\frac{c+a}{\sqrt{b}}+\frac{a+b}{\sqrt{c}} \geq 2\left(\sqrt{\frac{b c}{a}}+\sqrt{\frac{c a}{b}}+\sqrt{\frac{a b}{c}}\right)= \\
& =\left(\sqrt{\frac{b c}{a}}+\sqrt{\frac{c a}{b}}\right)+\left(\sqrt{\frac{c a}{b}}+\sqrt{\frac{a b}{c}}\right)+\left(\sqrt{\frac{a b}{c}}+\sqrt{\frac{b c}{a}}\right) \geq \\
& \geq 2(\sqrt{a}+\sqrt{b}+\sqrt{c}) \geq \sqrt{a}+\sqrt{b}+\sqrt{c}+3 \sqrt[6]{a b c}=\sqrt{a}+\sqrt{b}+\sqrt{c}+3 .
\end{aligned}
$$
Answer of Example Problem 3: $$C = 3$$


Problem: Let $x$ and $y$ be two positive real numbers such that $x + y = 1$. Determine the largest constant $C$ such that the following inequality holds for all $x, y$:

$$
\left(1+\frac{1}{x}\right)\left(1+\frac{1}{y}\right) \geq C.
$$

Solution:

## Response

To solve the problem, we start with the given inequality:

\[
\left(1+\frac{1}{x}\right)\left(1+\frac{1}{y}\right) \geq C
\]

where \( x + y = 1 \) and \( x, y > 0 \). We can rewrite the left-hand side:

\[
\left(1+\frac{1}{x}\right)\left(1+\frac{1}{y}\right) = \left(1 + \frac{1}{x} + \frac{1}{y} + \frac{1}{xy}\right)
\]

Substituting \( y = 1 - x \), we have:

\[
\frac{1}{y} = \frac{1}{1-x}
\]

Thus, we can express the left-hand side as:

\[
1 + \frac{1}{x} + \frac{1}{1-x} + \frac{1}{x(1-x)}
\]

Now, we simplify \( \frac{1}{x} + \frac{1}{1-x} \):

\[
\frac{1}{x} + \frac{1}{1-x} = \frac{1 - x + x}{x(1-x)} = \frac{1}{x(1-x)}
\]

So, we can rewrite the expression as:

\[
1 + \frac{1}{x(1-x)} + \frac{1}{x(1-x)} = 1 + 2\cdot\frac{1}{x(1-x)} = 1 + \frac{2}{x(1-x)}
\]

Next, we need to find the minimum value of \( \frac{2}{x(1-x)} \) for \( x \in (0, 1) \). The expression \( x(1-x) \) is a quadratic function that achieves its maximum at \( x = \frac{1}{2} \):

\[
x(1-x) = x - x^2
\]

The maximum value occurs at:

\[
x = \frac{1}{2} \implies x(1-x) = \frac{1}{2}\left(1 - \frac{1}{2}\right) = \frac{1}{4}
\]

Thus, the minimum value of \( \frac{2}{x(1-x)} \) occurs when \( x(1-x) \) is maximized:

\[
\frac{2}{x(1-x)} \text{ has a maximum value of } \frac{2}{\frac{1}{4}} = 8
\]

Therefore, the left-hand side becomes:

\[
1 + 8 = 9
\]

This means that:

\[
\left(1+\frac{1}{x}\right)\left(1+\frac{1}{y}\right) \geq 9
\]

Thus, the largest constant \( C \) such that the inequality holds for all positive \( x \) and \( y \) such that \( x + y = 1 \) is:

\[
C = 9
\]

Finally, we conclude:

The answer is \( C=9 \).