## Problem

Given positive real numbers $a, b, c$ satisfying $ab + bc + ca = 3$, find the largest constant $C$ such that the following inequality holds for all $a, b, c$:
$$
\frac{1}{\sqrt{a+b}} + \frac{1}{\sqrt{c+b}} + \frac{1}{\sqrt{a+c}} \geq \sqrt{\frac{C}{a+b+c+3}}.
$$

## Query

Task description: Please solve the problem with clear, rigorous, and logically sound steps. At the end of your response, state your answer in exactly this format: 'The answer is $C=X$', where X is your calculated numerical bound value. Example: 'The answer is $C=1$'.

Here are some example problems and solutions that are related to the problem you are solving:

Example Problem 1: Let $a, b, c$ be the side lengths, $h_{a}, h_{b}, h_{c}$ be the altitudes, respectively, and $r$ be the inradius of a triangle. Find the largest constant $C$ such that the following inequality holds for all triangles:
$$
\frac{1}{h_{a}-2 r}+\frac{1}{h_{b}-2 r}+\frac{1}{h_{c}-2 r} \geq C \cdot r
$$
Solution of Example Problem 1: By $\frac{1}{h_{a}}+\frac{1}{h_{b}}+\frac{1}{h_{c}}=\frac{1}{r}$ we obtain
$$
\frac{h_{a}-2 r}{h_{a}}+\frac{h_{b}-2 r}{h_{b}}+\frac{h_{c}-2 r}{h_{c}}=1
$$

Applying $A M \geq H M$ we get
$$
\left(\frac{h_{a}-2 r}{h_{a}}+\frac{h_{b}-2 r}{h_{b}}+\frac{h_{c}-2 r}{h_{c}}\right)\left(\frac{h_{a}}{h_{a}-2 r}+\frac{h_{b}}{h_{b}-2 r}+\frac{h_{c}}{h_{c}-2 r}\right) \geq 9
$$
i.e.
$$
\frac{h_{a}}{h_{a}-2 r}+\frac{h_{b}}{h_{b}-2 r}+\frac{h_{c}}{h_{c}-2 r} \geq 9
$$

Therefore
$$
\begin{aligned}
& \frac{2 r}{h_{a}-2 r}+\frac{2 r}{h_{b}-2 r}+\frac{2 r}{h_{c}-2 r} \\
& \quad=\frac{h_{a}-\left(h_{a}-2 r\right)}{h_{a}-2 r}+\frac{h_{b}-\left(h_{b}-2 r\right)}{h_{b}-2 r}+\frac{h_{c}-\left(h_{c}-2 r\right)}{h_{c}-2 r} \\
& \quad=\frac{h_{a}}{h_{a}-2 r}+\frac{h_{b}}{h_{b}-2 r}+\frac{h_{c}}{h_{c}-2 r}-3 \geq 9-3=6
\end{aligned}
$$
i.e.
$$
\frac{1}{h_{a}-2 r}+\frac{1}{h_{b}-2 r}+\frac{1}{h_{c}-2 r} \geq \frac{3}{r}
$$
Answer of Example Problem 1: $$C = 3$$

Example Problem 2: Let $a, b, c$ be positive real numbers such that $a^2 + b^2 + c^2 = 3abc$. Find the largest constant $C$ such that the following inequality holds for all $a, b, c$ satisfying the given constraint:
$$
\frac{a}{b^2 c^2} + \frac{b}{c^2 a^2} + \frac{c}{a^2 b^2} \geq \frac{C}{a+b+c}
$$
Solution of Example Problem 2: The given inequality is equivalent to
$$
\left(a^{3}+b^{3}+c^{3}\right)(a+b+c) \geq 9 a^{2} b^{2} c^{2}
$$

Applying the Cauchy-Schwarz inequality we have
$$
\left(a^{3}+b^{3}+c^{3}\right)(a+b+c) \geq\left(a^{2}+b^{2}+c^{2}\right)^{2}
$$

Since $a^{2}+b^{2}+c^{2}=3 a b c$ we obtain
$$
\left(a^{3}+b^{3}+c^{3}\right)(a+b+c) \geq\left(a^{2}+b^{2}+c^{2}\right)^{2}=(3 a b c)^{2}=9 a^{2} b^{2} c^{2}
$$

Equality holds if and only if $a=b=c=1$.
Answer of Example Problem 2: $$C = 9$$

Example Problem 3: Let $a, b, c$ be positive real numbers such that $a b c = 1$. Find the largest constant $C$ such that the following inequality holds for all $a, b, c$ satisfying the given constraint:
$$
\frac{b+c}{\sqrt{a}}+\frac{c+a}{\sqrt{b}}+\frac{a+b}{\sqrt{c}} \geq \sqrt{a}+\sqrt{b}+\sqrt{c}+C
$$
Solution of Example Problem 3: [Solution 1]
From the AM-GM Inequality, we have

$$
\begin{aligned}
& \frac{b+c}{\sqrt{a}}+\frac{c+a}{\sqrt{b}}+\frac{a+b}{\sqrt{c}} \geq 2\left(\sqrt{\frac{b c}{a}}+\sqrt{\frac{c a}{b}}+\sqrt{\frac{a b}{c}}\right)= \\
& =\left(\sqrt{\frac{b c}{a}}+\sqrt{\frac{c a}{b}}\right)+\left(\sqrt{\frac{c a}{b}}+\sqrt{\frac{a b}{c}}\right)+\left(\sqrt{\frac{a b}{c}}+\sqrt{\frac{b c}{a}}\right) \geq \\
& \geq 2(\sqrt{a}+\sqrt{b}+\sqrt{c}) \geq \sqrt{a}+\sqrt{b}+\sqrt{c}+3 \sqrt[6]{a b c}=\sqrt{a}+\sqrt{b}+\sqrt{c}+3 .
\end{aligned}
$$
Answer of Example Problem 3: $$C = 3$$


Problem: Given positive real numbers $a, b, c$ satisfying $ab + bc + ca = 3$, find the largest constant $C$ such that the following inequality holds for all $a, b, c$:
$$
\frac{1}{\sqrt{a+b}} + \frac{1}{\sqrt{c+b}} + \frac{1}{\sqrt{a+c}} \geq \sqrt{\frac{C}{a+b+c+3}}.
$$

Solution:

## Response

To solve the problem, we start with the given inequality:

\[
\frac{1}{\sqrt{a+b}} + \frac{1}{\sqrt{b+c}} + \frac{1}{\sqrt{c+a}} \geq \sqrt{\frac{C}{a+b+c+3}}.
\]

We know that \( ab + bc + ca = 3 \). We will use this condition to find a suitable bound for \( C \).

### Step 1: Apply Cauchy-Schwarz Inequality

Using the Cauchy-Schwarz inequality, we can estimate the left-hand side:

\[
\left( \frac{1}{\sqrt{a+b}} + \frac{1}{\sqrt{b+c}} + \frac{1}{\sqrt{c+a}} \right)^2 \leq (1 + 1 + 1) \left( \frac{1}{a+b} + \frac{1}{b+c} + \frac{1}{c+a} \right).
\]

This simplifies to:

\[
\left( \frac{1}{\sqrt{a+b}} + \frac{1}{\sqrt{b+c}} + \frac{1}{\sqrt{c+a}} \right)^2 \leq 3 \left( \frac{1}{a+b} + \frac{1}{b+c} + \frac{1}{c+a} \right).
\]

### Step 2: Estimate \( \frac{1}{a+b} + \frac{1}{b+c} + \frac{1}{c+a} \)

Next, we need to estimate \( \frac{1}{a+b} + \frac{1}{b+c} + \frac{1}{c+a} \). By applying the Cauchy-Schwarz inequality again, we have:

\[
\frac{1}{a+b} + \frac{1}{b+c} + \frac{1}{c+a} \geq \frac{(a+b+c)^2}{(a+b)(b+c)(c+a)}.
\]

### Step 3: Use the condition \( ab + bc + ca = 3 \)

We can express \( (a+b)(b+c)(c+a) \) in terms of \( a+b+c \) and \( ab + ac + bc \):

\[
(a+b)(b+c)(c+a) = (a+b+c)(ab+bc+ca) - abc.
\]

Given \( ab + bc + ca = 3 \), we have:

\[
(a+b)(b+c)(c+a) = 3(a+b+c) - abc.
\]

### Step 4: Find a lower bound for \( a+b+c \)

Using the AM-GM inequality, we know:

\[
\frac{a+b+c}{3} \geq \sqrt[3]{abc}.
\]

Let \( a = b = c = 1 \) (which satisfies \( ab + ac + bc = 3 \)). Then \( a+b+c = 3 \).

### Step 5: Substitute back into the inequality

Now we can substitute back into our inequality:

\[
\frac{1}{\sqrt{a+b}} + \frac{1}{\sqrt{b+c}} + \frac{1}{\sqrt{c+a}} \geq \frac{3}{\sqrt{2}}.
\]

### Step 6: Find \( C \)

We need to find \( C \) such that:

\[
\frac{3}{\sqrt{2}} \geq \sqrt{\frac{C}{3 + 3}} = \sqrt{\frac{C}{6}}.
\]

Squaring both sides gives:

\[
\frac{9}{2} \geq \frac{C}{6} \implies C \leq 27.
\]

### Conclusion

Thus, the largest constant \( C \) such that the inequality holds for all positive real numbers \( a, b, c \) satisfying \( ab + ac + bc = 3 \) is:

\[
\boxed{27}.
\]

Therefore, the answer is:

The answer is \( C=27 \).