## Problem

Find the smallest constant $C$ such that for all real numbers $x$ and $y$, the following inequality holds:
$$
x^2 + x + y^2 + y + C \geq x y
$$

## Query

Task description: Please solve the problem with clear, rigorous, and logically sound steps. At the end of your response, state your answer in exactly this format: 'The answer is $C=X$', where X is your calculated numerical bound value. Example: 'The answer is $C=1$'.

Here are some example problems and solutions that are related to the problem you are solving:

Example Problem 1: Let $a, b, c$ be the side lengths, $h_{a}, h_{b}, h_{c}$ be the altitudes, respectively, and $r$ be the inradius of a triangle. Find the largest constant $C$ such that the following inequality holds for all triangles:
$$
\frac{1}{h_{a}-2 r}+\frac{1}{h_{b}-2 r}+\frac{1}{h_{c}-2 r} \geq C \cdot r
$$
Solution of Example Problem 1: By $\frac{1}{h_{a}}+\frac{1}{h_{b}}+\frac{1}{h_{c}}=\frac{1}{r}$ we obtain
$$
\frac{h_{a}-2 r}{h_{a}}+\frac{h_{b}-2 r}{h_{b}}+\frac{h_{c}-2 r}{h_{c}}=1
$$

Applying $A M \geq H M$ we get
$$
\left(\frac{h_{a}-2 r}{h_{a}}+\frac{h_{b}-2 r}{h_{b}}+\frac{h_{c}-2 r}{h_{c}}\right)\left(\frac{h_{a}}{h_{a}-2 r}+\frac{h_{b}}{h_{b}-2 r}+\frac{h_{c}}{h_{c}-2 r}\right) \geq 9
$$
i.e.
$$
\frac{h_{a}}{h_{a}-2 r}+\frac{h_{b}}{h_{b}-2 r}+\frac{h_{c}}{h_{c}-2 r} \geq 9
$$

Therefore
$$
\begin{aligned}
& \frac{2 r}{h_{a}-2 r}+\frac{2 r}{h_{b}-2 r}+\frac{2 r}{h_{c}-2 r} \\
& \quad=\frac{h_{a}-\left(h_{a}-2 r\right)}{h_{a}-2 r}+\frac{h_{b}-\left(h_{b}-2 r\right)}{h_{b}-2 r}+\frac{h_{c}-\left(h_{c}-2 r\right)}{h_{c}-2 r} \\
& \quad=\frac{h_{a}}{h_{a}-2 r}+\frac{h_{b}}{h_{b}-2 r}+\frac{h_{c}}{h_{c}-2 r}-3 \geq 9-3=6
\end{aligned}
$$
i.e.
$$
\frac{1}{h_{a}-2 r}+\frac{1}{h_{b}-2 r}+\frac{1}{h_{c}-2 r} \geq \frac{3}{r}
$$
Answer of Example Problem 1: $$C = 3$$

Example Problem 2: Let $a, b, c$ be positive real numbers such that $a^2 + b^2 + c^2 = 3abc$. Find the largest constant $C$ such that the following inequality holds for all $a, b, c$ satisfying the given constraint:
$$
\frac{a}{b^2 c^2} + \frac{b}{c^2 a^2} + \frac{c}{a^2 b^2} \geq \frac{C}{a+b+c}
$$
Solution of Example Problem 2: The given inequality is equivalent to
$$
\left(a^{3}+b^{3}+c^{3}\right)(a+b+c) \geq 9 a^{2} b^{2} c^{2}
$$

Applying the Cauchy-Schwarz inequality we have
$$
\left(a^{3}+b^{3}+c^{3}\right)(a+b+c) \geq\left(a^{2}+b^{2}+c^{2}\right)^{2}
$$

Since $a^{2}+b^{2}+c^{2}=3 a b c$ we obtain
$$
\left(a^{3}+b^{3}+c^{3}\right)(a+b+c) \geq\left(a^{2}+b^{2}+c^{2}\right)^{2}=(3 a b c)^{2}=9 a^{2} b^{2} c^{2}
$$

Equality holds if and only if $a=b=c=1$.
Answer of Example Problem 2: $$C = 9$$

Example Problem 3: Let $a, b, c$ be positive real numbers such that $a b c = 1$. Find the largest constant $C$ such that the following inequality holds for all $a, b, c$ satisfying the given constraint:
$$
\frac{b+c}{\sqrt{a}}+\frac{c+a}{\sqrt{b}}+\frac{a+b}{\sqrt{c}} \geq \sqrt{a}+\sqrt{b}+\sqrt{c}+C
$$
Solution of Example Problem 3: [Solution 1]
From the AM-GM Inequality, we have

$$
\begin{aligned}
& \frac{b+c}{\sqrt{a}}+\frac{c+a}{\sqrt{b}}+\frac{a+b}{\sqrt{c}} \geq 2\left(\sqrt{\frac{b c}{a}}+\sqrt{\frac{c a}{b}}+\sqrt{\frac{a b}{c}}\right)= \\
& =\left(\sqrt{\frac{b c}{a}}+\sqrt{\frac{c a}{b}}\right)+\left(\sqrt{\frac{c a}{b}}+\sqrt{\frac{a b}{c}}\right)+\left(\sqrt{\frac{a b}{c}}+\sqrt{\frac{b c}{a}}\right) \geq \\
& \geq 2(\sqrt{a}+\sqrt{b}+\sqrt{c}) \geq \sqrt{a}+\sqrt{b}+\sqrt{c}+3 \sqrt[6]{a b c}=\sqrt{a}+\sqrt{b}+\sqrt{c}+3 .
\end{aligned}
$$
Answer of Example Problem 3: $$C = 3$$


Problem: Find the smallest constant $C$ such that for all real numbers $x$ and $y$, the following inequality holds:
$$
x^2 + x + y^2 + y + C \geq x y
$$

Solution:

## Response

To solve the inequality 

\[
x^2 + x + y^2 + y + C \geq xy,
\]

we can rearrange it to isolate \(C\):

\[
x^2 - xy + y^2 + x + y + C \geq 0.
\]

This can be viewed as a quadratic in \(x\):

\[
x^2 - xy + (y^2 + x + y + C) \geq 0.
\]

For this quadratic inequality to hold for all \(x\), the discriminant must be non-positive. The discriminant \(\Delta\) of the quadratic \(Ax^2 + Bx + C\) is given by:

\[
\Delta = B^2 - 4AC.
\]

In our case, \(A = 1\), \(B = -y\), and \(C = y^2 + x + y + C\). Thus, the discriminant is:

\[
\Delta = (-y)^2 - 4(1)(y^2 + x + y + C) = y^2 - 4(y^2 + x + y + C).
\]

Simplifying this gives:

\[
\Delta = y^2 - 4y^2 - 4x - 4y - 4C = -3y^2 - 4x - 4y - 4C.
\]

For the quadratic to be non-negative for all \(x\), we require:

\[
-3y^2 - 4y - 4C \leq 0.
\]

This must hold for all \(y\). The expression \(-3y^2 - 4y\) is a downward-opening parabola, and its maximum occurs at 

\[
y = -\frac{b}{2a} = -\frac{-4}{2 \cdot -3} = \frac{2}{3}.
\]

Calculating the maximum value at \(y = -\frac{2}{3}\):

\[
-3\left(-\frac{2}{3}\right)^2 - 4\left(-\frac{2}{3}\right) = -3 \cdot \frac{4}{9} + \frac{8}{3} = -\frac{4}{3} + \frac{8}{3} = \frac{4}{3}.
\]

Thus, we need:

\[
\frac{4}{3} - 4C \leq 0 \implies 4C \geq \frac{4}{3} \implies C \geq \frac{1}{3}.
\]

To check if \(C = \frac{1}{3}\) works, we substitute \(C\) back into the inequality:

\[
x^2 + x + y^2 + y + \frac{1}{3} \geq xy.
\]

Rearranging gives:

\[
x^2 - xy + y^2 + x + y + \frac{1}{3} \geq 0.
\]

The discriminant condition we derived earlier becomes:

\[
-3y^2 - 4y - \frac{4}{3} \leq 0.
\]

Multiplying through by \(-1\) (which reverses the inequality):

\[
3y^2 + 4y + \frac{4}{3} \geq 0.
\]

The discriminant of this quadratic is:

\[
4^2 - 4 \cdot 3 \cdot \frac{4}{3} = 16 - 16 = 0.
\]

Since the discriminant is zero, the quadratic has a double root and is non-negative for all \(y\). Thus, \(C = \frac{1}{3}\) is indeed the smallest constant satisfying the original inequality.

Therefore, the answer is 

\[
\text{The answer is } C = \frac{1}{3}.
\]