## Problem

Given $a, b, c \geq 0$ satisfying $a b+b c+c a>0$, find the largest constant $C$ such that the following inequality holds for all $a, b, c$:

$$
\sqrt{\frac{a}{b^2+b c+c^2}}+\sqrt{\frac{b}{c^2+c a+a^2}}+\sqrt{\frac{c}{a^2+a b+b^2}} \geq C \sqrt{\frac{a b+b c+c a}{(a+b)(b+c)(c+a)}}
$$

## Query

Task description: Please solve the problem with clear, rigorous, and logically sound steps. At the end of your response, state your answer in exactly this format: 'The answer is $C=X$', where X is your calculated numerical bound value. Example: 'The answer is $C=1$'.

Here are some example problems and solutions that are related to the problem you are solving:

Example Problem 1: Let $a, b, c$ be the side lengths, $h_{a}, h_{b}, h_{c}$ be the altitudes, respectively, and $r$ be the inradius of a triangle. Find the largest constant $C$ such that the following inequality holds for all triangles:
$$
\frac{1}{h_{a}-2 r}+\frac{1}{h_{b}-2 r}+\frac{1}{h_{c}-2 r} \geq C \cdot r
$$
Solution of Example Problem 1: By $\frac{1}{h_{a}}+\frac{1}{h_{b}}+\frac{1}{h_{c}}=\frac{1}{r}$ we obtain
$$
\frac{h_{a}-2 r}{h_{a}}+\frac{h_{b}-2 r}{h_{b}}+\frac{h_{c}-2 r}{h_{c}}=1
$$

Applying $A M \geq H M$ we get
$$
\left(\frac{h_{a}-2 r}{h_{a}}+\frac{h_{b}-2 r}{h_{b}}+\frac{h_{c}-2 r}{h_{c}}\right)\left(\frac{h_{a}}{h_{a}-2 r}+\frac{h_{b}}{h_{b}-2 r}+\frac{h_{c}}{h_{c}-2 r}\right) \geq 9
$$
i.e.
$$
\frac{h_{a}}{h_{a}-2 r}+\frac{h_{b}}{h_{b}-2 r}+\frac{h_{c}}{h_{c}-2 r} \geq 9
$$

Therefore
$$
\begin{aligned}
& \frac{2 r}{h_{a}-2 r}+\frac{2 r}{h_{b}-2 r}+\frac{2 r}{h_{c}-2 r} \\
& \quad=\frac{h_{a}-\left(h_{a}-2 r\right)}{h_{a}-2 r}+\frac{h_{b}-\left(h_{b}-2 r\right)}{h_{b}-2 r}+\frac{h_{c}-\left(h_{c}-2 r\right)}{h_{c}-2 r} \\
& \quad=\frac{h_{a}}{h_{a}-2 r}+\frac{h_{b}}{h_{b}-2 r}+\frac{h_{c}}{h_{c}-2 r}-3 \geq 9-3=6
\end{aligned}
$$
i.e.
$$
\frac{1}{h_{a}-2 r}+\frac{1}{h_{b}-2 r}+\frac{1}{h_{c}-2 r} \geq \frac{3}{r}
$$
Answer of Example Problem 1: $$C = 3$$

Example Problem 2: Let $a, b, c$ be positive real numbers such that $a^2 + b^2 + c^2 = 3abc$. Find the largest constant $C$ such that the following inequality holds for all $a, b, c$ satisfying the given constraint:
$$
\frac{a}{b^2 c^2} + \frac{b}{c^2 a^2} + \frac{c}{a^2 b^2} \geq \frac{C}{a+b+c}
$$
Solution of Example Problem 2: The given inequality is equivalent to
$$
\left(a^{3}+b^{3}+c^{3}\right)(a+b+c) \geq 9 a^{2} b^{2} c^{2}
$$

Applying the Cauchy-Schwarz inequality we have
$$
\left(a^{3}+b^{3}+c^{3}\right)(a+b+c) \geq\left(a^{2}+b^{2}+c^{2}\right)^{2}
$$

Since $a^{2}+b^{2}+c^{2}=3 a b c$ we obtain
$$
\left(a^{3}+b^{3}+c^{3}\right)(a+b+c) \geq\left(a^{2}+b^{2}+c^{2}\right)^{2}=(3 a b c)^{2}=9 a^{2} b^{2} c^{2}
$$

Equality holds if and only if $a=b=c=1$.
Answer of Example Problem 2: $$C = 9$$

Example Problem 3: Let $a, b, c$ be positive real numbers such that $a b c = 1$. Find the largest constant $C$ such that the following inequality holds for all $a, b, c$ satisfying the given constraint:
$$
\frac{b+c}{\sqrt{a}}+\frac{c+a}{\sqrt{b}}+\frac{a+b}{\sqrt{c}} \geq \sqrt{a}+\sqrt{b}+\sqrt{c}+C
$$
Solution of Example Problem 3: [Solution 1]
From the AM-GM Inequality, we have

$$
\begin{aligned}
& \frac{b+c}{\sqrt{a}}+\frac{c+a}{\sqrt{b}}+\frac{a+b}{\sqrt{c}} \geq 2\left(\sqrt{\frac{b c}{a}}+\sqrt{\frac{c a}{b}}+\sqrt{\frac{a b}{c}}\right)= \\
& =\left(\sqrt{\frac{b c}{a}}+\sqrt{\frac{c a}{b}}\right)+\left(\sqrt{\frac{c a}{b}}+\sqrt{\frac{a b}{c}}\right)+\left(\sqrt{\frac{a b}{c}}+\sqrt{\frac{b c}{a}}\right) \geq \\
& \geq 2(\sqrt{a}+\sqrt{b}+\sqrt{c}) \geq \sqrt{a}+\sqrt{b}+\sqrt{c}+3 \sqrt[6]{a b c}=\sqrt{a}+\sqrt{b}+\sqrt{c}+3 .
\end{aligned}
$$
Answer of Example Problem 3: $$C = 3$$


Problem: Given $a, b, c \geq 0$ satisfying $a b+b c+c a>0$, find the largest constant $C$ such that the following inequality holds for all $a, b, c$:

$$
\sqrt{\frac{a}{b^2+b c+c^2}}+\sqrt{\frac{b}{c^2+c a+a^2}}+\sqrt{\frac{c}{a^2+a b+b^2}} \geq C \sqrt{\frac{a b+b c+c a}{(a+b)(b+c)(c+a)}}
$$

Solution:

## Response

To solve the problem, we need to analyze the given inequality:

$$
\sqrt{\frac{a}{b^2+b c+c^2}}+\sqrt{\frac{b}{c^2+c a+a^2}}+\sqrt{\frac{c}{a^2+a b+b^2}} \geq C \sqrt{\frac{a b+b c+c a}{(a+b)(b+c)(c+a)}}
$$

We will denote:

- \( S = \sqrt{\frac{a}{b^2 + bc + c^2}} + \sqrt{\frac{b}{c^2 + ca + a^2}} + \sqrt{\frac{c}{a^2 + ab + b^2}} \)
- \( T = \sqrt{\frac{ab + bc + ca}{(a+b)(b+c)(c+a)}} \)

We want to find the largest constant \( C \) such that \( S \geq C T \).

### Step 1: Analyze the left-hand side \( S \)

Using the Cauchy-Schwarz inequality, we can estimate \( S \):

\[
S = \sqrt{\frac{a}{b^2 + bc + c^2}} + \sqrt{\frac{b}{c^2 + ca + a^2}} + \sqrt{\frac{c}{a^2 + ab + b^2}} \geq \frac{( \sqrt{a} + \sqrt{b} + \sqrt{c})^2}{\sqrt{(b^2 + bc + c^2)(c^2 + ca + a^2)(a^2 + ab + b^2)}}
\]

### Step 2: Analyze the right-hand side \( T \)

The term \( T \) can be simplified as follows:

\[
T = \sqrt{\frac{ab + bc + ca}{(a+b)(b+c)(c+a)}}
\]

### Step 3: Establish a relationship between \( S \) and \( T \)

To find \( C \), we will consider specific cases for \( a, b, c \) to derive bounds.

#### Case 1: Let \( a = b = 1 \) and \( c \to 0 \)

In this case:

- \( S \) becomes:
\[
S = \sqrt{\frac{1}{1^2 + 1 \cdot 0 + 0^2}} + \sqrt{\frac{1}{0^2 + 0 \cdot 1 + 1^2}} + \sqrt{\frac{0}{1^2 + 1 \cdot 0 + 0^2}} = 1 + 1 + 0 = 2
\]

- \( T \) becomes:
\[
T = \sqrt{\frac{1 \cdot 1 + 1 \cdot 0 + 0 \cdot 1}{(1+1)(1+0)(0+1)}} = \sqrt{\frac{1}{2}} = \frac{1}{\sqrt{2}}
\]

Thus, we have:

\[
2 \geq C \cdot \frac{1}{\sqrt{2}} \implies C \leq 2\sqrt{2}
\]

#### Case 2: Let \( a = b = c = 1 \)

In this case:

- \( S \) becomes:
\[
S = 3 \sqrt{\frac{1}{1^2 + 1 \cdot 1 + 1^2}} = 3 \sqrt{\frac{1}{3}} = \sqrt{3}
\]

- \( T \) becomes:
\[
T = \sqrt{\frac{1 + 1 + 1}{(1+1)(1+1)(1+1)}} = \sqrt{\frac{3}{8}} = \frac{\sqrt{3}}{2}
\]

Thus, we have:

\[
\sqrt{3} \geq C \cdot \frac{\sqrt{3}}{2} \implies C \leq 2
\]

### Conclusion

From the two cases, we have established that \( C \) must satisfy \( C \leq 2 \) and \( C \leq 2\sqrt{2} \). The tighter bound is \( C \leq 2 \).

Thus, the largest constant \( C \) such that the inequality holds for all non-negative \( a, b, c \) satisfying \( ab + bc + ca > 0 \) is:

The answer is \( C=2 \).