## Problem

Let $x, y, z \in [0,1]$. Determine the minimal constant $C$ such that the following inequality holds for all $x, y, z$:
$$
x(x-y)(z-x) \leq C.
$$

## Query

Task description: Please solve the problem with clear, rigorous, and logically sound steps. At the end of your response, state your answer in exactly this format: 'The answer is $C=X$', where X is your calculated numerical bound value. Example: 'The answer is $C=1$'.

Here are some example problems and solutions that are related to the problem you are solving:

Example Problem 1: Let $a, b, c$ be the side lengths, $h_{a}, h_{b}, h_{c}$ be the altitudes, respectively, and $r$ be the inradius of a triangle. Find the largest constant $C$ such that the following inequality holds for all triangles:
$$
\frac{1}{h_{a}-2 r}+\frac{1}{h_{b}-2 r}+\frac{1}{h_{c}-2 r} \geq C \cdot r
$$
Solution of Example Problem 1: By $\frac{1}{h_{a}}+\frac{1}{h_{b}}+\frac{1}{h_{c}}=\frac{1}{r}$ we obtain
$$
\frac{h_{a}-2 r}{h_{a}}+\frac{h_{b}-2 r}{h_{b}}+\frac{h_{c}-2 r}{h_{c}}=1
$$

Applying $A M \geq H M$ we get
$$
\left(\frac{h_{a}-2 r}{h_{a}}+\frac{h_{b}-2 r}{h_{b}}+\frac{h_{c}-2 r}{h_{c}}\right)\left(\frac{h_{a}}{h_{a}-2 r}+\frac{h_{b}}{h_{b}-2 r}+\frac{h_{c}}{h_{c}-2 r}\right) \geq 9
$$
i.e.
$$
\frac{h_{a}}{h_{a}-2 r}+\frac{h_{b}}{h_{b}-2 r}+\frac{h_{c}}{h_{c}-2 r} \geq 9
$$

Therefore
$$
\begin{aligned}
& \frac{2 r}{h_{a}-2 r}+\frac{2 r}{h_{b}-2 r}+\frac{2 r}{h_{c}-2 r} \\
& \quad=\frac{h_{a}-\left(h_{a}-2 r\right)}{h_{a}-2 r}+\frac{h_{b}-\left(h_{b}-2 r\right)}{h_{b}-2 r}+\frac{h_{c}-\left(h_{c}-2 r\right)}{h_{c}-2 r} \\
& \quad=\frac{h_{a}}{h_{a}-2 r}+\frac{h_{b}}{h_{b}-2 r}+\frac{h_{c}}{h_{c}-2 r}-3 \geq 9-3=6
\end{aligned}
$$
i.e.
$$
\frac{1}{h_{a}-2 r}+\frac{1}{h_{b}-2 r}+\frac{1}{h_{c}-2 r} \geq \frac{3}{r}
$$
Answer of Example Problem 1: $$C = 3$$

Example Problem 2: Let $a, b, c$ be positive real numbers such that $a^2 + b^2 + c^2 = 3abc$. Find the largest constant $C$ such that the following inequality holds for all $a, b, c$ satisfying the given constraint:
$$
\frac{a}{b^2 c^2} + \frac{b}{c^2 a^2} + \frac{c}{a^2 b^2} \geq \frac{C}{a+b+c}
$$
Solution of Example Problem 2: The given inequality is equivalent to
$$
\left(a^{3}+b^{3}+c^{3}\right)(a+b+c) \geq 9 a^{2} b^{2} c^{2}
$$

Applying the Cauchy-Schwarz inequality we have
$$
\left(a^{3}+b^{3}+c^{3}\right)(a+b+c) \geq\left(a^{2}+b^{2}+c^{2}\right)^{2}
$$

Since $a^{2}+b^{2}+c^{2}=3 a b c$ we obtain
$$
\left(a^{3}+b^{3}+c^{3}\right)(a+b+c) \geq\left(a^{2}+b^{2}+c^{2}\right)^{2}=(3 a b c)^{2}=9 a^{2} b^{2} c^{2}
$$

Equality holds if and only if $a=b=c=1$.
Answer of Example Problem 2: $$C = 9$$

Example Problem 3: Let $a, b, c$ be positive real numbers such that $a b c = 1$. Find the largest constant $C$ such that the following inequality holds for all $a, b, c$ satisfying the given constraint:
$$
\frac{b+c}{\sqrt{a}}+\frac{c+a}{\sqrt{b}}+\frac{a+b}{\sqrt{c}} \geq \sqrt{a}+\sqrt{b}+\sqrt{c}+C
$$
Solution of Example Problem 3: [Solution 1]
From the AM-GM Inequality, we have

$$
\begin{aligned}
& \frac{b+c}{\sqrt{a}}+\frac{c+a}{\sqrt{b}}+\frac{a+b}{\sqrt{c}} \geq 2\left(\sqrt{\frac{b c}{a}}+\sqrt{\frac{c a}{b}}+\sqrt{\frac{a b}{c}}\right)= \\
& =\left(\sqrt{\frac{b c}{a}}+\sqrt{\frac{c a}{b}}\right)+\left(\sqrt{\frac{c a}{b}}+\sqrt{\frac{a b}{c}}\right)+\left(\sqrt{\frac{a b}{c}}+\sqrt{\frac{b c}{a}}\right) \geq \\
& \geq 2(\sqrt{a}+\sqrt{b}+\sqrt{c}) \geq \sqrt{a}+\sqrt{b}+\sqrt{c}+3 \sqrt[6]{a b c}=\sqrt{a}+\sqrt{b}+\sqrt{c}+3 .
\end{aligned}
$$
Answer of Example Problem 3: $$C = 3$$


Problem: Let $x, y, z \in [0,1]$. Determine the minimal constant $C$ such that the following inequality holds for all $x, y, z$:
$$
x(x-y)(z-x) \leq C.
$$

Solution:

## Response

To solve the problem, we need to analyze the expression \( x(x-y)(z-x) \) for \( x, y, z \in [0, 1] \) and find the maximum value of this expression, which will give us the minimal constant \( C \) such that the inequality holds for all \( x, y, z \).

1. **Understanding the Expression**:
   The expression \( x(x-y)(z-x) \) can be rewritten as:
   \[
   x(zx - x^2 - yz + xy) = x^2(z-x) - xy(z-x)
   \]
   This shows that the expression is dependent on the values of \( x, y, z \).

2. **Finding Critical Points**:
   We will analyze the expression by considering the boundaries of the variables \( x, y, z \) since they are constrained to the interval \([0, 1]\).

3. **Case Analysis**:
   - **Case 1**: \( x = 0 \)
     \[
     0(0-y)(z-0) = 0
     \]
   - **Case 2**: \( x = 1 \)
     \[
     1(1-y)(z-1) = (1-y)(z-1)
     \]
     This expression can take values from \( 0 \) to \( 1 \) depending on \( y \) and \( z \).
   - **Case 3**: \( y = 0 \)
     \[
     x(x-0)(z-x) = x^2(z-x)
     \]
     This is maximized when \( z \) is maximized (i.e., \( z = 1 \)):
     \[
     x^2(1-x)
     \]
     The maximum of \( x^2(1-x) \) occurs at \( x = \frac{2}{3} \) (found by taking the derivative and setting it to zero):
     \[
     \left(\frac{2}{3}\right)^2\left(1 - \frac{2}{3}\right) = \frac{4}{9} \cdot \frac{1}{3} = \frac{4}{27}
     \]
   - **Case 4**: \( z = 0 \)
     \[
     x(x-y)(0-x) = -x^2(x-y)
     \]
     This is non-positive and does not contribute to the maximum.

4. **Maximizing the Expression**:
   We need to check the maximum values obtained from the cases:
   - From **Case 1**: \( 0 \)
   - From **Case 2**: \( (1-y)(z-1) \) can be \( 0 \) or negative.
   - From **Case 3**: The maximum value is \( \frac{4}{27} \).

5. **Conclusion**:
   The maximum value of \( x(x-y)(z-x) \) over the interval \( [0, 1] \) is \( \frac{4}{27} \). Therefore, the minimal constant \( C \) such that the inequality holds for all \( x, y, z \in [0, 1] \) is:

\[
\text{The answer is } C = \frac{4}{27}.
\]