## Problem

Let $a, b \geq 0$ and $(a+b)(1+4ab)=2$. Find the smallest constant $C$ such that the following inequality holds for all $a, b$ satisfying the given constraint:
$$
ab(a+b+ab) \leq C
$$

## Query

Task description: Please solve the problem with clear, rigorous, and logically sound steps. At the end of your response, state your answer in exactly this format: 'The answer is $C=X$', where X is your calculated numerical bound value. Example: 'The answer is $C=1$'.

Here are some example problems and solutions that are related to the problem you are solving:

Example Problem 1: Let $a, b, c$ be the side lengths, $h_{a}, h_{b}, h_{c}$ be the altitudes, respectively, and $r$ be the inradius of a triangle. Find the largest constant $C$ such that the following inequality holds for all triangles:
$$
\frac{1}{h_{a}-2 r}+\frac{1}{h_{b}-2 r}+\frac{1}{h_{c}-2 r} \geq C \cdot r
$$
Solution of Example Problem 1: By $\frac{1}{h_{a}}+\frac{1}{h_{b}}+\frac{1}{h_{c}}=\frac{1}{r}$ we obtain
$$
\frac{h_{a}-2 r}{h_{a}}+\frac{h_{b}-2 r}{h_{b}}+\frac{h_{c}-2 r}{h_{c}}=1
$$

Applying $A M \geq H M$ we get
$$
\left(\frac{h_{a}-2 r}{h_{a}}+\frac{h_{b}-2 r}{h_{b}}+\frac{h_{c}-2 r}{h_{c}}\right)\left(\frac{h_{a}}{h_{a}-2 r}+\frac{h_{b}}{h_{b}-2 r}+\frac{h_{c}}{h_{c}-2 r}\right) \geq 9
$$
i.e.
$$
\frac{h_{a}}{h_{a}-2 r}+\frac{h_{b}}{h_{b}-2 r}+\frac{h_{c}}{h_{c}-2 r} \geq 9
$$

Therefore
$$
\begin{aligned}
& \frac{2 r}{h_{a}-2 r}+\frac{2 r}{h_{b}-2 r}+\frac{2 r}{h_{c}-2 r} \\
& \quad=\frac{h_{a}-\left(h_{a}-2 r\right)}{h_{a}-2 r}+\frac{h_{b}-\left(h_{b}-2 r\right)}{h_{b}-2 r}+\frac{h_{c}-\left(h_{c}-2 r\right)}{h_{c}-2 r} \\
& \quad=\frac{h_{a}}{h_{a}-2 r}+\frac{h_{b}}{h_{b}-2 r}+\frac{h_{c}}{h_{c}-2 r}-3 \geq 9-3=6
\end{aligned}
$$
i.e.
$$
\frac{1}{h_{a}-2 r}+\frac{1}{h_{b}-2 r}+\frac{1}{h_{c}-2 r} \geq \frac{3}{r}
$$
Answer of Example Problem 1: $$C = 3$$

Example Problem 2: Let $a, b, c$ be positive real numbers such that $a^2 + b^2 + c^2 = 3abc$. Find the largest constant $C$ such that the following inequality holds for all $a, b, c$ satisfying the given constraint:
$$
\frac{a}{b^2 c^2} + \frac{b}{c^2 a^2} + \frac{c}{a^2 b^2} \geq \frac{C}{a+b+c}
$$
Solution of Example Problem 2: The given inequality is equivalent to
$$
\left(a^{3}+b^{3}+c^{3}\right)(a+b+c) \geq 9 a^{2} b^{2} c^{2}
$$

Applying the Cauchy-Schwarz inequality we have
$$
\left(a^{3}+b^{3}+c^{3}\right)(a+b+c) \geq\left(a^{2}+b^{2}+c^{2}\right)^{2}
$$

Since $a^{2}+b^{2}+c^{2}=3 a b c$ we obtain
$$
\left(a^{3}+b^{3}+c^{3}\right)(a+b+c) \geq\left(a^{2}+b^{2}+c^{2}\right)^{2}=(3 a b c)^{2}=9 a^{2} b^{2} c^{2}
$$

Equality holds if and only if $a=b=c=1$.
Answer of Example Problem 2: $$C = 9$$

Example Problem 3: Let $a, b, c$ be positive real numbers such that $a b c = 1$. Find the largest constant $C$ such that the following inequality holds for all $a, b, c$ satisfying the given constraint:
$$
\frac{b+c}{\sqrt{a}}+\frac{c+a}{\sqrt{b}}+\frac{a+b}{\sqrt{c}} \geq \sqrt{a}+\sqrt{b}+\sqrt{c}+C
$$
Solution of Example Problem 3: [Solution 1]
From the AM-GM Inequality, we have

$$
\begin{aligned}
& \frac{b+c}{\sqrt{a}}+\frac{c+a}{\sqrt{b}}+\frac{a+b}{\sqrt{c}} \geq 2\left(\sqrt{\frac{b c}{a}}+\sqrt{\frac{c a}{b}}+\sqrt{\frac{a b}{c}}\right)= \\
& =\left(\sqrt{\frac{b c}{a}}+\sqrt{\frac{c a}{b}}\right)+\left(\sqrt{\frac{c a}{b}}+\sqrt{\frac{a b}{c}}\right)+\left(\sqrt{\frac{a b}{c}}+\sqrt{\frac{b c}{a}}\right) \geq \\
& \geq 2(\sqrt{a}+\sqrt{b}+\sqrt{c}) \geq \sqrt{a}+\sqrt{b}+\sqrt{c}+3 \sqrt[6]{a b c}=\sqrt{a}+\sqrt{b}+\sqrt{c}+3 .
\end{aligned}
$$
Answer of Example Problem 3: $$C = 3$$


Problem: Let $a, b \geq 0$ and $(a+b)(1+4ab)=2$. Find the smallest constant $C$ such that the following inequality holds for all $a, b$ satisfying the given constraint:
$$
ab(a+b+ab) \leq C
$$

Solution:

## Response

To solve the problem, we start with the given constraint:

\[
(a+b)(1+4ab) = 2.
\]

We need to find the smallest constant \( C \) such that the inequality 

\[
ab(a+b+ab) \leq C
\]

holds for all non-negative \( a \) and \( b \) satisfying the constraint.

### Step 1: Express \( a+b \) in terms of \( ab \)

Let \( s = a + b \) and \( p = ab \). The constraint can be rewritten as:

\[
s(1 + 4p) = 2 \implies s = \frac{2}{1 + 4p}.
\]

### Step 2: Substitute \( s \) into the inequality

We need to express \( ab(a+b+ab) \) in terms of \( p \):

\[
ab(a+b+ab) = p\left(s + p\right) = p\left(\frac{2}{1 + 4p} + p\right).
\]

### Step 3: Simplify the expression

Substituting \( s \):

\[
ab(a+b+ab) = p\left(\frac{2}{1 + 4p} + p\right) = p\left(\frac{2 + p(1 + 4p)}{1 + 4p}\right) = \frac{p(2 + p + 4p^2)}{1 + 4p}.
\]

### Step 4: Analyze the function

Let 

\[
f(p) = \frac{p(2 + p + 4p^2)}{1 + 4p}.
\]

We need to find the maximum value of \( f(p) \) for \( p \geq 0 \) under the constraint \( s = \frac{2}{1 + 4p} \).

### Step 5: Find the maximum of \( f(p) \)

To find the maximum, we can differentiate \( f(p) \) with respect to \( p \) and set the derivative to zero. However, we can also evaluate \( f(p) \) at specific values of \( p \) to find the maximum.

1. **When \( p = 0 \)**:
   \[
   f(0) = 0.
   \]

2. **When \( p = \frac{1}{4} \)** (which is a reasonable guess since it simplifies the constraint):
   \[
   s = \frac{2}{1 + 4 \cdot \frac{1}{4}} = \frac{2}{2} = 1.
   \]
   Then \( ab = \frac{1}{4} \) and \( a + b = 1 \). The values \( a \) and \( b \) can be \( \frac{1}{2} \) each, thus:
   \[
   ab(a+b+ab) = \frac{1}{4}\left(1 + \frac{1}{4}\right) = \frac{1}{4} \cdot \frac{5}{4} = \frac{5}{16}.
   \]

3. **When \( p = \frac{1}{2} \)**:
   \[
   s = \frac{2}{1 + 4 \cdot \frac{1}{2}} = \frac{2}{3}.
   \]
   Then \( ab = \frac{1}{2} \) and \( a + b = \frac{2}{3} \). The values \( a \) and \( b \) can be \( \frac{1}{3} \) each, thus:
   \[
   ab(a+b+ab) = \frac{1}{2}\left(\frac{2}{3} + \frac{1}{2}\right) = \frac{1}{2}\left(\frac{4}{6} + \frac{3}{6}\right) = \frac{1}{2} \cdot \frac{7}{6} = \frac{7}{12}.
   \]

### Step 6: Compare values

We have calculated:

- \( f(0) = 0 \)
- \( f\left(\frac{1}{4}\right) = \frac{5}{16} \)
- \( f\left(\frac{1}{2}\right) = \frac{7}{12} \)

To find the maximum, we can convert \( \frac{5}{16} \) and \( \frac{7}{12} \) to a common denominator:

- \( \frac{5}{16} = \frac{15}{48} \)
- \( \frac{7}{12} = \frac{28}{48} \)

Thus, the maximum value of \( ab(a+b+ab) \) is \( \frac{7}{12} \).

### Conclusion

The smallest constant \( C \) such that the inequality holds for all \( a, b \) satisfying the constraint is:

\[
\boxed{C = \frac{7}{12}}.
\]

Thus, the final answer is:

The answer is \( C = \frac{7}{12} \).