## Problem

Let $a, b, c$ be positive real numbers such that $a+b+c=3$. Determine the maximal constant $C$ such that the following inequality holds for all $a, b, c$:

$$
\frac{a}{1+2 b^3}+\frac{b}{1+2 c^3}+\frac{c}{1+2 a^3} \geq C.
$$

## Query

Task description: Please solve the problem with clear, rigorous, and logically sound steps. At the end of your response, state your answer in exactly this format: 'The answer is $C=X$', where X is your calculated numerical bound value. Example: 'The answer is $C=1$'.

Here are some example problems and solutions that are related to the problem you are solving:

Example Problem 1: Let $a, b, c$ be the side lengths, $h_{a}, h_{b}, h_{c}$ be the altitudes, respectively, and $r$ be the inradius of a triangle. Find the largest constant $C$ such that the following inequality holds for all triangles:
$$
\frac{1}{h_{a}-2 r}+\frac{1}{h_{b}-2 r}+\frac{1}{h_{c}-2 r} \geq C \cdot r
$$
Solution of Example Problem 1: By $\frac{1}{h_{a}}+\frac{1}{h_{b}}+\frac{1}{h_{c}}=\frac{1}{r}$ we obtain
$$
\frac{h_{a}-2 r}{h_{a}}+\frac{h_{b}-2 r}{h_{b}}+\frac{h_{c}-2 r}{h_{c}}=1
$$

Applying $A M \geq H M$ we get
$$
\left(\frac{h_{a}-2 r}{h_{a}}+\frac{h_{b}-2 r}{h_{b}}+\frac{h_{c}-2 r}{h_{c}}\right)\left(\frac{h_{a}}{h_{a}-2 r}+\frac{h_{b}}{h_{b}-2 r}+\frac{h_{c}}{h_{c}-2 r}\right) \geq 9
$$
i.e.
$$
\frac{h_{a}}{h_{a}-2 r}+\frac{h_{b}}{h_{b}-2 r}+\frac{h_{c}}{h_{c}-2 r} \geq 9
$$

Therefore
$$
\begin{aligned}
& \frac{2 r}{h_{a}-2 r}+\frac{2 r}{h_{b}-2 r}+\frac{2 r}{h_{c}-2 r} \\
& \quad=\frac{h_{a}-\left(h_{a}-2 r\right)}{h_{a}-2 r}+\frac{h_{b}-\left(h_{b}-2 r\right)}{h_{b}-2 r}+\frac{h_{c}-\left(h_{c}-2 r\right)}{h_{c}-2 r} \\
& \quad=\frac{h_{a}}{h_{a}-2 r}+\frac{h_{b}}{h_{b}-2 r}+\frac{h_{c}}{h_{c}-2 r}-3 \geq 9-3=6
\end{aligned}
$$
i.e.
$$
\frac{1}{h_{a}-2 r}+\frac{1}{h_{b}-2 r}+\frac{1}{h_{c}-2 r} \geq \frac{3}{r}
$$
Answer of Example Problem 1: $$C = 3$$

Example Problem 2: Let $a, b, c$ be positive real numbers such that $a^2 + b^2 + c^2 = 3abc$. Find the largest constant $C$ such that the following inequality holds for all $a, b, c$ satisfying the given constraint:
$$
\frac{a}{b^2 c^2} + \frac{b}{c^2 a^2} + \frac{c}{a^2 b^2} \geq \frac{C}{a+b+c}
$$
Solution of Example Problem 2: The given inequality is equivalent to
$$
\left(a^{3}+b^{3}+c^{3}\right)(a+b+c) \geq 9 a^{2} b^{2} c^{2}
$$

Applying the Cauchy-Schwarz inequality we have
$$
\left(a^{3}+b^{3}+c^{3}\right)(a+b+c) \geq\left(a^{2}+b^{2}+c^{2}\right)^{2}
$$

Since $a^{2}+b^{2}+c^{2}=3 a b c$ we obtain
$$
\left(a^{3}+b^{3}+c^{3}\right)(a+b+c) \geq\left(a^{2}+b^{2}+c^{2}\right)^{2}=(3 a b c)^{2}=9 a^{2} b^{2} c^{2}
$$

Equality holds if and only if $a=b=c=1$.
Answer of Example Problem 2: $$C = 9$$

Example Problem 3: Let $a, b, c$ be positive real numbers such that $a b c = 1$. Find the largest constant $C$ such that the following inequality holds for all $a, b, c$ satisfying the given constraint:
$$
\frac{b+c}{\sqrt{a}}+\frac{c+a}{\sqrt{b}}+\frac{a+b}{\sqrt{c}} \geq \sqrt{a}+\sqrt{b}+\sqrt{c}+C
$$
Solution of Example Problem 3: [Solution 1]
From the AM-GM Inequality, we have

$$
\begin{aligned}
& \frac{b+c}{\sqrt{a}}+\frac{c+a}{\sqrt{b}}+\frac{a+b}{\sqrt{c}} \geq 2\left(\sqrt{\frac{b c}{a}}+\sqrt{\frac{c a}{b}}+\sqrt{\frac{a b}{c}}\right)= \\
& =\left(\sqrt{\frac{b c}{a}}+\sqrt{\frac{c a}{b}}\right)+\left(\sqrt{\frac{c a}{b}}+\sqrt{\frac{a b}{c}}\right)+\left(\sqrt{\frac{a b}{c}}+\sqrt{\frac{b c}{a}}\right) \geq \\
& \geq 2(\sqrt{a}+\sqrt{b}+\sqrt{c}) \geq \sqrt{a}+\sqrt{b}+\sqrt{c}+3 \sqrt[6]{a b c}=\sqrt{a}+\sqrt{b}+\sqrt{c}+3 .
\end{aligned}
$$
Answer of Example Problem 3: $$C = 3$$


Problem: Let $a, b, c$ be positive real numbers such that $a+b+c=3$. Determine the maximal constant $C$ such that the following inequality holds for all $a, b, c$:

$$
\frac{a}{1+2 b^3}+\frac{b}{1+2 c^3}+\frac{c}{1+2 a^3} \geq C.
$$

Solution:

## Response

To solve the problem, we need to find the largest constant \( C \) such that the following inequality holds for all positive real numbers \( a, b, c \) satisfying \( a + b + c = 3 \):

\[
\frac{a}{1 + 2b^3} + \frac{b}{1 + 2c^3} + \frac{c}{1 + 2a^3} \geq C.
\]

### Step 1: Analyze the expression

We will analyze the left-hand side of the inequality. The terms \( 1 + 2b^3 \), \( 1 + 2c^3 \), and \( 1 + 2a^3 \) are always positive since \( a, b, c \) are positive. 

### Step 2: Use symmetry and test cases

To find a lower bound for the left-hand side, we can test specific cases where \( a, b, c \) are equal. Let \( a = b = c = 1 \) (since \( a + b + c = 3 \)):

\[
\frac{1}{1 + 2 \cdot 1^3} + \frac{1}{1 + 2 \cdot 1^3} + \frac{1}{1 + 2 \cdot 1^3} = 3 \cdot \frac{1}{1 + 2} = 3 \cdot \frac{1}{3} = 1.
\]

This suggests that \( C \leq 1 \).

### Step 3: Prove that \( C = 1 \) is achievable

Next, we need to show that the inequality holds for all positive \( a, b, c \) such that \( a + b + c = 3 \). 

Using the Cauchy-Schwarz inequality, we can derive:

\[
\left( \frac{a}{1 + 2b^3} + \frac{b}{1 + 2c^3} + \frac{c}{1 + 2a^3} \right) \left( (1 + 2b^3) + (1 + 2c^3) + (1 + 2a^3) \right) \geq (a + b + c)^2.
\]

Calculating the second term:

\[
(1 + 2b^3) + (1 + 2c^3) + (1 + 2a^3) = 3 + 2(a^3 + b^3 + c^3).
\]

Thus, we have:

\[
\left( \frac{a}{1 + 2b^3} + \frac{b}{1 + 2c^3} + \frac{c}{1 + 2a^3} \right) (3 + 2(a^3 + b^3 + c^3)) \geq 9.
\]

### Step 4: Bound \( a^3 + b^3 + c^3 \)

Using the Power Mean inequality, we know:

\[
\sqrt[3]{\frac{a^3 + b^3 + c^3}{3}} \leq \frac{a + b + c}{3} = 1 \implies a^3 + b^3 + c^3 \leq 3.
\]

Substituting this into our inequality gives:

\[
\left( \frac{a}{1 + 2b^3} + \frac{b}{1 + 2c^3} + \frac{c}{1 + 2a^3} \right) (3 + 2 \cdot 3) \geq 9,
\]

which simplifies to:

\[
\left( \frac{a}{1 + 2b^3} + \frac{b}{1 + 2c^3} + \frac{c}{1 + 2a^3} \right) \cdot 9 \geq 9.
\]

Thus, we conclude:

\[
\frac{a}{1 + 2b^3} + \frac{b}{1 + 2c^3} + \frac{c}{1 + 2a^3} \geq 1.
\]

### Conclusion

Since we have shown that the inequality holds for all positive \( a, b, c \) such that \( a + b + c = 3 \) and that \( C = 1 \) is achievable, we conclude that the largest constant \( C \) is:

\[
\text{The answer is } C = 1.
\]