## Problem

Let $a, b > 0$ and $a + b \leq \frac{3}{2}$. Find the smallest constant $C$ such that the following inequality holds for all $a, b$ satisfying the given constraint:
$$
\frac{a}{a^2+1} + \frac{4b}{b^2+4} \leq C.
$$

## Query

Task description: Please solve the problem with clear, rigorous, and logically sound steps. At the end of your response, state your answer in exactly this format: 'The answer is $C=X$', where X is your calculated numerical bound value. Example: 'The answer is $C=1$'.

Here are some example problems and solutions that are related to the problem you are solving:

Example Problem 1: Let $a, b, c$ be the side lengths, $h_{a}, h_{b}, h_{c}$ be the altitudes, respectively, and $r$ be the inradius of a triangle. Find the largest constant $C$ such that the following inequality holds for all triangles:
$$
\frac{1}{h_{a}-2 r}+\frac{1}{h_{b}-2 r}+\frac{1}{h_{c}-2 r} \geq C \cdot r
$$
Solution of Example Problem 1: By $\frac{1}{h_{a}}+\frac{1}{h_{b}}+\frac{1}{h_{c}}=\frac{1}{r}$ we obtain
$$
\frac{h_{a}-2 r}{h_{a}}+\frac{h_{b}-2 r}{h_{b}}+\frac{h_{c}-2 r}{h_{c}}=1
$$

Applying $A M \geq H M$ we get
$$
\left(\frac{h_{a}-2 r}{h_{a}}+\frac{h_{b}-2 r}{h_{b}}+\frac{h_{c}-2 r}{h_{c}}\right)\left(\frac{h_{a}}{h_{a}-2 r}+\frac{h_{b}}{h_{b}-2 r}+\frac{h_{c}}{h_{c}-2 r}\right) \geq 9
$$
i.e.
$$
\frac{h_{a}}{h_{a}-2 r}+\frac{h_{b}}{h_{b}-2 r}+\frac{h_{c}}{h_{c}-2 r} \geq 9
$$

Therefore
$$
\begin{aligned}
& \frac{2 r}{h_{a}-2 r}+\frac{2 r}{h_{b}-2 r}+\frac{2 r}{h_{c}-2 r} \\
& \quad=\frac{h_{a}-\left(h_{a}-2 r\right)}{h_{a}-2 r}+\frac{h_{b}-\left(h_{b}-2 r\right)}{h_{b}-2 r}+\frac{h_{c}-\left(h_{c}-2 r\right)}{h_{c}-2 r} \\
& \quad=\frac{h_{a}}{h_{a}-2 r}+\frac{h_{b}}{h_{b}-2 r}+\frac{h_{c}}{h_{c}-2 r}-3 \geq 9-3=6
\end{aligned}
$$
i.e.
$$
\frac{1}{h_{a}-2 r}+\frac{1}{h_{b}-2 r}+\frac{1}{h_{c}-2 r} \geq \frac{3}{r}
$$
Answer of Example Problem 1: $$C = 3$$

Example Problem 2: Let $a, b, c$ be positive real numbers such that $a^2 + b^2 + c^2 = 3abc$. Find the largest constant $C$ such that the following inequality holds for all $a, b, c$ satisfying the given constraint:
$$
\frac{a}{b^2 c^2} + \frac{b}{c^2 a^2} + \frac{c}{a^2 b^2} \geq \frac{C}{a+b+c}
$$
Solution of Example Problem 2: The given inequality is equivalent to
$$
\left(a^{3}+b^{3}+c^{3}\right)(a+b+c) \geq 9 a^{2} b^{2} c^{2}
$$

Applying the Cauchy-Schwarz inequality we have
$$
\left(a^{3}+b^{3}+c^{3}\right)(a+b+c) \geq\left(a^{2}+b^{2}+c^{2}\right)^{2}
$$

Since $a^{2}+b^{2}+c^{2}=3 a b c$ we obtain
$$
\left(a^{3}+b^{3}+c^{3}\right)(a+b+c) \geq\left(a^{2}+b^{2}+c^{2}\right)^{2}=(3 a b c)^{2}=9 a^{2} b^{2} c^{2}
$$

Equality holds if and only if $a=b=c=1$.
Answer of Example Problem 2: $$C = 9$$

Example Problem 3: Let $a, b, c$ be positive real numbers such that $a b c = 1$. Find the largest constant $C$ such that the following inequality holds for all $a, b, c$ satisfying the given constraint:
$$
\frac{b+c}{\sqrt{a}}+\frac{c+a}{\sqrt{b}}+\frac{a+b}{\sqrt{c}} \geq \sqrt{a}+\sqrt{b}+\sqrt{c}+C
$$
Solution of Example Problem 3: [Solution 1]
From the AM-GM Inequality, we have

$$
\begin{aligned}
& \frac{b+c}{\sqrt{a}}+\frac{c+a}{\sqrt{b}}+\frac{a+b}{\sqrt{c}} \geq 2\left(\sqrt{\frac{b c}{a}}+\sqrt{\frac{c a}{b}}+\sqrt{\frac{a b}{c}}\right)= \\
& =\left(\sqrt{\frac{b c}{a}}+\sqrt{\frac{c a}{b}}\right)+\left(\sqrt{\frac{c a}{b}}+\sqrt{\frac{a b}{c}}\right)+\left(\sqrt{\frac{a b}{c}}+\sqrt{\frac{b c}{a}}\right) \geq \\
& \geq 2(\sqrt{a}+\sqrt{b}+\sqrt{c}) \geq \sqrt{a}+\sqrt{b}+\sqrt{c}+3 \sqrt[6]{a b c}=\sqrt{a}+\sqrt{b}+\sqrt{c}+3 .
\end{aligned}
$$
Answer of Example Problem 3: $$C = 3$$


Problem: Let $a, b > 0$ and $a + b \leq \frac{3}{2}$. Find the smallest constant $C$ such that the following inequality holds for all $a, b$ satisfying the given constraint:
$$
\frac{a}{a^2+1} + \frac{4b}{b^2+4} \leq C.
$$

Solution:

## Response

To solve the problem, we need to analyze the expression 

\[
\frac{a}{a^2+1} + \frac{4b}{b^2+4}
\]

under the constraint \( a + b \leq \frac{3}{2} \) where \( a, b > 0 \).

### Step 1: Analyze the individual terms

1. **For the term \( \frac{a}{a^2 + 1} \)**:
   - We can find the maximum value of this term by differentiating it. Let \( f(a) = \frac{a}{a^2 + 1} \).
   - The derivative is given by:
     \[
     f'(a) = \frac{(a^2 + 1)(1) - a(2a)}{(a^2 + 1)^2} = \frac{1 - a^2}{(a^2 + 1)^2}
     \]
   - Setting \( f'(a) = 0 \) gives \( 1 - a^2 = 0 \) or \( a = 1 \).
   - We check the second derivative or the behavior of \( f'(a) \) to determine if this is a maximum:
     - For \( a < 1 \), \( f'(a) > 0 \) (increasing).
     - For \( a > 1 \), \( f'(a) < 0 \) (decreasing).
   - Thus, \( f(a) \) achieves its maximum at \( a = 1 \):
     \[
     f(1) = \frac{1}{1^2 + 1} = \frac{1}{2}.
     \]

2. **For the term \( \frac{4b}{b^2 + 4} \)**:
   - Let \( g(b) = \frac{4b}{b^2 + 4} \).
   - The derivative is:
     \[
     g'(b) = \frac{(b^2 + 4)(4) - 4b(2b)}{(b^2 + 4)^2} = \frac{4(b^2 + 4 - 2b^2)}{(b^2 + 4)^2} = \frac{4(4 - b^2)}{(b^2 + 4)^2}.
     \]
   - Setting \( g'(b) = 0 \) gives \( 4 - b^2 = 0 \) or \( b = 2 \).
   - However, since \( b \) must be positive and \( a + b \leq \frac{3}{2} \), we need to check values of \( b \) within the constraint.
   - The maximum occurs at \( b = 2 \) but is not feasible under the constraint. We check \( b = 0 \) and \( b = \frac{3}{2} - a \).

### Step 2: Evaluate the maximum under the constraint

Given \( a + b \leq \frac{3}{2} \), we can express \( b \) as \( b = \frac{3}{2} - a \). Thus, we need to evaluate:

\[
\frac{a}{a^2 + 1} + \frac{4\left(\frac{3}{2} - a\right)}{\left(\frac{3}{2} - a\right)^2 + 4}.
\]

### Step 3: Find the maximum value

1. **Evaluate at endpoints**:
   - If \( a = 0 \), then \( b = \frac{3}{2} \):
     \[
     \frac{0}{0^2 + 1} + \frac{4 \cdot \frac{3}{2}}{\left(\frac{3}{2}\right)^2 + 4} = \frac{6}{\frac{9}{4} + 4} = \frac{6}{\frac{25}{4}} = \frac{24}{25}.
     \]
   - If \( a = \frac{3}{2} \), then \( b = 0 \):
     \[
     \frac{\frac{3}{2}}{\left(\frac{3}{2}\right)^2 + 1} + 0 = \frac{\frac{3}{2}}{\frac{9}{4} + 1} = \frac{\frac{3}{2}}{\frac{13}{4}} = \frac{6}{13}.
     \]

2. **Evaluate at \( a = 1 \)**:
   - Then \( b = \frac{1}{2} \):
     \[
     \frac{1}{1^2 + 1} + \frac{4 \cdot \frac{1}{2}}{\left(\frac{1}{2}\right)^2 + 4} = \frac{1}{2} + \frac{2}{\frac{1}{4} + 4} = \frac{1}{2} + \frac{2}{\frac{17}{4}} = \frac{1}{2} + \frac{8}{17} = \frac{17 + 16}{34} = \frac{33}{34}.
     \]

### Conclusion

The maximum value of \( \frac{a}{a^2 + 1} + \frac{4b}{b^2 + 4} \) under the constraint \( a + b \leq \frac{3}{2} \) is \( \frac{33}{34} \).

Thus, the smallest constant \( C \) such that the inequality holds is:

\[
\boxed{C = \frac{33}{34}}.
\]

The answer is \( C = \frac{33}{34} \).