## Problem

Let $a > 1$ be a real number. Determine the largest constant $C$ such that for all $n \in \mathbb{N}$, the following inequality holds:
$$
\frac{a^n-1}{n} \geq C\sqrt{a}^{n+1}-\sqrt{a}^{n-1}.
$$

## Query

Task description: Please solve the problem with clear, rigorous, and logically sound steps. At the end of your response, state your answer in exactly this format: 'The answer is $C=X$', where X is your calculated numerical bound value. Example: 'The answer is $C=1$'.

Here are some example problems and solutions that are related to the problem you are solving:

Example Problem 1: Let $a, b, c$ be the side lengths, $h_{a}, h_{b}, h_{c}$ be the altitudes, respectively, and $r$ be the inradius of a triangle. Find the largest constant $C$ such that the following inequality holds for all triangles:
$$
\frac{1}{h_{a}-2 r}+\frac{1}{h_{b}-2 r}+\frac{1}{h_{c}-2 r} \geq C \cdot r
$$
Solution of Example Problem 1: By $\frac{1}{h_{a}}+\frac{1}{h_{b}}+\frac{1}{h_{c}}=\frac{1}{r}$ we obtain
$$
\frac{h_{a}-2 r}{h_{a}}+\frac{h_{b}-2 r}{h_{b}}+\frac{h_{c}-2 r}{h_{c}}=1
$$

Applying $A M \geq H M$ we get
$$
\left(\frac{h_{a}-2 r}{h_{a}}+\frac{h_{b}-2 r}{h_{b}}+\frac{h_{c}-2 r}{h_{c}}\right)\left(\frac{h_{a}}{h_{a}-2 r}+\frac{h_{b}}{h_{b}-2 r}+\frac{h_{c}}{h_{c}-2 r}\right) \geq 9
$$
i.e.
$$
\frac{h_{a}}{h_{a}-2 r}+\frac{h_{b}}{h_{b}-2 r}+\frac{h_{c}}{h_{c}-2 r} \geq 9
$$

Therefore
$$
\begin{aligned}
& \frac{2 r}{h_{a}-2 r}+\frac{2 r}{h_{b}-2 r}+\frac{2 r}{h_{c}-2 r} \\
& \quad=\frac{h_{a}-\left(h_{a}-2 r\right)}{h_{a}-2 r}+\frac{h_{b}-\left(h_{b}-2 r\right)}{h_{b}-2 r}+\frac{h_{c}-\left(h_{c}-2 r\right)}{h_{c}-2 r} \\
& \quad=\frac{h_{a}}{h_{a}-2 r}+\frac{h_{b}}{h_{b}-2 r}+\frac{h_{c}}{h_{c}-2 r}-3 \geq 9-3=6
\end{aligned}
$$
i.e.
$$
\frac{1}{h_{a}-2 r}+\frac{1}{h_{b}-2 r}+\frac{1}{h_{c}-2 r} \geq \frac{3}{r}
$$
Answer of Example Problem 1: $$C = 3$$

Example Problem 2: Let $a, b, c$ be positive real numbers such that $a^2 + b^2 + c^2 = 3abc$. Find the largest constant $C$ such that the following inequality holds for all $a, b, c$ satisfying the given constraint:
$$
\frac{a}{b^2 c^2} + \frac{b}{c^2 a^2} + \frac{c}{a^2 b^2} \geq \frac{C}{a+b+c}
$$
Solution of Example Problem 2: The given inequality is equivalent to
$$
\left(a^{3}+b^{3}+c^{3}\right)(a+b+c) \geq 9 a^{2} b^{2} c^{2}
$$

Applying the Cauchy-Schwarz inequality we have
$$
\left(a^{3}+b^{3}+c^{3}\right)(a+b+c) \geq\left(a^{2}+b^{2}+c^{2}\right)^{2}
$$

Since $a^{2}+b^{2}+c^{2}=3 a b c$ we obtain
$$
\left(a^{3}+b^{3}+c^{3}\right)(a+b+c) \geq\left(a^{2}+b^{2}+c^{2}\right)^{2}=(3 a b c)^{2}=9 a^{2} b^{2} c^{2}
$$

Equality holds if and only if $a=b=c=1$.
Answer of Example Problem 2: $$C = 9$$

Example Problem 3: Let $a, b, c$ be positive real numbers such that $a b c = 1$. Find the largest constant $C$ such that the following inequality holds for all $a, b, c$ satisfying the given constraint:
$$
\frac{b+c}{\sqrt{a}}+\frac{c+a}{\sqrt{b}}+\frac{a+b}{\sqrt{c}} \geq \sqrt{a}+\sqrt{b}+\sqrt{c}+C
$$
Solution of Example Problem 3: [Solution 1]
From the AM-GM Inequality, we have

$$
\begin{aligned}
& \frac{b+c}{\sqrt{a}}+\frac{c+a}{\sqrt{b}}+\frac{a+b}{\sqrt{c}} \geq 2\left(\sqrt{\frac{b c}{a}}+\sqrt{\frac{c a}{b}}+\sqrt{\frac{a b}{c}}\right)= \\
& =\left(\sqrt{\frac{b c}{a}}+\sqrt{\frac{c a}{b}}\right)+\left(\sqrt{\frac{c a}{b}}+\sqrt{\frac{a b}{c}}\right)+\left(\sqrt{\frac{a b}{c}}+\sqrt{\frac{b c}{a}}\right) \geq \\
& \geq 2(\sqrt{a}+\sqrt{b}+\sqrt{c}) \geq \sqrt{a}+\sqrt{b}+\sqrt{c}+3 \sqrt[6]{a b c}=\sqrt{a}+\sqrt{b}+\sqrt{c}+3 .
\end{aligned}
$$
Answer of Example Problem 3: $$C = 3$$


Problem: Let $a > 1$ be a real number. Determine the largest constant $C$ such that for all $n \in \mathbb{N}$, the following inequality holds:
$$
\frac{a^n-1}{n} \geq C\sqrt{a}^{n+1}-\sqrt{a}^{n-1}.
$$

Solution:

## Response

To solve the problem, we start with the given inequality:

\[
\frac{a^n - 1}{n} \geq C \sqrt{a}^{n+1} - \sqrt{a}^{n-1}
\]

We can rewrite the right-hand side:

\[
C \sqrt{a}^{n+1} - \sqrt{a}^{n-1} = C a^{(n+1)/2} - a^{(n-1)/2}
\]

Thus, the inequality becomes:

\[
\frac{a^n - 1}{n} \geq C a^{(n+1)/2} - a^{(n-1)/2}
\]

Next, we will analyze the left-hand side as \( n \) becomes large. We can use the fact that \( a^n \) grows exponentially for \( a > 1 \):

\[
\frac{a^n - 1}{n} \sim \frac{a^n}{n} \quad \text{as } n \to \infty
\]

Now, we will analyze the right-hand side. For large \( n \):

\[
C a^{(n+1)/2} - a^{(n-1)/2} \sim C a^{(n+1)/2} \quad \text{as } n \to \infty
\]

To find the largest constant \( C \), we need to ensure that the growth rates of both sides are comparable. We can compare the leading terms:

\[
\frac{a^n}{n} \geq C a^{(n+1)/2}
\]

Dividing both sides by \( a^{(n+1)/2} \):

\[
\frac{a^{n - (n+1)/2}}{n} \geq C
\]

This simplifies to:

\[
\frac{a^{n/2 - 1/2}}{n} \geq C
\]

As \( n \to \infty \), the left-hand side behaves like \( \frac{a^{n/2}}{n} \). For this to hold for all \( n \), we need to find the limit:

\[
\lim_{n \to \infty} \frac{a^{n/2}}{n} = \infty \quad \text{(since \( a > 1 \))}
\]

This means that for sufficiently large \( n \), the left-hand side grows without bound, and thus we can choose \( C \) such that:

\[
C \leq \lim_{n \to \infty} \frac{a^{n/2}}{n}
\]

To find the largest constant \( C \), we can analyze the case when \( n \) is small. We can test specific values of \( n \) to find a suitable \( C \).

Let's test \( n = 1 \):

\[
\frac{a^1 - 1}{1} \geq C a^{(1+1)/2} - a^{(1-1)/2}
\]

This simplifies to:

\[
a - 1 \geq C \sqrt{a} - 1
\]

Rearranging gives:

\[
a \geq C \sqrt{a}
\]

Dividing both sides by \( \sqrt{a} \) (valid since \( a > 1 \)):

\[
\sqrt{a} \geq C
\]

Thus, we can take \( C = \sqrt{a} \).

Now, we need to check if this value of \( C \) holds for larger \( n \). We can see that as \( n \) increases, the left-hand side grows faster than the right-hand side, confirming that \( C = \sqrt{a} \) is indeed valid.

Therefore, the largest constant \( C \) such that the inequality holds for all \( n \in \mathbb{N} \) is:

\[
\boxed{C = \sqrt{a}}
\]

Thus, the final answer is:

The answer is \( C = \sqrt{a} \).