## Problem

Let $a, b, c > 0$ such that $a + b + c = abc$. Determine the largest constant $C$ such that the following inequality holds for all $a, b, c$:
$$
\frac{a}{b^3} + \frac{b}{c^3} + \frac{c}{a^3} \geq C.
$$

## Query

Task description: Please solve the problem with clear, rigorous, and logically sound steps. At the end of your response, state your answer in exactly this format: 'The answer is $C=X$', where X is your calculated numerical bound value. Example: 'The answer is $C=1$'.

Here are some example problems and solutions that are related to the problem you are solving:

Example Problem 1: Let $a, b, c$ be the side lengths, $h_{a}, h_{b}, h_{c}$ be the altitudes, respectively, and $r$ be the inradius of a triangle. Find the largest constant $C$ such that the following inequality holds for all triangles:
$$
\frac{1}{h_{a}-2 r}+\frac{1}{h_{b}-2 r}+\frac{1}{h_{c}-2 r} \geq C \cdot r
$$
Solution of Example Problem 1: By $\frac{1}{h_{a}}+\frac{1}{h_{b}}+\frac{1}{h_{c}}=\frac{1}{r}$ we obtain
$$
\frac{h_{a}-2 r}{h_{a}}+\frac{h_{b}-2 r}{h_{b}}+\frac{h_{c}-2 r}{h_{c}}=1
$$

Applying $A M \geq H M$ we get
$$
\left(\frac{h_{a}-2 r}{h_{a}}+\frac{h_{b}-2 r}{h_{b}}+\frac{h_{c}-2 r}{h_{c}}\right)\left(\frac{h_{a}}{h_{a}-2 r}+\frac{h_{b}}{h_{b}-2 r}+\frac{h_{c}}{h_{c}-2 r}\right) \geq 9
$$
i.e.
$$
\frac{h_{a}}{h_{a}-2 r}+\frac{h_{b}}{h_{b}-2 r}+\frac{h_{c}}{h_{c}-2 r} \geq 9
$$

Therefore
$$
\begin{aligned}
& \frac{2 r}{h_{a}-2 r}+\frac{2 r}{h_{b}-2 r}+\frac{2 r}{h_{c}-2 r} \\
& \quad=\frac{h_{a}-\left(h_{a}-2 r\right)}{h_{a}-2 r}+\frac{h_{b}-\left(h_{b}-2 r\right)}{h_{b}-2 r}+\frac{h_{c}-\left(h_{c}-2 r\right)}{h_{c}-2 r} \\
& \quad=\frac{h_{a}}{h_{a}-2 r}+\frac{h_{b}}{h_{b}-2 r}+\frac{h_{c}}{h_{c}-2 r}-3 \geq 9-3=6
\end{aligned}
$$
i.e.
$$
\frac{1}{h_{a}-2 r}+\frac{1}{h_{b}-2 r}+\frac{1}{h_{c}-2 r} \geq \frac{3}{r}
$$
Answer of Example Problem 1: $$C = 3$$

Example Problem 2: Let $a, b, c$ be positive real numbers such that $a^2 + b^2 + c^2 = 3abc$. Find the largest constant $C$ such that the following inequality holds for all $a, b, c$ satisfying the given constraint:
$$
\frac{a}{b^2 c^2} + \frac{b}{c^2 a^2} + \frac{c}{a^2 b^2} \geq \frac{C}{a+b+c}
$$
Solution of Example Problem 2: The given inequality is equivalent to
$$
\left(a^{3}+b^{3}+c^{3}\right)(a+b+c) \geq 9 a^{2} b^{2} c^{2}
$$

Applying the Cauchy-Schwarz inequality we have
$$
\left(a^{3}+b^{3}+c^{3}\right)(a+b+c) \geq\left(a^{2}+b^{2}+c^{2}\right)^{2}
$$

Since $a^{2}+b^{2}+c^{2}=3 a b c$ we obtain
$$
\left(a^{3}+b^{3}+c^{3}\right)(a+b+c) \geq\left(a^{2}+b^{2}+c^{2}\right)^{2}=(3 a b c)^{2}=9 a^{2} b^{2} c^{2}
$$

Equality holds if and only if $a=b=c=1$.
Answer of Example Problem 2: $$C = 9$$

Example Problem 3: Let $a, b, c$ be positive real numbers such that $a b c = 1$. Find the largest constant $C$ such that the following inequality holds for all $a, b, c$ satisfying the given constraint:
$$
\frac{b+c}{\sqrt{a}}+\frac{c+a}{\sqrt{b}}+\frac{a+b}{\sqrt{c}} \geq \sqrt{a}+\sqrt{b}+\sqrt{c}+C
$$
Solution of Example Problem 3: [Solution 1]
From the AM-GM Inequality, we have

$$
\begin{aligned}
& \frac{b+c}{\sqrt{a}}+\frac{c+a}{\sqrt{b}}+\frac{a+b}{\sqrt{c}} \geq 2\left(\sqrt{\frac{b c}{a}}+\sqrt{\frac{c a}{b}}+\sqrt{\frac{a b}{c}}\right)= \\
& =\left(\sqrt{\frac{b c}{a}}+\sqrt{\frac{c a}{b}}\right)+\left(\sqrt{\frac{c a}{b}}+\sqrt{\frac{a b}{c}}\right)+\left(\sqrt{\frac{a b}{c}}+\sqrt{\frac{b c}{a}}\right) \geq \\
& \geq 2(\sqrt{a}+\sqrt{b}+\sqrt{c}) \geq \sqrt{a}+\sqrt{b}+\sqrt{c}+3 \sqrt[6]{a b c}=\sqrt{a}+\sqrt{b}+\sqrt{c}+3 .
\end{aligned}
$$
Answer of Example Problem 3: $$C = 3$$


Problem: Let $a, b, c > 0$ such that $a + b + c = abc$. Determine the largest constant $C$ such that the following inequality holds for all $a, b, c$:
$$
\frac{a}{b^3} + \frac{b}{c^3} + \frac{c}{a^3} \geq C.
$$

Solution:

## Response

To solve the problem, we start with the condition given: \( a + b + c = abc \). We want to find the largest constant \( C \) such that the inequality 

\[
\frac{a}{b^3} + \frac{b}{c^3} + \frac{c}{a^3} \geq C
\]

holds for all positive \( a, b, c \) satisfying the condition.

### Step 1: Analyze the condition

From the condition \( a + b + c = abc \), we can express \( abc \) in terms of \( a, b, c \). This condition suggests a relationship between the variables that we can exploit.

### Step 2: Use substitutions

To simplify our analysis, we can use the substitutions \( a = \frac{x}{y}, b = \frac{y}{z}, c = \frac{z}{x} \) for positive \( x, y, z \). This gives us:

\[
\frac{x}{y} + \frac{y}{z} + \frac{z}{x} = \frac{x}{y} \cdot \frac{y}{z} \cdot \frac{z}{x} = 1
\]

This substitution maintains the symmetry of the problem and allows us to analyze the inequality more easily.

### Step 3: Rewrite the inequality

Substituting \( a, b, c \) into the inequality, we have:

\[
\frac{\frac{x}{y}}{\left(\frac{y}{z}\right)^3} + \frac{\frac{y}{z}}{\left(\frac{z}{x}\right)^3} + \frac{\frac{z}{x}}{\left(\frac{x}{y}\right)^3}
\]

This simplifies to:

\[
\frac{xz^3}{y^3} + \frac{y^3x}{z^3} + \frac{z^3y}{x^3}
\]

### Step 4: Apply AM-GM inequality

Using the AM-GM inequality, we can analyze the terms:

\[
\frac{xz^3}{y^3} + \frac{y^3x}{z^3} + \frac{z^3y}{x^3} \geq 3 \sqrt[3]{\frac{xz^3}{y^3} \cdot \frac{y^3x}{z^3} \cdot \frac{z^3y}{x^3}} = 3
\]

### Step 5: Conclusion

Thus, we find that:

\[
\frac{a}{b^3} + \frac{b}{c^3} + \frac{c}{a^3} \geq 3
\]

This shows that the largest constant \( C \) such that the inequality holds for all positive \( a, b, c \) satisfying \( a + b + c = abc \) is \( C = 3 \).

Therefore, the final answer is:

The answer is \( C=3 \).