## Problem

Let $a, b, c \geq 0$ and $a+b+c=3$. Determine the largest constant $C$ such that the following inequality holds for all $a, b, c$:

$$
\frac{a+1}{a+b+1}+\frac{b+1}{b+c+1}+\frac{c+1}{c+a+1} \geq C.
$$

## Query

Task description: Please solve the problem with clear, rigorous, and logically sound steps. At the end of your response, state your answer in exactly this format: 'The answer is $C=X$', where X is your calculated numerical bound value. Example: 'The answer is $C=1$'.

Here are some example problems and solutions that are related to the problem you are solving:

Example Problem 1: Let $a, b, c$ be the side lengths, $h_{a}, h_{b}, h_{c}$ be the altitudes, respectively, and $r$ be the inradius of a triangle. Find the largest constant $C$ such that the following inequality holds for all triangles:
$$
\frac{1}{h_{a}-2 r}+\frac{1}{h_{b}-2 r}+\frac{1}{h_{c}-2 r} \geq C \cdot r
$$
Solution of Example Problem 1: By $\frac{1}{h_{a}}+\frac{1}{h_{b}}+\frac{1}{h_{c}}=\frac{1}{r}$ we obtain
$$
\frac{h_{a}-2 r}{h_{a}}+\frac{h_{b}-2 r}{h_{b}}+\frac{h_{c}-2 r}{h_{c}}=1
$$

Applying $A M \geq H M$ we get
$$
\left(\frac{h_{a}-2 r}{h_{a}}+\frac{h_{b}-2 r}{h_{b}}+\frac{h_{c}-2 r}{h_{c}}\right)\left(\frac{h_{a}}{h_{a}-2 r}+\frac{h_{b}}{h_{b}-2 r}+\frac{h_{c}}{h_{c}-2 r}\right) \geq 9
$$
i.e.
$$
\frac{h_{a}}{h_{a}-2 r}+\frac{h_{b}}{h_{b}-2 r}+\frac{h_{c}}{h_{c}-2 r} \geq 9
$$

Therefore
$$
\begin{aligned}
& \frac{2 r}{h_{a}-2 r}+\frac{2 r}{h_{b}-2 r}+\frac{2 r}{h_{c}-2 r} \\
& \quad=\frac{h_{a}-\left(h_{a}-2 r\right)}{h_{a}-2 r}+\frac{h_{b}-\left(h_{b}-2 r\right)}{h_{b}-2 r}+\frac{h_{c}-\left(h_{c}-2 r\right)}{h_{c}-2 r} \\
& \quad=\frac{h_{a}}{h_{a}-2 r}+\frac{h_{b}}{h_{b}-2 r}+\frac{h_{c}}{h_{c}-2 r}-3 \geq 9-3=6
\end{aligned}
$$
i.e.
$$
\frac{1}{h_{a}-2 r}+\frac{1}{h_{b}-2 r}+\frac{1}{h_{c}-2 r} \geq \frac{3}{r}
$$
Answer of Example Problem 1: $$C = 3$$

Example Problem 2: Let $a, b, c$ be positive real numbers such that $a^2 + b^2 + c^2 = 3abc$. Find the largest constant $C$ such that the following inequality holds for all $a, b, c$ satisfying the given constraint:
$$
\frac{a}{b^2 c^2} + \frac{b}{c^2 a^2} + \frac{c}{a^2 b^2} \geq \frac{C}{a+b+c}
$$
Solution of Example Problem 2: The given inequality is equivalent to
$$
\left(a^{3}+b^{3}+c^{3}\right)(a+b+c) \geq 9 a^{2} b^{2} c^{2}
$$

Applying the Cauchy-Schwarz inequality we have
$$
\left(a^{3}+b^{3}+c^{3}\right)(a+b+c) \geq\left(a^{2}+b^{2}+c^{2}\right)^{2}
$$

Since $a^{2}+b^{2}+c^{2}=3 a b c$ we obtain
$$
\left(a^{3}+b^{3}+c^{3}\right)(a+b+c) \geq\left(a^{2}+b^{2}+c^{2}\right)^{2}=(3 a b c)^{2}=9 a^{2} b^{2} c^{2}
$$

Equality holds if and only if $a=b=c=1$.
Answer of Example Problem 2: $$C = 9$$

Example Problem 3: Let $a, b, c$ be positive real numbers such that $a b c = 1$. Find the largest constant $C$ such that the following inequality holds for all $a, b, c$ satisfying the given constraint:
$$
\frac{b+c}{\sqrt{a}}+\frac{c+a}{\sqrt{b}}+\frac{a+b}{\sqrt{c}} \geq \sqrt{a}+\sqrt{b}+\sqrt{c}+C
$$
Solution of Example Problem 3: [Solution 1]
From the AM-GM Inequality, we have

$$
\begin{aligned}
& \frac{b+c}{\sqrt{a}}+\frac{c+a}{\sqrt{b}}+\frac{a+b}{\sqrt{c}} \geq 2\left(\sqrt{\frac{b c}{a}}+\sqrt{\frac{c a}{b}}+\sqrt{\frac{a b}{c}}\right)= \\
& =\left(\sqrt{\frac{b c}{a}}+\sqrt{\frac{c a}{b}}\right)+\left(\sqrt{\frac{c a}{b}}+\sqrt{\frac{a b}{c}}\right)+\left(\sqrt{\frac{a b}{c}}+\sqrt{\frac{b c}{a}}\right) \geq \\
& \geq 2(\sqrt{a}+\sqrt{b}+\sqrt{c}) \geq \sqrt{a}+\sqrt{b}+\sqrt{c}+3 \sqrt[6]{a b c}=\sqrt{a}+\sqrt{b}+\sqrt{c}+3 .
\end{aligned}
$$
Answer of Example Problem 3: $$C = 3$$


Problem: Let $a, b, c \geq 0$ and $a+b+c=3$. Determine the largest constant $C$ such that the following inequality holds for all $a, b, c$:

$$
\frac{a+1}{a+b+1}+\frac{b+1}{b+c+1}+\frac{c+1}{c+a+1} \geq C.
$$

Solution:

## Response

To solve the problem, we need to analyze the inequality 

\[
\frac{a+1}{a+b+1}+\frac{b+1}{b+c+1}+\frac{c+1}{c+a+1} \geq C
\]

given the constraint \( a + b + c = 3 \) where \( a, b, c \geq 0 \).

### Step 1: Simplifying the Expression

We can rewrite each term in the sum:

\[
\frac{a+1}{a+b+1} = 1 - \frac{b}{a+b+1}
\]

Thus, we can express the entire sum as:

\[
\frac{a+1}{a+b+1} + \frac{b+1}{b+c+1} + \frac{c+1}{c+a+1} = 3 - \left( \frac{b}{a+b+1} + \frac{c}{b+c+1} + \frac{a}{c+a+1} \right)
\]

### Step 2: Finding a Lower Bound

To find a lower bound for the sum, we need to analyze the term 

\[
\frac{b}{a+b+1} + \frac{c}{b+c+1} + \frac{a}{c+a+1}
\]

We will use the Cauchy-Schwarz inequality:

\[
\left( \frac{b}{a+b+1} + \frac{c}{b+c+1} + \frac{a}{c+a+1} \right) \left( (a+b+1) + (b+c+1) + (c+a+1) \right) \geq (a+b+c)^2
\]

Calculating the second factor:

\[
(a+b+1) + (b+c+1) + (c+a+1) = 2(a+b+c) + 3 = 2 \cdot 3 + 3 = 9
\]

Thus, we have:

\[
\left( \frac{b}{a+b+1} + \frac{c}{b+c+1} + \frac{a}{c+a+1} \right) \cdot 9 \geq 9
\]

This implies:

\[
\frac{b}{a+b+1} + \frac{c}{b+c+1} + \frac{a}{c+a+1} \geq 1
\]

### Step 3: Putting It All Together

Substituting this back into our expression, we get:

\[
\frac{a+1}{a+b+1} + \frac{b+1}{b+c+1} + \frac{c+1}{c+a+1} \geq 3 - 1 = 2
\]

### Step 4: Conclusion

Thus, we have shown that:

\[
\frac{a+1}{a+b+1} + \frac{b+1}{b+c+1} + \frac{c+1}{c+a+1} \geq 2
\]

for all non-negative \( a, b, c \) such that \( a + b + c = 3 \). Therefore, the largest constant \( C \) such that the inequality holds is:

\[
\boxed{2}
\]

Thus, the final answer is:

The answer is \( C=2 \).