## Problem

Given $k > 1$ and $a, b, c > 0$ with $abc = k^3$, find the largest constant $C$ such that the following inequality holds for all $a, b, c$:

$$
\sum_{\text{cyc}}\left(\frac{1}{1+a}+\frac{1}{1+bc}\right) \geq C\left(\frac{1}{1+k}+\frac{1}{1+k^2}\right).
$$

## Query

Task description: Please solve the problem with clear, rigorous, and logically sound steps. At the end of your response, state your answer in exactly this format: 'The answer is $C=X$', where X is your calculated numerical bound value. Example: 'The answer is $C=1$'.

Here are some example problems and solutions that are related to the problem you are solving:

Example Problem 1: Let $a, b, c$ be the side lengths, $h_{a}, h_{b}, h_{c}$ be the altitudes, respectively, and $r$ be the inradius of a triangle. Find the largest constant $C$ such that the following inequality holds for all triangles:
$$
\frac{1}{h_{a}-2 r}+\frac{1}{h_{b}-2 r}+\frac{1}{h_{c}-2 r} \geq C \cdot r
$$
Solution of Example Problem 1: By $\frac{1}{h_{a}}+\frac{1}{h_{b}}+\frac{1}{h_{c}}=\frac{1}{r}$ we obtain
$$
\frac{h_{a}-2 r}{h_{a}}+\frac{h_{b}-2 r}{h_{b}}+\frac{h_{c}-2 r}{h_{c}}=1
$$

Applying $A M \geq H M$ we get
$$
\left(\frac{h_{a}-2 r}{h_{a}}+\frac{h_{b}-2 r}{h_{b}}+\frac{h_{c}-2 r}{h_{c}}\right)\left(\frac{h_{a}}{h_{a}-2 r}+\frac{h_{b}}{h_{b}-2 r}+\frac{h_{c}}{h_{c}-2 r}\right) \geq 9
$$
i.e.
$$
\frac{h_{a}}{h_{a}-2 r}+\frac{h_{b}}{h_{b}-2 r}+\frac{h_{c}}{h_{c}-2 r} \geq 9
$$

Therefore
$$
\begin{aligned}
& \frac{2 r}{h_{a}-2 r}+\frac{2 r}{h_{b}-2 r}+\frac{2 r}{h_{c}-2 r} \\
& \quad=\frac{h_{a}-\left(h_{a}-2 r\right)}{h_{a}-2 r}+\frac{h_{b}-\left(h_{b}-2 r\right)}{h_{b}-2 r}+\frac{h_{c}-\left(h_{c}-2 r\right)}{h_{c}-2 r} \\
& \quad=\frac{h_{a}}{h_{a}-2 r}+\frac{h_{b}}{h_{b}-2 r}+\frac{h_{c}}{h_{c}-2 r}-3 \geq 9-3=6
\end{aligned}
$$
i.e.
$$
\frac{1}{h_{a}-2 r}+\frac{1}{h_{b}-2 r}+\frac{1}{h_{c}-2 r} \geq \frac{3}{r}
$$
Answer of Example Problem 1: $$C = 3$$

Example Problem 2: Let $a, b, c$ be positive real numbers such that $a^2 + b^2 + c^2 = 3abc$. Find the largest constant $C$ such that the following inequality holds for all $a, b, c$ satisfying the given constraint:
$$
\frac{a}{b^2 c^2} + \frac{b}{c^2 a^2} + \frac{c}{a^2 b^2} \geq \frac{C}{a+b+c}
$$
Solution of Example Problem 2: The given inequality is equivalent to
$$
\left(a^{3}+b^{3}+c^{3}\right)(a+b+c) \geq 9 a^{2} b^{2} c^{2}
$$

Applying the Cauchy-Schwarz inequality we have
$$
\left(a^{3}+b^{3}+c^{3}\right)(a+b+c) \geq\left(a^{2}+b^{2}+c^{2}\right)^{2}
$$

Since $a^{2}+b^{2}+c^{2}=3 a b c$ we obtain
$$
\left(a^{3}+b^{3}+c^{3}\right)(a+b+c) \geq\left(a^{2}+b^{2}+c^{2}\right)^{2}=(3 a b c)^{2}=9 a^{2} b^{2} c^{2}
$$

Equality holds if and only if $a=b=c=1$.
Answer of Example Problem 2: $$C = 9$$

Example Problem 3: Let $a, b, c$ be positive real numbers such that $a b c = 1$. Find the largest constant $C$ such that the following inequality holds for all $a, b, c$ satisfying the given constraint:
$$
\frac{b+c}{\sqrt{a}}+\frac{c+a}{\sqrt{b}}+\frac{a+b}{\sqrt{c}} \geq \sqrt{a}+\sqrt{b}+\sqrt{c}+C
$$
Solution of Example Problem 3: [Solution 1]
From the AM-GM Inequality, we have

$$
\begin{aligned}
& \frac{b+c}{\sqrt{a}}+\frac{c+a}{\sqrt{b}}+\frac{a+b}{\sqrt{c}} \geq 2\left(\sqrt{\frac{b c}{a}}+\sqrt{\frac{c a}{b}}+\sqrt{\frac{a b}{c}}\right)= \\
& =\left(\sqrt{\frac{b c}{a}}+\sqrt{\frac{c a}{b}}\right)+\left(\sqrt{\frac{c a}{b}}+\sqrt{\frac{a b}{c}}\right)+\left(\sqrt{\frac{a b}{c}}+\sqrt{\frac{b c}{a}}\right) \geq \\
& \geq 2(\sqrt{a}+\sqrt{b}+\sqrt{c}) \geq \sqrt{a}+\sqrt{b}+\sqrt{c}+3 \sqrt[6]{a b c}=\sqrt{a}+\sqrt{b}+\sqrt{c}+3 .
\end{aligned}
$$
Answer of Example Problem 3: $$C = 3$$


Problem: Given $k > 1$ and $a, b, c > 0$ with $abc = k^3$, find the largest constant $C$ such that the following inequality holds for all $a, b, c$:

$$
\sum_{\text{cyc}}\left(\frac{1}{1+a}+\frac{1}{1+bc}\right) \geq C\left(\frac{1}{1+k}+\frac{1}{1+k^2}\right).
$$

Solution:

## Response

To solve the problem, we start with the given inequality:

\[
\sum_{\text{cyc}}\left(\frac{1}{1+a}+\frac{1}{1+bc}\right) \geq C\left(\frac{1}{1+k}+\frac{1}{1+k^2}\right).
\]

We will analyze the left-hand side of the inequality. The cyclic sum can be expanded as follows:

\[
\sum_{\text{cyc}} \frac{1}{1+a} + \sum_{\text{cyc}} \frac{1}{1+bc}.
\]

### Step 1: Analyze \(\sum_{\text{cyc}} \frac{1}{1+a}\)

Using the fact that \(abc = k^3\), we can apply the AM-HM inequality:

\[
\frac{1}{3} \left( \frac{1}{1+a} + \frac{1}{1+b} + \frac{1}{1+c} \right) \leq \frac{3}{3 + a + b + c}.
\]

### Step 2: Analyze \(\sum_{\text{cyc}} \frac{1}{1+bc}\)

For the second part, we can also apply the AM-HM inequality:

\[
\frac{1}{3} \left( \frac{1}{1+bc} + \frac{1}{1+ca} + \frac{1}{1+ab} \right) \leq \frac{3}{3 + bc + ca + ab}.
\]

### Step 3: Combine the results

Now we combine both parts:

\[
\sum_{\text{cyc}} \frac{1}{1+a} + \sum_{\text{cyc}} \frac{1}{1+bc} \geq \frac{3}{3 + a + b + c} + \frac{3}{3 + bc + ca + ab}.
\]

### Step 4: Find bounds for \(C\)

Next, we need to find a suitable \(C\) such that:

\[
\frac{3}{3 + a + b + c} + \frac{3}{3 + bc + ca + ab} \geq C\left(\frac{1}{1+k}+\frac{1}{1+k^2}\right).
\]

To find \(C\), we can test specific values of \(a, b, c\) that satisfy \(abc = k^3\). A natural choice is to set \(a = b = c = k\):

\[
\sum_{\text{cyc}} \frac{1}{1+k} + \sum_{\text{cyc}} \frac{1}{1+k^2} = 3\left(\frac{1}{1+k} + \frac{1}{1+k^2}\right).
\]

### Step 5: Evaluate the inequality

Substituting \(a = b = c = k\) into the inequality gives:

\[
3\left(\frac{1}{1+k} + \frac{1}{1+k^2}\right) \geq C\left(\frac{1}{1+k}+\frac{1}{1+k^2}\right).
\]

This simplifies to:

\[
3 \geq C.
\]

Thus, the largest constant \(C\) that satisfies the inequality for all \(a, b, c > 0\) with \(abc = k^3\) is:

\[
C = 3.
\]

### Conclusion

Therefore, the final answer is:

The answer is \(C=3\).