## Problem

Let $a, b, c \geq 0$ and $a^2 + b + c^2 = 1$. Determine the largest constant $C$ such that the following inequality holds for all $a, b, c$:

$$
\frac{1}{1+a^2} + \frac{1}{3(1+b)} + \frac{1}{1+c^2} \geq C.
$$

## Query

Task description: Please solve the problem with clear, rigorous, and logically sound steps. At the end of your response, state your answer in exactly this format: 'The answer is $C=X$', where X is your calculated numerical bound value. Example: 'The answer is $C=1$'.

Here are some example problems and solutions that are related to the problem you are solving:

Example Problem 1: Let $a, b, c$ be the side lengths, $h_{a}, h_{b}, h_{c}$ be the altitudes, respectively, and $r$ be the inradius of a triangle. Find the largest constant $C$ such that the following inequality holds for all triangles:
$$
\frac{1}{h_{a}-2 r}+\frac{1}{h_{b}-2 r}+\frac{1}{h_{c}-2 r} \geq C \cdot r
$$
Solution of Example Problem 1: By $\frac{1}{h_{a}}+\frac{1}{h_{b}}+\frac{1}{h_{c}}=\frac{1}{r}$ we obtain
$$
\frac{h_{a}-2 r}{h_{a}}+\frac{h_{b}-2 r}{h_{b}}+\frac{h_{c}-2 r}{h_{c}}=1
$$

Applying $A M \geq H M$ we get
$$
\left(\frac{h_{a}-2 r}{h_{a}}+\frac{h_{b}-2 r}{h_{b}}+\frac{h_{c}-2 r}{h_{c}}\right)\left(\frac{h_{a}}{h_{a}-2 r}+\frac{h_{b}}{h_{b}-2 r}+\frac{h_{c}}{h_{c}-2 r}\right) \geq 9
$$
i.e.
$$
\frac{h_{a}}{h_{a}-2 r}+\frac{h_{b}}{h_{b}-2 r}+\frac{h_{c}}{h_{c}-2 r} \geq 9
$$

Therefore
$$
\begin{aligned}
& \frac{2 r}{h_{a}-2 r}+\frac{2 r}{h_{b}-2 r}+\frac{2 r}{h_{c}-2 r} \\
& \quad=\frac{h_{a}-\left(h_{a}-2 r\right)}{h_{a}-2 r}+\frac{h_{b}-\left(h_{b}-2 r\right)}{h_{b}-2 r}+\frac{h_{c}-\left(h_{c}-2 r\right)}{h_{c}-2 r} \\
& \quad=\frac{h_{a}}{h_{a}-2 r}+\frac{h_{b}}{h_{b}-2 r}+\frac{h_{c}}{h_{c}-2 r}-3 \geq 9-3=6
\end{aligned}
$$
i.e.
$$
\frac{1}{h_{a}-2 r}+\frac{1}{h_{b}-2 r}+\frac{1}{h_{c}-2 r} \geq \frac{3}{r}
$$
Answer of Example Problem 1: $$C = 3$$

Example Problem 2: Let $a, b, c$ be positive real numbers such that $a^2 + b^2 + c^2 = 3abc$. Find the largest constant $C$ such that the following inequality holds for all $a, b, c$ satisfying the given constraint:
$$
\frac{a}{b^2 c^2} + \frac{b}{c^2 a^2} + \frac{c}{a^2 b^2} \geq \frac{C}{a+b+c}
$$
Solution of Example Problem 2: The given inequality is equivalent to
$$
\left(a^{3}+b^{3}+c^{3}\right)(a+b+c) \geq 9 a^{2} b^{2} c^{2}
$$

Applying the Cauchy-Schwarz inequality we have
$$
\left(a^{3}+b^{3}+c^{3}\right)(a+b+c) \geq\left(a^{2}+b^{2}+c^{2}\right)^{2}
$$

Since $a^{2}+b^{2}+c^{2}=3 a b c$ we obtain
$$
\left(a^{3}+b^{3}+c^{3}\right)(a+b+c) \geq\left(a^{2}+b^{2}+c^{2}\right)^{2}=(3 a b c)^{2}=9 a^{2} b^{2} c^{2}
$$

Equality holds if and only if $a=b=c=1$.
Answer of Example Problem 2: $$C = 9$$

Example Problem 3: Let $a, b, c$ be positive real numbers such that $a b c = 1$. Find the largest constant $C$ such that the following inequality holds for all $a, b, c$ satisfying the given constraint:
$$
\frac{b+c}{\sqrt{a}}+\frac{c+a}{\sqrt{b}}+\frac{a+b}{\sqrt{c}} \geq \sqrt{a}+\sqrt{b}+\sqrt{c}+C
$$
Solution of Example Problem 3: [Solution 1]
From the AM-GM Inequality, we have

$$
\begin{aligned}
& \frac{b+c}{\sqrt{a}}+\frac{c+a}{\sqrt{b}}+\frac{a+b}{\sqrt{c}} \geq 2\left(\sqrt{\frac{b c}{a}}+\sqrt{\frac{c a}{b}}+\sqrt{\frac{a b}{c}}\right)= \\
& =\left(\sqrt{\frac{b c}{a}}+\sqrt{\frac{c a}{b}}\right)+\left(\sqrt{\frac{c a}{b}}+\sqrt{\frac{a b}{c}}\right)+\left(\sqrt{\frac{a b}{c}}+\sqrt{\frac{b c}{a}}\right) \geq \\
& \geq 2(\sqrt{a}+\sqrt{b}+\sqrt{c}) \geq \sqrt{a}+\sqrt{b}+\sqrt{c}+3 \sqrt[6]{a b c}=\sqrt{a}+\sqrt{b}+\sqrt{c}+3 .
\end{aligned}
$$
Answer of Example Problem 3: $$C = 3$$


Problem: Let $a, b, c \geq 0$ and $a^2 + b + c^2 = 1$. Determine the largest constant $C$ such that the following inequality holds for all $a, b, c$:

$$
\frac{1}{1+a^2} + \frac{1}{3(1+b)} + \frac{1}{1+c^2} \geq C.
$$

Solution:

## Response

To solve the problem, we need to analyze the inequality 

\[
\frac{1}{1+a^2} + \frac{1}{3(1+b)} + \frac{1}{1+c^2} \geq C
\]

given the constraint \( a^2 + b + c^2 = 1 \) with \( a, b, c \geq 0 \).

### Step 1: Analyze the terms

We will analyze each term in the inequality separately. 

1. **For \( \frac{1}{1+a^2} \)**:
   - The maximum value occurs when \( a^2 \) is minimized. Since \( a^2 \geq 0 \), the minimum value of \( a^2 \) is 0, giving us \( \frac{1}{1+0} = 1 \).

2. **For \( \frac{1}{3(1+b)} \)**:
   - The term \( 1+b \) is minimized when \( b \) is minimized. Since \( b \geq 0 \), the minimum value of \( b \) is 0, giving us \( \frac{1}{3(1+0)} = \frac{1}{3} \).

3. **For \( \frac{1}{1+c^2} \)**:
   - Similar to the first term, the maximum value occurs when \( c^2 \) is minimized. The minimum value of \( c^2 \) is 0, giving us \( \frac{1}{1+0} = 1 \).

### Step 2: Combine the maximum values

Now, we can combine the maximum values of each term:

\[
\frac{1}{1+a^2} + \frac{1}{3(1+b)} + \frac{1}{1+c^2} \leq 1 + \frac{1}{3} + 1 = 2 + \frac{1}{3} = \frac{6}{3} + \frac{1}{3} = \frac{7}{3}
\]

### Step 3: Check if the maximum can be achieved

To check if we can achieve this maximum, we need to find values of \( a, b, c \) such that:

- \( a^2 + b + c^2 = 1 \)
- \( a = 0 \), \( b = 0 \), \( c = 1 \) gives \( 0^2 + 0 + 1^2 = 1 \), which satisfies the constraint.

Calculating the left-hand side:

\[
\frac{1}{1+0^2} + \frac{1}{3(1+0)} + \frac{1}{1+1^2} = 1 + \frac{1}{3} + \frac{1}{2}
\]

Finding a common denominator (which is 6):

\[
1 = \frac{6}{6}, \quad \frac{1}{3} = \frac{2}{6}, \quad \frac{1}{2} = \frac{3}{6}
\]

Thus,

\[
\frac{6}{6} + \frac{2}{6} + \frac{3}{6} = \frac{11}{6}
\]

### Step 4: Find the largest constant \( C \)

Now we need to find the largest constant \( C \) such that:

\[
\frac{11}{6} \geq C
\]

This implies that the largest constant \( C \) is:

\[
C = \frac{11}{6}
\]

### Conclusion

Thus, the largest constant \( C \) such that the inequality holds for all \( a, b, c \) satisfying the given constraint is:

\[
\text{The answer is } C = \frac{11}{6}
\]