## Problem

Let $a, b, c > 0$ such that $a+b+c=2$ and $a^2+b^2+c^2=2$. Determine the minimal constant $C$ such that the following inequality holds for all $a, b, c$ satisfying the given constraints:
$$
a b c \leq C.
$$

## Query

Task description: Please solve the problem with clear, rigorous, and logically sound steps. At the end of your response, state your answer in exactly this format: 'The answer is $C=X$', where X is your calculated numerical bound value. Example: 'The answer is $C=1$'.

Here are some example problems and solutions that are related to the problem you are solving:

Example Problem 1: Let $a, b, c$ be the side lengths, $h_{a}, h_{b}, h_{c}$ be the altitudes, respectively, and $r$ be the inradius of a triangle. Find the largest constant $C$ such that the following inequality holds for all triangles:
$$
\frac{1}{h_{a}-2 r}+\frac{1}{h_{b}-2 r}+\frac{1}{h_{c}-2 r} \geq C \cdot r
$$
Solution of Example Problem 1: By $\frac{1}{h_{a}}+\frac{1}{h_{b}}+\frac{1}{h_{c}}=\frac{1}{r}$ we obtain
$$
\frac{h_{a}-2 r}{h_{a}}+\frac{h_{b}-2 r}{h_{b}}+\frac{h_{c}-2 r}{h_{c}}=1
$$

Applying $A M \geq H M$ we get
$$
\left(\frac{h_{a}-2 r}{h_{a}}+\frac{h_{b}-2 r}{h_{b}}+\frac{h_{c}-2 r}{h_{c}}\right)\left(\frac{h_{a}}{h_{a}-2 r}+\frac{h_{b}}{h_{b}-2 r}+\frac{h_{c}}{h_{c}-2 r}\right) \geq 9
$$
i.e.
$$
\frac{h_{a}}{h_{a}-2 r}+\frac{h_{b}}{h_{b}-2 r}+\frac{h_{c}}{h_{c}-2 r} \geq 9
$$

Therefore
$$
\begin{aligned}
& \frac{2 r}{h_{a}-2 r}+\frac{2 r}{h_{b}-2 r}+\frac{2 r}{h_{c}-2 r} \\
& \quad=\frac{h_{a}-\left(h_{a}-2 r\right)}{h_{a}-2 r}+\frac{h_{b}-\left(h_{b}-2 r\right)}{h_{b}-2 r}+\frac{h_{c}-\left(h_{c}-2 r\right)}{h_{c}-2 r} \\
& \quad=\frac{h_{a}}{h_{a}-2 r}+\frac{h_{b}}{h_{b}-2 r}+\frac{h_{c}}{h_{c}-2 r}-3 \geq 9-3=6
\end{aligned}
$$
i.e.
$$
\frac{1}{h_{a}-2 r}+\frac{1}{h_{b}-2 r}+\frac{1}{h_{c}-2 r} \geq \frac{3}{r}
$$
Answer of Example Problem 1: $$C = 3$$

Example Problem 2: Let $a, b, c$ be positive real numbers such that $a^2 + b^2 + c^2 = 3abc$. Find the largest constant $C$ such that the following inequality holds for all $a, b, c$ satisfying the given constraint:
$$
\frac{a}{b^2 c^2} + \frac{b}{c^2 a^2} + \frac{c}{a^2 b^2} \geq \frac{C}{a+b+c}
$$
Solution of Example Problem 2: The given inequality is equivalent to
$$
\left(a^{3}+b^{3}+c^{3}\right)(a+b+c) \geq 9 a^{2} b^{2} c^{2}
$$

Applying the Cauchy-Schwarz inequality we have
$$
\left(a^{3}+b^{3}+c^{3}\right)(a+b+c) \geq\left(a^{2}+b^{2}+c^{2}\right)^{2}
$$

Since $a^{2}+b^{2}+c^{2}=3 a b c$ we obtain
$$
\left(a^{3}+b^{3}+c^{3}\right)(a+b+c) \geq\left(a^{2}+b^{2}+c^{2}\right)^{2}=(3 a b c)^{2}=9 a^{2} b^{2} c^{2}
$$

Equality holds if and only if $a=b=c=1$.
Answer of Example Problem 2: $$C = 9$$

Example Problem 3: Let $a, b, c$ be positive real numbers such that $a b c = 1$. Find the largest constant $C$ such that the following inequality holds for all $a, b, c$ satisfying the given constraint:
$$
\frac{b+c}{\sqrt{a}}+\frac{c+a}{\sqrt{b}}+\frac{a+b}{\sqrt{c}} \geq \sqrt{a}+\sqrt{b}+\sqrt{c}+C
$$
Solution of Example Problem 3: [Solution 1]
From the AM-GM Inequality, we have

$$
\begin{aligned}
& \frac{b+c}{\sqrt{a}}+\frac{c+a}{\sqrt{b}}+\frac{a+b}{\sqrt{c}} \geq 2\left(\sqrt{\frac{b c}{a}}+\sqrt{\frac{c a}{b}}+\sqrt{\frac{a b}{c}}\right)= \\
& =\left(\sqrt{\frac{b c}{a}}+\sqrt{\frac{c a}{b}}\right)+\left(\sqrt{\frac{c a}{b}}+\sqrt{\frac{a b}{c}}\right)+\left(\sqrt{\frac{a b}{c}}+\sqrt{\frac{b c}{a}}\right) \geq \\
& \geq 2(\sqrt{a}+\sqrt{b}+\sqrt{c}) \geq \sqrt{a}+\sqrt{b}+\sqrt{c}+3 \sqrt[6]{a b c}=\sqrt{a}+\sqrt{b}+\sqrt{c}+3 .
\end{aligned}
$$
Answer of Example Problem 3: $$C = 3$$


Problem: Let $a, b, c > 0$ such that $a+b+c=2$ and $a^2+b^2+c^2=2$. Determine the minimal constant $C$ such that the following inequality holds for all $a, b, c$ satisfying the given constraints:
$$
a b c \leq C.
$$

Solution:

## Response

To solve the problem, we start with the given conditions:

1. \( a + b + c = 2 \)
2. \( a^2 + b^2 + c^2 = 2 \)

From the first condition, we can express \( c \) in terms of \( a \) and \( b \):
\[
c = 2 - a - b.
\]

Next, we substitute \( c \) into the second condition:
\[
a^2 + b^2 + (2 - a - b)^2 = 2.
\]
Expanding the square:
\[
a^2 + b^2 + (4 - 4a - 4b + a^2 + 2ab + b^2) = 2.
\]
Combining like terms gives:
\[
2a^2 + 2b^2 + 2ab - 4a - 4b + 4 = 2.
\]
Simplifying this, we have:
\[
2a^2 + 2b^2 + 2ab - 4a - 4b + 2 = 0.
\]
Dividing the entire equation by 2:
\[
a^2 + b^2 + ab - 2a - 2b + 1 = 0.
\]

Now, we can rearrange this equation:
\[
a^2 + b^2 + ab - 2a - 2b + 1 = 0.
\]

Next, we will analyze the expression \( abc \). We can express \( abc \) in terms of \( a \) and \( b \):
\[
abc = ab(2 - a - b).
\]

To find the maximum value of \( abc \), we can use the method of Lagrange multipliers or analyze the critical points directly. However, we can also use the symmetry of the problem and the constraints to find the maximum.

Given the constraints, we can assume \( a, b, c \) are equal for maximum product due to the symmetry of the problem. Let \( a = b = c \). Then:
\[
3a = 2 \implies a = \frac{2}{3}.
\]
Substituting back to find \( abc \):
\[
abc = \left(\frac{2}{3}\right)^3 = \frac{8}{27}.
\]

Now we need to check if this is indeed the maximum. We can also check the case when two variables are equal and one is different. Let \( a = b \) and \( c = 2 - 2a \). Then:
\[
2a^2 + (2 - 2a)^2 = 2 \implies 2a^2 + 4 - 8a + 4a^2 = 2 \implies 6a^2 - 8a + 2 = 0.
\]
Solving this quadratic equation:
\[
3a^2 - 4a + 1 = 0.
\]
Using the quadratic formula:
\[
a = \frac{4 \pm \sqrt{(-4)^2 - 4 \cdot 3 \cdot 1}}{2 \cdot 3} = \frac{4 \pm \sqrt{16 - 12}}{6} = \frac{4 \pm 2}{6}.
\]
Thus, we have:
\[
a = 1 \quad \text{or} \quad a = \frac{1}{3}.
\]
For \( a = 1 \), \( b = 1 \), \( c = 0 \) gives \( abc = 0 \).

For \( a = \frac{1}{3} \), \( b = \frac{1}{3} \), \( c = \frac{4}{3} \):
\[
abc = \frac{1}{3} \cdot \frac{1}{3} \cdot \frac{4}{3} = \frac{4}{27}.
\]

Comparing all cases, the maximum value of \( abc \) occurs when \( a = b = c = \frac{2}{3} \):
\[
abc = \frac{8}{27}.
\]

Thus, the minimal constant \( C \) such that \( abc \leq C \) for all \( a, b, c \) satisfying the given constraints is:
\[
C = \frac{8}{27}.
\]

Therefore, the final answer is:
\[
\text{The answer is } C = \frac{8}{27}.
\]