## Problem

Let $a_1, a_2, \ldots, a_n$ be real numbers such that $a_1 + a_2 + \ldots + a_n = 0$ and $\max \{|a_i - a_j| \mid 1 \leq i, j \leq n\} \leq 1$. Consider the following expression:
$$
a_1^2 + a_2^2 + \ldots + a_n^2 \quad () \quad \frac{1}{n}\left[\frac{n}{2}\right]\left[\frac{n+1}{2}\right] 
$$

Determine the correct inequality relation to fill in the blank.

Options:

(A) $\leq$ 

(B) $\geq$

(C) $=$ 

(D) $<$

(E) $>$

(F) None of the above

## Query

Task description: Please solve the problem with clear, rigorous, and logically sound steps. At the end of your response, state your answer in exactly this format: 'The answer is (Letter) Symbol', where Letter is one of the given options. Example: 'The answer is (A) $\leq$'.

Here are some example problems and solutions that are related to the problem you are solving:

Example Problem 1: Let $n \in \mathbb{N}$, and $\alpha, \beta, \gamma$ be the angles of a given triangle. Consider the following inequality:
$$
\cot ^{n} \frac{\alpha}{2}+\cot ^{n} \frac{\beta}{2}+\cot ^{n} \frac{\gamma}{2} \quad () \quad 3^{\frac{n+2}{2}} .
$$

Determine the correct inequality relation to fill in the blank.

Options:

(A) $\leq$ 

(B) $\geq$

(C) $=$ 

(D) $<$

(E) $>$

(F) None of the above
Solution of Example Problem 1: We use the identity
$$
\cot \frac{\alpha}{2}+\cot \frac{\beta}{2}+\cot \frac{\gamma}{2}=\cot \frac{\alpha}{2} \cdot \cot \frac{\beta}{2} \cdot \cot \frac{\gamma}{2} .
$$

Since $\frac{\alpha}{2}, \frac{\beta}{2}, \frac{\gamma}{2} \in(0, \pi / 2)$ it follows that $\cot \frac{\alpha}{2}, \cot \frac{\beta}{2}, \cot \frac{\gamma}{2} \geq 0$.
Applying $A M \geq G M$ we have
$$
\cot \frac{\alpha}{2}+\cot \frac{\beta}{2}+\cot \frac{\gamma}{2} \geq 3 \sqrt[3]{\cot \frac{\alpha}{2} \cdot \cot \frac{\beta}{2} \cdot \cot \frac{\gamma}{2}}
$$
or
$$
\cot \frac{\alpha}{2} \cdot \cot \frac{\beta}{2} \cdot \cot \frac{\gamma}{2} \geq 3 \sqrt[3]{\cot \frac{\alpha}{2} \cdot \cot \frac{\beta}{2} \cdot \cot \frac{\gamma}{2}}
$$
i.e.
$$
\begin{equation*}
\cot \frac{\alpha}{2} \cdot \cot \frac{\beta}{2} \cdot \cot \frac{\gamma}{2} \geq 3^{3 / 2} \tag{1}
\end{equation*}
$$

Furthermore, using the power mean inequality we get
$$
\cot ^{n} \frac{\alpha}{2}+\cot ^{n} \frac{\beta}{2}+\cot ^{n} \frac{\gamma}{2} \geq 3\left(\cot \frac{\alpha}{2} \cdot \cot \frac{\beta}{2} \cdot \cot \frac{\gamma}{2}\right)^{n / 3} .
$$

Now from the previous inequality and (1) we obtain
$$
\cot ^{n} \frac{\alpha}{2}+\cot ^{n} \frac{\beta}{2}+\cot ^{n} \frac{\gamma}{2} \geq 3^{\frac{n+2}{2}}
$$

Equality occurs iff $\alpha=\beta=\gamma=\pi / 3$.
Answer of Example Problem 1: (B) $\geq$

Example Problem 2: Let $x, y, z > 1$ be real numbers such that $\frac{1}{x}+\frac{1}{y}+\frac{1}{z}=2$. Consider the following expressions:
$$
\sqrt{x-1}+\sqrt{y-1}+\sqrt{z-1} \quad () \quad \sqrt{x+y+z}
$$
Determine the correct inequality relation to fill in the blank.

Options:

(A) $\leq$ 

(B) $\geq$

(C) $=$ 

(D) $<$

(E) $>$

(F) None of the above
Solution of Example Problem 2: Let $x=a+1, y=b+1, z=c+1$, and clearly $a, b$ and $c$ are positive real numbers.

The initial condition $\frac{1}{x}+\frac{1}{y}+\frac{1}{z}=2$ becomes $\frac{1}{a+1}+\frac{1}{b+1}+\frac{1}{c+1}=2$, i.e.
$$
\begin{equation*}
a b+b c+c a+2 a b c=1 \tag{1}
\end{equation*}
$$

We need to show that
$$
\begin{equation*}
\sqrt{a}+\sqrt{b}+\sqrt{c} \leq \sqrt{a+b+c+3} \tag{2}
\end{equation*}
$$

After squaring inequality (2) we get
$$
a+b+c+2 \sqrt{a b}+2 \sqrt{b c}+2 \sqrt{c a} \leq a+b+c+3
$$
or
$$
2 \sqrt{a b}+2 \sqrt{b c}+2 \sqrt{c a} \leq 3
$$
i.e.
$$
\begin{equation*}
\sqrt{a b}+\sqrt{b c}+\sqrt{c a} \leq \frac{3}{2} \tag{3}
\end{equation*}
$$

Identity (1) is equivalent to
$$
(\sqrt{a b})^{2}+(\sqrt{b c})^{2}+(\sqrt{c a})^{2}+2(\sqrt{a b} \cdot \sqrt{b c} \cdot \sqrt{c a})=1
$$
so we may take
$$
\sqrt{a b}=\sin \frac{\alpha}{2}, \quad \sqrt{b c}=\sin \frac{\beta}{2}, \quad \sqrt{c a}=\sin \frac{\gamma}{2}
$$
where $\alpha, \beta, \gamma \in(0, \pi)$ and $\alpha+\beta+\gamma=\pi$.
Now inequality (3) is equivalent to
$$
\sin \frac{\alpha}{2}+\sin \frac{\beta}{2}+\sin \frac{\gamma}{2} \leq \frac{3}{2}
$$
where $\alpha, \beta, \gamma \in(0, \pi), \alpha+\beta+\gamma=\pi$, which is true by $N_{3}$ .,Applying the Cauchy-Schwarz inequality we have
$$
\left(\frac{x-1}{x}+\frac{y-1}{y}+\frac{z-1}{z}\right)(x+y+z) \geq(\sqrt{x-1}+\sqrt{y-1}+\sqrt{z-1})^{2} .
$$

Also
$$
\frac{x-1}{x}+\frac{y-1}{y}+\frac{z-1}{z}=3-\left(\frac{1}{x}+\frac{1}{y}+\frac{1}{z}\right)=1
$$

So
$$
x+y+z \geq(\sqrt{x-1}+\sqrt{y-1}+\sqrt{z-1})^{2}
$$
i.e.
$$
\sqrt{x+y+z} \geq \sqrt{x-1}+\sqrt{y-1}+\sqrt{z-1}
$$

Equality occurs iff $\frac{x-1}{x^{2}}=\frac{y-1}{y^{2}}=\frac{z-1}{z^{2}}$ and $\frac{1}{x}+\frac{1}{y}+\frac{1}{z}=2$, i.e. $x=y=z=3 / 2$.
Answer of Example Problem 2: (A) $\leq$

Example Problem 3: Let $x, y, z$ be positive real numbers satisfying the condition
$$
x^{2}+y^{2}+z^{2}+2 x y z=1.
$$

Consider the following expression:
$$
x+y+z \quad () \quad \frac{3}{2}.
$$

Determine the correct inequality relation to fill in the blank.

Options:

(A) $\leq$ 

(B) $\geq$

(C) $=$ 

(D) $<$

(E) $>$

(F) None of the above
Solution of Example Problem 3: Clearly, we must have $x, y, z \in(0,1)$. If we put $s=x+y+z$, we get immediately from the given relation

$$
s^{2}-2 s+1=2(1-x)(1-y)(1-z)
$$

Then, again by the AM-GM Inequality ( $1-x, 1-y, 1-z$ being positive), we obtain

$$
s^{2}-2 s+1 \leq 2\left(\frac{1-x+1-y+1-z}{3}\right)^{3}=2\left(\frac{3-s}{3}\right)^{3}
$$

After some easy calculations this yields

$$
2 s^{3}+9 s^{2}-27 \leq 0 \Leftrightarrow(2 s-3)(s+3)^{2} \leq 0
$$

and the conclusion is plain.
Answer of Example Problem 3: (A) $\leq$


Problem: Let $a_1, a_2, \ldots, a_n$ be real numbers such that $a_1 + a_2 + \ldots + a_n = 0$ and $\max \{|a_i - a_j| \mid 1 \leq i, j \leq n\} \leq 1$. Consider the following expression:
$$
a_1^2 + a_2^2 + \ldots + a_n^2 \quad () \quad \frac{1}{n}\left[\frac{n}{2}\right]\left[\frac{n+1}{2}\right] 
$$

Determine the correct inequality relation to fill in the blank.

Options:

(A) $\leq$ 

(B) $\geq$

(C) $=$ 

(D) $<$

(E) $>$

(F) None of the above

Solution:

## Response

To solve the problem, we start with the given conditions:

1. The sum of the numbers is zero: 
   \[
   a_1 + a_2 + \ldots + a_n = 0.
   \]
2. The maximum difference between any two numbers is at most 1:
   \[
   \max \{|a_i - a_j| \mid 1 \leq i, j \leq n\} \leq 1.
   \]

From the second condition, we can infer that all the \(a_i\) values lie within a range of 1 unit. Specifically, if we denote the minimum value among \(a_i\) as \(m\) and the maximum value as \(M\), we have:
\[
M - m \leq 1.
\]
This implies:
\[
m \leq a_i \leq m + 1 \quad \text{for all } i.
\]

Since the sum of all \(a_i\) is zero, we can express each \(a_i\) in terms of \(m\):
\[
a_i = m + b_i \quad \text{where } b_i \text{ are deviations from } m.
\]
Thus, we have:
\[
\sum_{i=1}^n b_i = 0.
\]

Next, we can express the sum of squares:
\[
a_1^2 + a_2^2 + \ldots + a_n^2 = \sum_{i=1}^n (m + b_i)^2 = \sum_{i=1}^n (m^2 + 2mb_i + b_i^2) = nm^2 + 2m\sum_{i=1}^n b_i + \sum_{i=1}^n b_i^2.
\]
Since \(\sum_{i=1}^n b_i = 0\), this simplifies to:
\[
a_1^2 + a_2^2 + \ldots + a_n^2 = nm^2 + \sum_{i=1}^n b_i^2.
\]

Now, we need to find a bound for \(\sum_{i=1}^n b_i^2\). Since \(b_i\) are deviations from \(m\) and \(M - m \leq 1\), we can say:
\[
|b_i| \leq \frac{1}{2} \quad \text{for all } i.
\]
This is because if \(m\) is the minimum, then \(M\) can be at most \(m + 1\), and thus the deviations \(b_i\) must lie within \([-0.5, 0.5]\).

Using the Cauchy-Schwarz inequality, we can estimate:
\[
\sum_{i=1}^n b_i^2 \geq \frac{(\sum_{i=1}^n b_i)^2}{n} = 0.
\]
However, we need a more precise bound. Since \(|b_i| \leq 0.5\), we have:
\[
\sum_{i=1}^n b_i^2 \leq n \left(\frac{1}{2}\right)^2 = \frac{n}{4}.
\]

Thus, we can write:
\[
a_1^2 + a_2^2 + \ldots + a_n^2 = nm^2 + \sum_{i=1}^n b_i^2 \leq nm^2 + \frac{n}{4}.
\]

Now, we need to relate this to the expression \(\frac{1}{n}\left[\frac{n}{2}\right]\left[\frac{n+1}{2}\right]\). 

The right-hand side can be simplified:
\[
\frac{1}{n}\left[\frac{n}{2}\right]\left[\frac{n+1}{2}\right] = \frac{1}{n} \cdot \frac{n}{2} \cdot \frac{n+1}{2} = \frac{(n+1)}{4}.
\]

Now, we need to show that:
\[
nm^2 + \sum_{i=1}^n b_i^2 \quad () \quad \frac{n+1}{4}.
\]

Since \(m\) can be chosen such that \(m = -\frac{1}{n}\) (to satisfy the sum being zero), we can analyze the case when \(m\) is at its maximum negative value. 

Thus, we can conclude that:
\[
a_1^2 + a_2^2 + \ldots + a_n^2 \leq \frac{n+1}{4}.
\]

Therefore, the correct inequality relation is:
\[
a_1^2 + a_2^2 + \ldots + a_n^2 \leq \frac{1}{n}\left[\frac{n}{2}\right]\left[\frac{n+1}{2}\right].
\]

Thus, the answer is:
The answer is (A) $\leq$.