## Problem

Let $x, y \in \mathbb{R}$ such that $(x+1)(y+2) = 8$. Consider the following expression:
$$
|xy - 10| \quad () \quad 7.
$$

Determine the correct inequality relation to fill in the blank.

Options:

(A) $\leq$ 

(B) $\geq$

(C) $=$ 

(D) $<$

(E) $>$

(F) None of the above

## Query

Task description: Please solve the problem with clear, rigorous, and logically sound steps. At the end of your response, state your answer in exactly this format: 'The answer is (Letter) Symbol', where Letter is one of the given options. Example: 'The answer is (A) $\leq$'.

Here are some example problems and solutions that are related to the problem you are solving:

Example Problem 1: Let $n \in \mathbb{N}$, and $\alpha, \beta, \gamma$ be the angles of a given triangle. Consider the following inequality:
$$
\cot ^{n} \frac{\alpha}{2}+\cot ^{n} \frac{\beta}{2}+\cot ^{n} \frac{\gamma}{2} \quad () \quad 3^{\frac{n+2}{2}} .
$$

Determine the correct inequality relation to fill in the blank.

Options:

(A) $\leq$ 

(B) $\geq$

(C) $=$ 

(D) $<$

(E) $>$

(F) None of the above
Solution of Example Problem 1: We use the identity
$$
\cot \frac{\alpha}{2}+\cot \frac{\beta}{2}+\cot \frac{\gamma}{2}=\cot \frac{\alpha}{2} \cdot \cot \frac{\beta}{2} \cdot \cot \frac{\gamma}{2} .
$$

Since $\frac{\alpha}{2}, \frac{\beta}{2}, \frac{\gamma}{2} \in(0, \pi / 2)$ it follows that $\cot \frac{\alpha}{2}, \cot \frac{\beta}{2}, \cot \frac{\gamma}{2} \geq 0$.
Applying $A M \geq G M$ we have
$$
\cot \frac{\alpha}{2}+\cot \frac{\beta}{2}+\cot \frac{\gamma}{2} \geq 3 \sqrt[3]{\cot \frac{\alpha}{2} \cdot \cot \frac{\beta}{2} \cdot \cot \frac{\gamma}{2}}
$$
or
$$
\cot \frac{\alpha}{2} \cdot \cot \frac{\beta}{2} \cdot \cot \frac{\gamma}{2} \geq 3 \sqrt[3]{\cot \frac{\alpha}{2} \cdot \cot \frac{\beta}{2} \cdot \cot \frac{\gamma}{2}}
$$
i.e.
$$
\begin{equation*}
\cot \frac{\alpha}{2} \cdot \cot \frac{\beta}{2} \cdot \cot \frac{\gamma}{2} \geq 3^{3 / 2} \tag{1}
\end{equation*}
$$

Furthermore, using the power mean inequality we get
$$
\cot ^{n} \frac{\alpha}{2}+\cot ^{n} \frac{\beta}{2}+\cot ^{n} \frac{\gamma}{2} \geq 3\left(\cot \frac{\alpha}{2} \cdot \cot \frac{\beta}{2} \cdot \cot \frac{\gamma}{2}\right)^{n / 3} .
$$

Now from the previous inequality and (1) we obtain
$$
\cot ^{n} \frac{\alpha}{2}+\cot ^{n} \frac{\beta}{2}+\cot ^{n} \frac{\gamma}{2} \geq 3^{\frac{n+2}{2}}
$$

Equality occurs iff $\alpha=\beta=\gamma=\pi / 3$.
Answer of Example Problem 1: (B) $\geq$

Example Problem 2: Let $x, y, z > 1$ be real numbers such that $\frac{1}{x}+\frac{1}{y}+\frac{1}{z}=2$. Consider the following expressions:
$$
\sqrt{x-1}+\sqrt{y-1}+\sqrt{z-1} \quad () \quad \sqrt{x+y+z}
$$
Determine the correct inequality relation to fill in the blank.

Options:

(A) $\leq$ 

(B) $\geq$

(C) $=$ 

(D) $<$

(E) $>$

(F) None of the above
Solution of Example Problem 2: Let $x=a+1, y=b+1, z=c+1$, and clearly $a, b$ and $c$ are positive real numbers.

The initial condition $\frac{1}{x}+\frac{1}{y}+\frac{1}{z}=2$ becomes $\frac{1}{a+1}+\frac{1}{b+1}+\frac{1}{c+1}=2$, i.e.
$$
\begin{equation*}
a b+b c+c a+2 a b c=1 \tag{1}
\end{equation*}
$$

We need to show that
$$
\begin{equation*}
\sqrt{a}+\sqrt{b}+\sqrt{c} \leq \sqrt{a+b+c+3} \tag{2}
\end{equation*}
$$

After squaring inequality (2) we get
$$
a+b+c+2 \sqrt{a b}+2 \sqrt{b c}+2 \sqrt{c a} \leq a+b+c+3
$$
or
$$
2 \sqrt{a b}+2 \sqrt{b c}+2 \sqrt{c a} \leq 3
$$
i.e.
$$
\begin{equation*}
\sqrt{a b}+\sqrt{b c}+\sqrt{c a} \leq \frac{3}{2} \tag{3}
\end{equation*}
$$

Identity (1) is equivalent to
$$
(\sqrt{a b})^{2}+(\sqrt{b c})^{2}+(\sqrt{c a})^{2}+2(\sqrt{a b} \cdot \sqrt{b c} \cdot \sqrt{c a})=1
$$
so we may take
$$
\sqrt{a b}=\sin \frac{\alpha}{2}, \quad \sqrt{b c}=\sin \frac{\beta}{2}, \quad \sqrt{c a}=\sin \frac{\gamma}{2}
$$
where $\alpha, \beta, \gamma \in(0, \pi)$ and $\alpha+\beta+\gamma=\pi$.
Now inequality (3) is equivalent to
$$
\sin \frac{\alpha}{2}+\sin \frac{\beta}{2}+\sin \frac{\gamma}{2} \leq \frac{3}{2}
$$
where $\alpha, \beta, \gamma \in(0, \pi), \alpha+\beta+\gamma=\pi$, which is true by $N_{3}$ .,Applying the Cauchy-Schwarz inequality we have
$$
\left(\frac{x-1}{x}+\frac{y-1}{y}+\frac{z-1}{z}\right)(x+y+z) \geq(\sqrt{x-1}+\sqrt{y-1}+\sqrt{z-1})^{2} .
$$

Also
$$
\frac{x-1}{x}+\frac{y-1}{y}+\frac{z-1}{z}=3-\left(\frac{1}{x}+\frac{1}{y}+\frac{1}{z}\right)=1
$$

So
$$
x+y+z \geq(\sqrt{x-1}+\sqrt{y-1}+\sqrt{z-1})^{2}
$$
i.e.
$$
\sqrt{x+y+z} \geq \sqrt{x-1}+\sqrt{y-1}+\sqrt{z-1}
$$

Equality occurs iff $\frac{x-1}{x^{2}}=\frac{y-1}{y^{2}}=\frac{z-1}{z^{2}}$ and $\frac{1}{x}+\frac{1}{y}+\frac{1}{z}=2$, i.e. $x=y=z=3 / 2$.
Answer of Example Problem 2: (A) $\leq$

Example Problem 3: Let $x, y, z$ be positive real numbers satisfying the condition
$$
x^{2}+y^{2}+z^{2}+2 x y z=1.
$$

Consider the following expression:
$$
x+y+z \quad () \quad \frac{3}{2}.
$$

Determine the correct inequality relation to fill in the blank.

Options:

(A) $\leq$ 

(B) $\geq$

(C) $=$ 

(D) $<$

(E) $>$

(F) None of the above
Solution of Example Problem 3: Clearly, we must have $x, y, z \in(0,1)$. If we put $s=x+y+z$, we get immediately from the given relation

$$
s^{2}-2 s+1=2(1-x)(1-y)(1-z)
$$

Then, again by the AM-GM Inequality ( $1-x, 1-y, 1-z$ being positive), we obtain

$$
s^{2}-2 s+1 \leq 2\left(\frac{1-x+1-y+1-z}{3}\right)^{3}=2\left(\frac{3-s}{3}\right)^{3}
$$

After some easy calculations this yields

$$
2 s^{3}+9 s^{2}-27 \leq 0 \Leftrightarrow(2 s-3)(s+3)^{2} \leq 0
$$

and the conclusion is plain.
Answer of Example Problem 3: (A) $\leq$


Problem: Let $x, y \in \mathbb{R}$ such that $(x+1)(y+2) = 8$. Consider the following expression:
$$
|xy - 10| \quad () \quad 7.
$$

Determine the correct inequality relation to fill in the blank.

Options:

(A) $\leq$ 

(B) $\geq$

(C) $=$ 

(D) $<$

(E) $>$

(F) None of the above

Solution:

## Response

To solve the problem, we start with the given equation:

\[
(x+1)(y+2) = 8.
\]

Expanding this, we have:

\[
xy + 2x + y + 2 = 8.
\]

Rearranging gives:

\[
xy + 2x + y = 6.
\]

We want to analyze the expression:

\[
|xy - 10| \quad () \quad 7.
\]

This can be rewritten as:

\[
|xy - 10| < 7 \quad \text{or} \quad |xy - 10| > 7.
\]

To find the bounds for \(xy\), we can express \(xy\) in terms of \(x\) and \(y\):

1. From \(xy + 2x + y = 6\), we can express \(y\) in terms of \(x\):

   \[
   y = 6 - xy - 2x.
   \]

2. Substitute \(y\) back into the original equation:

   \[
   (x + 1)(6 - xy - 2x + 2) = 8.
   \]

However, this approach can become complicated. Instead, we can analyze the expression \(xy\) directly.

From the equation \(xy + 2x + y = 6\), we can isolate \(xy\):

\[
xy = 6 - 2x - y.
\]

Now, we can substitute \(y\) from the original equation:

\[
y = \frac{8}{x + 1} - 2.
\]

Substituting this into the expression for \(xy\):

\[
xy = 6 - 2x - \left(\frac{8}{x + 1} - 2\right).
\]

This simplifies to:

\[
xy = 6 - 2x - \frac{8}{x + 1} + 2 = 8 - 2x - \frac{8}{x + 1}.
\]

Now we need to find the range of \(xy\):

1. **Finding the maximum and minimum values of \(xy\)**:

   We can analyze the function \(f(x) = 8 - 2x - \frac{8}{x + 1}\). To find critical points, we differentiate:

   \[
   f'(x) = -2 + \frac{8}{(x + 1)^2}.
   \]

   Setting \(f'(x) = 0\):

   \[
   -2 + \frac{8}{(x + 1)^2} = 0 \implies \frac{8}{(x + 1)^2} = 2 \implies (x + 1)^2 = 4 \implies x + 1 = 2 \text{ or } x + 1 = -2.
   \]

   Thus, \(x = 1\) or \(x = -3\). Since \(x\) must be real, we only consider \(x = 1\).

   Evaluating \(f(1)\):

   \[
   f(1) = 8 - 2(1) - \frac{8}{1 + 1} = 8 - 2 - 4 = 2.
   \]

   As \(x \to -1\), \(y\) approaches infinity, and as \(x \to \infty\), \(y\) approaches 0, leading to \(xy\) approaching 0.

2. **Finding bounds for \(xy\)**:

   Thus, we have:

   \[
   xy \text{ can take values from } 0 \text{ to } 2.
   \]

3. **Analyzing the expression**:

   Now we check the inequality:

   \[
   |xy - 10| < 7 \implies -7 < xy - 10 < 7 \implies 3 < xy < 17.
   \]

   Since \(xy\) can only take values from \(0\) to \(2\), it is clear that:

   \[
   xy < 3.
   \]

   Therefore, we conclude:

   \[
   |xy - 10| > 7.
   \]

Thus, the correct inequality relation is:

The answer is (B) $\geq$.