## Problem

For $a, b, c > 0$, find the largest constant $C$ such that the following inequality holds for all $a, b, c$:
$$
\frac{a^3}{a^3 + abc + b^3} + \frac{b^3}{b^3 + abc + c^3} + \frac{c^3}{c^3 + abc + a^3} \geq C.
$$

## Query

Task description: Please solve the problem with clear, rigorous, and logically sound steps. At the end of your response, state your answer in exactly this format: 'The answer is $C=X$', where X is your calculated numerical bound value. Example: 'The answer is $C=1$'.

Problem: For $a, b, c > 0$, find the largest constant $C$ such that the following inequality holds for all $a, b, c$:
$$
\frac{a^3}{a^3 + abc + b^3} + \frac{b^3}{b^3 + abc + c^3} + \frac{c^3}{c^3 + abc + a^3} \geq C.
$$

Solution:

## Response

To solve the problem, we need to analyze the inequality 

\[
\frac{a^3}{a^3 + abc + b^3} + \frac{b^3}{b^3 + abc + c^3} + \frac{c^3}{c^3 + abc + a^3} \geq C
\]

for positive \(a\), \(b\), and \(c\). We will find the largest constant \(C\) such that this inequality holds for all positive values of \(a\), \(b\), and \(c\).

### Step 1: Analyze the terms

Each term in the sum can be rewritten as follows:

\[
\frac{a^3}{a^3 + abc + b^3} = 1 - \frac{abc + b^3}{a^3 + abc + b^3}
\]

This shows that each term is less than 1, and we can express the entire sum as:

\[
\sum_{\text{cyc}} \frac{a^3}{a^3 + abc + b^3} = 3 - \sum_{\text{cyc}} \frac{abc + b^3}{a^3 + abc + b^3}
\]

### Step 2: Find a lower bound

To find a lower bound for the sum, we can consider specific cases for \(a\), \(b\), and \(c\). A natural choice is to set \(a = b = c = 1\):

\[
\frac{1^3}{1^3 + 1 \cdot 1 \cdot 1 + 1^3} = \frac{1}{1 + 1 + 1} = \frac{1}{3}
\]

Thus, we have:

\[
\frac{1}{3} + \frac{1}{3} + \frac{1}{3} = 1
\]

This suggests that \(C\) could be at most 1.

### Step 3: Check if \(C = 1\) holds

Next, we need to check if the inequality holds for \(C = 1\):

\[
\frac{a^3}{a^3 + abc + b^3} + \frac{b^3}{b^3 + abc + c^3} + \frac{c^3}{c^3 + abc + a^3} \geq 1
\]

Rearranging gives:

\[
\frac{a^3}{a^3 + abc + b^3} + \frac{b^3}{b^3 + abc + c^3} + \frac{c^3}{c^3 + abc + a^3} - 1 \geq 0
\]

This can be rewritten as:

\[
\sum_{\text{cyc}} \frac{a^3 - (a^3 + abc + b^3)}{a^3 + abc + b^3} \geq 0
\]

This simplifies to:

\[
\sum_{\text{cyc}} \frac{-abc - b^3}{a^3 + abc + b^3} \geq 0
\]

### Step 4: Use the AM-GM inequality

Using the AM-GM inequality, we can show that:

\[
a^3 + b^3 + abc \geq 3\sqrt[3]{a^3b^3c} = 3abc
\]

Thus, we can conclude that:

\[
\frac{a^3}{a^3 + abc + b^3} \geq \frac{a^3}{3abc} = \frac{a^2}{3b}
\]

Summing cyclically gives:

\[
\sum_{\text{cyc}} \frac{a^2}{3b} = \frac{1}{3} \sum_{\text{cyc}} \frac{a^2}{b}
\]

By the Cauchy-Schwarz inequality, we have:

\[
\sum_{\text{cyc}} \frac{a^2}{b} \geq \frac{(a+b+c)^2}{a+b+c} = a + b + c
\]

Thus, we can conclude that:

\[
\frac{1}{3} \sum_{\text{cyc}} \frac{a^2}{b} \geq 1
\]

### Conclusion

Since we have shown that the inequality holds for \(C = 1\) and cannot exceed this value, we conclude that the largest constant \(C\) such that the inequality holds for all positive \(a\), \(b\), and \(c\) is:

\[
\boxed{1}
\]

Thus, the final answer is:

The answer is \(C=1\).