## Problem

Let $a, b > 0$ and $a + b \leq \frac{3}{2}$. Find the smallest constant $C$ such that the following inequality holds for all $a, b$ satisfying the given constraint:
$$
\frac{a}{a^2+1} + \frac{4b}{b^2+4} \leq C.
$$

## Query

Task description: Please solve the problem with clear, rigorous, and logically sound steps. At the end of your response, state your answer in exactly this format: 'The answer is $C=X$', where X is your calculated numerical bound value. Example: 'The answer is $C=1$'.

Problem: Let $a, b > 0$ and $a + b \leq \frac{3}{2}$. Find the smallest constant $C$ such that the following inequality holds for all $a, b$ satisfying the given constraint:
$$
\frac{a}{a^2+1} + \frac{4b}{b^2+4} \leq C.
$$

Solution:

## Response

To find the smallest constant \( C \) such that 

\[
\frac{a}{a^2+1} + \frac{4b}{b^2+4} \leq C
\]

for all \( a, b > 0 \) satisfying \( a + b \leq \frac{3}{2} \), we will analyze the two terms separately and then combine the results.

### Step 1: Analyze \( \frac{a}{a^2 + 1} \)

Let \( f(a) = \frac{a}{a^2 + 1} \). We will find the maximum value of \( f(a) \) for \( a > 0 \).

To find the critical points, we compute the derivative:

\[
f'(a) = \frac{(a^2 + 1)(1) - a(2a)}{(a^2 + 1)^2} = \frac{a^2 + 1 - 2a^2}{(a^2 + 1)^2} = \frac{1 - a^2}{(a^2 + 1)^2}.
\]

Setting \( f'(a) = 0 \) gives \( 1 - a^2 = 0 \), or \( a = 1 \).

Next, we evaluate \( f(a) \) at \( a = 1 \):

\[
f(1) = \frac{1}{1^2 + 1} = \frac{1}{2}.
\]

We also check the limits as \( a \to 0 \) and \( a \to \infty \):

- As \( a \to 0 \), \( f(a) \to 0 \).
- As \( a \to \infty \), \( f(a) \to 0 \).

Thus, the maximum value of \( f(a) \) occurs at \( a = 1 \) and is \( \frac{1}{2} \).

### Step 2: Analyze \( \frac{4b}{b^2 + 4} \)

Let \( g(b) = \frac{4b}{b^2 + 4} \). We will find the maximum value of \( g(b) \) for \( b > 0 \).

We compute the derivative:

\[
g'(b) = \frac{(b^2 + 4)(4) - 4b(2b)}{(b^2 + 4)^2} = \frac{4b^2 + 16 - 8b^2}{(b^2 + 4)^2} = \frac{16 - 4b^2}{(b^2 + 4)^2}.
\]

Setting \( g'(b) = 0 \) gives \( 16 - 4b^2 = 0 \), or \( b^2 = 4 \), hence \( b = 2 \).

Next, we evaluate \( g(b) \) at \( b = 2 \):

\[
g(2) = \frac{4 \cdot 2}{2^2 + 4} = \frac{8}{4 + 4} = 1.
\]

We also check the limits as \( b \to 0 \) and \( b \to \infty \):

- As \( b \to 0 \), \( g(b) \to 0 \).
- As \( b \to \infty \), \( g(b) \to 0 \).

Thus, the maximum value of \( g(b) \) occurs at \( b = 2 \) and is \( 1 \).

### Step 3: Combine results under the constraint \( a + b \leq \frac{3}{2} \)

Now we need to find the maximum of 

\[
f(a) + g(b) \leq C
\]

under the constraint \( a + b \leq \frac{3}{2} \).

1. If \( a = 1 \), then \( b \leq \frac{3}{2} - 1 = \frac{1}{2} \):
   \[
   g\left(\frac{1}{2}\right) = \frac{4 \cdot \frac{1}{2}}{\left(\frac{1}{2}\right)^2 + 4} = \frac{2}{\frac{1}{4} + 4} = \frac{2}{\frac{17}{4}} = \frac{8}{17}.
   \]
   Thus, \( f(1) + g\left(\frac{1}{2}\right) = \frac{1}{2} + \frac{8}{17} = \frac{17}{34} + \frac{16}{34} = \frac{33}{34} \).

2. If \( b = 1 \), then \( a \leq \frac{3}{2} - 1 = \frac{1}{2} \):
   \[
   f\left(\frac{1}{2}\right) = \frac{\frac{1}{2}}{\left(\frac{1}{2}\right)^2 + 1} = \frac{\frac{1}{2}}{\frac{1}{4} + 1} = \frac{\frac{1}{2}}{\frac{5}{4}} = \frac{2}{5}.
   \]
   Thus, \( f\left(\frac{1}{2}\right) + g(1) = \frac{2}{5} + 1 = \frac{2}{5} + \frac{5}{5} = \frac{7}{5} = 1.4 \).

3. If \( a = \frac{3}{2} \) and \( b = 0 \):
   \[
   f\left(\frac{3}{2}\right) = \frac{\frac{3}{2}}{\left(\frac{3}{2}\right)^2 + 1} = \frac{\frac{3}{2}}{\frac{9}{4} + 1} = \frac{\frac{3}{2}}{\frac{13}{4}} = \frac{3 \cdot 4}{2 \cdot 13} = \frac{6}{13}.
   \]

### Conclusion

The maximum value of \( f(a) + g(b) \) under the constraint \( a + b \leq \frac{3}{2} \) is \( 1.4 \). Therefore, the smallest constant \( C \) such that the inequality holds for all \( a, b \) satisfying the constraint is 

\[
C = 1.4.
\]

Thus, the answer is 

\[
\text{The answer is } C = \frac{7}{5}.
\]