## Problem

Let $a, b > 0$ such that $a + b = 1$. Determine the largest constant $C$ such that the following inequality holds for all $a, b$:

$$
\left(a+\frac{1}{a}\right)^2+\left(b+\frac{1}{b}\right)^2 \geq C.
$$

## Query

Task description: Please solve the problem with clear, rigorous, and logically sound steps. At the end of your response, state your answer in exactly this format: 'The answer is $C=X$', where X is your calculated numerical bound value. Example: 'The answer is $C=1$'.

Problem: Let $a, b > 0$ such that $a + b = 1$. Determine the largest constant $C$ such that the following inequality holds for all $a, b$:

$$
\left(a+\frac{1}{a}\right)^2+\left(b+\frac{1}{b}\right)^2 \geq C.
$$

Solution:

## Response

To solve the problem, we start with the given inequality:

\[
\left(a+\frac{1}{a}\right)^2+\left(b+\frac{1}{b}\right)^2 \geq C
\]

for \( a, b > 0 \) and \( a + b = 1 \).

First, we can express \( b \) in terms of \( a \):

\[
b = 1 - a.
\]

Now, we rewrite the left-hand side of the inequality:

\[
\left(a + \frac{1}{a}\right)^2 + \left((1-a) + \frac{1}{1-a}\right)^2.
\]

Next, we simplify each term. The first term is:

\[
\left(a + \frac{1}{a}\right)^2 = a^2 + 2 + \frac{1}{a^2}.
\]

The second term is:

\[
\left((1-a) + \frac{1}{1-a}\right)^2 = (1-a)^2 + 2 + \frac{1}{(1-a)^2}.
\]

Thus, we can combine these:

\[
\left(a + \frac{1}{a}\right)^2 + \left((1-a) + \frac{1}{1-a}\right)^2 = \left(a^2 + \frac{1}{a^2} + 2\right) + \left((1-a)^2 + \frac{1}{(1-a)^2} + 2\right).
\]

This simplifies to:

\[
a^2 + (1-a)^2 + \frac{1}{a^2} + \frac{1}{(1-a)^2} + 4.
\]

Now, we know that:

\[
a^2 + (1-a)^2 = a^2 + (1 - 2a + a^2) = 2a^2 - 2a + 1 = 2(a^2 - a + \frac{1}{2}).
\]

Next, we need to analyze the term \( \frac{1}{a^2} + \frac{1}{(1-a)^2} \). We can use the Cauchy-Schwarz inequality:

\[
\left( \frac{1}{a^2} + \frac{1}{(1-a)^2} \right) \left( a^2 + (1-a)^2 \right) \geq (1 + 1)^2 = 4.
\]

Let \( x = a^2 + (1-a)^2 \). We have:

\[
x = 2a^2 - 2a + 1.
\]

The minimum value of \( x \) occurs when \( a = \frac{1}{2} \):

\[
x = 2\left(\frac{1}{2}\right)^2 - 2\left(\frac{1}{2}\right) + 1 = \frac{1}{2} - 1 + 1 = \frac{1}{2}.
\]

Thus, we can find the maximum of \( \frac{1}{a^2} + \frac{1}{(1-a)^2} \):

\[
\frac{1}{a^2} + \frac{1}{(1-a)^2} \geq \frac{4}{x}.
\]

Substituting \( x \) gives:

\[
\frac{1}{a^2} + \frac{1}{(1-a)^2} \geq \frac{4}{\frac{1}{2}} = 8.
\]

Now, we can combine everything:

\[
\left(a + \frac{1}{a}\right)^2 + \left((1-a) + \frac{1}{1-a}\right)^2 \geq 8 + 4 = 12.
\]

Thus, the largest constant \( C \) such that the inequality holds for all \( a, b > 0 \) with \( a + b = 1 \) is:

\[
C = 12.
\]

Therefore, the answer is:

\[
\text{The answer is } C=12.
\]