## Problem

Let $a, b, c > 0$ be positive real numbers such that $a b c = 1$. Consider the following inequality:
$$
\frac{a b}{a^2+b^2+\sqrt{c}}+\frac{b c}{b^2+c^2+\sqrt{a}}+\frac{c a}{c^2+a^2+\sqrt{b}} \quad () \quad \frac{3}{2}.
$$

Determine the correct inequality relation to fill in the blank.

Options:

(A) $\leq$ 

(B) $\geq$

(C) $=$ 

(D) $<$

(E) $>$

(F) None of the above

## Query

Task description: Please solve the problem with clear, rigorous, and logically sound steps. At the end of your response, state your answer in exactly this format: 'The answer is (Letter) Symbol', where Letter is one of the given options. Example: 'The answer is (A) $\leq$'.

Problem: Let $a, b, c > 0$ be positive real numbers such that $a b c = 1$. Consider the following inequality:
$$
\frac{a b}{a^2+b^2+\sqrt{c}}+\frac{b c}{b^2+c^2+\sqrt{a}}+\frac{c a}{c^2+a^2+\sqrt{b}} \quad () \quad \frac{3}{2}.
$$

Determine the correct inequality relation to fill in the blank.

Options:

(A) $\leq$ 

(B) $\geq$

(C) $=$ 

(D) $<$

(E) $>$

(F) None of the above

Solution:

## Response

To solve the problem, we need to analyze the given inequality:

\[
\frac{a b}{a^2+b^2+\sqrt{c}}+\frac{b c}{b^2+c^2+\sqrt{a}}+\frac{c a}{c^2+a^2+\sqrt{b}} \quad () \quad \frac{3}{2}.
\]

Given that \( a, b, c > 0 \) and \( abc = 1 \), we can use the AM-GM inequality to help us evaluate the left-hand side of the inequality.

### Step 1: Apply AM-GM Inequality

For each term in the sum, we can apply the AM-GM inequality:

\[
a^2 + b^2 + \sqrt{c} \geq 3 \sqrt[3]{a^2 b^2 \sqrt{c}}.
\]

Calculating the geometric mean:

\[
\sqrt[3]{a^2 b^2 \sqrt{c}} = \sqrt[3]{(ab)^2 \sqrt{c}} = \sqrt[3]{(ab)^2 (abc)^{1/3}} = \sqrt[3]{(ab)^2} \cdot \sqrt[3]{1} = \sqrt[3]{(ab)^2}.
\]

Thus, we have:

\[
a^2 + b^2 + \sqrt{c} \geq 3 \sqrt[3]{(ab)^2}.
\]

### Step 2: Substitute into the Inequality

Now substituting this back into our original expression:

\[
\frac{ab}{a^2 + b^2 + \sqrt{c}} \leq \frac{ab}{3 \sqrt[3]{(ab)^2}} = \frac{ab}{3 \cdot (ab)^{2/3}} = \frac{(ab)^{1/3}}{3}.
\]

### Step 3: Sum the Terms

Applying the same reasoning to the other two terms, we have:

\[
\frac{bc}{b^2 + c^2 + \sqrt{a}} \leq \frac{(bc)^{1/3}}{3},
\]
\[
\frac{ca}{c^2 + a^2 + \sqrt{b}} \leq \frac{(ca)^{1/3}}{3}.
\]

Thus, we can sum these inequalities:

\[
\frac{ab}{a^2 + b^2 + \sqrt{c}} + \frac{bc}{b^2 + c^2 + \sqrt{a}} + \frac{ca}{c^2 + a^2 + \sqrt{b}} \leq \frac{(ab)^{1/3}}{3} + \frac{(bc)^{1/3}}{3} + \frac{(ca)^{1/3}}{3}.
\]

### Step 4: Use the AM-GM Inequality Again

Now, we can apply AM-GM again to the right-hand side:

\[
\frac{(ab)^{1/3} + (bc)^{1/3} + (ca)^{1/3}}{3} \geq \sqrt[3]{(ab)(bc)(ca)} = \sqrt[3]{(abc)^2} = \sqrt[3]{1^2} = 1.
\]

Thus, we have:

\[
\frac{(ab)^{1/3} + (bc)^{1/3} + (ca)^{1/3}}{3} \geq 1 \implies (ab)^{1/3} + (bc)^{1/3} + (ca)^{1/3} \geq 3.
\]

### Step 5: Combine Results

Putting this all together, we find:

\[
\frac{(ab)^{1/3} + (bc)^{1/3} + (ca)^{1/3}}{3} \geq 1 \implies \frac{(ab)^{1/3}}{3} + \frac{(bc)^{1/3}}{3} + \frac{(ca)^{1/3}}{3} \geq 1.
\]

Thus, we conclude:

\[
\frac{ab}{a^2 + b^2 + \sqrt{c}} + \frac{bc}{b^2 + c^2 + \sqrt{a}} + \frac{ca}{c^2 + a^2 + \sqrt{b}} \leq 1.
\]

### Final Conclusion

Since we have shown that the left-hand side is less than or equal to 1, and we need to compare it to \( \frac{3}{2} \):

\[
\frac{3}{2} > 1.
\]

Thus, we conclude that:

\[
\frac{ab}{a^2+b^2+\sqrt{c}}+\frac{bc}{b^2+c^2+\sqrt{a}}+\frac{ca}{c^2+a^2+\sqrt{b}} < \frac{3}{2}.
\]

Therefore, the correct relation to fill in the blank is:

The answer is (D) $<$.