## Problem

Let $a, b, c$ be positive real numbers such that $abc = 1$. Consider the following inequality:
$$
\sum \frac{1}{b(a+b)} \quad () \quad \frac{5}{3}.
$$

Determine the correct inequality relation to fill in the blank.

Options:

(A) $\leq$ 

(B) $\geq$

(C) $=$ 

(D) $<$

(E) $>$

(F) None of the above

## Query

Task description: Please solve the problem with clear, rigorous, and logically sound steps. At the end of your response, state your answer in exactly this format: 'The answer is (Letter) Symbol', where Letter is one of the given options. Example: 'The answer is (A) $\leq$'.

Problem: Let $a, b, c$ be positive real numbers such that $abc = 1$. Consider the following inequality:
$$
\sum \frac{1}{b(a+b)} \quad () \quad \frac{5}{3}.
$$

Determine the correct inequality relation to fill in the blank.

Options:

(A) $\leq$ 

(B) $\geq$

(C) $=$ 

(D) $<$

(E) $>$

(F) None of the above

Solution:

## Response

To solve the inequality 

\[
\sum \frac{1}{b(a+b)} \quad () \quad \frac{5}{3},
\]

where \( a, b, c \) are positive real numbers such that \( abc = 1 \), we will analyze the left-hand side expression.

First, we can rewrite the sum:

\[
\sum \frac{1}{b(a+b)} = \frac{1}{b(a+b)} + \frac{1}{c(b+c)} + \frac{1}{a(c+a)}.
\]

Next, we will use the substitution \( a = \frac{x}{y}, b = \frac{y}{z}, c = \frac{z}{x} \) where \( x, y, z \) are positive real numbers. This substitution ensures that \( abc = 1 \).

Now, we can express each term in the sum:

1. For the first term:
   \[
   \frac{1}{b(a+b)} = \frac{1}{\frac{y}{z} \left(\frac{x}{y} + \frac{y}{z}\right)} = \frac{z}{y \left(\frac{xz}{y} + y\right)} = \frac{z}{\frac{xy + y^2}{y}} = \frac{zy}{xy + y^2}.
   \]

2. For the second term:
   \[
   \frac{1}{c(b+c)} = \frac{1}{\frac{z}{x} \left(\frac{y}{z} + \frac{z}{x}\right)} = \frac{x}{z \left(\frac{y}{z} + \frac{z}{x}\right)} = \frac{x}{\frac{y + z^2/x}{z}} = \frac{xy}{y + z^2/x}.
   \]

3. For the third term:
   \[
   \frac{1}{a(c+a)} = \frac{1}{\frac{x}{y} \left(\frac{z}{x} + \frac{x}{y}\right)} = \frac{y}{x \left(\frac{z + x^2/y}{x}\right)} = \frac{y^2}{z + x^2/y}.
   \]

Now, we can apply the Cauchy-Schwarz inequality to simplify our analysis. By Cauchy-Schwarz, we have:

\[
\left( \sum \frac{1}{b(a+b)} \right) \left( \sum b(a+b) \right) \geq (1 + 1 + 1)^2 = 9.
\]

Calculating \( \sum b(a+b) \):

\[
\sum b(a+b) = b(a+b) + c(b+c) + a(c+a) = ab + b^2 + bc + c^2 + ac + a^2.
\]

Using the AM-GM inequality, we know:

\[
ab + ac + bc + a^2 + b^2 + c^2 \geq 6 \sqrt[6]{(abc)^2} = 6,
\]

since \( abc = 1 \).

Thus, we have:

\[
\sum b(a+b) \geq 6.
\]

Now substituting back into our Cauchy-Schwarz result:

\[
\left( \sum \frac{1}{b(a+b)} \right) \cdot 6 \geq 9 \implies \sum \frac{1}{b(a+b)} \geq \frac{9}{6} = \frac{3}{2} = \frac{5}{3}.
\]

This shows that:

\[
\sum \frac{1}{b(a+b)} \geq \frac{5}{3}.
\]

Thus, the correct inequality to fill in the blank is:

\[
\sum \frac{1}{b(a+b)} \geq \frac{5}{3}.
\]

Therefore, the answer is:

The answer is (B) $\geq$.