## Problem

Let $a, b, c$ be positive numbers. Consider the following inequality:
$$
\frac{a^2}{b} + \frac{b^2}{c} + \frac{4c^2}{a} \quad () \quad -3a + b + 7c.
$$

Determine the correct inequality relation to fill in the blank.

Options:

(A) $\leq$ 

(B) $\geq$

(C) $=$ 

(D) $<$

(E) $>$

(F) None of the above

## Query

Task description: Please solve the problem with clear, rigorous, and logically sound steps. At the end of your response, state your answer in exactly this format: 'The answer is (Letter) Symbol', where Letter is one of the given options. Example: 'The answer is (A) $\leq$'.

Problem: Let $a, b, c$ be positive numbers. Consider the following inequality:
$$
\frac{a^2}{b} + \frac{b^2}{c} + \frac{4c^2}{a} \quad () \quad -3a + b + 7c.
$$

Determine the correct inequality relation to fill in the blank.

Options:

(A) $\leq$ 

(B) $\geq$

(C) $=$ 

(D) $<$

(E) $>$

(F) None of the above

Solution:

## Response

To solve the inequality 

\[
\frac{a^2}{b} + \frac{b^2}{c} + \frac{4c^2}{a} \quad () \quad -3a + b + 7c,
\]

we will analyze both sides of the inequality.

### Step 1: Analyze the left-hand side

The left-hand side is 

\[
L = \frac{a^2}{b} + \frac{b^2}{c} + \frac{4c^2}{a}.
\]

### Step 2: Apply the AM-GM Inequality

We can apply the Arithmetic Mean-Geometric Mean (AM-GM) inequality to each term in \(L\):

1. For the first term, we can write:
   \[
   \frac{a^2}{b} + b + b \geq 3\sqrt[3]{\frac{a^2}{b} \cdot b \cdot b} = 3\sqrt[3]{\frac{a^2 b^2}{b}} = 3\sqrt[3]{a^2 b}.
   \]

2. For the second term:
   \[
   \frac{b^2}{c} + c + c \geq 3\sqrt[3]{\frac{b^2}{c} \cdot c \cdot c} = 3\sqrt[3]{\frac{b^2 c^2}{c}} = 3\sqrt[3]{b^2 c}.
   \]

3. For the third term:
   \[
   \frac{4c^2}{a} + a + a \geq 3\sqrt[3]{\frac{4c^2}{a} \cdot a \cdot a} = 3\sqrt[3]{4c^2 a} = 3\sqrt[3]{4c^2 a}.
   \]

### Step 3: Combine the inequalities

Combining these inequalities, we have:

\[
L \geq 3\sqrt[3]{a^2 b} + 3\sqrt[3]{b^2 c} + 3\sqrt[3]{4c^2 a}.
\]

### Step 4: Analyze the right-hand side

The right-hand side is 

\[
R = -3a + b + 7c.
\]

### Step 5: Test specific values

To determine the relationship between \(L\) and \(R\), we can test specific values for \(a\), \(b\), and \(c\). 

Letâ€™s take \(a = 1\), \(b = 1\), and \(c = 1\):

- Then,
  \[
  L = \frac{1^2}{1} + \frac{1^2}{1} + \frac{4 \cdot 1^2}{1} = 1 + 1 + 4 = 6.
  \]
- And,
  \[
  R = -3 \cdot 1 + 1 + 7 \cdot 1 = -3 + 1 + 7 = 5.
  \]

In this case, we find that \(L = 6\) and \(R = 5\), so \(L > R\).

### Step 6: Generalize the result

Since we have shown that for \(a = 1\), \(b = 1\), and \(c = 1\), \(L > R\), we can conjecture that this holds for other positive values of \(a\), \(b\), and \(c\) as well. 

### Conclusion

Thus, we conclude that the correct inequality to fill in the blank is:

\[
\frac{a^2}{b} + \frac{b^2}{c} + \frac{4c^2}{a} \geq -3a + b + 7c.
\]

Therefore, the answer is:

The answer is (B) $\geq$.