## Problem

Let $a, b, c$ be positive real numbers such that $abc = 1$. Consider the following inequality:
$$
\sqrt[3]{a} + \sqrt[3]{b} + \sqrt[3]{c} \quad () \quad \sqrt[3]{3(3 + a + b + c + ab + bc + ca)}.
$$

Determine the correct inequality relation to fill in the blank.

Options:

(A) $\leq$ 

(B) $\geq$

(C) $=$ 

(D) $<$

(E) $>$

(F) None of the above

## Query

Task description: Please solve the problem with clear, rigorous, and logically sound steps. At the end of your response, state your answer in exactly this format: 'The answer is (Letter) Symbol', where Letter is one of the given options. Example: 'The answer is (A) $\leq$'.

Problem: Let $a, b, c$ be positive real numbers such that $abc = 1$. Consider the following inequality:
$$
\sqrt[3]{a} + \sqrt[3]{b} + \sqrt[3]{c} \quad () \quad \sqrt[3]{3(3 + a + b + c + ab + bc + ca)}.
$$

Determine the correct inequality relation to fill in the blank.

Options:

(A) $\leq$ 

(B) $\geq$

(C) $=$ 

(D) $<$

(E) $>$

(F) None of the above

Solution:

## Response

To solve the problem, we need to analyze the inequality involving the cube roots of the positive real numbers \( a, b, c \) under the condition that \( abc = 1 \).

We start with the left-hand side of the inequality:

\[
\sqrt[3]{a} + \sqrt[3]{b} + \sqrt[3]{c}
\]

Using the substitution \( x = \sqrt[3]{a} \), \( y = \sqrt[3]{b} \), and \( z = \sqrt[3]{c} \), we have \( xyz = \sqrt[3]{abc} = \sqrt[3]{1} = 1 \). Thus, we can rewrite the left-hand side as:

\[
x + y + z
\]

Next, we analyze the right-hand side of the inequality:

\[
\sqrt[3]{3(3 + a + b + c + ab + bc + ca)}
\]

We will express \( a, b, c \) in terms of \( x, y, z \):

\[
a = x^3, \quad b = y^3, \quad c = z^3
\]

Now, we need to compute \( a + b + c \) and \( ab + bc + ca \):

\[
a + b + c = x^3 + y^3 + z^3
\]

Using the identity for the sum of cubes, we have:

\[
x^3 + y^3 + z^3 = (x+y+z)(x^2 + y^2 + z^2 - xy - xz - yz) + 3xyz
\]

Since \( xyz = 1 \), we can simplify this to:

\[
x^3 + y^3 + z^3 = (x+y+z)(x^2 + y^2 + z^2 - xy - xz - yz) + 3
\]

Next, we compute \( ab + bc + ca \):

\[
ab + bc + ca = x^3y^3 + y^3z^3 + z^3x^3 = (xy)(yz) + (yz)(zx) + (zx)(xy) = (xy + yz + zx)(xyz) = xy + yz + zx
\]

Now we can substitute these into the right-hand side:

\[
3 + a + b + c + ab + bc + ca = 3 + (x^3 + y^3 + z^3) + (ab + bc + ca)
\]

Thus, we have:

\[
3 + x^3 + y^3 + z^3 + (xy + yz + zx)
\]

Now we need to analyze the inequality:

\[
x + y + z \quad () \quad \sqrt[3]{3(3 + x^3 + y^3 + z^3 + xy + yz + zx)}
\]

Using the AM-GM inequality, we know that:

\[
\frac{x + y + z}{3} \geq \sqrt[3]{xyz} = 1 \implies x + y + z \geq 3
\]

Now we need to compare \( x + y + z \) with the right-hand side. We can use the fact that \( x^3 + y^3 + z^3 \geq 3xyz = 3 \) (by AM-GM) to show that:

\[
x^3 + y^3 + z^3 \geq 3
\]

Thus, we can conclude that:

\[
3 + x^3 + y^3 + z^3 + (xy + yz + zx) \geq 3 + 3 + 0 = 6
\]

Now we can apply the AM-GM inequality again to \( x^3 + y^3 + z^3 \):

\[
\sqrt[3]{3(3 + x^3 + y^3 + z^3 + xy + yz + zx)} \geq \sqrt[3]{3(6)} = \sqrt[3]{18}
\]

Since \( x + y + z \geq 3 \), we can conclude that:

\[
x + y + z \leq \sqrt[3]{3(3 + x^3 + y^3 + z^3 + xy + yz + zx)}
\]

Thus, we have:

\[
\sqrt[3]{a} + \sqrt[3]{b} + \sqrt[3]{c} \leq \sqrt[3]{3(3 + a + b + c + ab + bc + ca)}
\]

Therefore, the correct relation to fill in the blank is:

The answer is (A) $\leq$.