## Problem

Let $a, b, c \geq 0$ be real numbers such that $a^2 + b^2 + c^2 = 3$. Consider the following inequality:
$$
\sum_{cyc} \frac{a}{a+2} \quad () \quad 1.
$$

Determine the correct inequality relation to fill in the blank.

Options:

(A) $\leq$ 

(B) $\geq$

(C) $=$ 

(D) $<$

(E) $>$

(F) None of the above

## Query

Task description: Please solve the problem with clear, rigorous, and logically sound steps. At the end of your response, state your answer in exactly this format: 'The answer is (Letter) Symbol', where Letter is one of the given options. Example: 'The answer is (A) $\leq$'.

Problem: Let $a, b, c \geq 0$ be real numbers such that $a^2 + b^2 + c^2 = 3$. Consider the following inequality:
$$
\sum_{cyc} \frac{a}{a+2} \quad () \quad 1.
$$

Determine the correct inequality relation to fill in the blank.

Options:

(A) $\leq$ 

(B) $\geq$

(C) $=$ 

(D) $<$

(E) $>$

(F) None of the above

Solution:

## Response

To solve the problem, we need to analyze the expression 

\[
\sum_{cyc} \frac{a}{a+2} = \frac{a}{a+2} + \frac{b}{b+2} + \frac{c}{c+2}
\]

under the constraint \( a^2 + b^2 + c^2 = 3 \) where \( a, b, c \geq 0 \).

### Step 1: Analyze the function \( f(x) = \frac{x}{x+2} \)

The function \( f(x) = \frac{x}{x+2} \) is increasing for \( x \geq 0 \) because its derivative 

\[
f'(x) = \frac{2}{(x+2)^2} > 0
\]

for \( x \geq 0 \). This means that larger values of \( a, b, c \) will yield larger values of \( f(a), f(b), f(c) \).

### Step 2: Use Cauchy-Schwarz Inequality

We can apply the Cauchy-Schwarz inequality to the sum:

\[
\left( \sum_{cyc} \frac{a}{a+2} \right) \left( \sum_{cyc} (a+2) \right) \geq (a+b+c)^2
\]

Calculating \( \sum_{cyc} (a+2) \):

\[
\sum_{cyc} (a+2) = (a+b+c) + 6
\]

Thus, we have:

\[
\left( \sum_{cyc} \frac{a}{a+2} \right) \left( a+b+c + 6 \right) \geq (a+b+c)^2
\]

### Step 3: Analyze the implications

Let \( S = a + b + c \). Then we can rewrite the inequality as:

\[
\sum_{cyc} \frac{a}{a+2} \geq \frac{(a+b+c)^2}{a+b+c + 6}
\]

### Step 4: Find bounds for \( S \)

Using the Cauchy-Schwarz inequality again on \( a^2 + b^2 + c^2 = 3 \):

\[
(a+b+c)^2 \leq 3(a^2 + b^2 + c^2) = 3 \cdot 3 = 9
\]

Thus, \( S^2 \leq 9 \) implies \( S \leq 3 \).

### Step 5: Evaluate the sum

Now we need to evaluate \( \sum_{cyc} \frac{a}{a+2} \) when \( a^2 + b^2 + c^2 = 3 \). 

1. **Case when \( a = b = c = 1 \)**:
   \[
   \sum_{cyc} \frac{1}{1+2} = 3 \cdot \frac{1}{3} = 1
   \]

2. **Case when \( a = \sqrt{3}, b = 0, c = 0 \)**:
   \[
   \frac{\sqrt{3}}{\sqrt{3}+2} < 1
   \]

3. **Case when \( a = 0, b = 0, c = \sqrt{3} \)**:
   \[
   \frac{\sqrt{3}}{\sqrt{3}+2} < 1
   \]

### Conclusion

From the analysis, we see that the maximum value of \( \sum_{cyc} \frac{a}{a+2} \) occurs when \( a = b = c = 1 \), yielding exactly 1. In all other cases, the sum is less than 1. Therefore, we conclude:

\[
\sum_{cyc} \frac{a}{a+2} < 1
\]

Thus, the correct inequality to fill in the blank is:

The answer is (D) $<$.