## Problem

Let $a, b, c > 0$ be positive real numbers such that $a + b + c = 1$. Consider the following inequality:
$$
5(a^2 + b^2 + c^2) \quad () \quad 6(a^3 + b^3 + c^3) + 1.
$$

Determine the correct inequality relation to fill in the blank.

Options:

(A) $\leq$ 

(B) $\geq$

(C) $=$ 

(D) $<$

(E) $>$

(F) None of the above

## Query

Task description: Please solve the problem with clear, rigorous, and logically sound steps. At the end of your response, state your answer in exactly this format: 'The answer is (Letter) Symbol', where Letter is one of the given options. Example: 'The answer is (A) $\leq$'.

Problem: Let $a, b, c > 0$ be positive real numbers such that $a + b + c = 1$. Consider the following inequality:
$$
5(a^2 + b^2 + c^2) \quad () \quad 6(a^3 + b^3 + c^3) + 1.
$$

Determine the correct inequality relation to fill in the blank.

Options:

(A) $\leq$ 

(B) $\geq$

(C) $=$ 

(D) $<$

(E) $>$

(F) None of the above

Solution:

## Response

To solve the problem, we need to analyze the inequality:

\[
5(a^2 + b^2 + c^2) \quad () \quad 6(a^3 + b^3 + c^3) + 1
\]

given that \( a, b, c > 0 \) and \( a + b + c = 1 \).

### Step 1: Express \( a^2 + b^2 + c^2 \) and \( a^3 + b^3 + c^3 \)

Using the identity for the sum of squares, we have:

\[
a^2 + b^2 + c^2 = (a + b + c)^2 - 2(ab + ac + bc) = 1^2 - 2(ab + ac + bc) = 1 - 2(ab + ac + bc)
\]

Let \( p = ab + ac + bc \). Then:

\[
a^2 + b^2 + c^2 = 1 - 2p
\]

### Step 2: Express \( a^3 + b^3 + c^3 \)

Using the identity for the sum of cubes, we have:

\[
a^3 + b^3 + c^3 = (a + b + c)(a^2 + b^2 + c^2 - ab - ac - bc) = 1 \cdot ((1 - 2p) - p) = 1 - 3p
\]

### Step 3: Substitute into the inequality

Now we substitute these expressions into the inequality:

\[
5(a^2 + b^2 + c^2) = 5(1 - 2p) = 5 - 10p
\]

\[
6(a^3 + b^3 + c^3) + 1 = 6(1 - 3p) + 1 = 6 - 18p + 1 = 7 - 18p
\]

### Step 4: Set up the inequality

We need to compare:

\[
5 - 10p \quad () \quad 7 - 18p
\]

### Step 5: Solve the inequality

We can rearrange this to find the relationship between \( p \):

\[
5 - 10p \quad () \quad 7 - 18p
\]

Subtract \( 5 \) from both sides:

\[
-10p \quad () \quad 2 - 18p
\]

Add \( 18p \) to both sides:

\[
8p \quad () \quad 2
\]

Dividing both sides by 8 (since \( p \geq 0 \)) gives:

\[
p \quad () \quad \frac{1}{4}
\]

### Step 6: Analyze \( p \)

The maximum value of \( p = ab + ac + bc \) occurs when \( a = b = c = \frac{1}{3} \):

\[
p = 3 \left(\frac{1}{3} \cdot \frac{1}{3}\right) = 3 \cdot \frac{1}{9} = \frac{1}{3}
\]

Since \( \frac{1}{3} > \frac{1}{4} \), we conclude that \( p \) can take values up to \( \frac{1}{3} \).

### Step 7: Determine the inequality

Since \( p \) can be at most \( \frac{1}{3} \), we have:

\[
p < \frac{1}{4} \quad \text{is not possible.}
\]

Thus, we conclude that:

\[
5(a^2 + b^2 + c^2) \geq 6(a^3 + b^3 + c^3) + 1
\]

### Final Answer

The correct inequality relation to fill in the blank is:

The answer is (B) $\geq$.