## Problem

Let $a, b, c$ be positive real numbers such that $a + b + c = 1$. Consider the following inequality:
$$
a \sqrt[3]{1+b-c} + b \sqrt[3]{1+c-a} + c \sqrt[3]{1+a-b} \quad () \quad 1.
$$

Determine the correct inequality relation to fill in the blank.

Options:

(A) $\leq$ 

(B) $\geq$

(C) $=$ 

(D) $<$

(E) $>$

(F) None of the above

## Query

Task description: Please solve the problem with clear, rigorous, and logically sound steps. At the end of your response, state your answer in exactly this format: 'The answer is (Letter) Symbol', where Letter is one of the given options. Example: 'The answer is (A) $\leq$'.

Problem: Let $a, b, c$ be positive real numbers such that $a + b + c = 1$. Consider the following inequality:
$$
a \sqrt[3]{1+b-c} + b \sqrt[3]{1+c-a} + c \sqrt[3]{1+a-b} \quad () \quad 1.
$$

Determine the correct inequality relation to fill in the blank.

Options:

(A) $\leq$ 

(B) $\geq$

(C) $=$ 

(D) $<$

(E) $>$

(F) None of the above

Solution:

## Response

To solve the problem, we need to analyze the expression 

\[
S = a \sqrt[3]{1+b-c} + b \sqrt[3]{1+c-a} + c \sqrt[3]{1+a-b}
\]

given the constraint \( a + b + c = 1 \) where \( a, b, c \) are positive real numbers.

First, we can rewrite the terms inside the cube roots:

1. \( 1 + b - c = 1 + b - (1 - a - b) = a + 2b - 1 \)
2. \( 1 + c - a = 1 + c - (1 - b - c) = b + 2c - 1 \)
3. \( 1 + a - b = 1 + a - (1 - c - a) = c + 2a - 1 \)

Thus, we can express \( S \) as:

\[
S = a \sqrt[3]{a + 2b - 1} + b \sqrt[3]{b + 2c - 1} + c \sqrt[3]{c + 2a - 1}
\]

Next, we will analyze the behavior of \( S \) under the constraint \( a + b + c = 1 \).

### Step 1: Check the case when \( a = b = c = \frac{1}{3} \)

Substituting \( a = b = c = \frac{1}{3} \):

\[
S = \frac{1}{3} \sqrt[3]{1 + \frac{1}{3} - \frac{1}{3}} + \frac{1}{3} \sqrt[3]{1 + \frac{1}{3} - \frac{1}{3}} + \frac{1}{3} \sqrt[3]{1 + \frac{1}{3} - \frac{1}{3}} 
\]

This simplifies to:

\[
S = \frac{1}{3} \sqrt[3]{1} + \frac{1}{3} \sqrt[3]{1} + \frac{1}{3} \sqrt[3]{1} = \frac{1}{3} + \frac{1}{3} + \frac{1}{3} = 1
\]

### Step 2: Check the general case

To analyze whether \( S \) is less than, greater than, or equal to 1 in general, we can apply the Cauchy-Schwarz inequality. 

Using Cauchy-Schwarz, we have:

\[
(a + b + c) \left( a \left(1+b-c\right)^{\frac{2}{3}} + b \left(1+c-a\right)^{\frac{2}{3}} + c \left(1+a-b\right)^{\frac{2}{3}} \right) \geq \left( S \right)^3
\]

Since \( a + b + c = 1 \), we can simplify this to:

\[
1 \cdot \left( a \left(1+b-c\right)^{\frac{2}{3}} + b \left(1+c-a\right)^{\frac{2}{3}} + c \left(1+a-b\right)^{\frac{2}{3}} \right) \geq S^3
\]

This implies:

\[
S^3 \leq a \left(1+b-c\right)^{\frac{2}{3}} + b \left(1+c-a\right)^{\frac{2}{3}} + c \left(1+a-b\right)^{\frac{2}{3}}
\]

### Step 3: Analyze the bounds

To show that \( S \leq 1 \), we can consider the case when one of the variables approaches 1 and the others approach 0. For example, let \( a \to 1 \) and \( b, c \to 0 \):

\[
S \to 1 \cdot \sqrt[3]{1 + 0 - 0} + 0 + 0 = 1
\]

Thus, \( S \) can reach 1 but does not exceed it.

### Conclusion

From the analysis, we find that \( S \) can equal 1 but does not exceed it for any positive \( a, b, c \) such that \( a + b + c = 1 \). Therefore, the correct inequality to fill in the blank is:

\[
S \leq 1
\]

Thus, the answer is:

The answer is (A) $\leq$.