## Problem

Let $a, b, c \geq 0$ be non-negative real numbers such that $a + b + c = 1$. Consider the following inequality:
$$
a^3 + b^3 + c^3 + 6abc \quad () \quad \frac{1}{3}.
$$

Determine the correct inequality relation to fill in the blank.

Options:

(A) $\leq$ 

(B) $\geq$

(C) $=$ 

(D) $<$

(E) $>$

(F) None of the above

## Query

Task description: Please solve the problem with clear, rigorous, and logically sound steps. At the end of your response, state your answer in exactly this format: 'The answer is (Letter) Symbol', where Letter is one of the given options. Example: 'The answer is (A) $\leq$'.

Problem: Let $a, b, c \geq 0$ be non-negative real numbers such that $a + b + c = 1$. Consider the following inequality:
$$
a^3 + b^3 + c^3 + 6abc \quad () \quad \frac{1}{3}.
$$

Determine the correct inequality relation to fill in the blank.

Options:

(A) $\leq$ 

(B) $\geq$

(C) $=$ 

(D) $<$

(E) $>$

(F) None of the above

Solution:

## Response

To solve the problem, we need to analyze the expression \( a^3 + b^3 + c^3 + 6abc \) under the constraint \( a + b + c = 1 \) where \( a, b, c \geq 0 \).

We can use the identity for the sum of cubes:

\[
a^3 + b^3 + c^3 - 3abc = (a+b+c)(a^2 + b^2 + c^2 - ab - ac - bc)
\]

Given that \( a + b + c = 1 \), we can rewrite the identity as:

\[
a^3 + b^3 + c^3 = 3abc + (a^2 + b^2 + c^2 - ab - ac - bc)
\]

Now, we can express \( a^2 + b^2 + c^2 \) in terms of \( a + b + c \):

\[
a^2 + b^2 + c^2 = (a+b+c)^2 - 2(ab + ac + bc) = 1 - 2(ab + ac + bc)
\]

Thus, we can substitute this back into our expression for \( a^3 + b^3 + c^3 \):

\[
a^3 + b^3 + c^3 = 3abc + (1 - 2(ab + ac + bc) - ab - ac - bc)
\]
\[
= 3abc + 1 - 3(ab + ac + bc)
\]

Now, we need to analyze the expression \( a^3 + b^3 + c^3 + 6abc \):

\[
a^3 + b^3 + c^3 + 6abc = 3abc + 1 - 3(ab + ac + bc) + 6abc
\]
\[
= 9abc + 1 - 3(ab + ac + bc)
\]

Next, we will use the AM-GM inequality to find bounds for \( a^3 + b^3 + c^3 + 6abc \).

By the AM-GM inequality, we have:

\[
\frac{a + b + c}{3} \geq \sqrt[3]{abc}
\]

Since \( a + b + c = 1 \):

\[
\frac{1}{3} \geq \sqrt[3]{abc} \implies abc \leq \frac{1}{27}
\]

Now, we can analyze the maximum value of \( a^3 + b^3 + c^3 \). By the Power Mean inequality, we have:

\[
\sqrt[3]{\frac{a^3 + b^3 + c^3}{3}} \geq \frac{a + b + c}{3} = \frac{1}{3}
\]

Thus:

\[
a^3 + b^3 + c^3 \geq \frac{1}{3}
\]

Now, we can combine this with our earlier expression:

\[
a^3 + b^3 + c^3 + 6abc \geq \frac{1}{3} + 6 \cdot 0 = \frac{1}{3}
\]

This shows that:

\[
a^3 + b^3 + c^3 + 6abc \geq \frac{1}{3}
\]

To check if equality can hold, consider the case when \( a = b = c = \frac{1}{3} \):

\[
a^3 + b^3 + c^3 = 3 \left( \frac{1}{3} \right)^3 = 3 \cdot \frac{1}{27} = \frac{1}{9}
\]
\[
abc = \left( \frac{1}{3} \right)^3 = \frac{1}{27}
\]
\[
6abc = 6 \cdot \frac{1}{27} = \frac{2}{9}
\]
\[
a^3 + b^3 + c^3 + 6abc = \frac{1}{9} + \frac{2}{9} = \frac{3}{9} = \frac{1}{3}
\]

Thus, we have shown that:

\[
a^3 + b^3 + c^3 + 6abc = \frac{1}{3}
\]

Therefore, the correct inequality relation to fill in the blank is:

\[
\boxed{=}
\]

Thus, the final answer is:

The answer is (C) $=$.