## Problem

Let $a, b > 0$ be positive real numbers such that $a + b \leq \frac{3}{2}$. Consider the following inequality:
$$
\frac{a}{2a^2+1} + \frac{4b}{3b^2+4} \quad () \quad \frac{7}{5}.
$$

Determine the correct inequality relation to fill in the blank.

Options:

(A) $\leq$ 

(B) $\geq$

(C) $=$ 

(D) $<$

(E) $>$

(F) None of the above

## Query

Task description: Please solve the problem with clear, rigorous, and logically sound steps. At the end of your response, state your answer in exactly this format: 'The answer is (Letter) Symbol', where Letter is one of the given options. Example: 'The answer is (A) $\leq$'.

Problem: Let $a, b > 0$ be positive real numbers such that $a + b \leq \frac{3}{2}$. Consider the following inequality:
$$
\frac{a}{2a^2+1} + \frac{4b}{3b^2+4} \quad () \quad \frac{7}{5}.
$$

Determine the correct inequality relation to fill in the blank.

Options:

(A) $\leq$ 

(B) $\geq$

(C) $=$ 

(D) $<$

(E) $>$

(F) None of the above

Solution:

## Response

To solve the problem, we need to analyze the expression 

\[
\frac{a}{2a^2+1} + \frac{4b}{3b^2+4}
\]

under the constraint \( a + b \leq \frac{3}{2} \) where \( a, b > 0 \).

### Step 1: Analyze the first term \(\frac{a}{2a^2 + 1}\)

We will first find the maximum value of \(\frac{a}{2a^2 + 1}\). To do this, we can differentiate the function with respect to \(a\):

Let \( f(a) = \frac{a}{2a^2 + 1} \).

Using the quotient rule:

\[
f'(a) = \frac{(2a^2 + 1)(1) - a(4a)}{(2a^2 + 1)^2} = \frac{2a^2 + 1 - 4a^2}{(2a^2 + 1)^2} = \frac{1 - 2a^2}{(2a^2 + 1)^2}
\]

Setting \( f'(a) = 0 \):

\[
1 - 2a^2 = 0 \implies a^2 = \frac{1}{2} \implies a = \frac{1}{\sqrt{2}}.
\]

Now we check the second derivative to confirm it's a maximum:

\[
f''(a) = \text{(complex expression, but we can check the sign)}.
\]

Instead, we can evaluate \( f(a) \) at the critical point and endpoints. 

### Step 2: Evaluate \( f(a) \) at \( a = \frac{1}{\sqrt{2}} \)

\[
f\left(\frac{1}{\sqrt{2}}\right) = \frac{\frac{1}{\sqrt{2}}}{2\left(\frac{1}{\sqrt{2}}\right)^2 + 1} = \frac{\frac{1}{\sqrt{2}}}{1 + 1} = \frac{1}{2\sqrt{2}}.
\]

### Step 3: Analyze the second term \(\frac{4b}{3b^2 + 4}\)

Let \( g(b) = \frac{4b}{3b^2 + 4} \).

Using a similar approach, we differentiate:

\[
g'(b) = \frac{(3b^2 + 4)(4) - 4b(6b)}{(3b^2 + 4)^2} = \frac{12b^2 + 16 - 24b^2}{(3b^2 + 4)^2} = \frac{16 - 12b^2}{(3b^2 + 4)^2}.
\]

Setting \( g'(b) = 0 \):

\[
16 - 12b^2 = 0 \implies b^2 = \frac{4}{3} \implies b = \frac{2}{\sqrt{3}}.
\]

### Step 4: Evaluate \( g(b) \) at \( b = \frac{2}{\sqrt{3}} \)

\[
g\left(\frac{2}{\sqrt{3}}\right) = \frac{4 \cdot \frac{2}{\sqrt{3}}}{3\left(\frac{2}{\sqrt{3}}\right)^2 + 4} = \frac{\frac{8}{\sqrt{3}}}{\frac{12}{3} + 4} = \frac{\frac{8}{\sqrt{3}}}{8} = \frac{1}{\sqrt{3}}.
\]

### Step 5: Combine the results

Now we need to find the maximum of 

\[
\frac{1}{2\sqrt{2}} + \frac{1}{\sqrt{3}}.
\]

Calculating these values:

\[
\frac{1}{2\sqrt{2}} \approx 0.3536, \quad \frac{1}{\sqrt{3}} \approx 0.5774.
\]

Adding these:

\[
\frac{1}{2\sqrt{2}} + \frac{1}{\sqrt{3}} \approx 0.3536 + 0.5774 = 0.931.
\]

### Step 6: Compare with \(\frac{7}{5} = 1.4\)

Since \(0.931 < 1.4\), we conclude that:

\[
\frac{a}{2a^2 + 1} + \frac{4b}{3b^2 + 4} < \frac{7}{5}.
\]

Thus, the correct inequality relation to fill in the blank is:

The answer is (D) $<$.