# Problem Entry

## Problem Type
bound

## Problem
Let $a, b, c, x, y, z$ be positive real numbers such that $x + y + z = 1$. Determine the maximal constant $C$ such that the following inequality holds for all $a, b, c, x, y, z$:

$$
a x + b y + c z + C \sqrt{(x y + y z + z x)(a b + b c + c a)} \leq a+b+c.
$$

## Current Solution
The inequality being homogeneous in $a, b, c$ we can assume that $a+b+c=1$. We apply this time the AM-GM Inequality and we find that
$a x+b y+c z+2 \sqrt{(x y+y z+z x)(a b+b c+c a)} \leq a x+b y+c z+x y+y z+z x+a b+b c+c a$.
Consequently,
$x y+y z+z x+a b+b c+c a=\frac{1-x^{2}-y^{2}-z^{2}}{2}+\frac{1-a^{2}-b^{2}-c^{2}}{2} \leq 1-a x-b y-c z$,
the last one being equivalent to $(x-a)^{2}+(y-b)^{2}+(z-c)^{2} \geq 0$.

Equality holds when $x = a$, $y = b$, $z = c$, that is, when the vectors $(x, y, z)$ and $(a, b, c)$ are equal. In this case, the inequality becomes an equality, and $C = 2$ gives the maximal value for which the inequality always holds.

Therefore, the answer is $C = 2$.

## Expected Answer
$C = 2$

## Enhanced Solution
**Enhanced Detailed Solution**

We wish to find the largest constant \(C\) for which
\[
  a x + b y + c z 
  
  + C \sqrt{\bigl(xy + yz + zx\bigr)\bigl(ab + bc + ca\bigr)}
  \;\le\;
  a + b + c
\]
holds for all positive real numbers \(a,b,c,x,y,z\) satisfying \(x+y+z=1\).  We shall show that the maximal such constant is \(C=2\).

---

**1. Homogenization**

The given inequality is homogeneous of degree 1 in \(a,b,c\), and also homogeneous of degree 1 in \(x,y,z\) after using \(x+y+z=1\).  Therefore, without loss of generality we may impose the normalization
\[
  a + b + c 
  = 1.
\]
Under this assumption the right-hand side becomes 1, so it suffices to prove
\[
  a x + b y + c z 
  + C \sqrt{(xy + yz + zx)igl(ab + bc + ca\bigr)} 
  \le 1.
\]

Let us introduce the symmetric sums
\[
  S_1 = a + b + c = 1,
  \quad
  S_2 = ab + bc + ca,
  \quad
  T_2 = xy + yz + zx.
\]
Then the inequality to prove is
\[
  a x + b y + c z 
  + C \sqrt{T_2 \, S_2}
  \le 1.
\]

**2. Application of the AM–GM inequality**

We apply the arithmetic–geometric mean inequality to the nonnegative numbers \(T_2\) and \(S_2\):
\[
  2\sqrt{T_2\,S_2} 
  \le T_2 + S_2.
\]
Hence for \(C=2\) we obtain
\[
  a x + b y + c z + 2\sqrt{T_2\,S_2}
  \le a x + b y + c z + (T_2 + S_2).
\]
It follows that it will be enough to show
\[
  a x + b y + c z + T_2 + S_2 
  \le 1.
\]

**3. Expressing \(T_2+S_2\) in terms of squares**

Recall the identities for any triple \((u,v,w)\):
\[
  uv + vw + wu 
  = \frac{(u+v+w)^2 - (u^2 + v^2 + w^2)}{2}.
\]
Applying this with \((u,v,w)=(x,y,z)\) and with \((u,v,w)=(a,b,c)\), together with \(x+y+z=1\) and \(a+b+c=1\), we get
\[
  T_2 = xy+yz+zx = \frac{1 - (x^2+y^2+z^2)}{2},
  \qquad
  S_2 = ab+bc+ca = \frac{1 - (a^2+b^2+c^2)}{2}.
\]
Hence
\[
  T_2 + S_2
  = \frac{1 - (x^2+y^2+z^2)}{2} + \frac{1 - (a^2+b^2+c^2)}{2} 
  = 1 
    - \frac{x^2+y^2+z^2 + a^2+b^2+c^2}{2}.
\]
Therefore,
\[
  a x + b y + c z + T_2 + S_2
  = a x + b y + c z 
    + 1 
    - \frac{x^2+y^2+z^2 + a^2+b^2+c^2}{2}.
\]
We wish to prove this is \(\le1\).  Equivalently,
\[
  a x + b y + c z 
  \le \frac{x^2 + y^2 + z^2 + a^2 + b^2 + c^2}{2}.
\]

**4. Final reduction to a sum of squares**

Rearrange the last inequality:
\[
  0 
  \le \frac{x^2 + y^2 + z^2 + a^2 + b^2 + c^2}{2} 
       - (a x + b y + c z)
  = \frac{1}{2}\sum_{\xi\in\{a,b,c\}} (\xi^2) 
     + \frac{1}{2}\sum_{\eta\in\{x,y,z\}} (\eta^2)
     - \sum_{\substack{\xi\in\{a,b,c\}\\\eta\in\{x,y,z\}}}
       \xi\,\eta\,
\]
which, upon grouping like terms, is exactly
\[
  \frac{1}{2}\bigl[(a-x)^2 + (b-y)^2 + (c-z)^2\bigr] 
  \ge 0.
\]
This last statement is manifestly true, since each square is nonnegative.  Thus we have shown
\[
  a x + b y + c z + 2\sqrt{T_2\,S_2} 
  \le a x + b y + c z + (T_2+S_2)
  \le 1,
\]
and therefore the original inequality holds for \(C=2\).

**5. Sharpness of \(C=2\)**

All inequalities above become equalities exactly when
  (i)  the AM–GM step satisfies \(T_2 = S_2\),
 (ii)  the sum of squares vanishes, i.e. \(a=x,\;b=y,\;c=z\).
In particular one sees that if \((a,b,c)=(x,y,z)\), then each step is an equality and the bound \(C=2\) cannot be increased further without violating the inequality in that case.

Hence the maximal constant is \(C=2\).

**Answer**

The answer is $C=2$.  
