# Problem Entry

## Problem Type
bound

## Problem
Let $a, b, c$ be positive real numbers such that $a b c=1$. Find the smallest largest $C$ such that the following inequality holds for all $a, b, c$ satisfying the given constraint:
$$
\frac{a}{\sqrt{7+b^{2}+c^{2}}}+\frac{b}{\sqrt{7+c^{2}+a^{2}}}+\frac{c}{\sqrt{7+a^{2}+b^{2}}} \geq C
$$

## Current Solution
Denote
$$
A=\frac{a}{\sqrt{7+b^{2}+c^{2}}}+\frac{b}{\sqrt{7+c^{2}+a^{2}}}+\frac{c}{\sqrt{7+a^{2}+b^{2}}}
$$
and
$$
B=a\left(7+b^{2}+c^{2}\right)+b\left(7+c^{2}+a^{2}\right)+c\left(7+a^{2}+b^{2}\right)
$$

By Hölder's inequality we have
$$
\begin{equation*}
A^{2} B \geq(a+b+c)^{3} . \tag{1}
\end{equation*}
$$

Furthermore
$$
\begin{align*}
B & =7(a+b+c)+(a+b+c)(a b+b c+c a)-3 \\
& \leq 7(a+b+c)+\frac{(a+b+c)^{3}}{3}-3 \leq(a+b+c)^{3} \tag{2}
\end{align*}
$$
and by (1) and (2) we obtain
$$
A^{2} \geq \frac{(a+b+c)^{3}}{B} \geq 1, \quad \text { i.e. } \quad A \geq 1
$$
as required.

Equality holds when $a = b = c = 1$, since then $abc = 1$ and $A = 3/\sqrt{9} = 1$. This gives the minimum value of $A$, so $C = 1$ is the largest constant for which the inequality always holds.

Therefore, the answer is $C = 1$.

## Expected Answer
$C = 1$

## Enhanced Solution
We wish to show that for all positive real numbers a,b,c satisfying abc=1,

    A := \frac{a}{\sqrt{7+b^2+c^2}} + \frac{b}{\sqrt{7+c^2+a^2}} + \frac{c}{\sqrt{7+a^2+b^2}} \ge C,

and to find the largest such constant C.

**Step 1: Introducing an auxiliary expression and applying Hölder’s inequality**

Define also

    B := a\,(7 + b^2 + c^2) \;+
         b\,(7 + c^2 + a^2) \;+
         c\,(7 + a^2 + b^2).

We now apply the following form of Hölder’s inequality to the three-term sum A:

    \bigl(\sum_{\text{cyc}} a\bigr)^3
      = \bigl(\sum_{\text{cyc}} a \cdot 1\cdot 1\bigr)^3
      \le \Bigl(\sum_{\text{cyc}} \frac{a}{\sqrt{7+b^2+c^2}}\Bigr)^2
            \Bigl(\sum_{\text{cyc}} a\,(7+b^2+c^2)\Bigr)
      = A^2\,B.

Hence

    (1) \quad A^2\,B \ge (a+b+c)^3.

**Step 2: Establishing an upper bound for B in terms of S = a+b+c**

Write S = a + b + c.  Then expand B:

    B = 7(a+b+c)
        + [a(b^2+c^2) + b(c^2+a^2) + c(a^2+b^2)].

Observe that

    a(b^2+c^2) + b(c^2+a^2) + c(a^2+b^2)
      = (a+b+c)(ab+bc+ca) - 3abc
      = S\,(ab+bc+ca) - 3,

since abc=1.  Therefore,

    B = 7S + S\,(ab+bc+ca) - 3.

By the well-known AM–GM inequality on the three nonnegative terms ab, bc, ca, we have

    ab + bc + ca \le \frac{(a+b+c)^2}{3} = \frac{S^2}{3}.

Hence

    B \le 7S + S\cdot\frac{S^2}{3} - 3 = 7S + \frac{S^3}{3} - 3.

Next, we use the fact that for positive a,b,c with abc=1, by AM–GM again,

    S = a+b+c \ge 3\sqrt[3]{abc} = 3.

Define the function f(S)=7S + S^3/3 -3.  We check that for S\ge3,

    f(S) \le S^3  \quad\Longleftrightarrow\quad 7S -3 \le \tfrac{2}{3}S^3.

At S=3 the two sides coincide: 7\cdot3 - 3 = 18 = (2/3)\cdot27, and for S>3 the derivative of the right‐hand side, 2S^2, exceeds the derivative of the left‐hand side, 7.  Therefore f(S) \le S^3 for all S\ge3.  We conclude

    (2) \quad B \le 7S + \frac{S^3}{3} - 3 \le S^3 = (a+b+c)^3.

**Step 3: Combining (1) and (2) to deduce A\ge1**

From (1) we have A^2\,B \ge (a+b+c)^3, and from (2) B \le (a+b+c)^3.  Hence

    A^2 \ge \frac{(a+b+c)^3}{B} \ge \frac{(a+b+c)^3}{(a+b+c)^3} = 1.

Since A>0, it follows that A\ge1.

**Step 4: Verification of equality case**

All inequalities used become equalities precisely when a=b=c.  Then

    abc=1 \implies a=b=c=1,
    A=3/\sqrt{7+1+1}=3/3=1,
    B=3\cdot(7+1+1)=27=(a+b+c)^3.

Thus the smallest possible value of A over the constraint abc=1 is 1, and this value is attained.

Therefore, the largest constant C satisfying the given inequality for all positive a,b,c with abc=1 is

The answer is $C=1$
