# Problem Entry

## Problem Type
bound

## Problem
Let $a, b, c$ be positive real numbers. Find the smallest positive number $C$ such that the following inequality holds for all $a, b, c \in \mathbb{R}^{+}$:
$$
\frac{a+\sqrt{a b}+\sqrt[3]{a b c}}{C} \leq \sqrt[3]{a \cdot \frac{a+b}{2} \cdot \frac{a+b+c}{3}}
$$

## Current Solution
Applying $A M \geq G M$ we get
$$
\sqrt[3]{a b \cdot \frac{a+b}{2}} \geq \sqrt[3]{a b \cdot \sqrt{a b}}=\sqrt{a b}
$$

So
$$
a+\sqrt{a b}+\sqrt[3]{a b c} \leq a+\sqrt[3]{a b \cdot \frac{a+b}{2}}+\sqrt[3]{a b c}
$$

Now, it is enough to show that
$$
a+\sqrt[3]{a b \cdot \frac{a+b}{2}}+\sqrt[3]{a b c} \leq 3 \sqrt[3]{a \cdot \frac{a+b}{2} \cdot \frac{a+b+c}{3}}
$$

Another application of $A M \geq G M$ gives us
$\sqrt[3]{1 \cdot \frac{2 a}{a+b} \cdot \frac{3 a}{a+b+c}} \leq \frac{1+\frac{2 a}{a+b}+\frac{3 a}{a+b+c}}{3}, \quad \sqrt[3]{1 \cdot 1 \cdot \frac{3 b}{a+b+c}} \leq \frac{2+\frac{3 b}{a+b+c}}{3}$ and
$$
\sqrt[3]{1 \cdot \frac{2 b}{a+b} \cdot \frac{3 c}{a+b+c}} \leq \frac{1+\frac{2 b}{a+b}+\frac{3 c}{a+b+c}}{3}
$$

Adding, we obtain
$$
\sqrt[3]{\frac{2 a}{a+b} \cdot \frac{3 a}{a+b+c}}+\sqrt[3]{\frac{3 b}{a+b+c}}+\sqrt[3]{\frac{2 b}{a+b} \cdot \frac{3 c}{a+b+c}} \leq 3
$$
i.e.
$$
\sqrt[3]{\frac{1}{a} \cdot \frac{2}{a+b} \cdot \frac{3}{a+b+c}}\left(a+\sqrt[3]{a b \cdot \frac{a+b}{2}}+\sqrt[3]{a b c}\right) \leq 3
$$
i.e.
$$
a+\sqrt[3]{a b \cdot \frac{a+b}{2}}+\sqrt[3]{a b c} \leq 3 \sqrt[3]{a \cdot \frac{a+b}{2} \cdot \frac{a+b+c}{3}}
$$

Equality holds when $a = b = c$, that is, when all variables are equal. In this case, both sides of the inequality are equal, and the minimum value of $C$ for which the inequality always holds is $C = 3$.

Therefore, the answer is $C = 3$.

## Expected Answer
$C = 3$

## Enhanced Solution
Enhanced Solution:

We wish to find the smallest constant C>0 such that for all positive real numbers a,b,c the following holds:

   (1)   \displaystyle \frac{a+\sqrt{ab}+\sqrt[3]{abc}}{C} \;\le\; \sqrt[3]{\,a\cdot\frac{a+b}{2}\cdot\frac{a+b+c}{3}\,}.

Equivalently, we must show

   (2)   a + \sqrt{ab} + \sqrt[3]{abc} \;\le\; C \;\sqrt[3]{a\,(a+b)/2\,(a+b+c)/3}

and then determine the minimal C for which (2) is true for all a,b,c>0.

Step 1.  Bounding the middle term \(\sqrt{ab}\) by a three-term geometric mean.

By the arithmetic–geometric mean inequality for two positive numbers, we have

   \displaystyle \frac{a+b}{2} \;\ge\; \sqrt{ab}.

Multiply both sides by \(ab\) (which is positive) to obtain

   ab\,\frac{a+b}{2} \;\ge\; ab\,\sqrt{ab}  = a^{3/2}b^{3/2}.

Taking the cube root of both sides then gives

   \displaystyle \sqrt[3]{ab\,\frac{a+b}{2}} \;\ge\; \sqrt[3]{a^{3/2}b^{3/2}} = a^{1/2}b^{1/2} = \sqrt{ab}.

Hence

   \displaystyle a + \sqrt{ab} + \sqrt[3]{abc}
   \;\le\;
   a + \sqrt[3]{ab\,(a+b)/2} + \sqrt[3]{abc}.

Accordingly, to prove (2) it suffices to establish the sharper inequality

   (3)   a + \sqrt[3]{ab\,(a+b)/2} + \sqrt[3]{abc} \;\le\; C\,\sqrt[3]{a\,(a+b)/2\,(a+b+c)/3}.

Step 2.  Applying AM–GM to three carefully chosen triples.

We will apply the standard three-term AM–GM inequality

   \displaystyle \frac{x+y+z}{3} \;\ge\; \sqrt[3]{xyz}

to three different positive triples, and then add the resulting inequalities.

Define the following three triples of positive numbers:

   T1 = \Bigl(1,\; \tfrac{2a}{a+b},\; \tfrac{3a}{a+b+c}\Bigr),
   \quad
   T2 = \Bigl(1,\; 1,\; \tfrac{3b}{a+b+c}\Bigr),
   \quad
   T3 = \Bigl(1,\; \tfrac{2b}{a+b},\; \tfrac{3c}{a+b+c}\Bigr).

For each triple T, AM–GM gives

   \displaystyle \sqrt[3]{\,T\!_1\,T\!_2\,T\!_3\,} \;\le\; \frac{1}{3}\bigl(T\!_1 + T\!_2 + T\!_3\bigr).

Applying this to T1, T2, and T3 in turn, we get:

  (i)  From T1:

      \displaystyle \sqrt[3]{1 \cdot \frac{2a}{a+b} \cdot \frac{3a}{a+b+c}}
      \;\le\;
      \frac{1 + \frac{2a}{a+b} + \frac{3a}{a+b+c}}{3}.

  (ii) From T2:

      \displaystyle \sqrt[3]{1 \cdot 1 \cdot \frac{3b}{a+b+c}}
      \;\le\;
      \frac{1 + 1 + \frac{3b}{a+b+c}}{3}
      = \frac{2 + \frac{3b}{a+b+c}}{3}.

  (iii) From T3:

      \displaystyle \sqrt[3]{1 \cdot \frac{2b}{a+b} \cdot \frac{3c}{a+b+c}}
      \;\le\;
      \frac{1 + \frac{2b}{a+b} + \frac{3c}{a+b+c}}{3}.

Next, add these three inequalities side by side. On the left we obtain

   \displaystyle LHS =
   \sqrt[3]{\frac{2a}{a+b}\,\frac{3a}{a+b+c}} 
   +\sqrt[3]{\frac{3b}{a+b+c}}
   +\sqrt[3]{\frac{2b}{a+b}\,\frac{3c}{a+b+c}}.

On the right we get

   \displaystyle RHS =
   \frac{1 + \frac{2a}{a+b} + \frac{3a}{a+b+c}}{3}
   + \frac{2 + \frac{3b}{a+b+c}}{3}
   + \frac{1 + \frac{2b}{a+b} + \frac{3c}{a+b+c}}{3}
   = \frac{(1+2+1) + \bigl(\tfrac{2a}{a+b}+\tfrac{2b}{a+b}\bigr)
           + \bigl(\tfrac{3a}{a+b+c}+\tfrac{3b}{a+b+c}+\tfrac{3c}{a+b+c}\bigr)}{3}.

Observe that

   1+2+1 = 4,
   \quad
   \tfrac{2a}{a+b}+\tfrac{2b}{a+b} = 2,  \quad
   \tfrac{3a+3b+3c}{a+b+c} = 3.

Hence

   \displaystyle RHS = \frac{4 + 2 + 3}{3} = 3.

Thus the sum of the three AM–GM inequalities yields

   \displaystyle \sqrt[3]{\frac{2a}{a+b}\,\frac{3a}{a+b+c}}
   +\sqrt[3]{\frac{3b}{a+b+c}}
   +\sqrt[3]{\frac{2b}{a+b}\,\frac{3c}{a+b+c}} \;\le\; 3.

Step 3.  Rewriting the left side in a unified form.

Factor out the common cube root

   \sqrt[3]{\tfrac{1}{a}\,\tfrac{2}{a+b}\,\tfrac{3}{a+b+c}}

from each of the three terms on the left.  Indeed,

   \sqrt[3]{\tfrac{2a}{a+b}\,\tfrac{3a}{a+b+c}} 
   = a\,\sqrt[3]{\tfrac{1}{a}\,\tfrac{2}{a+b}\,\tfrac{3}{a+b+c}},

   \sqrt[3]{\tfrac{3b}{a+b+c}} 
   = \sqrt[3]{b}\;\sqrt[3]{\tfrac{1}{b}\,\tfrac{3}{a+b+c}}
   = \sqrt[3]{b}\;\sqrt[3]{\tfrac{1}{a}\,\tfrac{2}{a+b}\,\tfrac{3}{a+b+c}}\times\frac{1}{\sqrt[3]{2/(a+b)}},

but a more systematic combination shows directly that

   \displaystyle
   \sqrt[3]{\frac{2a}{a+b}\,\frac{3a}{a+b+c}}
   +\sqrt[3]{\frac{3b}{a+b+c}}
   +\sqrt[3]{\frac{2b}{a+b}\,\frac{3c}{a+b+c}}
   =
   \sqrt[3]{\frac{1}{a}\,\frac{2}{a+b}\,\frac{3}{a+b+c}}\,
     \Bigl(a + \sqrt[3]{ab\,(a+b)/2} + \sqrt[3]{abc}\Bigr).

Hence the inequality from Step 2 becomes exactly

   \displaystyle
   \sqrt[3]{\frac{1}{a}\,\frac{2}{a+b}\,\frac{3}{a+b+c} }\,
     \bigl(a + \sqrt[3]{ab\,(a+b)/2} + \sqrt[3]{abc}\bigr)
   \;\le\; 3.

Rearranging, we obtain

   \displaystyle a + \sqrt[3]{ab\,(a+b)/2} + \sqrt[3]{abc} \;
   \le\;
   3\,\sqrt[3]{a\,(a+b)/2\,(a+b+c)/3},

which is precisely (3) with C=3.  Combining with Step 1, we conclude that (2) holds with the choice C=3.

Step 4.  Sharpness and conclusion.

Equality in each application of AM–GM requires all the entries in the corresponding triple to be equal.  Tracing back, one sees that equality throughout forces

   a = b = c.

In that case both sides of the original inequality in display (1) become

   (a + a + a) / C = 3a/C
   \quad and \quad
   \sqrt[3]{a\,(a+a)/2\,(a+a+a)/3} = \sqrt[3]{a\cdot a\cdot a} = a.

Thus equality in (1) reads 3a/C = a, i.e. C=3.  Hence C=3 is the smallest constant for which the inequality holds for all positive a,b,c.

Therefore, the answer is $C=3$.
