# Problem Entry

## Problem Type
bound

## Problem
Let $x, y, z \in \mathbb{R}^{+}$ such that $xyz \geq xy + yz + zx$. Find the largest constant $C$ such that the following inequality holds for all $x, y, z$ satisfying the given constraint:
$$
xyz \geq C(x + y + z)
$$

## Current Solution
Letting $\frac{1}{x}=a, \frac{1}{y}=b, \frac{1}{z}=c$, the initial condition $x y z \geq x y+y z+z x$ becomes
$$
\begin{equation*}
a+b+c \leq 1 \tag{1}
\end{equation*}
$$

We need to show that
$$
\begin{equation*}
x y z \geq 3(x+y+z) \quad \Leftrightarrow \quad 3(a b+b c+c a) \leq 1 \tag{2}
\end{equation*}
$$

Clearly
$$
\begin{equation*}
(a+b+c)^{2} \geq 3(a b+b c+c a) \tag{3}
\end{equation*}
$$

Now from (1) and (3) we obtain (2).

Equality holds when $a = b = c = \frac{1}{3}$, i.e., $x = y = z = 3$. In this case, $xyz = 27$ and $x + y + z = 9$, so $xyz = 3(x + y + z)$. Thus, the maximum value of $C$ for which the inequality always holds is $C = 3$.

Therefore, the answer is $C = 3$.

## Expected Answer
$C = 3$

## Enhanced Solution
We wish to find the largest constant C such that for all positive real x,y,z satisfying

    (I)    xyz \ge xy + yz + zx,

the following holds:

    (II)   xyz \ge C\,(x+y+z). 

Our strategy is to make the same substitution as in the original solution, then carry out every step with full justification.

Step 1.  Introduce new variables.
Let a = 1/x,
    b = 1/y,
    c = 1/z.
Since x,y,z are positive, so are a,b,c.  We then have

    xy = (1/a)(1/b) = 1/(ab),
    yz = 1/(bc),
    zx = 1/(ca),
    xyz = 1/(abc).

Step 2.  Rewrite condition (I) in terms of a,b,c.
From xyz \ge xy + yz + zx, divide both sides by the positive quantity xyz = 1/(abc).  Concretely,

    xyz \ge xy + yz + zx
    \iff 1/(abc) \ge 1/(ab) + 1/(bc) + 1/(ca)
    \iff 1 \ge c + a + b
    \iff a + b + c \le 1.

Thus the constraint (I) is equivalent to

    (1)    a + b + c \le 1,
with a,b,c > 0.

Step 3.  Rewrite the target inequality (II).
We want

    xyz \ge C(x+y+z)
    \iff 1/(abc) \ge C\bigl((1/a)+(1/b)+(1/c)\bigr)
    \iff 1/(abc) \ge C\,\frac{bc+ca+ab}{abc}
    \iff 1 \ge C\,(ab + bc + ca)
    \iff ab + bc + ca \le 1/C.

Thus to ensure (II) for all admissible a,b,c we must have

    (2)    ab + bc + ca \le 1/C
whenever a + b + c \le 1.

Step 4.  Find the maximal possible value of ab + bc + ca subject to a+b+c \le 1, a,b,c>0.
By the well-known inequality between the arithmetic mean of squares and the square of the arithmetic mean, or simply by expanding,

    (a + b + c)^{2}
    = a^{2} + b^{2} + c^{2} + 2(ab + bc + ca)
    \ge 3(ab + bc + ca),

since a^{2}+b^{2}+c^{2} \ge ab+bc+ca.  Therefore,

    ab + bc + ca \le \frac{(a+b+c)^{2}}{3} \le \frac{1^{2}}{3} = \frac{1}{3},

where in the last step we used a+b+c \le 1.  Thus the maximum possible value of ab+bc+ca under our constraint is 1/3.

Step 5.  Determine C.
From (2) we require ab+bc+ca \le 1/C for all admissible a,b,c.  Since the worst-case (largest) value of ab+bc+ca is 1/3, we must have

    1/3 \le 1/C   \quad\Longrightarrow\quad   C \le 3.

Conversely, setting C = 3 we see that

    ab + bc + ca \le 1/3   \implies   3(ab + bc + ca) \le 1,

which exactly recovers 1 \ge C(ab+bc+ca).  Hence C = 3 is the largest constant for which the inequality always holds.

Step 6.  Check the equality case.
Equality in the chaining

    (a+b+c)^{2} \ge 3(ab+bc+ca) \quad\text{and}\quad a+b+c \le 1

occurs exactly when a = b = c = 1/3.  This corresponds to x = y = z = 3, for which xyz = 27 and x+y+z = 9, indeed giving 27 = 3Â·9.  Thus the bound C=3 is sharp.

Therefore, the largest constant C satisfying xyz \ge C(x+y+z) under xyz \ge xy + yz + zx is

The answer is $C=3$.  
