# Problem Entry

## Problem Type
bound

## Problem
Let $x, y \geq 0$ be real numbers such that $x + y = 2$. Find the minimal constant $C$ such that the following inequality holds for all $x, y$ satisfying the given constraint:
$$
x^{2} y^{2}\left(x^{2}+y^{2}\right) \leq C
$$

## Current Solution
We homogenize as follows
$$
\begin{equation*}
x^{2} y^{2}\left(x^{2}+y^{2}\right) \leq 2\left(\frac{x+y}{2}\right)^{6} \quad \Leftrightarrow \quad(x+y)^{6} \geq 32 x^{2} y^{2}\left(x^{2}+y^{2}\right) \tag{1}
\end{equation*}
$$

If $x y=0$ then the given inequality clearly holds.
Therefore let us assume that $x y \neq 0$.
Since (1)) is homogenous, we may normalize with $x y=1$.
So $y=\frac{1}{x}$, and inequality (1) becomes
$$
\begin{equation*}
\left(x+\frac{1}{x}\right)^{6} \geq 32\left(x^{2}+\frac{1}{x^{2}}\right) \tag{2}
\end{equation*}
$$

Let $t=\left(x+\frac{1}{x}\right)^{2}$, then clearly $x^{2}+\frac{1}{x^{2}}=t-2$.
Therefore (2) is equivalent to
$$
t^{3} \geq 32(t-2)
$$

Clearly $t=\left(x+\frac{1}{x}\right)^{2} \geq 2^{2}=4$.
Let us consider the function $f(t)=t^{3}-32(t-2)$ on the interval $[4, \infty)$.
Since $f^{\prime}(t)=3 t^{2}-32$ we have that $f^{\prime}(t) \geq 0$ for all $t \geq \sqrt{\frac{32}{3}}>4$, i.e. it follows that $f$ is increasing on $[4, \infty)$, which implies that
$$
f(t) \geq f(4)=0
$$
$$
\begin{aligned}
& \Leftrightarrow \quad t^{3}-32(t-2) \geq 0 \\
& \Leftrightarrow \quad t^{3} \geq 32(t-2), \quad \text { for all } t \in[4, \infty)
\end{aligned}
$$
as required.

Equality holds when $x = y = 1$, since $x + y = 2$ and $x^2 y^2 (x^2 + y^2) = 1^2 \cdot 1^2 (1^2 + 1^2) = 2$. This gives the maximum value of the expression, so $C = 2$ is minimal such that the inequality always holds.

Therefore, the answer is $C = 2$.

## Expected Answer
$C = 2$

## Enhanced Solution
Enhanced Solution:

We wish to determine the smallest constant C such that for all nonnegative real x,y satisfying x+y=2,

    x^2 y^2 (x^2 + y^2) ≤ C.

Our goal is therefore to compute the maximum value of the homogeneous expression

    F(x,y) := x^2 y^2 (x^2 + y^2)

on the line segment { (x,y): x ≥ 0, y ≥ 0, x+y=2 } and to show that this maximum equals 2.

1. Homogenization and reduction to an inequality in one symmetric sum
------------------------------------------------------------
Observe that both sides of the proposed inequality

    x^2 y^2 (x^2 + y^2) ≤ C

are homogeneous of total degree 6 in (x,y).  In particular, if we can prove the sharper homogeneous inequality

    (x+y)^6 ≥ 32 · x^2 y^2 (x^2 + y^2)

for all x,y ≥0, then upon imposing the constraint x+y=2 this yields

    2^6 = (x+y)^6 ≥ 32·x^2 y^2 (x^2 + y^2)
    ⇒ x^2 y^2 (x^2 + y^2) ≤ 64/32 = 2.

Hence establishing

    (x+y)^6 ≥ 32 x^2 y^2 (x^2 + y^2)   (⋆)

is sufficient to conclude that the maximal value of x^2 y^2 (x^2 + y^2) under x+y=2 is at most 2.

2. Proving inequality (⋆) via normalization of xy
---------------------------------------------
The inequality (⋆) is itself homogeneous of degree 6.  Therefore we may, without loss of generality, impose the additional normalization xy = 1, at the cost of reducing the problem to one real variable.  Concretely, set

    xy = 1,    t := x + y.

By the AM–GM inequality we have t = x+y ≥ 2√{xy} = 2, so t ∈ [2, ∞).  Moreover,

    x^2 + y^2 = (x+y)^2 − 2xy = t^2 − 2.

Substituting xy=1 and x^2+y^2=t^2−2 into (⋆) gives the one‐variable inequality

    t^6 ≥ 32·(1)^2·(t^2 − 2)
    ⇔ t^6 ≥ 32(t^2 − 2).

3. Further reduction via a single variable
-----------------------------------
Introduce the auxiliary variable

    τ := t^2,   so   τ ∈ [4, ∞).

Then t^6 = (t^2)^3 = τ^3, and the inequality becomes

    τ^3 ≥ 32(τ − 2),    for all τ ≥ 4.

Define the function

    f(τ) := τ^3 − 32(τ − 2)  = τ^3 − 32τ + 64.

We will show f(τ) ≥ 0 on [4,∞).  Compute its derivative:

    f′(τ) = 3τ^2 − 32.

On the interval τ ≥ 4 one has

    3τ^2 ≥ 3·4^2 = 48 > 32,

so f′(τ) ≥ 48 − 32 = 16 > 0 for all τ ≥ 4.  Hence f is strictly increasing on [4,∞).  Therefore for all τ ≥ 4,

    f(τ) ≥ f(4) = 4^3 − 32·4 + 64 = 64 − 128 + 64 = 0.

This establishes τ^3 ≥ 32(τ − 2), i.e. the desired inequality in the single variable τ, and thus completes the proof of (⋆).

4. Conclusion and attainment of equality
--------------------------------
Combining the above, we have shown

    (x+y)^6 ≥ 32·x^2 y^2 (x^2 + y^2)

for all x,y ≥0.  Under the constraint x+y=2, this gives

    x^2 y^2 (x^2 + y^2) ≤ 2.

Hence the minimal constant C for which the original inequality holds is C=2.

Finally, equality in all steps occurs exactly when

    (i) xy = 1  and x+y = t = 2 ⇒ x = y = 1,

which indeed yields x+y=2 and x^2 y^2 (x^2+y^2) = 1·1·(1+1)=2.

Thus the maximum of x^2 y^2 (x^2 + y^2) on the domain is 2, and no smaller C can work.

The answer is $C=2$
