# Problem Entry

## Problem Type
bound

## Problem
Let $n > 2$ and let $x_{1}, x_{2}, \ldots, x_{n} > 0$ such that $\sum_{i=1}^{n} x_i = 1$. Find the maximal  constant $C$ such that the following inequality holds for all $x_{i}$:
$$
\prod_{i=1}^{n}\left(1+\frac{1}{x_{i}}\right) \geq C  \prod_{i=1}^{n}\left(\frac{n-x_{i}}{1-x_{i}}\right).
$$

## Current Solution
The most natural idea is to use the fact that

$$
\frac{n-x_{i}}{1-x_{i}}=1+\frac{n-1}{x_{1}+x_{2}+\cdots+x_{i-1}+x_{i+1}+\cdots+x_{n}}
$$

Thus, we have

$$
\prod_{i=1}^{n}\left(\frac{n-x_{i}}{1-x_{i}}\right) \leq \prod_{i=1}^{n}\left(1+\frac{1}{\sqrt[n-1]{x_{1} x_{2} \ldots x_{i-1} x_{i+1} \ldots x_{n}}}\right)
$$

and we have to prove the inequality

$$
\prod_{i=1}^{n}\left(1+\frac{1}{x_{i}}\right) \geq \prod_{i=1}^{n}\left(1+\frac{1}{\sqrt[n-1]{x_{1} x_{2} \ldots x_{i-1} x_{i+1} \ldots x_{n}}}\right)
$$

But this one is not very hard, because it follows immediately by multiplying the inequalities

$$
\prod_{j \neq i}\left(1+\frac{1}{x_{j}}\right) \geq\left(1+\sqrt[n-1]{\prod_{j \neq i} \frac{1}{x_{j}}}\right)^{n-1}
$$

obtained from Huygens Inequality.,We will prove even more, that

$$
\prod_{i=1}^{n}\left(1+\frac{1}{x_{i}}\right) \geq\left(\frac{n^{2}-1}{n}\right)^{n} \cdot \prod_{i=1}^{n} \frac{1}{1-x_{i}}
$$

It is clear that this inequality is stronger than the initial one. First, let us prove that

$$
\prod_{i=1}^{n} \frac{1+x_{i}}{1-x_{i}} \geq\left(\frac{n+1}{n-1}\right)^{n}
$$

This follows from Jensen's Inequality for the convex function $f(x)=\ln (1+x)-$ $\ln (1-x)$. So, it suffices to prove that

$$
\frac{\left(\frac{n+1}{n-1}\right)^{n}}{\prod_{i=1}^{n} x_{i}} \cdot \prod_{i=1}^{n}\left(1-x_{i}\right)^{2} \geq\left(\frac{n^{2}-1}{n}\right)^{n}
$$

But a quick look shows that this is exactly the inequality proved in the solution of the problem 121.

Equality holds when $x_1 = x_2 = \cdots = x_n = \frac{1}{n}$, since then all terms are equal and the AM-GM and Jensen inequalities used above become equalities. This gives the minimum value of $C$ for which the inequality always holds, so the maximal constant is $C = 1$.

Therefore, the answer is $C = 1$. 

## Expected Answer
$C =1$

## Enhanced Solution
Enhanced Solution:

We wish to determine the largest constant C such that for every integer n>2 and every choice of positive real numbers x_{1},x_{2},…,x_{n} satisfying \(x_{1}+x_{2}+\cdots+x_{n}=1\), the following inequality holds:

  \[   \prod_{i=1}^{n}\Bigl(1+\frac1{x_{i}}\Bigr) \;\ge\; C \;\prod_{i=1}^{n} \frac{n - x_{i}}{1 - x_{i}}.  \]

Our goal is to show that the maximal such constant is C=1.  We proceed in two main steps, following the original solution’s strategy but with full details and rigorous justifications.

1.  Reduction via AM–GM to a simpler product inequality
--------------------------------------------------------

Observe first that for each index i,

  \[
    \frac{n - x_i}{1 - x_i}
    = 1 + \frac{n - 1}{\,1 - x_i\,}
    = 1 + \frac{n - 1}{x_{1} + x_{2} + \cdots + x_{i-1} + x_{i+1} + \cdots + x_{n}}.
  \]

Since the sum of the n–1 terms \(x_{j}\) with \(j\neq i\) is positive, we may apply the AM–GM inequality to these \(n-1\) terms to obtain

  \[
    x_{1} + \cdots + x_{i-1} + x_{i+1} + \cdots + x_{n}
    \;\ge\; (n-1)\sqrt[n-1]{x_{1}x_{2}\cdots x_{i-1}\,x_{i+1}\cdots x_{n}}.
  \]

Hence

  \[
    \frac{n - x_i}{1 - x_i}
    \le
    1 + \frac{n - 1}{(n-1)\sqrt[n-1]{x_{1}\cdots x_{i-1}\,x_{i+1}\cdots x_{n}}}
    = 1 + \frac{1}{\sqrt[n-1]{\prod_{j\neq i}x_{j}}}.
  \]

Taking the product over i=1,2,…,n yields

  \[
    \prod_{i=1}^{n} \frac{n - x_i}{1 - x_i}
    \le
    \prod_{i=1}^{n} \Bigl(1 + \frac{1}{\sqrt[n-1]{\prod_{j\neq i}x_{j}}}\Bigr).
  \]

Thus it suffices to prove the stronger inequality

  \[
    \prod_{i=1}^{n} \Bigl(1 + \tfrac1{x_{i}}\Bigr)
    \;\ge\;
    \prod_{i=1}^{n} \Bigl(1 + \tfrac{1}{\sqrt[n-1]{\prod_{j\neq i}x_{j}}}\Bigr).
  \]

But this latter product–product comparison follows neatly by applying the following known fact (sometimes called a Huygens–type inequality):

  For any integer m≥1 and any positive numbers a_{1},…,a_{m},
  \[
    (1 + a_{1})(1 + a_{2})\cdots(1 + a_{m})
    \;\ge\;
    \bigl(1 + (a_{1}a_{2}\cdots a_{m})^{1/m}\bigr)^{m}.
  \]

Fix an index i and set m=n−1 and a_{j}=1/x_{j} for j≠i.  Then

  \[
    \prod_{j\neq i}\Bigl(1+\tfrac1{x_{j}}\Bigr)
    \ge
    \Bigl(1 + \bigl(\prod_{j\neq i} \tfrac1{x_{j}}\bigr)^{1/(n-1)}\Bigr)^{n-1}.
  \]

Now multiply these n inequalities as i runs from 1 to n.  On the left we get

  \[
    \prod_{i=1}^{n}\prod_{j\neq i}\Bigl(1+\tfrac1{x_{j}}\Bigr)
    = \prod_{j=1}^{n} \Bigl(1+\tfrac1{x_{j}}\Bigr)^{\,(n-1)}
  \]

while on the right we obtain

  \[
    \prod_{i=1}^{n}\Bigl(1 + (\textstyle\prod_{j\neq i}1/x_{j})^{1/(n-1)}\Bigr)^{n-1}
    = \biggl(\prod_{i=1}^{n}\Bigl(1 + (\prod_{j\neq i}1/x_{j})^{1/(n-1)}\Bigr)\biggr)^{n-1}.
  \]

Hence

  \[
    \Bigl(\prod_{j=1}^{n}(1+1/x_{j})\Bigr)^{n-1}
    \ge
    \Bigl(\prod_{i=1}^{n}(1 + (\prod_{j\neq i}1/x_{j})^{1/(n-1)})\Bigr)^{n-1}.
  \]

Taking the (n−1)th root of both sides yields exactly

  \[
    \prod_{i=1}^{n}\Bigl(1+\tfrac1{x_{i}}\Bigr)
    \;\ge\;
    \prod_{i=1}^{n}\Bigl(1 + \tfrac{1}{\sqrt[n-1]{\prod_{j\neq i}x_{j}}}\Bigr),
  \]

as required.  This establishes the desired inequality with the constant C=1.

2.  Verification of sharpness (equality case)
----------------------------------------------

All of the inequalities above (the AM–GM step and the product–product step) become equalities precisely when

  \[
    x_{1} = x_{2} = \cdots = x_{n} = \tfrac1{n}
  \]

because in each application of AM–GM or the Huygens–type inequality, equality holds exactly when the underlying positive quantities are all equal.  Substituting \(x_{i}=1/n\) into both sides shows that no larger constant C can satisfy the inequality for every choice of the x_{i}.  Hence the maximal constant is C=1.

Conclusion:

The answer is $C=1$.
