# Problem Entry

## Problem Type
bound

## Problem
Let $a, b, c > 0$ such that $abc = 1$. Find the maximal constant $C$ such that the following inequality holds for all $a, b, c$ satisfying the given constraint:
$$
(a+b)(b+c)(c+a) \geq C(a+b+c-1)
$$

## Current Solution
We will use the fact that $(a+b)(b+c)(c+a) \geq \frac{8}{9}(a+b+c)(a b+b c+c a)$. So, it is enough to prove that $\frac{2}{9}(a b+b c+c a)+\frac{1}{a+b+c} \geq 1$. Using the AM-GM Inequality, we can write

$$
\frac{2}{9}(a b+b c+c a)+\frac{1}{a+b+c} \geq 3 \sqrt[3]{\frac{(a b+b c+c a)^{2}}{81(a+b+c)}} \geq 1
$$

because

$$
(a b+b c+c a)^{2} \geq 3 a b c(a+b+c)=3(a+b+c)
$$

Equality holds when $a = b = c = 1$, since then $abc = 1$ and $(a+b)(b+c)(c+a) = 8$, $a+b+c-1 = 2$, so $C = 4$ is achieved. This gives the maximum value of $C$ for which the inequality always holds.

Therefore, the answer is $C = 4$.

## Expected Answer
$C = 4$

## Enhanced Solution
**Enhanced Solution**

Let us denote
  S = a + b + c,
  P = ab + bc + ca,
and recall that abc = 1.  Our goal is to find the largest constant C such that
  (a + b)(b + c)(c + a) \ge C\,(a + b + c - 1)
holds for all positive a,b,c with abc=1.

**Step 1.  Rewrite the left–hand side in terms of S and P.**
There is a well–known symmetric identity:
  (a + b)(b + c)(c + a)
  = (a + b + c)(ab + bc + ca) \;-
    abc
  = S\,P \, -\,1.   \quad(\text{since }abc=1).

Hence the inequality becomes
  S\,P - 1 \ge C\,(S - 1)
\quad\Longleftrightarrow\quad
  S\,P \ge C\,(S - 1) + 1 = C S - C + 1.

Dividing both sides by the positive quantity S, we get the equivalent form
  P \ge C \;-
      {C - 1\over S}
\quad\Longleftrightarrow\quad
  P + {C - 1\over S} \ge C.

Thus to prove the original inequality with a given C, it suffices to show
  P + \frac{C - 1}{S} \ge C
for all a,b,c>0 with abc=1.

**Step 2.  Obtain a preliminary estimate on (a+b)(b+c)(c+a).**
By the AM–GM inequality on the two positive numbers S and P,
  S \ge 3\,(abc)^{1/3} = 3,
  P \ge 3\,(abc)^{2/3} = 3.
Hence
  S\,P \ge 9,
and so from the identity above,
  (a+b)(b+c)(c+a) = S\,P - 1 \ge S\,P - \tfrac{1}{9}S\,P
    = \frac{8}{9}\,S\,P.
In other words, for all a,b,c>0 with abc=1 we have
  (a+b)(b+c)(c+a) \ge \frac{8}{9}\,S\,P.

**Step 3.  Specialize to C=4 and reduce to a single-variable inequality.**
We claim the maximal such C is 4.  Substitute C=4 into
  \frac{8}{9}\,S\,P \ge C\,(S - 1)
and divide by S>0 to obtain the equivalent
  \frac{8}{9}\,P \ge 4\Bigl(1 - \frac{1}{S}\Bigr)
\quad\Longleftrightarrow\quad
  \frac{2}{9}\,P \ge 1 - \frac{1}{S}
\quad\Longleftrightarrow\quad
  \frac{2}{9}\,P + \frac{1}{S} \ge 1.

Thus it remains to prove the inequality
   (★)\quad \frac{2}{9}(ab+bc+ca) + \frac{1}{a+b+c} \ge 1
for all a,b,c>0 with abc=1.

**Step 4.  Prove (★) by AM–GM and a classical symmetric bound.**
Write the left–hand side of (★) as a sum of three nonnegative terms:
  LHS = \underbrace{\tfrac{1}{9}P}_{T_1}
        + \underbrace{\tfrac{1}{9}P}_{T_2}
        + \underbrace{\tfrac{1}{a+b+c}}_{T_3}.
By the AM–GM inequality on the three terms T₁, T₂, T₃,
  \frac{T_1 + T_2 + T_3}{3}
  \ge \sqrt[3]{T_1\,T_2\,T_3}
  = \sqrt[3]{\frac{P}{9} \cdot \frac{P}{9} \cdot \frac{1}{S}}
  = \sqrt[3]{\frac{P^2}{81\,S}}.
Hence
  LHS \ge 3 \sqrt[3]{\frac{P^2}{81\,S}}.
It will suffice to show
  3\sqrt[3]{\frac{P^2}{81\,S}} \ge 1
\quad\Longleftrightarrow\quad
  \frac{P^2}{81\,S} \ge \frac{1}{27}
\quad\Longleftrightarrow\quad
  P^2 \ge 3\,S.

Finally, since abc=1, another well–known symmetric inequality gives
  (ab + bc + ca)^2 \ge 3\,abc\,(a+b+c) = 3S.
Thus indeed P^2 \ge 3S, and all steps are reversible under equality conditions.

**Step 5.  Check equality and conclude.**
Every inequality above becomes an equality exactly when
  a = b = c = 1
(it forces S=3, P=3).  In particular, at a=b=c=1 we have
  (a+b)(b+c)(c+a) = 8,
  a+b+c-1 = 2,
and so 8 = 4·2, showing C=4 is attained.  Since we have proved the chain of implications
  (a+b)(b+c)(c+a) ≥ \tfrac{8}{9}SP ≥ 4(S-1)  
for all a,b,c>0 with abc=1, and equality does occur at a=b=c=1, it follows that 4 is the maximal constant.

Therefore, the answer is $C=4$.
