# Problem Entry

## Problem Type
bound

## Problem
Let $a, b, c \in (-1, 1)$ be real numbers such that $a b + b c + a c = 1$. Find the largest constant $C$ such that the following inequality holds for all $a, b, c$ satisfying the given constraint:
$$
C \sqrt[3]{\left(1-a^{2}\right)\left(1-b^{2}\right)\left(1-c^{2}\right)} \leq 1 + (a + b + c)^2
$$

## Current Solution
Since $a, b, c \in(-1,1)$ we have $1-a^{2}, 1-b^{2}, 1-c^{2}>0$.
By $A M \geq G M$ we get
$$
\begin{aligned}
6 \sqrt[3]{\left(1-a^{2}\right)\left(1-b^{2}\right)\left(1-c^{2}\right)} & =2 \cdot 3 \sqrt[3]{\left(1-a^{2}\right)\left(1-b^{2}\right)\left(1-c^{2}\right)} \\
& \leq 2\left(1-a^{2}+1-b^{2}+1-c^{2}\right) \\
& =2\left(3-\left(a^{2}+b^{2}+c^{2}\right)\right) \\
& =6-2\left(a^{2}+b^{2}+c^{2}\right)
\end{aligned}
$$

We'll show that
$$
6-2\left(a^{2}+b^{2}+c^{2}\right) \leq 1+(a+b+c)^{2}
$$

This inequality is equivalent to
$$
6-2\left(a^{2}+b^{2}+c^{2}\right) \leq 1+a^{2}+b^{2}+c^{2}+2
$$
i.e.
$$
3 \leq 3\left(a^{2}+b^{2}+c^{2}\right)
$$
i.e.
$$
a^{2}+b^{2}+c^{2} \geq 1
$$
which is true since $a^{2}+b^{2}+c^{2} \geq a b+b c+a c=1$.

Equality holds when $a = b = c = \pm \frac{1}{\sqrt{3}}$, since then $ab + bc + ca = 1$ and $a^2 + b^2 + c^2 = 1$. In this case, the inequality becomes equality, so $C = 6$ is the largest possible value.

Therefore, the answer is $C = 6$.

## Expected Answer
$C = 6$

## Enhanced Solution
We wish to determine the largest constant C such that for all real a,b,c∈(−1,1) satisfying ab+bc+ca=1 the inequality

  C⋅³√{(1−a²)(1−b²)(1−c²)}  ≤  1 + (a+b+c)²

holds.  We will show in a step‐by‐step fashion that C=6 is the maximal value for which this inequality is valid.

1.  Positivity of the cubic root argument

   Since each of a,b,c lies strictly between −1 and 1, we have 1−a²>0, 1−b²>0, 1−c²>0.  Hence the product

     (1−a²)(1−b²)(1−c²)

   is strictly positive, and the real cube root ³√{(1−a²)(1−b²)(1−c²)} is well‐defined and positive.

2.  Applying the Arithmetic Mean—Geometric Mean inequality

   For any three nonnegative real numbers X,Y,Z the AM–GM inequality states

     (X+Y+Z)/3  ≥  (XYZ)^{1/3},

   with equality precisely when X=Y=Z.  We set

     X = 1−a²,   Y = 1−b²,   Z = 1−c².

   Then

     (1−a²)+(1−b²)+(1−c²)   ≥   3⋅³√{(1−a²)(1−b²)(1−c²)}.

   Multiplying both sides by 2 gives

     2[(1−a²)+(1−b²)+(1−c²)]  ≥  6⋅³√{(1−a²)(1−b²)(1−c²)}.

   Hence

     6⋅³√{(1−a²)(1−b²)(1−c²)}  ≤  2[3 − (a²+b²+c²)]  = 6 − 2(a²+b²+c²).

3.  Comparing with the right–hand side

   We will verify that

     6 − 2(a²+b²+c²)  ≤  1 + (a+b+c)².

   Rearrange the desired inequality as follows:

     6 − 2(a²+b²+c²)  ≤  1 + a² + b² + c² + 2(ab+bc+ca)

   (since (a+b+c)² = a²+b²+c² + 2(ab+bc+ca)).  Using the given constraint ab+bc+ca=1, the right‐hand side becomes

     1 + a² + b² + c² + 2⋅1  =  3 + (a² + b² + c²).

   Thus the inequality to prove is

     6 − 2(a²+b²+c²)  ≤  3 + (a²+b²+c²),

   or equivalently

     6 − 3  ≤  3(a²+b²+c²),

     3  ≤  3(a²+b²+c²),

     1  ≤  a² + b² + c².

4.  Justification of a²+b²+c² ≥ 1

   A well‐known identity relates the sums of squares and pairwise products:

     a² + b² + c² − (ab + bc + ca)
       = ½[(a−b)² + (b−c)² + (c−a)²]
       ≥  0.

   Since ab+bc+ca=1 by hypothesis, it follows that

     a² + b² + c²  ≥  ab + bc + ca  =  1.

   Therefore the inequality 1 ≤ a²+b²+c² is indeed valid for all admissible (a,b,c).

5.  Conclusion for C=6

   Combining steps 2 and 3, we deduce for C=6:

     6⋅³√{(1−a²)(1−b²)(1−c²)}  ≤  6 − 2(a²+b²+c²)  ≤  1 + (a+b+c)².

   Hence the original inequality holds for C=6.

6.  Sharpness of C=6 (equality case)

   Equality in the chain of inequalities requires simultaneously:
   •  In AM–GM: 1−a² = 1−b² = 1−c²,  i.e. |a|=|b|=|c|.
   •  In the rearrangement a²+b²+c² = ab+bc+ca =1.

   The choice a=b=c=1/√3 (or all three equal to −1/√3) satisfies both requirements:

     ab+bc+ca = 3⋅(1/√3)² = 1,    a²+b²+c² = 3⋅(1/3) =1,

   and then each of the inequalities above becomes an equality.  This shows that one cannot increase C beyond 6 without violating the desired inequality.

Therefore, the largest constant for which

  C⋅³√{(1−a²)(1−b²)(1−c²)}  ≤  1 + (a+b+c)²

holds under the constraint ab+bc+ca=1 is

The answer is $C=6$.  
