# Problem Entry

## Problem Type
bound

## Problem
Let $x, y, z > 0$ satisfy the condition $x + y + z = xyz$. Find the maximal constant $C$ such that the following inequality holds for all $x, y, z$ satisfying the given condition:
$$
xy + xz + yz \geq C + \sqrt{x^2 + 1} + \sqrt{y^2 + 1} + \sqrt{z^2 + 1}
$$

## Current Solution
Another improvement is as follows. Start from

$$
\frac{1}{x^{2}}+\frac{1}{y^{2}}+\frac{1}{z^{2}} \geq \frac{1}{x y}+\frac{1}{x z}+\frac{1}{y z}=1 \Rightarrow x^{2} y^{2}+x^{2} z^{2}+y^{2} z^{2} \geq x^{2} y^{2} z^{2}
$$

which is equivalent to

$$
(x y+x z+y z)^{2} \geq 2 x y z(x+y+z)+x^{2} y^{2} z^{2}=3(x+y+z)^{2}
$$

Further on,

$$
\begin{aligned}
& (x y+x z+y z-3)^{2}=(x y+x z+y z)^{2}-6(x y+x z+y z)+9 \geq \\
& \geq 3(x+y+z)^{2}-6(x y+x z+y z)+9=3\left(x^{2}+y^{2}+z^{2}\right)+9
\end{aligned}
$$

so that

$$
x y+x z+y z \geq 3+\sqrt{3\left(x^{2}+y^{2}+z^{2}\right)+9}
$$

But

$$
\sqrt{3\left(x^{2}+y^{2}+z^{2}\right)+9} \geq \sqrt{x^{2}+1}+\sqrt{y^{2}+1}+\sqrt{z^{2}+1}
$$

is a consequence of the Cauchy-Schwarz Inequality and we have a second improvement and proof for the desired inequality:

$$
\begin{aligned}
x y+x z+y z & \geq 3+\sqrt{3\left(x^{2}+y^{2}+z^{2}\right)+9} \geq \\
& \geq 3+\sqrt{x^{2}+1}+\sqrt{y^{2}+1}+\sqrt{z^{2}+1}
\end{aligned}
$$

Equality holds when $x = y = z = \sqrt{3}$, since then $x + y + z = 3\sqrt{3}$ and $xyz = (\sqrt{3})^3 = 3\sqrt{3}$, so the condition is satisfied. In this case, $xy + xz + yz = 3 \cdot 3 = 9$ and $\sqrt{x^2+1} = \sqrt{3+1} = 2$ for each variable, so $C = 9 - 3 \times 2 = 3$. This gives the minimum value of $xy + xz + yz - (\sqrt{x^2+1} + \sqrt{y^2+1} + \sqrt{z^2+1})$, so the maximal constant $C$ is $3$.

Therefore, the answer is $C = 3$. 

## Expected Answer
$C = 3$

## Enhanced Solution
We wish to show that for all positive real x,y,z satisfying

  x + y + z = x y z,

the following inequality holds with the largest possible constant C:

  x y + x z + y z \ge C + √(x²+1) + √(y²+1) + √(z²+1).

We shall prove step by step that C=3 is both valid and maximal.

1.  **From the condition to a symmetric quadratic bound.**
    Since x,y,z>0, by the AM–GM inequality applied to each pair we have
      1 / x² + 1 / y² ≥ 2 / (x y),
      1 / x² + 1 / z² ≥ 2 / (x z),
      1 / y² + 1 / z² ≥ 2 / (y z).
    Adding these three inequalities gives
      2 (1/x² + 1/y² + 1/z²) ≥ 2 (1/(xy) + 1/(xz) + 1/(yz)),
    so
      1/x² + 1/y² + 1/z² ≥ 1/(xy) + 1/(xz) + 1/(yz).
    But by the given condition x+y+z=xyz we have
      1/(xy) + 1/(xz) + 1/(yz)
        = (z + y + x) / (x y z)
        = (x+y+z)/(xyz)
        = 1.
    Therefore
      1/x² + 1/y² + 1/z² ≥ 1.

2.  **Translating into a bound on x²y² + y²z² + z²x².**
    Multiply both sides of
      1/x² + 1/y² + 1/z² ≥ 1
    by x² y² z² (which is positive).  This yields
      y² z² + x² z² + x² y² ≥ x² y² z².

3.  **Passing to (xy + yz + zx)².**
    Expand the square of the sum:
      (xy + yz + zx)²
        = x²y² + y²z² + z²x²   +  2 x y z (x + y + z).
    From the inequality in step 2 we replace x²y² + y²z² + z²x² by at least x²y²z², and use x+y+z=xyz, obtaining
      (xy+yz+zx)² ≥ x²y²z² + 2 x y z·(x+y+z)
                   = (xyz)² + 2(xyz)²
                   = 3 (xyz)²
                   = 3 (x+y+z)².

4.  **Shifting by 3 and extracting a square root.**
    Consider the nonnegative quantity
      (xy+yz+zx − 3)²
        = (xy+yz+zx)² − 6(xy+yz+zx) + 9.
    From step 3 we have (xy+yz+zx)² ≥ 3(x+y+z)², so
      (xy+yz+zx − 3)²
        ≥ 3(x+y+z)² − 6(xy+yz+zx) + 9.
    Rewrite the right–hand side as
      3[(x+y+z)² − 2(xy+yz+zx) + 3]
        = 3[x² + y² + z² + 3].
    Hence
      (xy+yz+zx − 3)² ≥ 3(x² + y² + z² + 3).
    Taking nonnegative square roots on both sides gives
      xy+yz+zx − 3 ≥ √[3(x² + y² + z² + 3)],
    or equivalently
      xy + yz + zx ≥ 3 + √[3(x² + y² + z² + 3)].

5.  **Comparing √[3(x²+y²+z²+3)] with √(x²+1)+√(y²+1)+√(z²+1).**
    We claim
      √[3(x²+y²+z²+3)] ≥ √(x²+1) + √(y²+1) + √(z²+1).
    Equivalently, squaring both sides (all terms positive) we must show
      3(x²+y²+z²+3)
        ≥ [√(x²+1) + √(y²+1) + √(z²+1)]²
        = (x²+1)+(y²+1)+(z²+1)
          + 2[√((x²+1)(y²+1)) + √((y²+1)(z²+1)) + √((z²+1)(x²+1))]
        = (x²+y²+z²+3)
          + 2∑_{sym} √((x²+1)(y²+1)).
    Rearranging, this is equivalent to
      2(x²+y²+z²+3) ≥ 2∑ √((x²+1)(y²+1))
    or
      x²+y²+z²+3 ≥ ∑ √((x²+1)(y²+1)).
    But by the AM–GM inequality for each pair (u,v) = (x²+1,y²+1) we have
      (x²+1)+(y²+1) ≥ 2√((x²+1)(y²+1)).
    Summing the three such inequalities for (x,y), (y,z), (z,x) gives exactly
      2(x²+y²+z²+3) ≥ 2∑ √((x²+1)(y²+1)),
    which completes the proof of this claim.

6.  **Conclusion.**
    Combining steps 4 and 5, we obtain
      xy + yz + zx
        ≥ 3 + √[3(x²+y²+z²+3)]
        ≥ 3 + [√(x²+1) + √(y²+1) + √(z²+1)],
    so the inequality holds with C = 3.

7.  **Optimality of C=3.**
    Equality throughout requires equality in each AM–GM step and in each square–root extraction.  This forces
      x = y = z,
    and from x + x + x = x·x·x we get 3x = x³, so x²=3 and x=√3.  Substituting, one checks
      xy+yz+zx = 3·3 = 9,
      √(x²+1) = √(3+1) = 2,
    hence
      xy+yz+zx − [√(x²+1)+√(y²+1)+√(z²+1)]
        = 9 − 3·2 = 3.
    Thus no larger C can satisfy the inequality for all admissible (x,y,z).

Therefore, the maximal constant is 3.

The answer is $C=3$.
