# Problem Entry

## Problem Type
bound

## Problem
Let $a, b, c \in \mathbb{R}^{+}$ with $a^{2}+b^{2}+c^{2}=3$. Determine the largest constant $C$ such that the following inequality holds for all $a, b, c$:
$$
\frac{a b}{c}+\frac{b c}{a}+\frac{c a}{b} \geq C.
$$

## Current Solution
The given inequality is equivalent to
$$
\begin{aligned}
& \left(\frac{a b}{c}+\frac{b c}{a}+\frac{c a}{b}\right)^{2} \geq 9 \\
& \quad \Leftrightarrow \quad \frac{a^{2} b^{2}}{c^{2}}+\frac{b^{2} c^{2}}{a^{2}}+\frac{c^{2} a^{2}}{b^{2}}+2\left(a^{2}+b^{2}+c^{2}\right) \geq 3\left(a^{2}+b^{2}+c^{2}\right)
\end{aligned}
$$
i.e.
$$
\frac{a^{2} b^{2}}{c^{2}}+\frac{b^{2} c^{2}}{a^{2}}+\frac{c^{2} a^{2}}{b^{2}} \geq a^{2}+b^{2}+c^{2}
$$

Furthermore, applying $A M \geq G M$ we get
$$
\frac{a^{2} b^{2}}{c^{2}}+\frac{b^{2} c^{2}}{a^{2}} \geq 2 b^{2}, \quad \frac{b^{2} c^{2}}{a^{2}}+\frac{c^{2} a^{2}}{b^{2}} \geq 2 c^{2}, \quad \frac{a^{2} b^{2}}{c^{2}}+\frac{c^{2} a^{2}}{b^{2}} \geq 2 a^{2}
$$

After adding these inequalities we obtain
$$
\frac{a^{2} b^{2}}{c^{2}}+\frac{b^{2} c^{2}}{a^{2}}+\frac{c^{2} a^{2}}{b^{2}} \geq a^{2}+b^{2}+c^{2}
$$
and we are done.

Equality holds when $a = b = c = 1$, since then $a^2 + b^2 + c^2 = 3$ and $\frac{ab}{c} + \frac{bc}{a} + \frac{ca}{b} = 3$. This gives the minimum value of the expression, so the largest constant $C$ for which the inequality always holds is $C = 3$.

Therefore, the answer is $C = 3$.

## Expected Answer
$C = 3$

## Enhanced Solution
We wish to find the greatest constant C such that for all positive real numbers a,b,c satisfying
a^2 + b^2 + c^2 = 3,
we have
    (ab)/c + (bc)/a + (ca)/b ≥ C.

Step 1.  Reformulate the problem in terms of a single expression S.  Define
    S := ab/c + bc/a + ca/b.
Since a,b,c>0, S>0, and it suffices to show S ≥ C.

Step 2.  Square S and expand.  Observe that
    S^2 = (ab/c + bc/a + ca/b)^2
        = (ab/c)^2 + (bc/a)^2 + (ca/b)^2
          + 2·[(ab/c)(bc/a) + (bc/a)(ca/b) + (ca/b)(ab/c)].
Next we simplify the mixed products:
    (ab/c)(bc/a) = b^2,
    (bc/a)(ca/b) = c^2,
    (ca/b)(ab/c) = a^2.
Hence
    S^2 = (a^2b^2/c^2 + b^2c^2/a^2 + c^2a^2/b^2) + 2(a^2 + b^2 + c^2).

Step 3.  Substitute the normalization a^2 + b^2 + c^2 = 3.  The previous line gives
    S^2 = (a^2b^2/c^2 + b^2c^2/a^2 + c^2a^2/b^2) + 2·3
        = (a^2b^2/c^2 + b^2c^2/a^2 + c^2a^2/b^2) + 6.
To prove S ≥ C, it suffices to prove S^2 ≥ C^2 (because S>0).  In particular, to show S ≥ 3 we will prove
    S^2 ≥ 9  ⇔  (a^2b^2/c^2 + b^2c^2/a^2 + c^2a^2/b^2) + 6 ≥ 9
               ⇔  a^2b^2/c^2 + b^2c^2/a^2 + c^2a^2/b^2 ≥ 3.
But since a^2 + b^2 + c^2 = 3, this is equivalent to
    a^2b^2/c^2 + b^2c^2/a^2 + c^2a^2/b^2 ≥ a^2 + b^2 + c^2.

Step 4.  Apply the AM–GM inequality in three pairwise fashions:
  1)  (a^2b^2/c^2) + (c^2a^2/b^2) ≥ 2·a^2,
  2)  (a^2b^2/c^2) + (b^2c^2/a^2) ≥ 2·b^2,
  3)  (b^2c^2/a^2) + (c^2a^2/b^2) ≥ 2·c^2.

Each follows from AM–GM: for example,
    (a^2b^2/c^2) + (c^2a^2/b^2) ≥ 2·√[(a^2b^2/c^2)(c^2a^2/b^2)]
                              = 2·a^2.

Step 5.  Add the three inequalities above:
    2·[(a^2b^2/c^2) + (b^2c^2/a^2) + (c^2a^2/b^2)] ≥ 2·(a^2 + b^2 + c^2).
Divide both sides by 2 to obtain exactly
    a^2b^2/c^2 + b^2c^2/a^2 + c^2a^2/b^2 ≥ a^2 + b^2 + c^2 = 3.
This completes the proof that S^2 ≥ 9, and since S>0, we conclude S ≥ 3.

Step 6.  Check when equality holds.  Each AM–GM step requires
a^2b^2/c^2 = c^2a^2/b^2 = b^2c^2/a^2, which force a = b = c.  Together
with a^2 + b^2 + c^2 = 3 we get a = b = c = 1, and then
    S = ab/c + bc/a + ca/b = 1·1/1 + 1·1/1 + 1·1/1 = 3.
Thus the minimal value of S over the given domain is 3, and hence the largest constant C for which
    ab/c + bc/a + ca/b ≥ C
always holds is C = 3.

The answer is $C=3$
