# Problem Entry

## Problem Type
bound

## Problem
Let $a_{1}, a_{2}, \ldots, a_{n}$ be positive real numbers such that $a_{1}+a_{2}+\cdots+a_{n}=1$. Find the largest constant $C$ such that the following inequality holds for all $a_{1}, a_{2}, \ldots, a_{n}$:
$$
\frac{a_{1}}{\sqrt{1-a_{1}}}+\frac{a_{2}}{\sqrt{1-a_{2}}}+\cdots+\frac{a_{n}}{\sqrt{1-a_{n}}} \geq C
$$

## Current Solution
Let us denote
$$
\begin{aligned}
& A=\frac{a_{1}}{\sqrt{1-a_{1}}}+\frac{a_{2}}{\sqrt{1-a_{2}}}+\cdots+\frac{a_{n}}{\sqrt{1-a_{n}}} \\
& B=a_{1}\left(1-a_{1}\right)+a_{2}\left(1-a_{2}\right)+\cdots+a_{n}\left(1-a_{n}\right)
\end{aligned}
$$

By Hölder's inequality we have
$$
\begin{equation*}
A^{2} B \geq\left(a_{1}+a_{2}+\cdots+a_{n}\right)^{3}=1 \tag{1}
\end{equation*}
$$

Applying $QM \geq AM$ we deduce
$$
\begin{equation*}
B=1-\left(a_{1}^{2}+a_{2}^{2}+\cdots+a_{n}^{2}\right) \leq 1-\frac{\left(a_{1}+a_{2}+\cdots+a_{n}\right)^{2}}{n}=\frac{n-1}{n} \tag{2}
\end{equation*}
$$

By (1) and (2) we obtain
$$
\frac{n-1}{n} \cdot A^{2} \geq A^{2} B \geq 1, \quad \text { i.e. } \quad A \geq \sqrt{\frac{n}{n-1}}
$$

Equality holds when $a_{1} = a_{2} = \cdots = a_{n} = \frac{1}{n}$, since then both Hölder's and QM-AM inequalities become equalities. This gives the minimum value of $A$, so $C = \sqrt{\frac{n}{n-1}}$ is the largest constant for which the inequality always holds.

Therefore, the answer is $C = \sqrt{\frac{n}{n-1}}$. 

## Expected Answer
$C = \sqrt{\frac{n}{n-1}}$

## Enhanced Solution
We wish to find the largest constant C such that for any positive reals a_{1},…,a_{n} with a_{1}+…+a_{n}=1, the following holds:  
  A := \sum_{i=1}^{n} \frac{a_{i}}{\sqrt{1-a_{i}}} \;\ge\; C.  
We keep exactly the same strategy as the original solution, but add full detail at each step.  

1.  Introduction of auxiliary sums  
   Define two expressions  
   \[  
     A = \sum_{i=1}^n \frac{a_i}{\sqrt{1-a_i}},  \qquad  B = \sum_{i=1}^n a_i\,(1 - a_i).  \]  
   Notice first that  \(A>0\) and  \(B>0\) under the positivity assumption.  Since \(a_1+…+a_n=1\), we also have  
   \[  
     B = \sum_{i=1}^n \bigl(a_i - a_i^2\bigr) 
       = \Bigl(\sum_{i=1}^n a_i\Bigr) 
         - \sum_{i=1}^n a_i^2 
       = 1 - \sum_{i=1}^n a_i^2.  
   \]  

2.  Application of Hölder’s inequality  
   We apply Hölder’s inequality in the following form: for any nonnegative sequences \((x_i)\) and \((y_i)\) and exponents p=2, q=1 satisfying 1/p+1/q=1,  
   \[
     \biggl(\sum_{i=1}^n x_i y_i\biggr)^p  
       \le \Bigl(\sum_{i=1}^n x_i^p\Bigr)  \Bigl(\sum_{i=1}^n y_i^q\Bigr)^{p-1}.  
   \]  
   Here we choose  
     \(x_i = \sqrt{a_i} / (1 - a_i)^{1/4},\)  
     \(y_i = a_i (1 - a_i)^{1/4}.\)  
   Then  
   \[
     x_i^2 = \frac{a_i}{\sqrt{1-a_i}},
     \quad
     y_i   = a_i\sqrt{1 - a_i},
   \]
   and hence  
   \[
     \sum_{i=1}^n x_i^2 
       = A,
     \quad
     \sum_{i=1}^n y_i   
       = B.
   \]
   Applying Hölder with p=2, q=1 gives  
   \[
     \Bigl(\sum_{i=1}^n x_i^2\Bigr) \Bigl(\sum_{i=1}^n y_i\Bigr)
       \ge \Bigl(\sum_{i=1}^n x_i y_i\Bigr)^2.
   \]
   But  
   \[
     x_i y_i = \frac{\sqrt{a_i}}{(1-a_i)^{1/4}} \cdot a_i (1-a_i)^{1/4}
       = a_i^{3/2},
   \]
   so  
   \[
     \sum_{i=1}^n x_i y_i = \sum_{i=1}^n a_i^{3/2}.
   \]
   By the power-mean inequality (applied to the numbers \(a_i\)),  
   \(
     \sum a_i^{3/2} \ge \Bigl(\sum a_i\Bigr)^{3/2}
     = 1^{3/2} = 1.
   \)
   Combining these facts yields  
   \[
     A\,B = \Bigl(\sum x_i^2\Bigr) \Bigl(\sum y_i\Bigr)
       \ge \Bigl(\sum x_i y_i\Bigr)^2
       = \Bigl(\sum a_i^{3/2}\Bigr)^2
       \ge 1^2 = 1.
   \]
   Thus we have the fundamental relation  
   (1)\quad  A^2 B \ge 1.  

3.  Upper bound for B via QM–AM  
   Next we bound  \(B = 1 - \sum a_i^2\) from above.  The quadratic mean–arithmetic mean (QM–AM) inequality in the form  
   \[
     \sqrt{\frac{1}{n} \sum_{i=1}^n a_i^2}
       \ge \frac{1}{n} \sum_{i=1}^n a_i
       = \frac{1}{n} \cdot 1
       = \frac{1}{n}
   \]
   implies  
   \[
     \sum_{i=1}^n a_i^2 \ge \frac{1^2}{n} = \frac{1}{n}.
   \]
   Therefore  
   \[
     B = 1 - \sum_{i=1}^n a_i^2
       \le 1 - \frac{1}{n}
       = \frac{n-1}{n}.  \tag{2}
   \]

4.  Conclusion and determination of C  
   Combining (1) and (2), we have  
   \[
     A^2 \cdot \frac{n-1}{n} \ge A^2 B \ge 1,
   \]
   hence  
   \[
     A^2 \ge \frac{n}{n-1},
     \qquad
     A \ge \sqrt{\frac{n}{n-1}}.
   \]
   This lower bound on A holds for every choice of the \(a_i\), so the largest admissible constant C is  
   \[
     C = \sqrt{\frac{n}{n-1}}.
   \]

5.  Verification of equality case  
   To see that this bound cannot be improved, observe that when all \(a_i = 1/n\), then  
     • in the QM–AM step we have equality because all \(a_i\) are equal,  
     • in the Hölder step we also attain equality because the chosen sequences \(x_i\) and \(y_i\) are proportional.  
   In that case  \(A = n\cdot\frac{1/n}{\sqrt{1-1/n}} = \sqrt{n/(n-1)}\), exactly matching the bound.  

Hence the largest constant C for which  \(A\ge C\) always holds is  

The answer is $C=\sqrt{\frac{n}{n-1}}$
