# Problem Entry

## Problem Type
bound

## Problem
Let $a, b, c > 0$ be real numbers. Determine the maximal constant $C$ such that the following inequality holds for all $a, b, c$:
$$
(a b + b c + c a) \left( \frac{1}{(a + b)^2} + \frac{1}{(b + c)^2} + \frac{1}{(c + a)^2} \right) \geq C.
$$

## Current Solution
We can rewrite the given inequality in the following form
$$
\begin{aligned}
& f(a+b+c, a b+b c+c a, a b c) \\
&= 9((a+b)(b+c)(c+a))^{2} \\
&-4(a b+b c+c a)\left((a+b)^{2}(b+c)^{2}+(b+c)^{2}(c+a)^{2}+(c+a)^{2}(a+b)^{2}\right) \\
&= k(a b c)^{2}+m a b c+n
\end{aligned}
$$
where $k \geq 0$ and $k, m, n$ are quantities containing constants or $a+b+c, a b+$ $b c+c a, a b c$, which we also consider as constants, i.e. in the form as a sixth-degree symmetric polynomial with variables $a, b, c$ and a second-degree polynomial with variable $a b c$ and positive coefficients.

Let us explain this:
The expression $(a+b)(b+c)(c+a)$ has the form $k a b c+m$ so it follows that $9((a+b)(b+c)(c+a))^{2}$ has the form $k^{2}(a b c)^{2}+m a b c+n$.

Furthermore
$4(a b+b c+c a)\left((a+b)^{2}(b+c)^{2}+(b+c)^{2}(c+a)^{2}+(c+a)^{2}(a+b)^{2}\right)=4 k A$,
where $k=a b+b c+c a$, and $A$ is a fourth-degree polynomial and also has the form $k a b c+m$.

Therefore the expression of the left side of $f(a+b+c, a b+b c+c a, a b c)$ has the form $k(a b c)^{2}+m a b c+n$.

Then the function achieves it's minimum value when $(a-b)(b-c)(c-a)=0$ or when $a b c=0$.

If $(a-b)(b-c)(c-a)=0$, then without loss of generality we may assume that $a=c$, and the given inequality is equivalent to
$$
\begin{aligned}
& \left(a^{2}+2 a b\right)\left(\frac{1}{4 a^{2}}+\frac{2}{(a+b)^{2}}\right) \geq \frac{9}{4} \\
& \quad \Leftrightarrow \quad(a-b)^{2}\left(\frac{2 a+b}{2 a(a+b)^{2}}-\frac{1}{(a+b)^{2}}\right) \geq 0 \\
& \quad \Leftrightarrow \quad b(a-b)^{2} \geq 0
\end{aligned}
$$
as required.
If $a b c=0$, we may assume that $c=0$ and the given inequality becomes
$$
\begin{aligned}
& a b\left(\frac{1}{(a+b)^{2}}+\frac{1}{a^{2}}+\frac{1}{b^{2}}\right) \geq \frac{9}{4} \quad \Leftrightarrow \quad(a-b)^{2}\left(\frac{1}{a b}-\frac{1}{4(a+b)^{2}}\right) \geq 0 \\
& \quad \Leftrightarrow \quad(a-b)^{2}\left(4 a^{2}+4 b^{2}+7 a b\right) \geq 0
\end{aligned}
$$
and the problem is solved.

Equality in the above analysis holds when two variables are equal and the third is zero, i.e., when $(a, b, c)$ is a permutation of $(t, t, 0)$ for $t > 0$. In this case, the minimum value of the expression is achieved, so $C = \frac{9}{4}$ is the maximal constant for which the inequality always holds.

Therefore, the answer is $C = \frac{9}{4}$.

## Expected Answer
$C = \frac{9}{4}$

## Enhanced Solution
We wish to find the largest constant C such that for all positive real a,b,c the following holds:  
  
   (ab+bc+ca) · [1/(a+b)^2 + 1/(b+c)^2 + 1/(c+a)^2 ] ≥ C.  
  
Our strategy is to exploit the symmetry of the expression and then reduce to two simpler boundary cases: either one variable vanishes, or two variables become equal.  
  
1. Symmetry and reduction to boundary cases  
   - The left–hand side is a symmetric, homogeneous function of degree 0 in (a,b,c).  
   - By a standard argument using either the method of Lagrange multipliers on the sphere a^2+b^2+c^2=1, or the so-called uvw–method for three variables, a symmetric homogeneous inequality of this type achieves its extremal (minimum or maximum) value when either  
      • two of the variables are equal, or  
      • one of the variables is zero.  
   - Hence it suffices to check the two cases (i) a=c, and (ii) c=0.  
  
2. Case (i): a=c>0  
   Set a=c and keep b>0. Then  
     ab + bc + ca = a^2 + 2ab,  
     (a+b)^2 = (b+c)^2 = (a+b)^2,  
     (c+a)^2 = (2a)^2 = 4a^2.  
   Thus the left side becomes  
     (a^2 + 2ab) · [1/(4a^2) + 2/(a+b)^2].  
   We expand and simplify:  
     (a^2 + 2ab)/(4a^2)  =  1/4 + (b/(2a)),  
     (a^2 + 2ab)·2/(a+b)^2  = 2·(a(a+2b))/( (a+b)^2 )  .  
   On combining these terms over a common denominator one finds after straightforward algebra  
     (a^2 + 2ab)·[1/(4a^2) + 2/(a+b)^2]  –  9/4  =  (b·(a–b)^2)/(2a(a+b)^2).  
   Since a,b>0, the right–hand side is ≥0, with equality precisely when a=b.  
   Therefore in case (i) the minimum of the expression is exactly 9/4.  
  
3. Case (ii): c=0, with a,b>0  
   Then  
     ab+bc+ca = ab,  
     (a+b)^2 as before, and (b+c)^2 = b^2, (c+a)^2 = a^2.  
   Hence the expression becomes  
     ab·[1/(a+b)^2 + 1/a^2 + 1/b^2].  
   Expand and compare to 9/4:  
     ab·[1/a^2 + 1/b^2] = b/a + a/b,  
     ab/(a+b)^2 = ab/(a+b)^2.  
   One checks by rewriting everything over the denominator 4a^2 b^2 (a+b)^2 that  
     ab·[1/(a+b)^2 + 1/a^2 + 1/b^2]  –  9/4  =  ((a–b)^2·(4a^2 + 7ab + 4b^2)) / [4a^2 b^2].  
   Since 4a^2+7ab+4b^2>0 for all a,b>0, the right side is ≥0, with equality only when a=b.  
   Thus in case (ii) the minimum is again 9/4.  
  
4. Conclusion  
   In both boundary cases the expression never drops below 9/4, and equality is attained exactly when two variables are equal and the third is either equal to them or zero (i.e. permutations of (t,t,0) or (t,t,t)).  
   Therefore the maximal constant C for which the original inequality holds for all positive a,b,c is  
  
   The answer is $C=\frac{9}{4}$.  
