# Problem Entry

## Problem Type
bound

## Problem
Let $k \in \mathbb{N}$, and $a_{1}, a_{2}, \ldots, a_{n}$ be positive real numbers such that $a_{1} + a_{2} + \cdots + a_{n} = 1$. Find the maximal constant $C$ such that the following inequality holds for all $a_{1}, a_{2}, \ldots, a_{n}$:
$$
a_{1}^{-k} + a_{2}^{-k} + \cdots + a_{n}^{-k} \geq C.
$$

## Current Solution
Since $A M \geq G M$ we have
$$
\sqrt[n]{a_{1} a_{2} \cdots a_{n}} \leq \frac{a_{1}+a_{2}+\cdots+a_{n}}{n}=\frac{1}{n}
$$
or
$$
n \leq \sqrt[n]{\frac{1}{a_{1}} \frac{1}{a_{2}} \cdots \frac{1}{a_{n}}}
$$

Hence
$$
n^{k} \leq \sqrt[n]{a_{1}^{-k} a_{2}^{-k} \cdots a_{n}^{-k}} \leq \frac{a_{1}^{-k}+a_{2}^{-k}+\cdots+a_{n}^{-k}}{n}
$$
i.e.
$$
a_{1}^{-k}+a_{2}^{-k}+\cdots+a_{n}^{-k} \geq n^{k+1}
$$
as required.

Equality holds when $a_1 = a_2 = \cdots = a_n = \frac{1}{n}$, since then $a_i^{-k} = n^k$ for each $i$, so the sum is $n \cdot n^k = n^{k+1}$. This gives the minimum value of the sum, so $C = n^{k+1}$ is the maximal constant for which the inequality always holds.

Therefore, the answer is $C = n^{k+1}$.

## Expected Answer
$C = n^{k+1}$

## Enhanced Solution
Enhanced Solution:

We wish to determine the largest constant C for which the inequality

  a_{1}^{-k} + a_{2}^{-k} + \cdots + a_{n}^{-k} \ge C

holds for every choice of positive real numbers a_{1},a_{2},\dots,a_{n} satisfying

  a_{1} + a_{2} + \cdots + a_{n} = 1.

Equivalently, we need to find the minimum possible value of the sum S = a_{1}^{-k} + a_{2}^{-k} + \cdots + a_{n}^{-k} under the constraint a_{1}+\cdots+a_{n}=1.  Once this minimum S_{\min} is found, we will have C = S_{\min}.

Step 1: Apply the AM–GM inequality to the numbers a_{1},a_{2},\dots,a_{n}.

  By the Arithmetic–Geometric Mean inequality (AM–GM), for positive reals a_{i},

    (a_{1}a_{2}\cdots a_{n})^{1/n} \;\le\; \frac{a_{1} + a_{2} + \cdots + a_{n}}{n}

  Since a_{1} + a_{2} + \cdots + a_{n} = 1,

    (a_{1}a_{2}\cdots a_{n})^{1/n} \le \frac{1}{n}.

  Raising both sides to the n-th power gives

    a_{1} a_{2} \cdots a_{n} \le n^{-n}

  and hence

    (a_{1} a_{2} \cdots a_{n})^{-1} \ge n^{n}.

Step 2: Relate the product bound to the sum S using AM–GM on the terms a_{i}^{-k}.

  Consider the n nonnegative numbers a_{1}^{-k},a_{2}^{-k},\dots,a_{n}^{-k}.  Again by AM–GM,

    \frac{a_{1}^{-k} + a_{2}^{-k} + \cdots + a_{n}^{-k}}{n} \;\ge\; \bigl(a_{1}^{-k}a_{2}^{-k}\cdots a_{n}^{-k}\bigr)^{1/n}.

  Observe that

    a_{1}^{-k}a_{2}^{-k}\cdots a_{n}^{-k} = (a_{1}a_{2}\cdots a_{n})^{-k}

  so

    \bigl(a_{1}^{-k}a_{2}^{-k}\cdots a_{n}^{-k}\bigr)^{1/n}
    = (a_{1}a_{2}\cdots a_{n})^{-k/n}
    \ge (n^{n})^{k/n} \quad=\; n^{k}.

  Therefore,

    \frac{a_{1}^{-k} + a_{2}^{-k} + \cdots + a_{n}^{-k}}{n} \ge n^{k}

  and multiplying both sides by n yields

    a_{1}^{-k} + a_{2}^{-k} + \cdots + a_{n}^{-k} \ge n^{k+1}.

Step 3: Justify optimality and equality case.

  The two applications of AM–GM become equalities precisely when all the terms are equal.  In the first application, equality requires

    a_{1} = a_{2} = \cdots = a_{n},

  and since their sum is 1, each a_{i} must be 1/n.  Substituting a_{i}=1/n into each a_{i}^{-k} gives (1/n)^{-k}=n^{k}, so the sum is n\cdot n^{k}=n^{k+1}.  Thus n^{k+1} is indeed the minimum possible value of S, and no larger constant C can work for all choices of the a_{i}.

Conclusion: The minimal value of

  a_{1}^{-k} + a_{2}^{-k} + \cdots + a_{n}^{-k}

under the condition a_{1}+\cdots+a_{n}=1 is n^{k+1}, hence the maximal constant C for which the original inequality holds identically is

The answer is $C = n^{k+1}$
