# Problem Entry

## Problem Type
bound

## Problem
Let $x, y, z \in \mathbb{R}^{+}$ such that $x + y + z = 1$. Find the maximal constant $C$ such that the following inequality holds for all $x, y, z$ satisfying the given constraint:
$$
\frac{x y}{z}+\frac{y z}{x}+\frac{z x}{y} \geq C
$$

## Current Solution
We have
$$
\begin{equation*}
\frac{x y}{z}+\frac{y z}{x}+\frac{z x}{y}=\frac{1}{2}\left(\frac{x y}{z}+\frac{y z}{x}\right)+\frac{1}{2}\left(\frac{y z}{x}+\frac{z x}{y}\right)+\frac{1}{2}\left(\frac{z x}{y}+\frac{x y}{z}\right) \tag{1}
\end{equation*}
$$

Since $A M \geq G M$ we have
$$
\frac{1}{2}\left(\frac{x y}{z}+\frac{y z}{x}\right) \geq \sqrt{\frac{x y}{z} \frac{y z}{x}}=y
$$

Analogously we get
$$
\frac{1}{2}\left(\frac{y z}{x}+\frac{z x}{y}\right) \geq z \quad \text { and } \quad \frac{1}{2}\left(\frac{z x}{y}+\frac{x y}{z}\right) \geq x
$$

Adding these three inequalities we obtain
$$
\frac{x y}{z}+\frac{y z}{x}+\frac{z x}{y} \geq x+y+z=1
$$

Equality holds if and only if $x = y = z$, that is, when $x = y = z = \frac{1}{3}$. In this case, the minimum value of the expression is achieved, so $C = 1$ is the maximal constant for which the inequality always holds.

Therefore, the answer is $C = 1$. 

## Expected Answer
$C = 1$

## Enhanced Solution
We wish to find the largest constant C such that for all positive real x,y,z satisfying x+y+z=1, the following holds:   
  
    S = \frac{xy}{z} + \frac{yz}{x} + \frac{zx}{y} \ge C.   
  
Our strategy is to (i) rewrite S in a symmetric way, (ii) apply the AM–GM inequality to carefully chosen pairs, and (iii) deduce the best possible C and the equality case.   
  
1. Symmetric decomposition of S.   
   Observe that each of the three terms in S can be paired in three different ways.  In fact, we can write   
   S = (xy/z + yz/x + zx/y)     
     = ½[(xy/z + yz/x) + (yz/x + zx/y) + (zx/y + xy/z)].    
   
   To verify this identity, note that expanding the right-hand side yields each of the three terms xy/z, yz/x, zx/y exactly twice, and the factor ½ then recovers exactly one copy of each.  Hence the identity is algebraically valid for all positive x,y,z.   
  
2. Applying AM–GM to each pair.   
   Recall that for any two positive reals a,b we have the arithmetic mean–geometric mean inequality (AM–GM):   
     (a + b)/2 ≥ √(ab),   
   with equality if and only if a = b.   
   
   We now apply this to each of the three pairs in our decomposition:   
     • For a = xy/z and b = yz/x, we get   
       (xy/z + yz/x)/2 ≥ √((xy/z)·(yz/x))   
                           = √( (x·y·y·z)/(z·x) )   
                           = √(y²)   
                           = y.   
     • For a = yz/x and b = zx/y, we get   
       (yz/x + zx/y)/2 ≥ √((yz/x)·(zx/y))   
                           = √(z²)   
                           = z.   
     • For a = zx/y and b = xy/z, we get   
       (zx/y + xy/z)/2 ≥ √((zx/y)·(xy/z))   
                           = √(x²)   
                           = x.   
   In each application, we have used positivity of x,y,z and the fact that √(u²)=u when u>0.   
  
3. Summing the three inequalities.   
   Adding the three AM–GM inequalities yields   
     ½(xy/z + yz/x) + ½(yz/x + zx/y) + ½(zx/y + xy/z)   
       ≥ x + y + z.   
   By step 1 this left side is exactly S, and by the given constraint x+y+z=1 we obtain   
     S ≥ 1.   
  
4. Determination of the maximal constant C and the equality case.   
   From S ≥ 1 for all positive x,y,z summing to 1, it follows that the largest possible constant C is at least 1.  To see that we cannot take any larger C, exhibit when equality S=1 occurs.  In each AM–GM step we needed a = b, namely   
     xy/z = yz/x,  yz/x = zx/y,  zx/y = xy/z.   
   The first equality gives x² = z², and since x,z>0 we deduce x=z.  Similarly the second gives y=z, hence x=y=z.  Finally the constraint x+y+z=1 forces x=y=z=1/3.   
   Substituting x=y=z=1/3 into S gives   
     S = 3·[(1/3·1/3)/(1/3)] = 3·(1/9)/(1/3) = 3·(1/9·3) = 3·(1/3)=1,   
   showing that indeed the bound S≥1 is sharp.  Thus the maximal constant C for which the inequality holds in all cases is C=1.   
  
Therefore, the answer is $C=1$
