# Problem Entry

## Problem Type
relation

## Problem
Let $a, b, c, x, y, z$ be positive real numbers such that $x + y + z = 1$. Consider the following expressions:
$$
a x + b y + c z + 2 \sqrt{(x y + y z + z x)(a b + b c + c a)} \quad () \quad a + b + c
$$
Determine the correct inequality relation to fill in the blank.

Options:

(A) $\leq$ 

(B) $\geq$

(C) $=$ 

(D) $<$

(E) $>$

(F) None of the above

## Current Solution
The inequality being homogeneous in $a, b, c$ we can assume that $a+b+c=1$. We apply this time the AM-GM Inequality and we find that
$a x+b y+c z+2 \sqrt{(x y+y z+z x)(a b+b c+c a)} \leq a x+b y+c z+x y+y z+z x+a b+b c+c a$.
Consequently,
$x y+y z+z x+a b+b c+c a=\frac{1-x^{2}-y^{2}-z^{2}}{2}+\frac{1-a^{2}-b^{2}-c^{2}}{2} \leq 1-a x-b y-c z$,
the last one being equivalent to $(x-a)^{2}+(y-b)^{2}+(z-c)^{2} \geq 0$. Therefore, the answer is (A) $\leq$.

## Expected Answer
(A) $\leq$

## Enhanced Solution
We wish to prove the inequality
   a x + b y + c z + 2\,\sqrt{(x y + y z + z x)\,(a b + b c + c a)} \;\le\; a + b + c,
where a,b,c,x,y,z are positive reals with x+y+z=1.  The original solution uses homogeneity and the AM–GM inequality; we now expand each step in detail.

1. Homogenization in a,b,c
   Observe that both sides of the desired inequality are homogeneous of degree 1 in (a,b,c).  Indeed,
     – The term a x + b y + c z is linear in a,b,c.
     – The term \sqrt{(x y + y z + z x)(a b + b c + c a)} is the square root of a product in which (a b + b c + c a) is homogeneous of degree 2 in (a,b,c), so the entire square root is homogeneous of degree 1.
   Likewise, a + b + c is homogeneous of degree 1.  Hence, without loss of generality we may impose the normalization
     a + b + c = 1.

2. Notation for symmetric sums
   Set
     S = x y + y z + z x,
     T = a b + b c + c a.
   Then the left‐hand side becomes a x + b y + c z + 2\,\sqrt{S\,T}.

3. Applying the AM–GM inequality
   By the classical AM–GM inequality on the two nonnegative numbers S and T,
     2\,\sqrt{S\,T} \;\le\; S + T.
   Therefore,
     a x + b y + c z + 2\,\sqrt{S\,T}
       \;\le\; a x + b y + c z + (S + T).

4. Expressing S and T in terms of squares
   Since x+y+z=1, we have
     (x+y+z)^2 = x^2 + y^2 + z^2 + 2S = 1
     \implies S = \frac{1 - (x^2+y^2+z^2)}{2}.
   Similarly, because a+b+c=1,
     T = \frac{1 - (a^2+b^2+c^2)}{2}.
   Hence
     a x + b y + c z + S + T
       = a x + b y + c z
         + \frac{1 - (x^2+y^2+z^2)}{2}
         + \frac{1 - (a^2+b^2+c^2)}{2}
       = a x + b y + c z + 1
         - \tfrac{1}{2}\bigl(x^2+y^2+z^2 + a^2+b^2+c^2\bigr).

5. Reducing to a sum of squares
   We now show
     a x + b y + c z + S + T \le 1.
   Equivalently,
     a x + b y + c z + 1 - \tfrac{1}{2}(x^2+y^2+z^2 + a^2+b^2+c^2) \le 1
   \iff a x + b y + c z \le \tfrac{1}{2}(x^2+y^2+z^2 + a^2+b^2+c^2).
   Multiply both sides by 2:
     2(a x + b y + c z) \le x^2+y^2+z^2 + a^2+b^2+c^2
   \iff (x^2 - 2a x + a^2) + (y^2 - 2b y + b^2) + (z^2 - 2c z + c^2) \ge 0
   \iff (x - a)^2 + (y - b)^2 + (z - c)^2 \ge 0.
   This last inequality is manifestly true, since a sum of squares is nonnegative.

6. Conclusion by chaining inequalities
   From Steps 3 and 5 we have
     a x + b y + c z + 2\sqrt{S\,T}
       \le a x + b y + c z + (S+T)
       \le 1.
   Recalling our normalization a+b+c=1, this yields
     a x + b y + c z + 2\sqrt{(x y + y z + z x)(a b + b c + c a)}
       \le a + b + c.
   Hence the correct relation is “≤.”

The answer is (A) ≤
