# Problem Entry

## Problem Type
relation

## Problem
Let $a, b, c$ be positive real numbers such that $a b + b c + c a = 3$. Consider the following inequality:
$$
\left(a^{3}-a+5\right)\left(b^{5}-b^{3}+5\right)\left(c^{7}-c^{5}+5\right) \quad () \quad 125 .
$$

Determine the correct inequality relation to fill in the blank.

Options:

(A) $\leq$ 

(B) $\geq$

(C) $=$ 

(D) $<$

(E) $>$

(F) None of the above

## Current Solution
For any real number $x$, the numbers $x-1, x^{2}-1, x^{3}-1$ and $x^{5}-1$ are of the same sign.

Therefore
$$
(x-1)\left(x^{2}-1\right) \geq 0, \quad\left(x^{2}-1\right)\left(x^{3}-1\right) \geq 0 \quad \text { and } \quad\left(x^{2}-1\right)\left(x^{5}-1\right) \geq 0
$$
i.e.
$$
\begin{aligned}
a^{3}-a^{2}-a+1 & \geq 0 \\
b^{5}-b^{3}-b^{2}+1 & \geq 0 \\
c^{7}-c^{5}-c^{2}+1 & \geq 0
\end{aligned}
$$

So it follows that
$$
a^{3}-a+5 \geq a^{2}+4, \quad b^{5}-b^{3}+5 \geq b^{2}+4 \quad \text { and } \quad c^{7}-c^{5}+5 \geq c^{2}+4
$$

Multiplying these inequalities gives us
$$
\begin{equation*}
\left(a^{3}-a+5\right)\left(b^{5}-b^{3}+5\right)\left(c^{7}-c^{5}+5\right) \geq\left(a^{2}+4\right)\left(b^{2}+4\right)\left(c^{2}+4\right) \tag{1}
\end{equation*}
$$

We'll prove that
$$
\begin{equation*}
\left(a^{2}+4\right)\left(b^{2}+4\right)\left(c^{2}+4\right) \geq 25(a b+b c+c a+2) \tag{2}
\end{equation*}
$$

We have
$$
\begin{aligned}
& \left(a^{2}+4\right)\left(b^{2}+4\right)\left(c^{2}+4\right) \\
& \quad=a^{2} b^{2} c^{2}+4\left(a^{2} b^{2}+b^{2} c^{2}+c^{2} a^{2}\right)+16\left(a^{2}+b^{2}+c^{2}\right)+64
\end{aligned}
$$
$$
\begin{align*}
= & a^{2} b^{2} c^{2}+\left(a^{2}+b^{2}+c^{2}\right)+2+4\left(a^{2} b^{2}+b^{2} c^{2}+c^{2} a^{2}+3\right) \\
& +15\left(a^{2}+b^{2}+c^{2}\right)+50 \tag{3}
\end{align*}
$$

By the obvious inequalities
$(a-b)^{2}+(b-c)^{2}+(c-a)^{2} \geq 0 \quad$ and $\quad(a b-1)^{2}+(b c-1)^{2}+(c a-1)^{2} \geq 0$
we obtain
$$
\begin{align*}
a^{2}+b^{2}+c^{2} & \geq a b+b c+c a  \tag{4}\\
a^{2} b^{2}+b^{2} c^{2}+c^{2} a^{2}+3 & \geq 2(a b+b c+c a) \tag{5}
\end{align*}
$$

We'll prove that
$$
\begin{equation*}
a^{2} b^{2} c^{2}+\left(a^{2}+b^{2}+c^{2}\right)+2 \geq 2(a b+b c+c a) \tag{6}
\end{equation*}
$$

Lemma Let $x, y, z>0$. Then
$$
3 x y z+x^{3}+y^{3}+z^{3} \geq 2\left((x y)^{3 / 2}+(y z)^{3 / 2}+(z x)^{3 / 2}\right)
$$

Proof By Schur's inequality and $A M \geq G M$ we have
$$
\begin{aligned}
x^{3}+y^{3}+z^{3}+3 x y z & \geq\left(x^{2} y+y^{2} x\right)+\left(z^{2} y+y^{2} z\right)+\left(x^{2} z+z^{2} x\right) \\
& \geq 2\left((x y)^{3 / 2}+(y z)^{3 / 2}+(z x)^{3 / 2}\right)
\end{aligned}
$$

By Lemma for $x=a^{2 / 3}, y=b^{2 / 3}, z=c^{2 / 3}$ we deduce
$$
3(a b c)^{2 / 3}+a^{2}+b^{2}+c^{2} \geq 2(a b+b c+c a)
$$

Therefore it suffices to prove that
$$
a^{2} b^{2} c^{2}+2 \geq 3(a b c)^{2 / 3}
$$
which follows immediately by $A M \geq G M$.
Thus we have proved inequality (6).
Now by (3), (4), (5) and (6) we obtain inequality (2).
Finally by (1), (2) and since $a b+b c+c a=3$ we obtain the required inequality. Equality occurs if and only if $a=b=c=1$. Therefore, the answer is (B) $\geq$.

## Expected Answer
(B) $\geq$

## Enhanced Solution
Solution:

We wish to determine whether
   (a^3 - a + 5)(b^5 - b^3 + 5)(c^7 - c^5 + 5)  • 125,
where “•” stands for one of the relations ≤, ≥, =, <, >, under the constraint a,b,c>0 and ab+bc+ca=3.

Our strategy follows the original approach but with fuller justification and clear logical steps.

Step 1.  A lower bound for each factor.
------------------------------------------------
Fix any positive x.  Observe that the four numbers x−1, x^2−1, x^3−1, x^5−1 all share the same sign:
 • If x≥1, then each is ≥0.
 • If 0<x≤1, then each is ≤0.
Hence the products
   (x−1)(x^2−1) ≥ 0,
   (x^2−1)(x^3−1) ≥ 0,
   (x^2−1)(x^5−1) ≥ 0.

Expanding these yields inequalities in each of a,b,c:
  (i)  (a−1)(a^2−1) ≥0  ⇒  a^3 − a^2 − a + 1 ≥ 0  ⇒  a^3 − a + 5 ≥ a^2 + 4,
  (ii) (b^2−1)(b^3−1) ≥0  ⇒  b^5 − b^3 − b^2 + 1 ≥ 0 ⇒  b^5 − b^3 + 5 ≥ b^2 + 4,
  (iii)(c^2−1)(c^5−1) ≥0  ⇒  c^7 − c^5 − c^2 + 1 ≥ 0 ⇒  c^7 − c^5 + 5 ≥ c^2 + 4.

Because each left–hand side a^3−a+5, b^5−b^3+5, c^7−c^5+5 is strictly positive (for example at x=1 it equals 5>0), we may multiply the three inequalities to obtain
   (1)
   (a^3−a+5)(b^5−b^3+5)(c^7−c^5+5)
     ≥ (a^2+4)(b^2+4)(c^2+4).

Step 2.  A lower bound for (a^2+4)(b^2+4)(c^2+4).
--------------------------------------------------------------
Expand the product:
   (a^2+4)(b^2+4)(c^2+4)
 = a^2 b^2 c^2
   + 4(a^2 b^2 + b^2 c^2 + c^2 a^2)
   +16(a^2 + b^2 + c^2)
   +64.

We now regroup terms as follows:
   = [a^2 b^2 c^2 + (a^2+b^2+c^2) + 2]
     + 4[ a^2 b^2 + b^2 c^2 + c^2 a^2 + 3 ]
     +15(a^2 + b^2 + c^2)
     +50.

We shall show each bracketed expression is at least a suitable multiple of S:=ab+bc+ca, then sum the results.

(2a)  By the trivial sum–of–squares,
     (a^2 + b^2 + c^2) − (ab+bc+ca)
     = ½[(a−b)^2 + (b−c)^2 + (c−a)^2] ≥ 0,
so
     a^2 + b^2 + c^2  ≥  S.        (Inequality A)

(2b)  By the same idea applied to ab and 1,
     (ab−1)^2 + (bc−1)^2 + (ca−1)^2 ≥0
⇒   a^2 b^2 + b^2 c^2 + c^2 a^2 + 3  ≥ 2(ab+bc+ca)
so
     a^2 b^2 + b^2 c^2 + c^2 a^2 + 3  ≥ 2S.   (Inequality B)

(2c)  We claim
     a^2 b^2 c^2 + (a^2+b^2+c^2) + 2  ≥  2S.
To prove this, set x=a^{2/3}, y=b^{2/3}, z=c^{2/3}.  Then x,y,z>0 and
   Schur’s inequality of degree 3 gives
     x^3 + y^3 + z^3 + 3xyz
       ≥ (x^2y + xy^2) + (y^2z + yz^2) + (z^2x + zx^2).
   By AM–GM on each pair x^2y + xy^2 ≥ 2(xy)^{3/2} etc., one obtains
     x^3 + y^3 + z^3 + 3xyz
       ≥ 2[(xy)^{3/2} + (yz)^{3/2} + (zx)^{3/2}].
Replacing x=a^{2/3}, etc., yields
   a^2 + b^2 + c^2  + 3(a b c)^{2/3}
     ≥  2(ab + bc + ca) = 2S.    (α)
Meanwhile, by AM–GM on the three numbers a^2 b^2 c^2, 1, 1,
   (a^2 b^2 c^2 + 1 + 1)/3  ≥  (a^2 b^2 c^2·1·1)^{1/3} = (abc)^{2/3},
so
   a^2 b^2 c^2 + 2  ≥  3(abc)^{2/3}.      (β)
Adding (α) and (β) term by term gives exactly
   a^2 b^2 c^2 + (a^2+b^2+c^2) + 2  ≥  2S.   (Inequality C)

Combining (Inequalities A, B, C) with our regrouping,
   (a^2+4)(b^2+4)(c^2+4)
 ≥ [≥2S] + 4[≥2S] + 15[≥S] + 50
 =  2S + 8S + 15S + 50
 =  25S + 50
 = 25(ab+bc+ca) + 50.
Since ab+bc+ca=3 by hypothesis, this yields
   (2)
   (a^2+4)(b^2+4)(c^2+4)  ≥  25·3 + 50  = 125.

Step 3.  Conclusion.
--------------------------
From (1) and (2) we chain
   (a^3−a+5)(b^5−b^3+5)(c^7−c^5+5)
     ≥ (a^2+4)(b^2+4)(c^2+4)
     ≥ 125.
Therefore the correct relation is “≥ 125.”  One checks equality throughout occurs exactly when a=b=c=1.

The answer is (B) ≥
