# Problem Entry

## Problem Type
relation

## Problem
Let $a, b, c$ be positive real numbers such that $a + b + c = 3$. Consider the following inequality:
$$
\frac{a^{2}}{a+2 b^{3}}+\frac{b^{2}}{b+2 c^{3}}+\frac{c^{2}}{c+2 a^{3}} \quad () \quad 1 .
$$
Determine the correct inequality relation to fill in the blank.

Options:

(A) $\leq$ 

(B) $\geq$

(C) $=$ 

(D) $<$

(E) $>$

(F) None of the above

## Current Solution
Applying $A M \geq G M$ gives us
$$
\frac{a^{2}}{a+2 b^{3}}=a-\frac{2 a b^{3}}{a+2 b^{3}} \geq a-\frac{2 a b^{3}}{3 \sqrt[3]{a b^{4}}}=a-\frac{2 b a^{2 / 3}}{3}
$$

Analogously
$$
\frac{b^{2}}{b+2 c^{3}} \geq b-\frac{2 c b^{2 / 3}}{3} \quad \text { and } \quad \frac{c^{2}}{c+2 a^{3}} \geq c-\frac{2 a c^{2 / 3}}{3}
$$

Adding these three inequalities implies
$$
\frac{a^{2}}{a+2 b^{2}}+\frac{b^{2}}{b+2 c^{2}}+\frac{c^{2}}{c+2 a^{2}} \geq(a+b+c)-\frac{2}{3}\left(b a^{2 / 3}+c b^{2 / 3}+a c^{2 / 3}\right)
$$

So it is enough to prove that
$$
(a+b+c)-\frac{2}{3}\left(b a^{2 / 3}+c b^{2 / 3}+a c^{2 / 3}\right) \geq 1
$$
i.e.
$$
\begin{equation*}
b a^{2 / 3}+c b^{2 / 3}+a c^{2 / 3} \leq 3 \tag{1}
\end{equation*}
$$

After another application of $A M \geq G M$ we get
$$
\begin{aligned}
b a^{2 / 3}+c b^{2 / 3}+a c^{2 / 3} & \leq \frac{b(2 a+1)+c(2 b+1)+a(2 c+1)}{3} \\
& =\frac{a+b+c+2(a b+b c+c a)}{3} \\
& \leq \frac{(a+b+c)+(a+b+c)^{2} / 3}{3}=\frac{3+2 \cdot 3^{2} / 3}{3}=3
\end{aligned}
$$
i.e. we have proved (1), and we are done.

Equality holds iff $a=b=c=1$. Therefore, the answer is (B) $\geq$.

## Expected Answer
(B) $\geq$

## Enhanced Solution
We wish to prove that for all positive real numbers a, b, c with a + b + c = 3, the following holds:
   
   \[\frac{a^{2}}{a + 2b^{3}} + \frac{b^{2}}{b + 2c^{3}} + \frac{c^{2}}{c + 2a^{3}} \;\ge\; 1.\]

Our strategy is to apply the Arithmetic–Geometric Mean (AM–GM) inequality in two stages: first to each denominator a + 2b³, and then to bound the cyclic sum a^{2/3}b + b^{2/3}c + c^{2/3}a.

1.  Bound each term a²/(a + 2b³) from below.
   
   For the denominator, observe by AM–GM on the three positive numbers a, b³, b³ that
   \[
     \frac{a + b^{3} + b^{3}}{3} \;\ge\; (a \cdot b^{3} \cdot b^{3})^{1/3} \,=\, a^{1/3} \; b^{2}.
   \]
   Therefore
   \[
     a + 2b^{3} \;=\; (a + b^{3} + b^{3}) \;\ge\; 3\,a^{1/3}\,b^{2}.
   \]
   We rewrite
   \[
     \frac{a^{2}}{a + 2b^{3}} 
     = a 
       - \frac{2\,a\,b^{3}}{a + 2b^{3}} 
     \;\ge\;
     a 
       - \frac{2\,a\,b^{3}}{3\,a^{1/3}\,b^{2}} 
     
     = a 
       - \frac{2}{3}\,a^{2/3}\,b.
   \]
   By the same reasoning (cyclically permuting a→b→c→a), we obtain three inequalities:
   \[
     \frac{a^{2}}{a + 2b^{3}} \ge a - \frac{2}{3}\,a^{2/3}b,
     \quad
     \frac{b^{2}}{b + 2c^{3}} \ge b - \frac{2}{3}\,b^{2/3}c,
     \quad
     \frac{c^{2}}{c + 2a^{3}} \ge c - \frac{2}{3}\,c^{2/3}a.
   \]
   Adding these three yields
   \[
     \sum_{\mathrm{cyc}} \frac{a^{2}}{a + 2b^{3}} 
     \;\ge\; 
     (a + b + c)
       
     - \frac{2}{3}\bigl(a^{2/3}b + b^{2/3}c + c^{2/3}a\bigr).
   \]
   Since a + b + c = 3 by hypothesis, this is equivalent to
   \[
     \frac{a^{2}}{a + 2b^{3}} + \frac{b^{2}}{b + 2c^{3}} + \frac{c^{2}}{c + 2a^{3}} 
     \;\ge\; 
     3 
       - \frac{2}{3}\bigl(a^{2/3}b + b^{2/3}c + c^{2/3}a\bigr).
   \]
   To conclude that the left–hand side \(\ge1\), it suffices to show
   \[
     a^{2/3}b + b^{2/3}c + c^{2/3}a \;\le\; 3.
   \]

2.  Prove the cyclic sum a^{2/3}b + b^{2/3}c + c^{2/3}a ≤ 3.

   We apply a weighted AM–GM inequality to each term of the form a^{2/3}b.  Namely, for positive a, b,
   \[
     \frac{2a + b}{3} \;\ge\; (a^{2}b)^{1/3} \;=\; a^{2/3}\,b^{1/3}.
   \]
   Multiply both sides by b^{2/3} to obtain:
   \[
     \frac{b^{2/3}(2a + b)}{3}
     \;\ge\;
     b^{2/3}\,a^{2/3}\,b^{1/3}
     
     = a^{2/3}\,b.
   \]
   Hence
   \[
     a^{2/3}b \;\le\; \frac{b\,(2a + b)}{3}.
   \]
   Summing cyclically,
   \[
     a^{2/3}b + b^{2/3}c + c^{2/3}a
     \;\le\;
     \frac{1}{3}\Bigl[b(2a + b) + c(2b + c) + a(2c + a)\Bigr]
     
     = \frac{2(ab + bc + ca) + (a + b + c)}{3}.
   \]
   Since for any positive a,b,c we have the well–known bound
   \[
     ab + bc + ca \;\le\; \frac{(a + b + c)^{2}}{3},
   \]
   and because a + b + c = 3, it follows that
   \[
     a^{2/3}b + b^{2/3}c + c^{2/3}a
     \;\le\;
     \frac{2\bigl(3^{2}/3\bigr) + 3}{3}
     
     = \frac{2\cdot 3 + 3}{3} = 3.
   \]

Combining the two stages shows
\[
  \frac{a^{2}}{a + 2b^{3}} + \frac{b^{2}}{b + 2c^{3}} + \frac{c^{2}}{c + 2a^{3}} \;\ge\; 1.
\]
Moreover, equality holds precisely when all the AM–GM inequalities used become equalities, which forces a = b = c = 1.  Therefore, the correct relation is “greater than or equal to.”

The answer is (B) ≥
