# Problem Entry

## Problem Type
relation

## Problem
Let $a, b, c$ be positive real numbers. Consider the following inequality:
$$
\frac{a+\sqrt{a b}+\sqrt[3]{a b c}}{3} \quad () \quad \sqrt[3]{a \cdot \frac{a+b}{2} \cdot \frac{a+b+c}{3}}
$$

Determine the correct inequality relation to fill in the blank.

Options:

(A) $\leq$ 

(B) $\geq$

(C) $=$ 

(D) $<$

(E) $>$

(F) None of the above

## Current Solution
Applying $A M \geq G M$ we get
$$
\sqrt[3]{a b \cdot \frac{a+b}{2}} \geq \sqrt[3]{a b \cdot \sqrt{a b}}=\sqrt{a b}
$$

So
$$
a+\sqrt{a b}+\sqrt[3]{a b c} \leq a+\sqrt[3]{a b \cdot \frac{a+b}{2}}+\sqrt[3]{a b c}
$$

Now, it is enough to show that
$$
a+\sqrt[3]{a b \cdot \frac{a+b}{2}}+\sqrt[3]{a b c} \leq 3 \sqrt[3]{a \cdot \frac{a+b}{2} \cdot \frac{a+b+c}{3}}
$$

Another application of $A M \geq G M$ gives us
$\sqrt[3]{1 \cdot \frac{2 a}{a+b} \cdot \frac{3 a}{a+b+c}} \leq \frac{1+\frac{2 a}{a+b}+\frac{3 a}{a+b+c}}{3}, \quad \sqrt[3]{1 \cdot 1 \cdot \frac{3 b}{a+b+c}} \leq \frac{2+\frac{3 b}{a+b+c}}{3}$ and
$$
\sqrt[3]{1 \cdot \frac{2 b}{a+b} \cdot \frac{3 c}{a+b+c}} \leq \frac{1+\frac{2 b}{a+b}+\frac{3 c}{a+b+c}}{3}
$$

Adding, we obtain
$$
\sqrt[3]{\frac{2 a}{a+b} \cdot \frac{3 a}{a+b+c}}+\sqrt[3]{\frac{3 b}{a+b+c}}+\sqrt[3]{\frac{2 b}{a+b} \cdot \frac{3 c}{a+b+c}} \leq 3
$$
i.e.
$$
\sqrt[3]{\frac{1}{a} \cdot \frac{2}{a+b} \cdot \frac{3}{a+b+c}}\left(a+\sqrt[3]{a b \cdot \frac{a+b}{2}}+\sqrt[3]{a b c}\right) \leq 3
$$
i.e.
$$
a+\sqrt[3]{a b \cdot \frac{a+b}{2}}+\sqrt[3]{a b c} \leq 3 \sqrt[3]{a \cdot \frac{a+b}{2} \cdot \frac{a+b+c}{3}}
$$ Therefore, the answer is (A) $\leq$.

## Expected Answer
(A) $\leq$

## Enhanced Solution
Enhanced Solution:

We wish to determine which of the relations “≤, ≥, =, <, >” holds in the inequality

  (a + √(a b) + ³√(a b c)) ⁄ 3  ()  ³√[a · ((a + b)/2) · ((a + b + c)/3)]

and show that the correct symbol is “≤.”  We will do so in two main steps, each time applying the Arithmetic Mean–Geometric Mean (AM–GM) inequality in a carefully chosen way, and we will keep the original strategy intact.

Step 1.  Replace √(a b) by a larger AM–GM expression.

We claim that

  √(a b)  ≤  ³√[a b · ((a + b)/2)].

Indeed, squaring both sides of the goal √(a b) ≤ ³√[a b · ((a + b)/2)] and then cubing gives the equivalent inequality

  (√(a b))³  ≤  a b · ((a + b)/2)
  ⟺  (a b)^(3/2)  ≤  (a b)·((a + b)/2)
  ⟺  √(a b)  ≤  (a + b)/2.

But (a + b)/2 ≥ √(a b) is precisely the two‐term AM–GM inequality applied to {a, b}.  Therefore

  √(a b)  ≤  ³√[a b · ((a + b)/2)],

and hence

  a + √(a b) + ³√(a b c)
    ≤  a + ³√[a b · ((a + b)/2)]  + ³√(a b c).

It remains to show that

  a + ³√[a b · ((a + b)/2)]  + ³√(a b c)
    ≤  3 · ³√[a · ((a + b)/2) · ((a + b + c)/3)].

Step 2.  Show the remaining three‐term sum is bounded by the right‐hand side.

Set

  M  :=  ³√[a · ((a + b)/2) · ((a + b + c)/3)],
  S  :=  a + ³√[a b · ((a + b)/2)] + ³√(a b c).

We will prove S ≤ 3 M by dividing both sides by M and applying AM–GM to three carefully chosen triples.

First observe that for each term T in S, the ratio T/M can be rewritten as a geometric mean of three nonnegative numbers:

1)  For T = a,
   
     a/M  =  a  ÷  ³√[a·((a + b)/2)·((a + b + c)/3)]
          =  ³√[ a³  ÷ (a·((a + b)/2)·((a + b + c)/3)) ]
          =  ³√[ 6a²/((a + b)(a + b + c)) ]
          =  ³√[ 1 · (2a/(a + b)) · (3a/(a + b + c)) ].

2)  For T = ³√[a b · ((a + b)/2)],
   
     T/M  =  ³√[ a b·((a + b)/2)  ÷  (a·((a + b)/2)·((a + b + c)/3)) ]
          =  ³√[ 3b/(a + b + c) ]
          =  ³√[ 1 · 1 · (3b/(a + b + c)) ].

3)  For T = ³√(a b c),
   
     T/M  =  ³√[ a b c  ÷  (a·((a + b)/2)·((a + b + c)/3)) ]
          =  ³√[ 6b c/((a + b)(a + b + c)) ]
          =  ³√[ 1 · (2b/(a + b)) · (3c/(a + b + c)) ].

Hence

  S/M
    =  ³√[1 · (2a/(a + b)) · (3a/(a + b + c))]
      + ³√[1 · 1 · (3b/(a + b + c))]
      + ³√[1 · (2b/(a + b)) · (3c/(a + b + c))].

We now apply the three‐term AM–GM inequality to each of the triples:

(i)  For {1, 2a/(a + b), 3a/(a + b + c)},
     (1 + (2a/(a + b)) + (3a/(a + b + c))) / 3 
       ≥  ³√[1·(2a/(a + b))·(3a/(a + b + c))].

(ii) For {1, 1, 3b/(a + b + c)},
     (1 + 1 + (3b/(a + b + c))) / 3 
       ≥  ³√[1·1·(3b/(a + b + c))].

(iii) For {1, 2b/(a + b), 3c/(a + b + c)},
     (1 + (2b/(a + b)) + (3c/(a + b + c))) / 3 
       ≥  ³√[1·(2b/(a + b))·(3c/(a + b + c))].

Adding these three inequalities gives

   S/M
  ≤ [ (1 + 2a/(a + b) + 3a/(a + b + c))
       + (1 + 1 + 3b/(a + b + c))
       + (1 + 2b/(a + b) + 3c/(a + b + c)) ] / 3
  = [ (1+1+1+1) + 2(a+b)/(a+b) + 3(a+b+c)/(a+b+c) ] / 3
  = [ 4 + 2 + 3 ] / 3  =  9/3  =  3.

Hence S/M ≤ 3, i.e.

  a + ³√[a b·((a + b)/2)] + ³√(a b c)
    ≤  3 · ³√[a·((a + b)/2)·((a + b + c)/3)].

Combining with Step 1, we conclude

  (a + √(a b) + ³√(a b c)) / 3
    ≤  ³√[a·((a + b)/2)·((a + b + c)/3)].

Therefore, the correct relation is “≤.”

Answer:
The answer is (A) ≤
