# Problem Entry

## Problem Type
relation

## Problem
Let $a, b, c$ be non-negative real numbers. Consider the following inequality:
$$
a^{3}+b^{3}+c^{3}+a b c \quad () \quad \frac{1}{7}(a+b+c)^{3} .
$$

Determine the correct inequality relation to fill in the blank.

Options:

(A) $\leq$ 

(B) $\geq$

(C) $=$ 

(D) $<$

(E) $>$

(F) None of the above

## Current Solution
We have
$$
\begin{aligned}
(a+b+c)^{3} & =a^{3}+b^{3}+c^{3}+3\left(a^{2}(b+c)+b^{2}(c+a)+c^{2}(a+b)\right)+6 a b c \\
& =\frac{T[3,0,0]}{2}+3 T[2,1,0]+T[1,1,1]
\end{aligned}
$$
and
$$
a^{3}+b^{3}+c^{3}+a b c=\frac{T[3,0,0]}{2}+\frac{T[1,1,1]}{6}
$$

So we need to prove that
$$
7\left(\frac{T[3,0,0]}{2}+\frac{T[1,1,1]}{6}\right) \geq \frac{T[3,0,0]}{2}+3 T[2,1,0]+T[1,1,1]
$$
i.e.
$$
3 T[3,0,0]+\frac{T[1,1,1]}{6} \geq 3 T[2,1,0]
$$
which is true according to $T[3,0,0] \geq T[2,1,0]$ and $T[1,1,1] \geq 0$ (Muirhead's theorem). Therefore, the answer is (B) $\geq$.

## Expected Answer
(B) $\geq$

## Enhanced Solution
We wish to determine which inequality sign correctly relates
\[a^{3}+b^{3}+c^{3}+a b c \;()\; \frac{1}{7}(a+b+c)^{3},\]
for all nonnegative real numbers \(a,b,c\).
Our goal is to show that
\[a^{3}+b^{3}+c^{3}+a b c\;\ge\;\frac{1}{7}(a+b+c)^{3}\]
and hence conclude that the correct sign is “\(\ge\)”.

1.  Expand \((a+b+c)^3\).
    By the multinomial theorem,
    \[
    (a+b+c)^3
    = a^3 + b^3 + c^3
      +3\bigl[a^2(b+c)+b^2(c+a)+c^2(a+b)\bigr]
      +6abc.
    \]

2.  Introduce symmetric sums notation.
    Define
    \[
    T[3,0,0] = a^3+b^3+c^3,
    \quad
    T[2,1,0] = a^2b + a^2c + b^2a + b^2c + c^2a + c^2b,
    \quad
    T[1,1,1] = 6abc.
    \]
    Then the expansion becomes
    \[
    (a+b+c)^3 = T[3,0,0] + 3\,T[2,1,0] + T[1,1,1].
    \]

3.  Express the left–hand side \(a^3+b^3+c^3 + abc\) in the same notation.
    Observe that \(abc = \tfrac{1}{6}T[1,1,1]\). Hence
    \[
    a^3+b^3+c^3 + abc
    = T[3,0,0] + \frac{1}{6}T[1,1,1].
    \]

4.  Multiply the proposed inequality by 7 to eliminate fractions.
    We want
    \[
    a^3+b^3+c^3 + abc \;\ge\; \frac{1}{7}(a+b+c)^3
    \quad\Longleftrightarrow\quad
    7\bigl(a^3+b^3+c^3 + abc\bigr) \;\ge\; (a+b+c)^3.
    \]
    Substituting the symmetric‐sum expressions gives
    \[
    7\Bigl(T[3,0,0] + \tfrac{1}{6}T[1,1,1]\Bigr)
    \;\ge\;
    T[3,0,0] + 3\,T[2,1,0] + T[1,1,1].
    \]
    Simplify the left side:
    \[
    7T[3,0,0] + \frac{7}{6}T[1,1,1]
    = 7T[3,0,0] + T[1,1,1] + \frac{1}{6}T[1,1,1]
    = 7T[3,0,0] + T[1,1,1] + \frac{1}{6}T[1,1,1].
    \]
    Subtract \(T[3,0,0] + T[1,1,1]\) from both sides to obtain the equivalent inequality
    \[
    6T[3,0,0] + \frac{1}{6}T[1,1,1]
    \;\ge\;
    3T[2,1,0].
    \]
    Or equivalently,
    \[
    3T[3,0,0] + \frac{1}{6}T[1,1,1]
    \;\ge\; 3T[2,1,0].
    \]

5.  Apply Muirhead’s inequality and nonnegativity.
    •  Because \((3,0,0)\) majorizes \((2,1,0)\), Muirhead’s theorem yields
       \(T[3,0,0] \ge T[2,1,0]\).
    •  Since \(a,b,c\ge0\), clearly \(T[1,1,1]=6abc\ge0\).

    Therefore
    \[
    3T[3,0,0] + \frac{1}{6}T[1,1,1]
    \;\ge\; 3T[2,1,0] + 0
    = 3T[2,1,0],
    \]
    as required.

Conclusion: the correct relation is “\(\ge\)”.

The answer is (B) ≥
