# Problem Entry

## Problem Type
relation

## Problem
Let $a, b, c$ be positive real numbers. Consider the following expressions:
$$
\frac{a^{3}}{b^{2}}+\frac{b^{3}}{c^{2}}+\frac{c^{3}}{a^{2}} \quad () \quad \frac{a^{2}}{b}+\frac{b^{2}}{c}+\frac{c^{2}}{a}
$$
Determine the correct inequality relation to fill in the blank.

Options:

(A) $\leq$ 

(B) $\geq$

(C) $=$ 

(D) $<$

(E) $>$

(F) None of the above

## Current Solution
By the Cauchy-Schwarz Inequality we have

$$
(a+b+c)\left(\frac{a^{3}}{b^{2}}+\frac{b^{3}}{c^{2}}+\frac{c^{3}}{a^{2}}\right) \geq\left(\frac{a^{2}}{b}+\frac{b^{2}}{c}+\frac{c^{2}}{a}\right)^{2}
$$

so we only have to prove that

$$
\frac{a^{2}}{b}+\frac{b^{2}}{c}+\frac{c^{2}}{a} \geq a+b+c
$$

But this follows immediately from the Cauchy-Schwarz Inequality. Therefore, the answer is (B) $\geq$.

## Expected Answer
(B) $\geq$

## Enhanced Solution
Enhanced Solution:

We wish to compare the two cyclic sums
  S₁ = a³/b² + b³/c² + c³/a²
and
  S₂ = a²/b  + b²/c  + c²/a
for arbitrary positive real numbers a,b,c.  We claim that
  S₁ ≥ S₂.

Step 1:  Apply the Cauchy–Schwarz inequality to the two sequences
    ( √(a³/b²),   √(b³/c²),   √(c³/a²) )
and
    ( √a,         √b,         √c ).
By Cauchy–Schwarz, the square of their dot product does not exceed the product of their sums of squares:  
  [ (a^(3/2)/b)·√a  +  (b^(3/2)/c)·√b  +  (c^(3/2)/a)·√c ]²
    ≤ [ a³/b² + b³/c² + c³/a² ] · [ a + b + c ].
But the dot product is exactly a²/b + b²/c + c²/a = S₂, so we obtain
  S₂²  ≤  S₁ · (a + b + c).
Since a+b+c>0, we rearrange to
  S₁  ≥  S₂² / (a + b + c).               (1)

Step 2:  To conclude S₁ ≥ S₂ it suffices by (1) to prove
  S₂² / (a + b + c)  ≥  S₂,
or equivalently (noting S₂>0)
  S₂  ≥  a + b + c.                         (2)

Step 3:  We again invoke Cauchy–Schwarz, now on the sequences
    ( √(a²/b),  √(b²/c),  √(c²/a) )
and
    ( √b,        √c,        √a ).
Their dot product is again √(a²/b)·√b + … = a + b + c, so  
  (a²/b + b²/c + c²/a) · (b + c + a)  ≥  (a + b + c)².
Since b+c+a = a+b+c >0, dividing both sides by (a+b+c) yields exactly
  S₂  =  a²/b + b²/c + c²/a  ≥  a + b + c.
This completes the justification of (2).

Combining (1) with (2) we deduce
  S₁  ≥  S₂,
as required.

Therefore the correct inequality relation is “≥.”

The answer is (B) ≥
