# Problem Entry

## Problem Type
relation

## Problem
Let $a, b, c$ be positive real numbers such that $a b c \geq 1$. Consider the following expressions:
$$
a + b + c \quad () \quad \frac{1+a}{1+b} + \frac{1+b}{1+c} + \frac{1+c}{1+a}
$$
Determine the correct inequality relation to fill in the blank.

Options:

(A) $\leq$ 

(B) $\geq$

(C) $=$ 

(D) $<$

(E) $>$

(F) None of the above

## Current Solution
We have
$$
\begin{aligned}
a & +b+c-\frac{1+a}{1+b}-\frac{1+b}{1+c}-\frac{1+c}{1+a} \\
& =\left(1+a-\frac{1+a}{1+b}\right)+\left(1+b-\frac{1+b}{1+c}\right)+\left(1+c-\frac{1+c}{1+a}\right)-3 \\
& =(1+a)\left(1-\frac{1}{1+b}\right)+(1+b)\left(1-\frac{1}{1+c}\right)+(1+c)\left(1-\frac{1}{1+a}\right)-3 \\
& =\frac{(1+a) b}{1+b}+\frac{(1+b) c}{1+c}+\frac{(1+c) a}{1+a}-3 \\
& \geq 3 \sqrt[3]{\frac{(1+a) b}{1+b} \cdot \frac{(1+b) c}{1+c} \cdot \frac{(1+c) a}{1+a}}-3 \\
& =3 \sqrt[3]{a b c}-3 \geq 0 \quad(a b c \geq 1)
\end{aligned}
$$

Equality occurs iff $a=b=c=1$. Therefore, the answer is (B) $\geq$.

## Expected Answer
(B) $\geq$

## Enhanced Solution
We wish to compare the two expressions

  E₁ = a + b + c
  and
  E₂ = \frac{1+a}{1+b} + \frac{1+b}{1+c} + \frac{1+c}{1+a},

under the hypothesis that a, b, c are positive real numbers with abc ≥ 1.  We will show that E₁ ≥ E₂, i.e.

  a + b + c \;≥\; \frac{1+a}{1+b} + \frac{1+b}{1+c} + \frac{1+c}{1+a}.

**Step 1: Form the difference and reorganize.**

Consider

  D = (a + b + c) 
       - \Bigl(\frac{1+a}{1+b} + \frac{1+b}{1+c} + \frac{1+c}{1+a}\Bigr).

To exploit symmetry and enable application of AM–GM, we add and subtract 3:

  D = \bigl[(a+1) - \tfrac{1+a}{1+b}\bigr]
      + \bigl[(b+1) - \tfrac{1+b}{1+c}\bigr]
      + \bigl[(c+1) - \tfrac{1+c}{1+a}\bigr]
      - 3.

**Step 2: Factor each bracket.**

For each cyclic term, observe that 1 + x > 0 and 1 + y > 0, so

  (1 + x) - \frac{1 + x}{1 + y} 
    = (1 + x)\Bigl(1 - \frac{1}{1 + y}\Bigr)
    = (1 + x)\frac{(1 + y) - 1}{1 + y}
    = \frac{(1 + x)\,y}{1 + y}.

Applying this with (x,y) = (a,b), (b,c), (c,a) gives

  D = \frac{(1+a)b}{1+b}
      + \frac{(1+b)c}{1+c}
      + \frac{(1+c)a}{1+a}
      - 3.

Each term \frac{(1+a)b}{1+b} is positive since a,b>0.

**Step 3: Apply the AM–GM inequality.**

By the arithmetic–geometric mean inequality for three positive numbers,

  \frac{X + Y + Z}{3} \;≥\; (XYZ)^{1/3},

with equality iff X = Y = Z.  Set

  X = \frac{(1+a)b}{1+b},
  Y = \frac{(1+b)c}{1+c},
  Z = \frac{(1+c)a}{1+a}.

Then

  X + Y + Z \;≥\; 3 \bigl(XYZ\bigr)^{1/3}.

Hence

  D = (X + Y + Z) - 3
    \;≥\; 3\bigl(XYZ\bigr)^{1/3} - 3.

**Step 4: Compute the product XYZ.**

Multiplying the three factors,

  XYZ
    = \frac{(1+a)b}{1+b} \cdot \frac{(1+b)c}{1+c} \cdot \frac{(1+c)a}{1+a}
    = \frac{a b c\,(1+a)(1+b)(1+c)}{(1+a)(1+b)(1+c)}
    = a b c.

Consequently,

  D \;≥\; 3\sqrt[3]{abc} - 3.

**Step 5: Use the hypothesis abc ≥ 1.**

Since abc ≥ 1, we have

  \sqrt[3]{abc} ≥ 1
  \quad⇒\quad
  3\sqrt[3]{abc} - 3 ≥ 0.

Therefore D ≥ 0, i.e.

  a + b + c - \Bigl(\frac{1+a}{1+b} + \frac{1+b}{1+c} + \frac{1+c}{1+a}\Bigr) ≥ 0,

which rearranges to the desired inequality

  a + b + c \;≥\; \frac{1+a}{1+b} + \frac{1+b}{1+c} + \frac{1+c}{1+a}.

**Step 6: Equality case.**

Equality in AM–GM holds precisely when
  X = Y = Z, 
that is,
  \frac{(1+a)b}{1+b} = \frac{(1+b)c}{1+c} = \frac{(1+c)a}{1+a}.
Coupled with abc = 1, this forces a = b = c = 1.  Thus the only equality case is a = b = c = 1.

Conclusion: We have proved

  a + b + c \;≥\; \frac{1+a}{1+b} + \frac{1+b}{1+c} + \frac{1+c}{1+a}

under the given conditions, with equality if and only if a = b = c = 1.

The answer is (B) ≥
