# Problem Entry

## Problem Type
bound

## Problem
Let $a, b, c \in (1,2)$ be real numbers. Find the largest constant $C$ such that the following inequality holds for all $a, b, c \in (1,2)$:
$$
\frac{b \sqrt{a}}{4 b \sqrt{c}-c \sqrt{a}}+\frac{c \sqrt{b}}{4 c \sqrt{a}-a \sqrt{b}}+\frac{a \sqrt{c}}{4 a \sqrt{b}-b \sqrt{c}} \geq C
$$

## Current Solution
Since $a, b, c \in(1,2)$ we have
$$
4 b \sqrt{c}-c \sqrt{a}>4 \sqrt{c}-2 \sqrt{c}=2 \sqrt{c}>0
$$

Analogously we get $4 c \sqrt{a}-a \sqrt{b}>0$ and $4 a \sqrt{b}-b \sqrt{c}>0$.
We'll prove that
$$
\begin{equation*}
\frac{b \sqrt{a}}{4 b \sqrt{c}-c \sqrt{a}} \geq \frac{a}{a+b+c} \tag{1}
\end{equation*}
$$

Since $4 b \sqrt{c}-c \sqrt{a}>0$ inequality (1) is
$$
\begin{array}{r}
b(a+b+c) \geq \sqrt{a}(4 b \sqrt{c}-c \sqrt{a}) \\
\Leftrightarrow \quad(a+b)(b+c) \geq 4 b \sqrt{a c}
\end{array}
$$
which is clearly true $(A M \geq G M)$.
Similarly we deduce that
$$
\begin{equation*}
\frac{c \sqrt{b}}{4 c \sqrt{a}-a \sqrt{b}} \geq \frac{b}{a+b+c} \tag{2}
\end{equation*}
$$
and
$$
\begin{equation*}
\frac{a \sqrt{c}}{4 a \sqrt{b}-b \sqrt{c}} \geq \frac{c}{a+b+c} \tag{3}
\end{equation*}
$$

Adding (1), (2) and (3) we get the required result.

Equality holds when $a = b = c$, and since $a, b, c \in (1,2)$, this occurs for any $a = b = c$ in $(1,2)$. In this case, each term becomes $\frac{a}{a+b+c} = \frac{1}{3}$, so the sum is $1$. This gives the minimum value of the expression, so $C = 1$ is the largest constant for which the inequality always holds.

Therefore, the answer is $C = 1$. 

## Expected Answer
$C = 1$

## Enhanced Solution
We wish to show that for all real a,b,c in the open interval (1,2),

    S = \frac{b\sqrt{a}}{4b\sqrt{c} - c\sqrt{a}} 
      + \frac{c\sqrt{b}}{4c\sqrt{a} - a\sqrt{b}} 
      + \frac{a\sqrt{c}}{4a\sqrt{b} - b\sqrt{c}} \;\ge\; C,

and then determine the largest possible constant C.  Our strategy is to bound each summand from below by a simpler fraction and then add.

1.  Positivity of denominators
--------------------------------
Since a,b,c>1, we have √a,√b,√c>1 as well.  For the first denominator,

    4b√c - c√a  >  4(1)√c - (2)√c  =  2√c  >  0.

Analogous reasoning shows 4c√a - a√b>0 and 4a√b - b√c>0.  Hence each denominator is strictly positive, and we may freely multiply or divide by these expressions without changing the direction of any inequality.

2.  Lower bound for the first term
--------------------------------------
We claim

    (1)    \frac{b\sqrt{a}}{4b\sqrt{c} - c\sqrt{a}} \;\ge\; \frac{a}{a + b + c}.

Because the denominator is positive, this is equivalent to

    b\sqrt{a} \;\bigl(a + b + c\bigr)  \;\ge\;  \; a\;\bigl(4b\sqrt{c} - c\sqrt{a}\bigr).

Expand both sides:

    LHS = b\sqrt{a}\,a + b\sqrt{a}\,b + b\sqrt{a}\,c  = a b\sqrt{a} + b^2\sqrt{a} + b c\sqrt{a},

    RHS = 4ab\sqrt{c} - a c\sqrt{a}.

Rewriting the inequality as LHS − RHS ≥ 0 gives

    a b\sqrt{a} + b^2\sqrt{a} + b c\sqrt{a}  − 4ab\sqrt{c} + a c\sqrt{a}  \ge 0

  ⇔  b^2\sqrt{a} + b c\sqrt{a} + a c\sqrt{a} + a b\sqrt{a}  − 4ab\sqrt{c}  ≥ 0

Group terms to factor (a+b)(b+c) on one side and 4b√(ac) on the other:

    (a + b)(b + c) \sqrt{a}  − 4b\sqrt{a}\sqrt{c}\sqrt{a}  ≥ 0

  ⇔  (a + b)(b + c)  ≥ 4b\sqrt{a c},

where we have divided by the positive quantity √a.  Finally, by the Arithmetic–Geometric Mean inequality applied to the two nonnegative numbers (a + b) and (b + c),

    (a + b)(b + c)  ≥  \bigl(\sqrt{(a+b)(b+c)}\bigr)^2
                  ≥  (b + \sqrt{ac})^2
                  ≥  4b\sqrt{a c},

since b + √(ac) ≥ 2√(b√(ac)) = 2b^(1/2)(ac)^(1/4)≥ 2b√(ac)/b.  Hence inequality (1) is established.

3.  Analogous bounds for the other terms
---------------------------------------------
By exactly the same reasoning, merely cycling the roles of (a,b,c) → (b,c,a) and then (c,a,b), we obtain

    (2)    \frac{c\sqrt{b}}{4c\sqrt{a} - a\sqrt{b}}  ≥  \frac{b}{a + b + c},

    (3)    \frac{a\sqrt{c}}{4a\sqrt{b} - b\sqrt{c}}  ≥  \frac{c}{a + b + c}.

4.  Summation and conclusion
--------------------------------
Adding (1), (2), (3) term by term gives

    S  =  \sum_{\mathrm{cyc}} \frac{b\sqrt{a}}{4b\sqrt{c} - c\sqrt{a}}  \;\ge\;  \sum_{\mathrm{cyc}} \frac{a}{a + b + c}  =  \frac{a + b + c}{a + b + c}  =  1.

Thus the expression S is always at least 1, so any constant C≤1 works.  

5.  Sharpness and equality case
----------------------------------
Equality in each AM–GM step, and hence in (1), (2), (3), occurs exactly when a=b=c.  Since a,b,c lie in (1,2), we can take any common value in that interval and achieve equality.  Therefore the bound is sharp, and the largest valid choice of C is 1.

The answer is $C=1$
