# Problem Entry

## Problem Type
relation

## Problem
Let $a, b, c$ be positive real numbers such that $a + b + c = 1$. Consider the following expressions:
$$
\left(a^{a} + b^{a} + c^{a}\right)\left(a^{b} + b^{b} + c^{b}\right)\left(a^{c} + b^{c} + c^{c}\right) \quad () \quad (\sqrt[3]{a} + \sqrt[3]{b} + \sqrt[3]{c})^{3}
$$
Determine the correct inequality relation to fill in the blank.

Options:

(A) $\leq$ 

(B) $\geq$

(C) $=$ 

(D) $<$

(E) $>$

(F) None of the above

## Current Solution
By Hölder's inequality we obtain
$$
\left(a^{a}+b^{a}+c^{a}\right)^{\frac{1}{3}}\left(a^{b}+b^{b}+c^{b}\right)^{\frac{1}{3}}\left(a^{c}+b^{c}+c^{c}\right)^{\frac{1}{3}} \geq a^{\frac{a+b+c}{3}}+b^{\frac{a+b+c}{3}}+c^{\frac{a+b+c}{3}}
$$

Since $a+b+c=1$, the conclusion follows. Therefore, the answer is (B) $\geq$.

## Expected Answer
(B) $\geq$

## Enhanced Solution
We wish to show in detail that for positive reals a,b,c with a+b+c=1,

    (a^a + b^a + c^a)
    · (a^b + b^b + c^b)
    · (a^c + b^c + c^c)
  ≥ (√[3]{a} + √[3]{b} + √[3]{c})^3.

We will apply Hölder’s inequality in a form adapted to three nonnegative sequences.

1.  Statement of Hölder’s inequality (three sequences).
    If {u_i}, {v_i}, {w_i} are nonnegative real sequences and p=q=r=3, then

      ∑_{i=1}^n u_i v_i w_i
      ≤ (∑_{i=1}^n u_i^3)^(1/3) · (∑_{i=1}^n v_i^3)^(1/3) · (∑_{i=1}^n w_i^3)^(1/3).

2.  Choice of sequences.
    Let the index i run over {1,2,3}.  Define
      u_i = a_i^(a/3),
      v_i = a_i^(b/3),
      w_i = a_i^(c/3),
    where (a_1,a_2,a_3) = (a,b,c).

    Then for each i,
      u_i v_i w_i = a_i^(a/3) · a_i^(b/3) · a_i^(c/3)
                 = a_i^((a+b+c)/3)
                 = a_i^(1/3)
    since a+b+c = 1.

3.  Apply Hölder.
    By Hölder’s inequality,

      ∑_{i=1}^3 u_i v_i w_i
      ≤ (∑_{i=1}^3 u_i^3)^(1/3) · (∑_{i=1}^3 v_i^3)^(1/3) · (∑_{i=1}^3 w_i^3)^(1/3).

    Substituting our definitions:

      Left‐hand side = ∑_{i=1}^3 a_i^(1/3)
                     = √[3]{a} + √[3]{b} + √[3]{c}.

      Right‐hand side factors:
        ∑_{i=1}^3 u_i^3 = ∑_{i=1}^3 a_i^a = a^a + b^a + c^a,
        ∑_{i=1}^3 v_i^3 = ∑_{i=1}^3 a_i^b = a^b + b^b + c^b,
        ∑_{i=1}^3 w_i^3 = ∑_{i=1}^3 a_i^c = a^c + b^c + c^c.

    Hence

      √[3]{a} + √[3]{b} + √[3]{c}
      ≤ (a^a + b^a + c^a)^(1/3)
        · (a^b + b^b + c^b)^(1/3)
        · (a^c + b^c + c^c)^(1/3).

4.  Raise both sides to the third power.

    Since both sides are nonnegative, we may cube the inequality without changing its direction:

      (√[3]{a} + √[3]{b} + √[3]{c})^3
      ≤ (a^a + b^a + c^a)
        · (a^b + b^b + c^b)
        · (a^c + b^c + c^c).

This is exactly the desired relation.  Therefore the correct inequality symbol is “≥”.

The answer is (B) ≥
