# Problem Entry

## Problem Type
relation

## Problem
Let $a, b, c \in (-1, 1)$ be real numbers such that $a b + b c + a c = 1$. Consider the following expressions:
$$
6 \sqrt[3]{\left(1-a^{2}\right)\left(1-b^{2}\right)\left(1-c^{2}\right)} \quad () \quad 1+(a+b+c)^{2}
$$
Determine the correct inequality relation to fill in the blank.

Options:

(A) $\leq$ 

(B) $\geq$

(C) $=$ 

(D) $<$

(E) $>$

(F) None of the above

## Current Solution
Since $a, b, c \in(-1,1)$ we have $1-a^{2}, 1-b^{2}, 1-c^{2}>0$.
By $A M \geq G M$ we get
$$
\begin{aligned}
6 \sqrt[3]{\left(1-a^{2}\right)\left(1-b^{2}\right)\left(1-c^{2}\right)} & =2 \cdot 3 \sqrt[3]{\left(1-a^{2}\right)\left(1-b^{2}\right)\left(1-c^{2}\right)} \\
& \leq 2\left(1-a^{2}+1-b^{2}+1-c^{2}\right) \\
& =2\left(3-\left(a^{2}+b^{2}+c^{2}\right)\right) \\
& =6-2\left(a^{2}+b^{2}+c^{2}\right)
\end{aligned}
$$

We'll show that
$$
6-2\left(a^{2}+b^{2}+c^{2}\right) \leq 1+(a+b+c)^{2}
$$

This inequality is equivalent to
$$
6-2\left(a^{2}+b^{2}+c^{2}\right) \leq 1+a^{2}+b^{2}+c^{2}+2
$$
i.e.
$$
3 \leq 3\left(a^{2}+b^{2}+c^{2}\right)
$$
i.e.
$$
a^{2}+b^{2}+c^{2} \geq 1
$$
which is true since $a^{2}+b^{2}+c^{2} \geq a b+b c+a c=1$.
Equality holds iff $a=b=c= \pm \frac{1}{\sqrt{3}}$. Therefore, the answer is (A) $\leq$.

## Expected Answer
(A) $\leq$

## Enhanced Solution
We wish to compare the two expressions
  E₁ = 6 \sqrt[3]{(1–a²)(1–b²)(1–c²)}
and
  E₂ = 1 + (a + b + c)²,
given that a, b, c ∈ (–1, 1) and ab + bc + ca = 1.  We will show step by step that
  E₁ ≤ E₂,
with equality precisely when a = b = c = ±1/√3.

1. Positivity and applicability of AM–GM

  Since each of a², b², c² lies in [0,1), we have
    1 – a² > 0,    1 – b² > 0,    1 – c² > 0.
  Hence the product (1–a²)(1–b²)(1–c²) is positive, and the arithmetic mean–geometric mean (AM–GM) inequality applies to the three positive numbers
    x = 1 – a²,   y = 1 – b²,   z = 1 – c².
  AM–GM gives:
    (x + y + z)/3  ≥  (xyz)^(1/3).
  Multiply both sides by 6 to relate to E₁:
    2(x + y + z)  ≥  6 (xyz)^(1/3)
  ⇔  6 \sqrt[3]{(1–a²)(1–b²)(1–c²)}  ≤  2[(1–a²) + (1–b²) + (1–c²)].
  Simplify the right side:
    (1–a²) + (1–b²) + (1–c²) = 3 – (a² + b² + c²),
  so
    E₁ = 6 \sqrt[3]{(1–a²)(1–b²)(1–c²)}  ≤  2[3 – (a² + b² + c²)]
    E₁ ≤ 6 – 2(a² + b² + c²).                      (I)

2. Comparing to E₂

  We now show that the upper bound on E₁ from (I) does not exceed E₂.  That is, we prove
    6 – 2(a² + b² + c²)  ≤  1 + (a + b + c)².
  Expand the right side:
    1 + (a + b + c)² = 1 + (a² + b² + c² + 2ab + 2bc + 2ca)
                   = (a² + b² + c²) + (2ab + 2bc + 2ca) + 1.
  Thus the inequality becomes
    6 – 2(a² + b² + c²)
      ≤ (a² + b² + c²) + 2(ab + bc + ca) + 1.
  Rearrange terms to collect like quantities on each side:
    6 – 2(a² + b² + c²) – [(a² + b² + c²) + 2(ab + bc + ca) + 1]  ≤ 0
  ⇔ 6 – 2S – S – 2T – 1  ≤ 0,  where we set S = a² + b² + c² and T = ab + bc + ca.
  Simplify constants and group S, T:
    (6 – 1) – 3S – 2T  ≤  0
  ⇔ 5 – 3S – 2T  ≤  0
  ⇔ 3S + 2T  ≥ 5.                                    (II)

3. Using the condition ab + bc + ca = 1

  We are given T = ab + bc + ca = 1.  Substitute into (II):
    3S + 2·1  ≥  5
  ⇔ 3S  ≥  3
  ⇔ S  ≥  1.
  But S = a² + b² + c².  To justify S ≥ 1, observe the well-known identity for any real a, b, c:
    (a – b)² + (b – c)² + (c – a)²  ≥  0.
  Expanding and simplifying gives
    2(a² + b² + c²) – 2(ab + bc + ca)  ≥  0
  ⇔ a² + b² + c²  ≥  ab + bc + ca.
  Since ab + bc + ca = 1, we conclude
    a² + b² + c²  ≥  1
  as required.  Hence (II) holds, and therefore
    6 – 2(a² + b² + c²)  ≤  1 + (a + b + c)².
  Together with (I) we obtain the chain
    E₁  ≤  6 – 2(a² + b² + c²)  ≤  E₂,
  establishing the desired inequality
    6 \sqrt[3]{(1–a²)(1–b²)(1–c²)}  ≤  1 + (a + b + c)².

4. Equality case

  For AM–GM to be an equality in step 1, we require
    1 – a² = 1 – b² = 1 – c²,
  hence a² = b² = c².  For the final step a² + b² + c² = ab + bc + ca to hold, we must also have (a – b)² + (b – c)² + (c – a)² = 0, which forces a = b = c.  Combining both facts yields
    a = b = c  and  a² = 1/3,
  i.e. a = b = c = ±1/√3.  One checks that ab + bc + ca = 3·(±1/√3)² = 1 indeed.

Therefore the required relational symbol is “≤”.  The answer in the prescribed format is:

The answer is (A) ≤
