# Problem Entry

## Problem Type
relation

## Problem
Let $x, y, z > 0$ satisfy the condition
$$
x + y + z = x y z.
$$
Consider the following expressions:
$$
x y + x z + y z \quad () \quad 3 + \sqrt{x^{2} + 1} + \sqrt{y^{2} + 1} + \sqrt{z^{2} + 1}.
$$
Determine the correct inequality relation to fill in the blank.

Options:

(A) $\leq$ 

(B) $\geq$

(C) $=$ 

(D) $<$

(E) $>$

(F) None of the above

## Current Solution
Another improvement is as follows. Start from

$$
\frac{1}{x^{2}}+\frac{1}{y^{2}}+\frac{1}{z^{2}} \geq \frac{1}{x y}+\frac{1}{x z}+\frac{1}{y z}=1 \Rightarrow x^{2} y^{2}+x^{2} z^{2}+y^{2} z^{2} \geq x^{2} y^{2} z^{2}
$$

which is equivalent to

$$
(x y+x z+y z)^{2} \geq 2 x y z(x+y+z)+x^{2} y^{2} z^{2}=3(x+y+z)^{2}
$$

Further on,

$$
\begin{aligned}
& (x y+x z+y z-3)^{2}=(x y+x z+y z)^{2}-6(x y+x z+y z)+9 \geq \\
& \geq 3(x+y+z)^{2}-6(x y+x z+y z)+9=3\left(x^{2}+y^{2}+z^{2}\right)+9
\end{aligned}
$$

so that

$$
x y+x z+y z \geq 3+\sqrt{3\left(x^{2}+y^{2}+z^{2}\right)+9}
$$

But

$$
\sqrt{3\left(x^{2}+y^{2}+z^{2}\right)+9} \geq \sqrt{x^{2}+1}+\sqrt{y^{2}+1}+\sqrt{z^{2}+1}
$$

is a consequence of the Cauchy-Schwarz Inequality and we have a second improvement and proof for the desired inequality:

$$
\begin{aligned}
x y+x z+y z & \geq 3+\sqrt{3\left(x^{2}+y^{2}+z^{2}\right)+9} \geq \\
& \geq 3+\sqrt{x^{2}+1}+\sqrt{y^{2}+1}+\sqrt{z^{2}+1}
\end{aligned}
$$ Therefore, the answer is (B) $\geq$.

## Expected Answer
(B) $\geq$

## Enhanced Solution
We wish to prove, for positive real x,y,z satisfying x+y+z=xyz, that

  (xy + xz + yz)   
        ?        
  3 + √(x²+1) + √(y²+1) + √(z²+1)

and to determine which of the six choices (A)≤, (B)≥, …, (F) none is correct.  The original proof shows that the “≥” direction holds; we now give a fully detailed, rigorous justification of each step.

1.  **Derive an upper bound on 1/xy + 1/yz + 1/zx via the condition x+y+z=xyz.**
   
   Since x,y,z>0, we may divide the defining equation x+y+z=xyz by xyz to obtain

      (1)
      1/yz + 1/zx + 1/xy   =   (x+y+z)/(xyz)   =   1.

2.  **Compare ∑1/x² with ∑1/(xy) by the elementary inequality (a−b)²≥0.**

   For any two positive numbers a,b we have a² + b² ≥ 2ab.  Applying this to the pairs
   (1/x,1/y), (1/y,1/z), (1/z,1/x), we get

      1/x² + 1/y²   ≥   2/(xy),
      1/y² + 1/z²   ≥   2/(yz),
      1/z² + 1/x²   ≥   2/(zx).

   Adding these three inequalities yields

      2⋅(1/x² + 1/y² + 1/z²)   ≥   2⋅(1/xy + 1/yz + 1/zx)

   or equivalently

      (2)
      1/x² + 1/y² + 1/z²   ≥   1/xy + 1/yz + 1/zx.

3.  **Combine (1) and (2) to get a polynomial inequality in x,y,z.**

   From (2) and the fact from (1) that the right–hand side equals 1, we have

      1/x² + 1/y² + 1/z²   ≥   1.

   Multiply both sides by x²y²z²>0 to obtain

      y²z² + x²z² + x²y²   ≥   x²y²z².

   Let S = xy + yz + zx.  Observe the identity

      S² = x²y² + y²z² + z²x²   +   2 xyz (x+y+z).

   Since x+y+z=xyz, we have 2xyz(x+y+z)=2x²y²z².  Hence

      S² = (x²y² + y²z² + z²x²) + 2x²y²z²
         ≥ x²y²z² + 2x²y²z²  = 3 x²y²z².

   Finally x²y²z² = (xyz)² = (x+y+z)², so we conclude

      (3)
      S²  ≥  3 (x+y+z)².

4.  **Rearrange (3) into an inequality for S−3.**

   Expand the square

      (S − 3)²   =   S² − 6S + 9.

   Using S² ≥ 3(x+y+z)², we get

      (S − 3)²  ≥  3(x+y+z)²  − 6S + 9.

   But 3(x+y+z)² = 3(x²+y²+z² + 2S) = 3(x²+y²+z²) + 6S.  Therefore

      3(x+y+z)² − 6S + 9  =  [3(x²+y²+z²) + 6S] − 6S + 9  =  3(x²+y²+z²) + 9.

   We conclude

      (4)
      (S − 3)²  ≥  3(x²+y²+z²) + 9.

   Since S=xy+yz+zx>0, taking nonnegative square roots yields

      S − 3  ≥  √[3(x²+y²+z²) + 9],

   i.e.

      (5)
      xy + yz + zx  ≥  3  +   √[3(x²+y²+z²) + 9].

5.  **Compare √[3(x²+y²+z²)+9] with √(x²+1)+√(y²+1)+√(z²+1) by Cauchy–Schwarz.**

   The Cauchy–Schwarz inequality in the form

      (1²+1²+1²)( (x²+1)+(y²+1)+(z²+1) )  ≥  [√(x²+1)+√(y²+1)+√(z²+1)]²

   gives

      3 [ (x²+y²+z²) + 3 ]  ≥  [√(x²+1)+√(y²+1)+√(z²+1)]²,

   hence

      (6)
      √[3(x²+y²+z²) + 9]   ≥   √(x²+1) + √(y²+1) + √(z²+1).

6.  **Chain the inequalities (5) and (6) to reach the final comparison.**

   From (5) we know
      xy + yz + zx  ≥  3 + √[3(x²+y²+z²) + 9],
   and from (6)
      √[3(x²+y²+z²) + 9]  ≥   √(x²+1)+√(y²+1)+√(z²+1).

   Therefore by transitivity of “≥,”

      xy + yz + zx  ≥  3  +  ( √(x²+1) + √(y²+1) + √(z²+1) ),

   which shows the correct relation sign is “≥.”

Answer: The answer is (B) ≥
