# Problem Entry

## Problem Type
relation

## Problem
Let $a, b, c \in \mathbb{R}^{+}$ with $a^{2}+b^{2}+c^{2}=3$. Consider the following expressions:
$$
\frac{a b}{c}+\frac{b c}{a}+\frac{c a}{b} \quad () \quad 3
$$
Determine the correct inequality relation to fill in the blank.

Options:

(A) $\leq$ 

(B) $\geq$

(C) $=$ 

(D) $<$

(E) $>$

(F) None of the above

## Current Solution
The given inequality is equivalent to
$$
\begin{aligned}
& \left(\frac{a b}{c}+\frac{b c}{a}+\frac{c a}{b}\right)^{2} \geq 9 \\
& \quad \Leftrightarrow \quad \frac{a^{2} b^{2}}{c^{2}}+\frac{b^{2} c^{2}}{a^{2}}+\frac{c^{2} a^{2}}{b^{2}}+2\left(a^{2}+b^{2}+c^{2}\right) \geq 3\left(a^{2}+b^{2}+c^{2}\right)
\end{aligned}
$$
i.e.
$$
\frac{a^{2} b^{2}}{c^{2}}+\frac{b^{2} c^{2}}{a^{2}}+\frac{c^{2} a^{2}}{b^{2}} \geq a^{2}+b^{2}+c^{2}
$$

Furthermore, applying $A M \geq G M$ we get
$$
\frac{a^{2} b^{2}}{c^{2}}+\frac{b^{2} c^{2}}{a^{2}} \geq 2 b^{2}, \quad \frac{b^{2} c^{2}}{a^{2}}+\frac{c^{2} a^{2}}{b^{2}} \geq 2 c^{2}, \quad \frac{a^{2} b^{2}}{c^{2}}+\frac{c^{2} a^{2}}{b^{2}} \geq 2 a^{2}
$$

After adding these inequalities we obtain
$$
\frac{a^{2} b^{2}}{c^{2}}+\frac{b^{2} c^{2}}{a^{2}}+\frac{c^{2} a^{2}}{b^{2}} \geq a^{2}+b^{2}+c^{2}
$$
and we are done. Therefore, the answer is (B) $\geq$.

## Expected Answer
(B) $\geq$

## Enhanced Solution
Enhanced Solution:

We wish to determine whether
  (ab/c + bc/a + ca/b)  ?  3,
given that a, b, c > 0 and
  a² + b² + c² = 3.
We will show step by step that
  ab/c + bc/a + ca/b ≥ 3.

1. Introduce the sum S
   Let S = ab/c + bc/a + ca/b.  Since each term is positive, S > 0.
   To compare S with 3, it suffices to compare their squares:
     S ≥ 3   ⇔   S² ≥ 9.

2. Expand S²
   Compute S² directly:
     S² = (ab/c + bc/a + ca/b)²
        = (ab/c)² + (bc/a)² + (ca/b)²
          + 2·[(ab/c)(bc/a) + (bc/a)(ca/b) + (ca/b)(ab/c)].
   Simplify each term:
     (ab/c)² = a²b² / c²,
     (bc/a)² = b²c² / a²,
     (ca/b)² = c²a² / b²,

   and for the mixed products,
     (ab/c)(bc/a) = b²,
     (bc/a)(ca/b) = c²,
     (ca/b)(ab/c) = a².

   Hence
     S² = [a²b²/c² + b²c²/a² + c²a²/b²]
           + 2·(a² + b² + c²).

3. Substitute a² + b² + c² = 3
   By hypothesis,
     a² + b² + c² = 3.
   Therefore,
     S² = (a²b²/c² + b²c²/a² + c²a²/b²) + 2·3
        = (a²b²/c² + b²c²/a² + c²a²/b²) + 6.
   The condition S² ≥ 9 becomes
     (a²b²/c² + b²c²/a² + c²a²/b²) + 6 ≥ 9
     ⇔ a²b²/c² + b²c²/a² + c²a²/b² ≥ 3.

4. Prove a²b²/c² + b²c²/a² + c²a²/b² ≥ a² + b² + c²
   Since a² + b² + c² = 3, it suffices to prove
     a²b²/c² + b²c²/a² + c²a²/b² ≥ a² + b² + c².

   We apply the AM–GM inequality in three pairwise forms:
   • Pair the first and second terms:
     (a²b²/c²) + (b²c²/a²)
       ≥ 2·√[ (a²b²/c²)·(b²c²/a²) ]
       = 2·√(b⁴) = 2b².

   • Pair the second and third terms:
     (b²c²/a²) + (c²a²/b²)
       ≥ 2·√[ (b²c²/a²)·(c²a²/b²) ]
       = 2·√(c⁴) = 2c².

   • Pair the third and first terms:
     (c²a²/b²) + (a²b²/c²)
       ≥ 2·√[ (c²a²/b²)·(a²b²/c²) ]
       = 2·√(a⁴) = 2a².

   Add these three inequalities:
     [ (a²b²/c² + b²c²/a²)  
       + (b²c²/a² + c²a²/b²) 
       + (c²a²/b² + a²b²/c² ) ]
     ≥ 2·(a² + b² + c²).

   The left-hand side counts each of the three terms a²b²/c²,
     b²c²/a², c²a²/b² exactly twice, so
     2·(a²b²/c² + b²c²/a² + c²a²/b²) ≥ 2·(a² + b² + c²).
   Divide both sides by 2:
     a²b²/c² + b²c²/a² + c²a²/b² ≥ a² + b² + c².

5. Conclude S² ≥ 9 and hence S ≥ 3
   Combining steps 3 and 4, we have shown
     a²b²/c² + b²c²/a² + c²a²/b² ≥ 3,
   so
     S² = (sum terms) + 6 ≥ 3 + 6 = 9,
   i.e. S² ≥ 9.  Since S > 0, it follows that
     S ≥ 3.

6. Final Answer
   Therefore,
     ab/c + bc/a + ca/b ≥ 3.

The answer is (B) ≥
