# Problem Entry

## Problem Type
relation

## Problem
Let $a, b, c$ be positive real numbers such that $a + b + c = 1$. Consider the following expressions:
$$
\frac{a}{a + b c} + \frac{b}{b + c a} + \frac{\sqrt{a b c}}{c + a b} \quad () \quad 1 + \frac{3 \sqrt{3}}{4}
$$
Determine the correct inequality relation to fill in the blank.

Options:

(A) $\leq$ 

(B) $\geq$

(C) $=$ 

(D) $<$

(E) $>$

(F) None of the above

## Current Solution
Since $a+b+c=1$ we use the following substitutions $a=x y, b=y z, c=$ $z x$, where $x, y, z>0$ and the given inequality becomes
$$
\frac{x y}{x y+(y z)(z x)}+\frac{y z}{y z+(z x)(x y)}+\frac{x y z}{z x+(x y)(y z)} \leq 1+\frac{3 \sqrt{3}}{4}
$$
i.e.
$$
\begin{equation*}
\frac{1}{1+z^{2}}+\frac{1}{1+x^{2}}+\frac{y}{1+y^{2}} \leq 1+\frac{3 \sqrt{3}}{4} \tag{1}
\end{equation*}
$$
where $x y+y z+z x=1$.

Since $x y+y z+z x=1$ according to Case 3 we may set $x=\tan \frac{\alpha}{2}, y=\tan \frac{\beta}{2}, z=$ $\tan \frac{\gamma}{2}$ where $\alpha, \beta, \gamma \in(0, \pi)$, and $\alpha+\beta+\gamma=\pi$.

Then inequality (1) becomes
$$
\frac{1}{1+\tan ^{2} \frac{\gamma}{2}}+\frac{1}{1+\tan ^{2} \frac{\alpha}{2}}+\frac{\tan \frac{\beta}{2}}{1+\tan ^{2} \frac{\beta}{2}} \leq 1+\frac{3 \sqrt{3}}{4}
$$
i.e.
$$
\cos ^{2} \frac{\gamma}{2}+\cos ^{2} \frac{\alpha}{2}+\frac{\sin \beta}{2} \leq 1+\frac{3 \sqrt{3}}{4}
$$

Using the trigonometric identity $\cos x=2 \cos ^{2} \frac{x}{2}-1$ the last inequality becomes
$$
\frac{\cos \gamma+1}{2}+\frac{\cos \alpha+1}{2}+\frac{\sin \beta}{2} \leq 1+\frac{3 \sqrt{3}}{4}
$$
i.e.
$$
\begin{equation*}
\cos \gamma+\cos \alpha+\sin \beta \leq \frac{3 \sqrt{3}}{2} \tag{2}
\end{equation*}
$$

We have
$$
\begin{aligned}
\cos \alpha+\cos \gamma+\sin \beta= & \cos \alpha+\cos \gamma+\sin (\pi-(\alpha+\gamma)) \\
= & \frac{2}{\sqrt{3}}\left(\frac{\sqrt{3}}{2} \cos \alpha+\frac{\sqrt{3}}{2} \cos \gamma\right) \\
& +\frac{1}{\sqrt{3}}(\sqrt{3} \sin \alpha \cos \gamma+\sqrt{3} \cos \alpha \sin \gamma) \\
\leq & \frac{1}{\sqrt{3}}\left(\frac{3}{4}+\cos ^{2} \alpha+\frac{3}{4}+\cos ^{2} \gamma\right) \\
= & \frac{1}{2 \sqrt{3}}\left(3 \sin ^{2} \alpha+\cos ^{2} \gamma+\cos ^{2} \alpha+3 \sin ^{2} \gamma\right) \\
= & \frac{\sqrt{3}}{2}+\frac{\sqrt{3}}{2}\left(\cos ^{2} \alpha+\sin ^{2} \alpha\right)+\frac{\sqrt{3}}{2}\left(\cos ^{2} \gamma+\sin ^{2} \gamma\right) \\
= & \frac{3 \sqrt{3}}{2} .
\end{aligned}
$$ Therefore, the answer is (A) $\leq$.

## Expected Answer
(A) $\leq$

## Enhanced Solution
We begin by restating the problem and its essential substitution, then transform the original sum into a symmetric trigonometric form, and finally show in a rigorous one-variable optimization that the desired inequality holds.

1.  Original expression and substitution

   We are given positive reals a, b, c with a + b + c = 1 and must compare
   E  =  a/(a + bc)
      +  b/(b + ca)
      +  √(abc)/(c + ab)
   against 1 + 3√3/4.

   A standard substitution when a + b + c = xy + yz + zx = 1 is
     a = x y,
     b = y z,
     c = z x,
   with x,y,z > 0.  Then bc = (y z)(z x) = x y z^2, etc., so
     a/(a + bc) = x y/(x y + x y z^2) = 1/(1 + z^2),
     b/(b + ca) = 1/(1 + x^2),
     √(abc)/(c + ab) = (x y z)/[z x + x y·y z]
                       = (x y z)/[x z(1 + y^2)]
                       = y/(1 + y^2).

   Hence the inequality E ≤ 1 + 3√3/4 becomes
     1/(1 + z^2)  +  1/(1 + x^2)  +  y/(1 + y^2)
     ≤  1  +  3√3/4,
   subject to x y + y z + z x = 1.

2.  Trigonometric half‐angle parametrization

   Since x y + y z + z x = 1, one may set
     x = tan(α/2),
     y = tan(β/2),
     z = tan(γ/2),
   where α, β, γ ∈ (0, π) and α + β + γ = π.  Then:

   – 1/(1 + z^2) = cos^2(γ/2).
   – 1/(1 + x^2) = cos^2(α/2).
   – y/(1 + y^2)
     = tan(β/2)/(1 + tan^2(β/2))
     = tan(β/2)/sec^2(β/2)
     = sin(β)/2.

   Thus the left side becomes
     cos^2(α/2) + cos^2(γ/2) + (sin β)/2,
   and the target inequality is
     cos^2(α/2) + cos^2(γ/2) + (sin β)/2
     ≤ 1 + 3√3/4.

3.  Rewriting in terms of cos α, cos γ, and sin β

   Use cos^2(t/2) = (1 + cos t)/2.  Then
     cos^2(α/2) + cos^2(γ/2)
     = (1 + cos α)/2 + (1 + cos γ)/2
     = 1 + (cos α + cos γ)/2.

   Hence the inequality is equivalent to
     1 + [cos α + cos γ]/2  +  (sin β)/2
     ≤ 1 + 3√3/4,
   i.e.
     cos α + cos γ + sin β  ≤  3√3/2.           (★)

4.  Reduction to one variable via symmetry

   Observe that β = π − (α + γ), so sin β = sin(α + γ).  Define S = α + γ.  Then α, γ > 0, S ∈ (0, π), and the expression
     F(α, γ) = cos α + cos γ + sin(α + γ)
   under fixed S is symmetric in α, γ, so its maximum on α + γ = S occurs when α = γ = S/2.  Hence it suffices to study the one‐variable function
     G(S) = 2 cos(S/2) + sin S,
   for 0 < S < π, and show G(S) ≤ 3√3/2.

5.  Maximizing G(S)

   Compute the derivative:
     G′(S) = − sin(S/2) + cos S.
   Setting G′(S) = 0 gives
     cos S = sin(S/2).
   Using the identity sin(S/2) = √[(1 − cos S)/2], square both sides:
     cos^2 S = (1 − cos S)/2
     ⇔ 2 cos^2 S + cos S − 1 = 0
     ⇔ (2 cos S − 1)(cos S + 1) = 0.
   In (0, π) the only solution is cos S = 1/2, i.e. S = π/3.  We compare endpoint values as well:

   – As S → 0+, G(S) → 2·1 + 0 = 2.
   – As S = π/3, G(π/3) = 2 cos(π/6) + sin(π/3) = 2·(√3/2) + (√3/2) = 3√3/2 ≈ 2.598.
   – As S → π−, G(S) → 2·0 + 0 = 0.

   Hence the maximum of G on (0, π) is G(π/3) = 3√3/2.  Therefore for all permissible α, γ, β,
     cos α + cos γ + sin β  ≤  3√3/2,
   establishing (★).

6.  Conclusion

   Retracing our substitutions shows the original sum
     = cos^2(α/2) + cos^2(γ/2) + (sin β)/2
     ≤ 1 + 3√3/4.
   Thus the correct relation is “≤.”

The answer is (A) ≤
