# Problem Entry

## Problem Type
relation

## Problem
Let $a_{1}, a_{2}, \ldots, a_{n}$ be positive real numbers such that $a_{1}+a_{2}+\cdots+a_{n}=1$. Consider the following inequality:
$$
\frac{a_{1}}{\sqrt{1-a_{1}}}+\frac{a_{2}}{\sqrt{1-a_{2}}}+\cdots+\frac{a_{n}}{\sqrt{1-a_{n}}} \quad () \quad \sqrt{\frac{n}{n-1}} .
$$

Determine the correct inequality relation to fill in the blank.

Options:

(A) $\leq$ 

(B) $\geq$

(C) $=$ 

(D) $<$

(E) $>$

(F) None of the above

## Current Solution
Let us denote
$$
\begin{aligned}
& A=\frac{a_{1}}{\sqrt{1-a_{1}}}+\frac{a_{2}}{\sqrt{1-a_{2}}}+\cdots+\frac{a_{n}}{\sqrt{1-a_{n}}} \\
& B=a_{1}\left(1-a_{1}\right)+a_{2}\left(1-a_{2}\right)+\cdots+a_{n}\left(1-a_{n}\right)
\end{aligned}
$$

By Hölder's inequality we have
$$
\begin{equation*}
A^{2} B \geq\left(a_{1}+a_{2}+\cdots+a_{n}\right)^{3}=1 \tag{1}
\end{equation*}
$$

Applying $Q M \geq A M$ we deduce
$$
\begin{equation*}
B=1-\left(a_{1}^{2}+a_{2}^{2}+\cdots+a_{n}^{2}\right) \leq 1-\frac{\left(a_{1}+a_{2}+\cdots+a_{n}\right)^{2}}{n}=\frac{n-1}{n} \tag{2}
\end{equation*}
$$

By (1) and (2) we obtain
$$
\frac{n-1}{n} \cdot A^{2} \geq A^{2} B \geq 1, \quad \text { i.e. } \quad A \geq \sqrt{\frac{n}{n-1}}
$$

Equality holds iff $a_{i}=\frac{1}{n}$, for every $i=1,2, \ldots, n$. Therefore, the answer is (B) $\geq$.

## Expected Answer
(B) $\geq$

## Enhanced Solution
Enhanced Solution:

We wish to show that for any positive real numbers a_{1},a_{2},…,a_{n} with sum 1,

      A := \sum_{i=1}^{n} \frac{a_{i}}{\sqrt{1 - a_{i}}}

satisfies

      A \ge \sqrt{\frac{n}{n - 1}}.

Our proof proceeds in two main steps:

1.  A Hölder‐type (or Cauchy–Schwarz) estimate giving A^{2}·B \ge 1, where

        B := \sum_{i=1}^{n} a_{i}(1 - a_{i}).

2.  A QM–AM (quadratic mean–arithmetic mean) estimate showing B \le \tfrac{n - 1}{n}.

Combining these two yields the desired lower bound on A.

Step 1: Establishing A^{2}·B \ge 1
--------------------------------------------------

Define two sequences of nonnegative numbers:

    x_{i} := \frac{a_{i}}{\sqrt{1 - a_{i}}},
    y_{i} := \sqrt{1 - a_{i}},

for i = 1,…,n.  Then x_{i}·y_{i} = a_{i}.  By the Cauchy–Schwarz inequality we have

    \Bigl(\sum_{i=1}^{n} x_{i}y_{i}\Bigr)^{2}
    \;\le\;
    \Bigl(\sum_{i=1}^{n} x_{i}^{2}\Bigr)\,\Bigl(\sum_{i=1}^{n} y_{i}^{2}\Bigr).

Observing that

    \sum_{i=1}^{n} x_{i}y_{i} = \sum_{i=1}^{n} a_{i} = 1,
    \sum_{i=1}^{n} x_{i}^{2} = \sum_{i=1}^{n} \frac{a_{i}^{2}}{1 - a_{i}},
    \sum_{i=1}^{n} y_{i}^{2} = \sum_{i=1}^{n} (1 - a_{i}) = B,

we obtain

    1^{2} \;\le\; \Bigl(\sum_{i=1}^{n} \frac{a_{i}^{2}}{1 - a_{i}}\Bigr)\,B.

On the other hand, by the Cauchy–Schwarz inequality again (or by a direct rearrangement argument), one checks

    \sum_{i=1}^{n} \frac{a_{i}^{2}}{1 - a_{i}}
    \;\le\;
    \Bigl(\sum_{i=1}^{n} \frac{a_{i}}{\sqrt{1 - a_{i}}}\Bigr)^{2}
    = A^{2}.

Combining, we conclude

    A^{2}\,B \;\ge\; 1.

Thus

    (1) \quad A^{2}B \ge 1.

Step 2: Establishing B \le (n - 1)/n
--------------------------------------------------

By definition,

    B = \sum_{i=1}^{n} a_{i}(1 - a_{i})
      = \sum_{i=1}^{n} a_{i} \;-
        \sum_{i=1}^{n} a_{i}^{2}
      = 1 - \sum_{i=1}^{n} a_{i}^{2}.

We now invoke the quadratic mean–arithmetic mean (QM–AM) inequality on the set \{a_{1},…,a_{n}\}:

    \sqrt{\frac{a_{1}^{2} + a_{2}^{2} + \cdots + a_{n}^{2}}{n}}
    \;\ge\;
    \frac{a_{1} + a_{2} + \cdots + a_{n}}{n}
    = \frac{1}{n}.

Squaring both sides gives

    \sum_{i=1}^{n} a_{i}^{2} \;\ge\; \frac{1}{n}.

Hence

    B = 1 - \sum_{i=1}^{n} a_{i}^{2}
      \le 1 - \frac{1}{n}
      = \frac{n - 1}{n}.

Thus

    (2) \quad B \le \frac{n - 1}{n}.

Step 3: Combining (1) and (2)
--------------------------------------------------

From (2) we replace B in (1) by its upper bound:

    A^{2} \cdot \frac{n - 1}{n} \ge A^{2}B \ge 1
    \quad\Longrightarrow\quad
    A^{2} \ge \frac{n}{n - 1}
    \quad\Longrightarrow\quad
    A \ge \sqrt{\frac{n}{n - 1}},

where we took the positive square root since A is clearly positive.

Equality Case
--------------

Both inequalities become equalities precisely when all a_{i} are equal.  Indeed:

•  In the QM–AM step equality holds iff a_{1}=a_{2}=⋯=a_{n}.
•  In the Cauchy–Schwarz step equality holds when the vectors (x_{1},…,x_{n}) and (y_{1},…,y_{n}) are proportional, which also forces a_{1}=⋯=a_{n}.

Since their sum is 1, each a_{i}=1/n, verifying that equality occurs in that case.

Conclusion
----------

We have shown

    \sum_{i=1}^{n} \frac{a_{i}}{\sqrt{1 - a_{i}}}
    \;\ge\;
    \sqrt{\frac{n}{n - 1}},

with equality iff a_{1}=a_{2}=⋯=a_{n}=1/n.  Therefore, the correct inequality is

"The answer is (B) ≥".
