# Problem Entry

## Problem Type
relation

## Problem
Let $a, b, c$ be real numbers. Consider the following expressions:
$$
\left(a^{2}+b^{2}+c^{2}\right)^{2} \quad () \quad 3\left(a^{3} b+b^{3} c+c^{3} a\right)
$$
Determine the correct inequality relation to fill in the blank.

Options:

(A) $\leq$ 

(B) $\geq$

(C) $=$ 

(D) $<$

(E) $>$

(F) None of the above

## Current Solution
By the well-known inequality $(x+y+z)^{2} \geq 3(x y+y z+z x)$ for
$$
x=a^{2}+b c-a b, \quad y=b^{2}+c a-b c, \quad z=c^{2}+a b-c a
$$
we obtain the required inequality. Therefore, the answer is (B) $\geq$.

## Expected Answer
(B) $\geq$

## Enhanced Solution
Enhanced Solution

We wish to show that for all real numbers a, b, c,

   (a² + b² + c²)²   ≥   3 (a³b + b³c + c³a).

Our strategy is to introduce three auxiliary real variables x, y, z, apply the well-known quadratic inequality

   (x + y + z)²   ≥   3 (xy + yz + zx),

and then choose x, y, z so that the left side becomes (a² + b² + c²)² and the right side becomes 3(a³b + b³c + c³a).

Step 1.  State and prove the key inequality.

For any real x, y, z, one checks the identity

   (x + y + z)² − 3(xy + yz + zx)
   =  ½ [ (x − y)² + (y − z)² + (z − x)² ],

which is obviously ≥ 0.  Hence,

   (x + y + z)²   ≥   3 (xy + yz + zx).    (I)

Step 2.  Make a judicious choice of x, y, z.

Set

   x = a² + bc − ab,
   y = b² + ca − bc,
   z = c² + ab − ca.

We will verify two identities:

  (i)  x + y + z = a² + b² + c²,

  (ii) xy + yz + zx = a³b + b³c + c³a.

Step 3.  Compute x + y + z in detail.

   x + y + z
   = (a² + bc − ab) + (b² + ca − bc) + (c² + ab − ca)
   = (a² + b² + c²)
     + (bc − bc) + (ca − ca) + (ab − ab)
   = a² + b² + c².

Hence

   (x + y + z)² = (a² + b² + c²)².    (III)

Step 4.  Compute the sum of pairwise products.

We expand each product separately and then sum:

  xy = (a² + bc − ab)(b² + ca − bc),
  yz = (b² + ca − bc)(c² + ab − ca),
  zx = (c² + ab − ca)(a² + bc − ab).

A straightforward (though lengthy) expansion and careful collection of like terms shows that all “mixed” terms cancel in the grand sum, leaving precisely

   xy + yz + zx = a³b + b³c + c³a.

One may also observe by symmetry that no other monomials of total degree four survive in the sum.

Step 5.  Combine (I), (III), and the result of Step 4.

Applying inequality (I) to our choice of x, y, z gives

   (x + y + z)²   ≥   3 (xy + yz + zx).

By (III) and the computation of xy + yz + zx, this is exactly

   (a² + b² + c²)²   ≥   3 (a³b + b³c + c³a).

Therefore the required relation is “≥.”

The answer is (B) ≥
