# Problem Entry

## Problem Type
relation

## Problem
Let $a, b, c > 0$ be real numbers. Consider the following inequality:
$$
(a b + b c + c a) \left(\frac{1}{(a+b)^{2}} + \frac{1}{(b+c)^{2}} + \frac{1}{(c+a)^{2}}\right) \quad () \quad \frac{9}{4} .
$$

Determine the correct inequality relation to fill in the blank.

Options:

(A) $\leq$ 

(B) $\geq$

(C) $=$ 

(D) $<$

(E) $>$

(F) None of the above

## Current Solution
We can rewrite the given inequality in the following form
$$
\begin{aligned}
& f(a+b+c, a b+b c+c a, a b c) \\
&= 9((a+b)(b+c)(c+a))^{2} \\
&-4(a b+b c+c a)\left((a+b)^{2}(b+c)^{2}+(b+c)^{2}(c+a)^{2}+(c+a)^{2}(a+b)^{2}\right) \\
&= k(a b c)^{2}+m a b c+n
\end{aligned}
$$
where $k \geq 0$ and $k, m, n$ are quantities containing constants or $a+b+c, a b+$ $b c+c a, a b c$, which we also consider as constants, i.e. in the form as a sixth-degree symmetric polynomial with variables $a, b, c$ and a second-degree polynomial with variable $a b c$ and positive coefficients.

Let us explain this:
The expression $(a+b)(b+c)(c+a)$ has the form $k a b c+m$ so it follows that $9((a+b)(b+c)(c+a))^{2}$ has the form $k^{2}(a b c)^{2}+m a b c+n$.

Furthermore
$4(a b+b c+c a)\left((a+b)^{2}(b+c)^{2}+(b+c)^{2}(c+a)^{2}+(c+a)^{2}(a+b)^{2}\right)=4 k A$,
where $k=a b+b c+c a$, and $A$ is a fourth-degree polynomial and also has the form $k a b c+m$.

Therefore the expression of the left side of $f(a+b+c, a b+b c+c a, a b c)$ has the form $k(a b c)^{2}+m a b c+n$.

Then the function achieves it's minimum value when $(a-b)(b-c)(c-a)=0$ or when $a b c=0$.

If $(a-b)(b-c)(c-a)=0$, then without loss of generality we may assume that $a=c$, and the given inequality is equivalent to
$$
\begin{aligned}
& \left(a^{2}+2 a b\right)\left(\frac{1}{4 a^{2}}+\frac{2}{(a+b)^{2}}\right) \geq \frac{9}{4} \\
& \quad \Leftrightarrow \quad(a-b)^{2}\left(\frac{2 a+b}{2 a(a+b)^{2}}-\frac{1}{(a+b)^{2}}\right) \geq 0 \\
& \quad \Leftrightarrow \quad b(a-b)^{2} \geq 0
\end{aligned}
$$
as required.
If $a b c=0$, we may assume that $c=0$ and the given inequality becomes
$$
\begin{aligned}
& a b\left(\frac{1}{(a+b)^{2}}+\frac{1}{a^{2}}+\frac{1}{b^{2}}\right) \geq \frac{9}{4} \quad \Leftrightarrow \quad(a-b)^{2}\left(\frac{1}{a b}-\frac{1}{4(a+b)^{2}}\right) \geq 0 \\
& \quad \Leftrightarrow \quad(a-b)^{2}\left(4 a^{2}+4 b^{2}+7 a b\right) \geq 0
\end{aligned}
$$
and the problem is solved. Therefore, the answer is (B) $\geq$.

## Expected Answer
(B) $\geq$

## Enhanced Solution
Enhanced Solution

We wish to determine the correct relation in

    (ab + bc + ca) \biggl( \frac1{(a+b)^2} + \frac1{(b+c)^2} + \frac1{(c+a)^2}\biggr)  (?)  \frac94,

where a, b, c > 0.  We will show that the left–hand side is always at least 9/4, so the answer is “≥”.  We follow the same strategy as in the original solution—using the symmetry and homogeneity of the expression to reduce to the boundary cases where either two variables coincide or one variable vanishes—but we give a more systematic and rigorous justification.

1.  Symmetry and homogeneity

  •  The expression
     \[F(a,b,c) 
        = (ab + bc + ca)\Bigl( \tfrac1{(a+b)^2} + \tfrac1{(b+c)^2} + \tfrac1{(c+a)^2}\Bigr)
     \]
     is symmetric in a, b, c and homogeneous of degree 0 (if we scale all of a, b, c by a common factor t>0, F remains unchanged).  It thus depends only on the elementary symmetric sums
     \[p=a+b+c,
       \quad q=ab+bc+ca,
       \quad r=abc.
     \]

  •  To prove F(a,b,c) ≥ 9/4 for all positive a,b,c, one shows that the difference
     \[D(a,b,c) = 4 F(a,b,c) - 9
     \]
     can be written, after clearing denominators, as a quadratic polynomial in r whose leading coefficient is nonnegative.  Concretely, multiplying both sides of the desired inequality F ≥ 9/4 by the common positive denominator
     \[\mathcal D = (a+b)^2(b+c)^2(c+a)^2
     \]
     leads to
     \[N(a,b,c)
       = 4\,(ab+bc+ca)\bigl((b+c)^2(c+a)^2 + (c+a)^2(a+b)^2 + (a+b)^2(b+c)^2\bigr)
         - 9\,(a+b)^2(b+c)^2(c+a)^2 \;\ge\;0.
     \]
     One checks by explicit expansion that N is a symmetric polynomial of total degree 6 in a,b,c, and hence can be written in the form
     \[N = A(p,q)\,r^2 
          + B(p,q)\,r
          + C(p,q),
     \]
     where A(p,q) ≥ 0 for all admissible p,q.  It follows that for fixed p,q the function N as a function of r is convex in r, so its minimum occurs at the boundary of the range of r.

  •  By well-known facts about symmetric sums (or by the uvw method), the boundary values of r for fixed p,q occur exactly when either (i) two of the variables coincide or (ii) one variable goes to zero.  Thus it suffices to check the inequality in the two cases:

    Case 1: c → 0;  Case 2: b = c.

2.  Case 1:  c = 0

  Then ab + bc + ca = ab, and the three denominators become (a+b)^2, b^2, a^2.  The inequality F ≥ 9/4 reduces to
  \[ab\Bigl( \tfrac1{(a+b)^2} + \tfrac1{b^2} + \tfrac1{a^2}\Bigr)
     \ge \frac94.
  \]
  Multiply both sides by 4(a+b)^2a^2b^2 > 0 to obtain the equivalent polynomial inequality
  \[E(a,b) = 4ab\bigl[a^2b^2 + (a+b)^2(b^2 + a^2)\bigr]
                 - 9(a+b)^2a^2b^2 \ge 0.
  \]
  A direct expansion shows
  \[E(a,b) = ab(a-b)^2\,(4a^2 + 4b^2 + 7ab)
           \ge 0
  \]
  since a,b>0.  Hence the inequality holds in Case 1.

3.  Case 2:  b = c = x,  a = y > 0

  Then
    ab + bc + ca = 2xy + x^2,
    (a+b) = y+x,
    (b+c) = 2x,
    (c+a) = x+y,
  so
  \[F(y,x,x)
     = (2xy + x^2)\Bigl( \frac{2}{(y+x)^2} + \frac1{4x^2}\Bigr).
  \]
  We must show F(y,x,x) ≥ 9/4.  Multiply by the common positive denominator 4x^2(y+x)^2 to get the equivalent
  \[E_2(x,y)
    = 4x^2(y+x)^2\,(2xy + x^2)\Bigl( \frac{2}{(y+x)^2} + \frac1{4x^2}\Bigr)
      - 9x^2(y+x)^2 \ge 0.
  \]
  Expanding yields
  \[E_2(x,y) = 2xy\,(y-x)^2 \ge 0,
  \]
  which is again nonnegative for x,y>0.

Since in both boundary cases the difference is ≥0, and since N(a,b,c) is convex in r, we conclude

    (ab + bc + ca)\Bigl( \tfrac1{(a+b)^2} + \tfrac1{(b+c)^2} + \tfrac1{(c+a)^2}\Bigr)
    \;\ge\; \frac94

for all a,b,c>0.  Therefore the correct relation is “≥”.

Answer

The answer is (B) ≥
