# Problem Entry

## Problem Type
relation

## Problem
Let $x, y, z \in \mathbb{R}^{+}$ such that $x + y + z = 1$. Consider the following expressions:
$$
\frac{x y}{z}+\frac{y z}{x}+\frac{z x}{y} \quad () \quad 1
$$
Determine the correct inequality relation to fill in the blank.

Options:

(A) $\leq$ 

(B) $\geq$

(C) $=$ 

(D) $<$

(E) $>$

(F) None of the above

## Current Solution
We have
$$
\begin{equation*}
\frac{x y}{z}+\frac{y z}{x}+\frac{z x}{y}=\frac{1}{2}\left(\frac{x y}{z}+\frac{y z}{x}\right)+\frac{1}{2}\left(\frac{y z}{x}+\frac{z x}{y}\right)+\frac{1}{2}\left(\frac{z x}{y}+\frac{x y}{z}\right) \tag{1}
\end{equation*}
$$

Since $A M \geq G M$ we have
$$
\frac{1}{2}\left(\frac{x y}{z}+\frac{y z}{x}\right) \geq \sqrt{\frac{x y}{z} \frac{y z}{x}}=y
$$

Analogously we get
$$
\frac{1}{2}\left(\frac{y z}{x}+\frac{z x}{y}\right) \geq z \quad \text { and } \quad \frac{1}{2}\left(\frac{z x}{y}+\frac{x y}{z}\right) \geq x
$$

Adding these three inequalities we obtain
$$
\frac{x y}{z}+\frac{y z}{x}+\frac{z x}{y} \geq x+y+z=1
$$

Equality holds if and only if $\frac{x y}{z}=\frac{y z}{x}=\frac{z x}{y}$, i.e. $x=y=z$. Since $x+y+z=1$ we get that equality holds iff $x=y=z=1 / 3$. Therefore, the answer is (B) $\geq$.

## Expected Answer
(B) $\geq$

## Enhanced Solution
Enhanced Detailed Solution:

Let x, y, z be positive real numbers satisfying x + y + z = 1. We wish to determine the correct inequality relation between

    S = \frac{x y}{z} + \frac{y z}{x} + \frac{z x}{y}

and the constant 1.

Step 1: Symmetric pairwise decomposition
--------------------------------------
We rewrite S as a sum of three pairwise averages. Observe that each term in S will appear twice if we sum the following three expressions and then divide by 2:

    (i)   \frac{1}{2}\Bigl(\frac{x y}{z} + \frac{y z}{x}\Bigr),
    (ii)  \frac{1}{2}\Bigl(\frac{y z}{x} + \frac{z x}{y}\Bigr),
    (iii) \frac{1}{2}\Bigl(\frac{z x}{y} + \frac{x y}{z}\Bigr).

Indeed, adding (i), (ii), and (iii) gives exactly

    \frac{x y}{z} + \frac{y z}{x} + \frac{z x}{y}.

Step 2: Application of the Arithmetic Mean–Geometric Mean inequality
-------------------------------------------------------------------
Recall the AM–GM inequality: for any two positive numbers A and B,

    \frac{A + B}{2} \ge \sqrt{A B},

with equality if and only if A = B.

We apply AM–GM to each of the three pairwise averages:

1. For A = \frac{x y}{z} and B = \frac{y z}{x},

    \frac{1}{2}\Bigl(\frac{x y}{z} + \frac{y z}{x}\Bigr) \ge \sqrt{\frac{x y}{z} \cdot \frac{y z}{x}} = \sqrt{y^2} = y.

2. For A = \frac{y z}{x} and B = \frac{z x}{y},

    \frac{1}{2}\Bigl(\frac{y z}{x} + \frac{z x}{y}\Bigr) \ge \sqrt{\frac{y z}{x} \cdot \frac{z x}{y}} = \sqrt{z^2} = z.

3. For A = \frac{z x}{y} and B = \frac{x y}{z},

    \frac{1}{2}\Bigl(\frac{z x}{y} + \frac{x y}{z}\Bigr) \ge \sqrt{\frac{z x}{y} \cdot \frac{x y}{z}} = \sqrt{x^2} = x.

Step 3: Summing the three inequalities
---------------------------------------
Adding the three results from Step 2 yields

    \frac{x y}{z} + \frac{y z}{x} + \frac{z x}{y} \ge x + y + z.

Since x + y + z = 1 by hypothesis, we conclude

    S = \frac{x y}{z} + \frac{y z}{x} + \frac{z x}{y} \ge 1.

Step 4: Condition for equality
-------------------------------
Equality in each AM–GM application occurs exactly when the two terms are equal:

    \frac{x y}{z} = \frac{y z}{x},  \quad \frac{y z}{x} = \frac{z x}{y},  \quad \frac{z x}{y} = \frac{x y}{z}.

From \frac{x y}{z} = \frac{y z}{x} we get x^2 = z^2, hence x = z (positivity ensures no sign ambiguity). Similarly, the other equalities force x = y = z. Combined with x + y + z = 1, we find x = y = z = 1/3.

Thus S \ge 1 for all positive x,y,z summing to 1, and equality holds precisely when x = y = z = 1/3.

Final Answer:
The answer is (B) ≥
