# Problem Entry

## Problem Type
bound

## Problem
Let $a, b, c$ be positive real numbers such that $a + b + c = 3$. Determine the largest constant $C$ such that the following inequality holds for all $a, b, c$:
$$
\frac{a^{3}+2}{b+2}+\frac{b^{3}+2}{c+2}+\frac{c^{3}+2}{a+2} \geq C.
$$

## Current Solution
By $A M \geq G M$ we have
$$
\frac{a^{3}+2}{b+2}=\frac{a^{3}+1+1}{b+2} \geq \frac{3 \sqrt[3]{a^{3} \cdot 1 \cdot 1}}{b+2}=\frac{3 a}{b+2}
$$

Similarly we get
$$
\frac{b^{3}+2}{c+2} \geq \frac{3 b}{c+2} \quad \text { and } \quad \frac{c^{3}+2}{a+2} \geq \frac{3 c}{a+2}
$$

Therefore
$$
\begin{equation*}
\frac{a^{3}+2}{b+2}+\frac{b^{3}+2}{c+2}+\frac{c^{3}+2}{a+2} \geq 3\left(\frac{a}{b+2}+\frac{b}{c+2}+\frac{c}{a+2}\right) \tag{1}
\end{equation*}
$$

Applying the Cauchy-Schwarz inequality we obtain
$$
\begin{align*}
\frac{a}{b+2}+\frac{b}{c+2}+\frac{c}{a+2} & =\frac{a^{2}}{a(b+2)}+\frac{b^{2}}{b(c+2)}+\frac{c^{2}}{c(a+2)} \\
& \geq \frac{(a+b+c)^{2}}{a(b+2)+b(c+2)+c(a+2)} \\
& =\frac{(a+b+c)^{2}}{a b+b c+c a+2(a+b+c)} \tag{2}
\end{align*}
$$

Since $(a+b+c)^{2} \geq 3(a b+b c+c a)$ we deduce that
$$
\begin{equation*}
\frac{1}{a b+b c+c a} \geq \frac{3}{(a+b+c)^{2}} \tag{3}
\end{equation*}
$$

From (2) and (3) we get
$$
\begin{align*}
\frac{a}{b+2}+\frac{b}{c+2}+\frac{c}{a+2} & \geq \frac{(a+b+c)^{2}}{a b+b c+c a+2(a+b+c)} \\
& \geq \frac{(a+b+c)^{2}}{(a+b+c)^{2} / 3+2(a+b+c)} \\
& =\frac{3(a+b+c)^{2}}{(a+b+c)^{2}+6(a+b+c)}=\frac{3(a+b+c)}{(a+b+c)+6} \tag{4}
\end{align*}
$$

Finally by (1), (4) and since $a+b+c=3$ we obtain
$$
A \geq 3\left(\frac{a}{b+2}+\frac{b}{c+2}+\frac{c}{a+2}\right) \geq \frac{9(a+b+c)}{(a+b+c)+6}=\frac{27}{9}=3
$$
as required. Equality occurs iff $a=b=c=1$.

Equality holds when $a = b = c = 1$, since then $a + b + c = 3$ and each term becomes $\frac{1^3 + 2}{1 + 2} = 1$, so the sum is $3$. Thus, the minimum value of the expression is $3$, so the largest constant $C$ is $3$.

Therefore, the answer is $C = 3$. 

## Expected Answer
$C = 3$

## Enhanced Solution
We wish to show that for all positive real numbers a, b, c satisfying a + b + c = 3,

    (a³ + 2)/(b + 2) + (b³ + 2)/(c + 2) + (c³ + 2)/(a + 2) ≥ C,

and to determine the largest possible constant C.  The original solution proceeds in two main steps: first applying the AM–GM inequality to each numerator, then applying the Cauchy–Schwarz inequality (together with a classical bound on ab + bc + ca) to the resulting cyclic sum.  We now present a fully detailed and rigorous derivation of the same result, preserving exactly that approach and arriving at the same final answer.

Step 1.  Reduction via AM–GM on each term

Fix one of the three fractions, say

    (a³ + 2)/(b + 2).

Observe that a³ + 2 = a³ + 1 + 1.  By the arithmetic–geometric mean inequality (AM–GM) for three nonnegative numbers x, y, z, we have

    (x + y + z)/3 ≥ ³√(xyz),

with equality if and only if x = y = z.  Applying this to x = a³, y = 1, z = 1, we get

    (a³ + 1 + 1)/3 ≥ ³√(a³·1·1) = a.

Hence

    a³ + 2 ≥ 3a,

and therefore

    (a³ + 2)/(b + 2) ≥ (3a)/(b + 2).

Exactly the same reasoning applies cyclically to the other two terms.  Summing these three inequalities yields

    (a³ + 2)/(b + 2) + (b³ + 2)/(c + 2) + (c³ + 2)/(a + 2)
      ≥ 3 [ a/(b + 2) + b/(c + 2) + c/(a + 2) ].

We label this reduction as inequality (1):

    (1)   A ≔ LHS ≥ 3·S ,   where   S = a/(b+2) + b/(c+2) + c/(a+2).

Step 2.  Lower bound for S via Cauchy–Schwarz and a bound on ab + bc + ca

We next produce a lower bound for the sum S.  Observe that each term a/(b+2) can be rewritten as a²/[a(b + 2)].  Thus

    S = a/(b+2) + b/(c+2) + c/(a+2)
      = a²/[a(b+2)] + b²/[b(c+2)] + c²/[c(a+2)].

We now apply the Cauchy–Schwarz inequality in the Titu’s lemma form:

    For any nonnegative u_i and positive v_i,  ∑(u_i²/v_i) ≥ (∑u_i)² / (∑v_i).

Here we take u₁ = a, v₁ = a(b+2);  u₂ = b, v₂ = b(c+2);  u₃ = c, v₃ = c(a+2).  Then

    a²/[a(b+2)] + b²/[b(c+2)] + c²/[c(a+2)]
      ≥ (a + b + c)² / [ a(b+2) + b(c+2) + c(a+2) ].

Since a + b + c = 3 by hypothesis, the numerator is (a + b + c)² = 9.  Hence

    S ≥ 9 / [ a(b+2) + b(c+2) + c(a+2) ].

Expand the denominator:

    a(b+2) + b(c+2) + c(a+2)
    = ab + 2a + bc + 2b + ca + 2c
    = (ab + bc + ca) + 2(a + b + c)
    = (ab + bc + ca) + 2·3
    = (ab + bc + ca) + 6.

Thus

    (2)   S ≥ 9 / [ (ab + bc + ca) + 6 ].

At this point we invoke a well-known inequality for nonnegative a, b, c:

    (a + b + c)² ≥ 3(ab + bc + ca),

which for a + b + c = 3 becomes

    9 ≥ 3(ab + bc + ca)   ⇒   ab + bc + ca ≤ 3.

Since ab + bc + ca is positive, we may safely invert the inequality to obtain

    1 / (ab + bc + ca) ≥ 1/3.

Equivalently,

    1 / [ (ab + bc + ca) + 6 ]
      = 1 / [ (ab + bc + ca) ] · 1 / [ 1 + 6/(ab + bc + ca) ]
      ≥ (1/3) · 1 / [ 1 + 6/3 ]
      = (1/3) · 1/3 = 1/9.

However, a more direct combination is obtained by observing

    ab + bc + ca ≤ (a + b + c)²/3 = 9/3 = 3
    ⇒ (ab + bc + ca) + 6 ≤ 3 + 6 = 9
    ⇒ 1/[(ab + bc + ca) + 6] ≥ 1/9.

Inserting this into (2) gives

    S ≥ 9 · (1/9) = 1.

Thus we have established the sharper bound

    (3)   S ≥ 3(a+b+c)/[(a+b+c)+6]  = 3·3/(3+6) = 1,

which coincides numerically with the previous conclusion.  For clarity, one can also rewrite (2) and then use ab + bc + ca ≤ 3 to get

    S ≥ 9 / [ (ab + bc + ca) + 6 ]
      ≥ 9 / (3 + 6) = 9/9 = 1.

Step 3.  Conclusion and determination of C

Combining (1) and the bound S ≥ 1, we obtain

    A = (a³+2)/(b+2) + (b³+2)/(c+2) + (c³+2)/(a+2)
      ≥ 3 · S
      ≥ 3 · 1
      = 3.

Hence for all positive a, b, c with a + b + c = 3, the given expression is at least 3.  Moreover, checking the case of equality in all the used inequalities:

  • In the AM–GM step x = a³, y = 1, z = 1 we need a³ = 1 = 1, so a = 1.
  • Cyclically, this forces b = c = 1.
  • In the Cauchy–Schwarz step equality requires the ratios u_i/v_i to be equal, which also holds when a = b = c.
  • Finally, in the bound ab + bc + ca ≤ 3 we have equality when a = b = c.

Thus equality throughout occurs exactly at a = b = c = 1, giving the expression value 3.  It follows that the largest constant C for which the inequality holds in all cases is

The answer is $C=3$
