# Problem Entry

## Problem Type
relation

## Problem
Let $a, b, c$ be positive real numbers such that $a b c = 1$. Consider the following inequality:
$$
\frac{1}{a^{3}(b+c)}+\frac{1}{b^{3}(c+a)}+\frac{1}{c^{3}(a+b)} \quad () \quad \frac{3}{2} .
$$

Determine the correct inequality relation to fill in the blank.

Options:

(A) $\leq$ 

(B) $\geq$

(C) $=$ 

(D) $<$

(E) $>$

(F) None of the above

## Current Solution
Without loss of generality we may assume that $a \geq b \geq c$.
Let $x=\frac{1}{a}, y=\frac{1}{b}, z=\frac{1}{c}$. Then clearly $x y z=1$.

We have
$$
\begin{aligned}
\frac{1}{a^{3}(b+c)}+\frac{1}{b^{3}(c+a)}+\frac{1}{c^{3}(a+b)} & =\frac{x^{3}}{1 / y+1 / z}+\frac{y^{3}}{1 / z+1 / x}+\frac{z^{3}}{1 / x+1 / y} \\
& =\frac{x^{2}}{y+z}+\frac{y^{2}}{z+x}+\frac{z^{2}}{x+y}
\end{aligned}
$$

Since $c \leq b \leq a$ we have $x \leq y \leq z$.
So clearly $x+y \leq z+x \leq y+z$ and $\frac{x}{y+z} \leq \frac{y}{z+x} \leq \frac{z}{x+y}$.
Now by the rearrangement inequality we get the following inequalities
$$
\begin{aligned}
& \frac{x^{2}}{y+z}+\frac{y^{2}}{z+x}+\frac{z^{2}}{x+y} \geq \frac{x y}{y+z}+\frac{y z}{z+x}+\frac{z x}{x+y} \\
& \frac{x^{2}}{y+z}+\frac{y^{2}}{z+x}+\frac{z^{2}}{x+y} \geq \frac{x z}{y+z}+\frac{y x}{z+x}+\frac{z y}{x+y}
\end{aligned}
$$

So we obtain
$$
\begin{aligned}
& 2\left(\frac{1}{a^{3}(b+c)}+\frac{1}{b^{3}(c+a)}+\frac{1}{c^{3}(a+b)}\right) \\
& \quad=2\left(\frac{x^{2}}{y+z}+\frac{y^{2}}{z+x}+\frac{z^{2}}{x+y}\right) \\
& \quad \geq \frac{x y}{y+z}+\frac{y z}{z+x}+\frac{z x}{x+y}+\frac{x z}{y+z}+\frac{y x}{z+x}+\frac{z y}{x+y} \\
& \quad=x+y+z \geq 3 \sqrt[3]{x y z}=3
\end{aligned}
$$
as required. Therefore, the answer is (B) $\geq$.

## Expected Answer
(B) $\geq$

## Enhanced Solution
Enhanced Solution:

1. Symmetry and Ordering
   Observe that the expression
   \[S=\frac{1}{a^{3}(b+c)}+\frac{1}{b^{3}(c+a)}+\frac{1}{c^{3}(a+b)}\]
   is symmetric in the variables a,b,c (i.e. it remains unchanged under any permutation of a,b,c).  Therefore, we may impose an ordering on a,b,c without loss of generality.  Specifically, assume
   \[a\ge b\ge c>0.\]

2. Reciprocal Substitution
   Define new positive variables
   \[x=\frac1a,
     \quad y=\frac1b,
     \quad z=\frac1c.
   \]
   Then abc=1 implies xyz=1.  Moreover,
   \[
     \frac{1}{a^{3}(b+c)}
     =\frac{x^{3}}{b+c}
     =x^{3}\cdot\frac{1}{\frac1y+\frac1z}
     =x^{3}\cdot\frac{yz}{y+z}
     =\frac{x^{2}}{y+z},
   \]
   and similarly for the other two terms.  Hence the sum becomes
   \[
     S=\frac{x^{2}}{y+z}+\frac{y^{2}}{z+x}+\frac{z^{2}}{x+y}.
   \]

3. Induced Ordering on x,y,z
   Since a\ge b\ge c, we have x=1/a\le y=1/b\le z=1/c.  Also, noting that y+z\ge z+x\ge x+y, it follows that
   \[
     \frac{x}{y+z}\le \frac{y}{z+x}\le \frac{z}{x+y}.
   \]

4. Application of the Rearrangement Inequality
   We now apply the classical Rearrangement Inequality to the two ascending sequences
   \[(x,y,z)\quad\text{and}\quad\Bigl(\frac{x}{y+z},\frac{y}{z+x},\frac{z}{x+y}\Bigr).
   \]
   The Rearrangement Inequality asserts that the maximum of
   \[x\cdot\frac{\alpha}{\dots}+y\cdot\frac{\beta}{\dots}+z\cdot\frac{\gamma}{\dots}
   \]
   occurs when the two sequences are similarly sorted (ascending with ascending), and any other pairing gives a lesser (or equal) sum.

   In particular, pairing (x,y,z) in order with (x/(y+z),y/(z+x),z/(x+y)) in order yields our target sum T:
   \[T=x\cdot\tfrac{x}{y+z}+y\cdot\tfrac{y}{z+x}+z\cdot\tfrac{z}{x+y}
     =\frac{x^{2}}{y+z}+\frac{y^{2}}{z+x}+\frac{z^{2}}{x+y}=S.
   \]
   Any other pairing—for example,
   \[x\leftrightarrow\tfrac{y}{z+x},
     \;y\leftrightarrow\tfrac{z}{x+y},
     \;z\leftrightarrow\tfrac{x}{y+z}
   \]
   or the similar rearrangement—produces a sum that is at most T.  Concretely, two such rearrangements give
   \[
     \frac{x^{2}}{y+z}+\frac{y^{2}}{z+x}+\frac{z^{2}}{x+y}
     \;\ge\;
     \frac{xy}{y+z}+\frac{yz}{z+x}+\frac{zx}{x+y},
   \]
   and
   \[
     \frac{x^{2}}{y+z}+\frac{y^{2}}{z+x}+\frac{z^{2}}{x+y}
     \;\ge\;
     \frac{xz}{y+z}+\frac{yx}{z+x}+\frac{zy}{x+y}.
   \]

5. Summing the Two Inequalities
   Adding these two inequalities term by term, we obtain
   \[
     2S \;=\;2\Bigl(\tfrac{x^{2}}{y+z}+\tfrac{y^{2}}{z+x}+\tfrac{z^{2}}{x+y}\Bigr)
     \;\ge\;
     \Bigl(\tfrac{xy}{y+z}+\tfrac{xz}{y+z}\Bigr)
     +\Bigl(\tfrac{yz}{z+x}+\tfrac{yx}{z+x}\Bigr)
     +\Bigl(\tfrac{zx}{x+y}+\tfrac{zy}{x+y}\Bigr).
   \]
   In each pair, the numerators combine:
   \[
     \frac{xy+xz}{y+z}=x,
     \quad\frac{yz+yx}{z+x}=y,
     \quad\frac{zx+zy}{x+y}=z.
   \]
   Hence the right-hand side simplifies to x+y+z, leading to
   \[
     2S \ge x+y+z.
   \]

6. Final Step: AM–GM Inequality
   Since x,y,z>0 and xyz=1, the Arithmetic Mean – Geometric Mean inequality gives
   \[
     \frac{x+y+z}{3}\ge \sqrt[3]{xyz}=1
     \quad\Longrightarrow\quad x+y+z\ge 3.
   \]
   Combining with 2S\ge x+y+z, we conclude
   \[
     2S\ge 3
     \quad\Longrightarrow\quad S\ge \tfrac{3}{2}.
   \]

7. Conclusion
   Therefore, the given inequality holds in the direction “\(\ge\)” and the correct choice is
   
The answer is (B) ≥
