# Problem Entry

## Problem Type
relation

## Problem
Let $a, b, c$ be positive real numbers such that $a+b+c=3$. Consider the following expressions:
$$
\frac{a^{3}+2}{b+2}+\frac{b^{3}+2}{c+2}+\frac{c^{3}+2}{a+2} \quad () \quad 3
$$
Determine the correct inequality relation to fill in the blank.

Options:

(A) $\leq$ 

(B) $\geq$

(C) $=$ 

(D) $<$

(E) $>$

(F) None of the above

## Current Solution
By $A M \geq G M$ we have
$$
\frac{a^{3}+2}{b+2}=\frac{a^{3}+1+1}{b+2} \geq \frac{3 \sqrt[3]{a^{3} \cdot 1 \cdot 1}}{b+2}=\frac{3 a}{b+2}
$$

Similarly we get
$$
\frac{b^{3}+2}{c+2} \geq \frac{3 b}{c+2} \quad \text { and } \quad \frac{c^{3}+2}{a+2} \geq \frac{3 c}{a+2}
$$

Therefore
$$
\begin{equation*}
\frac{a^{3}+2}{b+2}+\frac{b^{3}+2}{c+2}+\frac{c^{3}+2}{a+2} \geq 3\left(\frac{a}{b+2}+\frac{b}{c+2}+\frac{c}{a+2}\right) \tag{1}
\end{equation*}
$$

Applying the Cauchy-Schwarz inequality we obtain
$$
\begin{align*}
\frac{a}{b+2}+\frac{b}{c+2}+\frac{c}{a+2} & =\frac{a^{2}}{a(b+2)}+\frac{b^{2}}{b(c+2)}+\frac{c^{2}}{c(a+2)} \\
& \geq \frac{(a+b+c)^{2}}{a(b+2)+b(c+2)+c(a+2)} \\
& =\frac{(a+b+c)^{2}}{a b+b c+c a+2(a+b+c)} \tag{2}
\end{align*}
$$

Since $(a+b+c)^{2} \geq 3(a b+b c+c a)$ we deduce that
$$
\begin{equation*}
\frac{1}{a b+b c+c a} \geq \frac{3}{(a+b+c)^{2}} \tag{3}
\end{equation*}
$$

From (2) and (3) we get
$$
\begin{align*}
\frac{a}{b+2}+\frac{b}{c+2}+\frac{c}{a+2} & \geq \frac{(a+b+c)^{2}}{a b+b c+c a+2(a+b+c)} \\
& \geq \frac{(a+b+c)^{2}}{(a+b+c)^{2} / 3+2(a+b+c)} \\
& =\frac{3(a+b+c)^{2}}{(a+b+c)^{2}+6(a+b+c)}=\frac{3(a+b+c)}{(a+b+c)+6} \tag{4}
\end{align*}
$$

Finally by (1), (4) and since $a+b+c=3$ we obtain
$$
A \geq 3\left(\frac{a}{b+2}+\frac{b}{c+2}+\frac{c}{a+2}\right) \geq \frac{9(a+b+c)}{(a+b+c)+6}=\frac{27}{9}=3
$$
as required. Equality occurs iff $a=b=c=1$. Therefore, the answer is (B) $\geq$.

## Expected Answer
(B) $\geq$

## Enhanced Solution
We wish to determine the correct inequality relation between

    S = \frac{a^{3} + 2}{b + 2} + \frac{b^{3} + 2}{c + 2} + \frac{c^{3} + 2}{a + 2}

and the constant 3, under the constraint a, b, c > 0 and a + b + c = 3.

Step 1.  Apply the AM–GM inequality to each numerator.
For each term, note that a³ + 2 = a³ + 1 + 1, and since b + 2 > 0, we may write

    \frac{a^{3} + 2}{b + 2} 
    = \frac{a^{3} + 1 + 1}{b + 2} 
    \ge  \frac{3 \sqrt[3]{a^{3} \cdot 1 \cdot 1}}{b + 2} 
    = \frac{3a}{b + 2}.

The inequality holds because the arithmetic mean of three nonnegative terms is at least their geometric mean, and equality in AM–GM occurs precisely when a³ = 1 = 1, i.e. a = 1.  Similarly,

    \frac{b^{3} + 2}{c + 2} \ge \frac{3b}{c + 2},
    \quad
    \frac{c^{3} + 2}{a + 2} \ge \frac{3c}{a + 2}.

Summing these three inequalities yields

    (1)\quad
    S \;=\; \sum_{\mathrm{cyc}} \frac{a^{3} + 2}{b + 2} 
    \ge 3 \sum_{\mathrm{cyc}} \frac{a}{b + 2}.

Step 2.  Bound the sum \sum a/(b+2) via Cauchy–Schwarz.
Observe that for positive quantities we can write

    \frac{a}{b + 2} = \frac{a^{2}}{a\,(b + 2)},

so by the Cauchy–Schwarz inequality,

    \sum_{\mathrm{cyc}} \frac{a^{2}}{a\,(b + 2)}
    \ge \frac{(a + b + c)^{2}}{\sum_{\mathrm{cyc}} a\,(b + 2)}
    = \frac{(a + b + c)^{2}}{ab + bc + ca + 2(a + b + c)}.

Since a + b + c = 3, this becomes

    \sum_{\mathrm{cyc}} \frac{a}{b + 2}
    \ge \frac{3^{2}}{ab + bc + ca + 6}
    = \frac{9}{ab + bc + ca + 6}.

Step 3.  Use the well-known inequality (a + b + c)² ≥ 3(ab + bc + ca).
Because a + b + c = 3, we get

    ab + bc + ca \le \frac{(a + b + c)^{2}}{3} = 3.

Hence

    ab + bc + ca + 6 \le 3 + 6 = 9,

which implies

    \frac{9}{ab + bc + ca + 6} \ge \frac{9}{9} = 1.

Therefore,

    \sum_{\mathrm{cyc}} \frac{a}{b + 2} \ge 1.

Step 4.  Combine the estimates.
From (1) we have

    S \ge 3 \sum_{\mathrm{cyc}} \frac{a}{b + 2} \ge 3 \cdot 1 = 3.

Thus S ≥ 3, with equality exactly when all interim inequalities become equalities.  Checking each step shows that equality forces

a³ = 1, b³ = 1, c³ = 1 (from AM–GM), and ab + bc + ca = 3 (from (a + b + c)² = 3(ab + bc + ca)),
which together imply a = b = c = 1.

Conclusion.  The required relation is “≥”.

The answer is (B) ≥
