# Problem Entry

## Problem Type
relation

## Problem
Let $a, b, c$ be the side lengths of a given triangle. Consider the following expressions:
$$
a^{2}+b^{2}+c^{2} \quad () \quad 2(a b+b c+c a)
$$
Determine the correct inequality relation to fill in the blank.

Options:

(A) $\leq$ 

(B) $\geq$

(C) $=$ 

(D) $<$

(E) $>$

(F) None of the above

## Current Solution
Let $a=x+y, b=y+z, c=z+x, x, y, z>0$.
Then we have
$$
\begin{aligned}
& (x+y)^{2}+(y+z)^{2}+(z+x)^{2} \\
& \quad<2((x+y)(y+z)+(y+z)(z+x)+(z+x)(x+y))
\end{aligned}
$$
or
$$
x y+y z+z x>0
$$
which is clearly true. Therefore, the answer is (D) $<$.

## Expected Answer
(D) $<$

## Enhanced Solution
Enhanced Solution:

We wish to compare the two symmetric expressions in the side-lengths a, b, c of a triangle:

  S = a² + b² + c²   and   T = 2(ab + bc + ca)

and determine which of the relations “<, ≤, =, ≥, >” holds.

Step 1:  Justification of the Ravi Substitution
------------------------------------------------
Since a, b, c are the side-lengths of a triangle, they satisfy the triangle inequalities:

  a < b + c,
  b < c + a,
  c < a + b.

Equivalently, each of the quantities (b + c – a), (c + a – b), (a + b – c) is strictly positive.  We set

  x = (b + c – a)/2,
  y = (c + a – b)/2,
  z = (a + b – c)/2.

Then x, y, z > 0, and one readily checks that

  a = y + z,
  b = z + x,
  c = x + y.

This is the standard “Ravi substitution,” which encodes the triangle inequalities via x, y, z > 0.

Step 2:  Express S in terms of x, y, z
----------------------------------------
Substitute a = y + z, b = z + x, c = x + y into S:

  S = (y + z)² + (z + x)² + (x + y)²
    = [y² + 2yz + z²] + [z² + 2zx + x²] + [x² + 2xy + y²]
    = 2(x² + y² + z²) + 2(xy + yz + zx).

Step 3:  Express T in terms of x, y, z
----------------------------------------
First compute the pairwise products:

  (a b) = (y + z)(z + x) = yz + yx + z² + zx,
  (b c) = (z + x)(x + y) = zx + zy + x² + xy,
  (c a) = (x + y)(y + z) = xy + xz + y² + yz.

Summing these three:

  ab + bc + ca
  = (x² + y² + z²)
    + 3(xy + yz + zx).

Therefore
  T = 2(ab + bc + ca)
    = 2(x² + y² + z²) + 6(xy + yz + zx).

Step 4:  Compare S and T
------------------------
Compute the difference:

  S – T
  = [2(x² + y² + z²) + 2(xy + yz + zx)]
    – [2(x² + y² + z²) + 6(xy + yz + zx)]
  = –4(xy + yz + zx).

Since x, y, z are all strictly positive, their pairwise products sum xy + yz + zx > 0.  Hence

  S – T = –4(xy + yz + zx) < 0
      ⇒  S < T.

Conclusion
----------
We have shown that for any triangle with sides a, b, c,

  a² + b² + c²   <   2(ab + bc + ca).

Therefore the correct answer is

The answer is (D) <
