# Problem Entry

## Problem Type
relation

## Problem
Let $a, b, c$ be positive real numbers such that $a+b+c=6$. Consider the following expressions:
$$
\sqrt[3]{a b+b c}+\sqrt[3]{b c+c a}+\sqrt[3]{c a+a b} \quad () \quad 6 .
$$
Determine the correct inequality relation to fill in the blank.

Options:

(A) $\leq$ 

(B) $\geq$

(C) $=$ 

(D) $<$

(E) $>$

(F) None of the above

## Current Solution
By the power mean inequality we have
$$
\frac{\sqrt[3]{a b+b c}+\sqrt[3]{b c+c a}+\sqrt[3]{c a+a b}}{3} \leq \sqrt[3]{\frac{(a b+b c)+(b c+c a)+(c a+a b)}{3}}
$$
i.e.
$$
\begin{equation*}
\sqrt[3]{a b+b c}+\sqrt[3]{b c+c a}+\sqrt[3]{c a+a b} \leq \sqrt[3]{18(a b+b c+c a)} \tag{1}
\end{equation*}
$$

Since $a b+b c+c a \leq \frac{(a+b+c)^{2}}{3}=12$ by (1) we obtain
$$
\sqrt[3]{a b+b c}+\sqrt[3]{b c+c a}+\sqrt[3]{c a+a b} \leq \sqrt[3]{18 \cdot 12}=6
$$

Equality occurs if and only if $a=b=c=2$. Therefore, the answer is (A) $\leq$.

## Expected Answer
(A) $\leq$

## Enhanced Solution
Enhanced Solution:

We wish to compare the quantity
  S = √[3]{ab+bc} + √[3]{bc+ca} + √[3]{ca+ab}
with the number 6, under the constraint a,b,c>0 and a+b+c=6.

Step 1: Introduce auxiliary variables and apply the Power Mean (Jensen) inequality
-------------------------------------------------------------------------------
Let
  x₁ = ab + bc,
  x₂ = bc + ca,
  x₃ = ca + ab.
Each xᵢ is nonnegative.  Recall that the cube‐root function f(x)=x^{1/3} is concave on [0,∞).  By Jensen’s (or the Power Mean) inequality for three points,
  (1/3)[f(x₁)+f(x₂)+f(x₃)] ≤ f((x₁+x₂+x₃)/3).
Multiplying both sides by 3 gives
  √[3]{x₁} + √[3]{x₂} + √[3]{x₃} ≤ 3·√[3]{(x₁+x₂+x₃)/3}.
Substitute x₁+x₂+x₃ = (ab+bc)+(bc+ca)+(ca+ab) = 2(ab+bc+ca) to obtain
  S ≤ 3·√[3]{(2(ab+bc+ca)/3)}
     = √[3]{27·(2(ab+bc+ca)/3)}
     = √[3]{18·(ab+bc+ca)}.          (Inequality (1))

Step 2: Bound the symmetric sum ab+bc+ca
-----------------------------------------
Under the fixed sum a+b+c=6, a standard inequality yields
  ab + bc + ca ≤ (a+b+c)²/3 = 6²/3 = 12.
Indeed, one way to see this is:
  ab+bc+ca = [(a+b+c)² – (a²+b²+c²)]/2 ≤ [(a+b+c)² – (a²+b²+c²)/3]/2 = (a+b+c)²/3.

Step 3: Combine the estimates
------------------------------
Substitute ab+bc+ca ≤ 12 into (1):
  S ≤ √[3]{18·12} = √[3]{216} = 6.
Hence
  √[3]{ab+bc} + √[3]{bc+ca} + √[3]{ca+ab} ≤ 6.

Step 4: Equality case
---------------------
Both inequalities we used become equalities exactly when a=b=c.  In that case a=b=c=2, and indeed all x₁=x₂=x₃=2·2+2·2=8, so S=3·√[3]{8}=6.

Conclusion
----------
The required inequality relation is “≤”.

Answer:
The answer is (A) ≤
