# Problem Entry

## Problem Type
relation

## Problem
Let $a, b \in \mathbb{R}^{+}$. Consider the following inequality:
$$
4\left(a^{3}+b^{3}\right) \quad () \quad (a+b)^{3} .
$$

Determine the correct inequality relation to fill in the blank.

Options:

(A) $\leq$ 

(B) $\geq$

(C) $=$ 

(D) $<$

(E) $>$

(F) None of the above

## Current Solution
The function $f(x)=x^{3}$ is convex on $(0,+\infty)$, thus from Jensen's inequality it follows that
$$
\left(\frac{a+b}{2}\right)^{3} \leq \frac{a^{3}+b^{3}}{2} \Leftrightarrow 4\left(a^{3}+b^{3}\right) \geq(a+b)^{3}
$$ Therefore, the answer is (B) $\geq$.

## Expected Answer
(B) $\geq$

## Enhanced Solution
Enhanced Solution:

1. Identification of the relevant function and its domain
   We observe that the inequality to be compared involves expressions of the form a^3 and b^3.  To apply a standard inequality, define the function f : (0, +∞) → ℝ by
       f(x) = x^3.
   Since a, b ∈ ℝ^+, both a and b lie in the domain of f.

2. Verification of convexity of f on (0, +∞)
   Compute the first and second derivatives of f:
       f′(x) = 3x^2,
       f″(x) = 6x.
   For all x > 0, we have f″(x) = 6x > 0.  Therefore, f is strictly convex on the interval (0, +∞).

3. Application of Jensen’s inequality for two points
   Jensen’s inequality for a convex function f and weights λ, 1–λ (with 0 < λ < 1) states:
       f(λ x + (1–λ) y) ≤ λ f(x) + (1–λ) f(y).
   Here we choose x = a, y = b, and λ = 1/2.  Substituting these values gives:
       f((a + b)/2) ≤ ½ f(a) + ½ f(b).

4. Translation of Jensen’s inequality into the given expressions
   Replace f by x^3 in the above inequality:
       ((a + b)/2)^3 ≤ (a^3 + b^3)/2.
   Multiply both sides by 8 to clear denominators:
       (a + b)^3 ≤ 4 (a^3 + b^3).

5. Rearrangement to match the original inequality format
   The result (a + b)^3 ≤ 4(a^3 + b^3) can be rewritten as
       4 (a^3 + b^3) ≥ (a + b)^3.
   This establishes the desired comparison symbol between 4(a^3 + b^3) and (a + b)^3.

6. Conclusion
   By the above chain of rigorous deductions, we conclude that for all positive real a and b,
       4 (a^3 + b^3) ≥ (a + b)^3.

The answer is (B) ≥
