# Problem Entry

## Problem Type
relation

## Problem
Let $a, b, c$ be the lengths of the sides of a triangle. Consider the following expressions:
$$
(a+b-c)^{a}(b+c-a)^{b}(c+a-b)^{c} \quad () \quad a^{a} b^{b} c^{c}
$$
Determine the correct inequality relation to fill in the blank.

Options:

(A) $\leq$ 

(B) $\geq$

(C) $=$ 

(D) $<$

(E) $>$

(F) None of the above

## Current Solution
By the weighted power mean inequality we have
$$
\begin{aligned}
& \sqrt[a+b+c]{\left(\frac{a+b-c}{a}\right)^{a}\left(\frac{b+c-a}{b}\right)^{b}\left(\frac{c+a-b}{c}\right)^{c}} \\
& \leq \frac{1}{a+b+c}\left(a \cdot \frac{a+b-c}{a}+b \cdot \frac{b+c-a}{b}+c \cdot \frac{c+a-b}{c}\right)=1
\end{aligned}
$$
i.e.
$$
(a+b-c)^{a}(b+c-a)^{b}(c+a-b)^{c} \leq a^{a} b^{b} c^{c}
$$

Equality occurs iff $a=b=c$. Therefore, the answer is (A) $\leq$.

## Expected Answer
(A) $\leq$

## Enhanced Solution
Enhanced Detailed Solution:

1.  Problem restatement and conditions:
   Let a, b, c be the side–lengths of a triangle.  Then by definition we have a, b, c > 0 and they satisfy the triangle inequalities:
     a + b > c,
     b + c > a,
     c + a > b.
   In particular, each of the expressions a + b – c, b + c – a, c + a – b is strictly positive.

2.  Introduction of auxiliary positive quantities:
   Define three positive numbers
     x = (a + b – c)/a,
     y = (b + c – a)/b,
     z = (c + a – b)/c.
   Because a + b – c > 0, etc., we know x, y, z > 0.

3.  Reformulation of the desired inequality:
   We wish to compare
     (a + b – c)^{a} (b + c – a)^{b} (c + a – b)^{c}
   with
     a^{a} b^{b} c^{c}.
   Observe that
     (a + b – c)^{a} (b + c – a)^{b} (c + a – b)^{c}
     = (a x)^{a} (b y)^{b} (c z)^{c}
     = a^{a} b^{b} c^{c} · (x^{a} y^{b} z^{c}).
   Hence the inequality
     (a + b – c)^{a} (b + c – a)^{b} (c + a – b)^{c} ≤ a^{a} b^{b} c^{c}
   is equivalent to showing
     x^{a} y^{b} z^{c} ≤ 1.

4.  Application of the weighted AM–GM inequality:
   The weighted arithmetic–geometric mean inequality states that for any positive numbers x, y, z and positive weights a, b, c,
     (x^{a} y^{b} z^{c})^{1/(a + b + c)} ≤ (a x + b y + c z)/(a + b + c).
   Raise both sides to the power a + b + c to obtain
     x^{a} y^{b} z^{c} ≤ \bigl( (a x + b y + c z)/(a + b + c) \bigr)^{a + b + c}.

5.  Computation of the weighted average a x + b y + c z:
   Substitute the definitions of x, y, z:
     a x = a · (a + b – c)/a = a + b – c,
     b y = b · (b + c – a)/b = b + c – a,
     c z = c · (c + a – b)/c = c + a – b.
   Summing these three terms gives
     a x + b y + c z
       = (a + b – c) + (b + c – a) + (c + a – b)
       = [a + b + b + c + c + a] – [c + a + b]
       = 2(a + b + c) – (a + b + c)
       = a + b + c.
   Therefore the weighted arithmetic mean is
     (a x + b y + c z)/(a + b + c) = (a + b + c)/(a + b + c) = 1.

6.  Conclusion of the inequality chain:
   From step 4 we have
     x^{a} y^{b} z^{c} ≤ 1^{a + b + c} = 1.
   Hence,
     (a + b – c)^{a} (b + c – a)^{b} (c + a – b)^{c}
       = a^{a} b^{b} c^{c} · (x^{a} y^{b} z^{c})
       ≤ a^{a} b^{b} c^{c} · 1
       = a^{a} b^{b} c^{c}.
   This establishes the required inequality.

7.  Equality condition:
   The weighted AM–GM inequality becomes an equality precisely when x = y = z.  That is,
     (a + b – c)/a = (b + c – a)/b = (c + a – b)/c.
   Solving these proportionalities shows that a = b = c.  Hence equality holds if and only if the triangle is equilateral.

Final Answer:
The answer is (A) ≤
