# Problem Entry

## Problem Type
relation

## Problem
Let $x, y, z \in \mathbb{R}^{+}$ such that $x + y + z = 1$. Consider the following inequality:
$$
\frac{1}{1-x y}+\frac{1}{1-y z}+\frac{1}{1-z x} \quad () \quad \frac{27}{8} .
$$

Determine the correct inequality relation to fill in the blank.

Options:

(A) $\leq$ 

(B) $\geq$

(C) $=$ 

(D) $<$

(E) $>$

(F) None of the above

## Current Solution
Let $p=x+y+z=1, q=x y+y z+z x, r=x y z$.
It can easily be shown that
$$
(1-x y)(1-y z)(1-z x)=1-q+p r-r^{2}
$$
and
$$
(1-x y)(1-y z)+(1-y z)(1-z x)+(1-z x)(1-x y)=3-2 q+p r
$$

So the given inequality becomes
$$
\begin{gathered}
8(3-2 q+p r) \leq 27\left(1-q+p r-r^{2}\right) \\
\Leftrightarrow \quad 3-11 q+19 p r-27 r^{2} \geq 0
\end{gathered}
$$

Since $p=1$, we need to show that
$$
3-11 q+19 r-27 r^{2} \geq 0
$$

By $N_{5}: p^{3} \geq 27 r$ we have $1 \geq 27 r$, i.e. $r \geq 27 r^{2}$.

Therefore
$$
3-11 q+19 r-27 r^{2} \geq 3-11 q+19 r-r=3-11 q+18 r
$$

So it suffices to prove that
$$
3-11 q+18 r \geq 0
$$

We have
$$
\begin{aligned}
& 3-11 q+18 r \geq 0 \\
& \quad \Leftrightarrow \quad 3-11(x y+y z+z x)+18 x y z \geq 0 \\
& \quad \Leftrightarrow \quad 11(x y+y z+z x)-18 x y z \leq 3
\end{aligned}
$$

Applying $A M \geq G M$ we deduce
$$
\begin{aligned}
11(x y+y z+z x)-18 x y z & =x y(11-18 z)+11 z(x+y) \\
& \leq \frac{(x+y)^{2}}{4}(11-18 z)+11 z(x+y) \\
& =\frac{(1-z)^{2}}{4}(11-18 z)+11 z(1-z) \\
& =\frac{(1-z)((1-z)(11-18 z)+44 z)}{4} \\
& =\frac{4 z+3 z^{2}-18 z^{3}+11}{4}
\end{aligned}
$$

So it remains to show that
$$
\begin{aligned}
& \frac{4 z+3 z^{2}-18 z^{3}+11}{4} \leq 3 \\
& \quad \Leftrightarrow \quad 4 z+3 z^{2}-18 z^{3} \leq 1 \\
& \Leftrightarrow \quad 18 z^{3}-3 z^{2}-4 z+1 \geq 0 \\
& \Leftrightarrow \quad(3 z-1)^{2}(2 z+1) \geq 0
\end{aligned}
$$
which is obvious. Therefore, the answer is (A) $\leq$.

## Expected Answer
(A) $\leq$

## Enhanced Solution
We wish to determine the relationship between

    S = \frac{1}{1 - x y} + \frac{1}{1 - y z} + \frac{1}{1 - z x}

and

    \frac{27}{8},

subject to x, y, z > 0 and x + y + z = 1.  We will show that S ≤ 27/8.

1.  Symmetric-polynomial notation.  Set
   p = x + y + z = 1,
   q = xy + yz + zx,
   r = xyz.

2.  Express S in terms of p, q, r.  Observe that
   (1 − xy)(1 − yz)(1 − zx)
     = 1 − (xy + yz + zx) + (x y + y z + z x)·(x+y+z)·xyz
       − (xyz)²
     = 1 − q + p·r − r².

   Also, the sum of pairwise products of these three factors is
   (1 − xy)(1 − yz) + (1 − yz)(1 − zx) + (1 − zx)(1 − xy)
     = 3 − 2q + p·r.

   Therefore

     S
     = \sum_{cyc} \frac{1}{1 − x y}
     = \frac{(1−xy)(1−yz)+(1−yz)(1−zx)+(1−zx)(1−xy)}{(1−xy)(1−yz)(1−zx)}
     = \frac{3 − 2q + p r}{1 − q + p r − r²}.

3.  Reduce the inequality S ≤ 27/8 to a polynomial inequality.  Multiply both sides by 8(1−q+pr−r²)>0 to obtain

     8(3 − 2q + p r) ≤ 27(1 − q + p r − r²)
     ⇔ 24 −16q +8pr ≤ 27 −27q +27pr −27r²
     ⇔ 3 −11q +19p r −27r² ≥ 0.

   Since p = 1, this becomes

     3 − 11q + 19r −27r² ≥ 0.  (★)

4.  Lower-bound the quadratic part 19r −27r².  From the AM–GM inequality for three positive numbers we have

     p³ = (x + y + z)³ ≥ 27xyz = 27r
     ⇒ r ≤ 1/27.

   Hence 27r² ≤ r, i.e. 19r −27r² ≥ 19r − r = 18r.  Substituting into (★) yields the stronger requirement

     3 − 11q + 18r ≥ 0
     ⇔ 11q − 18r ≤ 3.

5.  Rewrite 11q − 18r in terms of x, y, z and apply an extremal bound.  Note

     11q − 18r = 11(xy + yz + zx) − 18xyz
               = xy(11 − 18z) + 11z(x + y).

   For fixed z, the sum x + y = 1 − z is constant, and the product xy is maximized when x = y = (1−z)/2.  Hence

     xy(11 − 18z) + 11z(1−z)
     ≤ \frac{(1−z)²}{4}(11 − 18z) + 11z(1−z).

   Simplify the right side:

     \frac{(1−z)²}{4}(11 − 18z) + 11z(1−z)
     = \frac{(1−z)igl[(1−z)(11 − 18z) + 44z\bigr]}{4}
     = \frac{11 + 4z + 3z² − 18z³}{4}.

   We must prove

     \frac{11 + 4z + 3z² − 18z³}{4} ≤ 3
     ⇔ 11 + 4z + 3z² − 18z³ ≤ 12
     ⇔ 18z³ − 3z² − 4z + 1 ≥ 0
     ⇔ (3z − 1)²(2z + 1) ≥ 0,

   which is evidently true for all real z.  Thus 11q − 18r ≤ 3.

6.  Conclusion.  We have shown step by step that S ≤ 27/8.  Therefore the correct relation is “≤”.

The answer is (A) ≤
