# Problem Entry

## Problem Type
relation

## Problem
Let \(a, b \in \mathbb{R}^{+}\) and \(n \in \mathbb{N}\). Consider the following inequality:
$$
(a+b)^{n}\left(a^{n}+b^{n}\right) \quad () \quad 2^{n}\left(a^{2 n}+b^{2 n}\right) .
$$

Determine the correct inequality relation to fill in the blank.

Options:

(A) $\leq$ 

(B) $\geq$

(C) $=$ 

(D) $<$

(E) $>$

(F) None of the above

## Current Solution
By the power mean inequality, for any $x, y \in \mathbb{R}^{+}, n \in \mathbb{N}$, we have
$$
\left(\frac{x+y}{2}\right)^{n} \leq \frac{x^{n}+y^{n}}{2}
$$

Therefore
$$
\begin{aligned}
(a+b)^{n}\left(a^{n}+b^{n}\right) & =2^{n}\left(\frac{a+b}{2}\right)^{n}\left(a^{n}+b^{n}\right) \\
& \leq 2^{n}\left(\frac{a^{n}+b^{n}}{2}\right)\left(a^{n}+b^{n}\right)=2^{n} \frac{\left(a^{n}+b^{n}\right)^{2}}{2} \\
& \leq 2^{n} \frac{2\left(a^{2 n}+b^{2 n}\right)}{2}=2^{n}\left(a^{2 n}+b^{2 n}\right)
\end{aligned}
$$ Therefore, the answer is (A) $\leq$.

## Expected Answer
(A) $\leq$

## Enhanced Solution
Enhanced Solution:

We wish to determine the correct inequality sign in
\[
(a+b)^{n}\,(a^{n}+b^{n})\;()\;2^{n}\,(a^{2n}+b^{2n}),
\]
where a,b>0 and n is a positive integer.  We shall prove
\[
(a+b)^{n}(a^{n}+b^{n})\le 2^{n}(a^{2n}+b^{2n}).
\]

1.  Recall the Power Mean (or generalized AM–GM) inequality for two positive numbers x,y and exponent n≥1:
   \[
   \Bigl(\frac{x+y}{2}\Bigr)^{n}\le\frac{x^{n}+y^{n}}{2}.
   \]
   Taking x=a and y=b, we get
   \[
   \Bigl(\frac{a+b}{2}\Bigr)^{n}\le\frac{a^{n}+b^{n}}{2}.
   \]
   Multiply both sides by 2ⁿ to obtain
   \[
   (a+b)^{n}=2^{n}\Bigl(\frac{a+b}{2}\Bigr)^{n}\le 2^{n}\,\frac{a^{n}+b^{n}}{2}
   =2^{n-1}(a^{n}+b^{n}).
   \]

2.  Multiply this last inequality by the positive factor (a^{n}+b^{n}):
   \[
   (a+b)^{n}(a^{n}+b^{n})\le 2^{n-1}(a^{n}+b^{n})^{2}.
   \]

3.  We apply the same Power Mean inequality again, now with u=a^{n}, v=b^{n} and exponent 2:
   \[
   \Bigl(\frac{u+v}{2}\Bigr)^{2}\le\frac{u^{2}+v^{2}}{2}
   \quad\Longrightarrow\quad
   (u+v)^{2}\le 2(u^{2}+v^{2}).
   \]
   Substituting u=a^{n}, v=b^{n}, this becomes
   \[
   (a^{n}+b^{n})^{2}\le 2\bigl(a^{2n}+b^{2n}\bigr).
   \]

4.  Combine the two derived bounds:
   \[
   (a+b)^{n}(a^{n}+b^{n})\le 2^{n-1}(a^{n}+b^{n})^{2}
   \le 2^{n-1}\cdot2\bigl(a^{2n}+b^{2n}\bigr)
   =2^{n}(a^{2n}+b^{2n}).
   \]

Hence the correct relation is “≤”.

The answer is (A) ≤
