# Problem Entry

## Problem Type
relation

## Problem
Let $a, b, c \in \mathbb{R}^{+}$. Consider the following inequality:
$$
\frac{(a+2 b+3 c)^{2}}{a^{2}+2 b^{2}+3 c^{2}} \quad () \quad 6 .
$$

Determine the correct inequality relation to fill in the blank.

Options:

(A) $\leq$ 

(B) $\geq$

(C) $=$ 

(D) $<$

(E) $>$

(F) None of the above

## Current Solution
For $m_{1}=\frac{1}{6}, m_{2}=\frac{2}{6}, m_{3}=\frac{3}{6}, n=3$ by the inequality
$$
M_{1}^{m}(a, b, c) \leq M_{2}^{m}(a, b, c)
$$
which is true due to the weighted power mean inequality, we obtain
$$
\frac{a+2 b+3 c}{6} \leq \sqrt{\frac{a^{2}+2 b^{2}+3 c^{2}}{6}}, \quad \text { i.e. } \quad \frac{(a+2 b+3 c)^{2}}{a^{2}+2 b^{2}+3 c^{2}} \leq 6
$$ Therefore, the answer is (A) $\leq$.

## Expected Answer
(A) $\leq$

## Enhanced Solution
Enhanced Solution:

We wish to determine the correct inequality relation between the two expressions

    (a + 2 b + 3 c)²  and  6 · (a² + 2 b² + 3 c²)

to decide how (a + 2 b + 3 c)² / (a² + 2 b² + 3 c²) compares with 6.  We use the weighted power mean inequality without changing the original approach.

Step 1: Introduce positive weights that sum to 1

  Let w₁ = 1/6,  w₂ = 2/6,  w₃ = 3/6.  Then each wᵢ > 0 and

      w₁ + w₂ + w₃ = (1 + 2 + 3)/6 = 1.

Step 2: Define the weighted arithmetic mean (first power mean) A and the weighted quadratic mean (second power mean) Q

  A = w₁·a + w₂·b + w₃·c
    = (1/6)·a + (2/6)·b + (3/6)·c
    = (a + 2b + 3c)/6,

  Q = \sqrt{w₁·a² + w₂·b² + w₃·c²}
    = \sqrt{(1/6)·a² + (2/6)·b² + (3/6)·c²}
    = \sqrt{(a² + 2b² + 3c²)/6}.

Step 3: Apply the weighted power mean inequality

  For any positive numbers xᵢ and weights wᵢ > 0 with sum 1, the power mean with exponent r is

      M_r = (w₁·x₁^r + w₂·x₂^r + w₃·x₃^r)^{1/r}.

  The inequality states that if r < s, then M_r ≤ M_s.  Here take r = 1 and s = 2, so

      A = M₁(a,b,c) ≤ M₂(a,b,c) = Q.

  Hence

      (a + 2b + 3c)/6  ≤  sqrt((a² + 2b² + 3c²)/6).

Step 4: Transform into the desired form

  Since both sides are nonnegative, we may square the inequality without changing its direction:

      [(a + 2b + 3c)/6]²  ≤  ( (a² + 2b² + 3c²)/6 ).

  Multiply both sides by 36 (which is positive), giving

      (a + 2b + 3c)²  ≤  6·(a² + 2b² + 3c²).

  Finally, divide both sides by (a² + 2b² + 3c²) (also positive) to isolate the original quotient:

      (a + 2b + 3c)² / (a² + 2b² + 3c²)  ≤  6.

Thus the correct relation is “≤”.

The answer is (A) ≤
