# Problem Entry

## Problem Type
relation

## Problem
Let $a, b, c \in \mathbb{R}^{+}$ such that $a+b+c=3$. Consider the following expressions:
$$
\sqrt{a(b+c)}+\sqrt{b(c+a)}+\sqrt{c(a+b)} \quad () \quad 3 \sqrt{2 a b c} .
$$
Determine the correct inequality relation to fill in the blank.

Options:

(A) $\leq$ 

(B) $\geq$

(C) $=$ 

(D) $<$

(E) $>$

(F) None of the above

## Current Solution
We have
$$
\sqrt{a b+a c} \geq \frac{\sqrt{2}}{2}(\sqrt{a b}+\sqrt{a c})
$$

Analogously
$$
\sqrt{b c+b a} \geq \frac{\sqrt{2}}{2}(\sqrt{b c}+\sqrt{b a}) \quad \text { and } \quad \sqrt{c a+c b} \geq \frac{\sqrt{2}}{2}(\sqrt{c a}+\sqrt{c b})
$$

So it suffices to show that
$$
\sqrt{2}(\sqrt{a b}+\sqrt{a c}+\sqrt{b c}) \geq 3 \sqrt{2 a b c}
$$
i.e.
$$
\begin{equation*}
\sqrt{a b}+\sqrt{a c}+\sqrt{b c} \geq 3 \sqrt{a b c} \tag{1}
\end{equation*}
$$

By $A M \geq G M$ we have
$$
\sqrt{a b}+\sqrt{a c}+\sqrt{b c} \geq 3 \sqrt[3]{a b c} \geq 3 \sqrt{a b c}
$$
where the last inequality is true since
$$
\sqrt[3]{a b c} \leq \frac{a+b+c}{3}=1, \quad \text { i.e. } \quad a b c \leq 1
$$ Therefore, the answer is (B) $\geq$.

## Expected Answer
(B) $\geq$

## Enhanced Solution
We wish to determine the correct inequality between

    S = √[a(b+c)] + √[b(c+a)] + √[c(a+b)]
and
    T = 3 √[2 a b c],

given a,b,c>0 with a+b+c=3.  The original solution uses the same chain of inequalities, and we now supply a fully detailed, step-by-step justification.

1.  Reduction via a two-term square‐root estimate

   Claim.  For any x,y≥0,
       √(x+y)  ≥  (√x + √y)/√2.
   Proof.  Square both sides:
       (√x + √y)² /2  =  (x + y + 2√{xy})/2
                      =  (x+y)/2 + √{xy}
   so the inequality √(x+y) ≥ (√x+√y)/√2 is equivalent to
       x+y  ≥  (x+y)/2 + √{xy}
     ⇔ (x+y)/2  ≥  √{xy},
   which is exactly the standard AM–GM inequality for x and y.

   We apply this estimate three times, with (x,y) chosen as (ab,ac), (bc,ba), (ca,cb) respectively.  For the first term:
       √[a(b+c)] = √(ab + ac)
                  ≥ (√{ab} + √{ac}) /√2.
   Similarly,
       √[b(c+a)] ≥ (√{bc} + √{ba})/√2,
       √[c(a+b)] ≥ (√{ca} + √{cb})/√2.

2.  Summing up the three estimates

   Adding the three inequalities gives
       S = √[a(b+c)] + √[b(c+a)] + √[c(a+b)]
         ≥ (1/√2)igl[(√{ab}+√{ac}) + (√{bc}+√{ba}) + (√{ca}+√{cb})igr]
         = ( √{ab} + √{bc} + √{ca} ) · (2/√2)
         = √2 (√{ab} + √{bc} + √{ca}).

   Hence it suffices to prove
       √2 (√{ab} + √{bc} + √{ca})  ≥  T = 3√(2 abc),
   i.e.
       √{ab} + √{bc} + √{ca}  ≥  3√(abc).    (★)

3.  Proving ★ by two applications of AM–GM

   (i)  First AM–GM on the three positive terms √{ab}, √{bc}, √{ca}:
       (√{ab} + √{bc} + √{ca})/3  ≥  (√{ab}·√{bc}·√{ca})^{1/3}
                              =  (abc)^{1/3}.
   Therefore
       √{ab} + √{bc} + √{ca}  ≥  3 (abc)^{1/3}.

   (ii)  Next, from a+b+c=3 we again invoke AM–GM to bound the product abc:
       (a + b + c)/3  ≥  (abc)^{1/3}
     ⇒ 1  ≥  (abc)^{1/3}
     ⇒ abc  ≤  1.
   Since 0 < abc ≤ 1, the function t↦t^x is decreasing in x for 0<t<1.  In particular,
       (abc)^{1/3}  ≥  (abc)^{1/2} = √(abc).
   Combining with the result of step (i) gives
       √{ab} + √{bc} + √{ca}  ≥  3 (abc)^{1/3}  ≥  3√(abc),
   which is exactly (★).

4.  Conclusion

   We have shown
       S ≥ √2 (√{ab} + √{bc} + √{ca})  ≥ √2·3√(abc)  =  3√(2 abc) = T.
   Hence the correct inequality sign is “≥”.

The answer is (B) ≥
