# Problem Entry

## Problem Type
bound

## Problem
Let $a, b, c$ be positive real numbers such that $a + b + c = 6$. Find the minimal constant $C$ such that the following inequality holds for all $a, b, c$ satisfying the given constraint:
$$
\sqrt[3]{a b + b c} + \sqrt[3]{b c + c a} + \sqrt[3]{c a + a b} \leq C
$$

## Current Solution
By the power mean inequality we have
$$
\frac{\sqrt[3]{a b+b c}+\sqrt[3]{b c+c a}+\sqrt[3]{c a+a b}}{3} \leq \sqrt[3]{\frac{(a b+b c)+(b c+c a)+(c a+a b)}{3}}
$$
i.e.
$$
\begin{equation*}
\sqrt[3]{a b+b c}+\sqrt[3]{b c+c a}+\sqrt[3]{c a+a b} \leq \sqrt[3]{18(a b+b c+c a)} \tag{1}
\end{equation*}
$$

Since $a b+b c+c a \leq \frac{(a+b+c)^{2}}{3}=12$ by (1) we obtain
$$
\sqrt[3]{a b+b c}+\sqrt[3]{b c+c a}+\sqrt[3]{c a+a b} \leq \sqrt[3]{18 \cdot 12}=6
$$

Equality occurs if and only if $a = b = c = 2$, which is when $a, b, c$ are all equal and $a + b + c = 6$. In this case, the maximum value of the expression is achieved, so $C = 6$ is the minimal constant for which the inequality always holds.

Therefore, the answer is $C = 6$. 

## Expected Answer
$C = 6$

## Enhanced Solution
We wish to show that for all positive real numbers a,b,c with a+b+c=6, the following holds:

    ∛(ab+bc) + ∛(bc+ca) + ∛(ca+ab)  ≤  C,

and to determine the smallest such constant C.

Step 1.  Introducing the three arguments for the cube-root function

Let x₁ = ab + bc,
    x₂ = bc + ca,
    x₃ = ca + ab.

Then our target expression is f(x₁)+f(x₂)+f(x₃), where we write f(x)=x^{1/3} for x>0.

Step 2.  Verifying concavity of f(x)=x^{1/3}

Compute the second derivative:

    f''(x) = −(2/9) x^{−5/3},

which is strictly negative for all x>0.  Hence f is strictly concave on (0,∞).

Step 3.  Applying Jensen’s inequality for a concave function

Jensen’s inequality for a concave function f states:

    (f(x₁) + f(x₂) + f(x₃)) / 3  ≤  f( (x₁ + x₂ + x₃)/3 ).

Equivalently,

    f(x₁) + f(x₂) + f(x₃)  ≤  3 · f( (x₁ + x₂ + x₃)/3 ).

Substituting x₁,x₂,x₃ gives

    ∛(ab+bc) + ∛(bc+ca) + ∛(ca+ab)
      ≤  3 · ∛( ( (ab+bc) + (bc+ca) + (ca+ab) ) / 3 ).  (1)

Step 4.  Simplifying the sum x₁ + x₂ + x₃

Observe that

    x₁ + x₂ + x₃ = (ab+bc) + (bc+ca) + (ca+ab)
                 = 2(ab + bc + ca).

Hence the right–hand side of (1) becomes

    3 · ∛( (2(ab+bc+ca)) / 3 )
  =  3 · ∛(2/3 · (ab+bc+ca))
  =  ∛( 27 · (2/3) · (ab+bc+ca) )
  =  ∛( 18 · (ab+bc+ca) ).

Thus we have derived the intermediate bound:

    ∛(ab+bc) + ∛(bc+ca) + ∛(ca+ab)
      ≤  ∛( 18 · (ab+bc+ca) ).  (2)

Step 5.  Bounding ab+bc+ca under the constraint a+b+c=6

A well-known symmetric inequality states that for any nonnegative a,b,c,

    ab + bc + ca  ≤  (a + b + c)² / 3.

Since a+b+c = 6, it follows that

    ab + bc + ca  ≤  6² / 3  =  12.

Substituting into (2) yields

    ∛(ab+bc) + ∛(bc+ca) + ∛(ca+ab)
      ≤  ∛(18 · 12)
      =  ∛(216)
      = 6.

Hence the expression never exceeds 6.

Step 6.  Checking that equality can occur

Both inequalities above become equalities precisely when a=b=c=2, because:

  • Jensen’s inequality is an equality if and only if x₁ = x₂ = x₃, i.e.
    ab+bc = bc+ca = ca+ab, which forces a=b=c.

  • The bound ab+bc+ca ≤ (a+b+c)²/3 is an equality only when a=b=c.

Under a=b=c=2 we indeed have a+b+c=6 and each of ab+bc, etc.
equals 8, giving ∛8+∛8+∛8 = 2+2+2 = 6.

Conclusion

We have shown that for all positive a,b,c with a+b+c=6,

    ∛(ab+bc) + ∛(bc+ca) + ∛(ca+ab)  ≤  6,

and that the constant 6 is attained (and hence minimal) when a=b=c=2.

The answer is $C=6$.
