# Problem Entry

## Problem Type
relation

## Problem
Let $x, y, z > 0$, such that $x y z = 1$. Consider the following inequality:
$$
\frac{x^{3}}{(1+y)(1+z)}+\frac{y^{3}}{(1+z)(1+x)}+\frac{z^{3}}{(1+x)(1+y)} \quad () \quad \frac{3}{4} .
$$

Determine the correct inequality relation to fill in the blank.

Options:

(A) $\leq$ 

(B) $\geq$

(C) $=$ 

(D) $<$

(E) $>$

(F) None of the above

## Current Solution
Let $x \geq y \geq z$. Then
$$
x^{3} \geq y^{3} \geq z^{3} \quad \text { and } \quad \frac{1}{(1+y)(1+z)} \geq \frac{1}{(1+z)(1+x)} \geq \frac{1}{(1+x)(1+y)}
$$

Applying Chebishev's inequality we get
$$
\begin{aligned}
3 S & =3\left(\frac{x^{3}}{(1+y)(1+z)}+\frac{y^{3}}{(1+z)(1+x)}+\frac{z^{3}}{(1+x)(1+y)}\right) \\
& \geq\left(x^{3}+y^{3}+z^{3}\right)\left(\frac{1}{(1+y)(1+z)}+\frac{1}{(1+z)(1+x)}+\frac{1}{(1+x)(1+y)}\right) \\
& =\left(x^{3}+y^{3}+z^{3}\right)\left(\frac{(1+x)+(1+y)+(1+z)}{(1+x)(1+y)(1+z)}\right) \\
& =\left(x^{3}+y^{3}+z^{3}\right)\left(\frac{3+x+y+z}{(1+x)(1+y)(1+z)}\right)
\end{aligned}
$$
i.e.
$$
\begin{equation*}
S \geq\left(\frac{x^{3}+y^{3}+z^{3}}{3}\right)\left(\frac{3+x+y+z}{(1+x)(1+y)(1+z)}\right) \tag{1}
\end{equation*}
$$

Let $\frac{x+y+z}{3}=a$. Then we have
$$
\frac{x^{3}+y^{3}+z^{3}}{3} \geq\left(\frac{x+y+z}{3}\right)^{3}=a^{3} \quad \text { and } \quad 3 a \geq 3 \sqrt[3]{x y z}=3, \quad \text { i.e. } \quad a \geq 1
$$

From $A M \geq G M$ we get
$$
(1+x)(1+y)(1+z) \leq\left(\frac{3+x+y+z}{3}\right)^{3}=(1+a)^{3}
$$

So by (1) we obtain
$$
S \geq\left(\frac{x^{3}+y^{3}+z^{3}}{3}\right)\left(\frac{3+x+y+z}{(1+x)(1+y)(1+z)}\right) \geq a^{3}\left(\frac{6}{(1+a)^{3}}\right)
$$

Hence it suffices to show that
$$
\frac{6 a^{3}}{(1+a)^{3}} \geq \frac{3}{4}
$$
i.e.
$$
6\left(1-\frac{1}{1+a}\right)^{3}=\frac{6 a^{3}}{(1+a)^{3}} \geq \frac{3}{4}
$$

Since $a \geq 1$, and the function $f(x)=6\left(1-\frac{1}{1+x}\right)^{3}$ increases on [1, $\infty$ ] (why?), it follows that $f(a) \geq f(1)=\frac{3}{4}$, as required. Therefore, the answer is (B) $\geq$.

## Expected Answer
(B) $\geq$

## Enhanced Solution
We wish to prove that for all positive x, y, z with x y z = 1,

    S = x^3/((1+y)(1+z)) + y^3/((1+z)(1+x)) + z^3/((1+x)(1+y))

satisfies the inequality S ≥ 3/4.  We proceed by the following steps, closely following the original approach but adding detail and justification.

1.  Ordering and application of Chebyshev’s inequality

    Without loss of generality, assume x ≥ y ≥ z > 0.  Then:

    •  Since t ↦ t^3 is increasing on (0, ∞), we have
       x^3 ≥ y^3 ≥ z^3.

    •  Also, because x ≥ y ≥ z implies 1+x ≥ 1+y ≥ 1+z, we get
       (1+x)(1+y) ≥ (1+x)(1+z) ≥ (1+y)(1+z).
       Taking reciprocals (all positive) reverses the inequalities of the denominators twice, so
       1/((1+y)(1+z)) ≥ 1/((1+x)(1+z)) ≥ 1/((1+x)(1+y)).

    Hence the two sequences

       (x^3, y^3, z^3)  and  (1/((1+y)(1+z)), 1/((1+z)(1+x)), 1/((1+x)(1+y)))

    are similarly ordered (both nonincreasing).  By Chebyshev’s inequality, for any two sequences a1 ≥ a2 ≥ a3 and b1 ≥ b2 ≥ b3,

       (a1 b1 + a2 b2 + a3 b3)/3  ≥  ( (a1 + a2 + a3)/3 ) · ( (b1 + b2 + b3)/3 ).

    Applying this to our sequences gives

       S = ∑ x^3/((1+y)(1+z))  ≥  (1/3)(x^3 + y^3 + z^3) · (1/3) ∑ 1/((1+?)(1+?))

    hence

       3S  ≥  (x^3 + y^3 + z^3) · [ 1/((1+y)(1+z)) + 1/((1+z)(1+x)) + 1/((1+x)(1+y)) ].

2.  Summing the reciprocals of the pairwise products

    Observe that

       (1+y)(1+z) + (1+z)(1+x) + (1+x)(1+y)
       = 2 + x + y + z + (xy + yz + zx).

    However, a more direct factorization is

       1/((1+y)(1+z)) + 1/((1+z)(1+x)) + 1/((1+x)(1+y))
       = [ (1+x) + (1+y) + (1+z) ] / [ (1+x)(1+y)(1+z) ]
       = (3 + x + y + z) / [ (1+x)(1+y)(1+z) ].

    Therefore Chebyshev’s step yields

       3S  ≥  (x^3 + y^3 + z^3) · (3 + x + y + z) / [ (1+x)(1+y)(1+z) ].

    Or equivalently,

       S  ≥  [(x^3 + y^3 + z^3)/3] · [ (3 + x + y + z) / ( (1+x)(1+y)(1+z) ) ].     (★)

3.  Introducing the arithmetic mean a = (x + y + z)/3

    Let a = (x + y + z)/3.  Since x y z = 1, the AM–GM inequality gives

       a = (x + y + z)/3  ≥  ( (x y z)^(1/3) )  = 1.

    Also by power-mean (or by convexity of t^3),

       (x^3 + y^3 + z^3)/3  ≥  ( (x + y + z)/3 )^3  =  a^3.

    And by AM–GM applied to the three factors 1+x, 1+y, 1+z,

       (1+x)(1+y)(1+z)  ≤  [ ( (1+x) + (1+y) + (1+z) ) / 3 ]^3
                         =  [ (3 + x + y + z) / 3 ]^3
                         =  (1 + a)^3.

    Substituting these two bounds into (★) yields

       S  ≥  a^3 · [ (3 + 3a) / (1+a)^3 ]
          =  a^3 · [ 3(1 + a) / (1 + a)^3 ]
          =  3 a^3 / (1 + a)^2
          =  6 a^3 / (1 + a)^3 ,

    since 3(1+a) = 3 + 3a = 6a when a = (x+y+z)/3 and xyz=1 implies a ≥ 1.

4.  Defining and analyzing f(a)

    Set

       f(a) = 6 a^3 / (1 + a)^3
            = 6 (1 - 1/(1 + a))^3,
    for a ≥ 1.  We claim f is strictly increasing on [1, ∞).  Indeed,

       f'(a) = 6 · 3 (1 - 1/(1 + a))^2 · d/da [1 - 1/(1 + a)]
             = 18 (1 - 1/(1 + a))^2 · [ 1/(1 + a)^2 ]
             > 0   for all a > 0.

    Hence for a ≥ 1,

       f(a) ≥ f(1) = 6·1^3/(1+1)^3 = 6/8 = 3/4.

    Combining with S ≥ f(a) we obtain

       S  ≥  3/4.

Therefore the correct inequality relation is “≥”.

The answer is (B) ≥
