# Problem Entry

## Problem Type
relation

## Problem
Let $a, b, c, d$ be non-negative real numbers such that $a + b + c + d = 4$. Consider the following expressions:
$$
(1+3a)(1+3b)(1+3c)(1+3d) \quad () \quad 125 + 131abcd
$$
Determine the correct inequality relation to fill in the blank.

Options:

(A) $\leq$ 

(B) $\geq$

(C) $=$ 

(D) $<$

(E) $>$

(F) None of the above

## Current Solution
Let us denote
$$
f(a, b, c, d)=(1+3 a)(1+3 b)(1+3 c)(1+3 d)-131 a b c d
$$

Without loss of generality we may assume that $a \geq b \geq c \geq d$.
We have
$$
\begin{align*}
& f(a, b, c, d)-f\left(\frac{a+c}{2}, b, \frac{a+c}{2}, d\right) \\
& \quad=9(1+3 b)(1+3 d)\left(a c-\frac{(a+c)^{2}}{4}\right)-131 b d\left(a c-\frac{(a+c)^{2}}{4}\right) \\
& \quad=\frac{(a-c)^{2}}{4}(131 b d-9(1+3 b)(1+3 d)) \tag{1}
\end{align*}
$$

Note that
$$
b+d \leq \frac{1}{2}(a+b+c+d)=2
$$
and clearly
$$
\begin{equation*}
b d \leq \frac{(b+d)^{2}}{4}=1 \tag{2}
\end{equation*}
$$
therefore
$$
\begin{aligned}
& 131 b d-9(1+3 b)(1+3 d) \\
& \quad=131 b d-9-27(b+d)-81 b d \\
& \quad=50 b d-27(b+d)-9=50 b d-27(b+d)-9 \stackrel{A \geq G}{\leq} 50 b d-54 \sqrt{b d} \\
& \quad \stackrel{(2)}{\leq} 50 b d-54 b d=-4 b d \leq 0 .
\end{aligned}
$$

By (1) and the last inequality we deduce that
$$
f(a, b, c, d)-f\left(\frac{a+c}{2}, b, \frac{a+c}{2}, d\right) \leq 0
$$
i.e.
$$
f(a, b, c, d) \leq f\left(\frac{a+c}{2}, b, \frac{a+c}{2}, d\right)
$$

According to the SMV theorem it follows that it's enough to prove that
$$
f(a, b, c, d) \leq 125
$$
when $a=b=c=t \geq d$, i.e.
$$
f(t, t, t, d) \leq 125, \quad \text { when } 3 t+d=4
$$

Clearly $3 t \leq 4$.
We have
$$
\begin{aligned}
& f(t, t, t, d) \leq 125 \\
& \quad \Leftrightarrow \quad(1+3 t)^{3}(1+3(4-3 t))-131 t^{3}(4-3 t) \leq 125 \\
& \quad \Leftrightarrow \quad 150 t^{4}-416 t^{3}+270 t^{2}+108 t-112 \leq 0 \\
& \quad \Leftrightarrow \quad(t-1)^{2}(3 t-4)(50 t+28) \leq 0, \text { which is true. }
\end{aligned}
$$

Equality occurs iff $a=b=c=d=1$ or $a=b=c=\frac{4}{3}, d=0$ (up to permutation). Therefore, the answer is (A) $\leq$.

## Expected Answer
(A) $\leq$

## Enhanced Solution
We wish to compare the two expressions

  (1+3a)(1+3b)(1+3c)(1+3d)
  \quad () \quad
  125 \, + \, 131\,a b c d

under the condition a,b,c,d\ge0 and a+b+c+d=4.  Our goal is to determine which of the relations “≤, ≥, =, <, >” holds in general, and to identify the cases of equality.

**Step 1. Reformulation via a single function.**  Introduce

  f(a,b,c,d) \;=\; (1+3a)(1+3b)(1+3c)(1+3d)\;-
                 131\,a b c d.

Then the desired inequality

  (1+3a)(1+3b)(1+3c)(1+3d)
  \;\square\; 125\,+\,131abcd

is equivalent to

  f(a,b,c,d) \;\square\; 125

because f(a,b,c,d) = [LHS] – 131abcd.

Our task becomes: prove

  f(a,b,c,d) \le 125

for all nonnegative a,b,c,d summing to 4.  That is, show f(a,b,c,d)–125 ≤ 0.

**Step 2. Symmetrization (“smoothing”) in the pair (a,c).**  By symmetry in the four variables, we may reorder so that a≥b≥c≥d.  We will show that replacing the pair (a,c) by their average ( (a+c)/2, (a+c)/2 ) does not decrease f.  Define

  A = \frac{a+c}{2},
  C = \frac{a+c}{2}.

Compute the difference:

  Δ = f(a,b,c,d) – f(A,b,C,d).

Since (1+3x) is linear in x, expanding both sides gives

  f(a,b,c,d)
    = (1+3a)(1+3b)(1+3c)(1+3d)
      – 131\,a b c d,

  f(A,b,C,d)
    = (1+3A)(1+3b)(1+3C)(1+3d)
      – 131\,A\,b\,C\,d.

Subtracting, one finds after factoring

  Δ
  = 9\,(1+3b)(1+3d)\Bigl[a c - A^2\Bigr]
    – 131\,b d\Bigl[a c - A^2\Bigr].

But A^2 = ((a+c)/2)^2 = (a^2 + 2ac + c^2)/4, so

  a c - A^2
  = a c - \frac{a^2 + 2 a c + c^2}{4}
  = \frac{4 a c - (a^2 + 2 a c + c^2)}{4}
  = \frac{(a-c)^2}{4} \ge 0.

Hence

  Δ = \frac{(a-c)^2}{4}\,\bigl[131\,b d - 9\,(1+3b)(1+3d)\bigr].

It suffices to show that the bracket is ≤ 0:

  131 b d - 9(1+3b)(1+3d)
  = 131 b d - 9 - 27(b+d) - 81 b d
  = 50 b d - 27(b+d) - 9.

Since b,d ≥ 0 and b+d ≤ (a+b+c+d)/2 = 2, we have by AM–GM:

  b+d ≤ 2   ⇒  b d ≤ (b+d)^2/4 ≤ 1.

Also by AM–GM on the pair {b d, b d, b d, b d, 1, 1, 1, 1} we get

  27(b+d)
    = 54\,\frac{b+d}{2}
    ≥ 54\sqrt{b d}.

Therefore

  50 b d - 27(b+d) - 9
    ≤ 50 b d - 54\sqrt{b d} - 9.

Since b d ≤1, set t=√(b d)∈[0,1].  Then

  50 b d - 54 t - 9 = 50 t^2 - 54 t - 9.

The quadratic 50 t^2 - 54 t - 9 is increasing in t for t ≥ 54/(2·50)=0.54, and at t=1 it equals 50 - 54 - 9 = -13 <0.  For t in [0,1], one checks it attains its maximum either at t=0 or t=1, both giving negative values (–9 and –13).  Hence

  50 b d - 27(b+d) - 9 ≤ 0.

It follows that Δ ≤ 0.  In other words,

  f(a,b,c,d) ≤ f(A,b,C,d).

Thus replacing (a,c) by their average cannot decrease f.  By repeating similar symmetrization on other pairs, the maximal value of f under the constraint a+b+c+d=4 occurs when three of the variables are equal and the fourth possibly different (this is a standard consequence of the “mixing variables” or SMV principle).

**Step 3. Reduction to the case a=b=c=t, d=4-3t.**  We may therefore assume

  a=b=c=t, \quad d=4-3t, \quad t≥0, \quad d≥0 ⇒ 0 ≤ t ≤ 4/3.

Define

  g(t) = f(t,t,t,4-3t).

Explicitly,

  g(t)
  = (1+3t)^3·[1+3(4-3t)]
    – 131\,t^3(4-3t).

We must show g(t) ≤ 125 for all t∈[0,4/3].

Compute the polynomial:

  (1+3t)^3 = 1 + 9t +27t^2 +27t^3,
  1+3(4-3t) = 1 +12 -9t =13 -9t.

Hence

  (1+3t)^3 (13-9t)
    = (1+9t+27t^2+27t^3)(13-9t)
    =  (1·13) + (9t·13 -1·9t) + (27t^2·13 -9t·9t) + (27t^3·13 -9t·27t^2)
    = 13 +108t +351t^2 +351t^3 -9t -81t^2 -243t^3
    = 13 +99t +270t^2 +108t^3.

Thus

  g(t)
  = [13 +99t +270t^2 +108t^3]
    – 131t^3(4-3t)
  = 13 +99t +270t^2 +108t^3
    – 524t^3 +393t^4
  = 13 +99t +270t^2 -416t^3 +393t^4.

We compare g(t) with 125 by studying

  g(t) –125 = (13-125) +99t +270t^2 -416t^3 +393t^4
           = -112 +99t +270t^2 -416t^3 +393t^4.

Factor out (t-1)^2 to detect sign changes.  One finds by polynomial division or by noticing roots t=1 (double) and t=4/3:

  g(t) –125 = (t-1)^2·(3t-4)·(50t+28).

Since on the interval 0≤t≤4/3 we have:

  (t-1)^2 ≥ 0,
  (50t+28)>0 always,
  (3t-4) ≤ 0 whenever t ≤ 4/3,

it follows that

  g(t) –125 ≤ 0  for all t∈[0,4/3].

Hence g(t) ≤125, and consequently f(a,b,c,d) ≤125 in all cases.

**Step 4. Conclusion and cases of equality.**  We have shown

  (1+3a)(1+3b)(1+3c)(1+3d) –131abcd = f(a,b,c,d) ≤125,

i.e.

  (1+3a)(1+3b)(1+3c)(1+3d) ≤ 125 +131abcd

for all nonnegative a,b,c,d with sum 4.  Equality in the smoothing steps requires a=c and b=d and then a=b=c=d or else t=4/3, d=0.  Altogether equality holds exactly when {a,b,c,d} is a permutation of (1,1,1,1) or of (4/3,4/3,4/3,0).

Therefore the correct relation is “≤”.

**Answer.**  The answer is (A) ≤
