# Problem Entry

## Problem Type
relation

## Problem
Let $a, b, c \in \mathbb{R}^{+}$. Consider the following inequality:
$$
(a+b+c)^{3} \quad () \quad a^{3}+b^{3}+c^{3}+24 a b c .
$$

Determine the correct inequality relation to fill in the blank.

Options:

(A) $\leq$ 

(B) $\geq$

(C) $=$ 

(D) $<$

(E) $>$

(F) None of the above

## Current Solution
We have
$$
\begin{aligned}
(a+b+c)^{3} & =a^{3}+b^{3}+c^{3}+6 a b c+3\left(a^{2} b+a^{2} c+b^{2} a+b^{2} c+c^{2} a+c^{2} b\right) \\
& \geq a^{3}+b^{3}+c^{3}+6 a b c+3 \cdot 6 \sqrt[6]{a^{6} b^{6} c^{6}}=a^{3}+b^{3}+c^{3}+24 a b c
\end{aligned}
$$

Equality holds if and only if $a=b=c$. Therefore, the answer is (B) $\geq$.

## Expected Answer
(B) $\geq$

## Enhanced Solution
We wish to compare
\[(a+b+c)^{3}\quad()\quad a^{3}+b^{3}+c^{3}+24abc\]
for positive real numbers a,b,c.  We proceed by expanding the left-hand side and then applying the AM–GM inequality to the mixed terms.

**Step 1. Expand \((a+b+c)^3\).**

By the multinomial (or binomial) expansion,
\[
(a+b+c)^{3}
= a^{3}+b^{3}+c^{3}
  + 3\bigl(a^{2}b + a^{2}c + b^{2}a + b^{2}c + c^{2}a + c^{2}b\bigr)
  + 6abc.
\]
Group the terms as follows:
\[
(a+b+c)^{3}
= \bigl(a^{3}+b^{3}+c^{3}\bigr)
  + 6abc
  + 3\sum_{\text{sym}} a^{2}b,
\]
where “\(\sum_{\text{sym}}a^{2}b\)” denotes the six terms
\(a^{2}b, a^{2}c, b^{2}a, b^{2}c, c^{2}a, c^{2}b\).

**Step 2. Apply AM–GM to the six mixed terms.**

By the Arithmetic Mean–Geometric Mean inequality, for any six positive numbers
\(x_{1},x_{2},\dots,x_{6}\),
\[
\frac{x_{1}+x_{2}+\cdots+x_{6}}{6}
\ge \sqrt[6]{x_{1}x_{2}\cdots x_{6}},
\]
with equality precisely when \(x_{1}=x_{2}=\cdots=x_{6}\).

Set
\[
x_{1} = a^{2}b,
\quad x_{2} = a^{2}c,
\quad x_{3} = b^{2}a,
\quad x_{4} = b^{2}c,
\quad x_{5} = c^{2}a,
\quad x_{6} = c^{2}b.
\]
Then their product is
\[
\prod_{i=1}^{6} x_{i}
= (a^{2}b)(a^{2}c)(b^{2}a)(b^{2}c)(c^{2}a)(c^{2}b)
= a^{6}b^{6}c^{6}=(abc)^{6}.
\]
Hence
\[
\sum_{\text{sym}} a^{2}b
= x_{1}+\cdots+x_{6}
\ge 6\sqrt[6]{(abc)^{6}} = 6\,abc.
\]

**Step 3. Combine the inequalities.**
Substitute back into the expansion:
\[
(a+b+c)^{3}
= a^{3}+b^{3}+c^{3}
  +6abc
  +3\sum_{\text{sym}}a^{2}b
\ge a^{3}+b^{3}+c^{3}
  +6abc
  +3\times(6abc)
= a^{3}+b^{3}+c^{3}+24abc.
\]
Thus we have shown
\[
(a+b+c)^{3} \ge a^{3}+b^{3}+c^{3}+24abc.
\]

**Step 4. Determine the equality case.**
Equality in AM–GM occurs exactly when
\(a^{2}b = a^{2}c = b^{2}a = b^{2}c = c^{2}a = c^{2}b\).
Since \(a,b,c>0\), this forces \(a=b=c\).  Hence the inequality is strict whenever the three variables are not all equal.

Therefore, the correct relation is “greater than or equal to.”  The answer is

The answer is (B) ≥
