# Problem Entry

## Problem Type
relation

## Problem
Let $a, b, c$ be any real numbers. Consider the following inequality:
$$
\sum\left(1+a^{2}\right)^{2}\left(1+b^{2}\right)^{2}(a-c)^{2}(b-c)^{2} \quad () \quad \left(1+a^{2}\right)\left(1+b^{2}\right)\left(1+c^{2}\right)(a-b)^{2}(b-c)^{2}(c-a)^{2}.
$$

Determine the correct inequality relation to fill in the blank.

Options:

(A) $\leq$ 

(B) $\geq$

(C) $=$ 

(D) $<$

(E) $>$

(F) None of the above

## Current Solution
The inequality can be also written as $\sum \frac{\left(1+a^{2}\right)\left(1+b^{2}\right)}{\left(1+c^{2}\right)(a-b)^{2}} \geq 1$ (of course, we may assume that $a, b, c$ are distinct). Now, adding the inequalities

$$
\frac{\left(1+a^{2}\right)\left(1+b^{2}\right)}{\left(1+c^{2}\right)(a-b)^{2}}+\frac{\left(1+b^{2}\right)\left(1+c^{2}\right)}{\left(1+a^{2}\right)(b-c)^{2}} \geq 2 \frac{1+b^{2}}{|a-b||c-b|}
$$

(which can be found using the AM-GM Inequality) we deduce that

$$
\sum \frac{\left(1+a^{2}\right)\left(1+b^{2}\right)}{\left(1+c^{2}\right)(a-b)^{2}} \geq \sum \frac{1+b^{2}}{|(b-a)(b-c)|}
$$

and so it is enough to prove that the last quantity is at least 1. But it follows from

$$
\sum \frac{1+b^{2}}{|(b-a)(b-c)|} \geq\left|\sum \frac{1+b^{2}}{(b-a)(b-c)}\right|=1
$$

and the problem is solved. Therefore, the answer is (B) $\geq$.

## Expected Answer
(B) $\geq$

## Enhanced Solution
We wish to prove that for all real numbers a,b,c (assumed distinct to avoid zero denominators), the following holds:

  ∑₍cyc₎ (1 + a²)²(1 + b²)²(a – c)²(b – c)²   ≥   (1 + a²)(1 + b²)(1 + c²)
                                    ·(a – b)²(b – c)²(c – a)².

1.  Reduction by a common positive factor
-----------------------------------------
Since for any real x we have 1 + x² > 0 and for distinct a,b we have (a – b)² > 0, the product

   D = (1 + a²)(1 + b²)(1 + c²)
       · (a – b)²(b – c)²(c – a)²

is strictly positive.  Dividing both sides of the given inequality by D (which does not change the direction of “≥”) yields the equivalent form

   ∑₍cyc₎
   { (1 + a²)²(1 + b²)²(a – c)²(b – c)² }
   / D   ≥  1.

Each term in the sum simplifies by canceling one factor of (1 + a²)(1 + b²) and the factors (a – c)²,(b – c)² against the corresponding ones in D (using (c – a)²=(a – c)²).  One obtains

   𝑋_{ab}  :=  (1 + a²)(1 + b²)
              ---------------------
              (1 + c²)
              (a – b)²

and similarly for the cyclic permutations.  Thus the inequality becomes

   X_{ab} + X_{bc} + X_{ca}  ≥  1.                                          (★)

2.  Applying AM–GM to pairs of terms
---------------------------------------
By the arithmetic–geometric mean inequality, for instance,

   X_{ab} + X_{bc}
   ≥  2 · √( X_{ab} · X_{bc} )
   =  2 · √{
          (1+a²)(1+b²)
          (1+b²)(1+c²)
        }
        / √{
          (1+c²)(1+a²)
          (a–b)²(b–c)²
        }
   =  2·(1 + b²) / |(a – b)(b – c)|.

By cyclically permuting (a,b,c) in this argument, we obtain three such inequalities.  Adding them gives

   2·(X_{ab} + X_{bc} + X_{ca})
   ≥  2·∑₍cyc₎ (1 + b²) / |(b – a)(b – c)|

and dividing by 2 yields

   X_{ab} + X_{bc} + X_{ca}
   ≥  ∑₍cyc₎  (1 + b²) / |(b – a)(b – c)|.                                  (★★)

Hence to prove (★) it suffices to show

   S := ∑₍cyc₎  (1 + b²) / |(b – a)(b – c)|  ≥  1.

3.  Concluding via a known algebraic identity
------------------------------------------------
First observe by the triangle inequality that

   S  ≥  |  ∑₍cyc₎  (1 + b²) / [(b – a)(b – c)]  |.

We claim the signed sum inside the absolute value equals 1.  Equivalently,

   ∑₍cyc₎  (1 + b²) / [(b – a)(b – c)]  =  1.

This identity can be seen most succinctly via Lagrange interpolation: the quadratic polynomial f(x)=1+x² is uniquely determined by its values at x=a,b,c.  Its Lagrange form is

   f(x)  =  (1+a²) · (x – b)(x – c)/[(a – b)(a – c)]
         + (1+b²) · (x – c)(x – a)/[(b – c)(b – a)]
         + (1+c²) · (x – a)(x – b)/[(c – a)(c – b)].

Extracting the coefficient of x² on both sides gives 1 on the left and

   (1+a²)/[(a – b)(a – c)]  +  (1+b²)/[(b – c)(b – a)]  +  (1+c²)/[(c – a)(c – b)]

on the right.  Hence the sum of those three fractions is exactly 1.  Returning to S, we have

   S  ≥  |1|  =  1.

Combining this with (★★) and the reduction in step 1 shows the original inequality holds in the form “≥.”

Therefore the correct choice is

The answer is (B) ≥
