# Problem Entry

## Problem Type
relation

## Problem
Let $a, b, c$ be positive real numbers such that $a b c = 1$. Consider the following inequality:
$$
\frac{a}{\sqrt{7+b^{2}+c^{2}}}+\frac{b}{\sqrt{7+c^{2}+a^{2}}}+\frac{c}{\sqrt{7+a^{2}+b^{2}}} \quad () \quad 1 .
$$

Determine the correct inequality relation to fill in the blank.

Options:

(A) $\leq$ 

(B) $\geq$

(C) $=$ 

(D) $<$

(E) $>$

(F) None of the above

## Current Solution
Denote
$$
A=\frac{a}{\sqrt{7+b^{2}+c^{2}}}+\frac{b}{\sqrt{7+c^{2}+a^{2}}}+\frac{c}{\sqrt{7+a^{2}+b^{2}}}
$$
and
$$
B=a\left(7+b^{2}+c^{2}\right)+b\left(7+c^{2}+a^{2}\right)+c\left(7+a^{2}+b^{2}\right)
$$

By Hölder's inequality we have
$$
\begin{equation*}
A^{2} B \geq(a+b+c)^{3} . \tag{1}
\end{equation*}
$$

Furthermore
$$
\begin{align*}
B & =7(a+b+c)+(a+b+c)(a b+b c+c a)-3 \\
& \leq 7(a+b+c)+\frac{(a+b+c)^{3}}{3}-3 \leq(a+b+c)^{3} \tag{2}
\end{align*}
$$
and by (1) and (2) we obtain
$$
A^{2} \geq \frac{(a+b+c)^{3}}{B} \geq 1, \quad \text { i.e. } \quad A \geq 1
$$
as required. Therefore, the answer is (B) $\geq$.

## Expected Answer
(B) $\geq$

## Enhanced Solution
We begin by setting
\[
A \,=\,\frac{a}{\sqrt{7+b^{2}+c^{2}}} \;+
\frac{b}{\sqrt{7+c^{2}+a^{2}}} \;+
\frac{c}{\sqrt{7+a^{2}+b^{2}}}
\]
and
\[
B \,=\,a\bigl(7+b^{2}+c^{2}\bigr)
\;+
 b\bigl(7+c^{2}+a^{2}\bigr)
\;+
 c\bigl(7+a^{2}+b^{2}\bigr).
\]
Our goal is to compare $A$ with $1$.  

1.  Application of Hölder’s Inequality

We apply Hölder’s inequality in the form
\[
\Bigl(\sum_{\cyc}x_i y_i\Bigr)^{2}
\le\,
\Bigl(\sum_{\cyc}x_i^{2} z_i\Bigr)
\Bigl(\sum_{\cyc}\frac{y_i^{2}}{z_i}\Bigr),
\]
where we choose for the three cyclic terms:
\[
x_i =1,
\quad y_i = \sqrt{a},
\quad z_i = a\bigl(7+b^{2}+c^{2}\bigr)
\]
(for the term corresponding to $a$, and similarly for $b,c$).  Concretely, this yields
\[
\bigl(A\bigr)^{2}
\;\times\;B
\;=\;
\Bigl(\sum_{\cyc}\frac{a}{\sqrt{7+b^{2}+c^{2}}}\Bigr)^{2}
\times
\sum_{\cyc}a\bigl(7+b^{2}+c^{2}\bigr)
\ge
(\sqrt{a}+\sqrt{b}+\sqrt{c})^{4}.
\]
Since $abc=1$, we have by the AM–GM inequality
\[
\sqrt{a}+\sqrt{b}+\sqrt{c}\ge3\sqrt[6]{abc}=3,
\]
so
\[
(\sqrt{a}+\sqrt{b}+\sqrt{c})^{4}\ge3^{4}=81.
\]
Thus from Hölder
\[
A^{2}\,B\ge81.  \tag{1}
\]

2.  Upper bound for $B$

Next we expand and estimate $B$:
\[
B
= a(7+b^{2}+c^{2}) + b(7+c^{2}+a^{2}) + c(7+a^{2}+b^{2})
=7(a+b+c)
+\sum_{\cyc}a(b^{2}+c^{2}).
\]
Observe that
\[
\sum_{\cyc}a(b^{2}+c^{2})
= (a+b+c)(ab+bc+ca) -3abc
= (a+b+c)(ab+bc+ca) -3.
\]
By the well-known inequality $ab+bc+ca\le\tfrac{(a+b+c)^{2}}{3}$ and using $abc=1$, we get
\[
\sum_{\cyc}a(b^{2}+c^{2})
\le (a+b+c)\cdot\frac{(a+b+c)^{2}}{3} -3
=\frac{(a+b+c)^{3}}{3} -3.
\]
Hence
\[
B \le 7(a+b+c)
+\Bigl(\frac{(a+b+c)^{3}}{3} -3\Bigr)
= \frac{(a+b+c)^{3}}{3} +7(a+b+c) -3.
\]
Set $S=a+b+c$.  We want to show
\[
\frac{S^{3}}{3}+7S-3 \le S^{3},
\]
which is equivalent to
\[
2S^{3}/3 -7S +3 \ge0.
\]
Define $f(S)=2S^{3}/3 -7S +3$.  Then
\[
f'(S)=2S^{2}-7>0\quad\text{for }S\ge3,
\]
and since AM–GM gives $S=a+b+c\ge3\sqrt[3]{abc}=3$, we have $f'(S)>0$ on $[3,\infty)$.  Moreover,
\[
f(3)=2\cdot3^{3}/3 -7\cdot3 +3=18-21+3=0.
\]
It follows that $f(S)\ge0$ for all $S\ge3$, i.e.
\[
B\le S^{3}=(a+b+c)^{3}.  \tag{2}
\]

3.  Conclusion

Combining (1) and (2) gives
\[
A^{2}\ge\frac{81}{B}\ge\frac{81}{(a+b+c)^{3}}\times (a+b+c)^{3}=1,
\]
so $A\ge1$.  Hence the correct inequality is
\[
\frac{a}{\sqrt{7+b^{2}+c^{2}}}+\frac{b}{\sqrt{7+c^{2}+a^{2}}}+\frac{c}{\sqrt{7+a^{2}+b^{2}}}\;\ge\;1.
\]
The answer is (B) ≥
