# Problem Entry

## Problem Type
relation

## Problem
Let $a, b, c$ be positive real numbers such that $a b c = 1$. Consider the following inequality:
$$
\frac{a}{a+b^{4}+c^{4}}+\frac{b}{b+c^{4}+a^{4}}+\frac{c}{c+a^{4}+b^{4}} \quad () \quad 1 .
$$

Determine the correct inequality relation to fill in the blank.

Options:

(A) $\leq$ 

(B) $\geq$

(C) $=$ 

(D) $<$

(E) $>$

(F) None of the above

## Current Solution
By the Cauchy-Schwarz inequality we have
$$
\frac{a}{a+b^{4}+c^{4}}=\frac{a\left(a^{3}+2\right)}{\left(a+b^{4}+c^{4}\right)\left(a^{3}+1+1\right)} \leq \frac{a\left(a^{3}+2\right)}{\left(a^{2}+b^{2}+c^{2}\right)^{2}}
$$

Similarly we get
$$
\frac{b}{b+c^{4}+a^{4}} \leq \frac{b\left(b^{3}+2\right)}{\left(a^{2}+b^{2}+c^{2}\right)^{2}} \quad \text { and } \quad \frac{c}{c+a^{4}+b^{4}} \leq \frac{c\left(c^{3}+2\right)}{\left(a^{2}+b^{2}+c^{2}\right)^{2}}
$$

Hence
$$
\frac{a}{a+b^{4}+c^{4}}+\frac{b}{b+c^{4}+a^{4}}+\frac{c}{c+a^{4}+b^{4}} \leq \frac{a^{4}+b^{4}+c^{4}+2(a+b+c)}{\left(a^{2}+b^{2}+c^{2}\right)^{2}}
$$
and we need to prove that
$$
\left(a^{2}+b^{2}+c^{2}\right)^{2} \geq a^{4}+b^{4}+c^{4}+2(a+b+c)
$$
which is equivalent to
$$
a^{2} b^{2}+b^{2} c^{2}+c^{2} a^{2} \geq a+b+c
$$

By the well-known inequality $a^{2} b^{2}+b^{2} c^{2}+c^{2} a^{2} \geq a b c(a+b+c)$ and $a b c=1$, we have
$$
a^{2} b^{2}+b^{2} c^{2}+c^{2} a^{2} \geq a b c(a+b+c)=a+b+c
$$
as required. Therefore, the answer is (A) $\leq$.

## Expected Answer
(A) $\leq$

## Enhanced Solution
We wish to show that for any positive reals a,b,c with abc=1, the cyclic sum
    S = a/(a + b^4 + c^4)  +  b/(b + c^4 + a^4)  +  c/(c + a^4 + b^4)
satisfies the inequality S ≤ 1.  We proceed in three main steps:

1.  Apply Cauchy–Schwarz to each term.
   Fix one term, say T = a/(a + b^4 + c^4).  Introduce the two vectors in ℝ^3:
     U = (√a,  √(b^4),  √(c^4))
     V = (√(a^3), 1, 1).
   Then by the Cauchy–Schwarz inequality,
     (U·V)²  ≤  ‖U‖² · ‖V‖².
   Here
     U·V  =  √a·√(a^3)  +  √(b^4)·1  +  √(c^4)·1
           =  a^2 + b^2 + c^2,
     ‖U‖² = a + b^4 + c^4,
     ‖V‖² = a^3 + 1 + 1 = a^3 + 2.
   Hence
     (a^2 + b^2 + c^2)²  ≤  (a + b^4 + c^4)(a^3 + 2)
   and consequently
     1/(a + b^4 + c^4)  ≤  (a^3 + 2)/(a^2 + b^2 + c^2)².
   Multiplying both sides by a>0 gives
     a/(a + b^4 + c^4)  ≤  a·(a^3 + 2)/(a^2 + b^2 + c^2)².
   The same argument, by cyclic permutation of (a,b,c), yields
     b/(b + c^4 + a^4)  ≤  b·(b^3 + 2)/(a^2 + b^2 + c^2)²,
     c/(c + a^4 + b^4)  ≤  c·(c^3 + 2)/(a^2 + b^2 + c^2)².

2.  Sum the three estimates.
   Adding the three upper bounds, we obtain
     S  ≤  [a(a^3 + 2) + b(b^3 + 2) + c(c^3 + 2)]/(a^2 + b^2 + c^2)²
        = [a^4 + b^4 + c^4  + 2(a + b + c)]/(a^2 + b^2 + c^2)².
   Therefore the desired inequality S ≤ 1 is equivalent to
     (a^4 + b^4 + c^4 + 2(a + b + c))  ≤  (a^2 + b^2 + c^2)².

3.  Reduce to a known symmetric inequality.
   Expand the right–hand side:
     (a^2 + b^2 + c^2)²
       = a^4 + b^4 + c^4  + 2(a^2b^2 + b^2c^2 + c^2a^2).
   Thus the inequality becomes
     a^4 + b^4 + c^4 + 2(a + b + c)
     ≤  a^4 + b^4 + c^4 + 2(a^2b^2 + b^2c^2 + c^2a^2)
   ⇔  a + b + c  ≤  a^2b^2 + b^2c^2 + c^2a^2.
   But by the well-known fact that for positive a,b,c,
     a^2b^2 + b^2c^2 + c^2a^2  ≥  abc (a + b + c),
   and using abc=1, we conclude
     a^2b^2 + b^2c^2 + c^2a^2  ≥  1·(a + b + c)  =  a + b + c.
   This completes the proof that S ≤ 1.

Hence the correct relation is “≤”.
The answer is (A) ≤
