# Problem Entry

## Problem Type
relation

## Problem
Let $a, b, c$ be positive real numbers. Consider the following inequality:
$$
\left(a^{2}+2\right)\left(b^{2}+2\right)\left(c^{2}+2\right) \quad () \quad 9(a b+b c+a c) .
$$

Determine the correct inequality relation to fill in the blank.

Options:

(A) $\leq$ 

(B) $\geq$

(C) $=$ 

(D) $<$

(E) $>$

(F) None of the above

## Current Solution
Let $a=\sqrt{2} \tan \alpha, b=\sqrt{2} \tan \beta, c=\sqrt{2} \tan \gamma$ where $\alpha, \beta, \gamma \in(0, \pi / 2)$. Then using the well-known identity $1+\tan ^{2} x=\frac{1}{\cos ^{2} x}$ the given inequality becomes
$$
\frac{8}{\cos ^{2} \alpha \cdot \cos ^{2} \beta \cdot \cos ^{2} \gamma} \geq 9\left(\frac{2}{\tan \alpha \tan \beta}+\frac{2}{\tan \beta \tan \gamma}+\frac{2}{\tan \gamma \tan \alpha}\right)
$$
i.e.
$\cos \alpha \cos \beta \cos \gamma(\cos \alpha \sin \beta \sin \gamma+\sin \alpha \cos \beta \sin \gamma+\sin \alpha \sin \beta \cos \gamma) \leq \frac{4}{9}$.

Also since
$$
\begin{aligned}
\cos (\alpha+\beta+\gamma)= & \cos \alpha \cos \beta \cos \gamma-\cos \alpha \sin \beta \sin \gamma-\sin \alpha \cos \beta \sin \gamma \\
& -\sin \alpha \sin \beta \cos \gamma
\end{aligned}
$$
inequality is equivalent to
$$
\begin{equation*}
\cos \alpha \cos \beta \cos \gamma(\cos \alpha \cos \beta \cos \gamma-\cos (\alpha+\beta+\gamma)) \leq \frac{4}{9} \tag{1}
\end{equation*}
$$

Let $\theta=\frac{\alpha+\beta+\gamma}{3}$.
Since $\cos \alpha, \cos \beta, \cos \gamma>0$, and since the function $\cos x$ is concave on $(0, \pi / 2)$ by the inequality $A M \geq G M$ and Jensen's inequality, we obtain
$$
\cos \alpha \cos \beta \cos \gamma \leq\left(\frac{\cos \alpha+\cos \beta+\cos \gamma}{3}\right)^{3} \leq \cos ^{3} \theta
$$

Therefore according to (1) we need to prove that
$$
\begin{equation*}
\cos ^{3} \theta\left(\cos ^{3} \theta-\cos 3 \theta\right) \leq \frac{4}{9} \tag{2}
\end{equation*}
$$

Using the trigonometric identity
$$
\cos 3 \theta=4 \cos ^{3} \theta-3 \cos \theta, \quad \text { i.e. } \quad \cos ^{3} \theta-\cos 3 \theta=3 \cos \theta-3 \cos ^{3} \theta
$$
inequality $(2)$ becomes
$$
\cos ^{4} \theta\left(1-\cos ^{2} \theta\right) \leq \frac{4}{27}
$$
which follows by the inequality $A M \geq G M$ :
$$
\left(\frac{\cos ^{2} \theta}{2} \cdot \frac{\cos ^{2} \theta}{2} \cdot\left(1-\cos ^{2} \theta\right)\right)^{3} \leq \frac{1}{3}\left(\frac{\cos ^{2} \theta}{2}+\frac{\cos ^{2} \theta}{2}+\left(1-\cos ^{2} \theta\right)\right)=\frac{1}{3}
$$

Equality occurs iff $\tan \alpha=\tan \beta=\tan \gamma=\frac{1}{\sqrt{2}}$, i.e. iff $a=b=c=1$. Therefore, the answer is (B) $\geq$.

## Expected Answer
(B) $\geq$

## Enhanced Solution
Enhanced Solution:

We wish to determine which of the relations “≤, ≥, =, <, >, None” makes the inequality

    (a²+2)(b²+2)(c²+2)  ( ? )  9(ab + bc + ca)

valid for all positive real a,b,c.  We shall show, by a chain of equivalent transformations and well–justified estimates, that the correct sign is “≥”.  Our approach proceeds in the following steps:

1.  Substitution via tangents.  Since a,b,c>0, we set

    a = √2 · tan α,
    b = √2 · tan β,
    c = √2 · tan γ,

with α,β,γ ∈ (0,π/2).  Then using 1 + tan²x = 1/cos²x we get

    a² + 2 = 2 tan²α + 2 = 2(1 + tan²α) = 2 / cos²α,

and similarly for b²+2 and c²+2.  Hence the left–hand side becomes

    (a²+2)(b²+2)(c²+2)
    = [2/cos²α]·[2/cos²β]·[2/cos²γ]
    = 8 / (cos²α·cos²β·cos²γ).

Meanwhile,

    ab + bc + ca = (√2 tanα)(√2 tanβ) + ... = 2(tanα tanβ + tanβ tanγ + tanγ tanα).

Thus the original inequality

    (a²+2)(b²+2)(c²+2)  (?)  9(ab+bc+ca)

becomes, after substitution,

    8 / (cos²α cos²β cos²γ)  (?)  9·2(tanα tanβ + tanβ tanγ + tanγ tanα).

2.  Clearing denominators.  Multiply both sides by cos²α cos²β cos²γ>0 to obtain an equivalent relation

    8  (?)  18 cos²α cos²β cos²γ ·(tanα tanβ + tanβ tanγ + tanγ tanα).

Since tanα tanβ = (sinα sinβ)/(cosα cosβ), we rewrite the right–hand side as

    18[cos²α cos²β cos²γ · tanα tanβ + …]
    = 18[cosα cosβ sinα sinβ·cos²γ + …]
    = 18 cosα cosβ cosγ [sinα sinβ cosγ + sinβ sinγ cosα + sinγ sinα cosβ].

Hence the inequality is equivalent to

    8  (?)  18 cosα cosβ cosγ ·(sinα sinβ cosγ + sinβ sinγ cosα + sinγ sinα cosβ).

Dividing both sides by 18>0 gives the final transformed requirement:

    cosα cosβ cosγ ·(sinα sinβ cosγ + sinβ sinγ cosα + sinγ sinα cosβ)  (?)  4/9.

3.  Rewriting via cos(α+β+γ).  Recall the identity

    cos(α+β+γ)
    = cosα cosβ cosγ
      − [cosα sinβ sinγ + sinα cosβ sinγ + sinα sinβ cosγ].

Hence

    sinα sinβ cosγ + sinβ sinγ cosα + sinγ sinα cosβ
    = cosα cosβ cosγ − cos(α+β+γ).

Substitution shows the transformed inequality is equivalent to

    cosα cosβ cosγ · [cosα cosβ cosγ − cos(α+β+γ)]  (?)  4/9.

4.  Symmetrization and Jensen’s inequality.  Let S = α+β+γ and define θ = S/3.  Since cosx is positive and concave on (0,π/2), by Jensen’s inequality we have

    (cosα + cosβ + cosγ)/3  ≤  cos((α+β+γ)/3) = cos θ.

Also by the AM–GM inequality,

    cosα cosβ cosγ  ≤  [(cosα + cosβ + cosγ)/3]³  ≤  (cos θ)³.

Thus

    cosα cosβ cosγ  ≤  cos³θ,

and consequently

    (cosα cosβ cosγ)²  ≤  cos⁶θ,

so that the left factor in our product satisfies

    cosα cosβ cosγ  ≤  cos³θ.

Moreover, replacing α+β+γ by 3θ in the second factor yields cos(α+β+γ) = cos 3θ.  Hence our inequality reduces to the one–variable form

    cos³θ · [cos³θ − cos 3θ]  (?)  4/9.

5.  Using the triple–angle formula.  From

    cos 3θ = 4 cos³θ − 3 cosθ,

we get

    cos³θ − cos 3θ = cos³θ − (4cos³θ − 3cosθ)
                   = 3cosθ − 3cos³θ
                   = 3cosθ(1 − cos²θ)
                   = 3cosθ sin²θ.

Therefore the one–variable inequality becomes

    cos³θ ·[3cosθ sin²θ]  (?)  4/9
  ⇔ 3cos⁴θ sin²θ  (?)  4/9
  ⇔ cos⁴θ sin²θ  (?)  4/27.

6.  Final AM–GM estimate.  We write

    cos⁴θ sin²θ = [ (cos²θ)/2 · (cos²θ)/2 · (sin²θ) ] ·4.

By the AM–GM inequality on the three nonnegative terms (cos²θ)/2, (cos²θ)/2, sin²θ,

    [(cos²θ)/2 + (cos²θ)/2 + sin²θ] / 3  ≥  [((cos²θ)/2)·((cos²θ)/2)·(sin²θ)]^(1/3).

But the left–hand side is

    [(cos²θ)+ sin²θ] / 3  = 1/3.

Hence

    [((cos²θ)/2)·((cos²θ)/2)·(sin²θ)]  ≤  (1/3)³ = 1/27.

Multiplying by 4 gives

    cos⁴θ sin²θ  ≤  4/27,

which is exactly the desired bound.  Throughout, each step is an equivalence or an inequality that preserves the “≥” direction, and at no point do we reverse the sign.  

Equality can occur only if all the AM–GM and Jensen estimates are equalities.  From Jensen we need α=β=γ, hence θ=α=β=γ.  From the final AM–GM we require (cos²θ)/2 = sin²θ, i.e.

    cos²θ = 2 sin²θ  ⇒  cot²θ = 2  ⇒  tanθ = 1/√2.

Thus a = √2 tanα = 1, and similarly b=c=1.  The boundary case (a,b,c)=(1,1,1) makes both sides equal.  

Accordingly, the original inequality holds in the form

    (a²+2)(b²+2)(c²+2)  ≥  9(ab + bc + ca)

for all positive a,b,c, with equality precisely at a=b=c=1.

The answer is (B) ≥
