# Problem Entry

## Problem Type
relation

## Problem
Let $a, b, c, d$ be positive real numbers such that $a^{2}+b^{2}+c^{2}+d^{2}=1$. Consider the following expressions:
$$
\sqrt{1-a}+\sqrt{1-b}+\sqrt{1-c}+\sqrt{1-d} \quad () \quad \sqrt{a}+\sqrt{b}+\sqrt{c}+\sqrt{d}
$$
Determine the correct inequality relation to fill in the blank.

Options:

(A) $\leq$ 

(B) $\geq$

(C) $=$ 

(D) $<$

(E) $>$

(F) None of the above

## Current Solution
First we'll show that
$$
\begin{equation*}
a+b+c+d \leq 2 \tag{1}
\end{equation*}
$$

We have
$$
\frac{a+b+c+d}{4} \leq \sqrt{\frac{a^{2}+b^{2}+c^{2}+d^{2}}{4}}=\frac{1}{2}
$$
i.e.
$$
a+b+c+d \leq 2
$$

Furthermore
$$
\begin{equation*}
\sqrt{1-a}-\sqrt{a}=\frac{(\sqrt{1-a}-\sqrt{a})(\sqrt{1-a}+\sqrt{a})}{\sqrt{1-a}+\sqrt{a}}=\frac{1-2 a}{\sqrt{1-a}+\sqrt{a}} \tag{2}
\end{equation*}
$$

By $A M \leq Q M$ we have
$$
\begin{equation*}
\frac{\sqrt{1-a}+\sqrt{a}}{2} \leq \sqrt{\frac{1-a+a}{2}}=\frac{1}{\sqrt{2}}, \quad \text { i.e. } \quad \frac{1}{\sqrt{1-a}+\sqrt{a}} \geq \frac{1}{\sqrt{2}} \tag{3}
\end{equation*}
$$

Using (2) and (3) we deduce
$$
\sqrt{1-a}-\sqrt{a} \geq \frac{1-2 a}{\sqrt{2}}
$$

Similarly
$$
\begin{aligned}
& \sqrt{1-b}-\sqrt{b} \geq \frac{1-2 b}{\sqrt{2}}, \quad \sqrt{1-c}-\sqrt{c} \geq \frac{1-2 c}{\sqrt{2}} \quad \text { and } \\
& \sqrt{1-d}-\sqrt{d} \geq \frac{1-2 d}{\sqrt{2}}
\end{aligned}
$$

So it follows that
$$
\begin{aligned}
& \sqrt{1-a}-\sqrt{a}+\sqrt{1-b}-\sqrt{b}+\sqrt{1-c}-\sqrt{c}+\sqrt{1-d}-\sqrt{d} \\
& \geq \frac{4-2(a+b+c+d)}{\sqrt{2}} \stackrel{(1)}{\geq} 0
\end{aligned}
$$
as required. Therefore, the answer is (B) $\geq$.

## Expected Answer
(B) $\geq$

## Enhanced Solution
Enhanced Solution:

We wish to compare the two sums

   S₁ = √(1–a) + √(1–b) + √(1–c) + √(1–d)
   S₂ = √a     + √b     + √c     + √d

and show that S₁ ≥ S₂ under the hypothesis a² + b² + c² + d² = 1 with a,b,c,d > 0.

Step 1.  Bound on a + b + c + d via the QM–AM Inequality
----------------------------------------------------------------
By the Quadratic Mean–Arithmetic Mean (QM–AM) inequality for the nonnegative numbers a,b,c,d, we have

   (a + b + c + d)/4  ≤  √[(a² + b² + c² + d²)/4].

Since a² + b² + c² + d² = 1, the right–hand side equals 1/2.  Hence

   a + b + c + d  ≤  2.                                          (1)

Step 2.  Comparison for each term √(1–x) – √x
----------------------------------------------------------------
Fix a variable x ∈ {a,b,c,d}.  Observe the difference

   √(1–x) – √x
 = [√(1–x) – √x]·[√(1–x) + √x] / [√(1–x) + √x]
 = (1 – 2x) / [√(1–x) + √x].                                    (2)

Since x ∈ (0,1) (because x² ≤ a² + b² + c² + d² = 1), the denominator √(1–x) + √x is strictly positive.  We now bound its reciprocal.

By QM–AM applied to √(1–x) and √x, we get

   [√(1–x) + √x]/2  ≤  √{ [ (√(1–x))² + (√x)² ] / 2 }
                   = √{ [ (1–x) + x ] / 2 } = 1/√2.

Thus

   √(1–x) + √x  ≤  2/√2  = √2,

or equivalently

   1 / [√(1–x) + √x]  ≥  1/√2.                              (3)

Combining (2) and (3) yields

   √(1–x) – √x  =  (1 – 2x) / [√(1–x) + √x]
                 ≥  (1 – 2x) · (1/√2)
                 = (1 – 2x)/√2.

Step 3.  Summation over a,b,c,d and conclusion
----------------------------------------------------------------
Summing the above inequality over x = a,b,c,d, we obtain

   ∑ (√(1–x) – √x)
   ≥  (1 – 2a + 1 – 2b + 1 – 2c + 1 – 2d)/√2
   = [4 – 2(a + b + c + d)] / √2.

By the bound (1), we know a + b + c + d ≤ 2, so

   4 – 2(a + b + c + d)  ≥  4 – 2·2  = 0.

Hence

   ∑ (√(1–x) – √x)  ≥  0
   ⟺ [√(1–a)+√(1–b)+√(1–c)+√(1–d)] – [√a+√b+√c+√d]  ≥  0
   ⟺ S₁ ≥ S₂.

This completes the proof without altering the original approach.  Therefore, the correct relation is

The answer is (B) ≥
