# Problem Entry

## Problem Type
relation

## Problem
Let $ABC$ be a triangle with side lengths $a, b, c$ and $\triangle A_1B_1C_1$ with side lengths $a+\frac{b}{2}, b+\frac{c}{2}, c+\frac{a}{2}$. Consider the following inequality involving the areas $P$ and $P_1$ of triangles $ABC$ and $A_1B_1C_1$ respectively:
$$
P_1 \quad () \quad \frac{9}{4} P .
$$

Determine the correct inequality relation to fill in the blank.

Options:

(A) $\leq$ 

(B) $\geq$

(C) $=$ 

(D) $<$

(E) $>$

(F) None of the above

## Current Solution
By Heron's formula for $\triangle A B C$ and $\triangle A_{1} B_{1} C_{1}$ we have
$$
16 P^{2}=(a+b+c)(a+b-c)(b+c-a)(a+c-b)
$$
and
$$
16 P_{1}^{2}=\frac{3}{16}(a+b+c)(-a+b+3 c)(-b+c+3 a)(-c+a+3 b)
$$

Since $a, b$ and $c$ are the side lengths of triangle there exist positive real numbers $p, q, r$ such that $a=q+r, b=r+p, c=p+q$.

Now we easily get that
$$
\begin{equation*}
\frac{P^{2}}{P_{1}^{2}}=\frac{16 p q r}{3(2 p+q)(2 q+r)(2 r+p)} \tag{1}
\end{equation*}
$$

So it suffices to show that
$$
(2 p+q)(2 q+r)(2 r+p) \geq 27 p q r
$$

Applying $A M \geq Q M$ we obtain
$$
\begin{align*}
(2 p+q)(2 q+r)(2 r+p) & =(p+p+q)(q+q+r)(r+r+p) \\
& \geq 3 \sqrt[3]{p^{2} q} \cdot 3 \sqrt[3]{q^{2} r} \cdot 3 \sqrt[3]{r^{2} p}=27 p q r \tag{2}
\end{align*}
$$

By (1) and (2) we get the desired result. Therefore, the answer is (B) $\geq$.

## Expected Answer
(B) $\geq$

## Enhanced Solution
We wish to compare the areas P of triangle ABC and P₁ of triangle A₁B₁C₁, where
  • sides of ABC are a,b,c;
  • sides of A₁B₁C₁ are a₁ = a + b/2,
                        b₁ = b + c/2,
                        c₁ = c + a/2.
We must decide which of the relations ≤, ≥, =, <, > holds in
  P₁   ()   (9/4) P
and show that the correct choice is “≥”.

1.  Heron’s formula for any triangle with sides x,y,z and semiperimeter s = (x+y+z)/2 states
       Area² = s·(s−x)·(s−y)·(s−z).
    (a)  For ΔABC, s = (a+b+c)/2, so
       P² = s(s−a)(s−b)(s−c)
           = [(a+b+c)/2]·[(b+c−a)/2]·[(c+a−b)/2]·[(a+b−c)/2].
    Multiply both sides by 16 to clear denominators:
       16 P² = (a+b+c)igl(b+c−aigr)igl(c+a−bigr)igl(a+b−cigr).

    (b)  For ΔA₁B₁C₁, its sides are a₁=(2a+b)/2, b₁=(2b+c)/2, c₁=(2c+a)/2.
         Its semiperimeter is
       s₁ = (a₁ + b₁ + c₁)/2
           = [ (2a+b)+(2b+c)+(2c+a) ]/(4)
           = 3(a+b+c)/4.
    Hence
       s₁ − a₁ = 3(a+b+c)/4 − (2a+b)/2
               = [3(a+b+c) − 2(2a+b)]/4
               = (−a + b +3c)/4,
    and similarly
       s₁ − b₁ = (−b + c +3a)/4,
       s₁ − c₁ = (−c + a +3b)/4.
    By Heron,
       P₁² = s₁(s₁−a₁)(s₁−b₁)(s₁−c₁)
             = [3(a+b+c)/4]·[(-a+b+3c)/4]·[(-b+c+3a)/4]·[(-c+a+3b)/4]
             = (3/256)	imes(a+b+c)(-a+b+3c)(-b+c+3a)(-c+a+3b). 
    Multiplying by 16,
       16 P₁² = (3/16)	imes(a+b+c)(-a+b+3c)(-b+c+3a)(-c+a+3b).

2.  Parametrization by positive reals p,q,r.  Since a,b,c form a triangle, set
       a = q + r,
       b = r + p,
       c = p + q.
    Then
       a+b+c = 2(p+q+r),
       b+c−a = 2p,
       c+a−b = 2q,
       a+b−c = 2r,
    and
       −a + b +3c = 2(2p+q),
       −b + c +3a = 2(2q+r),
       −c + a +3b = 2(2r+p).
    Substituting into the above formulas gives
       16 P²   = [2(p+q+r)]·(2p)·(2q)·(2r)
               = 16 pqr·(p+q+r),
       16 P₁² = (3/16)·[2(p+q+r)]·2(2p+q)·2(2q+r)·2(2r+p)
               = 3·(p+q+r)·(2p+q)·(2q+r)·(2r+p).
    Hence the ratio of squares is
       P₁² / P² = [3·(p+q+r)·(2p+q)·(2q+r)·(2r+p)] / [16·pqr·(p+q+r)]
                = 3·(2p+q)(2q+r)(2r+p) / [16·pqr].

3.  To prove P₁ ≥ (9/4) P, we square both sides and compare:
       P₁² ≥ (9/4)²·P² = (81/16)·P²
    is equivalent to
       P₁² / P² ≥ 81/16,
    i.e.
       3·(2p+q)(2q+r)(2r+p) / (16·pqr) ≥ 81/16
    ⇔ (2p+q)(2q+r)(2r+p) ≥ 27·pqr.

4.  Application of the AM–GM inequality:
    For any positive X,Y,Z we have (X+Y+Z) ≥ 3·(XYZ)^{1/3}.  Apply to
       X=p, Y=p, Z=q  ⇒  p+p+q ≥ 3·(p²q)^{1/3},
       X=q, Y=q, Z=r  ⇒  q+q+r ≥ 3·(q²r)^{1/3},
       X=r, Y=r, Z=p  ⇒  r+r+p ≥ 3·(r²p)^{1/3}.
    Multiplying these three inequalities gives
       (p+p+q)(q+q+r)(r+r+p) ≥ 3·3·3·(p²q·q²r·r²p)^{1/3}
       = 27·(p³q³r³)^{1/3} = 27·pqr.
    But the left–hand side is exactly (2p+q)(2q+r)(2r+p).  Hence
       (2p+q)(2q+r)(2r+p) ≥ 27·pqr
    as required.

Combining steps 3 and 4 shows
    P₁² ≥ (81/16)·P²,
so P₁ ≥ (9/4) P.  Therefore the correct inequality relation is “≥”.

The answer is (B) ≥
