# Problem Entry

## Problem Type
relation

## Problem
Let $x, y, z$ be non-negative real numbers. Consider the following inequality:
$$
8\left(x^{3}+y^{3}+z^{3}\right)^{2} \quad () \quad 9\left(x^{2}+y z\right)\left(y^{2}+x z\right)\left(z^{2}+x y\right) .
$$

Determine the correct inequality relation to fill in the blank.

Options:

(A) $\leq$ 

(B) $\geq$

(C) $=$ 

(D) $<$

(E) $>$

(F) None of the above

## Current Solution
If one of the numbers $x, y, z$ is zero, let us say $z=0$, then the above inequality is equivalent to
$$
8\left(x^{3}+y^{3}\right)^{2} \geq 9 x^{3} y^{3} \quad \text { or } \quad 8\left(x^{6}+y^{6}\right)+7 x^{3} y^{3} \geq 0
$$
which clearly holds.
Equality occurs iff $x=y=0$.
So let us assume that $x, y, z>0$.
Then
$$
x^{2}+y z \leq x^{2}+\frac{y^{2}+z^{2}}{2}=\frac{2 x^{2}+y^{2}+z^{2}}{2}
$$

Similarly
$$
y^{2}+x z \leq \frac{2 y^{2}+x^{2}+z^{2}}{2} \quad \text { and } \quad z^{2}+x y \leq \frac{2 z^{2}+x^{2}+y^{2}}{2}
$$

Hence
$$
\begin{align*}
& 9\left(x^{2}+y z\right)\left(y^{2}+x z\right)\left(z^{2}+x y\right) \\
& \quad \leq \frac{9}{8}\left(2 x^{2}+y^{2}+z^{2}\right)\left(2 y^{2}+x^{2}+z^{2}\right)\left(2 z^{2}+x^{2}+y^{2}\right) \\
& \quad \leq \frac{9}{8}\left(\frac{\left(2 x^{2}+y^{2}+z^{2}\right)+\left(2 y^{2}+x^{2}+z^{2}\right)+\left(2 z^{2}+x^{2}+y^{2}\right)}{3}\right)^{3} \\
& \quad=\frac{9}{8}\left(\frac{4\left(x^{2}+y^{2}+z^{2}\right)}{3}\right)^{3}=\frac{9 \cdot 4^{3}}{8}\left(\frac{x^{2}+y^{2}+z^{2}}{3}\right)^{3} \tag{1}
\end{align*}
$$

By the power mean inequality we have
$$
\sqrt{\frac{x^{2}+y^{2}+z^{2}}{3}} \leq \sqrt[3]{\frac{x^{3}+y^{3}+z^{3}}{3}}
$$
i.e.
$$
\begin{equation*}
\left(\frac{x^{2}+y^{2}+z^{2}}{3}\right)^{3} \leq\left(\frac{x^{3}+y^{3}+z^{3}}{3}\right)^{2} \tag{2}
\end{equation*}
$$

Finally, by (1) and (2) it follows that
$$
\begin{aligned}
9\left(x^{2}+y z\right)\left(y^{2}+x z\right)\left(z^{2}+x y\right) & \leq \frac{9 \cdot 4^{3}}{8}\left(\frac{x^{2}+y^{2}+z^{2}}{3}\right)^{3} \\
& \leq \frac{9 \cdot 4^{3}}{8}\left(\frac{x^{3}+y^{3}+z^{3}}{3}\right)^{2}=8\left(x^{3}+y^{3}+z^{3}\right)^{2}
\end{aligned}
$$ Therefore, the answer is (B) $\geq$.

## Expected Answer
(B) $\geq$

## Enhanced Solution
We wish to compare the two expressions
  8\,(x^3 + y^3 + z^3)^2
and
  9\,(x^2 + y z)\,(y^2 + x z)\,(z^2 + x y)
for non-negative real x, y, z and determine the correct relation between them.

1.  Case when at least one of x,y,z is zero.  
    Without loss of generality assume z = 0.  Then the second expression becomes
      9\,(x^2 + 0)\,(y^2 + 0)\,(0^2 + x y)
      = 9\,x^2\,y^2\,(x y)
      = 9\,x^3\,y^3.
    The first expression becomes
      8\,(x^3 + y^3)^2
      = 8\,(x^6 + 2x^3y^3 + y^6)
      = 8\,x^6 + 16\,x^3y^3 + 8\,y^6.
    Thus the inequality 8(x^3 + y^3)^2 ? 9 x^3 y^3 is equivalent to
      8 x^6 + 16 x^3 y^3 + 8 y^6 ? 9 x^3 y^3
    or
      8 x^6 + 7 x^3 y^3 + 8 y^6 ? 0,
    which is obviously true in the “≥” sense (all terms are nonnegative).  
    Hence in this case
      8(x^3 + y^3 + z^3)^2 ≥ 9(x^2 + y z)(y^2 + x z)(z^2 + x y).  
    Equality holds here only when x = y = 0 (so that both sides vanish).

2.  Case when x,y,z > 0.  We proceed by three steps of classical inequalities.

    (i)  Bound each factor x^2 + y z by AM–GM on y^2 and z^2:  
         y z ≤ (y^2 + z^2)/2  ⇒  x^2 + y z ≤ x^2 + (y^2+z^2)/2  = (2 x^2 + y^2 + z^2)/2.
         Similarly,
           y^2 + x z ≤ (2 y^2 + x^2 + z^2)/2,
           z^2 + x y ≤ (2 z^2 + x^2 + y^2)/2.
    Multiplying these three gives
      (x^2+yz)(y^2+xz)(z^2+xy)
      ≤ [ (2 x^2 + y^2 + z^2)/2 ]·[ (2 y^2 + x^2 + z^2)/2 ]·[ (2 z^2 + x^2 + y^2)/2 ]
      = (1/8)·(2 x^2 + y^2 + z^2)(2 y^2 + x^2 + z^2)(2 z^2 + x^2 + y^2).
    Hence
      9(x^2+yz)(y^2+xz)(z^2+xy)
      ≤ (9/8)·(2 x^2 + y^2 + z^2)(2 y^2 + x^2 + z^2)(2 z^2 + x^2 + y^2).

    (ii)  Apply AM–GM to the three sums (2x^2+y^2+z^2), (2y^2+x^2+z^2), (2z^2+x^2+y^2):
      (2 x^2 + y^2 + z^2)(2 y^2 + x^2 + z^2)(2 z^2 + x^2 + y^2)
      ≤ [ ( (2 x^2 + y^2 + z^2) + (2 y^2 + x^2 + z^2) + (2 z^2 + x^2 + y^2) ) / 3 ]^3.
    Observe the sum inside is
      (2x^2+y^2+z^2) + (2y^2+x^2+z^2) + (2z^2+x^2+y^2)
      = 4(x^2 + y^2 + z^2).
    Therefore
      (2 x^2 + y^2 + z^2)(2 y^2 + x^2 + z^2)(2 z^2 + x^2 + y^2)
      ≤ [4(x^2+y^2+z^2)/3]^3
      = (4^3/3^3)·(x^2+y^2+z^2)^3
      = (64/27)·(x^2+y^2+z^2)^3.
    Substituting back,
      9(x^2+yz)(y^2+xz)(z^2+xy)
      ≤ (9/8)·(64/27)·(x^2+y^2+z^2)^3
      = 8·(x^2+y^2+z^2)^3.

    (iii)  Finally use the power-mean (or Holder) inequality relating squares and cubes:
      [ (x^2+y^2+z^2)/3 ]^(1/2) ≤ [ (x^3+y^3+z^3)/3 ]^(1/3).
    Raising both sides to the sixth power gives
      [ (x^2+y^2+z^2)/3 ]^3 ≤ [ (x^3+y^3+z^3)/3 ]^2.
    Hence
      (x^2+y^2+z^2)^3 ≤ 3^3 · [ (x^3+y^3+z^3)/3 ]^2 = 27·[ (x^3+y^3+z^3)/3 ]^2
      = (1/3)·(x^3+y^3+z^3)^2.
    Combining this with the result of step (ii), we obtain
      9(x^2+yz)(y^2+xz)(z^2+xy)
      ≤ 8·(x^2+y^2+z^2)^3
      ≤ 8·[(x^3+y^3+z^3)^2/3]
      = 8·(x^3+y^3+z^3)^2.

3.  Conclusion and equality conditions.  
    In both cases we have shown
      8\,(x^3 + y^3 + z^3)^2 ≥ 9\,(x^2 + y z)\,(y^2 + x z)\,(z^2 + x y).
    Thus the correct relation is “≥.”  
    Equality occurs precisely when
      •  In case one variable is zero: x = y = z = 0,  
      •  In case all are positive: x = y = z (so that every application of AM–GM or power-mean becomes an equality).  

The answer is (B) ≥
