# Problem Entry

## Problem Type
bound

## Problem
Let $x, y, z \in \mathbb{R}^{+}$ such that $x + y + z = 1$. Determine the minimal constant $C$ such that the following inequality holds for all $x, y, z$:
$$
\frac{1}{1-x y}+\frac{1}{1-y z}+\frac{1}{1-z x} \leq C.
$$

## Current Solution
Let $p=x+y+z=1, q=x y+y z+z x, r=x y z$.
It can easily be shown that
$$
(1-x y)(1-y z)(1-z x)=1-q+p r-r^{2}
$$
and
$$
(1-x y)(1-y z)+(1-y z)(1-z x)+(1-z x)(1-x y)=3-2 q+p r
$$

So the given inequality becomes
$$
\begin{gathered}
8(3-2 q+p r) \leq 27\left(1-q+p r-r^{2}\right) \\
\Leftrightarrow \quad 3-11 q+19 p r-27 r^{2} \geq 0
\end{gathered}
$$

Since $p=1$, we need to show that
$$
3-11 q+19 r-27 r^{2} \geq 0
$$

By $N_{5}: p^{3} \geq 27 r$ we have $1 \geq 27 r$, i.e. $r \geq 27 r^{2}$.

Therefore
$$
3-11 q+19 r-27 r^{2} \geq 3-11 q+19 r-r=3-11 q+18 r
$$

So it suffices to prove that
$$
3-11 q+18 r \geq 0
$$

We have
$$
\begin{aligned}
& 3-11 q+18 r \geq 0 \\
& \quad \Leftrightarrow \quad 3-11(x y+y z+z x)+18 x y z \geq 0 \\
& \quad \Leftrightarrow \quad 11(x y+y z+z x)-18 x y z \leq 3
\end{aligned}
$$

Applying $A M \geq G M$ we deduce
$$
\begin{aligned}
11(x y+y z+z x)-18 x y z & =x y(11-18 z)+11 z(x+y) \\
& \leq \frac{(x+y)^{2}}{4}(11-18 z)+11 z(x+y) \\
& =(1-z)^{2}/4(11-18 z)+11 z(1-z) \\
& =\frac{(1-z)((1-z)(11-18 z)+44 z)}{4} \\
& =\frac{4 z+3 z^{2}-18 z^{3}+11}{4}
\end{aligned}
$$

So it remains to show that
$$
\begin{aligned}
& \frac{4 z+3 z^{2}-18 z^{3}+11}{4} \leq 3 \\
& \quad \Leftrightarrow \quad 4 z+3 z^{2}-18 z^{3} \leq 1 \\
& \Leftrightarrow \quad 18 z^{3}-3 z^{2}-4 z+1 \geq 0 \\
& \Leftrightarrow \quad(3 z-1)^{2}(2 z+1) \geq 0
\end{aligned}
$$
which is obvious.

Equality holds when $x = y = z = \frac{1}{3}$, since then $x + y + z = 1$ and $x y = y z = z x = \frac{1}{9}$, so $\frac{1}{1-x y} = \frac{1}{1-1/9} = \frac{9}{8}$, and the sum is $3 \times \frac{9}{8} = \frac{27}{8}$. This gives the maximum value of the sum, so $C = \frac{27}{8}$ is the minimal constant such that the inequality always holds.

Therefore, the answer is $C = \frac{27}{8}$.

## Expected Answer
$C = \frac{27}{8}$

## Enhanced Solution
Enhanced Solution:

1. Notation and Symmetric Sums
   Let x,y,z be positive real numbers satisfying x+y+z=1.  Define the elementary symmetric sums
     p = x+y+z = 1,
     q = xy + yz + zx,
     r = xyz.

2. Rewriting the Factors
   Observe that each factor in the denominators can be written in terms of q and r as follows:
     (1 - x y)(1 - y z)(1 - z x)
     = 1 - (xy + yz + zx) + (x+y+z)·xyz - (xyz)^2
     = 1 - q + p·r - r^2
     = 1 - q + r - r^2,  since p = 1.

   Similarly, the sum of the pairwise products of these factors is
     (1 - xy)(1 - yz) + (1 - yz)(1 - zx) + (1 - zx)(1 - xy)
     = 3 - 2q + p·r
     = 3 - 2q + r.

3. Converting the Inequality to a Polynomial Form
   The given inequality
     1/(1 - xy) + 1/(1 - yz) + 1/(1 - zx) ≤ C
   is equivalent—upon multiplying both sides by the positive quantity (1-xy)(1-yz)(1-zx)—to
     (1 - yz)(1 - zx) + (1 - zx)(1 - xy) + (1 - xy)(1 - yz)
     ≤ C · (1 - xy)(1 - yz)(1 - zx).

   Substituting the expressions from step 2, this becomes
     3 - 2q + r  ≤  C · (1 - q + r - r^2).

4. Determining the Best Constant C
   We test C = 27/8.  Multiply both sides by 8 to clear denominators:
     8(3 - 2q + r)  ≤  27(1 - q + r - r^2)
   ⇔ 24 - 16q + 8r  ≤  27 - 27q + 27r - 27r^2
   ⇔  3  - 11q + 19r - 27r^2  ≥  0.

5. Reducing the Inequality via an AM–GM Bound on r
   From the arithmetic–geometric mean inequality applied to x,y,z,
     (x+y+z)/3 ≥ (xyz)^{1/3}  ⇒  1/3 ≥ r^{1/3}  ⇒  r ≤ 1/27.
   Multiply both sides by r to get
     27 r^2 ≤ r  ⇒  -27r^2 ≥ -r  ⇒  19r - 27r^2 ≥ 18r.
   Hence
     3 - 11q + 19r - 27r^2  ≥  3 - 11q + 18r.
   It suffices to show
     3 - 11q + 18r  ≥  0.

6. Expressing in x,y,z and Applying AM–GM Again
   Write q = xy+yz+zx and r = xyz.  Then
     3 - 11q + 18r  ≥  0
   ⇔ 3 - 11(xy+yz+zx) + 18xyz  ≥  0
   ⇔ 11(xy+yz+zx) - 18xyz  ≤ 3.

   Group terms symmetrically in x,y, treating z as a parameter:
     11(xy+yz+zx) - 18xyz
     = xy·(11 - 18z)  +  11z·(x+y).
   Since x+y = 1 - z and by AM–GM on x,y,
     xy ≤ ((x+y)^2)/4 = (1 - z)^2/4,
   we obtain
     xy·(11 - 18z)  ≤  (1 - z)^2/4 · (11 - 18z),
     11z·(x+y)     = 11z(1 - z).
   Summing yields
     11(xy+yz+zx) - 18xyz
     ≤ [ (1 - z)^2 (11 - 18z) + 44z(1 - z ) ] / 4
     = [ 11 + 4z + 3z^2 - 18z^3 ] / 4.

   Thus it remains to prove
     [11 + 4z + 3z^2 - 18z^3]/4  ≤  3
   ⇔ 11 + 4z + 3z^2 - 18z^3  ≤ 12
   ⇔ 18z^3 - 3z^2 - 4z + 1  ≥ 0.

7. Factoring the Final Cubic
   A direct factorization shows
     18z^3 - 3z^2 - 4z + 1 = (3z - 1)^2 (2z + 1).
   Since z > 0, the factor (2z+1) is positive, and (3z - 1)^2 ≥ 0 for all z.  Hence the inequality is valid.

8. Equality Case and Conclusion
   Equality throughout occurs exactly when x = y = z = 1/3.  In that case each term is
     1/(1 - xy) = 1/(1 - 1/9) = 9/8,
   so the sum is 3·(9/8) = 27/8.  Therefore C = 27/8 is the minimal constant for which the original inequality holds.

The answer is $C=\frac{27}{8}$
