# Problem Entry

## Problem Type
bound

## Problem
Let $a, b \in \mathbb{R}^{+}$ and $n \in \mathbb{N}$. Find the smallest constant $C$ such that the following inequality holds for all $a, b \in \mathbb{R}^{+}$ and $n \in \mathbb{N}$:
$$
(a+b)^{n}\left(a^{n}+b^{n}\right) \leq C\left(a^{2 n}+b^{2 n}\right)
$$

## Current Solution
By the power mean inequality, for any $x, y \in \mathbb{R}^{+}, n \in \mathbb{N}$, we have
$$
\left(\frac{x+y}{2}\right)^{n} \leq \frac{x^{n}+y^{n}}{2}
$$

Therefore
$$
\begin{aligned}
(a+b)^{n}\left(a^{n}+b^{n}\right) & =2^{n}\left(\frac{a+b}{2}\right)^{n}\left(a^{n}+b^{n}\right) \\
& \leq 2^{n}\left(\frac{a^{n}+b^{n}}{2}\right)\left(a^{n}+b^{n}\right)=2^{n} \frac{\left(a^{n}+b^{n}\right)^{2}}{2} \\
& \leq 2^{n} \frac{2\left(a^{2 n}+b^{2 n}\right)}{2}=2^{n}\left(a^{2 n}+b^{2 n}\right)
\end{aligned}
$$

Equality holds when $a = b$, since all the inequalities above become equalities in this case. This gives the minimum value of $C$, so $C = 2^n$ is the smallest constant for which the inequality always holds.

Therefore, the answer is $C = 2^n$.

## Expected Answer
$C = 2^n$

## Enhanced Solution
Enhanced Solution:

We wish to find the smallest constant C such that for all positive real numbers a, b and every natural number n,

    (a + b)^{n}\,(a^{n} + b^{n}) \;\le\; C\,(a^{2n} + b^{2n}).

We proceed in two main steps, each employing a classical inequality, and we then check that equality forces a = b, which identifies the smallest possible C.

Step 1: Apply the Power–Mean (Jensen) inequality to (a + b)^{n}.
---------------------------------------------------------------------------------

Since the function f(x) = x^{n} is convex on (0,\infty) for every natural n, Jensen’s inequality for two points a and b (or equivalently the special case of the Power–Mean inequality) gives:

    f\bigl(\tfrac{a + b}{2}\bigr) \;\le\; \tfrac{f(a) + f(b)}{2},

that is,

    \bigl(\tfrac{a + b}{2}\bigr)^{n} \;\le\; \tfrac{a^{n} + b^{n}}{2}.

Multiplying both sides by 2^{n} yields:

    (a + b)^{n} \;=
    2^{n}\,\bigl(\tfrac{a + b}{2}\bigr)^{n}
    \;\le\; 2^{n}\,\tfrac{a^{n} + b^{n}}{2}
    \;=
    2^{n-1}\,(a^{n} + b^{n}).

Hence we have established

    (a + b)^{n}\,(a^{n} + b^{n})
    \;\le\;
    2^{n-1}\,(a^{n} + b^{n})^{2}.

Step 2: Bound (a^{n} + b^{n})^{2} in terms of a^{2n} + b^{2n}.
---------------------------------------------------------------------------------

We now use the elementary fact that for any real x, y,

    (x - y)^{2} \;\ge\; 0
    \quad\Longrightarrow\quad
    x^{2} + y^{2} \;\ge\; 2xy.

Set x = a^{n} and y = b^{n}.  Then

    (a^{n} + b^{n})^{2}
    = a^{2n} + 2a^{n}b^{n} + b^{2n}
    \le a^{2n} + b^{2n} + a^{2n} + b^{2n}
    = 2\,(a^{2n} + b^{2n}).

Substituting this estimate into the result of Step 1 gives

    (a + b)^{n}\,(a^{n} + b^{n})
    \;\le\;
    2^{n-1}\,(a^{n} + b^{n})^{2}
    \;\le\;
    2^{n-1}\,2\,(a^{2n} + b^{2n})
    = 2^{n}\,(a^{2n} + b^{2n}).

Conclusion and Sharpness:
---------------------------------------------------------------------------------

We have shown that for every a, b > 0 and n \in \mathbb{N},

    (a + b)^{n}\,(a^{n} + b^{n})
    \;\le\;
    2^{n}\,(a^{2n} + b^{2n}).

Thus one can take C = 2^{n}.

To see that this is the smallest possible constant, observe that equality in both employed inequalities occurs exactly when a = b:

 1.  In the power–mean step, equality holds if and only if a = b.
 2.  In the inequality (a^{n} + b^{n})^{2} \le 2(a^{2n} + b^{2n}),
      equality also requires a^{n} = b^{n}, i.e. a = b.

Hence when a = b the chain of inequalities becomes an equality, proving no smaller C can work for all positive a, b.

Therefore, the answer is $C = 2^n$.
