# Problem Entry

## Problem Type
bound

## Problem
Let $a, b, c \in (0,1)$ be real numbers. Find the smallest constant $C$ such that the following inequality holds for all $a, b, c \in (0,1)$:
$$
\sqrt{abc} + \sqrt{(1-a)(1-b)(1-c)} < C
$$

## Current Solution
For $x \in(0,1)$ we have $\sqrt{x}<\sqrt[3]{x}$.
So
$$
\begin{equation*}
\sqrt{a b c}<\sqrt[3]{a b c} \quad \text { and } \quad \sqrt{(1-a)(1-b)(1-c)}<\sqrt[3]{(1-a)(1-b)(1-c)} \tag{1}
\end{equation*}
$$

Using (1) and $A M \geq G M$ gives us
$$
\begin{aligned}
\sqrt{a b c}+\sqrt{(1-a)(1-b)(1-c)} & <\sqrt[3]{a b c}+\sqrt[3]{(1-a)(1-b)(1-c)} \\
& \leq \frac{a+b+c}{3}+\frac{1-a+1-b+1-c}{3}=1
\end{aligned}
$$

Equality in the above inequalities is never achieved for $a, b, c \in (0,1)$, since $\sqrt{x} < \sqrt[3]{x}$ strictly for $x \in (0,1)$. Thus, the sum is always strictly less than $1$, and $C = 1$ is the smallest constant for which the inequality always holds.

Therefore, the answer is $C = 1$. 

## Expected Answer
$C = 1$

## Enhanced Solution
**Solution Explanation**

We wish to show that for all real numbers a,b,c in the open interval (0,1), the quantity

    S = \sqrt{a b c} \;+
        \sqrt{(1-a)(1-b)(1-c)}

is strictly bounded above by 1, and hence the smallest constant C for which

    S < C

holds is C=1.

**Step 1: Comparing the square root and the cube root on (0,1)**

Claim: For every x in (0,1),

    \sqrt{x} < x^{1/3}.

Proof of claim: Since 0<x<1, raising x to a smaller positive exponent yields a larger value.  Equivalently, consider the function

    f(x) = x^{1/3} - x^{1/2}.

On the interval (0,1), we have x^{1/3}>x^{1/2} because exponentiation by 1/3 is a milder compression than exponentiation by 1/2.  More concretely, one can write

    x^{1/3} = x^{1/2} \cdot x^{-1/6} = \sqrt{x}\,x^{-1/6},

and since x^{-1/6}>1 when 0<x<1, it follows that x^{1/3}>\sqrt{x}.  This establishes the strict inequality.

Applying this to each factor, we obtain

    (i)   \sqrt{a b c} < (a b c)^{1/3},
    (ii)  \sqrt{(1-a)(1-b)(1-c)} < [(1-a)(1-b)(1-c)]^{1/3}.

Hence

    S = \sqrt{a b c} + \sqrt{(1-a)(1-b)(1-c)}
      < (a b c)^{1/3} + [(1-a)(1-b)(1-c)]^{1/3}.

**Step 2: Applying the AM–GM inequality**

Recall the Arithmetic Mean–Geometric Mean (AM–GM) inequality for three nonnegative numbers p,q,r:

    \frac{p+q+r}{3} \ge (p q r)^{1/3},

with equality if and only if p=q=r.  We apply this in two cases:

  •  Take p=a, q=b, r=c.  Then

       (a b c)^{1/3} \le \frac{a+b+c}{3}.

  •  Take p=1-a, q=1-b, r=1-c.  Then

       [(1-a)(1-b)(1-c)]^{1/3} \le \frac{(1-a)+(1-b)+(1-c)}{3}.

Adding these two inequalities gives

    (a b c)^{1/3} + [(1-a)(1-b)(1-c)]^{1/3}
       \le \frac{a+b+c}{3} + \frac{(1-a)+(1-b)+(1-c)}{3}
       = \frac{(a+b+c) + (3 - (a+b+c))}{3}
       = 1.

Combining with the strict inequalities from Step 1, we deduce

    S < (a b c)^{1/3} + [(1-a)(1-b)(1-c)]^{1/3} \le 1,

and therefore

    S < 1

for every choice of a,b,c in (0,1).

**Step 3: Verifying that the bound is the best possible**

We have shown S is strictly less than 1, but never attains 1 for any (a,b,c) in the open cube (0,1)^3.  Indeed:

  •  The inequality \sqrt{x}<x^{1/3} is strict for every x in (0,1).

  •  Even though AM–GM becomes equality when a=b=c and 1-a=1-b=1-c (forcing a=b=c=1/2), the first step remains strict at a=b=c=1/2 because \sqrt{1/2}< (1/2)^{1/3}.

Hence 1 is the least upper bound of S but is never reached.  Consequently, the smallest constant C satisfying

    \sqrt{a b c} + \sqrt{(1-a)(1-b)(1-c)} < C

for all a,b,c in (0,1) is

The answer is $C=1$
