# Problem Entry

## Problem Type
bound

## Problem
Let $a, b, c \in \mathbb{R}^{+}$ such that $a+b+c=3$. Find the largest constant $C$ such that the following inequality holds for all $a, b, c$ satisfying the given constraint:
$$
\sqrt{a(b+c)}+\sqrt{b(c+a)}+\sqrt{c(a+b)} \geq 3 \sqrt{C a b c}
$$

## Current Solution
We have
$$
\sqrt{a b+a c} \geq \frac{\sqrt{2}}{2}(\sqrt{a b}+\sqrt{a c})
$$

Analogously
$$
\sqrt{b c+b a} \geq \frac{\sqrt{2}}{2}(\sqrt{b c}+\sqrt{b a}) \quad \text { and } \quad \sqrt{c a+c b} \geq \frac{\sqrt{2}}{2}(\sqrt{c a}+\sqrt{c b})
$$

So it suffices to show that
$$
\sqrt{2}(\sqrt{a b}+\sqrt{a c}+\sqrt{b c}) \geq 3 \sqrt{2 a b c}
$$
i.e.
$$
\begin{equation*}
\sqrt{a b}+\sqrt{a c}+\sqrt{b c} \geq 3 \sqrt{a b c} \tag{1}
\end{equation*}
$$

By $A M \geq G M$ we have
$$
\sqrt{a b}+\sqrt{a c}+\sqrt{b c} \geq 3 \sqrt[3]{a b c} \geq 3 \sqrt{a b c}
$$
where the last inequality is true since
$$
\sqrt[3]{a b c} \leq \frac{a+b+c}{3}=1, \quad \text { i.e. } \quad a b c \leq 1
$$

Equality holds when $a = b = c = 1$, in which case $a + b + c = 3$ and $a b c = 1$. The inequality becomes $\sqrt{2}(\sqrt{1} + \sqrt{1} + \sqrt{1}) = 3\sqrt{2}$ on the left and $3\sqrt{2 \cdot 1} = 3\sqrt{2}$ on the right, so equality is achieved. This gives the maximum value of $C$ for which the inequality always holds, which is $C = 2$.

Therefore, the answer is $C = 2$.

## Expected Answer
$C = 2$

## Enhanced Solution
We wish to determine the largest constant C for which

  √[a(b+c)]  +  √[b(c+a)]  +  √[c(a+b)]  ≥  3 √[C a b c]

holds for all positive a,b,c with a+b+c=3.  The original solution uses a two-step approach: first, a pairwise estimate via Cauchy–Schwarz (or an elementary quadratic expansion), and second, an application of the arithmetic mean–geometric mean inequality together with the constraint a+b+c=3.  We now present a more detailed justification of each step, while preserving the same overall strategy.

**Step 1.  Pairwise estimate.**

For any two nonnegative real numbers x,y we have by the Cauchy–Schwarz inequality:

  (√x + √y)²  =  x + y + 2√{xy}  ≤  2(x + y).

Taking square-roots gives

  √x + √y  ≤  √[2(x + y)]  =  √2 · √(x + y).

Equivalently,

  √(x + y)  ≥  (√2 / 2) · (√x + √y).

Setting x = a b and y = a c yields

  √[a b + a c]  ≥  (√2 / 2) · (√{a b} + √{a c}).

By symmetry, the same estimate holds for the other two terms:

  √[b c + b a]  ≥  (√2 / 2) · (√{b c} + √{b a}),

  √[c a + c b]  ≥  (√2 / 2) · (√{c a} + √{c b}).

Adding these three inequalities, the left-hand side becomes

  √{a(b+c)} + √{b(c+a)} + √{c(a+b)},

while the right-hand side becomes

  (√2 / 2) · [ (√{a b}+√{a c}) + (√{b c}+√{b a}) + (√{c a}+√{c b}) ]

= √2 · (√{a b} + √{a c} + √{b c}).

Hence we have reduced the original inequality to showing

  √2 · (√{a b} + √{a c} + √{b c})  ≥  3 √[C a b c].

Equivalently,

  √{a b} + √{a c} + √{b c}  ≥  (3/√2) √[C a b c].    (⋆)

**Step 2.  Applying AM–GM under the constraint a+b+c=3.**

First, by the standard AM–GM inequality for three nonnegative terms:

  √{a b} + √{a c} + √{b c}  ≥  3 · ( √{a b} · √{a c} · √{b c} )^{1/3}
                                               =  3 · ( a b c )^{1/3}.

Thus the left side of (⋆) is at least 3·(a b c)^{1/3}.  It remains to ensure

  3 · (a b c)^{1/3}  ≥  (3/√2) · √[C a b c],

or, after dividing both sides by 3·√[a b c] > 0,

  (a b c)^{-1/6}  ≥  1/√2 · √C.

Since 0 < a b c ≤ 1 (because a+b+c=3 and AM–GM gives a b c ≤ 1), we have (a b c)^{-1/6} ≥ 1.  Therefore the strongest possible choice of C that makes

  (a b c)^{-1/6}  ≥  √C / √2

hold for all admissible a,b,c is C=2, because then √C/√2 = 1.  Any larger C would require (a b c)^{-1/6} ≥ something greater than 1, which fails when a=b=c=1.

**Step 3.  Verification of equality cases.**

All intermediate inequalities become equalities precisely when a=b=c.  Indeed:

 • In the Cauchy–Schwarz step √x + √y ≤ √2·√(x+y), equality requires x=y, i.e. a b = a c, etc., forcing b=c, and similarly c=a.  

 • In the AM–GM step √{a b}+√{a c}+√{b c} ≥ 3(a b c)^{1/3}, equality requires √{a b}=√{a c}=√{b c}, again giving a=b=c.  

Under the constraint a+b+c=3, that common value must be 1, so abc=1.  Substituting a=b=c=1 into the original inequality yields equality when C=2.

Hence the largest constant for which the given inequality holds for all positive a,b,c with a+b+c=3 is

The answer is $C=2$
