# Problem Entry

## Problem Type
bound

## Problem
Let $a, b, c$ be positive real numbers such that $a b c \geq 1$. Find the smallest constant $C$ such that the following inequality holds for all $a, b, c$ satisfying the given constraint:
$$
\frac{1}{a^{4}+b^{3}+c^{2}}+\frac{1}{b^{4}+c^{3}+a^{2}}+\frac{1}{c^{4}+a^{3}+b^{2}} \leq C
$$

## Current Solution
By the Cauchy-Schwarz inequality we have
$$
\frac{1}{a^{4}+b^{3}+c^{2}}=\frac{1+b+c^{2}}{\left(a^{4}+b^{3}+c^{2}\right)\left(1+b+c^{2}\right)} \leq \frac{1+b+c^{2}}{\left(a^{2}+b^{2}+c^{2}\right)^{2}}
$$

Similarly we get
$$
\frac{1}{b^{4}+c^{3}+a^{2}} \leq \frac{1+c+a^{2}}{\left(a^{2}+b^{2}+c^{2}\right)^{2}} \quad \text { and } \quad \frac{1}{c^{4}+a^{3}+b^{2}} \leq \frac{1+a+b^{2}}{\left(a^{2}+b^{2}+c^{2}\right)^{2}}
$$

It follows that
$$
\frac{1}{a^{4}+b^{3}+c^{2}}+\frac{1}{b^{4}+c^{3}+a^{2}}+\frac{1}{c^{4}+a^{3}+b^{2}} \leq \frac{a^{2}+b^{2}+c^{2}+a+b+c+3}{\left(a^{2}+b^{2}+c^{2}\right)^{2}}
$$

So it remains to prove that
$$
\frac{a^{2}+b^{2}+c^{2}+a+b+c+3}{\left(a^{2}+b^{2}+c^{2}\right)^{2}} \leq 1
$$

By $A M \geq G M$ we have $a+b+c \geq 3$ and $a^{2}+b^{2}+c^{2} \geq 3$.
Consider the well-known inequality $3\left(a^{2}+b^{2}+c^{2}\right) \geq(a+b+c)^{2}$.
Then we obtain
$$
\begin{aligned}
\frac{a^{2}+b^{2}+c^{2}+a+b+c+3}{\left(a^{2}+b^{2}+c^{2}\right)^{2}} & \leq \frac{a^{2}+b^{2}+c^{2}+\frac{(a+b+c)^{2}}{3}+\frac{(a+b+c)^{2}}{3}}{\left(a^{2}+b^{2}+c^{2}\right)^{2}} \\
& \leq \frac{a^{2}+b^{2}+c^{2}+\left(a^{2}+b^{2}+c^{2}\right)+\left(a^{2}+b^{2}+c^{2}\right)}{\left(a^{2}+b^{2}+c^{2}\right)^{2}} \\
& =\frac{3}{a^{2}+b^{2}+c^{2}} \leq 1
\end{aligned}
$$
as required.

Equality holds when $a = b = c = 1$, since then $a^2 + b^2 + c^2 = 3$, $a + b + c = 3$, and $a b c = 1$. In this case, each term becomes $\frac{1}{1^4 + 1^3 + 1^2} = \frac{1}{1 + 1 + 1} = \frac{1}{3}$, so the sum is $1$. Thus, the maximum value of the sum is $1$, and $C = 1$ is the smallest constant for which the inequality always holds.

Therefore, the answer is $C = 1$.

## Expected Answer
$C = 1$

## Enhanced Solution
Enhanced Solution:

We wish to prove that for all positive real numbers a,b,c satisfying abc ≥ 1, the following holds:

  (1)   1/(a^4 + b^3 + c^2)  +  1/(b^4 + c^3 + a^2)  +  1/(c^4 + a^3 + b^2)  ≤  C,

and to determine the smallest possible constant C.  We will show that C = 1.

Step 1.  A Cauchy–Schwarz lower bound on each denominator.

Fix the cyclic term 1/(a^4 + b^3 + c^2).  Observe that by the Cauchy–Schwarz inequality in the form

  (x_1^2 + x_2^2 + x_3^2)igl(y_1^2 + y_2^2 + y_3^2igr) ≥ (x_1 y_1 + x_2 y_2 + x_3 y_3)^2,

we may choose the vectors
  x = (a^2, b^{3/2}, c),
  y = (1, b^{1/2}, c),
so that
  x_1^2 + x_2^2 + x_3^2 = a^4 + b^3 + c^2,
  y_1^2 + y_2^2 + y_3^2 = 1 + b + c^2,
  x_1 y_1 + x_2 y_2 + x_3 y_3 = a^2·1 + b^{3/2}·b^{1/2} + c·c = a^2 + b^2 + c^2.

Hence
  (a^4 + b^3 + c^2)igl(1 + b + c^2igr)  ≥  (a^2 + b^2 + c^2)^2,

which rearranges to

  1/(a^4 + b^3 + c^2)  ≤  (1 + b + c^2) / (a^2 + b^2 + c^2)^2.

By applying the same argument cyclically, we obtain

  1/(b^4 + c^3 + a^2)  ≤  (1 + c + a^2) / (a^2 + b^2 + c^2)^2,
  1/(c^4 + a^3 + b^2)  ≤  (1 + a + b^2) / (a^2 + b^2 + c^2)^2.

Step 2.  Summing the three cyclic inequalities.

Denote S = a^2 + b^2 + c^2.  Summing gives

  LHS of (1)
  ≤ [ (1 + b + c^2) + (1 + c + a^2) + (1 + a + b^2 ) ] / S^2
  = [ (a^2 + b^2 + c^2) + (a + b + c) + 3 ] / S^2
  = [ S + (a + b + c) + 3 ] / S^2.

Therefore it suffices to show

  (2)   [ S + (a + b + c) + 3 ] / S^2  ≤  1,

for all a,b,c > 0 with abc ≥ 1.

Step 3.  Lower bounds via AM–GM.

By the arithmetic mean–geometric mean inequality on the three numbers a^2,b^2,c^2, we have

  (a^2 + b^2 + c^2)/3  ≥  (a^2 b^2 c^2)^{1/3}  =  (abc)^{2/3}  ≥  1^{2/3}  = 1.

Hence S = a^2 + b^2 + c^2  ≥ 3.

Similarly, applying AM–GM to a,b,c yields

  (a + b + c)/3  ≥  (abc)^{1/3}  ≥  1,  

so

  a + b + c  ≥ 3.

Step 4.  Verifying inequality (2).

Set X = a + b + c.  We have X ≥ 3.  We now bound the numerator N = S + X + 3 in terms of S alone.

First, from Step 3 we know S ≥ 3.  Also the well-known inequality

  3S  ≥  (a + b + c)^2  =  X^2

implies

  X^2 / 3  ≤  S.

Since X ≥ 3, the quadratic function f(X) = 2X^2/3  –  X – 3 satisfies

  f(3) = 2·9/3 – 3 – 3 = 6 – 6 = 0,

and f is increasing for X ≥ 3.  Hence for all X ≥ 3,

  2X^2/3  ≥  X + 3.

Therefore

  N = S + X + 3  ≤  S + (2X^2/3)
                     ≤  S + 2S    (since X^2/3 ≤ S)
                     =  3S.

Combining this with the bound on the sum in Step 2 gives

  LHS of (1)  ≤  N / S^2  ≤  3S / S^2  =  3 / S  ≤  3 / 3  = 1,

where in the last inequality we used S ≥ 3.  This completes the proof of the desired inequality with C = 1.

Step 5.  Attaining equality.

All inequalities above become equalities precisely when a=b=c=1.  Indeed,

  •  abc = 1,
  •  a^2 + b^2 + c^2 = 3,
  •  a + b + c = 3,
  •  the Cauchy–Schwarz bounds and the AM–GM bounds are tight.

In that case each term is 1/(1+1+1) = 1/3, so the sum is 1.  Hence C = 1 is the smallest constant for which the inequality always holds.

Final Answer:
The answer is $C=1$
