# Problem Entry

## Problem Type
bound

## Problem
Let $x, y, z > 0$ such that $xyz = 1$. Determine the largest constant $C$ such that the following inequality holds for all $x, y, z$:
$$
\frac{x^3}{(1+y)(1+z)} + \frac{y^3}{(1+z)(1+x)} + \frac{z^3}{(1+x)(1+y)} \geq C.
$$

## Current Solution
Let $x \geq y \geq z$. Then
$$
x^{3} \geq y^{3} \geq z^{3} \quad \text { and } \quad \frac{1}{(1+y)(1+z)} \geq \frac{1}{(1+z)(1+x)} \geq \frac{1}{(1+x)(1+y)}
$$

Applying Chebishev's inequality we get
$$
\begin{aligned}
3 S & =3\left(\frac{x^{3}}{(1+y)(1+z)}+\frac{y^{3}}{(1+z)(1+x)}+\frac{z^{3}}{(1+x)(1+y)}\right) \\
& \geq\left(x^{3}+y^{3}+z^{3}\right)\left(\frac{1}{(1+y)(1+z)}+\frac{1}{(1+z)(1+x)}+\frac{1}{(1+x)(1+y)}\right) \\
& =\left(x^{3}+y^{3}+z^{3}\right)\left(\frac{(1+x)+(1+y)+(1+z)}{(1+x)(1+y)(1+z)}\right) \\
& =\left(x^{3}+y^{3}+z^{3}\right)\left(\frac{3+x+y+z}{(1+x)(1+y)(1+z)}\right)
\end{aligned}
$$
i.e.
$$
\begin{equation*}
S \geq\left(\frac{x^{3}+y^{3}+z^{3}}{3}\right)\left(\frac{3+x+y+z}{(1+x)(1+y)(1+z)}\right) \tag{1}
\end{equation*}
$$

Let $\frac{x+y+z}{3}=a$. Then we have
$$
\frac{x^{3}+y^{3}+z^{3}}{3} \geq\left(\frac{x+y+z}{3}\right)^{3}=a^{3} \quad \text { and } \quad 3 a \geq 3 \sqrt[3]{x y z}=3, \quad \text { i.e. } \quad a \geq 1
$$

From $A M \geq G M$ we get
$$
(1+x)(1+y)(1+z) \leq\left(\frac{3+x+y+z}{3}\right)^{3}=(1+a)^{3}
$$

So by (1) we obtain
$$
S \geq\left(\frac{x^{3}+y^{3}+z^{3}}{3}\right)\left(\frac{3+x+y+z}{(1+x)(1+y)(1+z)}\right) \geq a^{3}\left(\frac{6}{(1+a)^{3}}\right)
$$

Hence it suffices to show that
$$
\frac{6 a^{3}}{(1+a)^{3}} \geq \frac{3}{4}
$$
i.e.
$$
6\left(1-\frac{1}{1+a}\right)^{3}=\frac{6 a^{3}}{(1+a)^{3}} \geq \frac{3}{4}
$$

Since $a \geq 1$, and the function $f(x)=6\left(1-\frac{1}{1+x}\right)^{3}$ increases on [1, $\infty$ ] (why?), it follows that $f(a) \geq f(1)=\frac{3}{4}$, as required.

Equality holds when $x = y = z = 1$, since $xyz = 1$ and $a = 1$. In this case, each term is $\frac{1}{2}$, so the sum is $\frac{3}{2}$, and the lower bound $C = \frac{3}{4}$ is achieved as the minimum value. Therefore, this gives the minimum value of the expression.

Therefore, the answer is $C = \frac{3}{4}$.

## Expected Answer
$C = \frac{3}{4}$

## Enhanced Solution
Enhanced Solution:

We wish to show that for all positive real numbers $x,y,z>0$ with $xyz=1$, the expression

S=\frac{x^3}{(1+y)(1+z)} + \frac{y^3}{(1+z)(1+x)} + \frac{z^3}{(1+x)(1+y)}

satisfies S\ge C, and to determine the largest such constant C.  The original approach uses Chebyshev’s inequality and classical mean inequalities.  We now present a more detailed, step-by-step, and fully justified argument without changing the overall strategy.

1. Ordering and application of Chebyshev’s inequality

  a. Without loss of generality, relabel so that
     x\ge y\ge z>0.
     Then also x^3\ge y^3\ge z^3.

  b. Observe that the three factors in the denominators satisfy
     (1+y)(1+z) \le (1+z)(1+x) \le (1+x)(1+y)
     because x\ge y\ge z implies 1+x\ge1+y\ge1+z.  Hence
     \frac1{(1+y)(1+z)} \ge \frac1{(1+z)(1+x)} \ge \frac1{(1+x)(1+y)}.

  c. We now invoke Chebyshev’s inequality for two sequences that are similarly ordered.  In general, if a_1\ge a_2\ge a_3 and b_1\ge b_2\ge b_3, then
     \frac{a_1b_1 + a_2b_2 + a_3b_3}3 \ge \Bigl(\frac{a_1+a_2+a_3}3\Bigr)\Bigl(\frac{b_1+b_2+b_3}3\Bigr).

  d. Apply this with a_i = x^3,y^3,z^3 and b_i = 1/((1+y)(1+z)),1/((1+z)(1+x)),1/((1+x)(1+y)).  Then

     (x^3/(1+y)(1+z) + y^3/(1+z)(1+x) + z^3/(1+x)(1+y))
     \quad\ge\quad
     \frac{x^3+y^3+z^3}3 \;\times\; \frac{1/(1+y)(1+z) + 1/(1+z)(1+x) + 1/(1+x)(1+y)}3.

     Multiplying both sides by 3, we obtain

     3S \ge (x^3+y^3+z^3) \cdot \Bigl(\frac1{(1+y)(1+z)} + \frac1{(1+z)(1+x)} + \frac1{(1+x)(1+y)}\Bigr).

2. Simplifying the sum of reciprocals

  a. Notice that
     \frac1{(1+y)(1+z)} + \frac1{(1+z)(1+x)} + \frac1{(1+x)(1+y)}
     
     = \frac{(1+x)+(1+y)+(1+z)}{(1+x)(1+y)(1+z)}
     = \frac{3 + (x+y+z)}{(1+x)(1+y)(1+z)}.

  b. Hence from step 1d we get the concise bound

     3S \ge (x^3 + y^3 + z^3) \;\frac{3 + (x+y+z)}{(1+x)(1+y)(1+z)}
     \quad\Longrightarrow\quad
     S \ge \Bigl(\frac{x^3+y^3+z^3}3\Bigr) \;\frac{3 + (x+y+z)}{(1+x)(1+y)(1+z)}.   \quad(1)

3. Introduction of the symmetric mean a = (x+y+z)/3

  a. Define a = (x+y+z)/3.  Since xyz=1, by the arithmetic–geometric means inequality on x,y,z we have
     a = \frac{x+y+z}3 \ge (xyz)^{1/3} = 1.

  b. Also by the Power Mean inequality (or simply by convexity of t\mapsto t^3 for t>0),
     \frac{x^3+y^3+z^3}3 \ge \Bigl(\frac{x+y+z}3\Bigr)^3 = a^3.

  c. Next, by AM–GM applied to (1+x),(1+y),(1+z),
     \frac{(1+x)+(1+y)+(1+z)}3 \ge \bigl((1+x)(1+y)(1+z)\bigr)^{1/3}.
     But (1+x)+(1+y)+(1+z) = 3 + (x+y+z) = 3(1+a).
     Therefore,
     (1+x)(1+y)(1+z) \le (\tfrac{3(1+a)}3)^3 = (1+a)^3.

4. Combining the inequalities into a single bound

  Substitute the two estimates of steps 3b and 3c into inequality (1) to obtain

     S \ge a^3 \times \frac{3 + (x+y+z)}{(1+x)(1+y)(1+z)}
         = a^3 \times \frac{3 + 3a}{(1+x)(1+y)(1+z)}
         = a^3 \times \frac{3(1+a)}{(1+x)(1+y)(1+z)}
         \ge a^3 \;\frac{3(1+a)}{(1+a)^3}
         = \frac{3a^3}{(1+a)^2}.

  A slightly stronger simplification observes that
     3(1+a)/(1+a)^3 = 3/(1+a)^2,
  so altogether

     S \ge \frac{3a^3}{(1+a)^2}.

5. Final reduction to a single-variable inequality

  Define the function
     f(a) = \frac{3a^3}{(1+a)^2}
     \quad\text{for }a\ge1.

  Our goal is to show f(a)\ge C for some C, and then find the largest such C.  Note that

     f'(a)
     = \frac{9a^2(1+a)^2 - 3a^3\cdot2(1+a)}{(1+a)^4}
     = \frac{3a^2(1+a)[3(1+a) - 2a]}{(1+a)^4}
     = \frac{3a^2(1+a)(3 + 3a - 2a)}{(1+a)^4}
     = \frac{3a^2(1+a)(3 + a)}{(1+a)^4} > 0
     \quad\text{for all }a>0.

  Hence f is strictly increasing on [1,\infty).  Therefore for all a\ge1,

     f(a) \ge f(1) = \frac{3\cdot1^3}{(1+1)^2} = \frac{3}{4}.

  Consequently, for every (x,y,z) with xyz=1 we have S\ge f(a)\ge 3/4.

6. Verification of equality case

  Equality f(a)=3/4 occurs exactly at a=1.  Since a=(x+y+z)/3=1 and xyz=1, by the equality conditions of AM–GM we must have x=y=z=1.  Substituting x=y=z=1 into the original expression gives

     S = 3\;\frac{1^3}{(1+1)(1+1)} = 3\;\frac{1}{2\cdot2} = \frac{3}{4}.

  This shows the bound is sharp and attained when x=y=z=1.

Therefore, the largest constant C for which S\ge C holds under the constraint xyz=1 is C=3/4.

The answer is $C=\frac{3}{4}$.
