## Problem

Let $a, b > 0$ and $a + b \leq \frac{3}{2}$. Find the smallest constant $C$ such that the following inequality holds for all $a, b$ satisfying the given constraint:
$$
\frac{a}{a^2+1} + \frac{4b}{b^2+4} \leq C.
$$

## Query

Task description: Please solve the problem with clear, rigorous, and logically sound steps. At the end of your response, state your answer in exactly this format: 'The answer is $C=X$', where X is your calculated numerical bound value. Example: 'The answer is $C=1$'.

Problem: Let $a, b > 0$ and $a + b \leq \frac{3}{2}$. Find the smallest constant $C$ such that the following inequality holds for all $a, b$ satisfying the given constraint:
$$
\frac{a}{a^2+1} + \frac{4b}{b^2+4} \leq C.
$$

Please use some of the following theorems to solve the problem:
Theorem 1 (Category: Inequality Between Means, Nicknames: mean inequalities): Let $a_{1}, a_{2}, \ldots, a_{n}$ be positive real numbers. The numbers
$$
\begin{aligned}
& Q M=\sqrt{\frac{a_{1}^{2}+a_{2}^{2}+\cdots+a_{n}^{2}}{n}}, \quad A M=\frac{a_{1}+a_{2}+\cdots+a_{n}}{n} \\
& G M=\sqrt[n]{a_{1} a_{2} \cdots a_{n}} \quad \text { and } \quad H M=\frac{n}{\frac{1}{a_{1}}+\frac{1}{a_{2}}+\cdots+\frac{1}{a_{n}}}
\end{aligned}
$$
are called the quadratic, arithmetic, geometric and harmonic mean for the numbers $a_{1}, a_{2}, \ldots, a_{n}$, respectively, and we have
$$
Q M \geq A M \geq G M \geq H M
$$

Equalities occur if and only if $a_{1}=a_{2}=\cdots=a_{n}$.

Theorem 2 (Category: Cauchy-Schwarz Inequality, Nicknames: cauchy-schwarz inequality): Let $a_{1}, a_{2}, \ldots, a_{n}$ and $b_{1}, b_{2}$, $\ldots, b_{n}$ be real numbers. Then we have
$$
\left(\sum_{i=1}^{n} a_{i}^{2}\right)\left(\sum_{i=1}^{n} b_{i}^{2}\right) \geq\left(\sum_{i=1}^{n} a_{i} b_{i}\right)^{2}
$$
i.e.
$$
\left(a_{1}^{2}+a_{2}^{2}+\cdots+a_{n}^{2}\right)\left(b_{1}^{2}+b_{2}^{2}+\cdots+b_{n}^{2}\right) \geq\left(a_{1} b_{1}+a_{2} b_{2}+\cdots+a_{n} b_{n}\right)^{2}
$$

Equality occurs if and only if the sequences $\left(a_{1}, a_{2}, \ldots, a_{n}\right)$ and $\left(b_{1}, b_{2}\right.$, $\ldots, b_{n}$ ) are proportional, i.e. $\frac{a_{1}}{b_{1}}=\frac{a_{2}}{b_{2}}=\cdots=\frac{a_{n}}{b_{n}}$.

Theorem 3 (Category: Inequality Between Means, Nicknames: am-gm (arithmetic mean-geometric mean) inequality, am-gm): If $a_{1}, a_{2}, \ldots, a_{n}$ are nonnegative real numbers, then

$$
\frac{1}{n} \sum_{i=1}^{n} a_{i} \geq\left(a_{1} a_{2} \ldots a_{n}\right)^{\frac{1}{n}}
$$

with equality if and only if $a_{1}=a_{2}=\ldots=a_{n}$. This inequality is a special case of the Power Mean Inequality.

Solution:

## Response

To find the smallest constant \( C \) such that the inequality 

\[
\frac{a}{a^2+1} + \frac{4b}{b^2+4} \leq C
\]

holds for all \( a, b > 0 \) satisfying \( a + b \leq \frac{3}{2} \), we will analyze each term separately and then combine the results.

### Step 1: Analyze the term \( \frac{a}{a^2 + 1} \)

We start by finding the maximum value of \( \frac{a}{a^2 + 1} \). To do this, we can differentiate the function:

Let \( f(a) = \frac{a}{a^2 + 1} \).

Calculating the derivative using the quotient rule:

\[
f'(a) = \frac{(a^2 + 1)(1) - a(2a)}{(a^2 + 1)^2} = \frac{a^2 + 1 - 2a^2}{(a^2 + 1)^2} = \frac{1 - a^2}{(a^2 + 1)^2}
\]

Setting \( f'(a) = 0 \) gives:

\[
1 - a^2 = 0 \implies a^2 = 1 \implies a = 1 \quad (\text{since } a > 0)
\]

Now we evaluate \( f(a) \) at \( a = 1 \):

\[
f(1) = \frac{1}{1^2 + 1} = \frac{1}{2}
\]

Next, we check the behavior of \( f(a) \) as \( a \to 0 \) and \( a \to \infty \):

- As \( a \to 0 \), \( f(a) \to 0 \).
- As \( a \to \infty \), \( f(a) \to 0 \).

Thus, the maximum value of \( f(a) \) occurs at \( a = 1 \) and is \( \frac{1}{2} \).

### Step 2: Analyze the term \( \frac{4b}{b^2 + 4} \)

Next, we analyze the term \( \frac{4b}{b^2 + 4} \). Let \( g(b) = \frac{4b}{b^2 + 4} \).

Calculating the derivative:

\[
g'(b) = \frac{(b^2 + 4)(4) - 4b(2b)}{(b^2 + 4)^2} = \frac{4b^2 + 16 - 8b^2}{(b^2 + 4)^2} = \frac{16 - 4b^2}{(b^2 + 4)^2}
\]

Setting \( g'(b) = 0 \):

\[
16 - 4b^2 = 0 \implies 4b^2 = 16 \implies b^2 = 4 \implies b = 2 \quad (\text{since } b > 0)
\]

Now we evaluate \( g(b) \) at \( b = 2 \):

\[
g(2) = \frac{4 \cdot 2}{2^2 + 4} = \frac{8}{4 + 4} = 1
\]

Next, we check the behavior of \( g(b) \) as \( b \to 0 \) and \( b \to \infty \):

- As \( b \to 0 \), \( g(b) \to 0 \).
- As \( b \to \infty \), \( g(b) \to 0 \).

Thus, the maximum value of \( g(b) \) occurs at \( b = 2 \) and is \( 1 \).

### Step 3: Combine results under the constraint \( a + b \leq \frac{3}{2} \)

Now we need to find the maximum of 

\[
\frac{a}{a^2 + 1} + \frac{4b}{b^2 + 4}
\]

under the constraint \( a + b \leq \frac{3}{2} \).

Let \( b = \frac{3}{2} - a \). We substitute this into the inequality:

\[
\frac{a}{a^2 + 1} + \frac{4\left(\frac{3}{2} - a\right)}{\left(\frac{3}{2} - a\right)^2 + 4}
\]

We need to find the maximum of this expression. However, we can also evaluate specific cases:

1. **Case 1**: \( a = 1, b = \frac{1}{2} \)

\[
\frac{1}{1^2 + 1} + \frac{4 \cdot \frac{1}{2}}{\left(\frac{1}{2}\right)^2 + 4} = \frac{1}{2} + \frac{2}{\frac{1}{4} + 4} = \frac{1}{2} + \frac{2}{\frac{17}{4}} = \frac{1}{2} + \frac{8}{17} = \frac{17 + 8}{34} = \frac{25}{34}
\]

2. **Case 2**: \( a = \frac{3}{2}, b = 0 \)

\[
\frac{\frac{3}{2}}{\left(\frac{3}{2}\right)^2 + 1} + 0 = \frac{\frac{3}{2}}{\frac{9}{4} + 1} = \frac{\frac{3}{2}}{\frac{13}{4}} = \frac{3 \cdot 4}{2 \cdot 13} = \frac{6}{13}
\]

3. **Case 3**: \( a = 0, b = \frac{3}{2} \)

\[
0 + \frac{4 \cdot \frac{3}{2}}{\left(\frac{3}{2}\right)^2 + 4} = \frac{6}{\frac{9}{4} + 4} = \frac{6}{\frac{25}{4}} = \frac{24}{25}
\]

### Conclusion

The maximum value we found is \( \frac{24}{25} \). Therefore, the smallest constant \( C \) such that the inequality holds for all \( a, b \) satisfying \( a + b \leq \frac{3}{2} \) is:

\[
C = \frac{24}{25}
\]

Thus, the final answer is:

\[
\text{The answer is } C = \frac{24}{25}
\]