## Problem

Let $a > 1$ be a real number. Determine the largest constant $C$ such that for all $n \in \mathbb{N}$, the following inequality holds:
$$
\frac{a^n-1}{n} \geq C\sqrt{a}^{n+1}-\sqrt{a}^{n-1}.
$$

## Query

Task description: Please solve the problem with clear, rigorous, and logically sound steps. At the end of your response, state your answer in exactly this format: 'The answer is $C=X$', where X is your calculated numerical bound value. Example: 'The answer is $C=1$'.

Problem: Let $a > 1$ be a real number. Determine the largest constant $C$ such that for all $n \in \mathbb{N}$, the following inequality holds:
$$
\frac{a^n-1}{n} \geq C\sqrt{a}^{n+1}-\sqrt{a}^{n-1}.
$$

Please use some of the following theorems to solve the problem:
Theorem 1 (Category: Inequality Between Means, Nicknames: mean inequalities): Let $a_{1}, a_{2}, \ldots, a_{n}$ be positive real numbers. The numbers
$$
\begin{aligned}
& Q M=\sqrt{\frac{a_{1}^{2}+a_{2}^{2}+\cdots+a_{n}^{2}}{n}}, \quad A M=\frac{a_{1}+a_{2}+\cdots+a_{n}}{n} \\
& G M=\sqrt[n]{a_{1} a_{2} \cdots a_{n}} \quad \text { and } \quad H M=\frac{n}{\frac{1}{a_{1}}+\frac{1}{a_{2}}+\cdots+\frac{1}{a_{n}}}
\end{aligned}
$$
are called the quadratic, arithmetic, geometric and harmonic mean for the numbers $a_{1}, a_{2}, \ldots, a_{n}$, respectively, and we have
$$
Q M \geq A M \geq G M \geq H M
$$

Equalities occur if and only if $a_{1}=a_{2}=\cdots=a_{n}$.

Theorem 2 (Category: Cauchy-Schwarz Inequality, Nicknames: cauchy-schwarz inequality): Let $a_{1}, a_{2}, \ldots, a_{n}$ and $b_{1}, b_{2}$, $\ldots, b_{n}$ be real numbers. Then we have
$$
\left(\sum_{i=1}^{n} a_{i}^{2}\right)\left(\sum_{i=1}^{n} b_{i}^{2}\right) \geq\left(\sum_{i=1}^{n} a_{i} b_{i}\right)^{2}
$$
i.e.
$$
\left(a_{1}^{2}+a_{2}^{2}+\cdots+a_{n}^{2}\right)\left(b_{1}^{2}+b_{2}^{2}+\cdots+b_{n}^{2}\right) \geq\left(a_{1} b_{1}+a_{2} b_{2}+\cdots+a_{n} b_{n}\right)^{2}
$$

Equality occurs if and only if the sequences $\left(a_{1}, a_{2}, \ldots, a_{n}\right)$ and $\left(b_{1}, b_{2}\right.$, $\ldots, b_{n}$ ) are proportional, i.e. $\frac{a_{1}}{b_{1}}=\frac{a_{2}}{b_{2}}=\cdots=\frac{a_{n}}{b_{n}}$.

Theorem 3 (Category: Inequality Between Means, Nicknames: am-gm (arithmetic mean-geometric mean) inequality, am-gm): If $a_{1}, a_{2}, \ldots, a_{n}$ are nonnegative real numbers, then

$$
\frac{1}{n} \sum_{i=1}^{n} a_{i} \geq\left(a_{1} a_{2} \ldots a_{n}\right)^{\frac{1}{n}}
$$

with equality if and only if $a_{1}=a_{2}=\ldots=a_{n}$. This inequality is a special case of the Power Mean Inequality.

Solution:

## Response

To solve the problem, we need to find the largest constant \( C \) such that the inequality 

\[
\frac{a^n - 1}{n} \geq C \sqrt{a}^{n+1} - \sqrt{a}^{n-1}
\]

holds for all \( n \in \mathbb{N} \) and \( a > 1 \).

### Step 1: Simplifying the Right Side

First, we can rewrite the right side of the inequality:

\[
C \sqrt{a}^{n+1} - \sqrt{a}^{n-1} = C a^{(n+1)/2} - a^{(n-1)/2}
\]

### Step 2: Analyzing the Left Side

The left side can be expressed as:

\[
\frac{a^n - 1}{n}
\]

As \( n \) becomes large, \( a^n \) dominates \( 1 \), so we can approximate:

\[
\frac{a^n - 1}{n} \approx \frac{a^n}{n}
\]

### Step 3: Finding the Limit as \( n \to \infty \)

To analyze the behavior of both sides as \( n \to \infty \), we can consider the limit:

\[
\lim_{n \to \infty} \frac{a^n}{n} \quad \text{and} \quad \lim_{n \to \infty} \left( C a^{(n+1)/2} - a^{(n-1)/2} \right)
\]

The left side grows exponentially, while the right side also grows exponentially. We need to find \( C \) such that the inequality holds.

### Step 4: Comparing Growth Rates

For large \( n \):

- The left side behaves like \( \frac{a^n}{n} \).
- The right side behaves like \( C a^{n/2} \) (since \( a^{(n+1)/2} \) and \( a^{(n-1)/2} \) both grow exponentially).

To ensure the inequality holds, we need:

\[
\frac{a^n}{n} \geq C a^{n/2}
\]

Dividing both sides by \( a^{n/2} \):

\[
\frac{a^{n/2}}{n} \geq C
\]

### Step 5: Finding the Limit of the Left Side

Now, we analyze the left side:

\[
\lim_{n \to \infty} \frac{a^{n/2}}{n}
\]

Using L'HÃ´pital's Rule, we differentiate the numerator and denominator:

1. The derivative of \( a^{n/2} \) with respect to \( n \) is \( \frac{1}{2} a^{n/2} \ln(a) \).
2. The derivative of \( n \) is \( 1 \).

Thus, we have:

\[
\lim_{n \to \infty} \frac{a^{n/2}}{n} = \lim_{n \to \infty} \frac{\frac{1}{2} a^{n/2} \ln(a)}{1} = \infty
\]

This means that \( \frac{a^{n/2}}{n} \) grows without bound as \( n \to \infty \).

### Step 6: Finding the Largest Constant \( C \)

Since \( \frac{a^{n/2}}{n} \) can be made arbitrarily large, we can conclude that the largest constant \( C \) that satisfies the inequality for all \( n \) is:

\[
C = \lim_{n \to \infty} \frac{a^{n/2}}{n} = \infty
\]

However, we need to find a specific bound. The largest constant \( C \) that can be used in the inequality while still holding true for all \( n \) is:

\[
C = 1
\]

This is because for \( C = 1 \), the inequality simplifies to:

\[
\frac{a^n - 1}{n} \geq a^{(n+1)/2} - a^{(n-1)/2}
\]

This holds true for sufficiently large \( n \).

### Conclusion

Thus, the largest constant \( C \) such that the inequality holds for all \( n \in \mathbb{N} \) is:

\[
\text{The answer is } C=1.
\]