## Problem

Let $x, y, z \in [-1, 3]$ such that $x + y + z = 3$. Find the smallest constant $C$ such that the following inequality holds for all $x, y, z$:
$$
x^2 + y^2 + z^2 \leq C.
$$

## Query

Task description: Please solve the problem with clear, rigorous, and logically sound steps. At the end of your response, state your answer in exactly this format: 'The answer is $C=X$', where X is your calculated numerical bound value. Example: 'The answer is $C=1$'.

Problem: Let $x, y, z \in [-1, 3]$ such that $x + y + z = 3$. Find the smallest constant $C$ such that the following inequality holds for all $x, y, z$:
$$
x^2 + y^2 + z^2 \leq C.
$$

Please use some of the following theorems to solve the problem:
Theorem 1 (Category: Inequality Between Means, Nicknames: mean inequalities): Let $a_{1}, a_{2}, \ldots, a_{n}$ be positive real numbers. The numbers
$$
\begin{aligned}
& Q M=\sqrt{\frac{a_{1}^{2}+a_{2}^{2}+\cdots+a_{n}^{2}}{n}}, \quad A M=\frac{a_{1}+a_{2}+\cdots+a_{n}}{n} \\
& G M=\sqrt[n]{a_{1} a_{2} \cdots a_{n}} \quad \text { and } \quad H M=\frac{n}{\frac{1}{a_{1}}+\frac{1}{a_{2}}+\cdots+\frac{1}{a_{n}}}
\end{aligned}
$$
are called the quadratic, arithmetic, geometric and harmonic mean for the numbers $a_{1}, a_{2}, \ldots, a_{n}$, respectively, and we have
$$
Q M \geq A M \geq G M \geq H M
$$

Equalities occur if and only if $a_{1}=a_{2}=\cdots=a_{n}$.

Theorem 2 (Category: Cauchy-Schwarz Inequality, Nicknames: cauchy-schwarz inequality): Let $a_{1}, a_{2}, \ldots, a_{n}$ and $b_{1}, b_{2}$, $\ldots, b_{n}$ be real numbers. Then we have
$$
\left(\sum_{i=1}^{n} a_{i}^{2}\right)\left(\sum_{i=1}^{n} b_{i}^{2}\right) \geq\left(\sum_{i=1}^{n} a_{i} b_{i}\right)^{2}
$$
i.e.
$$
\left(a_{1}^{2}+a_{2}^{2}+\cdots+a_{n}^{2}\right)\left(b_{1}^{2}+b_{2}^{2}+\cdots+b_{n}^{2}\right) \geq\left(a_{1} b_{1}+a_{2} b_{2}+\cdots+a_{n} b_{n}\right)^{2}
$$

Equality occurs if and only if the sequences $\left(a_{1}, a_{2}, \ldots, a_{n}\right)$ and $\left(b_{1}, b_{2}\right.$, $\ldots, b_{n}$ ) are proportional, i.e. $\frac{a_{1}}{b_{1}}=\frac{a_{2}}{b_{2}}=\cdots=\frac{a_{n}}{b_{n}}$.

Theorem 3 (Category: Inequality Between Means, Nicknames: am-gm (arithmetic mean-geometric mean) inequality, am-gm): If $a_{1}, a_{2}, \ldots, a_{n}$ are nonnegative real numbers, then

$$
\frac{1}{n} \sum_{i=1}^{n} a_{i} \geq\left(a_{1} a_{2} \ldots a_{n}\right)^{\frac{1}{n}}
$$

with equality if and only if $a_{1}=a_{2}=\ldots=a_{n}$. This inequality is a special case of the Power Mean Inequality.

Solution:

## Response

To find the smallest constant \( C \) such that the inequality 

\[
x^2 + y^2 + z^2 \leq C
\]

holds for all \( x, y, z \in [-1, 3] \) with the constraint \( x + y + z = 3 \), we can use the method of Lagrange multipliers or analyze the problem using the properties of quadratic forms and the given constraints.

### Step 1: Express \( z \) in terms of \( x \) and \( y \)

From the constraint \( x + y + z = 3 \), we can express \( z \) as:

\[
z = 3 - x - y
\]

### Step 2: Substitute \( z \) into the expression

Now, substituting \( z \) into the expression for \( x^2 + y^2 + z^2 \):

\[
x^2 + y^2 + z^2 = x^2 + y^2 + (3 - x - y)^2
\]

Expanding \( (3 - x - y)^2 \):

\[
(3 - x - y)^2 = 9 - 6x - 6y + x^2 + 2xy + y^2
\]

Thus, we have:

\[
x^2 + y^2 + z^2 = x^2 + y^2 + 9 - 6x - 6y + x^2 + 2xy + y^2
\]

Combining like terms:

\[
= 2x^2 + 2y^2 + 2xy - 6x - 6y + 9
\]

### Step 3: Simplify the expression

We can factor out a 2 from the first three terms:

\[
= 2(x^2 + y^2 + xy) - 6(x + y) + 9
\]

### Step 4: Analyze the bounds of \( x \) and \( y \)

Given \( x, y, z \in [-1, 3] \), we need to find the maximum of \( x^2 + y^2 + z^2 \) under the constraint \( x + y + z = 3 \).

### Step 5: Consider the extreme values

1. **Case 1**: \( x = 3, y = 0, z = 0 \)
   \[
   x^2 + y^2 + z^2 = 3^2 + 0^2 + 0^2 = 9
   \]

2. **Case 2**: \( x = 0, y = 3, z = 0 \)
   \[
   x^2 + y^2 + z^2 = 0^2 + 3^2 + 0^2 = 9
   \]

3. **Case 3**: \( x = 0, y = 0, z = 3 \)
   \[
   x^2 + y^2 + z^2 = 0^2 + 0^2 + 3^2 = 9
   \]

4. **Case 4**: \( x = -1, y = -1, z = 5 \) (not valid since \( z \) exceeds 3)

5. **Case 5**: \( x = -1, y = 3, z = 1 \)
   \[
   x^2 + y^2 + z^2 = (-1)^2 + 3^2 + 1^2 = 1 + 9 + 1 = 11
   \]

6. **Case 6**: \( x = 1, y = 1, z = 1 \)
   \[
   x^2 + y^2 + z^2 = 1^2 + 1^2 + 1^2 = 3
   \]

### Step 6: Find the maximum value

From the cases analyzed, the maximum value of \( x^2 + y^2 + z^2 \) occurs in Case 5, yielding:

\[
x^2 + y^2 + z^2 = 11
\]

### Conclusion

Thus, the smallest constant \( C \) such that the inequality holds for all \( x, y, z \) under the given conditions is:

\[
\boxed{11}
\]

Therefore, the answer is 

\[
\text{The answer is } C=11.
\]