## Problem

Let $a, b, c$ be positive real numbers such that $abc = 1$. Consider the following inequality:
$$
\sum \frac{1}{b(a+b)} \quad () \quad \frac{5}{3}.
$$

Determine the correct inequality relation to fill in the blank.

Options:

(A) $\leq$ 

(B) $\geq$

(C) $=$ 

(D) $<$

(E) $>$

(F) None of the above

## Query

Task description: Please solve the problem with clear, rigorous, and logically sound steps. At the end of your response, state your answer in exactly this format: 'The answer is (Letter) Symbol', where Letter is one of the given options. Example: 'The answer is (A) $\leq$'.

Problem: Let $a, b, c$ be positive real numbers such that $abc = 1$. Consider the following inequality:
$$
\sum \frac{1}{b(a+b)} \quad () \quad \frac{5}{3}.
$$

Determine the correct inequality relation to fill in the blank.

Options:

(A) $\leq$ 

(B) $\geq$

(C) $=$ 

(D) $<$

(E) $>$

(F) None of the above

Please use some of the following theorems to solve the problem:
Theorem 1 (Category: Inequality Between Means, Nicknames: mean inequalities): Let $a_{1}, a_{2}, \ldots, a_{n}$ be positive real numbers. The numbers
$$
\begin{aligned}
& Q M=\sqrt{\frac{a_{1}^{2}+a_{2}^{2}+\cdots+a_{n}^{2}}{n}}, \quad A M=\frac{a_{1}+a_{2}+\cdots+a_{n}}{n} \\
& G M=\sqrt[n]{a_{1} a_{2} \cdots a_{n}} \quad \text { and } \quad H M=\frac{n}{\frac{1}{a_{1}}+\frac{1}{a_{2}}+\cdots+\frac{1}{a_{n}}}
\end{aligned}
$$
are called the quadratic, arithmetic, geometric and harmonic mean for the numbers $a_{1}, a_{2}, \ldots, a_{n}$, respectively, and we have
$$
Q M \geq A M \geq G M \geq H M
$$

Equalities occur if and only if $a_{1}=a_{2}=\cdots=a_{n}$.

Theorem 2 (Category: Cauchy-Schwarz Inequality, Nicknames: cauchy-schwarz inequality): Let $a_{1}, a_{2}, \ldots, a_{n}$ and $b_{1}, b_{2}$, $\ldots, b_{n}$ be real numbers. Then we have
$$
\left(\sum_{i=1}^{n} a_{i}^{2}\right)\left(\sum_{i=1}^{n} b_{i}^{2}\right) \geq\left(\sum_{i=1}^{n} a_{i} b_{i}\right)^{2}
$$
i.e.
$$
\left(a_{1}^{2}+a_{2}^{2}+\cdots+a_{n}^{2}\right)\left(b_{1}^{2}+b_{2}^{2}+\cdots+b_{n}^{2}\right) \geq\left(a_{1} b_{1}+a_{2} b_{2}+\cdots+a_{n} b_{n}\right)^{2}
$$

Equality occurs if and only if the sequences $\left(a_{1}, a_{2}, \ldots, a_{n}\right)$ and $\left(b_{1}, b_{2}\right.$, $\ldots, b_{n}$ ) are proportional, i.e. $\frac{a_{1}}{b_{1}}=\frac{a_{2}}{b_{2}}=\cdots=\frac{a_{n}}{b_{n}}$.

Theorem 3 (Category: Inequality Between Means, Nicknames: am-gm (arithmetic mean-geometric mean) inequality, am-gm): If $a_{1}, a_{2}, \ldots, a_{n}$ are nonnegative real numbers, then

$$
\frac{1}{n} \sum_{i=1}^{n} a_{i} \geq\left(a_{1} a_{2} \ldots a_{n}\right)^{\frac{1}{n}}
$$

with equality if and only if $a_{1}=a_{2}=\ldots=a_{n}$. This inequality is a special case of the Power Mean Inequality.

Solution:

## Response

To solve the inequality 

\[
\sum \frac{1}{b(a+b)} \quad () \quad \frac{5}{3}
\]

given that \(abc = 1\) for positive real numbers \(a, b, c\), we will analyze the left-hand side using the Cauchy-Schwarz inequality.

### Step 1: Apply Cauchy-Schwarz Inequality

We can apply the Cauchy-Schwarz inequality in the following way:

\[
\left( \sum_{cyc} \frac{1}{b(a+b)} \right) \left( \sum_{cyc} b(a+b) \right) \geq \left( \sum_{cyc} 1 \right)^2
\]

Calculating the right-hand side:

\[
\sum_{cyc} 1 = 3 \quad \Rightarrow \quad \left( \sum_{cyc} 1 \right)^2 = 3^2 = 9
\]

Now we need to compute \( \sum_{cyc} b(a+b) \):

\[
\sum_{cyc} b(a+b) = ab + ac + ba + bc + ca + cb = ab + ac + bc + ab + ac + bc = 2(ab + ac + bc)
\]

Thus, we have:

\[
\left( \sum_{cyc} \frac{1}{b(a+b)} \right) (2(ab + ac + bc)) \geq 9
\]

### Step 2: Rearranging the Inequality

Rearranging gives us:

\[
\sum_{cyc} \frac{1}{b(a+b)} \geq \frac{9}{2(ab + ac + bc)}
\]

### Step 3: Use AM-GM Inequality

Now, we can apply the AM-GM inequality to \(ab + ac + bc\):

\[
ab + ac + bc \geq 3\sqrt[3]{(abc)^2} = 3\sqrt[3]{1^2} = 3
\]

### Step 4: Substitute Back

Substituting this back into our inequality gives:

\[
\sum_{cyc} \frac{1}{b(a+b)} \geq \frac{9}{2 \cdot 3} = \frac{9}{6} = \frac{3}{2}
\]

### Step 5: Compare with \(\frac{5}{3}\)

Now we need to compare \(\frac{3}{2}\) with \(\frac{5}{3}\):

\[
\frac{3}{2} = \frac{9}{6} \quad \text{and} \quad \frac{5}{3} = \frac{10}{6}
\]

Since \(\frac{9}{6} < \frac{10}{6}\), we conclude that:

\[
\sum_{cyc} \frac{1}{b(a+b)} < \frac{5}{3}
\]

### Conclusion

Thus, the correct inequality relation to fill in the blank is:

\[
\sum \frac{1}{b(a+b)} \quad < \quad \frac{5}{3}
\]

Therefore, the answer is:

The answer is (D) $<$.