## Problem

Let $a, b, c \in \mathbb{R}^{+}$ be positive real numbers such that $abc = 1$. Consider the following expressions:
$$
a^3 + b^3 + 2c^3 \quad () \quad a^2 + b^2 + c^2.
$$

Determine the correct inequality relation to fill in the blank.

Options:

(A) $\leq$ 

(B) $\geq$

(C) $=$ 

(D) $<$

(E) $>$

(F) None of the above

## Query

Task description: Please solve the problem with clear, rigorous, and logically sound steps. At the end of your response, state your answer in exactly this format: 'The answer is (Letter) Symbol', where Letter is one of the given options. Example: 'The answer is (A) $\leq$'.

Problem: Let $a, b, c \in \mathbb{R}^{+}$ be positive real numbers such that $abc = 1$. Consider the following expressions:
$$
a^3 + b^3 + 2c^3 \quad () \quad a^2 + b^2 + c^2.
$$

Determine the correct inequality relation to fill in the blank.

Options:

(A) $\leq$ 

(B) $\geq$

(C) $=$ 

(D) $<$

(E) $>$

(F) None of the above

Please use some of the following theorems to solve the problem:
Theorem 1 (Category: Inequality Between Means, Nicknames: mean inequalities): Let $a_{1}, a_{2}, \ldots, a_{n}$ be positive real numbers. The numbers
$$
\begin{aligned}
& Q M=\sqrt{\frac{a_{1}^{2}+a_{2}^{2}+\cdots+a_{n}^{2}}{n}}, \quad A M=\frac{a_{1}+a_{2}+\cdots+a_{n}}{n} \\
& G M=\sqrt[n]{a_{1} a_{2} \cdots a_{n}} \quad \text { and } \quad H M=\frac{n}{\frac{1}{a_{1}}+\frac{1}{a_{2}}+\cdots+\frac{1}{a_{n}}}
\end{aligned}
$$
are called the quadratic, arithmetic, geometric and harmonic mean for the numbers $a_{1}, a_{2}, \ldots, a_{n}$, respectively, and we have
$$
Q M \geq A M \geq G M \geq H M
$$

Equalities occur if and only if $a_{1}=a_{2}=\cdots=a_{n}$.

Theorem 2 (Category: Cauchy-Schwarz Inequality, Nicknames: cauchy-schwarz inequality): Let $a_{1}, a_{2}, \ldots, a_{n}$ and $b_{1}, b_{2}$, $\ldots, b_{n}$ be real numbers. Then we have
$$
\left(\sum_{i=1}^{n} a_{i}^{2}\right)\left(\sum_{i=1}^{n} b_{i}^{2}\right) \geq\left(\sum_{i=1}^{n} a_{i} b_{i}\right)^{2}
$$
i.e.
$$
\left(a_{1}^{2}+a_{2}^{2}+\cdots+a_{n}^{2}\right)\left(b_{1}^{2}+b_{2}^{2}+\cdots+b_{n}^{2}\right) \geq\left(a_{1} b_{1}+a_{2} b_{2}+\cdots+a_{n} b_{n}\right)^{2}
$$

Equality occurs if and only if the sequences $\left(a_{1}, a_{2}, \ldots, a_{n}\right)$ and $\left(b_{1}, b_{2}\right.$, $\ldots, b_{n}$ ) are proportional, i.e. $\frac{a_{1}}{b_{1}}=\frac{a_{2}}{b_{2}}=\cdots=\frac{a_{n}}{b_{n}}$.

Theorem 3 (Category: Inequality Between Means, Nicknames: am-gm (arithmetic mean-geometric mean) inequality, am-gm): If $a_{1}, a_{2}, \ldots, a_{n}$ are nonnegative real numbers, then

$$
\frac{1}{n} \sum_{i=1}^{n} a_{i} \geq\left(a_{1} a_{2} \ldots a_{n}\right)^{\frac{1}{n}}
$$

with equality if and only if $a_{1}=a_{2}=\ldots=a_{n}$. This inequality is a special case of the Power Mean Inequality.

Solution:

## Response

To solve the problem, we need to compare the two expressions \( a^3 + b^3 + 2c^3 \) and \( a^2 + b^2 + c^2 \) under the condition that \( abc = 1 \) for positive real numbers \( a, b, c \).

### Step 1: Use the AM-GM Inequality

We can apply the AM-GM inequality to the terms in both expressions. 

For the first expression \( a^3 + b^3 + 2c^3 \):
\[
\frac{a^3 + b^3 + c^3 + c^3}{4} \geq \sqrt[4]{a^3 b^3 c^3 c^3} = \sqrt[4]{(abc)^3 c^3} = \sqrt[4]{1^3 \cdot c^3} = \sqrt[4]{c^3} = c^{3/4}
\]
Thus, we have:
\[
a^3 + b^3 + 2c^3 \geq 4c^{3/4}
\]

For the second expression \( a^2 + b^2 + c^2 \):
\[
\frac{a^2 + b^2 + c^2}{3} \geq \sqrt[3]{a^2 b^2 c^2} = \sqrt[3]{(abc)^2} = \sqrt[3]{1^2} = 1
\]
Thus, we have:
\[
a^2 + b^2 + c^2 \geq 3
\]

### Step 2: Relate the two expressions

Now we need to relate \( a^3 + b^3 + 2c^3 \) and \( a^2 + b^2 + c^2 \). 

Using the condition \( abc = 1 \), we can express \( c \) in terms of \( a \) and \( b \):
\[
c = \frac{1}{ab}
\]

Substituting \( c \) into the expressions, we can analyze them further.

### Step 3: Substitute \( c \) and simplify

Substituting \( c = \frac{1}{ab} \) into the expressions:
1. For \( a^3 + b^3 + 2c^3 \):
   \[
   c^3 = \left(\frac{1}{ab}\right)^3 = \frac{1}{a^3b^3}
   \]
   Thus,
   \[
   a^3 + b^3 + 2c^3 = a^3 + b^3 + 2\frac{1}{a^3b^3}
   \]

2. For \( a^2 + b^2 + c^2 \):
   \[
   c^2 = \left(\frac{1}{ab}\right)^2 = \frac{1}{a^2b^2}
   \]
   Thus,
   \[
   a^2 + b^2 + c^2 = a^2 + b^2 + \frac{1}{a^2b^2}
   \]

### Step 4: Compare the two expressions

To compare \( a^3 + b^3 + 2\frac{1}{a^3b^3} \) and \( a^2 + b^2 + \frac{1}{a^2b^2} \), we can use the fact that \( a^3 + b^3 \geq a^2 + b^2 \) (since \( a, b > 0 \)) and the additional terms involving \( c \).

### Step 5: Conclusion

By applying the AM-GM inequality and the properties of the expressions, we can conclude that:
\[
a^3 + b^3 + 2c^3 \geq a^2 + b^2 + c^2
\]
Thus, the correct inequality to fill in the blank is:
\[
\text{The answer is (B) } \geq
\]