## Problem

Let $a, b, c \geq 0$ be real numbers such that $a^2 + b^2 + c^2 = 3$. Consider the following inequality:
$$
\sum_{cyc} \frac{a}{a+2} \quad () \quad 1.
$$

Determine the correct inequality relation to fill in the blank.

Options:

(A) $\leq$ 

(B) $\geq$

(C) $=$ 

(D) $<$

(E) $>$

(F) None of the above

## Query

Task description: Please solve the problem with clear, rigorous, and logically sound steps. At the end of your response, state your answer in exactly this format: 'The answer is (Letter) Symbol', where Letter is one of the given options. Example: 'The answer is (A) $\leq$'.

Problem: Let $a, b, c \geq 0$ be real numbers such that $a^2 + b^2 + c^2 = 3$. Consider the following inequality:
$$
\sum_{cyc} \frac{a}{a+2} \quad () \quad 1.
$$

Determine the correct inequality relation to fill in the blank.

Options:

(A) $\leq$ 

(B) $\geq$

(C) $=$ 

(D) $<$

(E) $>$

(F) None of the above

Please use some of the following theorems to solve the problem:
Theorem 1 (Category: Inequality Between Means, Nicknames: mean inequalities): Let $a_{1}, a_{2}, \ldots, a_{n}$ be positive real numbers. The numbers
$$
\begin{aligned}
& Q M=\sqrt{\frac{a_{1}^{2}+a_{2}^{2}+\cdots+a_{n}^{2}}{n}}, \quad A M=\frac{a_{1}+a_{2}+\cdots+a_{n}}{n} \\
& G M=\sqrt[n]{a_{1} a_{2} \cdots a_{n}} \quad \text { and } \quad H M=\frac{n}{\frac{1}{a_{1}}+\frac{1}{a_{2}}+\cdots+\frac{1}{a_{n}}}
\end{aligned}
$$
are called the quadratic, arithmetic, geometric and harmonic mean for the numbers $a_{1}, a_{2}, \ldots, a_{n}$, respectively, and we have
$$
Q M \geq A M \geq G M \geq H M
$$

Equalities occur if and only if $a_{1}=a_{2}=\cdots=a_{n}$.

Theorem 2 (Category: Cauchy-Schwarz Inequality, Nicknames: cauchy-schwarz inequality): Let $a_{1}, a_{2}, \ldots, a_{n}$ and $b_{1}, b_{2}$, $\ldots, b_{n}$ be real numbers. Then we have
$$
\left(\sum_{i=1}^{n} a_{i}^{2}\right)\left(\sum_{i=1}^{n} b_{i}^{2}\right) \geq\left(\sum_{i=1}^{n} a_{i} b_{i}\right)^{2}
$$
i.e.
$$
\left(a_{1}^{2}+a_{2}^{2}+\cdots+a_{n}^{2}\right)\left(b_{1}^{2}+b_{2}^{2}+\cdots+b_{n}^{2}\right) \geq\left(a_{1} b_{1}+a_{2} b_{2}+\cdots+a_{n} b_{n}\right)^{2}
$$

Equality occurs if and only if the sequences $\left(a_{1}, a_{2}, \ldots, a_{n}\right)$ and $\left(b_{1}, b_{2}\right.$, $\ldots, b_{n}$ ) are proportional, i.e. $\frac{a_{1}}{b_{1}}=\frac{a_{2}}{b_{2}}=\cdots=\frac{a_{n}}{b_{n}}$.

Theorem 3 (Category: Inequality Between Means, Nicknames: am-gm (arithmetic mean-geometric mean) inequality, am-gm): If $a_{1}, a_{2}, \ldots, a_{n}$ are nonnegative real numbers, then

$$
\frac{1}{n} \sum_{i=1}^{n} a_{i} \geq\left(a_{1} a_{2} \ldots a_{n}\right)^{\frac{1}{n}}
$$

with equality if and only if $a_{1}=a_{2}=\ldots=a_{n}$. This inequality is a special case of the Power Mean Inequality.

Solution:

## Response

To solve the inequality 

\[
\sum_{cyc} \frac{a}{a+2} \quad () \quad 1
\]

given the condition \( a^2 + b^2 + c^2 = 3 \) and \( a, b, c \geq 0 \), we will analyze the expression \( \frac{a}{a+2} \).

### Step 1: Analyze the function \( f(x) = \frac{x}{x+2} \)

The function \( f(x) = \frac{x}{x+2} \) is increasing for \( x \geq 0 \). This can be verified by computing its derivative:

\[
f'(x) = \frac{(x+2)(1) - x(1)}{(x+2)^2} = \frac{2}{(x+2)^2} > 0 \quad \text{for } x \geq 0.
\]

### Step 2: Apply Cauchy-Schwarz Inequality

Using the Cauchy-Schwarz inequality, we can estimate the sum:

\[
\sum_{cyc} \frac{a}{a+2} = \sum_{cyc} \frac{a^2}{a^2 + 2a}.
\]

Applying Cauchy-Schwarz:

\[
\left( \sum_{cyc} \frac{a^2}{a^2 + 2a} \right) \left( \sum_{cyc} (a^2 + 2a) \right) \geq \left( \sum_{cyc} a \right)^2.
\]

Calculating \( \sum_{cyc} (a^2 + 2a) \):

\[
\sum_{cyc} (a^2 + 2a) = (a^2 + b^2 + c^2) + 2(a + b + c) = 3 + 2(a + b + c).
\]

Thus, we have:

\[
\left( \sum_{cyc} \frac{a^2}{a^2 + 2a} \right) (3 + 2(a + b + c)) \geq (a + b + c)^2.
\]

### Step 3: Bound \( a + b + c \)

Using the Cauchy-Schwarz inequality again, we have:

\[
(a + b + c)^2 \leq 3(a^2 + b^2 + c^2) = 3 \cdot 3 = 9.
\]

Thus, \( a + b + c \leq 3 \).

### Step 4: Substitute back into the inequality

Now substituting back, we have:

\[
\left( \sum_{cyc} \frac{a^2}{a^2 + 2a} \right) (3 + 2(a + b + c)) \geq (a + b + c)^2 \leq 9.
\]

This gives us:

\[
\sum_{cyc} \frac{a^2}{a^2 + 2a} \geq \frac{(a + b + c)^2}{3 + 2(a + b + c)}.
\]

### Step 5: Evaluate the limit

To find the maximum of \( \sum_{cyc} \frac{a}{a+2} \), we can consider the case when \( a = b = c = 1 \):

\[
\sum_{cyc} \frac{1}{1+2} = 3 \cdot \frac{1}{3} = 1.
\]

### Conclusion

Since we have shown that \( \sum_{cyc} \frac{a}{a+2} \) can reach 1 and is bounded above by 1, we conclude that:

\[
\sum_{cyc} \frac{a}{a+2} \leq 1.
\]

Thus, the correct inequality relation to fill in the blank is:

\[
\sum_{cyc} \frac{a}{a+2} \leq 1.
\]

Therefore, the answer is:

The answer is (A) $\leq$.