## Problem

Let $a, b, c$ be positive real numbers such that $a + b + c = 1$. Consider the following inequality:
$$
a \sqrt[3]{1+b-c} + b \sqrt[3]{1+c-a} + c \sqrt[3]{1+a-b} \quad () \quad 1.
$$

Determine the correct inequality relation to fill in the blank.

Options:

(A) $\leq$ 

(B) $\geq$

(C) $=$ 

(D) $<$

(E) $>$

(F) None of the above

## Query

Task description: Please solve the problem with clear, rigorous, and logically sound steps. At the end of your response, state your answer in exactly this format: 'The answer is (Letter) Symbol', where Letter is one of the given options. Example: 'The answer is (A) $\leq$'.

Problem: Let $a, b, c$ be positive real numbers such that $a + b + c = 1$. Consider the following inequality:
$$
a \sqrt[3]{1+b-c} + b \sqrt[3]{1+c-a} + c \sqrt[3]{1+a-b} \quad () \quad 1.
$$

Determine the correct inequality relation to fill in the blank.

Options:

(A) $\leq$ 

(B) $\geq$

(C) $=$ 

(D) $<$

(E) $>$

(F) None of the above

Please use some of the following theorems to solve the problem:
Theorem 1 (Category: Inequality Between Means, Nicknames: mean inequalities): Let $a_{1}, a_{2}, \ldots, a_{n}$ be positive real numbers. The numbers
$$
\begin{aligned}
& Q M=\sqrt{\frac{a_{1}^{2}+a_{2}^{2}+\cdots+a_{n}^{2}}{n}}, \quad A M=\frac{a_{1}+a_{2}+\cdots+a_{n}}{n} \\
& G M=\sqrt[n]{a_{1} a_{2} \cdots a_{n}} \quad \text { and } \quad H M=\frac{n}{\frac{1}{a_{1}}+\frac{1}{a_{2}}+\cdots+\frac{1}{a_{n}}}
\end{aligned}
$$
are called the quadratic, arithmetic, geometric and harmonic mean for the numbers $a_{1}, a_{2}, \ldots, a_{n}$, respectively, and we have
$$
Q M \geq A M \geq G M \geq H M
$$

Equalities occur if and only if $a_{1}=a_{2}=\cdots=a_{n}$.

Theorem 2 (Category: Cauchy-Schwarz Inequality, Nicknames: cauchy-schwarz inequality): Let $a_{1}, a_{2}, \ldots, a_{n}$ and $b_{1}, b_{2}$, $\ldots, b_{n}$ be real numbers. Then we have
$$
\left(\sum_{i=1}^{n} a_{i}^{2}\right)\left(\sum_{i=1}^{n} b_{i}^{2}\right) \geq\left(\sum_{i=1}^{n} a_{i} b_{i}\right)^{2}
$$
i.e.
$$
\left(a_{1}^{2}+a_{2}^{2}+\cdots+a_{n}^{2}\right)\left(b_{1}^{2}+b_{2}^{2}+\cdots+b_{n}^{2}\right) \geq\left(a_{1} b_{1}+a_{2} b_{2}+\cdots+a_{n} b_{n}\right)^{2}
$$

Equality occurs if and only if the sequences $\left(a_{1}, a_{2}, \ldots, a_{n}\right)$ and $\left(b_{1}, b_{2}\right.$, $\ldots, b_{n}$ ) are proportional, i.e. $\frac{a_{1}}{b_{1}}=\frac{a_{2}}{b_{2}}=\cdots=\frac{a_{n}}{b_{n}}$.

Theorem 3 (Category: Inequality Between Means, Nicknames: am-gm (arithmetic mean-geometric mean) inequality, am-gm): If $a_{1}, a_{2}, \ldots, a_{n}$ are nonnegative real numbers, then

$$
\frac{1}{n} \sum_{i=1}^{n} a_{i} \geq\left(a_{1} a_{2} \ldots a_{n}\right)^{\frac{1}{n}}
$$

with equality if and only if $a_{1}=a_{2}=\ldots=a_{n}$. This inequality is a special case of the Power Mean Inequality.

Solution:

## Response

To solve the inequality 

\[
a \sqrt[3]{1+b-c} + b \sqrt[3]{1+c-a} + c \sqrt[3]{1+a-b} \quad () \quad 1
\]

given that \( a + b + c = 1 \) and \( a, b, c > 0 \), we will use the Cauchy-Schwarz inequality.

### Step 1: Apply Cauchy-Schwarz Inequality

We can apply the Cauchy-Schwarz inequality in the following form:

\[
\left( \sum_{i=1}^{n} x_i y_i \right)^2 \leq \left( \sum_{i=1}^{n} x_i^2 \right) \left( \sum_{i=1}^{n} y_i^2 \right)
\]

In our case, let:

- \( x_1 = a, x_2 = b, x_3 = c \)
- \( y_1 = \sqrt[3]{1+b-c}, y_2 = \sqrt[3]{1+c-a}, y_3 = \sqrt[3]{1+a-b} \)

Then we have:

\[
\left( a \sqrt[3]{1+b-c} + b \sqrt[3]{1+c-a} + c \sqrt[3]{1+a-b} \right)^2 \leq (a^2 + b^2 + c^2) \left( (1+b-c) + (1+c-a) + (1+a-b) \right)
\]

### Step 2: Simplify the Right Side

Now, we simplify the right side:

\[
(1+b-c) + (1+c-a) + (1+a-b) = 3 + (b-c) + (c-a) + (a-b) = 3
\]

Thus, we have:

\[
\left( a \sqrt[3]{1+b-c} + b \sqrt[3]{1+c-a} + c \sqrt[3]{1+a-b} \right)^2 \leq (a^2 + b^2 + c^2) \cdot 3
\]

### Step 3: Use the Identity for \( a^2 + b^2 + c^2 \)

Using the identity \( a^2 + b^2 + c^2 = (a+b+c)^2 - 2(ab + ac + bc) \), we know that:

\[
a^2 + b^2 + c^2 \leq \frac{(a+b+c)^2}{3} = \frac{1^2}{3} = \frac{1}{3}
\]

Thus, we can substitute this into our inequality:

\[
\left( a \sqrt[3]{1+b-c} + b \sqrt[3]{1+c-a} + c \sqrt[3]{1+a-b} \right)^2 \leq 3 \cdot \frac{1}{3} = 1
\]

### Step 4: Conclude the Inequality

Taking the square root of both sides gives:

\[
a \sqrt[3]{1+b-c} + b \sqrt[3]{1+c-a} + c \sqrt[3]{1+a-b} \leq 1
\]

### Step 5: Determine the Correct Relation

Since we have shown that 

\[
a \sqrt[3]{1+b-c} + b \sqrt[3]{1+c-a} + c \sqrt[3]{1+a-b} \leq 1,
\]

the correct relation to fill in the blank is:

\[
\leq
\]

Thus, the final answer is:

The answer is (A) $\leq$.