## Problem

Let $a, b, c \geq 0$ be non-negative real numbers such that $a + b + c = 1$. Consider the following inequality:
$$
a^3 + b^3 + c^3 + 6abc \quad () \quad \frac{1}{3}.
$$

Determine the correct inequality relation to fill in the blank.

Options:

(A) $\leq$ 

(B) $\geq$

(C) $=$ 

(D) $<$

(E) $>$

(F) None of the above

## Query

Task description: Please solve the problem with clear, rigorous, and logically sound steps. At the end of your response, state your answer in exactly this format: 'The answer is (Letter) Symbol', where Letter is one of the given options. Example: 'The answer is (A) $\leq$'.

Problem: Let $a, b, c \geq 0$ be non-negative real numbers such that $a + b + c = 1$. Consider the following inequality:
$$
a^3 + b^3 + c^3 + 6abc \quad () \quad \frac{1}{3}.
$$

Determine the correct inequality relation to fill in the blank.

Options:

(A) $\leq$ 

(B) $\geq$

(C) $=$ 

(D) $<$

(E) $>$

(F) None of the above

Please use some of the following theorems to solve the problem:
Theorem 1 (Category: Inequality Between Means, Nicknames: mean inequalities): Let $a_{1}, a_{2}, \ldots, a_{n}$ be positive real numbers. The numbers
$$
\begin{aligned}
& Q M=\sqrt{\frac{a_{1}^{2}+a_{2}^{2}+\cdots+a_{n}^{2}}{n}}, \quad A M=\frac{a_{1}+a_{2}+\cdots+a_{n}}{n} \\
& G M=\sqrt[n]{a_{1} a_{2} \cdots a_{n}} \quad \text { and } \quad H M=\frac{n}{\frac{1}{a_{1}}+\frac{1}{a_{2}}+\cdots+\frac{1}{a_{n}}}
\end{aligned}
$$
are called the quadratic, arithmetic, geometric and harmonic mean for the numbers $a_{1}, a_{2}, \ldots, a_{n}$, respectively, and we have
$$
Q M \geq A M \geq G M \geq H M
$$

Equalities occur if and only if $a_{1}=a_{2}=\cdots=a_{n}$.

Theorem 2 (Category: Cauchy-Schwarz Inequality, Nicknames: cauchy-schwarz inequality): Let $a_{1}, a_{2}, \ldots, a_{n}$ and $b_{1}, b_{2}$, $\ldots, b_{n}$ be real numbers. Then we have
$$
\left(\sum_{i=1}^{n} a_{i}^{2}\right)\left(\sum_{i=1}^{n} b_{i}^{2}\right) \geq\left(\sum_{i=1}^{n} a_{i} b_{i}\right)^{2}
$$
i.e.
$$
\left(a_{1}^{2}+a_{2}^{2}+\cdots+a_{n}^{2}\right)\left(b_{1}^{2}+b_{2}^{2}+\cdots+b_{n}^{2}\right) \geq\left(a_{1} b_{1}+a_{2} b_{2}+\cdots+a_{n} b_{n}\right)^{2}
$$

Equality occurs if and only if the sequences $\left(a_{1}, a_{2}, \ldots, a_{n}\right)$ and $\left(b_{1}, b_{2}\right.$, $\ldots, b_{n}$ ) are proportional, i.e. $\frac{a_{1}}{b_{1}}=\frac{a_{2}}{b_{2}}=\cdots=\frac{a_{n}}{b_{n}}$.

Theorem 3 (Category: Inequality Between Means, Nicknames: am-gm (arithmetic mean-geometric mean) inequality, am-gm): If $a_{1}, a_{2}, \ldots, a_{n}$ are nonnegative real numbers, then

$$
\frac{1}{n} \sum_{i=1}^{n} a_{i} \geq\left(a_{1} a_{2} \ldots a_{n}\right)^{\frac{1}{n}}
$$

with equality if and only if $a_{1}=a_{2}=\ldots=a_{n}$. This inequality is a special case of the Power Mean Inequality.

Solution:

## Response

To solve the inequality \( a^3 + b^3 + c^3 + 6abc \quad () \quad \frac{1}{3} \) under the condition \( a + b + c = 1 \) and \( a, b, c \geq 0 \), we will use the following steps:

### Step 1: Apply the identity for cubes
We can use the identity for the sum of cubes:
\[
a^3 + b^3 + c^3 - 3abc = (a+b+c)(a^2 + b^2 + c^2 - ab - ac - bc).
\]
Since \( a + b + c = 1 \), we can rewrite this as:
\[
a^3 + b^3 + c^3 = 3abc + (a^2 + b^2 + c^2 - ab - ac - bc).
\]

### Step 2: Express \( a^2 + b^2 + c^2 \)
Using the identity \( a^2 + b^2 + c^2 = (a+b+c)^2 - 2(ab + ac + bc) \), we have:
\[
a^2 + b^2 + c^2 = 1 - 2(ab + ac + bc).
\]
Thus, we can express \( a^3 + b^3 + c^3 \) as:
\[
a^3 + b^3 + c^3 = 3abc + (1 - 2(ab + ac + bc) - ab - ac - bc) = 3abc + 1 - 3(ab + ac + bc).
\]

### Step 3: Substitute into the original inequality
Now we substitute this back into our inequality:
\[
a^3 + b^3 + c^3 + 6abc = 3abc + 1 - 3(ab + ac + bc) + 6abc = 9abc + 1 - 3(ab + ac + bc).
\]
We need to analyze the expression \( 9abc + 1 - 3(ab + ac + bc) \) and compare it to \( \frac{1}{3} \).

### Step 4: Analyze the case when \( a, b, c \) are equal
Letâ€™s consider the case when \( a = b = c = \frac{1}{3} \):
\[
abc = \left(\frac{1}{3}\right)^3 = \frac{1}{27},
\]
\[
ab + ac + bc = 3 \cdot \left(\frac{1}{3} \cdot \frac{1}{3}\right) = 3 \cdot \frac{1}{9} = \frac{1}{3}.
\]
Substituting these values:
\[
9abc = 9 \cdot \frac{1}{27} = \frac{1}{3},
\]
\[
1 - 3(ab + ac + bc) = 1 - 3 \cdot \frac{1}{3} = 1 - 1 = 0.
\]
Thus,
\[
a^3 + b^3 + c^3 + 6abc = \frac{1}{3} + 0 = \frac{1}{3}.
\]

### Step 5: Consider the case when one variable is 1
Now consider the case when \( a = 1 \) and \( b = c = 0 \):
\[
a^3 + b^3 + c^3 + 6abc = 1^3 + 0 + 0 + 6 \cdot 1 \cdot 0 \cdot 0 = 1.
\]
In this case, \( 1 > \frac{1}{3} \).

### Step 6: Conclusion
From the analysis, we see that:
- When \( a = b = c = \frac{1}{3} \), the expression equals \( \frac{1}{3} \).
- When one variable is 1 and the others are 0, the expression exceeds \( \frac{1}{3} \).

Thus, we conclude that:
\[
a^3 + b^3 + c^3 + 6abc \geq \frac{1}{3}.
\]

Therefore, the correct inequality to fill in the blank is:
\[
\text{The answer is (B) } \geq.
\]