## Problem

Let $a, b > 0$ be positive real numbers such that $a + b \leq \frac{3}{2}$. Consider the following inequality:
$$
\frac{a}{2a^2+1} + \frac{4b}{3b^2+4} \quad () \quad \frac{7}{5}.
$$

Determine the correct inequality relation to fill in the blank.

Options:

(A) $\leq$ 

(B) $\geq$

(C) $=$ 

(D) $<$

(E) $>$

(F) None of the above

## Query

Task description: Please solve the problem with clear, rigorous, and logically sound steps. At the end of your response, state your answer in exactly this format: 'The answer is (Letter) Symbol', where Letter is one of the given options. Example: 'The answer is (A) $\leq$'.

Problem: Let $a, b > 0$ be positive real numbers such that $a + b \leq \frac{3}{2}$. Consider the following inequality:
$$
\frac{a}{2a^2+1} + \frac{4b}{3b^2+4} \quad () \quad \frac{7}{5}.
$$

Determine the correct inequality relation to fill in the blank.

Options:

(A) $\leq$ 

(B) $\geq$

(C) $=$ 

(D) $<$

(E) $>$

(F) None of the above

Please use some of the following theorems to solve the problem:
Theorem 1 (Category: Inequality Between Means, Nicknames: mean inequalities): Let $a_{1}, a_{2}, \ldots, a_{n}$ be positive real numbers. The numbers
$$
\begin{aligned}
& Q M=\sqrt{\frac{a_{1}^{2}+a_{2}^{2}+\cdots+a_{n}^{2}}{n}}, \quad A M=\frac{a_{1}+a_{2}+\cdots+a_{n}}{n} \\
& G M=\sqrt[n]{a_{1} a_{2} \cdots a_{n}} \quad \text { and } \quad H M=\frac{n}{\frac{1}{a_{1}}+\frac{1}{a_{2}}+\cdots+\frac{1}{a_{n}}}
\end{aligned}
$$
are called the quadratic, arithmetic, geometric and harmonic mean for the numbers $a_{1}, a_{2}, \ldots, a_{n}$, respectively, and we have
$$
Q M \geq A M \geq G M \geq H M
$$

Equalities occur if and only if $a_{1}=a_{2}=\cdots=a_{n}$.

Theorem 2 (Category: Cauchy-Schwarz Inequality, Nicknames: cauchy-schwarz inequality): Let $a_{1}, a_{2}, \ldots, a_{n}$ and $b_{1}, b_{2}$, $\ldots, b_{n}$ be real numbers. Then we have
$$
\left(\sum_{i=1}^{n} a_{i}^{2}\right)\left(\sum_{i=1}^{n} b_{i}^{2}\right) \geq\left(\sum_{i=1}^{n} a_{i} b_{i}\right)^{2}
$$
i.e.
$$
\left(a_{1}^{2}+a_{2}^{2}+\cdots+a_{n}^{2}\right)\left(b_{1}^{2}+b_{2}^{2}+\cdots+b_{n}^{2}\right) \geq\left(a_{1} b_{1}+a_{2} b_{2}+\cdots+a_{n} b_{n}\right)^{2}
$$

Equality occurs if and only if the sequences $\left(a_{1}, a_{2}, \ldots, a_{n}\right)$ and $\left(b_{1}, b_{2}\right.$, $\ldots, b_{n}$ ) are proportional, i.e. $\frac{a_{1}}{b_{1}}=\frac{a_{2}}{b_{2}}=\cdots=\frac{a_{n}}{b_{n}}$.

Theorem 3 (Category: Inequality Between Means, Nicknames: am-gm (arithmetic mean-geometric mean) inequality, am-gm): If $a_{1}, a_{2}, \ldots, a_{n}$ are nonnegative real numbers, then

$$
\frac{1}{n} \sum_{i=1}^{n} a_{i} \geq\left(a_{1} a_{2} \ldots a_{n}\right)^{\frac{1}{n}}
$$

with equality if and only if $a_{1}=a_{2}=\ldots=a_{n}$. This inequality is a special case of the Power Mean Inequality.

Solution:

## Response

To solve the inequality 

\[
\frac{a}{2a^2+1} + \frac{4b}{3b^2+4} \quad () \quad \frac{7}{5}
\]

given the constraint \( a + b \leq \frac{3}{2} \) with \( a, b > 0 \), we will analyze each term separately and then combine the results.

### Step 1: Analyze the first term

Consider the term \( \frac{a}{2a^2 + 1} \). We will find its maximum value under the constraint \( a + b \leq \frac{3}{2} \).

To maximize \( \frac{a}{2a^2 + 1} \), we can use calculus. Let \( f(a) = \frac{a}{2a^2 + 1} \). We find the derivative:

\[
f'(a) = \frac{(2a^2 + 1)(1) - a(4a)}{(2a^2 + 1)^2} = \frac{2a^2 + 1 - 4a^2}{(2a^2 + 1)^2} = \frac{1 - 2a^2}{(2a^2 + 1)^2}
\]

Setting \( f'(a) = 0 \) gives \( 1 - 2a^2 = 0 \) or \( a^2 = \frac{1}{2} \), thus \( a = \frac{1}{\sqrt{2}} \).

Now we check the second derivative to confirm it's a maximum:

\[
f''(a) = \text{(complex expression, but we can check the sign)}.
\]

Instead, we can evaluate \( f(a) \) at the endpoints of the interval defined by \( a + b \leq \frac{3}{2} \).

1. If \( a = \frac{3}{2} \) and \( b = 0 \):
   \[
   f\left(\frac{3}{2}\right) = \frac{\frac{3}{2}}{2\left(\frac{3}{2}\right)^2 + 1} = \frac{\frac{3}{2}}{2 \cdot \frac{9}{4} + 1} = \frac{\frac{3}{2}}{\frac{18}{4} + 1} = \frac{\frac{3}{2}}{\frac{22}{4}} = \frac{3 \cdot 4}{2 \cdot 22} = \frac{6}{11}.
   \]

2. If \( a = 0 \) and \( b = \frac{3}{2} \):
   \[
   f(0) = 0.
   \]

3. If \( a = \frac{1}{2} \) and \( b = 1 \):
   \[
   f\left(\frac{1}{2}\right) = \frac{\frac{1}{2}}{2\left(\frac{1}{2}\right)^2 + 1} = \frac{\frac{1}{2}}{2 \cdot \frac{1}{4} + 1} = \frac{\frac{1}{2}}{\frac{1}{2} + 1} = \frac{\frac{1}{2}}{\frac{3}{2}} = \frac{1}{3}.
   \]

### Step 2: Analyze the second term

Now consider \( \frac{4b}{3b^2 + 4} \). We will similarly find its maximum value.

Let \( g(b) = \frac{4b}{3b^2 + 4} \). The derivative is:

\[
g'(b) = \frac{(3b^2 + 4)(4) - 4b(6b)}{(3b^2 + 4)^2} = \frac{12b^2 + 16 - 24b^2}{(3b^2 + 4)^2} = \frac{-12b^2 + 16}{(3b^2 + 4)^2}.
\]

Setting \( g'(b) = 0 \) gives \( -12b^2 + 16 = 0 \) or \( b^2 = \frac{4}{3} \), thus \( b = \frac{2}{\sqrt{3}} \).

We check the values at the endpoints:

1. If \( b = \frac{3}{2} \) and \( a = 0 \):
   \[
   g\left(\frac{3}{2}\right) = \frac{4 \cdot \frac{3}{2}}{3\left(\frac{3}{2}\right)^2 + 4} = \frac{6}{\frac{27}{4} + 4} = \frac{6}{\frac{27}{4} + \frac{16}{4}} = \frac{6}{\frac{43}{4}} = \frac{24}{43}.
   \]

2. If \( b = 0 \):
   \[
   g(0) = 0.
   \]

3. If \( b = 1 \) and \( a = \frac{1}{2} \):
   \[
   g(1) = \frac{4 \cdot 1}{3 \cdot 1^2 + 4} = \frac{4}{3 + 4} = \frac{4}{7}.
   \]

### Step 3: Combine results

Now we combine the maximum values found:

- Maximum of \( \frac{a}{2a^2 + 1} \) is \( \frac{6}{11} \).
- Maximum of \( \frac{4b}{3b^2 + 4} \) is \( \frac{4}{7} \).

Now we need to check if 

\[
\frac{6}{11} + \frac{4}{7} \quad () \quad \frac{7}{5}.
\]

Finding a common denominator for \( \frac{6}{11} + \frac{4}{7} \):

\[
\frac{6 \cdot 7 + 4 \cdot 11}{77} = \frac{42 + 44}{77} = \frac{86}{77}.
\]

Now we compare \( \frac{86}{77} \) with \( \frac{7}{5} \):

Converting \( \frac{7}{5} \) to a fraction with a denominator of 77:

\[
\frac{7 \cdot 77}{5 \cdot 77} = \frac{539}{385}.
\]

Now we compare \( \frac{86}{77} \) and \( \frac{539}{385} \):

Cross-multiplying gives:

\[
86 \cdot 385 \quad \text{and} \quad 539 \cdot 77.
\]

Calculating:

- \( 86 \cdot 385 = 33110 \)
- \( 539 \cdot 77 = 41401 \)

Since \( 33110 < 41401 \), we have 

\[
\frac{86}{77} < \frac{7}{5}.
\]

Thus, the correct inequality is 

\[
\frac{a}{2a^2 + 1} + \frac{4b}{3b^2 + 4} < \frac{7}{5}.
\]

### Conclusion

The answer is (D) $<$.