## Problem

Find the smallest constant $C$ such that for all real numbers $x$ and $y$, the following inequality holds:
$$
x^2 + x + y^2 + y + C \geq x y
$$

## Query

Task description: Please solve the problem with clear, rigorous, and logically sound steps. At the end of your response, state your answer in exactly this format: 'The answer is $C=X$', where X is your calculated numerical bound value. Example: 'The answer is $C=1$'.

Problem: Find the smallest constant $C$ such that for all real numbers $x$ and $y$, the following inequality holds:
$$
x^2 + x + y^2 + y + C \geq x y
$$

Solution:

## Response

To find the smallest constant \( C \) such that the inequality 

\[
x^2 + x + y^2 + y + C \geq xy
\]

holds for all real numbers \( x \) and \( y \), we can rearrange the inequality as follows:

\[
x^2 - xy + y^2 + x + y + C \geq 0.
\]

This is a quadratic expression in terms of \( x \):

\[
x^2 - xy + (y^2 + x + y + C) \geq 0.
\]

For this quadratic in \( x \) to be non-negative for all \( x \), the discriminant must be non-positive. The discriminant \( D \) of the quadratic \( ax^2 + bx + c \) is given by \( D = b^2 - 4ac \). Here, we have:

- \( a = 1 \)
- \( b = -y \)
- \( c = y^2 + x + y + C \)

Thus, the discriminant is:

\[
D = (-y)^2 - 4(1)(y^2 + x + y + C) = y^2 - 4(y^2 + x + y + C).
\]

Simplifying this, we get:

\[
D = y^2 - 4y^2 - 4x - 4y - 4C = -3y^2 - 4x - 4y - 4C.
\]

For the quadratic to be non-negative for all \( x \), we require:

\[
-3y^2 - 4y - 4C \leq 0 \quad \text{for all } y.
\]

This is a quadratic in \( y \) with coefficients:

- \( a = -3 \)
- \( b = -4 \)
- \( c = -4C \)

The discriminant of this quadratic must be non-positive:

\[
D_y = (-4)^2 - 4(-3)(-4C) = 16 - 12C.
\]

Setting the discriminant \( D_y \leq 0 \) gives:

\[
16 - 12C \leq 0.
\]

Solving for \( C \):

\[
16 \leq 12C \implies C \geq \frac{16}{12} = \frac{4}{3}.
\]

Thus, the smallest constant \( C \) that satisfies the inequality for all \( x \) and \( y \) is 

\[
C = \frac{4}{3}.
\]

To verify, we can substitute \( C = \frac{4}{3} \) back into the original inequality and check if it holds for various values of \( x \) and \( y \). 

Therefore, the answer is 

\[
\text{The answer is } C = \frac{4}{3}.
\]