## Problem

Let $x, y, z \in [0,1]$. Determine the minimal constant $C$ such that the following inequality holds for all $x, y, z$:
$$
x(x-y)(z-x) \leq C.
$$

## Query

Task description: Please solve the problem with clear, rigorous, and logically sound steps. At the end of your response, state your answer in exactly this format: 'The answer is $C=X$', where X is your calculated numerical bound value. Example: 'The answer is $C=1$'.

Problem: Let $x, y, z \in [0,1]$. Determine the minimal constant $C$ such that the following inequality holds for all $x, y, z$:
$$
x(x-y)(z-x) \leq C.
$$

Solution:

## Response

To solve the problem, we need to analyze the expression \( x(x-y)(z-x) \) for \( x, y, z \in [0, 1] \) and find the minimal constant \( C \) such that the inequality holds for all possible values of \( x, y, z \) in that range.

1. **Understanding the Expression**:
   The expression \( x(x-y)(z-x) \) can be broken down as follows:
   - \( x \) is a factor that scales the entire expression and is bounded between 0 and 1.
   - \( (x-y) \) can be positive or negative depending on the values of \( x \) and \( y \).
   - \( (z-x) \) can also be positive or negative depending on the values of \( z \) and \( x \).

2. **Finding Critical Points**:
   We will analyze the expression by considering the boundaries of the variables \( x, y, z \) in the interval \([0, 1]\).

   - **Case 1**: Let \( x = 0 \):
     \[
     0(0-y)(z-0) = 0.
     \]

   - **Case 2**: Let \( x = 1 \):
     \[
     1(1-y)(z-1) = (1-y)(z-1).
     \]
     Here, \( (1-y) \) is non-negative when \( y \leq 1 \) and \( (z-1) \) is non-positive when \( z \leq 1 \). Thus, this expression is non-positive and does not exceed 0.

   - **Case 3**: Let \( y = 0 \):
     \[
     x(x-0)(z-x) = x^2(z-x).
     \]
     This expression is non-negative for \( x \in [0, 1] \) and \( z \in [0, 1] \).

   - **Case 4**: Let \( z = 0 \):
     \[
     x(x-y)(0-x) = -x^2(x-y).
     \]
     This expression is non-positive when \( x \geq y \) and non-negative when \( x < y \).

3. **Maximizing the Expression**:
   To find the maximum value of \( x(x-y)(z-x) \), we can consider specific values of \( x, y, z \):
   - Let \( x = 1 \), \( y = 0 \), and \( z = 1 \):
     \[
     1(1-0)(1-1) = 1 \cdot 1 \cdot 0 = 0.
     \]
   - Let \( x = 1 \), \( y = 1 \), and \( z = 1 \):
     \[
     1(1-1)(1-1) = 0.
     \]
   - Let \( x = 0.5 \), \( y = 0 \), and \( z = 1 \):
     \[
     0.5(0.5-0)(1-0.5) = 0.5 \cdot 0.5 \cdot 0.5 = 0.125.
     \]

4. **Finding the Maximum Value**:
   We can also check the case where \( x = 0.5 \), \( y = 0.5 \), and \( z = 1 \):
   \[
   0.5(0.5-0.5)(1-0.5) = 0.5 \cdot 0 \cdot 0.5 = 0.
   \]
   The maximum value we have found so far is \( 0.125 \).

5. **Conclusion**:
   After checking various combinations of \( x, y, z \) in the interval \([0, 1]\), we find that the maximum value of \( x(x-y)(z-x) \) does not exceed \( 0.125 \). Therefore, the minimal constant \( C \) such that the inequality holds for all \( x, y, z \in [0, 1] \) is \( 0.125 \).

Thus, the answer is \( C = 0.125 \).

The answer is \( C = 0.125 \).