## Problem

Let $a, b, c \geq 0$ and $a^2 + b + c^2 = 1$. Determine the largest constant $C$ such that the following inequality holds for all $a, b, c$:

$$
\frac{1}{1+a^2} + \frac{1}{3(1+b)} + \frac{1}{1+c^2} \geq C.
$$

## Query

Task description: Please solve the problem with clear, rigorous, and logically sound steps. At the end of your response, state your answer in exactly this format: 'The answer is $C=X$', where X is your calculated numerical bound value. Example: 'The answer is $C=1$'.

Problem: Let $a, b, c \geq 0$ and $a^2 + b + c^2 = 1$. Determine the largest constant $C$ such that the following inequality holds for all $a, b, c$:

$$
\frac{1}{1+a^2} + \frac{1}{3(1+b)} + \frac{1}{1+c^2} \geq C.
$$

Solution:

## Response

To solve the problem, we need to find the largest constant \( C \) such that the inequality 

\[
\frac{1}{1+a^2} + \frac{1}{3(1+b)} + \frac{1}{1+c^2} \geq C
\]

holds for all non-negative \( a, b, c \) satisfying the constraint \( a^2 + b + c^2 = 1 \).

### Step 1: Analyze the terms

We will analyze each term in the inequality separately.

1. **Term \( \frac{1}{1+a^2} \)**:
   - Since \( a^2 \geq 0 \), we have \( 1 + a^2 \geq 1 \), thus \( \frac{1}{1+a^2} \leq 1 \).
   - The maximum value occurs when \( a = 0 \), giving \( \frac{1}{1+0^2} = 1 \).

2. **Term \( \frac{1}{3(1+b)} \)**:
   - Since \( b \geq 0 \), we have \( 1 + b \geq 1 \), thus \( \frac{1}{3(1+b)} \leq \frac{1}{3} \).
   - The maximum value occurs when \( b = 0 \), giving \( \frac{1}{3(1+0)} = \frac{1}{3} \).

3. **Term \( \frac{1}{1+c^2} \)**:
   - Similar to the first term, since \( c^2 \geq 0 \), we have \( 1 + c^2 \geq 1 \), thus \( \frac{1}{1+c^2} \leq 1 \).
   - The maximum value occurs when \( c = 0 \), giving \( \frac{1}{1+0^2} = 1 \).

### Step 2: Consider the constraint

Given the constraint \( a^2 + b + c^2 = 1 \), we can explore specific cases to find the minimum value of the left-hand side of the inequality.

### Step 3: Test specific cases

1. **Case 1: \( a = 1, b = 0, c = 0 \)**:
   \[
   \frac{1}{1+1^2} + \frac{1}{3(1+0)} + \frac{1}{1+0^2} = \frac{1}{2} + \frac{1}{3} + 1 = \frac{1}{2} + \frac{1}{3} + 1 = \frac{3}{6} + \frac{2}{6} + \frac{6}{6} = \frac{11}{6}.
   \]

2. **Case 2: \( a = 0, b = 1, c = 0 \)**:
   \[
   \frac{1}{1+0^2} + \frac{1}{3(1+1)} + \frac{1}{1+0^2} = 1 + \frac{1}{6} + 1 = 2 + \frac{1}{6} = \frac{12}{6} + \frac{1}{6} = \frac{13}{6}.
   \]

3. **Case 3: \( a = 0, b = 0, c = 1 \)**:
   \[
   \frac{1}{1+0^2} + \frac{1}{3(1+0)} + \frac{1}{1+1^2} = 1 + \frac{1}{3} + \frac{1}{2} = 1 + \frac{2}{6} + \frac{3}{6} = 1 + \frac{5}{6} = \frac{11}{6}.
   \]

4. **Case 4: \( a = 0, b = 0, c = 1 \)**:
   \[
   \frac{1}{1+0^2} + \frac{1}{3(1+0)} + \frac{1}{1+1^2} = 1 + \frac{1}{3} + \frac{1}{2} = 1 + \frac{2}{6} + \frac{3}{6} = 1 + \frac{5}{6} = \frac{11}{6}.
   \]

### Step 4: Find the minimum value

From the cases tested, the minimum value of the left-hand side occurs in Case 1 and Case 3, yielding \( \frac{11}{6} \) as the minimum value.

### Conclusion

Thus, the largest constant \( C \) such that the inequality holds for all \( a, b, c \) satisfying the constraint is 

\[
C = \frac{11}{6}.
\]

Therefore, the final answer is:

\[
\text{The answer is } C = \frac{11}{6}.
\]