## Problem

Let $a, b, c \geq 0$ be non-negative real numbers such that $a + b + c = 1$. Consider the following inequality:
$$
7(ab + bc + ca) \quad () \quad 3 + 9abc.
$$

Determine the correct inequality relation to fill in the blank.

Options:

(A) $\leq$ 

(B) $\geq$

(C) $=$ 

(D) $<$

(E) $>$

(F) None of the above

## Query

Task description: Please solve the problem with clear, rigorous, and logically sound steps. At the end of your response, state your answer in exactly this format: 'The answer is (Letter) Symbol', where Letter is one of the given options. Example: 'The answer is (A) $\leq$'.

Problem: Let $a, b, c \geq 0$ be non-negative real numbers such that $a + b + c = 1$. Consider the following inequality:
$$
7(ab + bc + ca) \quad () \quad 3 + 9abc.
$$

Determine the correct inequality relation to fill in the blank.

Options:

(A) $\leq$ 

(B) $\geq$

(C) $=$ 

(D) $<$

(E) $>$

(F) None of the above

Solution:

## Response

To solve the inequality \( 7(ab + bc + ca) \quad () \quad 3 + 9abc \) under the condition \( a + b + c = 1 \) with \( a, b, c \geq 0 \), we will analyze both sides of the inequality.

First, we can express \( ab + bc + ca \) in terms of \( a, b, c \). Using the identity:

\[
(ab + bc + ca) = \frac{(a+b+c)^2 - (a^2 + b^2 + c^2)}{2}
\]

Since \( a + b + c = 1 \), we have:

\[
(ab + bc + ca) = \frac{1^2 - (a^2 + b^2 + c^2)}{2} = \frac{1 - (a^2 + b^2 + c^2)}{2}
\]

Next, we can express \( abc \) in terms of \( a, b, c \). The maximum value of \( abc \) occurs when \( a, b, c \) are as equal as possible, given the constraint \( a + b + c = 1 \). The maximum occurs at \( a = b = c = \frac{1}{3} \):

\[
abc = \left(\frac{1}{3}\right)\left(\frac{1}{3}\right)\left(\frac{1}{3}\right) = \frac{1}{27}
\]

Now, we will analyze the left-hand side \( 7(ab + bc + ca) \):

1. **Finding the maximum of \( ab + bc + ca \)**:
   - If \( a = b = c = \frac{1}{3} \):
   \[
   ab + bc + ca = 3 \cdot \left(\frac{1}{3} \cdot \frac{1}{3}\right) = 3 \cdot \frac{1}{9} = \frac{1}{3}
   \]

   - Therefore, the maximum value of \( 7(ab + bc + ca) \) is:
   \[
   7 \cdot \frac{1}{3} = \frac{7}{3}
   \]

2. **Finding the maximum of \( 3 + 9abc \)**:
   - Using \( abc = \frac{1}{27} \):
   \[
   9abc = 9 \cdot \frac{1}{27} = \frac{1}{3}
   \]
   - Thus, the maximum value of \( 3 + 9abc \) is:
   \[
   3 + \frac{1}{3} = \frac{10}{3}
   \]

Now we compare the maximum values of both sides:

- The maximum of \( 7(ab + bc + ca) \) is \( \frac{7}{3} \).
- The maximum of \( 3 + 9abc \) is \( \frac{10}{3} \).

Since \( \frac{7}{3} < \frac{10}{3} \), we conclude that:

\[
7(ab + bc + ca) < 3 + 9abc
\]

Thus, the correct inequality to fill in the blank is:

The answer is (D) \( < \).