## Problem

Let $a, b, c \in (0,1)$. Consider the following inequality:
$$
\sqrt{a b c} + \sqrt{(1-a)(1-b)(1-c)} \quad () \quad 1.
$$

Determine the correct inequality relation to fill in the blank.

Options:

(A) $\leq$ 

(B) $\geq$

(C) $=$ 

(D) $<$

(E) $>$

(F) None of the above

## Query

Task description: Please solve the problem with clear, rigorous, and logically sound steps. At the end of your response, state your answer in exactly this format: 'The answer is (Letter) Symbol', where Letter is one of the given options. Example: 'The answer is (A) $\leq$'.

Problem: Let $a, b, c \in (0,1)$. Consider the following inequality:
$$
\sqrt{a b c} + \sqrt{(1-a)(1-b)(1-c)} \quad () \quad 1.
$$

Determine the correct inequality relation to fill in the blank.

Options:

(A) $\leq$ 

(B) $\geq$

(C) $=$ 

(D) $<$

(E) $>$

(F) None of the above

Solution:

## Response

To solve the problem, we need to analyze the expression 

\[
\sqrt{abc} + \sqrt{(1-a)(1-b)(1-c)}
\]

where \( a, b, c \in (0, 1) \).

### Step 1: Analyze the terms

1. **First term**: \( \sqrt{abc} \)
   - Since \( a, b, c \in (0, 1) \), it follows that \( abc \in (0, 1) \). Therefore, \( \sqrt{abc} \in (0, 1) \).

2. **Second term**: \( \sqrt{(1-a)(1-b)(1-c)} \)
   - Similarly, since \( 1-a, 1-b, 1-c \in (0, 1) \), we have \( (1-a)(1-b)(1-c) \in (0, 1) \). Thus, \( \sqrt{(1-a)(1-b)(1-c)} \in (0, 1) \).

### Step 2: Bound the sum

Both terms \( \sqrt{abc} \) and \( \sqrt{(1-a)(1-b)(1-c)} \) are positive and less than 1. Therefore, we can write:

\[
\sqrt{abc} + \sqrt{(1-a)(1-b)(1-c)} < 1 + 1 = 2
\]

However, we need to determine if the sum is less than, greater than, or equal to 1.

### Step 3: Consider extreme cases

1. **Case 1**: Let \( a = b = c = 0.5 \).
   - Then, \( \sqrt{abc} = \sqrt{0.5 \cdot 0.5 \cdot 0.5} = \sqrt{0.125} = \frac{\sqrt{2}}{4} \).
   - Also, \( \sqrt{(1-a)(1-b)(1-c)} = \sqrt{0.5 \cdot 0.5 \cdot 0.5} = \frac{\sqrt{2}}{4} \).
   - Thus, the sum is \( \frac{\sqrt{2}}{4} + \frac{\sqrt{2}}{4} = \frac{\sqrt{2}}{2} \approx 0.707 < 1 \).

2. **Case 2**: Let \( a = b = c \) approach 1 (e.g., \( a = b = c = 0.99 \)).
   - Then, \( \sqrt{abc} \approx \sqrt{0.970299} \approx 0.985 \).
   - Also, \( \sqrt{(1-a)(1-b)(1-c)} \approx \sqrt{(0.01)(0.01)(0.01)} = \sqrt{0.000001} = 0.001 \).
   - Thus, the sum is approximately \( 0.985 + 0.001 = 0.986 < 1 \).

3. **Case 3**: Let \( a = b = c \) approach 0 (e.g., \( a = b = c = 0.01 \)).
   - Then, \( \sqrt{abc} \approx \sqrt{0.000001} = 0.001 \).
   - Also, \( \sqrt{(1-a)(1-b)(1-c)} \approx \sqrt{(0.99)(0.99)(0.99)} \approx \sqrt{0.970299} \approx 0.985 \).
   - Thus, the sum is approximately \( 0.001 + 0.985 = 0.986 < 1 \).

### Conclusion

In all cases considered, the sum \( \sqrt{abc} + \sqrt{(1-a)(1-b)(1-c)} \) is always less than 1. Therefore, we conclude that:

\[
\sqrt{abc} + \sqrt{(1-a)(1-b)(1-c)} < 1
\]

Thus, the correct inequality to fill in the blank is:

The answer is (D) $<$.