## Problem

Let $a, b, c > 0$ be positive real numbers such that $\frac{1}{a} + \frac{1}{b} + \frac{1}{c} = \sqrt{abc}$. Consider the following inequality:
$$
abc \quad () \quad \sqrt{3(a+b+c)}.
$$
Determine the correct inequality relation to fill in the blank.

Options:

(A) $\leq$ 

(B) $\geq$

(C) $=$ 

(D) $<$

(E) $>$

(F) None of the above

## Query

Task description: Please solve the problem with clear, rigorous, and logically sound steps. At the end of your response, state your answer in exactly this format: 'The answer is (Letter) Symbol', where Letter is one of the given options. Example: 'The answer is (A) $\leq$'.

Problem: Let $a, b, c > 0$ be positive real numbers such that $\frac{1}{a} + \frac{1}{b} + \frac{1}{c} = \sqrt{abc}$. Consider the following inequality:
$$
abc \quad () \quad \sqrt{3(a+b+c)}.
$$
Determine the correct inequality relation to fill in the blank.

Options:

(A) $\leq$ 

(B) $\geq$

(C) $=$ 

(D) $<$

(E) $>$

(F) None of the above

Solution:

## Response

To solve the problem, we start with the given condition:

\[
\frac{1}{a} + \frac{1}{b} + \frac{1}{c} = \sqrt{abc}.
\]

This can be rewritten as:

\[
\frac{bc + ac + ab}{abc} = \sqrt{abc}.
\]

Multiplying both sides by \(abc\) (which is positive since \(a, b, c > 0\)), we obtain:

\[
bc + ac + ab = abc \sqrt{abc}.
\]

Next, we want to analyze the inequality:

\[
abc \quad () \quad \sqrt{3(a+b+c)}.
\]

To explore this inequality, we can apply the AM-GM inequality, which states that for any non-negative real numbers \(x_1, x_2, \ldots, x_n\):

\[
\frac{x_1 + x_2 + \ldots + x_n}{n} \geq \sqrt[n]{x_1 x_2 \ldots x_n}.
\]

Applying AM-GM to \(a, b, c\):

\[
\frac{a + b + c}{3} \geq \sqrt[3]{abc}.
\]

This implies:

\[
a + b + c \geq 3\sqrt[3]{abc}.
\]

Now, we can multiply both sides by \(\sqrt{3}\):

\[
\sqrt{3(a + b + c)} \geq \sqrt{3} \cdot 3\sqrt[3]{abc} = 3\sqrt{3}\sqrt[3]{abc}.
\]

Next, we need to relate \(abc\) to \(\sqrt{3(a+b+c)}\). We can use the condition we derived earlier. We know that:

\[
bc + ac + ab = abc \sqrt{abc}.
\]

Using the Cauchy-Schwarz inequality on \( (1, 1, 1) \) and \( (a, b, c) \):

\[
(1 + 1 + 1)(a + b + c) \geq (1 + 1 + 1)^2 = 9.
\]

Thus, we have:

\[
3(a + b + c) \geq 9 \implies a + b + c \geq 3.
\]

Now, we can analyze the inequality \(abc\) in relation to \(\sqrt{3(a+b+c)}\). 

Using the AM-GM inequality again, we have:

\[
\sqrt{3(a+b+c)} \geq 3\sqrt[3]{abc}.
\]

This suggests that \(abc\) is likely less than or equal to \(\sqrt{3(a+b+c)}\). 

To check if \(abc \leq \sqrt{3(a+b+c)}\) holds, we can consider the case when \(a = b = c\). Let \(a = b = c = k\):

\[
\frac{3}{k} = \sqrt{k^3} \implies 3 = k^{3/2} \implies k = \left(\frac{3}{1}\right)^{\frac{2}{3}} = 3^{2/3}.
\]

Then:

\[
abc = k^3 = (3^{2/3})^3 = 3^2 = 9,
\]
and

\[
\sqrt{3(a+b+c)} = \sqrt{3(3k)} = \sqrt{9k} = 3.
\]

Thus, we find that:

\[
abc = 9 \quad \text{and} \quad \sqrt{3(a+b+c)} = 3.
\]

This shows that \(abc\) can be greater than \(\sqrt{3(a+b+c)}\) in some cases, but we need to check if it can be equal or less.

After analyzing the conditions and applying inequalities, we conclude that:

\[
abc \geq \sqrt{3(a+b+c)}.
\]

Thus, the correct inequality to fill in the blank is:

\[
\text{The answer is (B) } \geq.
\]