## Problem

Let $a, b, c > 0$ be positive real numbers such that $ab + bc + ca = 1$. Consider the following inequality:
$$
a b c\left(a+\sqrt{a^2+1}\right)\left(b+\sqrt{b^2+1}\right)\left(c+\sqrt{c^2+1}\right) \quad () \quad 2.
$$

Determine the correct inequality relation to fill in the blank.

Options:

(A) $\leq$ 

(B) $\geq$

(C) $=$ 

(D) $<$

(E) $>$

(F) None of the above

## Query

Task description: Please solve the problem with clear, rigorous, and logically sound steps. At the end of your response, state your answer in exactly this format: 'The answer is (Letter) Symbol', where Letter is one of the given options. Example: 'The answer is (A) $\leq$'.

Problem: Let $a, b, c > 0$ be positive real numbers such that $ab + bc + ca = 1$. Consider the following inequality:
$$
a b c\left(a+\sqrt{a^2+1}\right)\left(b+\sqrt{b^2+1}\right)\left(c+\sqrt{c^2+1}\right) \quad () \quad 2.
$$

Determine the correct inequality relation to fill in the blank.

Options:

(A) $\leq$ 

(B) $\geq$

(C) $=$ 

(D) $<$

(E) $>$

(F) None of the above

Solution:

## Response

To solve the problem, we need to analyze the expression given in the inequality:

\[
abc\left(a+\sqrt{a^2+1}\right)\left(b+\sqrt{b^2+1}\right)\left(c+\sqrt{c^2+1}\right)
\]

and compare it to 2 under the condition \( ab + bc + ca = 1 \).

### Step 1: Analyze the terms

First, we note that for any positive real number \( x \), the term \( x + \sqrt{x^2 + 1} \) can be simplified. We can rewrite it as:

\[
x + \sqrt{x^2 + 1} = \sqrt{x^2 + 1} + x
\]

This expression is always greater than \( \sqrt{x^2 + 1} \) since \( x > 0 \).

### Step 2: Bound the terms

We can also analyze the term \( \sqrt{x^2 + 1} \):

\[
\sqrt{x^2 + 1} \geq 1 \quad \text{(since \( x^2 \geq 0 \))}
\]

Thus, we have:

\[
x + \sqrt{x^2 + 1} \geq x + 1
\]

### Step 3: Apply the condition

Given \( ab + bc + ca = 1 \), we can use the AM-GM inequality:

\[
\frac{ab + bc + ca}{3} \geq \sqrt[3]{(abc)^2}
\]

This implies:

\[
\frac{1}{3} \geq \sqrt[3]{(abc)^2} \implies abc \leq \frac{1}{\sqrt{3\sqrt{3}}} = \frac{1}{3\sqrt{3}} \approx 0.192
\]

### Step 4: Estimate the product

Now we need to estimate the product:

\[
\left(a + \sqrt{a^2 + 1}\right)\left(b + \sqrt{b^2 + 1}\right)\left(c + \sqrt{c^2 + 1}\right)
\]

Using the earlier bound, we can say:

\[
\left(a + \sqrt{a^2 + 1}\right) \geq \left(a + 1\right)
\]

Thus, we can estimate:

\[
\left(a + \sqrt{a^2 + 1}\right)\left(b + \sqrt{b^2 + 1}\right)\left(c + \sqrt{c^2 + 1}\right) \geq (a + 1)(b + 1)(c + 1)
\]

### Step 5: Combine the estimates

Now we can combine our estimates:

\[
abc\left(a+\sqrt{a^2+1}\right)\left(b+\sqrt{b^2+1}\right)\left(c+\sqrt{c^2+1}\right) \geq abc(a + 1)(b + 1)(c + 1)
\]

### Step 6: Check the inequality

To check if this is greater than or less than 2, we can consider specific values for \( a, b, c \) that satisfy \( ab + bc + ca = 1 \). 

For example, let \( a = b = c = \frac{1}{\sqrt{3}} \):

\[
ab + bc + ca = 3 \cdot \left(\frac{1}{\sqrt{3}}\right)^2 = 1
\]

Calculating \( abc \):

\[
abc = \left(\frac{1}{\sqrt{3}}\right)^3 = \frac{1}{3\sqrt{3}}
\]

Calculating \( a + \sqrt{a^2 + 1} \):

\[
a + \sqrt{a^2 + 1} = \frac{1}{\sqrt{3}} + \sqrt{\frac{1}{3} + 1} = \frac{1}{\sqrt{3}} + \sqrt{\frac{4}{3}} = \frac{1}{\sqrt{3}} + \frac{2}{\sqrt{3}} = \frac{3}{\sqrt{3}} = \sqrt{3}
\]

Thus, we have:

\[
abc \cdot \left(\sqrt{3}\right)^3 = \frac{1}{3\sqrt{3}} \cdot 3\sqrt{3} = 1
\]

Since \( 1 < 2 \), we conclude that:

\[
abc\left(a+\sqrt{a^2+1}\right)\left(b+\sqrt{b^2+1}\right)\left(c+\sqrt{c^2+1}\right) < 2
\]

### Conclusion

Thus, the correct inequality relation to fill in the blank is:

The answer is (D) $<$.