## Problem

Let $x, y, z$ be positive real numbers. Consider the following inequality:
$$
\left(\frac{2x}{y}+3\right)\left(\frac{3y}{z}+1\right)\left(\frac{z}{x}+1\right) \quad () \quad 2+\frac{2(x+y+z)}{\sqrt[3]{x y z}}.
$$

Determine the correct inequality relation to fill in the blank.

Options:

(A) $\leq$ 

(B) $\geq$

(C) $=$ 

(D) $<$

(E) $>$

(F) None of the above

## Query

Task description: Please solve the problem with clear, rigorous, and logically sound steps. At the end of your response, state your answer in exactly this format: 'The answer is (Letter) Symbol', where Letter is one of the given options. Example: 'The answer is (A) $\leq$'.

Problem: Let $x, y, z$ be positive real numbers. Consider the following inequality:
$$
\left(\frac{2x}{y}+3\right)\left(\frac{3y}{z}+1\right)\left(\frac{z}{x}+1\right) \quad () \quad 2+\frac{2(x+y+z)}{\sqrt[3]{x y z}}.
$$

Determine the correct inequality relation to fill in the blank.

Options:

(A) $\leq$ 

(B) $\geq$

(C) $=$ 

(D) $<$

(E) $>$

(F) None of the above

Solution:

## Response

To solve the inequality 

\[
\left(\frac{2x}{y}+3\right)\left(\frac{3y}{z}+1\right)\left(\frac{z}{x}+1\right) \quad () \quad 2+\frac{2(x+y+z)}{\sqrt[3]{x y z}},
\]

we will analyze both sides of the inequality step by step.

### Step 1: Analyze the left-hand side

We start with the left-hand side:

\[
L = \left(\frac{2x}{y}+3\right)\left(\frac{3y}{z}+1\right)\left(\frac{z}{x}+1\right).
\]

We can rewrite each term:

1. \(\frac{2x}{y} + 3\) can be seen as a sum of a positive term and a constant.
2. \(\frac{3y}{z} + 1\) is also a sum of a positive term and a constant.
3. \(\frac{z}{x} + 1\) follows the same pattern.

### Step 2: Apply AM-GM Inequality

Using the AM-GM inequality, we can estimate each term:

1. \(\frac{2x}{y} + 3 \geq 2\sqrt{2x \cdot 3y} = 2\sqrt{6xy}\).
2. \(\frac{3y}{z} + 1 \geq 2\sqrt{3y \cdot z} = 2\sqrt{3yz}\).
3. \(\frac{z}{x} + 1 \geq 2\sqrt{z \cdot x} = 2\sqrt{zx}\).

Thus, we have:

\[
L \geq (2\sqrt{6xy})(2\sqrt{3yz})(2\sqrt{zx}) = 8\sqrt{6 \cdot 3 \cdot (xyz)^2} = 24\sqrt{xyz}.
\]

### Step 3: Analyze the right-hand side

Now, we analyze the right-hand side:

\[
R = 2 + \frac{2(x+y+z)}{\sqrt[3]{xyz}}.
\]

Using the AM-GM inequality again, we have:

\[
x + y + z \geq 3\sqrt[3]{xyz}.
\]

Thus,

\[
\frac{2(x+y+z)}{\sqrt[3]{xyz}} \geq \frac{2 \cdot 3\sqrt[3]{xyz}}{\sqrt[3]{xyz}} = 6.
\]

So we can conclude:

\[
R \geq 2 + 6 = 8.
\]

### Step 4: Compare L and R

Now we need to compare \(L\) and \(R\). We have established:

- \(L \geq 24\sqrt{xyz}\)
- \(R \geq 8\)

To determine the relationship between \(L\) and \(R\), we need to consider specific cases. 

### Step 5: Test specific values

Letâ€™s test \(x = y = z = 1\):

- Then \(L = \left(\frac{2 \cdot 1}{1} + 3\right)\left(\frac{3 \cdot 1}{1} + 1\right)\left(\frac{1}{1} + 1\right) = (2 + 3)(3 + 1)(1 + 1) = 5 \cdot 4 \cdot 2 = 40\).
- And \(R = 2 + \frac{2(1 + 1 + 1)}{\sqrt[3]{1 \cdot 1 \cdot 1}} = 2 + \frac{2 \cdot 3}{1} = 2 + 6 = 8\).

In this case, \(L = 40\) and \(R = 8\), so \(L > R\).

### Conclusion

Since we have shown that \(L\) can be greater than \(R\) in specific cases, we can conclude that the inequality is:

\[
\left(\frac{2x}{y}+3\right)\left(\frac{3y}{z}+1\right)\left(\frac{z}{x}+1\right) \geq 2+\frac{2(x+y+z)}{\sqrt[3]{x y z}}.
\]

Thus, the correct option to fill in the blank is:

The answer is (B) $\geq$.