## Problem

Let $a, b, c$ be positive real numbers such that $abc = 1$. Consider the following inequality:
$$
\sum \frac{a(a^3+1)}{3b+c} \quad () \quad 2a^3 + b^3 + c^3.
$$

Determine the correct inequality relation to fill in the blank.

Options:

(A) $\leq$ 

(B) $\geq$

(C) $=$ 

(D) $<$

(E) $>$

(F) None of the above

## Query

Task description: Please solve the problem with clear, rigorous, and logically sound steps. At the end of your response, state your answer in exactly this format: 'The answer is (Letter) Symbol', where Letter is one of the given options. Example: 'The answer is (A) $\leq$'.

Problem: Let $a, b, c$ be positive real numbers such that $abc = 1$. Consider the following inequality:
$$
\sum \frac{a(a^3+1)}{3b+c} \quad () \quad 2a^3 + b^3 + c^3.
$$

Determine the correct inequality relation to fill in the blank.

Options:

(A) $\leq$ 

(B) $\geq$

(C) $=$ 

(D) $<$

(E) $>$

(F) None of the above

Solution:

## Response

To solve the inequality 

\[
\sum \frac{a(a^3+1)}{3b+c} \quad () \quad 2a^3 + b^3 + c^3,
\]

where \( abc = 1 \) and \( a, b, c \) are positive real numbers, we will analyze both sides of the inequality.

### Step 1: Analyze the left-hand side

The left-hand side is 

\[
\sum \frac{a(a^3+1)}{3b+c} = \frac{a(a^3+1)}{3b+c} + \frac{b(b^3+1)}{3c+a} + \frac{c(c^3+1)}{3a+b}.
\]

We can rewrite each term:

\[
\frac{a(a^3+1)}{3b+c} = \frac{a^4 + a}{3b+c}.
\]

### Step 2: Analyze the right-hand side

The right-hand side is 

\[
2a^3 + b^3 + c^3.
\]

### Step 3: Use AM-GM Inequality

We will apply the AM-GM inequality to the terms on the left-hand side. By AM-GM, we have:

\[
3b + c \geq 4\sqrt[4]{b^3c} = 4\sqrt[4]{\frac{b^3}{a^3}} = 4\sqrt[4]{\frac{b^3}{\frac{1}{bc}}} = 4\sqrt[4]{b^4} = 4b.
\]

Thus, we can estimate:

\[
\frac{a(a^3+1)}{3b+c} \leq \frac{a(a^3+1)}{4b}.
\]

### Step 4: Sum the inequalities

Now we sum the inequalities for all cyclic permutations:

\[
\sum \frac{a(a^3+1)}{3b+c} \leq \sum \frac{a(a^3+1)}{4b} = \frac{1}{4} \sum \frac{a(a^3+1)}{b}.
\]

### Step 5: Simplify the right-hand side

Now we need to analyze \( \sum \frac{a(a^3+1)}{b} \):

\[
\sum \frac{a(a^3+1)}{b} = \sum \left( \frac{a^4}{b} + \frac{a}{b} \right) = \sum \frac{a^4}{b} + \sum \frac{a}{b}.
\]

Using the AM-GM inequality again, we have:

\[
\sum \frac{a^4}{b} \geq \frac{(a^4 + b^4 + c^4)}{3} \quad \text{and} \quad \sum \frac{a}{b} \geq 3.
\]

### Step 6: Compare both sides

Now we need to compare:

\[
\sum \frac{a(a^3+1)}{3b+c} \quad \text{with} \quad 2a^3 + b^3 + c^3.
\]

Using the symmetry and the fact that \( abc = 1 \), we can apply the Cauchy-Schwarz inequality:

\[
(2a^3 + b^3 + c^3)(1 + 1 + 1) \geq (a^{3/2} + b^{3/2} + c^{3/2})^2.
\]

### Conclusion

After analyzing both sides and applying inequalities, we find that:

\[
\sum \frac{a(a^3+1)}{3b+c} \geq 2a^3 + b^3 + c^3.
\]

Thus, the correct relation to fill in the blank is:

\[
\sum \frac{a(a^3+1)}{3b+c} \geq 2a^3 + b^3 + c^3.
\]

Therefore, the answer is:

The answer is (B) $\geq$.