## Problem

Let $a, b, c > 0$ such that $a+b+c=2$ and $a^2+b^2+c^2=2$. Determine the minimal constant $C$ such that the following inequality holds for all $a, b, c$ satisfying the given constraints:
$$
a b c \leq C.
$$

## Query

Task description: Please solve the problem with clear, rigorous, and logically sound steps. At the end of your response, state your answer in exactly this format: 'The answer is $C=X$', where X is your calculated numerical bound value. Example: 'The answer is $C=1$'.

Problem: Let $a, b, c > 0$ such that $a+b+c=2$ and $a^2+b^2+c^2=2$. Determine the minimal constant $C$ such that the following inequality holds for all $a, b, c$ satisfying the given constraints:
$$
a b c \leq C.
$$

Solution:

## Response

To solve the problem, we start with the given conditions:

1. \( a + b + c = 2 \)
2. \( a^2 + b^2 + c^2 = 2 \)

From the first condition, we can express \( c \) in terms of \( a \) and \( b \):
\[
c = 2 - a - b.
\]

Next, we substitute \( c \) into the second condition:
\[
a^2 + b^2 + (2 - a - b)^2 = 2.
\]
Expanding the square:
\[
(2 - a - b)^2 = 4 - 4(a + b) + (a + b)^2 = 4 - 4(a + b) + a^2 + 2ab + b^2.
\]
Thus, we have:
\[
a^2 + b^2 + 4 - 4(a + b) + a^2 + 2ab + b^2 = 2.
\]
Combining like terms gives:
\[
2a^2 + 2b^2 + 2ab - 4(a + b) + 4 = 2.
\]
Simplifying this, we get:
\[
2a^2 + 2b^2 + 2ab - 4(a + b) + 2 = 0.
\]
Dividing through by 2:
\[
a^2 + b^2 + ab - 2(a + b) + 1 = 0.
\]
Rearranging gives:
\[
a^2 + b^2 + ab - 2a - 2b + 1 = 0.
\]

Next, we can analyze the expression \( abc \). We will use the method of Lagrange multipliers or symmetry to find the maximum value of \( abc \) under the given constraints.

To find the maximum of \( abc \), we can use the method of symmetry. We assume \( a = b \) and find \( c \):
\[
2a + c = 2 \implies c = 2 - 2a.
\]
Substituting into the second condition:
\[
2a^2 + (2 - 2a)^2 = 2.
\]
Expanding gives:
\[
2a^2 + 4 - 8a + 4a^2 = 2 \implies 6a^2 - 8a + 2 = 0.
\]
Dividing through by 2:
\[
3a^2 - 4a + 1 = 0.
\]
Using the quadratic formula:
\[
a = \frac{4 \pm \sqrt{(-4)^2 - 4 \cdot 3 \cdot 1}}{2 \cdot 3} = \frac{4 \pm \sqrt{16 - 12}}{6} = \frac{4 \pm 2}{6}.
\]
This gives:
\[
a = 1 \quad \text{or} \quad a = \frac{1}{3}.
\]

1. If \( a = 1 \), then \( b = 1 \) and \( c = 0 \), which does not satisfy \( a, b, c > 0 \).
2. If \( a = b = \frac{1}{3} \), then \( c = 2 - \frac{2}{3} = \frac{4}{3} \).

Now we calculate \( abc \):
\[
abc = \left(\frac{1}{3}\right)\left(\frac{1}{3}\right)\left(\frac{4}{3}\right) = \frac{4}{27}.
\]

Next, we check if this is indeed the maximum. We can also check the case where \( a = b = c \):
\[
3a = 2 \implies a = \frac{2}{3} \implies abc = \left(\frac{2}{3}\right)^3 = \frac{8}{27}.
\]

Comparing the two values:
- \( \frac{4}{27} \) from \( a = b = \frac{1}{3}, c = \frac{4}{3} \)
- \( \frac{8}{27} \) from \( a = b = c = \frac{2}{3} \)

The maximum value of \( abc \) is \( \frac{8}{27} \).

Thus, the minimal constant \( C \) such that \( abc \leq C \) for all \( a, b, c \) satisfying the given constraints is:
\[
C = \frac{8}{27}.
\]

Finally, we state the answer in the required format:
The answer is \( C = \frac{8}{27} \).