## Problem

Let $x, y, z \in \mathbb{R}$. Consider the following expression:
$$
\frac{x^2-y^2}{2x^2+1} + \frac{y^2-z^2}{2y^2+1} + \frac{z^2-x^2}{2z^2+1} \quad () \quad 0.
$$

Determine the correct inequality relation to fill in the blank.

Options:

(A) $\leq$ 

(B) $\geq$

(C) $=$ 

(D) $<$

(E) $>$

(F) None of the above

## Query

Task description: Please solve the problem with clear, rigorous, and logically sound steps. At the end of your response, state your answer in exactly this format: 'The answer is (Letter) Symbol', where Letter is one of the given options. Example: 'The answer is (A) $\leq$'.

Problem: Let $x, y, z \in \mathbb{R}$. Consider the following expression:
$$
\frac{x^2-y^2}{2x^2+1} + \frac{y^2-z^2}{2y^2+1} + \frac{z^2-x^2}{2z^2+1} \quad () \quad 0.
$$

Determine the correct inequality relation to fill in the blank.

Options:

(A) $\leq$ 

(B) $\geq$

(C) $=$ 

(D) $<$

(E) $>$

(F) None of the above

Solution:

## Response

To analyze the expression 

\[
S = \frac{x^2 - y^2}{2x^2 + 1} + \frac{y^2 - z^2}{2y^2 + 1} + \frac{z^2 - x^2}{2z^2 + 1},
\]

we will evaluate each term and their contributions to the overall sum \( S \).

### Step 1: Analyze Each Term

1. **First Term**: 
   \[
   \frac{x^2 - y^2}{2x^2 + 1}
   \]
   This term is positive if \( x^2 > y^2 \) and negative if \( x^2 < y^2 \).

2. **Second Term**: 
   \[
   \frac{y^2 - z^2}{2y^2 + 1}
   \]
   This term is positive if \( y^2 > z^2 \) and negative if \( y^2 < z^2 \).

3. **Third Term**: 
   \[
   \frac{z^2 - x^2}{2z^2 + 1}
   \]
   This term is positive if \( z^2 > x^2 \) and negative if \( z^2 < x^2 \).

### Step 2: Consider the Cases

To understand the behavior of \( S \), we can consider specific cases for \( x, y, z \):

- **Case 1**: Let \( x = y = z \). Then,
  \[
  S = \frac{x^2 - x^2}{2x^2 + 1} + \frac{x^2 - x^2}{2x^2 + 1} + \frac{x^2 - x^2}{2x^2 + 1} = 0.
  \]

- **Case 2**: Let \( x = 1, y = 0, z = 0 \). Then,
  \[
  S = \frac{1^2 - 0^2}{2 \cdot 1^2 + 1} + \frac{0^2 - 0^2}{2 \cdot 0^2 + 1} + \frac{0^2 - 1^2}{2 \cdot 0^2 + 1} = \frac{1}{3} + 0 - 1 = \frac{1}{3} - 1 = -\frac{2}{3}.
  \]

- **Case 3**: Let \( x = 0, y = 1, z = 0 \). Then,
  \[
  S = \frac{0^2 - 1^2}{2 \cdot 0^2 + 1} + \frac{1^2 - 0^2}{2 \cdot 1^2 + 1} + \frac{0^2 - 0^2}{2 \cdot 0^2 + 1} = -1 + \frac{1}{3} + 0 = -1 + \frac{1}{3} = -\frac{2}{3}.
  \]

### Step 3: General Behavior

From the cases we have analyzed, we see that:

- When \( x = y = z \), \( S = 0 \).
- When \( x, y, z \) are not equal, \( S \) can take negative values.

### Step 4: Conclusion

The expression \( S \) can be zero or negative depending on the values of \( x, y, z \). Therefore, we can conclude that:

\[
S \quad () \quad 0
\]

is best filled with \( \leq \) since \( S \) can be equal to zero or less than zero.

Thus, the correct answer is:

The answer is (A) $\leq$.